PREFIX ac: <https://linked.data.gov.au/def/address-classes>
PREFIX dcat: <http://www.w3.org/ns/dcat#>
PREFIX dcterms: <http://purl.org/dc/terms/>
PREFIX isoroles: <http://def.isotc211.org/iso19115/-1/2018/CitationAndResponsiblePartyInformation/code/CI_RoleCode/>
PREFIX prov: <http://www.w3.org/ns/prov#>
PREFIX rdfs: <http://www.w3.org/2000/01/rdf-schema#>
PREFIX skos: <http://www.w3.org/2004/02/skos/core#>
PREFIX xsd: <http://www.w3.org/2001/XMLSchema#>

ac:landmark
    a skos:Concept ;
    skos:altLabel "LA"@en ;
    skos:definition "Addresses that specify a location by reference to a named landmark."@en ;
    skos:historyNote "Queensland address data" ;
    skos:inScheme ac: ;
    skos:prefLabel "Landmark"@en ;
.

ac:postal
    a skos:Concept ;
    skos:altLabel "PO"@en ;
    skos:definition "Addresses that specify points of postal delivery which have no definite relation to the location of the recipient, such as post office boxes, overseas defence force addresses, and general delivery offices."@en ;
    skos:historyNote "Queensland address data" ;
    skos:inScheme ac: ;
    skos:prefLabel "Postal"@en ;
.

ac:thoroughfare
    a skos:Concept ;
    skos:altLabel "TH"@en ;
    skos:definition "Addresses that specify a location by reference to a thoroughfare. A thoroughfare is an access route such as road or waterway along which an address access point can be determined."@en ;
    skos:historyNote "Queensland address data" ;
    skos:inScheme ac: ;
    skos:narrower
        ac:street ,
        ac:water ;
    skos:prefLabel "Thoroughfare"@en ;
.

ac:unknown
    a skos:Concept ;
    skos:altLabel "U"@en ;
    skos:definition "Unknown address assignation standard."@en ;
    skos:historyNote "Queensland address data" ;
    skos:inScheme ac: ;
    skos:prefLabel "Unknown"@en ;
.

ac:street
    a skos:Concept ;
    skos:altLabel "ST"@en ;
    skos:definition "Address assigned according to one of the standards for a site accessed from a road."@en ;
    skos:historyNote "Queensland address data" ;
    skos:inScheme ac: ;
    skos:narrower
        ac:street-rural ,
        ac:street-urban ;
    skos:prefLabel "Street"@en ;
.

ac:street-rural
    a skos:Concept ;
    skos:altLabel "RU"@en ;
    skos:definition "Address assigned according to the standard for a site accessed from a rural road."@en ;
    skos:historyNote "Queensland address data" ;
    skos:inScheme ac: ;
    skos:prefLabel "Rural"@en ;
.

ac:street-urban
    a skos:Concept ;
    skos:altLabel "UR"@en ;
    skos:definition "Address assigned according to the standard for a site accessed from an urban road."@en ;
    skos:historyNote "Queensland address data" ;
    skos:inScheme ac: ;
    skos:prefLabel "Urban"@en ;
.

ac:water
    a skos:Concept ;
    skos:altLabel "WA"@en ;
    skos:definition "Address assigned according to one of the standards for a site accessed from a water feature or island."@en ;
    skos:historyNote "Queensland address data" ;
    skos:inScheme ac: ;
    skos:narrower
        ac:water-inlet ,
        ac:water-island ,
        ac:water-river ;
    skos:prefLabel "Water"@en ;
.

ac:water-inlet
    a skos:Concept ;
    skos:altLabel "IN"@en ;
    skos:definition "Address assigned according to the standard for a site accessed from an inlet or bay."@en ;
    skos:historyNote "Queensland address data" ;
    skos:inScheme ac: ;
    skos:prefLabel "Inlet"@en ;
.

ac:water-island
    a skos:Concept ;
    skos:altLabel "IS"@en ;
    skos:definition "Address assigned according to the standard for a site on an island with no road access."@en ;
    skos:historyNote "Queensland address data" ;
    skos:inScheme ac: ;
    skos:prefLabel "Island"@en ;
.

ac:water-river
    a skos:Concept ;
    skos:altLabel "RI"@en ;
    skos:definition "Address assigned according to the standard for a site accessed from a river or creek."@en ;
    skos:historyNote "Queensland address data" ;
    skos:inScheme ac: ;
    skos:prefLabel "River"@en ;
.

ac:
    a skos:ConceptScheme ;
    dcterms:created "2023-06-01"^^xsd:date ;
    dcterms:creator [
            a prov:Agent ;
            rdfs:label "Department Of Resources"
        ] ;
    dcterms:identifier "address-classes"^^xsd:token ;
    dcterms:modified "2023-07-31"^^xsd:date ;
    dcterms:publisher [
            a prov:Agent ;
            rdfs:label "Icsm"
        ] ;
    skos:definition "This vocabulary describes the address classes or types used in address allocation. "@en ;
    skos:hasTopConcept
        ac:landmark ,
        ac:postal ,
        ac:street ,
        ac:street-rural ,
        ac:street-urban ,
        ac:thoroughfare ,
        ac:unknown ,
        ac:water ,
        ac:water-inlet ,
        ac:water-island ,
        ac:water-river ;
    skos:historyNote "This vocabulary was created by the Queensland Spatial Information services." ;
    skos:prefLabel "Address Classes"@en ;
    prov:qualifiedAttribution [
            dcat:hadRole isoroles:custodian ;
            prov:agent [
                    a prov:Agent ;
                    rdfs:label "Icsm"
                ]
        ] ;
.

