PREFIX cs: <https://linked.data.gov.au/def/go-categories>
PREFIX dcterms: <http://purl.org/dc/terms/>
PREFIX owl: <http://www.w3.org/2002/07/owl#>
PREFIX rdfs: <http://www.w3.org/2000/01/rdf-schema#>
PREFIX reg: <http://purl.org/linked-data/registry#>
PREFIX schema: <https://schema.org/>
PREFIX skos: <http://www.w3.org/2004/02/skos/core#>
PREFIX xsd: <http://www.w3.org/2001/XMLSchema#>

cs:abandoned-mine
    a skos:Concept ;
    rdfs:isDefinedBy cs: ;
    skos:definition "An underground site used for the extraction of minerals currently not in use."@en ;
    skos:historyNote "PSMA" ;
    skos:inScheme cs: ;
    skos:prefLabel "Abandoned Mine"@en ;
.

cs:abandoned-quarry
    a skos:Concept ;
    rdfs:isDefinedBy cs: ;
    skos:definition "An open surface excavation used for the extraction of stone currently not in use."@en ;
    skos:historyNote "PSMA" ;
    skos:inScheme cs: ;
    skos:prefLabel "Abandoned Quarry"@en ;
.

cs:abattoir
    a skos:Concept ;
    rdfs:isDefinedBy cs: ;
    skos:altLabel
        "Slaughterhouse"@en ,
        "knacker's yard"@en ,
        "knackery"@en ;
    skos:definition "A place where animals are slaughtered"@en ;
    skos:historyNote "PSMA" ;
    skos:inScheme cs: ;
    skos:prefLabel "Abattoir"@en ;
.

cs:abbey
    a skos:Concept ;
    rdfs:isDefinedBy cs: ;
    skos:altLabel
        "convent"@en ,
        "monastery"@en ;
    skos:definition "A building or buildings occupied by monks or nuns under an abbot or abbess."@en ;
    skos:historyNote "GNR" ;
    skos:inScheme cs: ;
    skos:prefLabel "Abbey"@en ;
.

cs:abyssal-plain
    a skos:Concept ;
    rdfs:isDefinedBy cs: ;
    skos:definition "An extensive, flat or gently sloping region, usually found at depths greater than 4000 m."@en ;
    skos:historyNote "Definition from General Bathymetric Chart of the Oceans (GEBCO) Sub-Committee on Undersea Features Names (SCUFN)." ;
    skos:inScheme cs: ;
    skos:prefLabel "Abyssal Plain"@en ;
    schema:citation "https://iho.int/en/basic-documents-1"^^xsd:anyURI ;
.

cs:academy
    a skos:Concept ;
    rdfs:isDefinedBy cs: ;
    skos:definition "To be defined."@en ;
    skos:inScheme cs: ;
    skos:prefLabel "Academy"@en ;
.

cs:accommodations
    a skos:Concept ;
    rdfs:isDefinedBy cs: ;
    skos:definition "Places primarily used for short term accommodation, usually for recreational purposes."@en ;
    skos:inScheme cs: ;
    skos:narrower
        cs:camp-ground ,
        cs:holiday-park ;
    skos:prefLabel "Accommodations"@en ;
.

cs:adit
    a skos:Concept ;
    rdfs:isDefinedBy cs: ;
    skos:definition "An almost horizontal shaft into a mine, for access or drainage."@en ;
    skos:historyNote "PSMA" ;
    skos:inScheme cs: ;
    skos:prefLabel "Adit"@en ;
.

cs:administrative-area
    a skos:Concept ;
    rdfs:isDefinedBy cs: ;
    skos:definition "Places with officially defined boundaries for governance purposes."@en ;
    skos:historyNote "Agreed at ICSM PNWG Meeting 2022" ;
    skos:inScheme cs: ;
    skos:narrower
        cs:agricultural-area ,
        cs:antarctic-land ,
        cs:catchment-mangement ,
        cs:county ,
        cs:federal-electorate ,
        cs:land-district ,
        cs:local-government-area ,
        cs:local-government-area-ward ,
        cs:locality ,
        cs:mining-centre ,
        cs:parish ,
        cs:pastoral-district ,
        cs:protected-area ,
        cs:state-electorate ,
        cs:state-territory ,
        cs:tourist-region ,
        cs:town-site ;
    skos:prefLabel "Administrative Area"@en ;
    skos:topConceptOf cs: ;
.

cs:aged-care
    a skos:Concept ;
    rdfs:isDefinedBy cs: ;
    skos:definition "A facility that supports the care of the elderly"@en ;
    skos:historyNote "PSMA; Agreed at ICSM PNWG Meeting 2022" ;
    skos:inScheme cs: ;
    skos:narrower cs:residential-aged-care ;
    skos:prefLabel "Aged Care"@en ;
.

cs:agricultural-area
    a skos:Concept ;
    rdfs:isDefinedBy cs: ;
    skos:definition "An area defined for agricultural purposes"@en ;
    skos:inScheme cs: ;
    skos:prefLabel "Agricultural Area"@en ;
.

cs:agriculture
    a skos:Concept ;
    rdfs:isDefinedBy cs: ;
    skos:definition "Places where agricultural activities are undertaken"@en ;
    skos:inScheme cs: ;
    skos:narrower
        cs:dairy ,
        cs:farm ,
        cs:paddock ,
        cs:plantation ,
        cs:stockyard ,
        cs:vineyard ;
    skos:prefLabel "Agricultural Activity Area"@en ;
.

cs:air-force-base
    a skos:Concept ;
    rdfs:isDefinedBy cs: ;
    skos:definition "A facility used by the Air Force for the operation and/or training of personnel and their aircraft"@en ;
    skos:historyNote "PSMA" ;
    skos:inScheme cs: ;
    skos:prefLabel "Air Force Base"@en ;
.

cs:air-transport-infrastructure
    a skos:Concept ;
    rdfs:isDefinedBy cs: ;
    skos:definition "An area for air traffic and support infrastructure"@en ;
    skos:inScheme cs: ;
    skos:narrower
        cs:airport ,
        cs:hangar ,
        cs:helipad ,
        cs:heliport ,
        cs:landing-area ;
    skos:prefLabel "Air Transport Infrastructure"@en ;
.

cs:airport
    a skos:Concept ;
    rdfs:isDefinedBy cs: ;
    skos:altLabel "Aerodrome"@en ;
    skos:definition "A regulated landing and taking off area for civil aircraft, usually equipped with runways and aircraft maintenance and passenger facilities."@en ;
    skos:historyNote "PSMA" ;
    skos:inScheme cs: ;
    skos:prefLabel "Airport"@en ;
.

cs:alumina-refinery
    a skos:Concept ;
    rdfs:isDefinedBy cs: ;
    skos:definition "A refinery for extracting Aluminium"@en ;
    skos:historyNote "PSMA" ;
    skos:inScheme cs: ;
    skos:prefLabel "Alumina Refinery"@en ;
.

cs:ambulance-station
    a skos:Concept ;
    rdfs:isDefinedBy cs: ;
    skos:definition "A structure or other area set aside for storage ofambulance vehicles and medical equipment"@en ;
    skos:historyNote "PSMA" ;
    skos:inScheme cs: ;
    skos:prefLabel "Ambulance Station"@en ;
.

cs:ampitheatre
    a skos:Concept ;
    rdfs:isDefinedBy cs: ;
    skos:altLabel
        "basin"@en ,
        "natural amphitheatre"@en ;
    skos:definition "A circular or oval area of ground, surrounded by tiers of seats on a steep slope, for open-air public performances"@en ;
    skos:historyNote "VMFEAT" ;
    skos:inScheme cs: ;
    skos:prefLabel "Amphitheatre"@en ;
.

cs:anchorage
    a skos:Concept ;
    rdfs:isDefinedBy cs: ;
    skos:altLabel
        "Roadstead"@en ,
        "haven"@en ,
        "natural harbour"@en ;
    skos:definition "A natural area in which vessels anchor or may anchor"@en ;
    skos:historyNote "GNR" ;
    skos:inScheme cs: ;
    skos:prefLabel "Anchorage"@en ;
.

cs:antarctic-land
    a skos:Concept ;
    rdfs:isDefinedBy cs: ;
    skos:definition "Large continental area defined by natural boundaries, or partly by natural boundaries and partly by boundaries of political convenience. The term was formally used by explorers for newly discovered lengths of coastline, cf. coast. Outside the area covered by this work the term may be synonymous with territory. The use of land does not refer to the ground, rather it is a generic part of a toponym."@en ;
    skos:historyNote "Concept and definition from the Australian Antarctic Division." ;
    skos:inScheme cs: ;
    skos:prefLabel "Antarctic Land"@en ;
    schema:citation "https://data.aad.gov.au/aadc/ftc/display_feature_type.cfm?feature_type_code=389"^^xsd:anyURI ;
.

cs:antarctic-specially-managed-areas
    a skos:Concept ;
    rdfs:isDefinedBy cs: ;
    skos:altLabel "ASMA"@en ;
    skos:definition "Areas intended to facilitate cooperation between nations operating in close proximity to each other, with a view to minimising environmental impacts. ASMAs may contain zones where various restrictions and permits might apply, and activities within ASMAs are governed by a code of conduct. Designated under the Antarctic Treaty System."@en ;
    skos:historyNote "Concept and definition from the Australian Antarctic Division." ;
    skos:inScheme cs: ;
    skos:prefLabel "Antarctic Specially Managed Areas"@en ;
.

cs:antarctic-specially-protected-areas
    a skos:Concept ;
    rdfs:isDefinedBy cs: ;
    skos:altLabel "ASPA"@en ;
    skos:definition "Areas set aside to protect outstanding environmental, scientific, historic, aesthetic or wilderness values, any combination of those values, or ongoing or planned scientific research. Designated under the Antarctic Treaty System."@en ;
    skos:historyNote "Concept and definition from the Australian Antarctic Division." ;
    skos:inScheme cs: ;
    skos:prefLabel "Antarctic Specially Protected Areas"@en ;
.

cs:aquaculture
    a skos:Concept ;
    rdfs:isDefinedBy cs: ;
    skos:definition "A place for the cultivation of freshwater and marine resources, both plant and animal."@en ;
    skos:historyNote "PSMA" ;
    skos:inScheme cs: ;
    skos:narrower cs:hatchery ;
    skos:prefLabel "Aquacultural Activity Area"@en ;
.

cs:aquarium
    a skos:Concept ;
    rdfs:isDefinedBy cs: ;
    skos:definition "A facility for the public display of aquatic species"@en ;
    skos:historyNote "PSMA" ;
    skos:inScheme cs: ;
    skos:prefLabel "Aquarium"@en ;
.

cs:aquatic-passage
    a skos:Concept ;
    rdfs:isDefinedBy cs: ;
    skos:altLabel
        "Narrows"@en ,
        "Rip"@en ,
        "Strait"@en ;
    skos:definition "A navigable route, specifically one through REEFS ,ISLANDS, LANDS or shallow waters"@en ;
    skos:historyNote "new" ;
    skos:inScheme cs: ;
    skos:prefLabel "Aquatic Passage"@en ;
.

cs:aquifer
    a skos:Concept ;
    rdfs:isDefinedBy cs: ;
    skos:altLabel "artesian basin"@en ;
    skos:definition "An underground waterbody."@en ;
    skos:historyNote "Feature renamed from Aquifier to Aquifer" ;
    skos:inScheme cs: ;
    skos:prefLabel "Aquifer"@en ;
.

cs:arboretum
    a skos:Concept ;
    rdfs:isDefinedBy cs: ;
    skos:definition "A place where trees or shrubs are cultivated for their scientific or educational interest."@en ;
    skos:historyNote "PSMA" ;
    skos:inScheme cs: ;
    skos:prefLabel "Arboretum"@en ;
.

cs:army-base
    a skos:Concept ;
    rdfs:isDefinedBy cs: ;
    skos:definition "A facility used by the army for the operation and/or training of personnel and their vehicles"@en ;
    skos:historyNote "PSMA" ;
    skos:inScheme cs: ;
    skos:prefLabel "Army Base"@en ;
.

cs:art-gallery
    a skos:Concept ;
    rdfs:isDefinedBy cs: ;
    skos:definition "An area or facility which displays art works"@en ;
    skos:historyNote "PSMA" ;
    skos:inScheme cs: ;
    skos:prefLabel "Art Gallery"@en ;
.

cs:athletic-field
    a skos:Concept ;
    rdfs:isDefinedBy cs: ;
    skos:altLabel "Athletic Track"@en ;
    skos:definition "A place where training and competitions are held."@en ;
    skos:historyNote "PSMA; Agreed at ICSM PNWG Meeting 2022" ;
    skos:inScheme cs: ;
    skos:prefLabel "Athletic Field"@en ;
.

cs:atoll
    a skos:Concept ;
    rdfs:isDefinedBy cs: ;
    skos:definition "A coral island consisting of a reef surrounding a lagoon"@en ;
    skos:inScheme cs: ;
    skos:prefLabel "Atoll"@en ;
.

cs:bank
    a skos:Concept ;
    rdfs:isDefinedBy cs: ;
    skos:definition "The sloping ground along the edge of water."@en ;
    skos:inScheme cs: ;
    skos:narrower cs:marine-bank ;
    skos:prefLabel "Bank"@en ;
.

cs:bar
    a skos:Concept ;
    rdfs:isDefinedBy cs: ;
    skos:altLabel
        "Sandbank"@en ,
        "Sandbar"@en ;
    skos:definition "A BAR of sand, coral, mud formed in a SEA or RIVER, exposed at low tide and formed by the action of the tides or currents."@en ;
    skos:historyNote "PSMA" ;
    skos:inScheme cs: ;
    skos:prefLabel "Bar"@en ;
.

cs:barracks
    a skos:Concept ;
    rdfs:isDefinedBy cs: ;
    skos:definition "A building or buildings used for the lodgement or residence of defence personnel"@en ;
    skos:historyNote "VMFEAT" ;
    skos:inScheme cs: ;
    skos:prefLabel "Barracks"@en ;
.

cs:baseball-field
    a skos:Concept ;
    rdfs:isDefinedBy cs: ;
    skos:definition "A place where baseball is played."@en ;
    skos:historyNote "VMFEAT" ;
    skos:inScheme cs: ;
    skos:prefLabel "Baseball Field"@en ;
.

cs:basin
    a skos:Concept ;
    rdfs:isDefinedBy cs: ;
    skos:definition "A hollow or trough in the surface of the land, synonymous with cirque, or an almost landlocked body of water off an inlet or sound; the term may be applied also to submarine features."@en ;
    skos:historyNote "Concept and definition from the Australian Antarctic Division." ;
    skos:inScheme cs: ;
    skos:narrower
        cs:marine-basin ,
        cs:subglacial-basin ;
    skos:prefLabel "Basin"@en ;
    schema:citation "https://data.aad.gov.au/aadc/ftc/display_feature_type.cfm?feature_type_code=354"^^xsd:anyURI ;
.

cs:basketball-court
    a skos:Concept ;
    rdfs:isDefinedBy cs: ;
    skos:definition "A place where basketball is played."@en ;
    skos:historyNote "PSMA" ;
    skos:inScheme cs: ;
    skos:prefLabel "Basketball Court"@en ;
.

cs:battery
    a skos:Concept ;
    rdfs:isDefinedBy cs: ;
    skos:definition "A stone crushing works for ore extraction, as used on gold fields"@en ;
    skos:historyNote "PSMA" ;
    skos:inScheme cs: ;
    skos:prefLabel "Battery"@en ;
.

cs:bay
    a skos:Concept ;
    rdfs:isDefinedBy cs: ;
    skos:altLabel "Cove"@en ;
    skos:definition "A well-marked indentation made by the sea or a lake into its shoreline."@en ;
    skos:historyNote "VMFEAT" ;
    skos:inScheme cs: ;
    skos:prefLabel "Bay"@en ;
.

cs:beach
    a skos:Concept ;
    rdfs:isDefinedBy cs: ;
    skos:altLabel "Shore"@en ;
    skos:definition "A sloping shore along water that is periodically washed by waves or tides and is usually covered in sand or gravel."@en ;
    skos:inScheme cs: ;
    skos:prefLabel "Beach"@en ;
.

cs:beacon
    a skos:Concept ;
    rdfs:isDefinedBy cs: ;
    skos:altLabel
        "BUOY"@en ,
        "Light"@en ,
        "Navigation bouy"@en ;
    skos:definition "A structure to provide a navigational signal for vessels or aircraft"@en ;
    skos:historyNote "PSMA" ;
    skos:inScheme cs: ;
    skos:prefLabel "Beacon"@en ;
.

cs:bench
    a skos:Concept ;
    rdfs:isDefinedBy cs: ;
    skos:altLabel
        "terrace"@en ,
        "tiers"@en ;
    skos:definition "A flat ledge on sloping ground."@en ;
    skos:inScheme cs: ;
    skos:prefLabel "Bench"@en ;
.

cs:bend
    a skos:Concept ;
    rdfs:isDefinedBy cs: ;
    skos:altLabel
        "loop"@en ,
        "meander"@en ,
        "river bend."@en ;
    skos:definition "A curve in the course of a STREAM"@en ;
    skos:historyNote "Agreed at ICSM PNWG Meeting 2022" ;
    skos:inScheme cs: ;
    skos:prefLabel "Bend"@en ;
.

cs:bicycle-track
    a skos:Concept ;
    rdfs:isDefinedBy cs: ;
    skos:altLabel
        "bike path"@en ,
        "bikeway"@en ,
        "cycleway"@en ;
    skos:definition "A trail designed for bicycle traffic in the main. This is not a shared roadway with vehicular traffic. Main use is cycling."@en ;
    skos:historyNote "Agreed at ICSM PNWG Meeting 2022" ;
    skos:inScheme cs: ;
    skos:prefLabel "Bicycle Track"@en ;
.

cs:biomass-power-station
    a skos:Concept ;
    rdfs:isDefinedBy cs: ;
    skos:definition "A process plant that creates power from biomass sources."@en ;
    skos:inScheme cs: ;
    skos:prefLabel "Biomass Power Station"@en ;
.

cs:blowhole
    a skos:Concept ;
    rdfs:isDefinedBy cs: ;
    skos:definition "A hole near the seashore that has been formed in the roof of a CAVE, and through which air and possibly water are forced by the rising tide."@en ;
    skos:historyNote "GNR" ;
    skos:inScheme cs: ;
    skos:prefLabel "Blowhole"@en ;
.

cs:bmx-track
    a skos:Concept ;
    rdfs:isDefinedBy cs: ;
    skos:definition "A place where bikes are used for recreation or racing."@en ;
    skos:historyNote "PSMA" ;
    skos:inScheme cs: ;
    skos:prefLabel "Bmx Track"@en ;
.

cs:boat-ramp
    a skos:Concept ;
    rdfs:isDefinedBy cs: ;
    skos:altLabel
        "boat launch"@en ,
        "landing ramp"@en ,
        "launching ramp"@en ,
        "slipway"@en ;
    skos:definition "A sloping construction to facilitate launching or retrieving vessels from water."@en ;
    skos:historyNote "Agreed at ICSM PNWG Meeting 2022" ;
    skos:inScheme cs: ;
    skos:prefLabel "Boat Ramp"@en ;
.

cs:boating-club
    a skos:Concept ;
    rdfs:isDefinedBy cs: ;
    skos:definition "A building where boats are stored or from where boating related activities conducted."@en ;
    skos:historyNote "PSMA" ;
    skos:inScheme cs: ;
    skos:prefLabel "Boating Club"@en ;
.

cs:bombing-range
    a skos:Concept ;
    rdfs:isDefinedBy cs: ;
    skos:altLabel "Rocket Range"@en ;
    skos:definition "A tract of land on which the military conducts bombing practice"@en ;
    skos:historyNote "GNR" ;
    skos:inScheme cs: ;
    skos:prefLabel "Bombing Range"@en ;
.

cs:bore
    a skos:Concept ;
    rdfs:isDefinedBy cs: ;
    skos:altLabel "artesian well"@en ;
    skos:definition "A deep vertical hole of a small diameter made to obtain water."@en ;
    skos:historyNote "Agreed at ICSM PNWG Meeting 2022" ;
    skos:inScheme cs: ;
    skos:prefLabel "Bore"@en ;
.

cs:botanic-gardens
    a skos:Concept ;
    rdfs:isDefinedBy cs: ;
    skos:definition "A park or reserve which contains specialised collections of plants"@en ;
    skos:historyNote "GNR" ;
    skos:inScheme cs: ;
    skos:prefLabel "Botanic Gardens"@en ;
.

cs:bowling-green
    a skos:Concept ;
    rdfs:isDefinedBy cs: ;
    skos:definition "An area of closely mown turf on which the game of bowls is played."@en ;
    skos:historyNote "PSMA" ;
    skos:inScheme cs: ;
    skos:prefLabel "Bowling Green"@en ;
.

cs:brewery
    a skos:Concept ;
    rdfs:isDefinedBy cs: ;
    skos:definition "An establishment for brewing beer, ale."@en ;
    skos:historyNote "PSMA" ;
    skos:inScheme cs: ;
    skos:prefLabel "Brewery"@en ;
.

cs:brickworks
    a skos:Concept ;
    rdfs:isDefinedBy cs: ;
    skos:definition "A place where bricks are made"@en ;
    skos:historyNote "PSMA" ;
    skos:inScheme cs: ;
    skos:prefLabel "Brickworks"@en ;
.

cs:bridge
    a skos:Concept ;
    rdfs:isDefinedBy cs: ;
    skos:definition "To be defined."@en ;
    skos:historyNote "Added by QLD 2024-03-05" ;
    skos:inScheme cs: ;
    skos:narrower
        cs:footbridge ,
        cs:rail-bridge ,
        cs:road-bridge ;
    skos:prefLabel "Bridge"@en ;
.

cs:building
    a skos:Concept ;
    rdfs:isDefinedBy cs: ;
    skos:definition "Name of a building, not classified elsewhere."@en ;
    skos:inScheme cs: ;
    skos:prefLabel "Building"@en ;
.

cs:bus-depot
    a skos:Concept ;
    rdfs:isDefinedBy cs: ;
    skos:definition "An area for storage and maintenance of buses"@en ;
    skos:historyNote "PSMA" ;
    skos:inScheme cs: ;
    skos:prefLabel "Bus Depot"@en ;
.

cs:bus-route
    a skos:Concept ;
    rdfs:isDefinedBy cs: ;
    skos:definition "The set route taken by a bus service."@en ;
    skos:historyNote "PSMA" ;
    skos:inScheme cs: ;
    skos:prefLabel "Bus Route"@en ;
.

cs:bus-stop
    a skos:Concept ;
    rdfs:isDefinedBy cs: ;
    skos:definition "A designated place where buses stop for passengers to board or alight."@en ;
    skos:historyNote "PSMA 2023-09-13" ;
    skos:inScheme cs: ;
    skos:prefLabel "Bus Stop"@en ;
.

cs:bush-nursing-hospital
    a skos:Concept ;
    rdfs:isDefinedBy cs: ;
    skos:definition "A hospital that operates primarily in the rural areas"@en ;
    skos:historyNote "PSMA" ;
    skos:inScheme cs: ;
    skos:prefLabel "Bush Nursing Hospital"@en ;
.

cs:business
    a skos:Concept ;
    rdfs:isDefinedBy cs: ;
    skos:definition "Places where the major activity is of a commercial nature."@en ;
    skos:inScheme cs: ;
    skos:narrower
        cs:cinema ,
        cs:entertainment-centre ,
        cs:market ,
        cs:post-office ,
        cs:racetrack ,
        cs:shopping-centre ;
    skos:prefLabel "Business"@en ;
.

cs:business-college
    a skos:Concept ;
    rdfs:isDefinedBy cs: ;
    skos:definition "To be defined."@en ;
    skos:inScheme cs: ;
    skos:prefLabel "Business College"@en ;
.

cs:busway
    a skos:Concept ;
    rdfs:isDefinedBy cs: ;
    skos:definition "To be defined."@en ;
    skos:historyNote "Added by QLD 2024-03-05" ;
    skos:inScheme cs: ;
    skos:prefLabel "Busway"@en ;
.

cs:cableway
    a skos:Concept ;
    rdfs:isDefinedBy cs: ;
    skos:altLabel
        "J-Bar"@en ,
        "Poma Gondola"@en ,
        "T-Bar"@en ,
        "chair lift"@en ,
        "gondola lift"@en ,
        "surface lift"@en ;
    skos:definition "A series of chairs, bars or cabins attached to a power-driven cable for conveying people."@en ;
    skos:historyNote "PSMA; Agreed at ICSM PNWG Meeting 2022" ;
    skos:inScheme cs: ;
    skos:prefLabel "Cableway"@en ;
.

cs:cairn
    a skos:Concept ;
    rdfs:isDefinedBy cs: ;
    skos:definition "A pyramidal heap of stones to mark a SUMMIT, TRACK, boundary, historical event, or a memorial to a person"@en ;
    skos:historyNote "PSMA" ;
    skos:inScheme cs: ;
    skos:prefLabel "Cairn"@en ;
.

cs:camp-ground
    a skos:Concept ;
    rdfs:isDefinedBy cs: ;
    skos:altLabel
        "Camp"@en ,
        "Camp site"@en ;
    skos:definition "An area where a camp has been established or where it would be suitable to establish one; an area, often provided with amenities, where it is permitted to set up a camp."@en ;
    skos:historyNote "PSMA" ;
    skos:inScheme cs: ;
    skos:prefLabel "Camp Ground"@en ;
.

cs:canal
    a skos:Concept ;
    rdfs:isDefinedBy cs: ;
    skos:definition "An artificial waterway constructed for navigation and/or water power."@en ;
    skos:inScheme cs: ;
    skos:prefLabel "Canal"@en ;
.

cs:cape
    a skos:Concept ;
    rdfs:isDefinedBy cs: ;
    skos:altLabel
        "Headland"@en ,
        "head"@en ;
    skos:definition "An elevated protrusion of land into the sea, more prominent than a POINT"@en ;
    skos:historyNote "GNR" ;
    skos:inScheme cs: ;
    skos:prefLabel "Cape"@en ;
.

cs:car-park
    a skos:Concept ;
    rdfs:isDefinedBy cs: ;
    skos:altLabel "Parking station"@en ;
    skos:definition "An area or building which is designed or adapted for the parking of cars."@en ;
    skos:historyNote "Agreed at ICSM PNWG Meeting 2022" ;
    skos:inScheme cs: ;
    skos:prefLabel "Car Park"@en ;
.

cs:caravan-park
    a skos:Concept ;
    rdfs:isDefinedBy cs: ;
    skos:definition "A bounded area in which caravans are, or can be, parked, or where caravan type accommodation can be obtained; domestic facilities may be provided"@en ;
    skos:historyNote "PSMA" ;
    skos:inScheme cs: ;
    skos:prefLabel "Caravan Park"@en ;
.

cs:care-facility
    a skos:Concept ;
    rdfs:isDefinedBy cs: ;
    skos:definition "Facility to support persons requiring care for reasons not directly related to a medical need."@en ;
    skos:inScheme cs: ;
    skos:narrower
        cs:aged-care ,
        cs:child-care ,
        cs:disability-support-facility ;
    skos:prefLabel "Care Facility"@en ;
    skos:topConceptOf cs: ;
.

cs:cargo-terminal
    a skos:Concept ;
    rdfs:isDefinedBy cs: ;
    skos:altLabel "Container Terminal"@en ;
    skos:definition "A site used to manage and store freight."@en ;
    skos:inScheme cs: ;
    skos:prefLabel "Cargo Terminal"@en ;
.

cs:catchment-mangement
    a skos:Concept ;
    rdfs:isDefinedBy cs: ;
    skos:definition "An administrative bounded area proclaimed for water catchment protection"@en ;
    skos:inScheme cs: ;
    skos:prefLabel "Catchment Management"@en ;
.

cs:causeway
    a skos:Concept ;
    rdfs:isDefinedBy cs: ;
    skos:definition "a structure that facilitates the crossing of road, railway or watercourse over under or through another feature"@en ;
    skos:historyNote "GNR" ;
    skos:inScheme cs: ;
    skos:prefLabel "Causeway"@en ;
.

cs:cave
    a skos:Concept ;
    rdfs:isDefinedBy cs: ;
    skos:definition "A hollowed-out chamber in the Earth, or in the side of a CLIFF or HILL; especially a larger natural cavity in the earth with an opening to the surface"@en ;
    skos:historyNote "PSMA" ;
    skos:inScheme cs: ;
    skos:narrower
        cs:cavern ,
        cs:grotto ,
        cs:lava-tube ;
    skos:prefLabel "Cave"@en ;
.

cs:cavern
    a skos:Concept ;
    rdfs:isDefinedBy cs: ;
    skos:definition "To be defined."@en ;
    skos:inScheme cs: ;
    skos:prefLabel "Cavern"@en ;
.

cs:cay
    a skos:Concept ;
    rdfs:isDefinedBy cs: ;
    skos:definition "An area of sand or coral above sea level"@en ;
    skos:inScheme cs: ;
    skos:prefLabel "Cay"@en ;
.

cs:cement-plant
    a skos:Concept ;
    rdfs:isDefinedBy cs: ;
    skos:definition "A place where cement is manufactured."@en ;
    skos:historyNote "PSMA" ;
    skos:inScheme cs: ;
    skos:prefLabel "Cement Plant"@en ;
.

cs:cemetery
    a skos:Concept ;
    rdfs:isDefinedBy cs: ;
    skos:altLabel "burial site"@en ;
    skos:definition "An operational place/area for burying the dead"@en ;
    skos:historyNote "PSMA" ;
    skos:inScheme cs: ;
    skos:prefLabel "Cemetery"@en ;
.

cs:chapel
    a skos:Concept ;
    rdfs:isDefinedBy cs: ;
    skos:definition "A place of worship connected with and subsidiary to a CHURCH; a place of worship other than a CHURCH or cathedral, especially in public institutions."@en ;
    skos:historyNote "GNR" ;
    skos:inScheme cs: ;
    skos:prefLabel "Chapel"@en ;
.

cs:child-care
    a skos:Concept ;
    rdfs:isDefinedBy cs: ;
    skos:altLabel
        "creche"@en ,
        "nursery"@en ,
        "play group"@en ;
    skos:definition "A facility to care for children."@en ;
    skos:historyNote "PSMA" ;
    skos:inScheme cs: ;
    skos:prefLabel "Child Care"@en ;
.

cs:childrens-hospital
    a skos:Concept ;
    rdfs:isDefinedBy cs: ;
    skos:definition "To be defined."@en ;
    skos:historyNote "Added by QLD 2024-03-05" ;
    skos:inScheme cs: ;
    skos:prefLabel "Childrens Hospital"@en ;
.

cs:church
    a skos:Concept ;
    rdfs:isDefinedBy cs: ;
    skos:definition "A building used for religious worship. Includes all christian dominations."@en ;
    skos:historyNote "PSMA" ;
    skos:inScheme cs: ;
    skos:prefLabel "Church"@en ;
.

cs:cinema
    a skos:Concept ;
    rdfs:isDefinedBy cs: ;
    skos:definition "A place designed for the exhibition of films."@en ;
    skos:historyNote "PSMA" ;
    skos:inScheme cs: ;
    skos:narrower cs:drive-in-theatre ;
    skos:prefLabel "Cinema"@en ;
.

cs:cirque
    a skos:Concept ;
    rdfs:isDefinedBy cs: ;
    skos:definition "A deep rounded hollow on a mountain side formed by glacial action and usually occupied by a remnant glacier or neve."@en ;
    skos:inScheme cs: ;
    skos:prefLabel "Cirque"@en ;
.

cs:clay-pan
    a skos:Concept ;
    rdfs:isDefinedBy cs: ;
    skos:definition "A small depression, intermittently containing water, which holds clay deposits."@en ;
    skos:inScheme cs: ;
    skos:prefLabel "Clay Pan"@en ;
.

cs:cliff
    a skos:Concept ;
    rdfs:isDefinedBy cs: ;
    skos:altLabel
        "bluff"@en ,
        "breakaway"@en ,
        "buttress"@en ,
        "crag"@en ,
        "jump up"@en ,
        "precipice"@en ,
        "rockface"@en ;
    skos:definition "A perpendicular or steep face of rock of considerable height either inland or along the coast"@en ;
    skos:historyNote "PSMA; Agreed at ICSM PNWG Meeting 2022" ;
    skos:inScheme cs: ;
    skos:prefLabel "Cliff"@en ;
.

cs:clumps
    a skos:Concept ;
    rdfs:isDefinedBy cs: ;
    skos:definition "To be defined."@en ;
    skos:inScheme cs: ;
    skos:prefLabel "Clumps"@en ;
.

cs:coal-field
    a skos:Concept ;
    rdfs:isDefinedBy cs: ;
    skos:definition "An area in which coal resources have been identified."@en ;
    skos:inScheme cs: ;
    skos:prefLabel "Coal Field"@en ;
.

cs:coal-power-station
    a skos:Concept ;
    rdfs:isDefinedBy cs: ;
    skos:definition "A process plant that creates power from coal."@en ;
    skos:inScheme cs: ;
    skos:prefLabel "Coal Power Station"@en ;
.

cs:coast
    a skos:Concept ;
    rdfs:isDefinedBy cs: ;
    skos:altLabel "Coastline"@en ;
    skos:definition "Boundary between land and sea, applied in place-names to lengths of coastline determined partly by the history of their discovery and partly by convenient demarcation points"@en ;
    skos:historyNote "Concept and definition from the Australian Antarctic Division." ;
    skos:inScheme cs: ;
    skos:prefLabel "Coast"@en ;
    schema:citation "https://data.aad.gov.au/aadc/ftc/display_feature_type.cfm?feature_type_code=366"^^xsd:anyURI ;
.

cs:coast-guard
    a skos:Concept ;
    rdfs:isDefinedBy cs: ;
    skos:altLabel
        "marine rescue"@en ,
        "volunteer marine rescue"@en ;
    skos:definition "A maritime facility supporting the activities of a coast guard."@en ;
    skos:historyNote "VMFEAT" ;
    skos:inScheme cs: ;
    skos:prefLabel "Coast Guard"@en ;
.

cs:coastal-reserve
    a skos:Concept ;
    rdfs:isDefinedBy cs: ;
    skos:definition "An area of land adjacent to the sea, set apart, as by a state or nation, to be preserved in its natural state for the benefit of the public."@en ;
    skos:historyNote "PSMA" ;
    skos:inScheme cs: ;
    skos:prefLabel "Coastal Reserve"@en ;
.

cs:colony
    a skos:Concept ;
    rdfs:isDefinedBy cs: ;
    skos:altLabel "Wallow"@en ;
    skos:definition "A place where animals gather."@en ;
    skos:inScheme cs: ;
    skos:prefLabel "Colony"@en ;
.

cs:commemorative-tree
    a skos:Concept ;
    rdfs:isDefinedBy cs: ;
    skos:altLabel "Tree"@en ;
    skos:definition "To be defined."@en ;
    skos:inScheme cs: ;
    skos:prefLabel "Commemorative Tree"@en ;
.

cs:commune
    a skos:Concept ;
    rdfs:isDefinedBy cs: ;
    skos:definition "A group of families or individuals living together and sharing possessions, interests and or responsibilities."@en ;
    skos:inScheme cs: ;
    skos:prefLabel "Commune"@en ;
.

cs:communication-infrastructure
    a skos:Concept ;
    rdfs:isDefinedBy cs: ;
    skos:definition "Location or equipment facilitating the transmission of information."@en ;
    skos:inScheme cs: ;
    skos:narrower
        cs:communication-tower ,
        cs:fibre-optic-cable ,
        cs:radio-communication-facility ,
        cs:radio-station ,
        cs:telephone-exchange ,
        cs:television-communication-facility ,
        cs:television-station ;
    skos:prefLabel "Communication Infrastructure"@en ;
.

cs:communication-tower
    a skos:Concept ;
    rdfs:isDefinedBy cs: ;
    skos:altLabel
        "broadcasting tower"@en ,
        "mobile phone tower"@en ,
        "phone tower"@en ,
        "radio mast"@en ,
        "radio tower"@en ,
        "television tower"@en ;
    skos:definition "A structure that supports communication devices"@en ;
    skos:historyNote "Agreed at ICSM PNWG Meeting 2022" ;
    skos:inScheme cs: ;
    skos:prefLabel "Communication Tower"@en ;
.

cs:community-centre
    a skos:Concept ;
    rdfs:isDefinedBy cs: ;
    skos:altLabel
        "community home"@en ,
        "multicultural centre"@en ;
    skos:definition "A building used by members of the community for social gatherings, educational activities."@en ;
    skos:historyNote "PSMA" ;
    skos:inScheme cs: ;
    skos:prefLabel "Community Centre"@en ;
.

cs:community-facility
    a skos:Concept ;
    rdfs:isDefinedBy cs: ;
    skos:definition "Places to support specific public activities"@en ;
    skos:inScheme cs: ;
    skos:narrower
        cs:ampitheatre ,
        cs:arboretum ,
        cs:art-gallery ,
        cs:botanic-gardens ,
        cs:cemetery ,
        cs:community-centre ,
        cs:community-gardens ,
        cs:conservatory ,
        cs:group-camp ,
        cs:hall ,
        cs:library ,
        cs:museum ,
        cs:park ,
        cs:picnic-site ,
        cs:rotunda ,
        cs:showground ;
    skos:prefLabel "Community Facility"@en ;
.

cs:community-gardens
    a skos:Concept ;
    rdfs:isDefinedBy cs: ;
    skos:definition "A piece of land which is managed and encourages members of the community to cultivate primarily for the production of food and to contribute to sustainability."@en ;
    skos:inScheme cs: ;
    skos:prefLabel "Community Gardens"@en ;
.

cs:community-health-centre
    a skos:Concept ;
    rdfs:isDefinedBy cs: ;
    skos:definition "A health facility that caters for the community, urban and rural"@en ;
    skos:historyNote "PSMA" ;
    skos:inScheme cs: ;
    skos:prefLabel "Community Health Centre"@en ;
.

cs:community-living
    a skos:Concept ;
    rdfs:isDefinedBy cs: ;
    skos:definition "Places that provide medium to long term accommodation in a structured environment"@en ;
    skos:inScheme cs: ;
    skos:narrower
        cs:commune ,
        cs:residential-aged-care ,
        cs:retirement-village ;
    skos:prefLabel "Community Living"@en ;
.

cs:conservation-park
    a skos:Concept ;
    rdfs:isDefinedBy cs: ;
    skos:altLabel "BioSphere Reserve"@en ;
    skos:definition "An area of land which is not a National Park but is protected to ensure the cultural heritage and/or natural features are safeguarded."@en ;
    skos:historyNote "PSMA" ;
    skos:inScheme cs: ;
    skos:prefLabel "Conservation Park"@en ;
.

cs:conservatory
    a skos:Concept ;
    rdfs:isDefinedBy cs: ;
    skos:definition "a public building with a glass roof and walls and used for growing delicate plants"@en ;
    skos:historyNote "PSMA" ;
    skos:inScheme cs: ;
    skos:prefLabel "Conservatory"@en ;
.

cs:continent
    a skos:Concept ;
    rdfs:isDefinedBy cs: ;
    skos:definition "One of the main continuous bodies of land on the earth's surface."@en ;
    skos:historyNote "Definition form the Oxford English Dictionary." ;
    skos:inScheme cs: ;
    skos:prefLabel "Continent"@en ;
    schema:citation "https://www.oed.com/search/dictionary/?scope=Entries&q=continent"^^xsd:anyURI ;
.

cs:control-tower
    a skos:Concept ;
    rdfs:isDefinedBy cs: ;
    skos:altLabel "port control tower/harbour control tower"@en ;
    skos:definition "Air and shipping control towers"@en ;
    skos:inScheme cs: ;
    skos:prefLabel "Control Tower"@en ;
.

cs:coral-reef
    a skos:Concept ;
    rdfs:isDefinedBy cs: ;
    skos:definition "To be defined."@en ;
    skos:historyNote "Added by QLD 2024-03-05" ;
    skos:inScheme cs: ;
    skos:prefLabel "Coral Reef"@en ;
.

cs:corner
    a skos:Concept ;
    rdfs:isDefinedBy cs: ;
    skos:definition "A place where two boundaries meet; a region; a remote place"@en ;
    skos:historyNote "Agreed at ICSM PNWG Meeting 2022" ;
    skos:inScheme cs: ;
    skos:prefLabel "Corner"@en ;
.

cs:county
    a skos:Concept ;
    rdfs:isDefinedBy cs: ;
    skos:definition "A subdivision of Australia into land units"@en ;
    skos:historyNote "PSMA" ;
    skos:inScheme cs: ;
    skos:prefLabel "County"@en ;
.

cs:crater
    a skos:Concept ;
    rdfs:isDefinedBy cs: ;
    skos:definition "A bowl-shaped hollow in the Earth's surface"@en ;
    skos:historyNote "PSMA" ;
    skos:inScheme cs: ;
    skos:narrower
        cs:meteorite-crater ,
        cs:volcanic-crater ;
    skos:prefLabel "Crater"@en ;
.

cs:croquet-green
    a skos:Concept ;
    rdfs:isDefinedBy cs: ;
    skos:definition "An area of land on which the game of Croquet is played."@en ;
    skos:historyNote "PSMA" ;
    skos:inScheme cs: ;
    skos:prefLabel "Croquet Green"@en ;
.

cs:cultural-feature
    a skos:Concept ;
    rdfs:isDefinedBy cs: ;
    skos:definition "Places that support activities and interactions of the community"@en ;
    skos:inScheme cs: ;
    skos:narrower
        cs:accommodations ,
        cs:agriculture ,
        cs:aquaculture ,
        cs:business ,
        cs:community-facility ,
        cs:community-living ,
        cs:industrial-production-facility ,
        cs:landmark ,
        cs:place-of-worship ,
        cs:recreational-facility ,
        cs:tourist-attraction ;
    skos:prefLabel "Cultural Feature"@en ;
    skos:topConceptOf cs: ;
.

cs:cycle-crossing
    a skos:Concept ;
    rdfs:isDefinedBy cs: ;
    skos:definition "A structure that facilitates the crossing of road, railway or watercourse over under or through another feature."@en ;
    skos:historyNote "new" ;
    skos:inScheme cs: ;
    skos:prefLabel "Cycle Crossing"@en ;
.

cs:dairy
    a skos:Concept ;
    rdfs:isDefinedBy cs: ;
    skos:definition "A site that processes milk and or milk related products."@en ;
    skos:historyNote "PSMA" ;
    skos:inScheme cs: ;
    skos:prefLabel "Dairy"@en ;
.

cs:dam
    a skos:Concept ;
    rdfs:isDefinedBy cs: ;
    skos:altLabel
        "catch"@en ,
        "farm bank"@en ,
        "farm dam"@en ;
    skos:definition "A small structure in generally undrained areas, built to contain water for stock purposes"@en ;
    skos:historyNote "GNR" ;
    skos:inScheme cs: ;
    skos:prefLabel "Dam"@en ;
.

cs:dam-wall
    a skos:Concept ;
    rdfs:isDefinedBy cs: ;
    skos:definition "A large man-made structure of earth, masonry, built across a stream or river to impound water for any purpose."@en ;
    skos:historyNote "Agreed at ICSM PNWG Meeting 2022" ;
    skos:inScheme cs: ;
    skos:prefLabel "Dam Wall"@en ;
.

cs:day-procedure-centre
    a skos:Concept ;
    rdfs:isDefinedBy cs: ;
    skos:altLabel "day surgery centre"@en ;
    skos:definition "A facility which undertakes minor medical procedures that do not require the patient to stay overnight as part of their recovery"@en ;
    skos:historyNote "PSMA" ;
    skos:inScheme cs: ;
    skos:prefLabel "Day Procedure Centre"@en ;
.

cs:defence-site
    a skos:Concept ;
    rdfs:isDefinedBy cs: ;
    skos:definition "An area of land or facility used for defence operations and/or training."@en ;
    skos:inScheme cs: ;
    skos:narrower
        cs:air-force-base ,
        cs:army-base ,
        cs:barracks ,
        cs:bombing-range ,
        cs:defence-training-area ,
        cs:naval-base ;
    skos:prefLabel "Defence Site"@en ;
    skos:topConceptOf cs: ;
.

cs:defence-training-area
    a skos:Concept ;
    rdfs:isDefinedBy cs: ;
    skos:definition "An area of land or facility used for the training of defence personnel."@en ;
    skos:inScheme cs: ;
    skos:prefLabel "Defence Training Area"@en ;
.

cs:dental-hospital
    a skos:Concept ;
    rdfs:isDefinedBy cs: ;
    skos:definition "To be defined."@en ;
    skos:historyNote "Added by QLD 2024-03-05" ;
    skos:inScheme cs: ;
    skos:prefLabel "Dental Hospital"@en ;
.

cs:depression
    a skos:Concept ;
    rdfs:isDefinedBy cs: ;
    skos:altLabel "Natural amphitheater"@en ;
    skos:definition "Any hollow or relatively sunken area, on land"@en ;
    skos:inScheme cs: ;
    skos:prefLabel "Depression"@en ;
.

cs:desert
    a skos:Concept ;
    rdfs:isDefinedBy cs: ;
    skos:definition "An almost barren tract of land on which precipitation is so scant or spasmodic that it will not adequately support vegetation"@en ;
    skos:historyNote "Agreed at ICSM PNWG Meeting 2022" ;
    skos:inScheme cs: ;
    skos:prefLabel "Desert"@en ;
.

cs:diplomatic-mission
    a skos:Concept ;
    rdfs:isDefinedBy cs: ;
    skos:altLabel
        "Consulate"@en ,
        "Embassy"@en ,
        "High Commission"@en ;
    skos:definition "Office of a country's diplomatic representatives."@en ;
    skos:historyNote "PSMA" ;
    skos:inScheme cs: ;
    skos:prefLabel "Diplomatic Mission"@en ;
.

cs:disability-support-facility
    a skos:Concept ;
    rdfs:isDefinedBy cs: ;
    skos:definition "A facility to support the care of those with disabilities."@en ;
    skos:historyNote "PSMA" ;
    skos:inScheme cs: ;
    skos:prefLabel "Disability Support Facility"@en ;
.

cs:distillery
    a skos:Concept ;
    rdfs:isDefinedBy cs: ;
    skos:definition "A place where spirits are manufactured"@en ;
    skos:historyNote "PSMA" ;
    skos:inScheme cs: ;
    skos:prefLabel "Distillery"@en ;
.

cs:dock
    a skos:Concept ;
    rdfs:isDefinedBy cs: ;
    skos:altLabel
        "Dry dock"@en ,
        "wet dock"@en ;
    skos:definition "A structure where a vessel is constructed or repaired"@en ;
    skos:historyNote "GNR" ;
    skos:inScheme cs: ;
    skos:prefLabel "Dock"@en ;
.

cs:drain
    a skos:Concept ;
    rdfs:isDefinedBy cs: ;
    skos:altLabel
        "Bore drain"@en ,
        "Culvert"@en ;
    skos:definition "An artificially constructed WATERCOURSE designed for the purpose of removing surplus water from the land surface. Can be open or closed"@en ;
    skos:historyNote "GNR" ;
    skos:inScheme cs: ;
    skos:prefLabel "Drain"@en ;
.

cs:drive-in-theatre
    a skos:Concept ;
    rdfs:isDefinedBy cs: ;
    skos:altLabel "Drive-in"@en ;
    skos:definition "To be defined."@en ;
    skos:inScheme cs: ;
    skos:prefLabel "Drive In Theatre"@en ;
.

cs:dune
    a skos:Concept ;
    rdfs:isDefinedBy cs: ;
    skos:altLabel
        "Sandhill"@en ,
        "Sandhills"@en ;
    skos:definition "A mound or ridge of drifted sand, occurring on the sea coast, near inland water bodies and in deserts"@en ;
    skos:historyNote "new" ;
    skos:inScheme cs: ;
    skos:prefLabel "Dune"@en ;
.

cs:early-education
    a skos:Concept ;
    rdfs:isDefinedBy cs: ;
    skos:altLabel
        "Kindergarten"@en ,
        "preschool"@en ;
    skos:definition "Pre-school to prepare children for primary education."@en ;
    skos:historyNote "PSMA" ;
    skos:inScheme cs: ;
    skos:prefLabel "Early Education Facility"@en ;
.

cs:education-complex
    a skos:Concept ;
    rdfs:isDefinedBy cs: ;
    skos:altLabel "Education Precinct"@en ;
    skos:definition "Education area containing multiple types of education centres"@en ;
    skos:historyNote "PSMA; Agreed at ICSM PNWG Meeting 2022" ;
    skos:inScheme cs: ;
    skos:prefLabel "Education Complex"@en ;
.

cs:educational-facility
    a skos:Concept ;
    rdfs:isDefinedBy cs: ;
    skos:definition "Places for the delivery of instruction and training"@en ;
    skos:inScheme cs: ;
    skos:narrower
        cs:academy ,
        cs:business-college ,
        cs:early-education ,
        cs:education-complex ,
        cs:further-education ,
        cs:school ,
        cs:school-camp ;
    skos:prefLabel "Educational Facility"@en ;
    skos:topConceptOf cs: ;
.

cs:emergency-complex
    a skos:Concept ;
    rdfs:isDefinedBy cs: ;
    skos:altLabel "Emergency Precinct"@en ;
    skos:definition "Emergency facility area containing multiple types of emergency facilities; each may have its own name."@en ;
    skos:historyNote "PSMA; Agreed at ICSM PNWG Meeting 2022" ;
    skos:inScheme cs: ;
    skos:prefLabel "Emergency Complex"@en ;
.

cs:emergency-control-centre
    a skos:Concept ;
    rdfs:isDefinedBy cs: ;
    skos:definition "A facility to coordinate multiple agencies."@en ;
    skos:historyNote "VMFEAT" ;
    skos:inScheme cs: ;
    skos:prefLabel "Emergency Control Centre"@en ;
.

cs:emergency-facility
    a skos:Concept ;
    rdfs:isDefinedBy cs: ;
    skos:definition "Places for the governance of emergency services"@en ;
    skos:inScheme cs: ;
    skos:narrower
        cs:ambulance-station ,
        cs:coast-guard ,
        cs:emergency-complex ,
        cs:emergency-control-centre ,
        cs:fire-lookout ,
        cs:fire-station ,
        cs:lifesaving-club ,
        cs:neighbourhood-safer-place ,
        cs:police-station ,
        cs:refuge ,
        cs:ses-facility ;
    skos:prefLabel "Emergency Facility"@en ;
    skos:topConceptOf cs: ;
.

cs:energy-infrastructure
    a skos:Concept ;
    rdfs:isDefinedBy cs: ;
    skos:definition "Facilities related to the generation/transmission/storage of power"@en ;
    skos:inScheme cs: ;
    skos:narrower
        cs:gas-pipeline ,
        cs:gas-plant ,
        cs:oil-pipeline ,
        cs:power-distribution ,
        cs:power-station ,
        cs:power-sub-station ,
        cs:power-sub-transmission ,
        cs:power-terminal-station ,
        cs:power-transmission ,
        cs:wind-turbine ;
    skos:prefLabel "Energy Infrastructure"@en ;
.

cs:entertainment-centre
    a skos:Concept ;
    rdfs:isDefinedBy cs: ;
    skos:altLabel
        "Conference Centre"@en ,
        "Exhibition Centre"@en ,
        "Theatre"@en ;
    skos:definition "A place for where the public can be entertained and or be educated."@en ;
    skos:historyNote "PSMA" ;
    skos:inScheme cs: ;
    skos:prefLabel "Entertainment Centre"@en ;
.

cs:entrance
    a skos:Concept ;
    rdfs:isDefinedBy cs: ;
    skos:definition "A passageway into enclosed waters"@en ;
    skos:historyNote "PSMA" ;
    skos:inScheme cs: ;
    skos:prefLabel "Entrance"@en ;
.

cs:equestrian-centre
    a skos:Concept ;
    rdfs:isDefinedBy cs: ;
    skos:definition "A place related to horses and riding."@en ;
    skos:historyNote "GNR" ;
    skos:inScheme cs: ;
    skos:prefLabel "Equestrian Centre"@en ;
.

cs:escarpment
    a skos:Concept ;
    rdfs:isDefinedBy cs: ;
    skos:altLabel "Scarp"@en ;
    skos:definition "The steep slope terminating a plateau or any level or upland surface"@en ;
    skos:historyNote "Agreed at ICSM PNWG Meeting 2022" ;
    skos:inScheme cs: ;
    skos:narrower cs:marine-escarpment ;
    skos:prefLabel "Escarpment"@en ;
.

cs:estuary
    a skos:Concept ;
    rdfs:isDefinedBy cs: ;
    skos:definition "(a) The portion of a RIVER where tidal effects are evident and where fresh water and sea water mix (b) The widening out lower portion of a tidal RIVER"@en ;
    skos:historyNote "GNR" ;
    skos:inScheme cs: ;
    skos:prefLabel "Estuary"@en ;
.

cs:eye-and-ear-hospital
    a skos:Concept ;
    rdfs:isDefinedBy cs: ;
    skos:definition "To be defined."@en ;
    skos:historyNote "Added by QLD 2024-03-05" ;
    skos:inScheme cs: ;
    skos:prefLabel "Eye and Ear Hospital"@en ;
.

cs:farm
    a skos:Concept ;
    rdfs:isDefinedBy cs: ;
    skos:altLabel
        "Agriculture establishment"@en ,
        "Research establishment"@en ,
        "Special purpose farm"@en ;
    skos:definition "A tract of land devoted for agricultural or horticultural purposes"@en ;
    skos:historyNote "PSMA" ;
    skos:inScheme cs: ;
    skos:prefLabel "Farm"@en ;
.

cs:federal-electorate
    a skos:Concept ;
    rdfs:isDefinedBy cs: ;
    skos:definition "An administrative area of Australia represented by a member of Parliament elected at a House of Representatives election."@en ;
    skos:inScheme cs: ;
    skos:prefLabel "Federal Electorate"@en ;
.

cs:fence
    a skos:Concept ;
    rdfs:isDefinedBy cs: ;
    skos:definition "A structure used to enclose an area."@en ;
    skos:inScheme cs: ;
    skos:prefLabel "Fence"@en ;
.

cs:ferry-route
    a skos:Concept ;
    rdfs:isDefinedBy cs: ;
    skos:definition "The set route taken by a ferry service"@en ;
    skos:historyNote "PSMA" ;
    skos:inScheme cs: ;
    skos:prefLabel "Ferry Route"@en ;
.

cs:fibre-optic-cable
    a skos:Concept ;
    rdfs:isDefinedBy cs: ;
    skos:definition "A cable used for the distribution of digital communications"@en ;
    skos:historyNote "NEW" ;
    skos:inScheme cs: ;
    skos:prefLabel "Fibre Optic Cable"@en ;
.

cs:fire-lookout
    a skos:Concept ;
    rdfs:isDefinedBy cs: ;
    skos:altLabel
        "Fire Tower"@en ,
        "Observation Tower"@en ;
    skos:definition "A high structure used to keep watch against the danger of fire."@en ;
    skos:historyNote "PSMA" ;
    skos:inScheme cs: ;
    skos:prefLabel "Fire Lookout"@en ;
.

cs:fire-station
    a skos:Concept ;
    rdfs:isDefinedBy cs: ;
    skos:definition "A building where the fire brigade, fire engines and other equipment are housed."@en ;
    skos:historyNote "PSMA; Agreed at ICSM PNWG Meeting 2022" ;
    skos:inScheme cs: ;
    skos:narrower
        cs:forest-industry-fire-station ,
        cs:rural-fire-station ;
    skos:prefLabel "Fire Station"@en ;
.

cs:firebreak
    a skos:Concept ;
    rdfs:isDefinedBy cs: ;
    skos:altLabel "Fireguard"@en ;
    skos:definition "A strip of ploughed or cleared land made to check the spread of fire."@en ;
    skos:historyNote "PSMA; Agreed at ICSM PNWG Meeting 2022" ;
    skos:inScheme cs: ;
    skos:prefLabel "Firebreak"@en ;
.

cs:firing-range
    a skos:Concept ;
    rdfs:isDefinedBy cs: ;
    skos:altLabel
        "Rifle range"@en ,
        "Shooting range"@en ;
    skos:definition "An area set aside for shooting practice."@en ;
    skos:historyNote "VMFEAT; Agreed at ICSM PNWG Meeting 2022" ;
    skos:inScheme cs: ;
    skos:prefLabel "Firing Range"@en ;
.

cs:fjord
    a skos:Concept ;
    rdfs:isDefinedBy cs: ;
    skos:definition "A long narrow inlet of the sea between high steep cliffs."@en ;
    skos:inScheme cs: ;
    skos:prefLabel "Fjord"@en ;
.

cs:ford
    a skos:Concept ;
    rdfs:isDefinedBy cs: ;
    skos:altLabel "Crossing"@en ;
    skos:definition "The shallow part of a river or other body of water which may be crossed by vehicle or by wading."@en ;
    skos:historyNote "Agreed at ICSM PNWG Meeting 2022" ;
    skos:inScheme cs: ;
    skos:prefLabel "Ford"@en ;
.

cs:foreshore
    a skos:Concept ;
    rdfs:isDefinedBy cs: ;
    skos:definition "To be defined."@en ;
    skos:inScheme cs: ;
    skos:prefLabel "Foreshore"@en ;
.

cs:forest
    a skos:Concept ;
    rdfs:isDefinedBy cs: ;
    skos:altLabel
        "Brushwood"@en ,
        "Copse"@en ,
        "Glade"@en ,
        "Grove"@en ,
        "Thicket"@en ,
        "Wood"@en ;
    skos:definition "A large wooded area having a thick growth of trees and plants."@en ;
    skos:inScheme cs: ;
    skos:prefLabel "Forest"@en ;
.

cs:forest-industry-fire-station
    a skos:Concept ;
    rdfs:isDefinedBy cs: ;
    skos:definition "To be defined."@en ;
    skos:inScheme cs: ;
    skos:prefLabel "Forest Industry Fire Station"@en ;
.

cs:fountain
    a skos:Concept ;
    rdfs:isDefinedBy cs: ;
    skos:definition "To be defined."@en ;
    skos:inScheme cs: ;
    skos:prefLabel "Fountain"@en ;
.

cs:further-education
    a skos:Concept ;
    rdfs:isDefinedBy cs: ;
    skos:altLabel "Further Education Facility"@en ;
    skos:definition "Post secondary education facility"@en ;
    skos:historyNote "PSMA; Agreed at ICSM PNWG Meeting 2022" ;
    skos:inScheme cs: ;
    skos:narrower
        cs:tafe-facility ,
        cs:university ;
    skos:prefLabel "Tertiary Education Facility"@en ;
.

cs:gas-field
    a skos:Concept ;
    rdfs:isDefinedBy cs: ;
    skos:definition "An area in which gas resources have been identified."@en ;
    skos:inScheme cs: ;
    skos:prefLabel "Gas Field"@en ;
.

cs:gas-pipeline
    a skos:Concept ;
    rdfs:isDefinedBy cs: ;
    skos:definition "A long pipe, typically underground, used to transport gas over long distances"@en ;
    skos:historyNote "new" ;
    skos:inScheme cs: ;
    skos:prefLabel "Gas Pipeline"@en ;
.

cs:gas-plant
    a skos:Concept ;
    rdfs:isDefinedBy cs: ;
    skos:altLabel
        "gas conditioning plant"@en ,
        "gas processing plant"@en ;
    skos:definition "A place where gas is processed and/ or stored"@en ;
    skos:historyNote "VMFEAT; Agreed at ICSM PNWG Meeting 2022" ;
    skos:inScheme cs: ;
    skos:prefLabel "Gas Plant"@en ;
.

cs:gas-platform
    a skos:Concept ;
    rdfs:isDefinedBy cs: ;
    skos:definition "A large structure with facilities to drill wells, to extract and process natural gas."@en ;
    skos:inScheme cs: ;
    skos:prefLabel "Gas Platform"@en ;
.

cs:gas-power-station
    a skos:Concept ;
    rdfs:isDefinedBy cs: ;
    skos:definition "A process plant that creates power from gas."@en ;
    skos:inScheme cs: ;
    skos:prefLabel "Gas Power Station"@en ;
.

cs:gas-well
    a skos:Concept ;
    rdfs:isDefinedBy cs: ;
    skos:definition "A hole drilled into the ground to extract gas."@en ;
    skos:inScheme cs: ;
    skos:prefLabel "Gas Well"@en ;
.

cs:gate
    a skos:Concept ;
    rdfs:isDefinedBy cs: ;
    skos:definition "A structure used to regulate movement associated with road"@en ;
    skos:historyNote "Agreed at ICSM PNWG Meeting 2022" ;
    skos:inScheme cs: ;
    skos:prefLabel "Gate"@en ;
.

cs:general-hospital
    a skos:Concept ;
    rdfs:isDefinedBy cs: ;
    skos:definition "An institution in which sick or injured persons are given medical or surgical treatment"@en ;
    skos:historyNote "PSMA" ;
    skos:inScheme cs: ;
    skos:prefLabel "General Hospital"@en ;
.

cs:general-hospital-emergency
    a skos:Concept ;
    rdfs:isDefinedBy cs: ;
    skos:definition "A general hospital with 24-hour emergency service"@en ;
    skos:historyNote "PSMA" ;
    skos:inScheme cs: ;
    skos:prefLabel "General Hospital with Emergency"@en ;
.

cs:geothermal-power-station
    a skos:Concept ;
    rdfs:isDefinedBy cs: ;
    skos:definition "A process plant that creates power from geothermal sources."@en ;
    skos:inScheme cs: ;
    skos:prefLabel "Geothermal Power Station"@en ;
.

cs:glacier
    a skos:Concept ;
    rdfs:isDefinedBy cs: ;
    skos:definition "A mass of snow and ice continuously moving from higher to lower ground or, if afloat, continuously spreading."@en ;
    skos:historyNote "Concept and definition from the Australian Antarctic Division." ;
    skos:inScheme cs: ;
    skos:prefLabel "Glacier"@en ;
    schema:citation "https://data.aad.gov.au/aadc/ftc/display_feature_type.cfm?feature_type_code=196"^^xsd:anyURI ;
.

cs:gold-field
    a skos:Concept ;
    rdfs:isDefinedBy cs: ;
    skos:definition "An area in which gold deposits have been found and where mines have been established."@en ;
    skos:historyNote "GNR" ;
    skos:inScheme cs: ;
    skos:prefLabel "Gold Field"@en ;
.

cs:gold-refinery
    a skos:Concept ;
    rdfs:isDefinedBy cs: ;
    skos:definition "A refinery for extracting gold."@en ;
    skos:historyNote "PSMA" ;
    skos:inScheme cs: ;
    skos:prefLabel "Gold Refinery"@en ;
.

cs:golf-course
    a skos:Concept ;
    rdfs:isDefinedBy cs: ;
    skos:altLabel "Golf Driving Range"@en ;
    skos:definition "A ground or course over which golf is played"@en ;
    skos:historyNote "PSMA" ;
    skos:inScheme cs: ;
    skos:prefLabel "Golf Course"@en ;
.

cs:gorge
    a skos:Concept ;
    rdfs:isDefinedBy cs: ;
    skos:altLabel
        "CHASM"@en ,
        "Canyon"@en ,
        "RAVINE"@en ;
    skos:definition "A valley which is more than usually deep and narrow, with steep walls"@en ;
    skos:historyNote "PSMA" ;
    skos:inScheme cs: ;
    skos:prefLabel "Gorge"@en ;
.

cs:grandstand
    a skos:Concept ;
    rdfs:isDefinedBy cs: ;
    skos:definition "A terraced block of seats, usually under a roof, commanding the best view."@en ;
    skos:historyNote "PSMA" ;
    skos:inScheme cs: ;
    skos:prefLabel "Grandstand"@en ;
.

cs:grassland
    a skos:Concept ;
    rdfs:isDefinedBy cs: ;
    skos:definition "An area in which the natural vegetation consists primarily of perennial grasses."@en ;
    skos:inScheme cs: ;
    skos:prefLabel "Grassland"@en ;
.

cs:greyhound-racetrack
    a skos:Concept ;
    rdfs:isDefinedBy cs: ;
    skos:definition "A track enclosed by rails with start and finish points over which a specific bread of dog is raced."@en ;
    skos:historyNote "VMFEAT" ;
    skos:inScheme cs: ;
    skos:prefLabel "Greyhound Racetrack"@en ;
.

cs:grotto
    a skos:Concept ;
    rdfs:isDefinedBy cs: ;
    skos:definition "To be defined."@en ;
    skos:inScheme cs: ;
    skos:prefLabel "Grotto"@en ;
.

cs:group-camp
    a skos:Concept ;
    rdfs:isDefinedBy cs: ;
    skos:altLabel "Scout Camp"@en ;
    skos:definition "A place where tents, cabins, or other temporary structures are erected for the use by a particular group."@en ;
    skos:historyNote "PSMA" ;
    skos:inScheme cs: ;
    skos:prefLabel "Group Camp"@en ;
.

cs:gulf
    a skos:Concept ;
    rdfs:isDefinedBy cs: ;
    skos:altLabel "BIGHT"@en ;
    skos:definition "An area of sea partly enclosed by land, taking the form of a long narrow stretch of water larger than a loop."@en ;
    skos:inScheme cs: ;
    skos:prefLabel "Gulf"@en ;
.

cs:gurdwara
    a skos:Concept ;
    rdfs:isDefinedBy cs: ;
    skos:definition "Sikh place of worship."@en ;
    skos:historyNote "PSMA" ;
    skos:inScheme cs: ;
    skos:prefLabel "Gurdwara"@en ;
.

cs:hall
    a skos:Concept ;
    rdfs:isDefinedBy cs: ;
    skos:altLabel "Town Hall"@en ;
    skos:definition "A building where people may gather"@en ;
    skos:historyNote "PSMA" ;
    skos:inScheme cs: ;
    skos:prefLabel "Hall"@en ;
.

cs:hangar
    a skos:Concept ;
    rdfs:isDefinedBy cs: ;
    skos:definition "Facility for housing aircraft and or associated infrastructure."@en ;
    skos:historyNote "PSMA" ;
    skos:inScheme cs: ;
    skos:prefLabel "Hangar"@en ;
.

cs:harbour
    a skos:Concept ;
    rdfs:isDefinedBy cs: ;
    skos:definition "An artificially improved body of water providing protection for vessels, and often anchorage and docking facilities."@en ;
    skos:historyNote "GNR" ;
    skos:inScheme cs: ;
    skos:prefLabel "Harbour"@en ;
.

cs:harness-racetrack
    a skos:Concept ;
    rdfs:isDefinedBy cs: ;
    skos:altLabel "Trotting track"@en ;
    skos:definition "A track enclosed by rails with start and finish points over which standardbred horses are harnessed to race."@en ;
    skos:historyNote "VMFOI" ;
    skos:inScheme cs: ;
    skos:prefLabel "Harness Racetrack"@en ;
.

cs:hatchery
    a skos:Concept ;
    rdfs:isDefinedBy cs: ;
    skos:definition "To be defined."@en ;
    skos:inScheme cs: ;
    skos:prefLabel "Hatchery"@en ;
.

cs:health-facility
    a skos:Concept ;
    rdfs:isDefinedBy cs: ;
    skos:definition "a building for treatment of people"@en ;
    skos:inScheme cs: ;
    skos:narrower
        cs:community-health-centre ,
        cs:hospital ,
        cs:maternal-and-child-health-centre ,
        cs:medical-centre ;
    skos:prefLabel "Health Facility"@en ;
    skos:topConceptOf cs: ;
.

cs:helipad
    a skos:Concept ;
    rdfs:isDefinedBy cs: ;
    skos:definition "A place for helicopters to land and take-off, like 'runway' is to 'airport'"@en ;
    skos:historyNote "VMTRANS" ;
    skos:inScheme cs: ;
    skos:prefLabel "Helipad"@en ;
.

cs:heliport
    a skos:Concept ;
    rdfs:isDefinedBy cs: ;
    skos:definition "An airport for helicopters."@en ;
    skos:historyNote "PSMA" ;
    skos:inScheme cs: ;
    skos:prefLabel "Heliport"@en ;
.

cs:hill
    a skos:Concept ;
    rdfs:isDefinedBy cs: ;
    skos:altLabel
        "Butte"@en ,
        "Hillock"@en ,
        "KNOB"@en ,
        "KNOLL"@en ,
        "MESA"@en ,
        "SUGARLOAF"@en ,
        "TOR"@en ;
    skos:definition "A small portion of the Earth's surface elevated above its surroundings. In general, a feature is not considered a mountain unless its elevation, from foot to summit, is well over 300m, but the distinction is arbitrary"@en ;
    skos:historyNote "PSMA; Agreed at ICSM PNWG Meeting 2022" ;
    skos:inScheme cs: ;
    skos:narrower cs:marine-hill ;
    skos:prefLabel "Hill"@en ;
.

cs:historic-site
    a skos:Concept ;
    rdfs:isDefinedBy cs: ;
    skos:altLabel "ruin"@en ;
    skos:definition "A specific place or site which has at one time been the site of an event or activity which is now remembered or commemorated."@en ;
    skos:historyNote "PSMA" ;
    skos:inScheme cs: ;
    skos:prefLabel "Historic Site"@en ;
.

cs:hockey-ground
    a skos:Concept ;
    rdfs:isDefinedBy cs: ;
    skos:definition "A place where hockey is played."@en ;
    skos:historyNote "PSMA" ;
    skos:inScheme cs: ;
    skos:prefLabel "Hockey Ground"@en ;
.

cs:holiday-park
    a skos:Concept ;
    rdfs:isDefinedBy cs: ;
    skos:altLabel "Tourist Park"@en ;
    skos:definition "A site for holidaymakers which offers various types of accommodation including caravan or tent sites."@en ;
    skos:inScheme cs: ;
    skos:narrower cs:caravan-park ;
    skos:prefLabel "Holiday Park"@en ;
.

cs:homestead
    a skos:Concept ;
    rdfs:isDefinedBy cs: ;
    skos:definition "A main residence on a horticultural or agricultural farm."@en ;
    skos:historyNote "PSMA" ;
    skos:inScheme cs: ;
    skos:prefLabel "Homestead"@en ;
.

cs:horse-riding-trail
    a skos:Concept ;
    rdfs:isDefinedBy cs: ;
    skos:altLabel "Bridle path"@en ;
    skos:definition "A trail designed for horse riding traffic in the main."@en ;
    skos:historyNote "new" ;
    skos:inScheme cs: ;
    skos:prefLabel "Horse Riding Trail"@en ;
.

cs:hospital
    a skos:Concept ;
    rdfs:isDefinedBy cs: ;
    skos:definition "To be defined."@en ;
    skos:historyNote "Added by QLD 2024-03-05" ;
    skos:inScheme cs: ;
    skos:narrower
        cs:bush-nursing-hospital ,
        cs:day-procedure-centre ,
        cs:general-hospital ,
        cs:general-hospital-emergency ,
        cs:hospital-complex ,
        cs:specialised-hospital ;
    skos:prefLabel "Hospital"@en ;
.

cs:hospital-complex
    a skos:Concept ;
    rdfs:isDefinedBy cs: ;
    skos:altLabel "Hospital Precinct"@en ;
    skos:definition "An area containing multiple hospitals"@en ;
    skos:historyNote "PSMA; Agreed at ICSM PNWG Meeting 2022" ;
    skos:inScheme cs: ;
    skos:prefLabel "Hospital Complex"@en ;
.

cs:hut
    a skos:Concept ;
    rdfs:isDefinedBy cs: ;
    skos:definition "A simple, usually small, building which may be used for temporary accommodation, as for bushwalkers or skiers."@en ;
    skos:historyNote "PSMA" ;
    skos:inScheme cs: ;
    skos:prefLabel "Hut"@en ;
.

cs:hydroelectric-power-station
    a skos:Concept ;
    rdfs:isDefinedBy cs: ;
    skos:altLabel "Hydro Power Station"@en ;
    skos:definition "A process plant that creates power from gravity induced flow of water."@en ;
    skos:inScheme cs: ;
    skos:prefLabel "Hydroelectric Power Station"@en ;
.

cs:hydrological-feature
    a skos:Concept ;
    rdfs:isDefinedBy cs: ;
    skos:definition "Natural or man-made places which relate to the surface and underground water or marine environments"@en ;
    skos:inScheme cs: ;
    skos:narrower
        cs:anchorage ,
        cs:water-body ,
        cs:water-infrastructure ,
        cs:water-point ,
        cs:waterway ;
    skos:prefLabel "Hydrological Feature"@en ;
    skos:topConceptOf cs: ;
.

cs:ice-dome
    a skos:Concept ;
    rdfs:isDefinedBy cs: ;
    skos:definition "A rounded and gently sloping elevation in the surface of an inland ice sheet. Ice domes do not have precisely defined margins and may cover very large areas - more than 100,000km sq."@en ;
    skos:historyNote "Concept and definition from the Australian Antarctic Division." ;
    skos:inScheme cs: ;
    skos:prefLabel "Ice Dome"@en ;
    schema:citation "https://data.aad.gov.au/aadc/ftc/display_feature_type.cfm?feature_type_code=167"^^xsd:anyURI ;
.

cs:ice-feature
    a skos:Concept ;
    rdfs:isDefinedBy cs: ;
    skos:definition "Feature related to ice forms."@en ;
    skos:inScheme cs: ;
    skos:narrower
        cs:glacier ,
        cs:ice-dome ,
        cs:ice-field ,
        cs:ice-massif ,
        cs:ice-rise ,
        cs:ice-shelf ,
        cs:ice-stream ,
        cs:ice-tongue ,
        cs:ice-wall ,
        cs:icefall ,
        cs:neve ;
    skos:prefLabel "Ice Feature"@en ;
    skos:topConceptOf cs: ;
.

cs:ice-field
    a skos:Concept ;
    rdfs:isDefinedBy cs: ;
    skos:definition "Flat glaciated area, underlying topography is not completely levelled out"@en ;
    skos:historyNote "Concept and definition from the Australian Antarctic Division." ;
    skos:inScheme cs: ;
    skos:prefLabel "Ice Field"@en ;
    schema:citation "https://data.aad.gov.au/aadc/ftc/display_feature_type.cfm?feature_type_code=210"^^xsd:anyURI ;
.

cs:ice-massif
    a skos:Concept ;
    rdfs:isDefinedBy cs: ;
    skos:definition "Compact group of mountain heights, which may be partly or almost entirely ice-covered."@en ;
    skos:historyNote "Concept and definition from the Australian Antarctic Division." ;
    skos:inScheme cs: ;
    skos:prefLabel "Ice Massif"@en ;
    schema:citation "https://data.aad.gov.au/aadc/ftc/display_feature_type.cfm?feature_type_code=392"^^xsd:anyURI ;
.

cs:ice-rise
    a skos:Concept ;
    rdfs:isDefinedBy cs: ;
    skos:definition "A mass of ice resting on rock and surrounded either by an ice shelf, or partly by an ice shelf and partly by sea. No rock is exposed and there may be none above sea level. Ice rises often have a dome-shaped surface. The largest known is about 100km across."@en ;
    skos:historyNote "Concept and definition from the Australian Antarctic Division." ;
    skos:inScheme cs: ;
    skos:prefLabel "Ice Rise"@en ;
    schema:citation "https://data.aad.gov.au/aadc/ftc/display_feature_type.cfm?feature_type_code=213"^^xsd:anyURI ;
.

cs:ice-shelf
    a skos:Concept ;
    rdfs:isDefinedBy cs: ;
    skos:definition "A floating ice sheet of considerable thickness attached to a coast. Ice shelves are usually of great horizontal extent and have a level or gently undulating surface. They are nourished by the accumulation of snow and often by seaward extension of land glaciers. Limited areas may be aground. The seaward edge is termed an ice front."@en ;
    skos:historyNote "Concept and definition from the Australian Antarctic Division." ;
    skos:inScheme cs: ;
    skos:prefLabel "Ice Shelf"@en ;
    schema:citation "https://data.aad.gov.au/aadc/ftc/display_feature_type.cfm?feature_type_code=298"^^xsd:anyURI ;
.

cs:ice-stream
    a skos:Concept ;
    rdfs:isDefinedBy cs: ;
    skos:definition "Part of an ice sheet in which the ice flows more rapidly and not necessarily in the same direction as the surrounding ice. The margins are sometimes clearly marked by a change in direction of the surface slope, but may be indistinct."@en ;
    skos:historyNote "Concept and definition from the Australian Antarctic Division." ;
    skos:inScheme cs: ;
    skos:prefLabel "Ice Stream"@en ;
    schema:citation "https://data.aad.gov.au/aadc/ftc/display_feature_type.cfm?feature_type_code=215"^^xsd:anyURI ;
.

cs:ice-tongue
    a skos:Concept ;
    rdfs:isDefinedBy cs: ;
    skos:definition "A projection of the ice edge up to several km in length caused by wind and current."@en ;
    skos:historyNote "Concept and definition from the Australian Antarctic Division." ;
    skos:inScheme cs: ;
    skos:prefLabel "Ice Tongue"@en ;
    schema:citation "https://data.aad.gov.au/aadc/ftc/display_feature_type.cfm?feature_type_code=325"^^xsd:anyURI ;
.

cs:icefall
    a skos:Concept ;
    rdfs:isDefinedBy cs: ;
    skos:definition "The portion of a glacier at a point of steep descent, segmented by many transverse crevasses into separate blocks."@en ;
    skos:historyNote "Concept and definition from the Australian Antarctic Division." ;
    skos:inScheme cs: ;
    skos:prefLabel "Icefall"@en ;
    schema:citation "https://data.aad.gov.au/aadc/ftc/display_feature_type.cfm?feature_type_code=218"^^xsd:anyURI ;
.

cs:indigenous-protected-area
    a skos:Concept ;
    rdfs:isDefinedBy cs: ;
    skos:altLabel "IPA"@en ;
    skos:definition "An Indigenous Protected Area is an area of Indigenous-owned land or sea where Traditional Owners have entered into an agreement with the Australian Government to promote biodiversity and cultural resource conservation."@en ;
    skos:historyNote "PSMA" ;
    skos:inScheme cs: ;
    skos:prefLabel "Indigenous Protected Area"@en ;
.

cs:industrial-production-facility
    a skos:Concept ;
    rdfs:isDefinedBy cs: ;
    skos:definition "Places where the major activity is of a manufacturing or processing nature"@en ;
    skos:inScheme cs: ;
    skos:narrower
        cs:abattoir ,
        cs:brewery ,
        cs:brickworks ,
        cs:cement-plant ,
        cs:distillery ,
        cs:steel-works ,
        cs:sugar-refinery ,
        cs:tannery ,
        cs:timber-operations ,
        cs:winery ;
    skos:prefLabel "Industrial Production Facility"@en ;
.

cs:inlet
    a skos:Concept ;
    rdfs:isDefinedBy cs: ;
    skos:altLabel "ARM"@en ;
    skos:definition "A small indentation in a waterline usually tapering towards its head"@en ;
    skos:historyNote "GNR" ;
    skos:inScheme cs: ;
    skos:prefLabel "Inlet"@en ;
.

cs:iron-ore-processor
    a skos:Concept ;
    rdfs:isDefinedBy cs: ;
    skos:definition "An iron ore processing plant"@en ;
    skos:historyNote "PSMA" ;
    skos:inScheme cs: ;
    skos:prefLabel "Iron Ore Processor"@en ;
.

cs:irrigation-channel
    a skos:Concept ;
    rdfs:isDefinedBy cs: ;
    skos:altLabel "Aqueduct"@en ;
    skos:definition "An artificial watercourse used for irrigation. Can be open or closed"@en ;
    skos:inScheme cs: ;
    skos:prefLabel "Irrigation Channel"@en ;
.

cs:island
    a skos:Concept ;
    rdfs:isDefinedBy cs: ;
    skos:definition "A tract of land completely surrounded by water."@en ;
    skos:historyNote "VMLITE" ;
    skos:inScheme cs: ;
    skos:narrower
        cs:atoll ,
        cs:cay ,
        cs:clumps ,
        cs:islet ,
        cs:offshore-rock ,
        cs:skerry ;
    skos:prefLabel "Island"@en ;
.

cs:island-group
    a skos:Concept ;
    rdfs:isDefinedBy cs: ;
    skos:altLabel "Archipelago"@en ;
    skos:definition "A group of islands often with a common name which covers the group. The islands may have their own individual names. The island group can include any combination of rocks, reefs, islets and island names"@en ;
    skos:inScheme cs: ;
    skos:prefLabel "Island Group"@en ;
.

cs:islet
    a skos:Concept ;
    rdfs:isDefinedBy cs: ;
    skos:altLabel "Isle"@en ;
    skos:definition "A small island"@en ;
    skos:inScheme cs: ;
    skos:prefLabel "Islet"@en ;
.

cs:isthmus
    a skos:Concept ;
    rdfs:isDefinedBy cs: ;
    skos:altLabel "Neck"@en ;
    skos:definition "A narrow portion of land enclosed on each side by water and connecting two larger bodies of land"@en ;
    skos:inScheme cs: ;
    skos:prefLabel "Isthmus"@en ;
.

cs:jetty
    a skos:Concept ;
    rdfs:isDefinedBy cs: ;
    skos:definition "A structure of stone or timber projecting into water, often for private use and significantly smaller than a pier."@en ;
    skos:historyNote "GNR; Agreed at ICSM PNWG Meeting 2022" ;
    skos:inScheme cs: ;
    skos:prefLabel "Jetty"@en ;
.

cs:junction
    a skos:Concept ;
    rdfs:isDefinedBy cs: ;
    skos:altLabel
        "Road Bend"@en ,
        "Road corner"@en ;
    skos:definition "A place where RIVERS, ROADS or RAILWAYS intersect."@en ;
    skos:historyNote "PSMA" ;
    skos:inScheme cs: ;
    skos:prefLabel "Junction"@en ;
.

cs:lagoon
    a skos:Concept ;
    rdfs:isDefinedBy cs: ;
    skos:definition "An enclosed area of shallow salt or brackish water which is partly or completely separated from the SEA."@en ;
    skos:inScheme cs: ;
    skos:prefLabel "Lagoon"@en ;
.

cs:lake
    a skos:Concept ;
    rdfs:isDefinedBy cs: ;
    skos:altLabel
        "back water"@en ,
        "backwash"@en ,
        "billabong"@en ,
        "fresh water lagoon"@en ,
        "oxbow"@en ;
    skos:definition "A body of fresh or salt water, natural or artificial, enclosed or nearly enclosed by land; it may or may not have in and outflowing water (either permanent, intermittent or largely dry)"@en ;
    skos:historyNote "GNR" ;
    skos:inScheme cs: ;
    skos:prefLabel "Lake"@en ;
.

cs:land-district
    a skos:Concept ;
    rdfs:isDefinedBy cs: ;
    skos:altLabel "Land Division"@en ;
    skos:definition "A classification of land to assist in the administration of land"@en ;
    skos:historyNote "WA: 7/12/2017" ;
    skos:inScheme cs: ;
    skos:prefLabel "Land District"@en ;
.

cs:landfill
    a skos:Concept ;
    rdfs:isDefinedBy cs: ;
    skos:definition "A site where refuse is dumped and covered with earth."@en ;
    skos:historyNote "VMFEAT" ;
    skos:inScheme cs: ;
    skos:prefLabel "Landfill"@en ;
.

cs:landform
    a skos:Concept ;
    rdfs:isDefinedBy cs: ;
    skos:definition "Natural features of the Earth's surface"@en ;
    skos:inScheme cs: ;
    skos:narrower
        cs:bank ,
        cs:bar ,
        cs:basin ,
        cs:beach ,
        cs:bench ,
        cs:blowhole ,
        cs:cape ,
        cs:cave ,
        cs:cirque ,
        cs:cliff ,
        cs:coast ,
        cs:continent ,
        cs:crater ,
        cs:depression ,
        cs:desert ,
        cs:dune ,
        cs:escarpment ,
        cs:foreshore ,
        cs:gorge ,
        cs:hill ,
        cs:island ,
        cs:island-group ,
        cs:isthmus ,
        cs:ledge ,
        cs:moraine ,
        cs:mountain ,
        cs:nunatak ,
        cs:pan ,
        cs:pass ,
        cs:peak ,
        cs:peninsula ,
        cs:plain ,
        cs:plateau ,
        cs:pocket ,
        cs:point ,
        cs:range ,
        cs:ridge ,
        cs:rock ,
        cs:rockhole ,
        cs:slope ,
        cs:spit ,
        cs:tidal-flat ,
        cs:trench ,
        cs:valley ,
        cs:wall ;
    skos:prefLabel "Landform"@en ;
.

cs:landing-area
    a skos:Concept ;
    rdfs:isDefinedBy cs: ;
    skos:altLabel
        "Airfield"@en ,
        "Airstrip"@en ,
        "Runway"@en ,
        "landing ground"@en ;
    skos:definition "For the operation of aircraft, may be public or private."@en ;
    skos:historyNote "GNR" ;
    skos:inScheme cs: ;
    skos:prefLabel "Landing Area"@en ;
.

cs:landing-place
    a skos:Concept ;
    rdfs:isDefinedBy cs: ;
    skos:definition "A place where boats receive or discharge passengers and/or freight."@en ;
    skos:historyNote "Agreed at ICSM PNWG Meeting 2022" ;
    skos:inScheme cs: ;
    skos:prefLabel "Landing Place"@en ;
.

cs:landmark
    a skos:Concept ;
    rdfs:isDefinedBy cs: ;
    skos:definition "Places that are a recognised entity by the community for specific identification purposes."@en ;
    skos:inScheme cs: ;
    skos:narrower
        cs:building ,
        cs:colony ,
        cs:corner ,
        cs:fence ,
        cs:historic-site ,
        cs:homestead ,
        cs:hut ,
        cs:junction ,
        cs:levee ,
        cs:lookout ,
        cs:monument ,
        cs:outstation ,
        cs:rural-property ,
        cs:ship-wreck ,
        cs:survey-marker ;
    skos:prefLabel "Landmark"@en ;
.

cs:lava-tube
    a skos:Concept ;
    rdfs:isDefinedBy cs: ;
    skos:definition "To be defined."@en ;
    skos:inScheme cs: ;
    skos:prefLabel "Lava Tube"@en ;
.

cs:law-court
    a skos:Concept ;
    rdfs:isDefinedBy cs: ;
    skos:altLabel
        "COURT"@en ,
        "COURT HOUSE Supreme Court"@en ,
        "High Court OR TRIBUNAL"@en ,
        "Magistrates Court"@en ;
    skos:definition "A building which houses a tribunal which has power to adjudicate in civil, criminal or military matters."@en ;
    skos:historyNote "VMFEAT" ;
    skos:inScheme cs: ;
    skos:prefLabel "Law Court"@en ;
.

cs:ledge
    a skos:Concept ;
    rdfs:isDefinedBy cs: ;
    skos:definition "A narrow shelf-like projection on a cliff or on the side of a hill or mountain."@en ;
    skos:inScheme cs: ;
    skos:prefLabel "Ledge"@en ;
.

cs:legal-institution
    a skos:Concept ;
    rdfs:isDefinedBy cs: ;
    skos:definition "A facility relating to law or justice."@en ;
    skos:inScheme cs: ;
    skos:narrower
        cs:diplomatic-mission ,
        cs:law-court ,
        cs:prison ;
    skos:prefLabel "Legal Institution"@en ;
    skos:topConceptOf cs: ;
.

cs:library
    a skos:Concept ;
    rdfs:isDefinedBy cs: ;
    skos:definition "A place in which literary materials, such as books, periodicals, newspapers, pamphlets, prints, records, and tapes, are kept for reading, reference, or lending."@en ;
    skos:historyNote "PSMA" ;
    skos:inScheme cs: ;
    skos:prefLabel "Library"@en ;
.

cs:lifesaving-club
    a skos:Concept ;
    rdfs:isDefinedBy cs: ;
    skos:altLabel "Surf lifesaving club"@en ;
    skos:definition "A patrol and response service for those that are in difficulty in the water"@en ;
    skos:historyNote "PSMA; Agreed at ICSM PNWG Meeting 2022" ;
    skos:inScheme cs: ;
    skos:prefLabel "Lifesaving Club"@en ;
.

cs:light-rail-tunnel
    a skos:Concept ;
    rdfs:isDefinedBy cs: ;
    skos:definition "To be defined."@en ;
    skos:inScheme cs: ;
    skos:prefLabel "Light Rail Tunnel"@en ;
.

cs:lighthouse
    a skos:Concept ;
    rdfs:isDefinedBy cs: ;
    skos:definition "A distinctive structure on or off the COAST, exhibiting a major LIGHT designed to serve as an aid to navigation"@en ;
    skos:historyNote "PSMA" ;
    skos:inScheme cs: ;
    skos:prefLabel "Lighthouse"@en ;
.

cs:liquid-waste-disposal-site
    a skos:Concept ;
    rdfs:isDefinedBy cs: ;
    skos:altLabel "Dump point"@en ;
    skos:definition "A place for the disposal of liquid waste."@en ;
    skos:historyNote "PSMA" ;
    skos:inScheme cs: ;
    skos:prefLabel "Liquid Waste Disposal Site"@en ;
.

cs:local-government-area
    a skos:Concept ;
    rdfs:isDefinedBy cs: ;
    skos:altLabel
        "LGA"@en ,
        "Municipality"@en ,
        "Shire"@en ;
    skos:definition "A regional division of a State or Territory administered by local government"@en ;
    skos:inScheme cs: ;
    skos:prefLabel "Local Government Area"@en ;
.

cs:local-government-area-ward
    a skos:Concept ;
    rdfs:isDefinedBy cs: ;
    skos:altLabel
        "Division"@en ,
        "Local Government Area Division"@en ,
        "Ward"@en ;
    skos:definition "A division of a local government for electoral purposes."@en ;
    skos:inScheme cs: ;
    skos:prefLabel "Local Government Area Ward"@en ;
.

cs:locality
    a skos:Concept ;
    rdfs:isDefinedBy cs: ;
    skos:altLabel
        "Bounded Locality"@en ,
        "Suburb"@en ;
    skos:definition "An administrative bounded area distinguished for its community and/or landscape characteristics: in metropolitan areas it is commonly referred to as a ‘suburb’; it provides an official reference point for addressing purposes"@en ;
    skos:historyNote "VMADMIN" ;
    skos:inScheme cs: ;
    skos:prefLabel "Locality"@en ;
.

cs:lock
    a skos:Concept ;
    rdfs:isDefinedBy cs: ;
    skos:definition "A stretch of water in a RIVER or CANAL enclosed by gates fitted with sluices to enable craft to be raised from one water level to another"@en ;
    skos:inScheme cs: ;
    skos:prefLabel "Lock"@en ;
.

cs:lookout
    a skos:Concept ;
    rdfs:isDefinedBy cs: ;
    skos:altLabel "viewing platform"@en ;
    skos:definition "An observation or viewing point often a man-made structure."@en ;
    skos:historyNote "PSMA" ;
    skos:inScheme cs: ;
    skos:prefLabel "Lookout"@en ;
.

cs:mall
    a skos:Concept ;
    rdfs:isDefinedBy cs: ;
    skos:definition "To be defined."@en ;
    skos:historyNote "Added by QLD 2024-03-05" ;
    skos:inScheme cs: ;
    skos:prefLabel "Mall"@en ;
.

cs:marina
    a skos:Concept ;
    rdfs:isDefinedBy cs: ;
    skos:altLabel
        "Key"@en ,
        "Quay"@en ;
    skos:definition "An area provided with berthing and shore facilities (including toilets, water and rubbish disposal) particularly for yachts and other pleasure craft"@en ;
    skos:inScheme cs: ;
    skos:prefLabel "Marina"@en ;
.

cs:marine-apron
    a skos:Concept ;
    rdfs:isDefinedBy cs: ;
    skos:altLabel "Archipelagic Apron"@en ;
    skos:definition "A gently dipping SLOPE, with a smooth surface, commonly found around groups of islands and SEAMOUNTS."@en ;
    skos:historyNote "Definition from General Bathymetric Chart of the Oceans (GEBCO) Sub-Committee on Undersea Features Names (SCUFN)." ;
    skos:inScheme cs: ;
    skos:prefLabel "Marine Apron"@en ;
    schema:citation "https://iho.int/en/basic-documents-1"^^xsd:anyURI ;
.

cs:marine-caldera
    a skos:Concept ;
    rdfs:isDefinedBy cs: ;
    skos:definition "A roughly circular, cauldron-like depression generally characterised by steep sides and formed by collapse, or partial collapse, during or following a volcanic eruption."@en ;
    skos:historyNote "Definition from General Bathymetric Chart of the Oceans (GEBCO) Sub-Committee on Undersea Features Names (SCUFN)." ;
    skos:inScheme cs: ;
    skos:prefLabel "Marine Caldera"@en ;
    schema:citation "https://iho.int/en/basic-documents-1"^^xsd:anyURI ;
.

cs:marine-canyon
    a skos:Concept ;
    rdfs:isDefinedBy cs: ;
    skos:definition "An elongated, narrow, steep-sided depression that generally deepens down-slope."@en ;
    skos:historyNote "Definition from General Bathymetric Chart of the Oceans (GEBCO) Sub-Committee on Undersea Features Names (SCUFN)." ;
    skos:inScheme cs: ;
    skos:prefLabel "Marine Canyon"@en ;
    schema:citation "https://iho.int/en/basic-documents-1"^^xsd:anyURI ;
.

cs:marine-continental-margin
    a skos:Concept ;
    rdfs:isDefinedBy cs: ;
    skos:definition "The zone, generally consisting of SHELF, SLOPE and CONTINENTAL RISE, separating the continent from the deep seafloor or ABYSSAL PLAIN. Occasionally a TRENCH may be present in place of a CONTINENTAL RISE."@en ;
    skos:historyNote "Definition from General Bathymetric Chart of the Oceans (GEBCO) Sub-Committee on Undersea Features Names (SCUFN)." ;
    skos:inScheme cs: ;
    skos:prefLabel "Marine Continental Margin"@en ;
    schema:citation "https://iho.int/en/basic-documents-1"^^xsd:anyURI ;
.

cs:marine-fan
    a skos:Concept ;
    rdfs:isDefinedBy cs: ;
    skos:definition "A relatively smooth depositional feature continuously deepening away from a sediment source commonly located at the lower termination of a CANYON or canyon system."@en ;
    skos:historyNote "Definition from General Bathymetric Chart of the Oceans (GEBCO) Sub-Committee on Undersea Features Names (SCUFN)." ;
    skos:inScheme cs: ;
    skos:prefLabel "Marine Fan"@en ;
    schema:citation "https://iho.int/en/basic-documents-1"^^xsd:anyURI ;
.

cs:marine-fracture-zone
    a skos:Concept ;
    rdfs:isDefinedBy cs: ;
    skos:definition "A long narrow zone of irregular topography formed by the movement of tectonic plates associated with an offset of a spreading ridge axis, characterised by steep-sided and/or asymmetrical ridges, troughs or escarpments"@en ;
    skos:historyNote "Definition from General Bathymetric Chart of the Oceans (GEBCO) Sub-Committee on Undersea Features Names (SCUFN)." ;
    skos:inScheme cs: ;
    skos:prefLabel "Marine Fracture Zone"@en ;
    schema:citation "https://iho.int/en/basic-documents-1"^^xsd:anyURI ;
.

cs:marine-hole
    a skos:Concept ;
    rdfs:isDefinedBy cs: ;
    skos:definition "A depression of limited extent with all sides rising steeply from a relatively flat bottom."@en ;
    skos:historyNote "Definition from General Bathymetric Chart of the Oceans (GEBCO) Sub-Committee on Undersea Features Names (SCUFN)." ;
    skos:inScheme cs: ;
    skos:prefLabel "Marine Hole"@en ;
    schema:citation "https://iho.int/en/basic-documents-1"^^xsd:anyURI ;
.

cs:marine-knoll
    a skos:Concept ;
    rdfs:isDefinedBy cs: ;
    skos:definition "A distinct ELEVATION with a rounded profile less than 1000m above the surrounding relief as measured from the deepest isobath that surrounds most of the feature."@en ;
    skos:historyNote "Definition from General Bathymetric Chart of the Oceans (GEBCO) Sub-Committee on Undersea Features Names (SCUFN)." ;
    skos:inScheme cs: ;
    skos:prefLabel "Marine Knoll"@en ;
    schema:citation "https://iho.int/en/basic-documents-1"^^xsd:anyURI ;
.

cs:marine-levee
    a skos:Concept ;
    rdfs:isDefinedBy cs: ;
    skos:definition "A depositional embankment bordering a CANYON, VALLEY or SEA CHANNEL."@en ;
    skos:historyNote "Definition from General Bathymetric Chart of the Oceans (GEBCO) Sub-Committee on Undersea Features Names (SCUFN)." ;
    skos:inScheme cs: ;
    skos:prefLabel "Marine Levee"@en ;
    schema:citation "https://iho.int/en/basic-documents-1"^^xsd:anyURI ;
.

cs:marine-moat
    a skos:Concept ;
    rdfs:isDefinedBy cs: ;
    skos:definition "An annular or partially annular depression commonly located at the base of SEAMOUNTS, islands and other isolated ELEVATIONs."@en ;
    skos:historyNote "Definition from General Bathymetric Chart of the Oceans (GEBCO) Sub-Committee on Undersea Features Names (SCUFN)." ;
    skos:inScheme cs: ;
    skos:prefLabel "Marine Moat"@en ;
    schema:citation "https://iho.int/en/basic-documents-1"^^xsd:anyURI ;
.

cs:marine-mound
    a skos:Concept ;
    rdfs:isDefinedBy cs: ;
    skos:definition "A distinct ELEVATION with a rounded profile generally less than 500m above the surrounding relief as measured from the deepest isobath that surrounds most of the feature, commonly formed by the expulsion of fluids or by coral reef development, sedimentation and (bio)erosion."@en ;
    skos:historyNote "Definition from General Bathymetric Chart of the Oceans (GEBCO) Sub-Committee on Undersea Features Names (SCUFN)." ;
    skos:inScheme cs: ;
    skos:prefLabel "Marine Mound"@en ;
    schema:citation "https://iho.int/en/basic-documents-1"^^xsd:anyURI ;
.

cs:marine-mud-volcano
    a skos:Concept ;
    rdfs:isDefinedBy cs: ;
    skos:definition "A MOUND or cone-shaped ELEVATION formed by the expulsion of non-magmatic liquids and gasses."@en ;
    skos:historyNote "Definition from General Bathymetric Chart of the Oceans (GEBCO) Sub-Committee on Undersea Features Names (SCUFN)." ;
    skos:inScheme cs: ;
    skos:prefLabel "Marine Mud Volcano"@en ;
    schema:citation "https://iho.int/en/basic-documents-1"^^xsd:anyURI ;
.

cs:marine-park
    a skos:Concept ;
    rdfs:isDefinedBy cs: ;
    skos:altLabel "Aquatic Reserve"@en ;
    skos:definition "An area of sea, set apart, as by a state or nation, to be preserved in its natural state for the benefit of the public."@en ;
    skos:inScheme cs: ;
    skos:prefLabel "Marine Park"@en ;
.

cs:marine-peak
    a skos:Concept ;
    rdfs:isDefinedBy cs: ;
    skos:definition "A conical or pointed ELEVATION at the summit of a larger feature."@en ;
    skos:historyNote "Definition from General Bathymetric Chart of the Oceans (GEBCO) Sub-Committee on Undersea Features Names (SCUFN)." ;
    skos:inScheme cs: ;
    skos:prefLabel "Marine Peak"@en ;
    schema:citation "https://iho.int/en/basic-documents-1"^^xsd:anyURI ;
.

cs:marine-pinnacle
    a skos:Concept ;
    rdfs:isDefinedBy cs: ;
    skos:definition "A spire-shaped pillar either isolated or at the summit of a larger feature."@en ;
    skos:historyNote "Definition from General Bathymetric Chart of the Oceans (GEBCO) Sub-Committee on Undersea Features Names (SCUFN)." ;
    skos:inScheme cs: ;
    skos:prefLabel "Marine Pinnacle"@en ;
    schema:citation "https://iho.int/en/basic-documents-1"^^xsd:anyURI ;
.

cs:marine-province
    a skos:Concept ;
    rdfs:isDefinedBy cs: ;
    skos:definition "A geographically distinct region with a number of shared physiographic characteristics that contrast with those in the surrounding areas."@en ;
    skos:historyNote "Definition from General Bathymetric Chart of the Oceans (GEBCO) Sub-Committee on Undersea Features Names (SCUFN)." ;
    skos:inScheme cs: ;
    skos:prefLabel "Marine Province"@en ;
    schema:citation "https://iho.int/en/basic-documents-1"^^xsd:anyURI ;
.

cs:marine-reef
    a skos:Concept ;
    rdfs:isDefinedBy cs: ;
    skos:definition "A shallow ELEVATION composed of consolidated material that may constitute a hazard to surface navigation."@en ;
    skos:historyNote "Definition from General Bathymetric Chart of the Oceans (GEBCO) Sub-Committee on Undersea Features Names (SCUFN)." ;
    skos:inScheme cs: ;
    skos:narrower cs:coral-reef ;
    skos:prefLabel "Marine Reef"@en ;
    schema:citation "https://iho.int/en/basic-documents-1"^^xsd:anyURI ;
.

cs:marine-ridge
    a skos:Concept ;
    rdfs:isDefinedBy cs: ;
    skos:altLabel "Undersea ridge"@en ;
    skos:definition "An elongated ELEVATION of varying complexity, size and gradient."@en ;
    skos:historyNote "Definition from General Bathymetric Chart of the Oceans (GEBCO) Sub-Committee on Undersea Features Names (SCUFN). Undersea ridge from https://data.aad.gov.au/aadc/ftc/display_feature_type.cfm?feature_type_code=432" ;
    skos:inScheme cs: ;
    skos:narrower cs:mid-ocean-ridge ;
    skos:prefLabel "Marine Ridge"@en ;
    schema:citation "https://iho.int/en/basic-documents-1"^^xsd:anyURI ;
.

cs:marine-rift
    a skos:Concept ;
    rdfs:isDefinedBy cs: ;
    skos:definition "An elongated depression bounded by two or more faults formed as a breach or split between two bodies that were once joined."@en ;
    skos:historyNote "Definition from General Bathymetric Chart of the Oceans (GEBCO) Sub-Committee on Undersea Features Names (SCUFN)." ;
    skos:inScheme cs: ;
    skos:prefLabel "Marine Rift"@en ;
    schema:citation "https://iho.int/en/basic-documents-1"^^xsd:anyURI ;
.

cs:marine-rise
    a skos:Concept ;
    rdfs:isDefinedBy cs: ;
    skos:definition "A broad ELEVATION that generally rises gently and smoothly from the surrounding relief."@en ;
    skos:historyNote "Definition from General Bathymetric Chart of the Oceans (GEBCO) Sub-Committee on Undersea Features Names (SCUFN)." ;
    skos:inScheme cs: ;
    skos:prefLabel "Marine Rise"@en ;
    schema:citation "https://iho.int/en/basic-documents-1"^^xsd:anyURI ;
.

cs:marine-saddle
    a skos:Concept ;
    rdfs:isDefinedBy cs: ;
    skos:altLabel "Pass"@en ;
    skos:definition "A broad pass or col in a RIDGE, RISE or other ELEVATION."@en ;
    skos:historyNote "Definition from General Bathymetric Chart of the Oceans (GEBCO) Sub-Committee on Undersea Features Names (SCUFN)." ;
    skos:inScheme cs: ;
    skos:prefLabel "Marine Saddle"@en ;
    schema:citation "https://iho.int/en/basic-documents-1"^^xsd:anyURI ;
.

cs:marine-salt-dome
    a skos:Concept ;
    rdfs:isDefinedBy cs: ;
    skos:definition "A distinct ELEVATION, often with a rounded profile, one km or more in diameter that is the geomorphologic expression of a diapir formed by vertical intrusion of salt. Commonly found in a PROVINCE of similar features."@en ;
    skos:historyNote "Definition from General Bathymetric Chart of the Oceans (GEBCO) Sub-Committee on Undersea Features Names (SCUFN)." ;
    skos:inScheme cs: ;
    skos:prefLabel "Marine Salt Dome"@en ;
    schema:citation "https://iho.int/en/basic-documents-1"^^xsd:anyURI ;
.

cs:marine-sand-ridge
    a skos:Concept ;
    rdfs:isDefinedBy cs: ;
    skos:definition "An elongated feature of unconsolidated sediment of limited vertical relief and sometimes crescent shaped. Commonly found in a PROVINCE of similar features."@en ;
    skos:historyNote "Definition from General Bathymetric Chart of the Oceans (GEBCO) Sub-Committee on Undersea Features Names (SCUFN)." ;
    skos:inScheme cs: ;
    skos:prefLabel "Marine Sand Ridge"@en ;
    schema:citation "https://iho.int/en/basic-documents-1"^^xsd:anyURI ;
.

cs:marine-shelf
    a skos:Concept ;
    rdfs:isDefinedBy cs: ;
    skos:altLabel
        "Borderland"@en ,
        "Continental Shelf"@en ,
        "Shelf Break"@en ,
        "Shelf Edge"@en ;
    skos:definition "The flat or gently sloping region adjacent to a continent or around an island that extends from the low water line to a depth, generally about 200m, where there is a marked increase in downward slope."@en ;
    skos:historyNote "Definition from General Bathymetric Chart of the Oceans (GEBCO) Sub-Committee on Undersea Features Names (SCUFN)." ;
    skos:inScheme cs: ;
    skos:prefLabel "Marine Shelf"@en ;
    schema:citation "https://iho.int/en/basic-documents-1"^^xsd:anyURI ;
.

cs:marine-shoal
    a skos:Concept ;
    rdfs:isDefinedBy cs: ;
    skos:altLabel
        "Patches"@en ,
        "Shallows"@en ;
    skos:definition "A shallow ELEVATION composed of unconsolidated material that may constitute a hazard to surface navigation."@en ;
    skos:historyNote "Definition from General Bathymetric Chart of the Oceans (GEBCO) Sub-Committee on Undersea Features Names (SCUFN)." ;
    skos:inScheme cs: ;
    skos:prefLabel "Marine Shoal"@en ;
    schema:citation "https://iho.int/en/basic-documents-1"^^xsd:anyURI ;
.

cs:marine-sill
    a skos:Concept ;
    rdfs:isDefinedBy cs: ;
    skos:definition "A relatively shallow barrier between BASINS that may inhibit water movement."@en ;
    skos:historyNote "Definition from General Bathymetric Chart of the Oceans (GEBCO) Sub-Committee on Undersea Features Names (SCUFN)." ;
    skos:inScheme cs: ;
    skos:prefLabel "Marine Sill"@en ;
    schema:citation "https://iho.int/en/basic-documents-1"^^xsd:anyURI ;
.

cs:marine-spur
    a skos:Concept ;
    rdfs:isDefinedBy cs: ;
    skos:altLabel "Promontory"@en ;
    skos:definition "A subordinate RIDGE protruding from a larger feature."@en ;
    skos:historyNote "Definition from General Bathymetric Chart of the Oceans (GEBCO) Sub-Committee on Undersea Features Names (SCUFN)." ;
    skos:inScheme cs: ;
    skos:prefLabel "Marine Spur"@en ;
    schema:citation "https://iho.int/en/basic-documents-1"^^xsd:anyURI ;
.

cs:marine-terrace
    a skos:Concept ;
    rdfs:isDefinedBy cs: ;
    skos:definition "A flat or gently sloping region, generally long and narrow, bounded along one edge by a steeper descending slope and along the other by a steeper ascending slope."@en ;
    skos:historyNote "Definition from General Bathymetric Chart of the Oceans (GEBCO) Sub-Committee on Undersea Features Names (SCUFN)." ;
    skos:inScheme cs: ;
    skos:prefLabel "Marine Terrace"@en ;
    schema:citation "https://iho.int/en/basic-documents-1"^^xsd:anyURI ;
.

cs:marine-trough
    a skos:Concept ;
    rdfs:isDefinedBy cs: ;
    skos:definition "A long depression, generally wide and flat bottomed with symmetrical and parallel sides"@en ;
    skos:historyNote "Definition from General Bathymetric Chart of the Oceans (GEBCO) Sub-Committee on Undersea Features Names (SCUFN)." ;
    skos:inScheme cs: ;
    skos:narrower cs:deep ;
    skos:prefLabel "Marine Trough"@en ;
    schema:citation "https://iho.int/en/basic-documents-1"^^xsd:anyURI ;
.

cs:market
    a skos:Concept ;
    rdfs:isDefinedBy cs: ;
    skos:definition "An open space or covered building(s) in which provisions are exposed for sale"@en ;
    skos:historyNote "PSMA" ;
    skos:inScheme cs: ;
    skos:prefLabel "Market"@en ;
.

cs:maternal-and-child-health-centre
    a skos:Concept ;
    rdfs:isDefinedBy cs: ;
    skos:altLabel
        "MACH"@en ,
        "MCH"@en ,
        "Maternal Child Health"@en ,
        "Maternal and Child Health"@en ;
    skos:definition "A health facility that caters for the maternal and child health needs of a community"@en ;
    skos:historyNote "PSMA; Agreed at ICSM PNWG Meeting 2022" ;
    skos:inScheme cs: ;
    skos:prefLabel "Maternal and Child Health Centre"@en ;
.

cs:medical-centre
    a skos:Concept ;
    rdfs:isDefinedBy cs: ;
    skos:altLabel "Doctors surgery"@en ;
    skos:definition "A doctors surgery"@en ;
    skos:historyNote "PSMA" ;
    skos:inScheme cs: ;
    skos:prefLabel "Medical Centre"@en ;
.

cs:memorial
    a skos:Concept ;
    rdfs:isDefinedBy cs: ;
    skos:definition "To be defined."@en ;
    skos:inScheme cs: ;
    skos:prefLabel "Memorial"@en ;
.

cs:meteorite-crater
    a skos:Concept ;
    rdfs:isDefinedBy cs: ;
    skos:altLabel "Impact Crater"@en ;
    skos:definition "A hollow caused by the fall of a meteorite on to the Earth's surface"@en ;
    skos:inScheme cs: ;
    skos:prefLabel "Meteorite Crater"@en ;
.

cs:mid-ocean-ridge
    a skos:Concept ;
    rdfs:isDefinedBy cs: ;
    skos:definition "To be defined."@en ;
    skos:inScheme cs: ;
    skos:prefLabel "Mid-Ocean Ridge"@en ;
    schema:citation "https://iho.int/en/basic-documents-1"^^xsd:anyURI ;
.

cs:mine
    a skos:Concept ;
    rdfs:isDefinedBy cs: ;
    skos:definition "Places related to the extraction of mined materials."@en ;
    skos:historyNote "Added by QLD 2024-03-05" ;
    skos:inScheme cs: ;
    skos:narrower
        cs:abandoned-mine ,
        cs:open-cut-mine ,
        cs:underground-mine ;
    skos:prefLabel "Mine"@en ;
.

cs:mineral-field
    a skos:Concept ;
    rdfs:isDefinedBy cs: ;
    skos:definition "An area in which mineral resources have been identified."@en ;
    skos:inScheme cs: ;
    skos:narrower
        cs:coal-field ,
        cs:gold-field ,
        cs:oil-gas-field ,
        cs:opal-field ;
    skos:prefLabel "Mineral Field"@en ;
.

cs:mineral-sand-processing-plant
    a skos:Concept ;
    rdfs:isDefinedBy cs: ;
    skos:definition "A refinery for extracting rare metals."@en ;
    skos:historyNote "PSMA" ;
    skos:inScheme cs: ;
    skos:prefLabel "Mineral Sand Processing Plant"@en ;
.

cs:mining-feature
    a skos:Concept ;
    rdfs:isDefinedBy cs: ;
    skos:definition "Place pertaining to the adminstration extraction and processing of minerals, rock, gas and oil."@en ;
    skos:inScheme cs: ;
    skos:narrower
        cs:mineral-field ,
        cs:mining-centre ,
        cs:resource-extraction-feature ,
        cs:resource-processing-facility ;
    skos:prefLabel "Mining Feature"@en ;
    skos:topConceptOf cs: ;
.

cs:mission
    a skos:Concept ;
    rdfs:isDefinedBy cs: ;
    skos:definition "An establishment administered by a religious community for the spiritual and social welfare of others."@en ;
    skos:historyNote "GNR" ;
    skos:inScheme cs: ;
    skos:prefLabel "Mission"@en ;
.

cs:mondir
    a skos:Concept ;
    rdfs:isDefinedBy cs: ;
    skos:definition "Hindu place of worship."@en ;
    skos:historyNote "GNR" ;
    skos:inScheme cs: ;
    skos:prefLabel "Mondir"@en ;
.

cs:monument
    a skos:Concept ;
    rdfs:isDefinedBy cs: ;
    skos:definition "Anything by which the memory of persons or things are preserved; anything that serves as a memorial to a person, event, or of past times."@en ;
    skos:historyNote "Agreed at ICSM PNWG Meeting 2022" ;
    skos:inScheme cs: ;
    skos:narrower
        cs:cairn ,
        cs:commemorative-tree ,
        cs:fountain ,
        cs:memorial ,
        cs:obelisk ,
        cs:shrine ;
    skos:prefLabel "Monument"@en ;
.

cs:moraine
    a skos:Concept ;
    rdfs:isDefinedBy cs: ;
    skos:definition "A mound, ridge, or other distinct accumulation of unsorted, unstratified glacial drift, predominantly till, deposited primarily by direct action of glacier ice, in a variety of topographic landforms that are independent of control by the surface on which the drift lies."@en ;
    skos:historyNote "Concept and definition from the Australian Antarctic Division." ;
    skos:inScheme cs: ;
    skos:prefLabel "Moraine"@en ;
    schema:citation "https://data.aad.gov.au/aadc/ftc/display_feature_type.cfm?feature_type_code=245"^^xsd:anyURI ;
.

cs:mosque
    a skos:Concept ;
    rdfs:isDefinedBy cs: ;
    skos:definition "Muslim place of worship."@en ;
    skos:historyNote "PSMA" ;
    skos:inScheme cs: ;
    skos:prefLabel "Mosque"@en ;
.

cs:motor-track
    a skos:Concept ;
    rdfs:isDefinedBy cs: ;
    skos:altLabel "Auto track"@en ;
    skos:definition "A circuit or course used for racing vehicles"@en ;
    skos:historyNote "PSMA" ;
    skos:inScheme cs: ;
    skos:prefLabel "Motor Track"@en ;
.

cs:mountain
    a skos:Concept ;
    rdfs:isDefinedBy cs: ;
    skos:definition "A natural elevation of the Earth's surface rising more or less abruptly from the surrounding level, and attaining an altitude which, relative to adjacent elevations, is impressive or notable. In general the elevation of a mountain is more than 300m from foot to summit, but this distinction is arbitrary"@en ;
    skos:historyNote "PSMA" ;
    skos:inScheme cs: ;
    skos:narrower
        cs:seamount ,
        cs:subglacial-mount ;
    skos:prefLabel "Mountain"@en ;
.

cs:mountain-bike-track
    a skos:Concept ;
    rdfs:isDefinedBy cs: ;
    skos:altLabel "mountain bike trail"@en ;
    skos:definition "A trail designed for mountain bike traffic in the main."@en ;
    skos:historyNote "Agreed at ICSM PNWG Meeting 2022" ;
    skos:inScheme cs: ;
    skos:prefLabel "Mountain Bike Track"@en ;
.

cs:multiuse-trail
    a skos:Concept ;
    rdfs:isDefinedBy cs: ;
    skos:altLabel
        "multi use trail"@en ,
        "rail trail"@en ,
        "shared use trail"@en ;
    skos:definition "A pathway designed for shared use access, being walking and bicycle traffic and may also include horse riding or skiing or may be any combination of multiple use. Main uses cycling and walking."@en ;
    skos:historyNote "Agreed at ICSM PNWG Meeting 2022" ;
    skos:inScheme cs: ;
    skos:prefLabel "Multiuse Trail"@en ;
.

cs:museum
    a skos:Concept ;
    rdfs:isDefinedBy cs: ;
    skos:altLabel "Museum Precinct"@en ;
    skos:definition "An institution that cares for (conserves) a collection of artefacts and other objects of scientific, artistic, cultural, or historical importance and makes them available for public viewing"@en ;
    skos:historyNote "PSMA" ;
    skos:inScheme cs: ;
    skos:prefLabel "Museum"@en ;
.

cs:national-park
    a skos:Concept ;
    rdfs:isDefinedBy cs: ;
    skos:altLabel
        "Wilderness Area"@en ,
        "Wilderness Park"@en ;
    skos:definition "An area of land, set apart, as by a state or nation, to be preserved in its natural state for the benefit of the public."@en ;
    skos:historyNote "GNR" ;
    skos:inScheme cs: ;
    skos:prefLabel "National Park"@en ;
.

cs:naval-base
    a skos:Concept ;
    rdfs:isDefinedBy cs: ;
    skos:definition "A facility used by the navy for the operation and/or training of personnel and their vessels"@en ;
    skos:historyNote "Agreed at ICSM PNWG Meeting 2022" ;
    skos:inScheme cs: ;
    skos:prefLabel "Naval Base"@en ;
.

cs:neighbourhood
    a skos:Concept ;
    rdfs:isDefinedBy cs: ;
    skos:altLabel "Unbounded Locality"@en ;
    skos:definition "Does not have officially recognised and registered boundaries hence an unbounded locality. For this reason a neighbourhood name cannot be used for addressing purposes"@en ;
    skos:historyNote "PSMA" ;
    skos:inScheme cs: ;
    skos:prefLabel "Neighbourhood"@en ;
.

cs:neighbourhood-safer-place
    a skos:Concept ;
    rdfs:isDefinedBy cs: ;
    skos:altLabel
        "BPLR"@en ,
        "NSP"@en ,
        "bushfire place of last resort"@en ;
    skos:definition "An area or premises that may as a last resort provide some sanctuary from the life threatening effects of a bushfire. I.e. direct flame contact or radiant heat."@en ;
    skos:historyNote "PSMA; Agreed at ICSM PNWG Meeting 2022" ;
    skos:inScheme cs: ;
    skos:prefLabel "Neighbourhood Safer Place"@en ;
.

cs:netball-court
    a skos:Concept ;
    rdfs:isDefinedBy cs: ;
    skos:definition "A place where netball is played."@en ;
    skos:historyNote "PSMA" ;
    skos:inScheme cs: ;
    skos:prefLabel "Netball Court"@en ;
.

cs:neve
    a skos:Concept ;
    rdfs:isDefinedBy cs: ;
    skos:definition "The crystalline or granular snow on the upper part of a glacier, which has not yet been compressed into ice; a field or bed of frozen snow."@en ;
    skos:historyNote "Concept and definition from the Australian Antarctic Division." ;
    skos:inScheme cs: ;
    skos:prefLabel "Neve"@en ;
    schema:citation "https://data.aad.gov.au/aadc/ftc/display_feature_type.cfm?feature_type_code=396"^^xsd:anyURI ;
.

cs:nickel-refinery
    a skos:Concept ;
    rdfs:isDefinedBy cs: ;
    skos:definition "A refinery for extracting nickel."@en ;
    skos:historyNote "PSMA" ;
    skos:inScheme cs: ;
    skos:prefLabel "Nickel Refinery"@en ;
.

cs:nunatak
    a skos:Concept ;
    rdfs:isDefinedBy cs: ;
    skos:definition "A small mountain, rocky crag or outcrop projecting from a glacier, ice shelf or snowfield."@en ;
    skos:historyNote "Concept and definition from the Australian Antarctic Division." ;
    skos:inScheme cs: ;
    skos:prefLabel "Nunatak"@en ;
    schema:citation "https://data.aad.gov.au/aadc/ftc/display_feature_type.cfm?feature_type_code=397"^^xsd:anyURI ;
.

cs:obelisk
    a skos:Concept ;
    rdfs:isDefinedBy cs: ;
    skos:definition "To be defined."@en ;
    skos:inScheme cs: ;
    skos:prefLabel "Obelisk"@en ;
.

cs:observatory
    a skos:Concept ;
    rdfs:isDefinedBy cs: ;
    skos:definition "An institution or building specially designed and equipped for observing meteorological and astronomical phenomena."@en ;
    skos:inScheme cs: ;
    skos:narrower cs:weather-station ;
    skos:prefLabel "Observatory"@en ;
.

cs:ocean
    a skos:Concept ;
    rdfs:isDefinedBy cs: ;
    skos:definition "Any of the geographical divisions of the vast body of salt water which covers almost three quarters of the earth’s surface."@en ;
    skos:historyNote "Macquarie Dictionary" ;
    skos:inScheme cs: ;
    skos:narrower cs:sea ;
    skos:prefLabel "Ocean"@en ;
.

cs:oil-field
    a skos:Concept ;
    rdfs:isDefinedBy cs: ;
    skos:definition "An area in which oil resources have been identified."@en ;
    skos:inScheme cs: ;
    skos:prefLabel "Oil Field"@en ;
.

cs:oil-gas-field
    a skos:Concept ;
    rdfs:isDefinedBy cs: ;
    skos:definition "An area in which oil and gas resources have been identified."@en ;
    skos:historyNote "GNR; Agreed at ICSM PNWG Meeting 2022" ;
    skos:inScheme cs: ;
    skos:narrower
        cs:gas-field ,
        cs:oil-field ;
    skos:prefLabel "Oil and Gas Field"@en ;
.

cs:oil-gas-platform
    a skos:Concept ;
    rdfs:isDefinedBy cs: ;
    skos:altLabel
        "drilling rig"@en ,
        "offshore platform"@en ;
    skos:definition "A large structure with facilities to drill wells, to extract and process oil and natural gas."@en ;
    skos:historyNote "PSMA; Agreed at ICSM PNWG Meeting 2022" ;
    skos:inScheme cs: ;
    skos:narrower
        cs:gas-platform ,
        cs:oil-platform ;
    skos:prefLabel "Oil and Gas Platform"@en ;
.

cs:oil-gas-well
    a skos:Concept ;
    rdfs:isDefinedBy cs: ;
    skos:definition "A hole drilled into the ground to extract oil or gas."@en ;
    skos:historyNote "Agreed at ICSM PNWG Meeting 2022" ;
    skos:inScheme cs: ;
    skos:narrower
        cs:gas-well ,
        cs:oil-well ;
    skos:prefLabel "Oil and Gas Well"@en ;
.

cs:oil-pipeline
    a skos:Concept ;
    rdfs:isDefinedBy cs: ;
    skos:definition "A long pipe, typically underground, used to transport oil over long distances"@en ;
    skos:historyNote "new" ;
    skos:inScheme cs: ;
    skos:prefLabel "Oil Pipeline"@en ;
.

cs:oil-platform
    a skos:Concept ;
    rdfs:isDefinedBy cs: ;
    skos:altLabel "oil rig"@en ;
    skos:definition "A large structure with facilities to drill wells, to extract and process oil."@en ;
    skos:inScheme cs: ;
    skos:prefLabel "Oil Platform"@en ;
.

cs:oil-refinery
    a skos:Concept ;
    rdfs:isDefinedBy cs: ;
    skos:definition "An industrial processing plant where crude oil is refined to produce petroleum product."@en ;
    skos:historyNote "PSMA" ;
    skos:inScheme cs: ;
    skos:prefLabel "Oil Refinery"@en ;
.

cs:oil-well
    a skos:Concept ;
    rdfs:isDefinedBy cs: ;
    skos:definition "A hole drilled into the ground to extract oil."@en ;
    skos:inScheme cs: ;
    skos:prefLabel "Oil Well"@en ;
.

cs:opal-field
    a skos:Concept ;
    rdfs:isDefinedBy cs: ;
    skos:definition "An area in which opals have been found and where mines have been established."@en ;
    skos:historyNote "GNR" ;
    skos:inScheme cs: ;
    skos:prefLabel "Opal Field"@en ;
.

cs:open-cut-mine
    a skos:Concept ;
    rdfs:isDefinedBy cs: ;
    skos:altLabel
        "open pit mine"@en ,
        "open surface mine"@en ,
        "strip mine"@en ;
    skos:definition "A place or area from which commercial minerals are removed from the Earth"@en ;
    skos:historyNote "PSMA; Agreed at ICSM PNWG Meeting 2022" ;
    skos:inScheme cs: ;
    skos:prefLabel "Open Cut Mine"@en ;
.

cs:outcamp
    a skos:Concept ;
    rdfs:isDefinedBy cs: ;
    skos:altLabel
        "Aboriginal Location"@en ,
        "Homelands"@en ;
    skos:definition "Small Aboriginal community outside of the main community."@en ;
    skos:inScheme cs: ;
    skos:prefLabel "Outcamp"@en ;
.

cs:outstation
    a skos:Concept ;
    rdfs:isDefinedBy cs: ;
    skos:altLabel "Aboriginal outstation"@en ;
    skos:definition "Accomodation outside of the main homestead complex within a pastoral property."@en ;
    skos:historyNote "GNR" ;
    skos:inScheme cs: ;
    skos:prefLabel "Outstation"@en ;
.

cs:paddock
    a skos:Concept ;
    rdfs:isDefinedBy cs: ;
    skos:altLabel "Field"@en ;
    skos:definition "A specific area, typically within a farm or pastoral property."@en ;
    skos:inScheme cs: ;
    skos:prefLabel "Paddock"@en ;
.

cs:pan
    a skos:Concept ;
    rdfs:isDefinedBy cs: ;
    skos:definition "A small depression, intermittently containing water, which may sometimes hold deposits, typically clay or salt."@en ;
    skos:inScheme cs: ;
    skos:narrower
        cs:clay-pan ,
        cs:salt-pan ;
    skos:prefLabel "Pan"@en ;
.

cs:parish
    a skos:Concept ;
    rdfs:isDefinedBy cs: ;
    skos:altLabel "Hundred"@en ;
    skos:definition "A subdivision of the COUNTIES into land units"@en ;
    skos:historyNote "Agreed at ICSM PNWG Meeting 2022" ;
    skos:inScheme cs: ;
    skos:prefLabel "Parish"@en ;
.

cs:park
    a skos:Concept ;
    rdfs:isDefinedBy cs: ;
    skos:altLabel
        "City Square"@en ,
        "Common"@en ,
        "Forecourt"@en ,
        "Local Park"@en ,
        "Rec Reserve"@en ;
    skos:definition "An area of land often with recreational and other facilities which is set aside for public use"@en ;
    skos:historyNote "NEW" ;
    skos:inScheme cs: ;
    skos:prefLabel "Park"@en ;
.

cs:pass
    a skos:Concept ;
    rdfs:isDefinedBy cs: ;
    skos:altLabel
        "col"@en ,
        "gap"@en ,
        "saddle"@en ;
    skos:definition "A break or GAP in a MOUNTAIN RANGE permitting easier passage from one side to the other"@en ;
    skos:historyNote "PSMA" ;
    skos:inScheme cs: ;
    skos:narrower cs:marine-gap ;
    skos:prefLabel "Pass"@en ;
.

cs:pastoral-district
    a skos:Concept ;
    rdfs:isDefinedBy cs: ;
    skos:definition "A classification of land to assist in the administration of pastoral runs."@en ;
    skos:inScheme cs: ;
    skos:prefLabel "Pastoral District"@en ;
.

cs:peak
    a skos:Concept ;
    rdfs:isDefinedBy cs: ;
    skos:altLabel
        "aiguille"@en ,
        "height"@en ,
        "needle"@en ,
        "pillar"@en ,
        "pinnacle"@en ,
        "rock column"@en ,
        "summit"@en ;
    skos:definition "A high point of a mountain or a ridge"@en ;
    skos:historyNote "GNR" ;
    skos:inScheme cs: ;
    skos:prefLabel "Peak"@en ;
.

cs:peninsula
    a skos:Concept ;
    rdfs:isDefinedBy cs: ;
    skos:altLabel "Promontory"@en ;
    skos:definition "An area of land almost surrounded by water and significantly larger than a CAPE"@en ;
    skos:historyNote "PSMA" ;
    skos:inScheme cs: ;
    skos:prefLabel "Peninsula"@en ;
.

cs:picnic-site
    a skos:Concept ;
    rdfs:isDefinedBy cs: ;
    skos:altLabel
        "DUA"@en ,
        "Day Use Area"@en ,
        "Picnic area"@en ;
    skos:definition "A tract of land reserved for day picnic purposes, sometimes with constructed fireplaces and other facilities"@en ;
    skos:historyNote "VMFEAT" ;
    skos:inScheme cs: ;
    skos:prefLabel "Picnic Site"@en ;
.

cs:pier
    a skos:Concept ;
    rdfs:isDefinedBy cs: ;
    skos:definition "A long narrow structure extending into the water to afford a berthing place for vessels; also serves as a pleasure promenade"@en ;
    skos:inScheme cs: ;
    skos:prefLabel "Pier"@en ;
.

cs:place-of-worship
    a skos:Concept ;
    rdfs:isDefinedBy cs: ;
    skos:definition "Places used for spirtual observation or cermonial purposes."@en ;
    skos:inScheme cs: ;
    skos:narrower
        cs:abbey ,
        cs:chapel ,
        cs:church ,
        cs:gurdwara ,
        cs:mission ,
        cs:mondir ,
        cs:mosque ,
        cs:synagogue ,
        cs:vihara ;
    skos:prefLabel "Place of Worship"@en ;
.

cs:plain
    a skos:Concept ;
    rdfs:isDefinedBy cs: ;
    skos:altLabel
        "alluvial plain"@en ,
        "clearing"@en ,
        "downs"@en ,
        "flat"@en ,
        "lava plain"@en ,
        "prairie"@en ,
        "volcanic plain"@en ;
    skos:definition "A tract of country, at least 2500 hectares in extent, the general surface of which is comparatively flat and which is sparsely, if at all, timbered."@en ;
    skos:historyNote "PSMA; Agreed at ICSM PNWG Meeting 2022" ;
    skos:inScheme cs: ;
    skos:prefLabel "Plain"@en ;
.

cs:plateau
    a skos:Concept ;
    rdfs:isDefinedBy cs: ;
    skos:altLabel
        "Platform"@en ,
        "Tableland"@en ;
    skos:definition "An elevated tract of comparatively flat or level land"@en ;
    skos:historyNote "PSMA" ;
    skos:inScheme cs: ;
    skos:narrower cs:marine-plateau ;
    skos:prefLabel "Plateau"@en ;
.

cs:playground
    a skos:Concept ;
    rdfs:isDefinedBy cs: ;
    skos:definition "An outdoor area for children's play."@en ;
    skos:historyNote "PSMA" ;
    skos:inScheme cs: ;
    skos:prefLabel "Playground"@en ;
.

cs:pocket
    a skos:Concept ;
    rdfs:isDefinedBy cs: ;
    skos:definition "An area of land encompassed by the meander of a river."@en ;
    skos:historyNote "QLD" ;
    skos:inScheme cs: ;
    skos:prefLabel "Pocket"@en ;
.

cs:point
    a skos:Concept ;
    rdfs:isDefinedBy cs: ;
    skos:definition "A small protrusion of land into the sea or a lake, often the outer end of a larger landform such as a CAPE"@en ;
    skos:historyNote "GNR" ;
    skos:inScheme cs: ;
    skos:prefLabel "Point"@en ;
.

cs:police-station
    a skos:Concept ;
    rdfs:isDefinedBy cs: ;
    skos:definition "An office of the local police force; it may or may not have an associated lock-up"@en ;
    skos:historyNote "PSMA; Agreed at ICSM PNWG Meeting 2022" ;
    skos:inScheme cs: ;
    skos:prefLabel "Police Station"@en ;
.

cs:populated-place
    a skos:Concept ;
    rdfs:isDefinedBy cs: ;
    skos:definition "Places relating to population entities, both current and historical"@en ;
    skos:inScheme cs: ;
    skos:narrower
        cs:neighbourhood ,
        cs:outcamp ,
        cs:population-centre ,
        cs:settlement ;
    skos:prefLabel "Populated Place"@en ;
    skos:topConceptOf cs: ;
.

cs:population-centre
    a skos:Concept ;
    rdfs:isDefinedBy cs: ;
    skos:altLabel
        "City"@en ,
        "Town"@en ,
        "Township"@en ,
        "Village"@en ;
    skos:definition "A significant place where there is permanent human habitation, infrastructure and services."@en ;
    skos:inScheme cs: ;
    skos:prefLabel "Population Centre"@en ;
.

cs:port
    a skos:Concept ;
    rdfs:isDefinedBy cs: ;
    skos:definition "A place provided with terminal and transfer facilities for loading and discharging cargo or passengers, usually located in a HARBOUR"@en ;
    skos:inScheme cs: ;
    skos:prefLabel "Port"@en ;
.

cs:post-office
    a skos:Concept ;
    rdfs:isDefinedBy cs: ;
    skos:definition "A local office for receiving, distributing and transmitting mail, providing telecommunication services."@en ;
    skos:historyNote "PSMA" ;
    skos:inScheme cs: ;
    skos:prefLabel "Post Office"@en ;
.

cs:power-distribution
    a skos:Concept ;
    rdfs:isDefinedBy cs: ;
    skos:definition "A wire used for the distribution of electricity"@en ;
    skos:historyNote "PSMA" ;
    skos:inScheme cs: ;
    skos:prefLabel "Power Distribution"@en ;
.

cs:power-station
    a skos:Concept ;
    rdfs:isDefinedBy cs: ;
    skos:definition "A process plant that creates power from one or more sources."@en ;
    skos:historyNote "Agreed at ICSM PNWG Meeting 2022" ;
    skos:inScheme cs: ;
    skos:narrower
        cs:biomass-power-station ,
        cs:coal-power-station ,
        cs:gas-power-station ,
        cs:geothermal-power-station ,
        cs:hydroelectric-power-station ,
        cs:solar-power-station ,
        cs:wind-farm ;
    skos:prefLabel "Power Station"@en ;
.

cs:power-sub-station
    a skos:Concept ;
    rdfs:isDefinedBy cs: ;
    skos:altLabel
        "Power Sub Station"@en ,
        "Power Terminal Station"@en ,
        "Zone Substation"@en ;
    skos:definition "A facility whose primary purpose is to convert incoming sub-transmission voltages to high voltage distribution voltages -usually owned by the distribution company"@en ;
    skos:historyNote "PSMA; Agreed at ICSM PNWG Meeting 2022" ;
    skos:inScheme cs: ;
    skos:prefLabel "Power Sub Station"@en ;
.

cs:power-sub-transmission
    a skos:Concept ;
    rdfs:isDefinedBy cs: ;
    skos:altLabel "Power Subtransmission"@en ;
    skos:definition "A wire used for the transmission of electricity usually < 66KV"@en ;
    skos:historyNote "PSMA; Agreed at ICSM PNWG Meeting 2022" ;
    skos:inScheme cs: ;
    skos:prefLabel "Power Sub Transmission"@en ;
.

cs:power-terminal-station
    a skos:Concept ;
    rdfs:isDefinedBy cs: ;
    skos:altLabel "power terminal"@en ;
    skos:definition "A facility whose primary purpose is to convert incoming transmission voltages to voltages suitable for distribution networks-usually owned by the transmission company"@en ;
    skos:historyNote "PSMA" ;
    skos:inScheme cs: ;
    skos:prefLabel "Power Terminal Station"@en ;
.

cs:power-transmission
    a skos:Concept ;
    rdfs:isDefinedBy cs: ;
    skos:definition "A wire used for the transmission of electricity usually > 66KV"@en ;
    skos:historyNote "PSMA" ;
    skos:inScheme cs: ;
    skos:prefLabel "Power Transmission"@en ;
.

cs:primary-school
    a skos:Concept ;
    rdfs:isDefinedBy cs: ;
    skos:definition "An education facility that caters for 5- 12 year olds, private and public"@en ;
    skos:historyNote "PSMA" ;
    skos:inScheme cs: ;
    skos:prefLabel "Primary School"@en ;
.

cs:primary-secondary-school
    a skos:Concept ;
    rdfs:isDefinedBy cs: ;
    skos:altLabel "Combined school"@en ;
    skos:definition "A combined primary and secondary school."@en ;
    skos:historyNote "PSMA; Agreed at ICSM PNWG Meeting 2022" ;
    skos:inScheme cs: ;
    skos:prefLabel "Primary and Secondary School"@en ;
.

cs:prison
    a skos:Concept ;
    rdfs:isDefinedBy cs: ;
    skos:altLabel
        "detention centre"@en ,
        "gaol"@en ,
        "jail"@en ,
        "rehabilitation centre"@en ,
        "remand centre"@en ;
    skos:definition "A building where persons are legally committed for punishment or while awaiting trial"@en ;
    skos:historyNote "PSMA; Agreed at ICSM PNWG Meeting 2022" ;
    skos:inScheme cs: ;
    skos:prefLabel "Prison"@en ;
.

cs:protected-area
    a skos:Concept ;
    rdfs:isDefinedBy cs: ;
    skos:definition "An area of land and/or sea especially dedicated to the protection and maintenance of biological diversity and/or of natural and associated cultural resources. The area is managed through legal or other effective means."@en ;
    skos:historyNote "Definition from the Australian Antarctic Division." ;
    skos:inScheme cs: ;
    skos:narrower
        cs:antarctic-specially-managed-areas ,
        cs:antarctic-specially-protected-areas ,
        cs:coastal-reserve ,
        cs:conservation-park ,
        cs:indigenous-protected-area ,
        cs:marine-park ,
        cs:national-park ,
        cs:state-forest ;
    skos:prefLabel "Protected Area"@en ;
    schema:citation "https://data.aad.gov.au/aadc/ftc/display_feature_type.cfm?feature_type_code=267"^^xsd:anyURI ;
.

cs:pumping-station
    a skos:Concept ;
    rdfs:isDefinedBy cs: ;
    skos:definition "A pumping station to support water flows"@en ;
    skos:historyNote "PSMA" ;
    skos:inScheme cs: ;
    skos:prefLabel "Pumping Station"@en ;
.

cs:quarry
    a skos:Concept ;
    rdfs:isDefinedBy cs: ;
    skos:altLabel
        "Clay pit"@en ,
        "pit"@en ;
    skos:definition "An open surface excavation used for the extraction of stone."@en ;
    skos:historyNote "PSMA" ;
    skos:inScheme cs: ;
    skos:narrower cs:abandoned-quarry ;
    skos:prefLabel "Quarry"@en ;
.

cs:racecourse
    a skos:Concept ;
    rdfs:isDefinedBy cs: ;
    skos:altLabel "Horse Racetrack"@en ;
    skos:definition "A piece of ground on which horse races are held for public entertainment; any place where horse races are held."@en ;
    skos:historyNote "PSMA" ;
    skos:inScheme cs: ;
    skos:prefLabel "Racecourse"@en ;
.

cs:racetrack
    a skos:Concept ;
    rdfs:isDefinedBy cs: ;
    skos:definition "A typically oval course or track on which races are held."@en ;
    skos:historyNote "Added by QLD 2024-03-05. Definition form the Oxford English Dictionary." ;
    skos:inScheme cs: ;
    skos:narrower
        cs:greyhound-racetrack ,
        cs:harness-racetrack ,
        cs:motor-track ,
        cs:racecourse ;
    skos:prefLabel "Racetrack"@en ;
.

cs:radio-communication-facility
    a skos:Concept ;
    rdfs:isDefinedBy cs: ;
    skos:altLabel "Radio broadcasting facility"@en ;
    skos:definition "An antenna for the transmission of sound by radio waves to a widely dispersed audience through radio receivers"@en ;
    skos:historyNote "PSMA" ;
    skos:inScheme cs: ;
    skos:prefLabel "Radio Communication Facility"@en ;
.

cs:radio-station
    a skos:Concept ;
    rdfs:isDefinedBy cs: ;
    skos:definition "A facility to operate the transmission of radio broadcasts"@en ;
    skos:historyNote "PSMA" ;
    skos:inScheme cs: ;
    skos:prefLabel "Radio Station"@en ;
.

cs:rail
    a skos:Concept ;
    rdfs:isDefinedBy cs: ;
    skos:definition "A track or set of tracks of iron or steel rails used for the passage of rail"@en ;
    skos:inScheme cs: ;
    skos:narrower cs:light-rail ;
    skos:prefLabel "Rail"@en ;
.

cs:rail-cutting
    a skos:Concept ;
    rdfs:isDefinedBy cs: ;
    skos:definition "An excavation in the Earth's surface to create a thoroughfare for a rail line"@en ;
    skos:inScheme cs: ;
    skos:prefLabel "Rail Cutting"@en ;
.

cs:rail-transport-infrastructure
    a skos:Concept ;
    rdfs:isDefinedBy cs: ;
    skos:definition "The course of a transport mode"@en ;
    skos:inScheme cs: ;
    skos:narrower
        cs:cableway ,
        cs:cableway-terminal ,
        cs:light-rail ,
        cs:light-rail-station ,
        cs:rail-bridge ,
        cs:rail-cutting ,
        cs:rail-station ,
        cs:rail-tunnel ,
        cs:rail-yard ,
        cs:railway ,
        cs:siding ;
    skos:prefLabel "Rail Transport Infrastructure"@en ;
.

cs:rail-yard
    a skos:Concept ;
    rdfs:isDefinedBy cs: ;
    skos:altLabel
        "marshalling yard"@en ,
        "railway yard"@en ;
    skos:definition "An area of railway tracks and sidings for storage and maintenance of trains"@en ;
    skos:inScheme cs: ;
    skos:prefLabel "Rail Yard"@en ;
.

cs:railway
    a skos:Concept ;
    rdfs:isDefinedBy cs: ;
    skos:definition "A track or set of tracks of iron or steel rails used for the passage of trains"@en ;
    skos:historyNote "PSMA" ;
    skos:inScheme cs: ;
    skos:prefLabel "Railway"@en ;
.

cs:range
    a skos:Concept ;
    rdfs:isDefinedBy cs: ;
    skos:altLabel
        "Hills"@en ,
        "Mountain Chain"@en ,
        "Mountain range"@en ,
        "Mountains"@en ;
    skos:definition "A series or line of MOUNTAINs or HILLs with or without PEAKs in which the crests are relatively narrow"@en ;
    skos:historyNote "GNR" ;
    skos:inScheme cs: ;
    skos:narrower cs:seamount-chain ;
    skos:prefLabel "Range"@en ;
.

cs:rapids
    a skos:Concept ;
    rdfs:isDefinedBy cs: ;
    skos:definition "Portions of a STREAM with accelerated current where it descends rapidly without a break in the slope of the bed sufficient to form a WATERFALL"@en ;
    skos:historyNote "GNR" ;
    skos:inScheme cs: ;
    skos:prefLabel "Rapids"@en ;
.

cs:reach
    a skos:Concept ;
    rdfs:isDefinedBy cs: ;
    skos:definition "A straight portion of WATERCOURSE from one BEND to another"@en ;
    skos:inScheme cs: ;
    skos:prefLabel "Reach"@en ;
.

cs:recreational-facility
    a skos:Concept ;
    rdfs:isDefinedBy cs: ;
    skos:definition "Places where the major activity is of a sporting nature."@en ;
    skos:inScheme cs: ;
    skos:narrower
        cs:athletic-field ,
        cs:baseball-field ,
        cs:basketball-court ,
        cs:bmx-track ,
        cs:boating-club ,
        cs:bowling-green ,
        cs:croquet-green ,
        cs:equestrian-centre ,
        cs:firing-range ,
        cs:golf-course ,
        cs:grandstand ,
        cs:hockey-ground ,
        cs:netball-court ,
        cs:playground ,
        cs:rowing-course ,
        cs:skate-park ,
        cs:sport-facility ,
        cs:sports-complex ,
        cs:sportsground ,
        cs:surfing-spot ,
        cs:swimming-pool ,
        cs:tennis-court ,
        cs:velodrome ;
    skos:prefLabel "Recreational Facility"@en ;
.

cs:refuge
    a skos:Concept ;
    rdfs:isDefinedBy cs: ;
    skos:altLabel
        "Community Fire Refuge"@en ,
        "Cyclone shelter."@en ;
    skos:definition "A purpose built or modified structure to provide shelter and supplies to community members in the event of an emergency"@en ;
    skos:historyNote "PSMA; Agreed at ICSM PNWG Meeting 2022" ;
    skos:inScheme cs: ;
    skos:prefLabel "Refuge"@en ;
.

cs:reservoir
    a skos:Concept ;
    rdfs:isDefinedBy cs: ;
    skos:definition "An artificial LAKE for the storage, regulation and control of water for domestic or other use"@en ;
    skos:historyNote "GNR" ;
    skos:inScheme cs: ;
    skos:prefLabel "Reservoir"@en ;
.

cs:resource-extraction-feature
    a skos:Concept ;
    rdfs:isDefinedBy cs: ;
    skos:definition "Feature related to extraction of resources."@en ;
    skos:inScheme cs: ;
    skos:narrower
        cs:adit ,
        cs:mine ,
        cs:oil-gas-platform ,
        cs:oil-gas-well ,
        cs:quarry ;
    skos:prefLabel "Resource Extraction Feature"@en ;
.

cs:resource-processing-facility
    a skos:Concept ;
    rdfs:isDefinedBy cs: ;
    skos:definition "A facility for treating or preparing mined materials."@en ;
    skos:inScheme cs: ;
    skos:narrower
        cs:alumina-refinery ,
        cs:battery ,
        cs:gold-refinery ,
        cs:iron-ore-processor ,
        cs:mineral-sand-processing-plant ,
        cs:nickel-refinery ,
        cs:oil-refinery ,
        cs:smelter ;
    skos:prefLabel "Resource Processing Facility"@en ;
.

cs:rest-area
    a skos:Concept ;
    rdfs:isDefinedBy cs: ;
    skos:definition "An area at the side of a road or highway for vehicles to stop away from traffic; possibly with toilet and/or picnic facilities"@en ;
    skos:historyNote "PSMA" ;
    skos:inScheme cs: ;
    skos:prefLabel "Rest Area"@en ;
.

cs:retirement-village
    a skos:Concept ;
    rdfs:isDefinedBy cs: ;
    skos:altLabel
        "retirement complex"@en ,
        "retirement estate"@en ;
    skos:definition "A complex containing residential premises that are intended to be occupied by retired persons."@en ;
    skos:historyNote "PSMA" ;
    skos:inScheme cs: ;
    skos:prefLabel "Retirement Village"@en ;
.

cs:ridge
    a skos:Concept ;
    rdfs:isDefinedBy cs: ;
    skos:altLabel "SPUR"@en ;
    skos:definition "A long and narrow stretch of elevated ground, either isolated or located in a RANGE"@en ;
    skos:historyNote "PSMA" ;
    skos:inScheme cs: ;
    skos:prefLabel "Ridge"@en ;
.

cs:road
    a skos:Concept ;
    rdfs:isDefinedBy cs: ;
    skos:altLabel "Busway"@en ;
    skos:definition "Defined paths for the movement of vehicles"@en ;
    skos:inScheme cs: ;
    skos:narrower cs:mall ;
    skos:prefLabel "Road"@en ;
.

cs:road-cutting
    a skos:Concept ;
    rdfs:isDefinedBy cs: ;
    skos:definition "An excavation in the Earth's surface to create a thoroughfare for a road"@en ;
    skos:historyNote "icsm" ;
    skos:inScheme cs: ;
    skos:prefLabel "Road Cutting"@en ;
.

cs:road-transport-infrastructure
    a skos:Concept ;
    rdfs:isDefinedBy cs: ;
    skos:definition "The course of a transport mode"@en ;
    skos:inScheme cs: ;
    skos:narrower
        cs:bus-depot ,
        cs:bus-route ,
        cs:bus-station ,
        cs:bus-stop ,
        cs:busway ,
        cs:car-park ,
        cs:causeway ,
        cs:ford ,
        cs:gate ,
        cs:rest-area ,
        cs:road ,
        cs:road-bridge ,
        cs:road-cutting ,
        cs:road-tunnel ,
        cs:roundabout ,
        cs:taxi-rank ,
        cs:toll ,
        cs:tourist-route ,
        cs:weighbridge ;
    skos:prefLabel "Road Transport Infrastructure"@en ;
.

cs:rock
    a skos:Concept ;
    rdfs:isDefinedBy cs: ;
    skos:altLabel
        "BOULDER"@en ,
        "Castle"@en ,
        "Monolith"@en ,
        "OUTCROP"@en ,
        "Stack"@en ;
    skos:definition "A prominent or isolated outcrop of stone"@en ;
    skos:historyNote "new" ;
    skos:inScheme cs: ;
    skos:narrower cs:offshore-rock ;
    skos:prefLabel "Rock"@en ;
.

cs:rock-wall
    a skos:Concept ;
    rdfs:isDefinedBy cs: ;
    skos:definition "A perpendicular or steep face of rock, considerable in height."@en ;
    skos:inScheme cs: ;
    skos:prefLabel "Rock Wall"@en ;
.

cs:rockhole
    a skos:Concept ;
    rdfs:isDefinedBy cs: ;
    skos:altLabel
        "Gnamma Hole"@en ,
        "Native Well"@en ,
        "runaway hole"@en ,
        "sink hole"@en ;
    skos:definition "A hole excavated in solid rock by water action."@en ;
    skos:inScheme cs: ;
    skos:prefLabel "Rockhole"@en ;
.

cs:rotunda
    a skos:Concept ;
    rdfs:isDefinedBy cs: ;
    skos:altLabel
        "band stand"@en ,
        "pavilion"@en ;
    skos:definition "A building which has a circular plan, espcially with a dome, typically found within a park or reserve."@en ;
    skos:historyNote "VMFEAT" ;
    skos:inScheme cs: ;
    skos:prefLabel "Rotunda"@en ;
.

cs:roundabout
    a skos:Concept ;
    rdfs:isDefinedBy cs: ;
    skos:definition "A road junction at which traffic moves in one direction around a central island to reach one of the roads converging on it"@en ;
    skos:historyNote "VMTRANS" ;
    skos:inScheme cs: ;
    skos:prefLabel "Roundabout"@en ;
.

cs:rowing-course
    a skos:Concept ;
    rdfs:isDefinedBy cs: ;
    skos:definition "An area of water on which rowing is undertaken."@en ;
    skos:historyNote "PSMA" ;
    skos:inScheme cs: ;
    skos:prefLabel "Rowing Course"@en ;
.

cs:rural-fire-station
    a skos:Concept ;
    rdfs:isDefinedBy cs: ;
    skos:definition "A building in a rural area where the fire brigade, fire engines and other equipment are housed."@en ;
    skos:inScheme cs: ;
    skos:prefLabel "Rural Fire Station"@en ;
.

cs:rural-property
    a skos:Concept ;
    rdfs:isDefinedBy cs: ;
    skos:altLabel
        "Pastoral property"@en ,
        "Rural station"@en ;
    skos:definition "To be defined."@en ;
    skos:historyNote "Added by QLD 2024-03-05" ;
    skos:inScheme cs: ;
    skos:prefLabel "Rural Property"@en ;
.

cs:salt-pan
    a skos:Concept ;
    rdfs:isDefinedBy cs: ;
    skos:definition "A small depression, intermittently containing water, which holds salt deposits."@en ;
    skos:inScheme cs: ;
    skos:prefLabel "Salt Pan"@en ;
.

cs:school
    a skos:Concept ;
    rdfs:isDefinedBy cs: ;
    skos:definition "And educational facility for children."@en ;
    skos:historyNote "Added by QLD 2024-03-19" ;
    skos:inScheme cs: ;
    skos:narrower
        cs:primary-school ,
        cs:primary-secondary-school ,
        cs:secondary-school ,
        cs:special-school ;
    skos:prefLabel "School"@en ;
.

cs:school-camp
    a skos:Concept ;
    rdfs:isDefinedBy cs: ;
    skos:definition "A camping facility administered by an education centre"@en ;
    skos:historyNote "PSMA; Agreed at ICSM PNWG Meeting 2022" ;
    skos:inScheme cs: ;
    skos:prefLabel "School Camp"@en ;
.

cs:scrap-yard
    a skos:Concept ;
    rdfs:isDefinedBy cs: ;
    skos:altLabel
        "Salvage yard"@en ,
        "Wreckers"@en ,
        "Wrecking yard"@en ,
        "junkyard"@en ;
    skos:definition "A site on which anything discarded as useless, unwanted or wornout may be dumped."@en ;
    skos:historyNote "PSMA; Agreed at ICSM PNWG Meeting 2022" ;
    skos:inScheme cs: ;
    skos:prefLabel "Scrap Yard"@en ;
.

cs:scrub
    a skos:Concept ;
    rdfs:isDefinedBy cs: ;
    skos:altLabel "Heath"@en ;
    skos:definition "A tract of country, not large in extent, which is uncultivated and which bears a dense growth of low-growing bushes or shrubs."@en ;
    skos:inScheme cs: ;
    skos:prefLabel "Scrub"@en ;
.

cs:sea
    a skos:Concept ;
    rdfs:isDefinedBy cs: ;
    skos:definition "One of the smaller divisions of the OCEANS, especially if partly enclosed by land"@en ;
    skos:historyNote "VMFEAT" ;
    skos:inScheme cs: ;
    skos:prefLabel "Sea"@en ;
.

cs:sea-channel
    a skos:Concept ;
    rdfs:isDefinedBy cs: ;
    skos:altLabel "Channel"@en ;
    skos:definition "An elongated, meandering depression, usually occurring on a gently sloping plain or FAN."@en ;
    skos:historyNote "Definition from General Bathymetric Chart of the Oceans (GEBCO) Sub-Committee on Undersea Features Names (SCUFN)." ;
    skos:inScheme cs: ;
    skos:prefLabel "Sea Channel"@en ;
    schema:citation "https://iho.int/en/basic-documents-1"^^xsd:anyURI ;
.

cs:secondary-school
    a skos:Concept ;
    rdfs:isDefinedBy cs: ;
    skos:altLabel "High school"@en ;
    skos:definition "An education facility that caters for 12- 18 year olds, private and public"@en ;
    skos:historyNote "PSMA" ;
    skos:inScheme cs: ;
    skos:prefLabel "Secondary School"@en ;
.

cs:ses-facility
    a skos:Concept ;
    rdfs:isDefinedBy cs: ;
    skos:altLabel "State Emergency Services Facility"@en ;
    skos:definition "State Emergency Services Facility."@en ;
    skos:inScheme cs: ;
    skos:prefLabel "SES Facility"@en ;
.

cs:settlement
    a skos:Concept ;
    rdfs:isDefinedBy cs: ;
    skos:definition "A small rural community, typically outside a larger urban area."@en ;
    skos:inScheme cs: ;
    skos:prefLabel "Settlement"@en ;
.

cs:sewage-treatment-plant
    a skos:Concept ;
    rdfs:isDefinedBy cs: ;
    skos:definition "A facility for the process of removing contaminants from wastewater"@en ;
    skos:historyNote "PSMA" ;
    skos:inScheme cs: ;
    skos:prefLabel "Sewage Treatment Plant"@en ;
.

cs:sewer-pipeline
    a skos:Concept ;
    rdfs:isDefinedBy cs: ;
    skos:definition "A long pipe, typically underground used to transport sewage over long distances."@en ;
    skos:historyNote "new" ;
    skos:inScheme cs: ;
    skos:prefLabel "Sewer Pipeline"@en ;
.

cs:ship-wreck
    a skos:Concept ;
    rdfs:isDefinedBy cs: ;
    skos:altLabel "Wreck"@en ;
    skos:definition "The ruined remains of a stranded or sunken vessel which has been rendered useless."@en ;
    skos:historyNote "PSMA" ;
    skos:inScheme cs: ;
    skos:prefLabel "Ship Wreck"@en ;
.

cs:shopping-centre
    a skos:Concept ;
    rdfs:isDefinedBy cs: ;
    skos:altLabel
        "Arcade"@en ,
        "Mall"@en ,
        "Plaza"@en ,
        "Shopping Precinct"@en ;
    skos:definition "Typically a named area/property or group of retail businesses with their own infrastructure such as carparks."@en ;
    skos:historyNote "PSMA" ;
    skos:inScheme cs: ;
    skos:prefLabel "Shopping Cemtre"@en ;
.

cs:showground
    a skos:Concept ;
    rdfs:isDefinedBy cs: ;
    skos:definition "A tract of land with pavilion(s) and arena(s) for exhibition and display of livestock and produce"@en ;
    skos:historyNote "PSMA" ;
    skos:inScheme cs: ;
    skos:prefLabel "Showground"@en ;
.

cs:shrine
    a skos:Concept ;
    rdfs:isDefinedBy cs: ;
    skos:definition "To be defined."@en ;
    skos:inScheme cs: ;
    skos:prefLabel "Shrine"@en ;
.

cs:siding
    a skos:Concept ;
    rdfs:isDefinedBy cs: ;
    skos:altLabel "rail sidings"@en ;
    skos:definition "A short branch off a RAILWAY track, often connected at both ends to the mainline track, and used for shunting or for loading, unloading, and storing goods trucks"@en ;
    skos:historyNote "PSMA" ;
    skos:inScheme cs: ;
    skos:prefLabel "Siding"@en ;
.

cs:skate-park
    a skos:Concept ;
    rdfs:isDefinedBy cs: ;
    skos:definition "A place where the primary activity is skating or skateboarding."@en ;
    skos:historyNote "PSMA" ;
    skos:inScheme cs: ;
    skos:prefLabel "Skate Park"@en ;
.

cs:skerry
    a skos:Concept ;
    rdfs:isDefinedBy cs: ;
    skos:definition "A reef or rocky island"@en ;
    skos:inScheme cs: ;
    skos:prefLabel "Skerry"@en ;
.

cs:ski-trail
    a skos:Concept ;
    rdfs:isDefinedBy cs: ;
    skos:definition "A trail designed for downhill or cross country in the main."@en ;
    skos:historyNote "new" ;
    skos:inScheme cs: ;
    skos:prefLabel "Ski Trail"@en ;
.

cs:slope
    a skos:Concept ;
    rdfs:isDefinedBy cs: ;
    skos:altLabel
        "Hillside"@en ,
        "Toboggan run"@en ,
        "gradiants"@en ,
        "ski slopes"@en ;
    skos:definition "A gradient on the side or end of an elevated relief feature."@en ;
    skos:inScheme cs: ;
    skos:narrower cs:marine-slope ;
    skos:prefLabel "Slope"@en ;
.

cs:smelter
    a skos:Concept ;
    rdfs:isDefinedBy cs: ;
    skos:altLabel "Foundry"@en ;
    skos:definition "An industrial plant for smelting"@en ;
    skos:inScheme cs: ;
    skos:prefLabel "Smelter"@en ;
.

cs:soak
    a skos:Concept ;
    rdfs:isDefinedBy cs: ;
    skos:definition "A hollow, often in sandy soil and around the base of granite rocks, where water collects, on or below the surface of the ground."@en ;
    skos:inScheme cs: ;
    skos:prefLabel "Soak"@en ;
.

cs:solar-power-station
    a skos:Concept ;
    rdfs:isDefinedBy cs: ;
    skos:altLabel "Solar Farm"@en ;
    skos:definition "A process plant that creates power from the sun."@en ;
    skos:inScheme cs: ;
    skos:prefLabel "Solar Power Station"@en ;
.

cs:sound
    a skos:Concept ;
    rdfs:isDefinedBy cs: ;
    skos:definition "A relatively long arm of a sea or ocean forming a channel between an island and the mainland or connecting two larger bodies, as, a sea and the ocean, or two parts of the same body; usually wider and more extensive than a strait."@en ;
    skos:inScheme cs: ;
    skos:prefLabel "Sound"@en ;
.

cs:special-school
    a skos:Concept ;
    rdfs:isDefinedBy cs: ;
    skos:altLabel
        "SSP"@en ,
        "schools for specific purposes"@en ,
        "special education school"@en ,
        "special needs school"@en ,
        "specialist school"@en ;
    skos:definition "An educational facility that caters for those with learning disabilities"@en ;
    skos:historyNote "PSMA; Agreed at ICSM PNWG Meeting 2022" ;
    skos:inScheme cs: ;
    skos:prefLabel "Special School"@en ;
.

cs:specialised-hospital
    a skos:Concept ;
    rdfs:isDefinedBy cs: ;
    skos:definition "A hospital specifically for the care of a specific group or part of the body"@en ;
    skos:inScheme cs: ;
    skos:narrower
        cs:childrens-hospital ,
        cs:dental-hospital ,
        cs:eye-and-ear-hospital ,
        cs:womens-hospital ;
    skos:prefLabel "Specialised Hospital"@en ;
.

cs:spit
    a skos:Concept ;
    rdfs:isDefinedBy cs: ;
    skos:altLabel "sandspit"@en ;
    skos:definition "A narrow strip of land projecting into a body of water from the coast"@en ;
    skos:historyNote "GNR" ;
    skos:inScheme cs: ;
    skos:prefLabel "Spit"@en ;
.

cs:sport-facility
    a skos:Concept ;
    rdfs:isDefinedBy cs: ;
    skos:altLabel
        "Arena"@en ,
        "Fitness Centre"@en ,
        "Pavillion"@en ,
        "Sport Centre"@en ,
        "Sports Stadium"@en ;
    skos:definition "a place, amenity, or piece of equipment related to sport provided for a particular purpose."@en ;
    skos:historyNote "PSMA; Agreed at ICSM PNWG Meeting 2022" ;
    skos:inScheme cs: ;
    skos:prefLabel "Sport Facility"@en ;
.

cs:sports-complex
    a skos:Concept ;
    rdfs:isDefinedBy cs: ;
    skos:altLabel "Sports Precinct"@en ;
    skos:definition "Area containing multiple recreation facilities"@en ;
    skos:historyNote "PSMA; Agreed at ICSM PNWG Meeting 2022" ;
    skos:inScheme cs: ;
    skos:prefLabel "Sports Complex"@en ;
.

cs:sportsground
    a skos:Concept ;
    rdfs:isDefinedBy cs: ;
    skos:altLabel
        "Multiple sports"@en ,
        "Oval"@en ,
        "Playing Field"@en ,
        "Sports ground or field"@en ;
    skos:definition "A reserve used for sporting fixtures"@en ;
    skos:inScheme cs: ;
    skos:prefLabel "Sportsground"@en ;
.

cs:spring
    a skos:Concept ;
    rdfs:isDefinedBy cs: ;
    skos:altLabel
        "Hot spring"@en ,
        "Pool spring"@en ,
        "mineral spring"@en ;
    skos:definition "A flow of water issuing naturally out of the ground, either continuously or intermittently"@en ;
    skos:historyNote "VMHYDRO" ;
    skos:inScheme cs: ;
    skos:prefLabel "Spring"@en ;
.

cs:state
    a skos:Concept ;
    rdfs:isDefinedBy cs: ;
    skos:definition "One of the six constituent political entities that together, along with other territories, form the federation known as the Commonwealth of Australia."@en ;
    skos:inScheme cs: ;
    skos:prefLabel "State"@en ;
.

cs:state-border-section
    a skos:Concept ;
    rdfs:isDefinedBy cs: ;
    skos:definition "A named line that makes up part of the border of a state or territory."@en ;
    skos:historyNote "Refined label from original state border feature type." ;
    skos:inScheme cs: ;
    skos:prefLabel "State Border Section"@en ;
    skos:topConceptOf cs: ;
.

cs:state-electorate
    a skos:Concept ;
    rdfs:isDefinedBy cs: ;
    skos:definition "An adminstrative division of a State or Territory represented by a member of Parliament elected at a House of Representatives election."@en ;
    skos:inScheme cs: ;
    skos:prefLabel "State Electorate"@en ;
.

cs:state-forest
    a skos:Concept ;
    rdfs:isDefinedBy cs: ;
    skos:altLabel
        "FOREST RESERVE"@en ,
        "TIMBER RESERVE"@en ;
    skos:definition "An area of protected forest under a Forest Act."@en ;
    skos:historyNote "GNR" ;
    skos:inScheme cs: ;
    skos:prefLabel "State Forest"@en ;
.

cs:state-territory
    a skos:Concept ;
    rdfs:isDefinedBy cs: ;
    skos:definition "Any of the sixteen major divisions which contribute to the federated Commonwealth of Australia."@en ;
    skos:inScheme cs: ;
    skos:narrower
        cs:state ,
        cs:territory ;
    skos:prefLabel "State Or Territory"@en ;
.

cs:steel-works
    a skos:Concept ;
    rdfs:isDefinedBy cs: ;
    skos:definition "A factory where steel is made and formed into girders, rails and other goods."@en ;
    skos:inScheme cs: ;
    skos:prefLabel "Steel Works"@en ;
.

cs:stock-route
    a skos:Concept ;
    rdfs:isDefinedBy cs: ;
    skos:definition "A route designated for droving stock, with the intent of avoiding vehicular traffic"@en ;
    skos:inScheme cs: ;
    skos:prefLabel "Stock Route"@en ;
.

cs:stockyard
    a skos:Concept ;
    rdfs:isDefinedBy cs: ;
    skos:altLabel
        "Yard"@en ,
        "Yards"@en ;
    skos:definition "An enclosure forming a pen for livestock"@en ;
    skos:historyNote "PSMA" ;
    skos:inScheme cs: ;
    skos:prefLabel "Stockyard"@en ;
.

cs:subglacial-feature
    a skos:Concept ;
    rdfs:isDefinedBy cs: ;
    skos:altLabel "Under Ice Feature"@en ;
    skos:definition "Natural features of the Earth's surface under ice"@en ;
    skos:inScheme cs: ;
    skos:narrower
        cs:subglacial-basin ,
        cs:subglacial-mount ,
        cs:subglacial-trench ;
    skos:prefLabel "Subglacial Feature"@en ;
.

cs:sugar-refinery
    a skos:Concept ;
    rdfs:isDefinedBy cs: ;
    skos:definition "A refinery to convert sugar cane and sugar beets into crystallized sugar and sugar syrups"@en ;
    skos:historyNote "PSMA" ;
    skos:inScheme cs: ;
    skos:prefLabel "Sugar Refinery"@en ;
.

cs:surfing-spot
    a skos:Concept ;
    rdfs:isDefinedBy cs: ;
    skos:altLabel "Surf Break"@en ;
    skos:definition "A place where waves break on the shore or reef identified as suitable for surfing."@en ;
    skos:inScheme cs: ;
    skos:prefLabel "Surfing Spot"@en ;
.

cs:survey-marker
    a skos:Concept ;
    rdfs:isDefinedBy cs: ;
    skos:altLabel
        "horizontal control point"@en ,
        "permanent survey mark"@en ,
        "pillar"@en ,
        "survey cairn"@en ,
        "survey monument"@en ,
        "survey obelisk"@en ,
        "triangulation station"@en ,
        "trig point"@en ,
        "trigonometric point"@en ,
        "trigonometric station"@en ;
    skos:definition "A control mark used in surveys."@en ;
    skos:historyNote "PSMA; Agreed at ICSM PNWG Meeting 2022" ;
    skos:inScheme cs: ;
    skos:prefLabel "Survey Marker"@en ;
.

cs:swimming-pool
    a skos:Concept ;
    rdfs:isDefinedBy cs: ;
    skos:altLabel
        "Baths"@en ,
        "aquatic centre"@en ,
        "enclosure"@en ;
    skos:definition "An artificial pool for swimming."@en ;
    skos:historyNote "PSMA" ;
    skos:inScheme cs: ;
    skos:prefLabel "Swimming Pool"@en ;
.

cs:synagogue
    a skos:Concept ;
    rdfs:isDefinedBy cs: ;
    skos:definition "Jewish place of worship."@en ;
    skos:historyNote "PSMA" ;
    skos:inScheme cs: ;
    skos:prefLabel "Synagogue"@en ;
.

cs:tafe-facility
    a skos:Concept ;
    rdfs:isDefinedBy cs: ;
    skos:altLabel
        "TAFE"@en ,
        "institute of technology"@en ;
    skos:definition "Post secondary (TAFE) education."@en ;
    skos:historyNote "PSMA; Agreed at ICSM PNWG Meeting 2022" ;
    skos:inScheme cs: ;
    skos:prefLabel "Technical and Further Education Facility"@en ;
.

cs:tannery
    a skos:Concept ;
    rdfs:isDefinedBy cs: ;
    skos:definition "A building where animal hides and skins are processed into leather"@en ;
    skos:inScheme cs: ;
    skos:prefLabel "Tannery"@en ;
.

cs:taxi-rank
    a skos:Concept ;
    rdfs:isDefinedBy cs: ;
    skos:definition "A designated place where taxis stop for passengers to board or alight."@en ;
    skos:historyNote "PSMA" ;
    skos:inScheme cs: ;
    skos:prefLabel "Taxi Rank"@en ;
.

cs:telephone-exchange
    a skos:Concept ;
    rdfs:isDefinedBy cs: ;
    skos:altLabel
        "Telegraph Office"@en ,
        "Telephone office"@en ;
    skos:definition "A facility to establish telecommunication connections."@en ;
    skos:historyNote "GNR" ;
    skos:inScheme cs: ;
    skos:prefLabel "Telephone Exchange"@en ;
.

cs:television-communication-facility
    a skos:Concept ;
    rdfs:isDefinedBy cs: ;
    skos:altLabel "Television broadcasting facility"@en ;
    skos:definition "An antenna for transmission of sound and images by radio waves to a widely dispersed audience through television receivers"@en ;
    skos:historyNote "GNR" ;
    skos:inScheme cs: ;
    skos:prefLabel "Television Communication Facility"@en ;
.

cs:television-station
    a skos:Concept ;
    rdfs:isDefinedBy cs: ;
    skos:definition "A facility to operate the transmission of television broadcasts"@en ;
    skos:historyNote "PSMA" ;
    skos:inScheme cs: ;
    skos:prefLabel "Television Station"@en ;
.

cs:tennis-court
    a skos:Concept ;
    rdfs:isDefinedBy cs: ;
    skos:definition "A place where tennis is played."@en ;
    skos:historyNote "PSMA" ;
    skos:inScheme cs: ;
    skos:prefLabel "Tennis Court"@en ;
.

cs:terrain-feature
    a skos:Concept ;
    rdfs:isDefinedBy cs: ;
    skos:definition "Places that reflect the physical attributes of the land surface"@en ;
    skos:inScheme cs: ;
    skos:narrower
        cs:landform ,
        cs:subglacial-feature ,
        cs:undersea-feature ;
    skos:prefLabel "Terrain Feature"@en ;
    skos:topConceptOf cs: ;
.

cs:territory
    a skos:Concept ;
    rdfs:isDefinedBy cs: ;
    skos:definition "A geographic region in the Commonwealth of Australia under the jurisdiction of the Federal Government of Australia, that is not part of a State."@en ;
    skos:inScheme cs: ;
    skos:prefLabel "Territory"@en ;
.

cs:theme-park
    a skos:Concept ;
    rdfs:isDefinedBy cs: ;
    skos:definition "To be defined."@en ;
    skos:inScheme cs: ;
    skos:prefLabel "Theme Park"@en ;
.

cs:tidal-flat
    a skos:Concept ;
    rdfs:isDefinedBy cs: ;
    skos:definition "A large area of nearly level land, usually of mud, covered at high water and attached to the SHORE"@en ;
    skos:historyNote "GNR" ;
    skos:inScheme cs: ;
    skos:prefLabel "Tidal Flat"@en ;
.

cs:timber-operations
    a skos:Concept ;
    rdfs:isDefinedBy cs: ;
    skos:altLabel
        "Mill"@en ,
        "Mill Operations"@en ,
        "Paper Mill"@en ,
        "Sawmill"@en ;
    skos:definition "A place where trees are milled to create timber and or paper."@en ;
    skos:historyNote "VMFEAT" ;
    skos:inScheme cs: ;
    skos:prefLabel "Timber Operations"@en ;
.

cs:toll
    a skos:Concept ;
    rdfs:isDefinedBy cs: ;
    skos:altLabel "Turnpike"@en ;
    skos:definition "A structure used to regulate movement associated with road or rail."@en ;
    skos:historyNote "new" ;
    skos:inScheme cs: ;
    skos:prefLabel "Toll"@en ;
.

cs:tourist-attraction
    a skos:Concept ;
    rdfs:isDefinedBy cs: ;
    skos:altLabel "amusement centre"@en ;
    skos:definition "A place or facility which attracts people to visit."@en ;
    skos:historyNote "PSMA" ;
    skos:inScheme cs: ;
    skos:narrower
        cs:aquarium ,
        cs:theme-park ,
        cs:zoo ;
    skos:prefLabel "Tourist Attraction"@en ;
.

cs:tourist-region
    a skos:Concept ;
    rdfs:isDefinedBy cs: ;
    skos:definition "A relatively large area, usually within the bounds of a State or Territory, which is distinguished by certain common characteristics, natural or cultural, and recognised as such for various tourist administrative or cultural purposes."@en ;
    skos:inScheme cs: ;
    skos:prefLabel "Tourist Region"@en ;
.

cs:tourist-route
    a skos:Concept ;
    rdfs:isDefinedBy cs: ;
    skos:altLabel
        "Tourist Drive"@en ,
        "Tourist Way"@en ;
    skos:definition "A route specifically identified for tourists through an area of natural or cultural beauty and/or interest."@en ;
    skos:inScheme cs: ;
    skos:prefLabel "Tourist Route"@en ;
.

cs:town-site
    a skos:Concept ;
    rdfs:isDefinedBy cs: ;
    skos:definition "An original crown subdivision of land within a PARISH or HUNDRED which has officially recognised and gazetted boundaries."@en ;
    skos:inScheme cs: ;
    skos:prefLabel "Town Site"@en ;
.

cs:track
    a skos:Concept ;
    rdfs:isDefinedBy cs: ;
    skos:altLabel "Trail"@en ;
    skos:definition "A defined path, route or trail"@en ;
    skos:inScheme cs: ;
    skos:narrower
        cs:bicycle-track ,
        cs:cycle-crossing ,
        cs:firebreak ,
        cs:foot-tunnel ,
        cs:footbridge ,
        cs:horse-riding-trail ,
        cs:mountain-bike-track ,
        cs:multiuse-trail ,
        cs:ski-trail ,
        cs:stock-route ,
        cs:walking-track ;
    skos:prefLabel "Track"@en ;
.

cs:transfer-station
    a skos:Concept ;
    rdfs:isDefinedBy cs: ;
    skos:altLabel
        "Composting Facility"@en ,
        "Recycling Depot"@en ;
    skos:definition "A site used for the tempory sorting of refuse."@en ;
    skos:historyNote "PSMA" ;
    skos:inScheme cs: ;
    skos:prefLabel "Transfer Station"@en ;
.

cs:transport-infrastructure
    a skos:Concept ;
    rdfs:isDefinedBy cs: ;
    skos:definition "Places associated with the movement of people, goods, freight and cargo"@en ;
    skos:inScheme cs: ;
    skos:narrower
        cs:air-transport-infrastructure ,
        cs:bridge ,
        cs:rail ,
        cs:rail-transport-infrastructure ,
        cs:road-transport-infrastructure ,
        cs:track ,
        cs:transport-terminal ,
        cs:tunnel ,
        cs:walkway ,
        cs:water-transport-infrastructure ;
    skos:prefLabel "Transport Infrastructure"@en ;
    skos:topConceptOf cs: ;
.

cs:transport-terminal
    a skos:Concept ;
    rdfs:isDefinedBy cs: ;
    skos:altLabel "Transport Station"@en ;
    skos:definition "A structure beside transportation infrastructure with facilities for passengers to board or alight"@en ;
    skos:inScheme cs: ;
    skos:narrower
        cs:bus-station ,
        cs:cableway-terminal ,
        cs:ferry-station ,
        cs:rail-station ;
    skos:prefLabel "Transport Terminal"@en ;
.

cs:trench
    a skos:Concept ;
    rdfs:isDefinedBy cs: ;
    skos:definition "To be defined."@en ;
    skos:historyNote "Added by QLD 2024-03-05" ;
    skos:inScheme cs: ;
    skos:narrower
        cs:marine-trench ,
        cs:subglacial-trench ;
    skos:prefLabel "Trench"@en ;
.

cs:tunnel
    a skos:Concept ;
    rdfs:isDefinedBy cs: ;
    skos:definition "To be defined."@en ;
    skos:historyNote "Added by QLD 2024-03-05" ;
    skos:inScheme cs: ;
    skos:narrower
        cs:foot-tunnel ,
        cs:rail-tunnel ,
        cs:road-tunnel ,
        cs:tram-tunnel ;
    skos:prefLabel "Tunnel"@en ;
.

cs:unclassified
    a skos:Concept ;
    rdfs:isDefinedBy cs: ;
    skos:definition "Classification for place names which are yet to be assigned a group. Work is ongoing to classify."@en ;
    skos:inScheme cs: ;
    skos:prefLabel "Unclassified"@en ;
    skos:topConceptOf cs: ;
.

cs:underground-mine
    a skos:Concept ;
    rdfs:isDefinedBy cs: ;
    skos:altLabel
        "mineshaft"@en ,
        "shaft"@en ,
        "sub-surface mine"@en ;
    skos:definition "A place or area from which commercial minerals are removed from the Earth"@en ;
    skos:historyNote "Agreed at ICSM PNWG Meeting 2022" ;
    skos:inScheme cs: ;
    skos:prefLabel "Underground Mine"@en ;
.

cs:undersea-feature
    a skos:Concept ;
    rdfs:isDefinedBy cs: ;
    skos:definition "Natural features of the Earth's surface under water"@en ;
    skos:inScheme cs: ;
    skos:narrower
        cs:abyssal-plain ,
        cs:deep ,
        cs:guyot ,
        cs:marine-apron ,
        cs:marine-bank ,
        cs:marine-basin ,
        cs:marine-caldera ,
        cs:marine-canyon ,
        cs:marine-continental-margin ,
        cs:marine-escarpment ,
        cs:marine-fan ,
        cs:marine-fracture-zone ,
        cs:marine-gap ,
        cs:marine-hill ,
        cs:marine-hole ,
        cs:marine-knoll ,
        cs:marine-levee ,
        cs:marine-moat ,
        cs:marine-mound ,
        cs:marine-mud-volcano ,
        cs:marine-peak ,
        cs:marine-pinnacle ,
        cs:marine-plateau ,
        cs:marine-province ,
        cs:marine-reef ,
        cs:marine-ridge ,
        cs:marine-rift ,
        cs:marine-rise ,
        cs:marine-saddle ,
        cs:marine-salt-dome ,
        cs:marine-sand-ridge ,
        cs:marine-shelf ,
        cs:marine-shoal ,
        cs:marine-sill ,
        cs:marine-slope ,
        cs:marine-spur ,
        cs:marine-terrace ,
        cs:marine-trench ,
        cs:marine-trough ,
        cs:marine-valley ,
        cs:sea-channel ,
        cs:seamount ,
        cs:seamount-chain ,
        cs:subglacial-basin ;
    skos:prefLabel "Undersea Feature"@en ;
.

cs:university
    a skos:Concept ;
    rdfs:isDefinedBy cs: ;
    skos:definition "An educational institution for both instruction and examination in the higher branches of knowledge with the power to confer degrees"@en ;
    skos:historyNote "PSMA" ;
    skos:inScheme cs: ;
    skos:prefLabel "University"@en ;
.

cs:utility-infrastructure
    a skos:Concept ;
    rdfs:isDefinedBy cs: ;
    skos:definition "Places relating to the provision of information and functional services in the community."@en ;
    skos:inScheme cs: ;
    skos:narrower
        cs:communication-infrastructure ,
        cs:energy-infrastructure ,
        cs:observatory ,
        cs:waste ;
    skos:prefLabel "Utility Infrastructure"@en ;
    skos:topConceptOf cs: ;
.

cs:valley
    a skos:Concept ;
    rdfs:isDefinedBy cs: ;
    skos:altLabel
        "DALE"@en ,
        "DELL"@en ,
        "Glen"@en ,
        "VALE"@en ;
    skos:definition "A long area of lower elevation within an area of elevated relief, bounded by hills or mountains, usually with a river flowing through it, and formed by erosion or by movements in the earth's crust"@en ;
    skos:historyNote "PSMA" ;
    skos:inScheme cs: ;
    skos:narrower cs:marine-valley ;
    skos:prefLabel "Valley"@en ;
.

cs:vegetation
    a skos:Concept ;
    rdfs:isDefinedBy cs: ;
    skos:definition "Places named as a result of the naturally occuring flora"@en ;
    skos:inScheme cs: ;
    skos:narrower
        cs:forest ,
        cs:grassland ,
        cs:scrub ;
    skos:prefLabel "Vegetation"@en ;
    skos:topConceptOf cs: ;
.

cs:velodrome
    a skos:Concept ;
    rdfs:isDefinedBy cs: ;
    skos:definition "An arena with a suitably banked track for cycle races"@en ;
    skos:historyNote "VMFEAT" ;
    skos:inScheme cs: ;
    skos:prefLabel "Velodrome"@en ;
.

cs:vihara
    a skos:Concept ;
    rdfs:isDefinedBy cs: ;
    skos:definition "Buddhist place of worship."@en ;
    skos:historyNote "PSMA" ;
    skos:inScheme cs: ;
    skos:prefLabel "Vihara"@en ;
.

cs:vineyard
    a skos:Concept ;
    rdfs:isDefinedBy cs: ;
    skos:definition "A plantation of grapevines, for producing grapes for winemaking."@en ;
    skos:historyNote "PSMA" ;
    skos:inScheme cs: ;
    skos:narrower cs:plantation ;
    skos:prefLabel "Vineyard"@en ;
.

cs:volcanic-crater
    a skos:Concept ;
    rdfs:isDefinedBy cs: ;
    skos:definition "A funnel-shaped hollow at the top of the cone of a volcano"@en ;
    skos:inScheme cs: ;
    skos:prefLabel "Volcanic Crater"@en ;
.

cs:walking-track
    a skos:Concept ;
    rdfs:isDefinedBy cs: ;
    skos:altLabel
        "boardwalk"@en ,
        "hiking trail"@en ;
    skos:definition "A trail designed for foot traffic in the main. This is not a shared roadway with vehicular traffic. Main use is walking."@en ;
    skos:historyNote "PSMA 2017-12-07; Agreed at ICSM PNWG Meeting 2022" ;
    skos:inScheme cs: ;
    skos:prefLabel "Walking Track"@en ;
.

cs:walkway
    a skos:Concept ;
    rdfs:isDefinedBy cs: ;
    skos:altLabel "Pathway"@en ;
    skos:definition "Designated path primarily for pedestrian use."@en ;
    skos:historyNote "Added by QLD 2024-03-05" ;
    skos:inScheme cs: ;
    skos:prefLabel "Walkway"@en ;
.

cs:wall
    a skos:Concept ;
    rdfs:isDefinedBy cs: ;
    skos:definition "A perpendicular or steep face of a feature, considerable in height."@en ;
    skos:inScheme cs: ;
    skos:narrower
        cs:breakwater ,
        cs:ice-wall ,
        cs:rock-wall ;
    skos:prefLabel "Wall"@en ;
.

cs:waste
    a skos:Concept ;
    rdfs:isDefinedBy cs: ;
    skos:definition "An area for disposal of various types of material."@en ;
    skos:inScheme cs: ;
    skos:narrower
        cs:landfill ,
        cs:liquid-waste-disposal-site ,
        cs:scrap-yard ,
        cs:sewage-treatment-plant ,
        cs:sewer-pipeline ,
        cs:transfer-station ;
    skos:prefLabel "Waste Infrastructure"@en ;
.

cs:water-body
    a skos:Concept ;
    rdfs:isDefinedBy cs: ;
    skos:definition "Natural or constructed places where a body of water may be available"@en ;
    skos:inScheme cs: ;
    skos:narrower
        cs:aquatic-passage ,
        cs:bay ,
        cs:entrance ,
        cs:fjord ,
        cs:gulf ,
        cs:inlet ,
        cs:ocean ,
        cs:sound ;
    skos:prefLabel "Waterbody"@en ;
.

cs:water-infrastructure
    a skos:Concept ;
    rdfs:isDefinedBy cs: ;
    skos:definition "Places that indicate constructed features associated with water."@en ;
    skos:inScheme cs: ;
    skos:narrower
        cs:boat-ramp ,
        cs:breakwater ,
        cs:dam-wall ,
        cs:groyne ,
        cs:harbour ,
        cs:jetty ,
        cs:landing-place ,
        cs:lock ,
        cs:pumping-station ,
        cs:water-pipeline ,
        cs:water-plant ,
        cs:weir ;
    skos:prefLabel "Water Infrastructure"@en ;
.

cs:water-pipeline
    a skos:Concept ;
    rdfs:isDefinedBy cs: ;
    skos:definition "A long pipe used to transport water over long distances."@en ;
    skos:historyNote "new" ;
    skos:inScheme cs: ;
    skos:prefLabel "Water Pipeline"@en ;
.

cs:water-plant
    a skos:Concept ;
    rdfs:isDefinedBy cs: ;
    skos:definition "A facility for the processes of making water more acceptable to end-users"@en ;
    skos:historyNote "PSMA; Agreed at ICSM PNWG Meeting 2022" ;
    skos:inScheme cs: ;
    skos:prefLabel "Water Treatment Plant"@en ;
.

cs:water-point
    a skos:Concept ;
    rdfs:isDefinedBy cs: ;
    skos:definition "Natural or constructed places where water may be available"@en ;
    skos:inScheme cs: ;
    skos:narrower
        cs:bore ,
        cs:soak ,
        cs:spring ,
        cs:water-tank ,
        cs:waterhole ;
    skos:prefLabel "Water Point"@en ;
.

cs:water-tank
    a skos:Concept ;
    rdfs:isDefinedBy cs: ;
    skos:altLabel
        "Water Tower"@en ,
        "elevated water tank"@en ;
    skos:definition "A large container for the storage of water."@en ;
    skos:inScheme cs: ;
    skos:prefLabel "Water Tank"@en ;
.

cs:water-transport-infrastructure
    a skos:Concept ;
    rdfs:isDefinedBy cs: ;
    skos:definition "infrastructure to support navigation, safety, watercraft and shipping activities."@en ;
    skos:inScheme cs: ;
    skos:narrower
        cs:beacon ,
        cs:cargo-terminal ,
        cs:control-tower ,
        cs:dock ,
        cs:ferry-route ,
        cs:ferry-station ,
        cs:lighthouse ,
        cs:marina ,
        cs:pier ,
        cs:port ,
        cs:wharf ;
    skos:prefLabel "Water Transport Infrastructure"@en ;
.

cs:waterbody
    a skos:Concept ;
    rdfs:isDefinedBy cs: ;
    skos:definition "Natural or constructed places where a body of water may be available"@en ;
    skos:inScheme cs: ;
    skos:narrower
        cs:aquifer ,
        cs:dam ,
        cs:lagoon ,
        cs:lake ,
        cs:reservoir ,
        cs:wetland ;
    skos:prefLabel "Waterbody"@en ;
    skos:topConceptOf cs: ;
.

cs:watercourse
    a skos:Concept ;
    rdfs:isDefinedBy cs: ;
    skos:altLabel
        "Anabranch"@en ,
        "Brook"@en ,
        "Rivulet"@en ,
        "Run"@en ,
        "Stream"@en ,
        "creek"@en ,
        "gully"@en ,
        "river"@en ;
    skos:definition "A course of running water (either permanent, intermittent or largely dry)"@en ;
    skos:inScheme cs: ;
    skos:prefLabel "Watercourse"@en ;
.

cs:waterfall
    a skos:Concept ;
    rdfs:isDefinedBy cs: ;
    skos:altLabel
        "cascade"@en ,
        "cataract"@en ,
        "fall"@en ,
        "falls"@en ;
    skos:definition "A sudden descent of water over a step in the bed of a STREAM."@en ;
    skos:historyNote "VMHYDRO" ;
    skos:inScheme cs: ;
    skos:prefLabel "Waterfall"@en ;
.

cs:waterhole
    a skos:Concept ;
    rdfs:isDefinedBy cs: ;
    skos:altLabel
        "pond"@en ,
        "pool"@en ,
        "rock pool"@en ;
    skos:definition "A small body of still or standing water, permanent or temporary, often in the bed of an intermittent RIVER or STREAM, and sometimes SPRING fed, chiefly one of natural formation."@en ;
    skos:historyNote "GNR" ;
    skos:inScheme cs: ;
    skos:prefLabel "Waterhole"@en ;
.

cs:waterway
    a skos:Concept ;
    rdfs:isDefinedBy cs: ;
    skos:definition "Natural or constructed places that are associated with the movement of water"@en ;
    skos:inScheme cs: ;
    skos:narrower
        cs:bend ,
        cs:canal ,
        cs:drain ,
        cs:estuary ,
        cs:irrigation-channel ,
        cs:rapids ,
        cs:reach ,
        cs:watercourse ,
        cs:waterfall ;
    skos:prefLabel "Waterway"@en ;
.

cs:weather-station
    a skos:Concept ;
    rdfs:isDefinedBy cs: ;
    skos:altLabel
        "Automatic Weather Station"@en ,
        "Meteorological Station"@en ;
    skos:definition "An installation equipped and used for the making of meteorological observation."@en ;
    skos:inScheme cs: ;
    skos:prefLabel "Weather Station"@en ;
.

cs:weighbridge
    a skos:Concept ;
    rdfs:isDefinedBy cs: ;
    skos:definition "A device located at the side of a road for weighing vehicles and their loads"@en ;
    skos:historyNote "PSMA" ;
    skos:inScheme cs: ;
    skos:prefLabel "Weighbridge"@en ;
.

cs:weir
    a skos:Concept ;
    rdfs:isDefinedBy cs: ;
    skos:altLabel
        "Spillway"@en ,
        "barrage"@en ;
    skos:definition "A low barrier across a watercourse over which water is allowed to flow steadily. A weir raises the water level upstream, and can also be used to measure flow and control the depth of water impounded"@en ;
    skos:historyNote "GNR 2023-09-19" ;
    skos:inScheme cs: ;
    skos:prefLabel "Weir"@en ;
.

cs:wetland
    a skos:Concept ;
    rdfs:isDefinedBy cs: ;
    skos:altLabel
        "Bog"@en ,
        "Marsh"@en ,
        "Morass"@en ,
        "Salt marsh"@en ,
        "Swamp"@en ;
    skos:definition "Areas inundated or saturated by surface or groundwater at a frequency and duration sufficient to support vegetation typical of SWAMPS, MARSHES, bogs."@en ;
    skos:historyNote "GNR; Agreed at ICSM PNWG Meeting 2022" ;
    skos:inScheme cs: ;
    skos:prefLabel "Wetland"@en ;
.

cs:wharf
    a skos:Concept ;
    rdfs:isDefinedBy cs: ;
    skos:definition "A platform, contiguous to and more or less parallel with the shoreline, alongside which ships may be secured for loading or unloading cargo or passengers"@en ;
    skos:historyNote "HY_WATER_STRUCT_LINE" ;
    skos:inScheme cs: ;
    skos:prefLabel "Wharf"@en ;
.

cs:wind-farm
    a skos:Concept ;
    rdfs:isDefinedBy cs: ;
    skos:definition "Consists of a group of individual wind turbines which are connected to the electric power transmission network."@en ;
    skos:historyNote "VMFEAT" ;
    skos:inScheme cs: ;
    skos:prefLabel "Wind Farm"@en ;
.

cs:wind-turbine
    a skos:Concept ;
    rdfs:isDefinedBy cs: ;
    skos:definition "A turbine used to generate electricity in areas with strong, steady winds, sometimes offshore"@en ;
    skos:historyNote "VMFEAT" ;
    skos:inScheme cs: ;
    skos:prefLabel "Wind Turbine"@en ;
.

cs:winery
    a skos:Concept ;
    rdfs:isDefinedBy cs: ;
    skos:altLabel
        "Cellar"@en ,
        "Cellar door"@en ;
    skos:definition "A commercial establishment where wine is made."@en ;
    skos:inScheme cs: ;
    skos:prefLabel "Winery"@en ;
.

cs:womens-hospital
    a skos:Concept ;
    rdfs:isDefinedBy cs: ;
    skos:definition "To be defined."@en ;
    skos:historyNote "Added by QLD 2024-03-05" ;
    skos:inScheme cs: ;
    skos:prefLabel "Womens Hospital"@en ;
.

cs:zoo
    a skos:Concept ;
    rdfs:isDefinedBy cs: ;
    skos:altLabel
        "Wildlife Park"@en ,
        "Wildlife sanctuary"@en ,
        "zoological gardens"@en ;
    skos:definition "An establishment which maintains a collection of wild animals, typically in a park or gardens, for study, conservation, or display to the public."@en ;
    skos:historyNote "PSMA; Agreed at ICSM PNWG Meeting 2022" ;
    skos:inScheme cs: ;
    skos:prefLabel "Zoo"@en ;
.

cs:breakwater
    a skos:Concept ;
    rdfs:isDefinedBy cs: ;
    skos:altLabel
        "mole"@en ,
        "sea wall"@en ;
    skos:definition """A natural or artificial structure along a coast 
capable of checking the force of the waves, 
thereby reducing beach erosion."""@en ;
    skos:historyNote "Definition from Geographical Names Board, NSW" ;
    skos:inScheme cs: ;
    skos:narrower
        cs:groyne ,
        cs:levee ;
    skos:prefLabel "Breakwater"@en ;
    schema:citation "https://www.gnb.nsw.gov.au/__data/assets/pdf_file/0011/59627/Glossary_of_Designation_Values.pdf"^^xsd:anyURI ;
.

cs:bus-station
    a skos:Concept ;
    rdfs:isDefinedBy cs: ;
    skos:definition "A structure beside the road with facilities for passengers to board or alight"@en ;
    skos:historyNote "Agreed at ICSM PNWG Meeting 2022" ;
    skos:inScheme cs: ;
    skos:prefLabel "Bus Station"@en ;
.

cs:cableway-terminal
    a skos:Concept ;
    rdfs:isDefinedBy cs: ;
    skos:definition "A building associated with a cableway."@en ;
    skos:historyNote "PSMA" ;
    skos:inScheme cs: ;
    skos:prefLabel "Cableway Terminal"@en ;
.

cs:ferry-station
    a skos:Concept ;
    rdfs:isDefinedBy cs: ;
    skos:altLabel "Passenger Terminal"@en ;
    skos:definition "A designated place where ferries stop for passengers to board or alight"@en ;
    skos:historyNote "NEW" ;
    skos:inScheme cs: ;
    skos:prefLabel "Ferry Station"@en ;
.

cs:foot-tunnel
    a skos:Concept ;
    rdfs:isDefinedBy cs: ;
    skos:altLabel "subway"@en ;
    skos:definition "A passageway for pedestrians through or under an obstruction."@en ;
    skos:historyNote "new" ;
    skos:inScheme cs: ;
    skos:prefLabel "Foot Tunnel"@en ;
.

cs:footbridge
    a skos:Concept ;
    rdfs:isDefinedBy cs: ;
    skos:definition "A structure spanning a rail line, river, road or the like affording safe passage for pedestrians"@en ;
    skos:historyNote "PSMA; Agreed at ICSM PNWG Meeting 2022" ;
    skos:inScheme cs: ;
    skos:prefLabel "Footbridge"@en ;
.

cs:groyne
    a skos:Concept ;
    rdfs:isDefinedBy cs: ;
    skos:definition "A low artificial wall-like structure constructed of timber, stone, concrete or steel, usually extending roughly perpendicular to the SHORELINE and designed to protect the SHORE from erosion or to trap sand."@en ;
    skos:historyNote "GNR" ;
    skos:inScheme cs: ;
    skos:prefLabel "Groyne"@en ;
.

cs:guyot
    a skos:Concept ;
    rdfs:isDefinedBy cs: ;
    skos:altLabel "Tablemount"@en ;
    skos:definition "A SEAMOUNT with a comparatively smooth flat top."@en ;
    skos:historyNote "Definition from General Bathymetric Chart of the Oceans (GEBCO) Sub-Committee on Undersea Features Names (SCUFN)." ;
    skos:inScheme cs: ;
    skos:prefLabel "Guyot"@en ;
    schema:citation "https://iho.int/en/basic-documents-1"^^xsd:anyURI ;
.

cs:ice-wall
    a skos:Concept ;
    rdfs:isDefinedBy cs: ;
    skos:definition "An ice cliff forming the seaward margin of an inland ice sheet, ice cap, ice piedmont or ice rise. The rock basement may be at or below sea level."@en ;
    skos:historyNote "Concept and definition from the Australian Antarctic Division." ;
    skos:inScheme cs: ;
    skos:prefLabel "Ice Wall"@en ;
    schema:citation "https://data.aad.gov.au/aadc/ftc/display_feature_type.cfm?feature_type_code=343"^^xsd:anyURI ;
.

cs:levee
    a skos:Concept ;
    rdfs:isDefinedBy cs: ;
    skos:definition "An embankment built to confine a river from flooding."@en ;
    skos:inScheme cs: ;
    skos:prefLabel "Levee"@en ;
.

cs:light-rail
    a skos:Concept ;
    rdfs:isDefinedBy cs: ;
    skos:altLabel
        "tram line"@en ,
        "tramway"@en ;
    skos:definition "A track or set of tracks of iron or steel rails used for the passage of light rail"@en ;
    skos:historyNote "new" ;
    skos:inScheme cs: ;
    skos:prefLabel "Light Rail"@en ;
.

cs:light-rail-station
    a skos:Concept ;
    rdfs:isDefinedBy cs: ;
    skos:altLabel
        "tram station"@en ,
        "tram stop"@en ;
    skos:definition "A structure beside a light rail line with facilities for receiving and discharging passengers"@en ;
    skos:historyNote "Added 2023-09-19" ;
    skos:inScheme cs: ;
    skos:prefLabel "Light Rail Station"@en ;
.

cs:marine-bank
    a skos:Concept ;
    rdfs:isDefinedBy cs: ;
    skos:altLabel "Cap"@en ;
    skos:definition "An elevation of the seafloor at depths generally less than 200m, but sufficient for safe surface navigation commonly found on the continental shelf or near an island."@en ;
    skos:historyNote "Definition from General Bathymetric Chart of the Oceans (GEBCO) Sub-Committee on Undersea Features Names (SCUFN)." ;
    skos:inScheme cs: ;
    skos:prefLabel "Marine Bank"@en ;
    schema:citation "https://iho.int/en/basic-documents-1"^^xsd:anyURI ;
.

cs:marine-basin
    a skos:Concept ;
    rdfs:isDefinedBy cs: ;
    skos:definition "A depression more or less equidimensional in plan and of variable extent."@en ;
    skos:historyNote "Definition from General Bathymetric Chart of the Oceans (GEBCO) Sub-Committee on Undersea Features Names (SCUFN)." ;
    skos:inScheme cs: ;
    skos:narrower cs:deep ;
    skos:prefLabel "Marine Basin"@en ;
    schema:citation "https://iho.int/en/basic-documents-1"^^xsd:anyURI ;
.

cs:marine-escarpment
    a skos:Concept ;
    rdfs:isDefinedBy cs: ;
    skos:altLabel "Marine Scarp"@en ;
    skos:definition "An elongated, characteristically linear, steep SLOPE separating horizontal or gently sloping areas of the sea floor."@en ;
    skos:historyNote "Definition from General Bathymetric Chart of the Oceans (GEBCO) Sub-Committee on Undersea Features Names (SCUFN)." ;
    skos:inScheme cs: ;
    skos:prefLabel "Marine Escarpment"@en ;
    schema:citation "https://iho.int/en/basic-documents-1"^^xsd:anyURI ;
.

cs:marine-gap
    a skos:Concept ;
    rdfs:isDefinedBy cs: ;
    skos:definition "A narrow break in a RIDGE, RISE or other ELEVATION."@en ;
    skos:historyNote "Definition from General Bathymetric Chart of the Oceans (GEBCO) Sub-Committee on Undersea Features Names (SCUFN). Passage as a previous alternative label removed due to conflict with Aquatic Passage." ;
    skos:inScheme cs: ;
    skos:prefLabel "Marine Gap"@en ;
    schema:citation "https://iho.int/en/basic-documents-1"^^xsd:anyURI ;
.

cs:marine-hill
    a skos:Concept ;
    rdfs:isDefinedBy cs: ;
    skos:altLabel "Abyssal Hill"@en ;
    skos:definition "A distinct ELEVATION generally of irregular shape, less than 1000m above the surrounding relief as measured from the deepest isobath that surrounds most of the feature."@en ;
    skos:historyNote "Definition from General Bathymetric Chart of the Oceans (GEBCO) Sub-Committee on Undersea Features Names (SCUFN)." ;
    skos:inScheme cs: ;
    skos:prefLabel "Marine Hill"@en ;
    schema:citation "https://iho.int/en/basic-documents-1"^^xsd:anyURI ;
.

cs:marine-plateau
    a skos:Concept ;
    rdfs:isDefinedBy cs: ;
    skos:definition "A large, relatively flat ELEVATION that is higher than the surrounding relief with one or more relatively steep sides."@en ;
    skos:historyNote "Definition from General Bathymetric Chart of the Oceans (GEBCO) Sub-Committee on Undersea Features Names (SCUFN)." ;
    skos:inScheme cs: ;
    skos:prefLabel "Marine Plateau"@en ;
    schema:citation "https://iho.int/en/basic-documents-1"^^xsd:anyURI ;
.

cs:marine-slope
    a skos:Concept ;
    rdfs:isDefinedBy cs: ;
    skos:altLabel
        "Archipelagic Apron"@en ,
        "Continental Rise"@en ,
        "Continental Slope"@en ,
        "Scarp"@en ;
    skos:definition "The sloping region that deepens from a SHELF to the point where there is a general decrease in gradient."@en ;
    skos:historyNote "Definition from General Bathymetric Chart of the Oceans (GEBCO) Sub-Committee on Undersea Features Names (SCUFN)." ;
    skos:inScheme cs: ;
    skos:prefLabel "Marine Slope"@en ;
    schema:citation "https://iho.int/en/basic-documents-1"^^xsd:anyURI ;
.

cs:marine-trench
    a skos:Concept ;
    rdfs:isDefinedBy cs: ;
    skos:definition "A long, deep, asymmetrical depression with relatively steep sides, that is associated with subduction."@en ;
    skos:historyNote "Definition from General Bathymetric Chart of the Oceans (GEBCO) Sub-Committee on Undersea Features Names (SCUFN)." ;
    skos:inScheme cs: ;
    skos:narrower cs:deep ;
    skos:prefLabel "Marine Trench"@en ;
    schema:citation "https://iho.int/en/basic-documents-1"^^xsd:anyURI ;
.

cs:marine-valley
    a skos:Concept ;
    rdfs:isDefinedBy cs: ;
    skos:altLabel
        "Median Valley"@en ,
        "Sea Valley"@en ,
        "Seabight"@en ,
        "Submarine Valley"@en ;
    skos:definition "An elongated depression that generally widens and deepens down-slope"@en ;
    skos:historyNote "Definition from General Bathymetric Chart of the Oceans (GEBCO) Sub-Committee on Undersea Features Names (SCUFN)." ;
    skos:inScheme cs: ;
    skos:prefLabel "Marine Valley"@en ;
    schema:citation "https://iho.int/en/basic-documents-1"^^xsd:anyURI ;
.

cs:mining-centre
    a skos:Concept ;
    rdfs:isDefinedBy cs: ;
    skos:definition "A facility built to support a mine or other area from which ores, precious stones or minerals are or were extracted from the earth."@en ;
    skos:historyNote "PSMA (feature), WA (definition added 12/21/2023)" ;
    skos:inScheme cs: ;
    skos:prefLabel "Mining Centre"@en ;
.

cs:offshore-rock
    a skos:Concept ;
    rdfs:isDefinedBy cs: ;
    skos:definition "A typically unvegetated rock protruding from the sea."@en ;
    skos:inScheme cs: ;
    skos:prefLabel "Offshore Rock"@en ;
.

cs:plantation
    a skos:Concept ;
    rdfs:isDefinedBy cs: ;
    skos:altLabel "Orchard"@en ;
    skos:definition "A plot in which trees are planted and cultivated, usually for commercial purposes"@en ;
    skos:historyNote "PSMA" ;
    skos:inScheme cs: ;
    skos:prefLabel "Plantation"@en ;
.

cs:rail-bridge
    a skos:Concept ;
    rdfs:isDefinedBy cs: ;
    skos:definition "A structure over an obstruction affording safe rail passage."@en ;
    skos:historyNote "PSMA" ;
    skos:inScheme cs: ;
    skos:prefLabel "Rail Bridge"@en ;
.

cs:rail-station
    a skos:Concept ;
    rdfs:isDefinedBy cs: ;
    skos:altLabel
        "railway station"@en ,
        "station"@en ,
        "train station"@en ;
    skos:definition "A structure beside a railway line with facilities for receiving and discharging passengers and freight."@en ;
    skos:historyNote "PSMA; Agreed at ICSM PNWG Meeting 2022" ;
    skos:inScheme cs: ;
    skos:narrower cs:light-rail-station ;
    skos:prefLabel "Rail Station"@en ;
.

cs:rail-tunnel
    a skos:Concept ;
    rdfs:isDefinedBy cs: ;
    skos:definition "A passageway for trains through or under an obstruction."@en ;
    skos:historyNote "PSMA" ;
    skos:inScheme cs: ;
    skos:narrower
        cs:light-rail-tunnel ,
        cs:tram-tunnel ;
    skos:prefLabel "Rail Tunnel"@en ;
.

cs:residential-aged-care
    a skos:Concept ;
    rdfs:isDefinedBy cs: ;
    skos:definition "A residential facility that supports the care of the elderly."@en ;
    skos:inScheme cs: ;
    skos:prefLabel "Residential Aged Care"@en ;
.

cs:road-bridge
    a skos:Concept ;
    rdfs:isDefinedBy cs: ;
    skos:altLabel
        "flyover"@en ,
        "overpass"@en ;
    skos:definition "A structure spanning a rail line, river, road or the like affording safe road passage."@en ;
    skos:historyNote "new" ;
    skos:inScheme cs: ;
    skos:prefLabel "Road Bridge"@en ;
.

cs:road-tunnel
    a skos:Concept ;
    rdfs:isDefinedBy cs: ;
    skos:altLabel "underpass"@en ;
    skos:definition "A passageway for motor vehicles through or under an obstruction."@en ;
    skos:historyNote "new" ;
    skos:inScheme cs: ;
    skos:prefLabel "Road Tunnel"@en ;
.

cs:seamount
    a skos:Concept ;
    rdfs:isDefinedBy cs: ;
    skos:definition "A distinct generally equidimensional ELEVATION greater than 1000m above the surrounding relief as measured from the deepest isobath that surrounds most of the feature."@en ;
    skos:historyNote "Definition from General Bathymetric Chart of the Oceans (GEBCO) Sub-Committee on Undersea Features Names (SCUFN)." ;
    skos:inScheme cs: ;
    skos:narrower cs:guyot ;
    skos:prefLabel "Seamount"@en ;
    schema:citation "https://iho.int/en/basic-documents-1"^^xsd:anyURI ;
.

cs:seamount-chain
    a skos:Concept ;
    rdfs:isDefinedBy cs: ;
    skos:definition "A linear or arcuate alignment of discrete SEAMOUNTS."@en ;
    skos:historyNote "Definition from General Bathymetric Chart of the Oceans (GEBCO) Sub-Committee on Undersea Features Names (SCUFN)." ;
    skos:inScheme cs: ;
    skos:prefLabel "Seamount Chain"@en ;
    schema:citation "https://iho.int/en/basic-documents-1"^^xsd:anyURI ;
.

cs:subglacial-mount
    a skos:Concept ;
    rdfs:isDefinedBy cs: ;
    skos:altLabel "Subglacial Mountain"@en ;
    skos:definition "Subglacial: a term meaning 'beneath the ice'. Mountain: A mass of land considerably higher than its surroundings and of greater altitude than a hill"@en ;
    skos:historyNote "Derived from definition from the Australian Antarctic Division." ;
    skos:inScheme cs: ;
    skos:prefLabel "Subglacial Mount"@en ;
    schema:citation "https://data.aad.gov.au/aadc/ftc/display_feature_type.cfm?feature_type_code=427"^^xsd:anyURI ;
.

cs:subglacial-trench
    a skos:Concept ;
    rdfs:isDefinedBy cs: ;
    skos:definition "Subglacial: a term meaning 'beneath the ice'. Trench: A deep, or elongated trough, in a floor of the ocean"@en ;
    skos:inScheme cs: ;
    skos:prefLabel "Subglacial Trench"@en ;
.

cs:tram-tunnel
    a skos:Concept ;
    rdfs:isDefinedBy cs: ;
    skos:definition "To be defined."@en ;
    skos:inScheme cs: ;
    skos:prefLabel "Tram Tunnel"@en ;
.

cs:subglacial-basin
    a skos:Concept ;
    rdfs:isDefinedBy cs: ;
    skos:definition "Subglacial: a term meaning 'beneath the ice'. Basin: a very large depression occupied by sea water, ie. an ocean basin."@en ;
    skos:historyNote "Concept and definition from the Australian Antarctic Division." ;
    skos:inScheme cs: ;
    skos:prefLabel "Subglacial Basin"@en ;
    schema:citation "https://data.aad.gov.au/aadc/ftc/display_feature_type.cfm?feature_type_code=426"^^xsd:anyURI ;
.

cs:deep
    a skos:Concept ;
    rdfs:isDefinedBy cs: ;
    skos:definition "A localised depression within the confines of a larger feature, such as a trough, basin or trench"@en ;
    skos:historyNote "Definition from General Bathymetric Chart of the Oceans (GEBCO) Sub-Committee on Undersea Features Names (SCUFN)." ;
    skos:inScheme cs: ;
    skos:prefLabel "Deep"@en ;
    schema:citation "https://iho.int/en/basic-documents-1"^^xsd:anyURI ;
.

cs:
    a skos:ConceptScheme ;
    dcterms:created "2015-01-01"^^xsd:date ;
    dcterms:modified "2024-03-19"^^xsd:date ;
    reg:status <https://linked.data.gov.au/def/reg-statuses/experimental> ;
    owl:versionIRI <https://linked.data.gov.au/def/go-categories/1.0.1> ;
    skos:definition "A hierarchy of Geographical (Place) Object categories"@en ;
    skos:hasTopConcept
        cs:administrative-area ,
        cs:care-facility ,
        cs:cultural-feature ,
        cs:defence-site ,
        cs:educational-facility ,
        cs:emergency-facility ,
        cs:health-facility ,
        cs:hydrological-feature ,
        cs:ice-feature ,
        cs:legal-institution ,
        cs:mining-feature ,
        cs:populated-place ,
        cs:state-border-section ,
        cs:terrain-feature ,
        cs:transport-infrastructure ,
        cs:unclassified ,
        cs:utility-infrastructure ,
        cs:vegetation ,
        cs:waterbody ;
    skos:historyNote "This vocabulary was originally generated from the Geoscience Australia's Composite Gazetteer of Australia, and has been amended by the Department of Resources to refine and expand the vocabulary."@en ;
    skos:prefLabel "Geographical Object Categories"@en ;
    schema:creator [
            a schema:Organization ;
            schema:name "Place Names Working Group" ;
            schema:url ""^^xsd:anyURI
        ] ;
    schema:keywords
        "Geographic Names" ,
        "Geographic Objects" ,
        "Place Names" ;
    schema:publisher [
            a schema:Organization ;
            schema:name "Department Of Resources" ;
            schema:url ""^^xsd:anyURI
        ] ;
    schema:version "1.0.1" ;
.

