PREFIX dcat: <http://www.w3.org/ns/dcat#>
PREFIX dcterms: <http://purl.org/dc/terms/>
PREFIX isoroles: <http://def.isotc211.org/iso19115/-1/2018/CitationAndResponsiblePartyInformation/code/CI_RoleCode/>
PREFIX pa: <https://linked.data.gov.au/def/positional-accuracy>
PREFIX prov: <http://www.w3.org/ns/prov#>
PREFIX rdfs: <http://www.w3.org/2000/01/rdf-schema#>
PREFIX skos: <http://www.w3.org/2004/02/skos/core#>
PREFIX xsd: <http://www.w3.org/2001/XMLSchema#>

pa:100m
    a skos:Concept ;
    skos:altLabel "Remote"@en ;
    skos:definition "Minimum spatial accuracy of plus or minus 100 metres. Typically remote area capture."@en ;
    skos:historyNote "Queensland Roads and Tracks dataset, influenced by the Queensland Spatial Information Council Digital Road Network Standard." ;
    skos:inScheme pa: ;
    skos:prefLabel "100m"@en ;
.

pa:25m
    a skos:Concept ;
    skos:altLabel "Rural"@en ;
    skos:definition "Minimum spatial accuracy of plus or minus 25 metres. Typically rural capture."@en ;
    skos:historyNote "Queensland Roads and Tracks dataset, influenced by the Queensland Spatial Information Council Digital Road Network Standard." ;
    skos:inScheme pa: ;
    skos:prefLabel "25m"@en ;
.

pa:2m
    a skos:Concept ;
    skos:altLabel "Urban"@en ;
    skos:definition "Minimum spatial accuracy of plus or minus 2 metres. Typically urban capture."@en ;
    skos:historyNote "Queensland Roads and Tracks dataset, influenced by the Queensland Spatial Information Council Digital Road Network Standard." ;
    skos:inScheme pa: ;
    skos:prefLabel "2m"@en ;
.

pa:5m
    a skos:Concept ;
    skos:altLabel "Peri-Urban"@en ;
    skos:definition "Minimum spatial accuracy of plus or minus 5 metres. Typically peri-urban capture."@en ;
    skos:historyNote "Queensland Roads and Tracks dataset, influenced by the Queensland Spatial Information Council Digital Road Network Standard." ;
    skos:inScheme pa: ;
    skos:prefLabel "5m"@en ;
.

pa:unknown
    a skos:Concept ;
    skos:altLabel "U"@en ;
    skos:definition "Minimum spatial accuracy unknown."@en ;
    skos:historyNote "Queensland Roads and Tracks dataset, influenced by the Queensland Spatial Information Council Digital Road Network Standard." ;
    skos:inScheme pa: ;
    skos:prefLabel "Unknown"@en ;
.

pa:
    a skos:ConceptScheme ;
    dcterms:created "2023-05-31"^^xsd:date ;
    dcterms:creator [
            a prov:Agent ;
            rdfs:label "Department Of Resources"
        ] ;
    dcterms:identifier "positional-accuracy"^^xsd:token ;
    dcterms:modified "2023-05-31"^^xsd:date ;
    dcterms:publisher [
            a prov:Agent ;
            rdfs:label "Icsm"
        ] ;
    skos:definition "This vocabulary describes categories of positional accuracy information to indicate the spatial accuracy of data capture. "@en ;
    skos:hasTopConcept
        pa:100m ,
        pa:25m ,
        pa:2m ,
        pa:5m ,
        pa:unknown ;
    skos:historyNote "This vocabulary was created by the Queensland Spatial Information services." ;
    skos:prefLabel "Positional Accuracy"@en ;
    prov:qualifiedAttribution [
            dcat:hadRole isoroles:custodian ;
            prov:agent [
                    a prov:Agent ;
                    rdfs:label "Icsm"
                ]
        ] ;
.

