PREFIX dcat: <http://www.w3.org/ns/dcat#>
PREFIX dcterms: <http://purl.org/dc/terms/>
PREFIX isoroles: <http://def.isotc211.org/iso19115/-1/2018/CitationAndResponsiblePartyInformation/code/CI_RoleCode/>
PREFIX lrrs: <https://linked.data.gov.au/def/local-road-regional-significance-indicator>
PREFIX prov: <http://www.w3.org/ns/prov#>
PREFIX rdfs: <http://www.w3.org/2000/01/rdf-schema#>
PREFIX skos: <http://www.w3.org/2004/02/skos/core#>
PREFIX xsd: <http://www.w3.org/2001/XMLSchema#>

lrrs:local-road-of-regional-significance
    a skos:Concept ;
    dcterms:provenance "Queensland Roads and Tracks dataset" ;
    skos:altLabel
        "T"@en ,
        "True"@en ;
    skos:definition "Road is designated as a Local Road of Regional Significance."@en ;
    skos:inScheme <https://linked.data.gov.au/def/lrrs-indicator> ;
    skos:prefLabel "Local Road of Regional Significance"@en ;
.

lrrs:not-local-road-of-regional-significance
    a skos:Concept ;
    dcterms:provenance "Queensland Roads and Tracks dataset" ;
    skos:altLabel
        "F"@en ,
        "False"@en ;
    skos:definition "Road is not designated as a Local Road of Regional Significance."@en ;
    skos:inScheme <https://linked.data.gov.au/def/lrrs-indicator> ;
    skos:prefLabel "Not Local Road of Regional Significance"@en ;
.

lrrs:unknown
    a skos:Concept ;
    dcterms:provenance "Queensland Roads and Tracks dataset" ;
    skos:altLabel "U"@en ;
    skos:definition "Unknown - It is not known if the road is designated as a Local Road of Regional Significance."@en ;
    skos:inScheme <https://linked.data.gov.au/def/lrrs-indicator> ;
    skos:prefLabel "Unknown"@en ;
.

<https://linked.data.gov.au/def/lrrs-indicator>
    a skos:ConceptScheme ;
    dcterms:created "2023-05-31"^^xsd:date ;
    dcterms:creator [
            a prov:Agent ;
            rdfs:label "Department Of Resources"
        ] ;
    dcterms:identifier "lrrs-indicator"^^xsd:token ;
    dcterms:modified "2023-05-31"^^xsd:date ;
    dcterms:publisher [
            a prov:Agent ;
            rdfs:label "Icsm"
        ] ;
    skos:definition "This vocabulary describes whether a road is designated as a local road of regional significance (LRSS)."@en ;
    skos:prefLabel "Local Road of Regional Significance Indicator"@en ;
    prov:qualifiedAttribution [
            dcat:hadRole isoroles:custodian ;
            prov:agent [
                    a prov:Agent ;
                    rdfs:label "Icsm"
                ]
        ] ;
.

