PREFIX dcat: <http://www.w3.org/ns/dcat#>
PREFIX dcterms: <http://purl.org/dc/terms/>
PREFIX isoroles: <http://def.isotc211.org/iso19115/-1/2018/CitationAndResponsiblePartyInformation/code/CI_RoleCode/>
PREFIX prov: <http://www.w3.org/ns/prov#>
PREFIX rcr: <https://linked.data.gov.au/def/road-cadastral-relationship>
PREFIX rdfs: <http://www.w3.org/2000/01/rdf-schema#>
PREFIX skos: <http://www.w3.org/2004/02/skos/core#>
PREFIX xsd: <http://www.w3.org/2001/XMLSchema#>

rcr:not-related
    a skos:Concept ;
    skos:definition "Road segment is not related to an area of road in the cadastre."@en ;
    skos:historyNote "Queensland Roads and Tracks dataset" ;
    skos:inScheme rcr: ;
    skos:prefLabel "No Relationship To Cadastral Road Area"@en ;
.

rcr:related-off
    a skos:Concept ;
    skos:definition "Road segment is related to an area of road in the cadastre, but part of the centreline lies outside of this area."@en ;
    skos:historyNote "Queensland Roads and Tracks dataset" ;
    skos:inScheme rcr: ;
    skos:prefLabel "Off Alignment To Cadastral Road Area"@en ;
.

rcr:related-within
    a skos:Concept ;
    skos:definition "Road segment is related to an area of road in the cadastre, and the centreline lies inside of this area."@en ;
    skos:historyNote "Queensland Roads and Tracks dataset" ;
    skos:inScheme rcr: ;
    skos:prefLabel "Within Cadastral Road Area"@en ;
.

rcr:unknown
    a skos:Concept ;
    skos:altLabel
        "U"@en ,
        "Unknown"@en ;
    skos:definition "Unknown if the road segment is related to an area of road in the cadastre."@en ;
    skos:historyNote "Queensland Roads and Tracks dataset" ;
    skos:inScheme rcr: ;
    skos:prefLabel "Unknown Relationship To Cadastral Road Area"@en ;
.

rcr:
    a skos:ConceptScheme ;
    dcterms:created "2023-05-31"^^xsd:date ;
    dcterms:creator [
            a prov:Agent ;
            rdfs:label "Department Of Resources"
        ] ;
    dcterms:identifier "road-cadastral-relationship"^^xsd:token ;
    dcterms:modified "2023-05-31"^^xsd:date ;
    dcterms:publisher [
            a prov:Agent ;
            rdfs:label "Icsm"
        ] ;
    skos:definition "This vocabulary describes the relationship, or alignment, of a road to a cadastral road area."@en ;
    skos:hasTopConcept
        rcr:not-related ,
        rcr:related-off ,
        rcr:related-within ,
        rcr:unknown ;
    skos:historyNote "This vocabulary was created by the Queensland Spatial Information services." ;
    skos:prefLabel "Road Cadastral Relationship"@en ;
    prov:qualifiedAttribution [
            dcat:hadRole isoroles:custodian ;
            prov:agent [
                    a prov:Agent ;
                    rdfs:label "Icsm"
                ]
        ] ;
.

