PREFIX dcat: <http://www.w3.org/ns/dcat#>
PREFIX dcterms: <http://purl.org/dc/terms/>
PREFIX isoroles: <http://def.isotc211.org/iso19115/-1/2018/CitationAndResponsiblePartyInformation/code/CI_RoleCode/>
PREFIX lc: <https://linked.data.gov.au/def/road-lane-count>
PREFIX prov: <http://www.w3.org/ns/prov#>
PREFIX rdfs: <http://www.w3.org/2000/01/rdf-schema#>
PREFIX skos: <http://www.w3.org/2004/02/skos/core#>
PREFIX xsd: <http://www.w3.org/2001/XMLSchema#>

lc:one
    a skos:Concept ;
    skos:definition "Two vehicles cannot pass each other without both having to move off the formed surface."@en ;
    skos:historyNote "Queensland Roads and Tracks dataset" ;
    skos:inScheme lc: ;
    skos:prefLabel "One"@en ;
.

lc:two-or-more
    a skos:Concept ;
    skos:definition "Two vehicles can pass each other without having to move off the formed surface."@en ;
    skos:historyNote "Queensland Roads and Tracks dataset" ;
    skos:inScheme lc: ;
    skos:prefLabel "Two or more"@en ;
.

lc:unknown
    a skos:Concept ;
    skos:definition "The lane count is not currently known."@en ;
    skos:historyNote "Queensland Roads and Tracks dataset" ;
    skos:inScheme lc: ;
    skos:prefLabel "Unknown"@en ;
.

lc:
    a skos:ConceptScheme ;
    dcterms:created "2023-05-30"^^xsd:date ;
    dcterms:creator [
            a prov:Agent ;
            rdfs:label "Department Of Resources"
        ] ;
    dcterms:identifier "road-lane-count"^^xsd:token ;
    dcterms:modified "2023-05-30"^^xsd:date ;
    dcterms:publisher [
            a prov:Agent ;
            rdfs:label "Icsm"
        ] ;
    skos:definition "This vocabulary describes the number of lanes that indicate whether vehicles are able to travel past each other on the formed surface of the road. "@en ;
    skos:hasTopConcept
        lc:one ,
        lc:two-or-more ,
        lc:unknown ;
    skos:historyNote "This vocabulary was created by the Queensland Spatial Information services." ;
    skos:prefLabel "Road Lane Count"@en ;
    prov:qualifiedAttribution [
            dcat:hadRole isoroles:custodian ;
            prov:agent [
                    a prov:Agent ;
                    rdfs:label "Icsm"
                ]
        ] ;
.

