PREFIX dcterms: <http://purl.org/dc/terms/>
PREFIX dq-iso-19157: <https://linked.data.gov.au/def/iso-19157-data-quality-dimension/>
PREFIX dq-iso-25012: <https://linked.data.gov.au/def/iso-iec-25012-data-quality-dimension/>
PREFIX dqv: <http://www.w3.org/ns/dqv#>
PREFIX rdfs: <http://www.w3.org/2000/01/rdf-schema#>
PREFIX skos: <http://www.w3.org/2004/02/skos/core#>
PREFIX xsd: <http://www.w3.org/2001/XMLSchema#>

dq-iso-25012:accessibility
    a
        skos:Concept ,
        dqv:Dimension ;
    skos:historyNote "Extracted from ISO 25012" ;
    dcterms:source "https://www.w3.org/TR/vocab-dqv/#DimentsionsMetricsHints"^^xsd:anyURI ;
    rdfs:isDefinedBy <https://iso25000.com/index.php/en/iso-25000-standards/iso-25012> ;
    skos:broader dq-iso-25012:inherentSystemDependentDataQuality ;
    skos:definition "The degree to which data can be accessed in a specific context of use, particularly by people who need supporting technology or special configuration because of some disability."@en ;
    skos:inScheme <https://linked.data.gov.au/def/iso-iec-25012-data-quality-dimension> ;
    skos:prefLabel "Accessibility (ISO25012)"@en ;
    dqv:inCategory dq-iso-25012:inherentSystemDependentDataQuality ;
.

dq-iso-25012:accuracy
    a
        skos:Concept ,
        dqv:Dimension ;
    skos:historyNote "Extracted from ISO 25012" ;
    dcterms:source "https://www.w3.org/TR/vocab-dqv/#DimentsionsMetricsHints"^^xsd:anyURI ;
    rdfs:isDefinedBy <https://iso25000.com/index.php/en/iso-25000-standards/iso-25012> ;
    skos:broader dq-iso-25012:inherentDataQuality ;
    skos:closeMatch
        dq-iso-19157:PositionalAccuracy ,
        dq-iso-19157:ThematicAccuracy ;
    skos:definition "The degree to which data has attributes that correctly represent the true value of the intended attribute of a concept or event in a specific context of use."@en ;
    skos:inScheme <https://linked.data.gov.au/def/iso-iec-25012-data-quality-dimension> ;
    skos:prefLabel "Accuracy (ISO25012)"@en ;
    dqv:inCategory dq-iso-25012:inherentDataQuality ;
.

dq-iso-25012:availability
    a
        skos:Concept ,
        dqv:Dimension ;
    skos:historyNote "Extracted from ISO 25012" ;
    dcterms:source "https://www.w3.org/TR/vocab-dqv/#DimentsionsMetricsHints"^^xsd:anyURI ;
    rdfs:isDefinedBy <https://iso25000.com/index.php/en/iso-25000-standards/iso-25012> ;
    skos:broader dq-iso-25012:systemDependentDataQuality ;
    skos:definition "The degree to which data has attributes that enable it to be retrieved by authorized users and/or applications in a specific context of use."@en ;
    skos:inScheme <https://linked.data.gov.au/def/iso-iec-25012-data-quality-dimension> ;
    skos:prefLabel "Availability"@en ;
    dqv:inCategory dq-iso-25012:systemDependentDataQuality ;
.

dq-iso-25012:completeness
    a
        skos:Concept ,
        dqv:Dimension ;
    skos:historyNote "Extracted from ISO 25012" ;
    dcterms:source "https://www.w3.org/TR/vocab-dqv/#DimentsionsMetricsHints"^^xsd:anyURI ;
    rdfs:isDefinedBy <https://iso25000.com/index.php/en/iso-25000-standards/iso-25012> ;
    skos:broader dq-iso-25012:inherentDataQuality ;
    skos:closeMatch dq-iso-19157:completeness ;
    skos:definition "The degree to which subject data associated with an entity has values for all expected attributes and related entity instances in a specific context of use."@en ;
    skos:exactMatch dq-iso-19157:CompletenessOmission ;
    skos:inScheme <https://linked.data.gov.au/def/iso-iec-25012-data-quality-dimension> ;
    skos:prefLabel "Completeness (ISO25012)"@en ;
    dqv:inCategory dq-iso-25012:inherentDataQuality ;
.

dq-iso-25012:compliance
    a
        skos:Concept ,
        dqv:Dimension ;
    skos:historyNote "Extracted from ISO 25012" ;
    dcterms:source "https://www.w3.org/TR/vocab-dqv/#DimentsionsMetricsHints"^^xsd:anyURI ;
    rdfs:isDefinedBy <https://iso25000.com/index.php/en/iso-25000-standards/iso-25012> ;
    skos:broader dq-iso-25012:inherentSystemDependentDataQuality ;
    skos:closeMatch dq-iso-19157:UsabilityElement ;
    skos:definition "The degree to which data has attributes that adhere to standards, conventions or regulations in force and similar rules relating to data quality in a specific context of use."@en ;
    skos:inScheme <https://linked.data.gov.au/def/iso-iec-25012-data-quality-dimension> ;
    skos:prefLabel "Compliance"@en ;
    dqv:inCategory dq-iso-25012:inherentSystemDependentDataQuality ;
.

dq-iso-25012:confidentiality
    a
        skos:Concept ,
        dqv:Dimension ;
    skos:historyNote "Extracted from ISO 25012" ;
    dcterms:source "https://www.w3.org/TR/vocab-dqv/#DimentsionsMetricsHints"^^xsd:anyURI ;
    rdfs:isDefinedBy <https://iso25000.com/index.php/en/iso-25000-standards/iso-25012> ;
    skos:broader dq-iso-25012:inherentSystemDependentDataQuality ;
    skos:definition "The degree to which data has attributes that ensure that it is only accessible and interpretable by authorized users in a specific context of use. Confidentiality is an aspect of information security (together with availability, integrity) as defined in ISO/IEC 13335-1:2004."@en ;
    skos:inScheme <https://linked.data.gov.au/def/iso-iec-25012-data-quality-dimension> ;
    skos:prefLabel "Confidentiality"@en ;
    dqv:inCategory dq-iso-25012:inherentSystemDependentDataQuality ;
.

dq-iso-25012:consistency
    a
        skos:Concept ,
        dqv:Dimension ;
    skos:historyNote "Extracted from ISO 25012" ;
    dcterms:source "https://www.w3.org/TR/vocab-dqv/#DimentsionsMetricsHints"^^xsd:anyURI ;
    rdfs:isDefinedBy <https://iso25000.com/index.php/en/iso-25000-standards/iso-25012> ;
    skos:broader dq-iso-25012:inherentDataQuality ;
    skos:closeMatch dq-iso-19157:LogicalConsistency ;
    skos:definition "The degree to which data has attributes that are free from contradiction and are coherent with other data in a specific context of use. It can be either or both among data regarding one entity and across similar data for comparable entities."@en ;
    skos:inScheme <https://linked.data.gov.au/def/iso-iec-25012-data-quality-dimension> ;
    skos:prefLabel "Consistency"@en ;
    dqv:inCategory dq-iso-25012:inherentDataQuality ;
.

dq-iso-25012:credibility
    a
        skos:Concept ,
        dqv:Dimension ;
    skos:historyNote "Extracted from ISO 25012" ;
    dcterms:source "https://www.w3.org/TR/vocab-dqv/#DimentsionsMetricsHints"^^xsd:anyURI ;
    rdfs:isDefinedBy <https://iso25000.com/index.php/en/iso-25000-standards/iso-25012> ;
    skos:broader dq-iso-25012:inherentDataQuality ;
    skos:definition "The degree to which data has attributes that are regarded as true and believable by users in a specific context of use. Credibility includes the concept of authenticity (the truthfulness of origins, attributions, commitments)."@en ;
    skos:inScheme <https://linked.data.gov.au/def/iso-iec-25012-data-quality-dimension> ;
    skos:prefLabel "Credibility"@en ;
    dqv:inCategory dq-iso-25012:inherentDataQuality ;
.

dq-iso-25012:currentness
    a
        skos:Concept ,
        dqv:Dimension ;
    skos:historyNote "Extracted from ISO 25012" ;
    dcterms:source "https://www.w3.org/TR/vocab-dqv/#DimentsionsMetricsHints"^^xsd:anyURI ;
    rdfs:isDefinedBy <https://iso25000.com/index.php/en/iso-25000-standards/iso-25012> ;
    skos:broader dq-iso-25012:inherentDataQuality ;
    skos:definition "The degree to which data has attributes that are of the right age in a specific context of use."@en ;
    skos:inScheme <https://linked.data.gov.au/def/iso-iec-25012-data-quality-dimension> ;
    skos:prefLabel "Currentness"@en ;
    dqv:inCategory dq-iso-25012:inherentDataQuality ;
.

dq-iso-25012:efficiency
    a
        skos:Concept ,
        dqv:Dimension ;
    skos:historyNote "Extracted from ISO 25012" ;
    dcterms:source "https://www.w3.org/TR/vocab-dqv/#DimentsionsMetricsHints"^^xsd:anyURI ;
    rdfs:isDefinedBy <https://iso25000.com/index.php/en/iso-25000-standards/iso-25012> ;
    skos:broader dq-iso-25012:inherentSystemDependentDataQuality ;
    skos:definition "The degree to which data has attributes that can be processed and provide the expected levels of performance by using the appropriate amounts and types of resources in a specific context of use."@en ;
    skos:inScheme <https://linked.data.gov.au/def/iso-iec-25012-data-quality-dimension> ;
    skos:prefLabel "Efficiency"@en ;
    dqv:inCategory dq-iso-25012:inherentSystemDependentDataQuality ;
.

dq-iso-25012:portability
    a
        skos:Concept ,
        dqv:Dimension ;
    skos:historyNote "Extracted from ISO 25012" ;
    dcterms:source "https://www.w3.org/TR/vocab-dqv/#DimentsionsMetricsHints"^^xsd:anyURI ;
    rdfs:isDefinedBy <https://iso25000.com/index.php/en/iso-25000-standards/iso-25012> ;
    skos:broader dq-iso-25012:systemDependentDataQuality ;
    skos:definition "The degree to which data has attributes that enable it to be installed, replaced or moved from one system to another preserving the existing quality in a specific context of use."@en ;
    skos:inScheme <https://linked.data.gov.au/def/iso-iec-25012-data-quality-dimension> ;
    skos:prefLabel "Portability"@en ;
    dqv:inCategory dq-iso-25012:systemDependentDataQuality ;
.

dq-iso-25012:precision
    a
        skos:Concept ,
        dqv:Dimension ;
    skos:historyNote "Extracted from ISO 25012" ;
    dcterms:source "https://www.w3.org/TR/vocab-dqv/#DimentsionsMetricsHints"^^xsd:anyURI ;
    rdfs:isDefinedBy <https://iso25000.com/index.php/en/iso-25000-standards/iso-25012> ;
    skos:broader dq-iso-25012:inherentSystemDependentDataQuality ;
    skos:closeMatch dq-iso-19157:ThematicAccuracy ;
    skos:definition "The degree to which data has attributes that are exact or that provide discrimination in a specific context of use."@en ;
    skos:inScheme <https://linked.data.gov.au/def/iso-iec-25012-data-quality-dimension> ;
    skos:prefLabel "Precision"@en ;
    dqv:inCategory dq-iso-25012:inherentSystemDependentDataQuality ;
.

dq-iso-25012:recoverability
    a
        skos:Concept ,
        dqv:Dimension ;
    skos:historyNote "Extracted from ISO 25012" ;
    dcterms:source "https://www.w3.org/TR/vocab-dqv/#DimentsionsMetricsHints"^^xsd:anyURI ;
    rdfs:isDefinedBy <https://iso25000.com/index.php/en/iso-25000-standards/iso-25012> ;
    skos:broader dq-iso-25012:systemDependentDataQuality ;
    skos:definition "The degree to which data has attributes that enable it to maintain and preserve a specified level of operations and quality, even in the event of failure, in a specific context of use."@en ;
    skos:inScheme <https://linked.data.gov.au/def/iso-iec-25012-data-quality-dimension> ;
    skos:prefLabel "Recoverability"@en ;
    dqv:inCategory dq-iso-25012:systemDependentDataQuality ;
.

dq-iso-25012:traceability
    a
        skos:Concept ,
        dqv:Dimension ;
    skos:historyNote "Extracted from ISO 25012" ;
    dcterms:source "https://www.w3.org/TR/vocab-dqv/#DimentsionsMetricsHints"^^xsd:anyURI ;
    rdfs:isDefinedBy <https://iso25000.com/index.php/en/iso-25000-standards/iso-25012> ;
    skos:broader dq-iso-25012:inherentSystemDependentDataQuality ;
    skos:definition "The degree to which data has attributes that provide an audit trail of access to the data and of any changes made to the data in a specific context of use."@en ;
    skos:inScheme <https://linked.data.gov.au/def/iso-iec-25012-data-quality-dimension> ;
    skos:prefLabel "Traceability"@en ;
    dqv:inCategory dq-iso-25012:inherentSystemDependentDataQuality ;
.

dq-iso-25012:understandability
    a
        skos:Concept ,
        dqv:Dimension ;
    skos:historyNote "Extracted from ISO 25012" ;
    dcterms:source "https://www.w3.org/TR/vocab-dqv/#DimentsionsMetricsHints"^^xsd:anyURI ;
    rdfs:isDefinedBy <https://iso25000.com/index.php/en/iso-25000-standards/iso-25012> ;
    skos:broader dq-iso-25012:inherentSystemDependentDataQuality ;
    skos:definition "The degree to which data has attributes that enable it to be read and interpreted by users, and are expressed in appropriate languages, symbols and units in a specific context of use. Some information about data understandability are provided by metadata."@en ;
    skos:inScheme <https://linked.data.gov.au/def/iso-iec-25012-data-quality-dimension> ;
    skos:prefLabel "Understandability"@en ;
    dqv:inCategory dq-iso-25012:inherentSystemDependentDataQuality ;
.

dq-iso-25012:systemDependentDataQuality
    a
        skos:Concept ,
        dqv:Category ;
    rdfs:label "System-dependent data quality"@en ;
    skos:historyNote "Extracted from ISO 25012" ;
    dcterms:source "https://www.w3.org/TR/vocab-dqv/#DimentsionsMetricsHints"^^xsd:anyURI ;
    rdfs:isDefinedBy <https://iso25000.com/index.php/en/iso-25000-standards/iso-25012> ;
    skos:definition "System dependent data quality refers to the degree to which data quality is reached and preserved within a computer system when data is used under specified conditions."@en ;
    skos:inScheme <https://linked.data.gov.au/def/iso-iec-25012-data-quality-dimension> ;
    skos:prefLabel "System-Dependent Data Quality"@en ;
    skos:topConceptOf <https://linked.data.gov.au/def/iso-iec-25012-data-quality-dimension> ;
.

dq-iso-25012:inherentDataQuality
    a
        skos:Concept ,
        dqv:Category ;
    skos:historyNote "Extracted from ISO 25012" ;
    dcterms:source "https://www.w3.org/TR/vocab-dqv/#DimentsionsMetricsHints"^^xsd:anyURI ;
    rdfs:isDefinedBy <https://iso25000.com/index.php/en/iso-25000-standards/iso-25012> ;
    skos:definition "Inherent data quality refers to the degree to which quality characteristics of data have the intrinsic potential to satisfy stated and implied needs when data is used under specified conditions."@en ;
    skos:inScheme <https://linked.data.gov.au/def/iso-iec-25012-data-quality-dimension> ;
    skos:prefLabel "Inherent data quality"@en ;
    skos:topConceptOf <https://linked.data.gov.au/def/iso-iec-25012-data-quality-dimension> ;
.

dq-iso-25012:inherentSystemDependentDataQuality
    a
        skos:Concept ,
        dqv:Category ;
    skos:historyNote "Extracted from ISO 25012" ;
    dcterms:source "https://www.w3.org/TR/vocab-dqv/#DimentsionsMetricsHints"^^xsd:anyURI ;
    rdfs:isDefinedBy <https://iso25000.com/index.php/en/iso-25000-standards/iso-25012> ;
    skos:definition "Data quality that is both in the inherent and system-dependent quality categories, inherent referes to the degree to which data has the intrinsic potential to satisfy needs and system-dependent is about the quality which is preserved by the system it is contained within."@en ;
    skos:inScheme <https://linked.data.gov.au/def/iso-iec-25012-data-quality-dimension> ;
    skos:prefLabel "Inherent and System-Dependent Data Quality"@en ;
    skos:related
        dq-iso-25012:inherentDataQuality ,
        dq-iso-25012:systemDependentDataQuality ;
    skos:topConceptOf <https://linked.data.gov.au/def/iso-iec-25012-data-quality-dimension> ;
.

<https://linked.data.gov.au/def/iso-iec-25012-data-quality-dimension>
    a skos:ConceptScheme ;
    dcterms:created "2020-11-16"^^xsd:date ;
    dcterms:creator <https://linked.data.gov.au/def/gsq-alias/des> ;
    dcterms:modified "2023-03-10"^^xsd:date ;
    skos:historyNote "Extracted from ISO 25012" ;
    dcterms:publisher <https://linked.data.gov.au/def/gsq-alias/gsq> ;
    skos:definition "ISO25012 Data Quality Dimensions, as extracted from the standard"@en ;
    skos:hasTopConcept
        dq-iso-25012:inherentDataQuality ,
        dq-iso-25012:inherentSystemDependentDataQuality ,
        dq-iso-25012:systemDependentDataQuality ;
    skos:prefLabel "ISO25012 Data Quality Dimensions"@en ;
.

