PREFIX dcterms: <http://purl.org/dc/terms/>
PREFIX dq-iso-19157: <https://linked.data.gov.au/def/iso-19157-data-quality-dimension/>
PREFIX dq-iso-25012: <https://linked.data.gov.au/def/iso-iec-25012-data-quality-dimension/>
PREFIX dqv: <http://www.w3.org/ns/dqv#>
PREFIX rdfs: <http://www.w3.org/2000/01/rdf-schema#>
PREFIX skos: <http://www.w3.org/2004/02/skos/core#>
PREFIX xsd: <http://www.w3.org/2001/XMLSchema#>

dq-iso-19157:AbsoluteExternalPositionalAccuracy
    a
        skos:Concept ,
        dqv:Dimension ;
    skos:historyNote "ISO 19157" ;
    rdfs:isDefinedBy <https://www.iso.org/standard/32575.html> ;
    skos:broader dq-iso-19157:PositionalAccuracy ;
    skos:definition "Closeness of reported coordinate values to values accepted as or being true"@en ;
    skos:inScheme <https://linked.data.gov.au/def/iso-19157-data-quality-dimension> ;
    skos:prefLabel "Absolute External Positional Accuracy"@en ;
.

dq-iso-19157:AccuracyOfATimeMeasurement
    a
        skos:Concept ,
        dqv:Dimension ;
    skos:historyNote "ISO 19157" ;
    rdfs:isDefinedBy <https://www.iso.org/standard/32575.html> ;
    skos:broader dq-iso-19157:TemporalQuality ;
    skos:definition "Correctness of the temporal references of an item (reporting of error in time measurement)"@en ;
    skos:inScheme <https://linked.data.gov.au/def/iso-19157-data-quality-dimension> ;
    skos:prefLabel "Accuracy of a Time Measurement"@en ;
.

dq-iso-19157:CompletenessCommission
    a
        skos:Concept ,
        dqv:Dimension ;
    skos:historyNote "ISO 19157" ;
    rdfs:isDefinedBy <https://www.iso.org/standard/32575.html> ;
    skos:broader dq-iso-19157:Completeness ;
    skos:definition "Excess data present in the data set, as described by the scope"@en ;
    skos:inScheme <https://linked.data.gov.au/def/iso-19157-data-quality-dimension> ;
    skos:prefLabel "Completeness Commission"@en ;
.

dq-iso-19157:CompletenessOmission
    a
        skos:Concept ,
        dqv:Dimension ;
    skos:historyNote "ISO 19157" ;
    rdfs:isDefinedBy <https://www.iso.org/standard/32575.html> ;
    skos:broader dq-iso-19157:Completeness ;
    skos:definition "Data absent from the data set, as described by the scope"@en ;
    skos:exactMatch dq-iso-25012:completeness ;
    skos:inScheme <https://linked.data.gov.au/def/iso-19157-data-quality-dimension> ;
    skos:prefLabel "Completeness Omission"@en ;
.

dq-iso-19157:ConceptualConsistency
    a
        skos:Concept ,
        dqv:Dimension ;
    skos:historyNote "ISO 19157" ;
    rdfs:isDefinedBy <https://www.iso.org/standard/32575.html> ;
    skos:broader dq-iso-19157:LogicalConsistency ;
    skos:definition "Adherence to rules of the conceptual schema"@en ;
    skos:inScheme <https://linked.data.gov.au/def/iso-19157-data-quality-dimension> ;
    skos:prefLabel "Conceptual Consistency"@en ;
.

dq-iso-19157:Confidence
    a
        skos:Concept ,
        dqv:Dimension ;
    skos:historyNote "ISO 19157" ;
    rdfs:isDefinedBy <https://www.iso.org/standard/32575.html> ;
    skos:broader dq-iso-19157:Metaquality ;
    skos:definition "Trustworthiness of a data quality result "@en ;
    skos:inScheme <https://linked.data.gov.au/def/iso-19157-data-quality-dimension> ;
    skos:prefLabel "Confidence"@en ;
.

dq-iso-19157:DomainConsistency
    a
        skos:Concept ,
        dqv:Dimension ;
    skos:historyNote "ISO 19157" ;
    rdfs:isDefinedBy <https://www.iso.org/standard/32575.html> ;
    skos:broader dq-iso-19157:LogicalConsistency ;
    skos:definition "Adherence of values to the value domains"@en ;
    skos:inScheme <https://linked.data.gov.au/def/iso-19157-data-quality-dimension> ;
    skos:prefLabel "Domain Consistency"@en ;
.

dq-iso-19157:FormatConsistency
    a
        skos:Concept ,
        dqv:Dimension ;
    skos:historyNote "ISO 19157" ;
    rdfs:isDefinedBy <https://www.iso.org/standard/32575.html> ;
    skos:broader dq-iso-19157:LogicalConsistency ;
    skos:definition "Degree to which data are stored in accordance with the physical structure of the data set, as described by the scope"@en ;
    skos:inScheme <https://linked.data.gov.au/def/iso-19157-data-quality-dimension> ;
    skos:prefLabel "Format Consistency"@en ;
.

dq-iso-19157:GriddedDataPositionalAccuracy
    a
        skos:Concept ,
        dqv:Dimension ;
    skos:historyNote "ISO 19157" ;
    rdfs:isDefinedBy <https://www.iso.org/standard/32575.html> ;
    skos:broader dq-iso-19157:PositionalAccuracy ;
    skos:definition "Closeness of gridded data position values to values accepted as or being true"@en ;
    skos:inScheme <https://linked.data.gov.au/def/iso-19157-data-quality-dimension> ;
    skos:prefLabel "Gridded Data Positional Accuracy"@en ;
.

dq-iso-19157:Homogeneity
    a
        skos:Concept ,
        dqv:Dimension ;
    skos:historyNote "ISO 19157" ;
    rdfs:isDefinedBy <https://www.iso.org/standard/32575.html> ;
    skos:broader dq-iso-19157:Metaquality ;
    skos:definition "Expected or tested uniformity of the results obtained for a data quality evaluation"@en ;
    skos:inScheme <https://linked.data.gov.au/def/iso-19157-data-quality-dimension> ;
    skos:prefLabel "Homogeneity"@en ;
.

dq-iso-19157:NonQuantitativeAttributeCorrectness
    a
        skos:Concept ,
        dqv:Dimension ;
    skos:historyNote "ISO 19157" ;
    rdfs:isDefinedBy <https://www.iso.org/standard/32575.html> ;
    skos:broader dq-iso-19157:ThematicAccuracy ;
    skos:definition "Correctness of non-quantitative attributes"@en ;
    skos:inScheme <https://linked.data.gov.au/def/iso-19157-data-quality-dimension> ;
    skos:prefLabel "NonQuantitative Attribute Correctness"@en ;
.

dq-iso-19157:QuantitativeAttributeAccuracy
    a
        skos:Concept ,
        dqv:Dimension ;
    skos:historyNote "ISO 19157" ;
    rdfs:isDefinedBy <https://www.iso.org/standard/32575.html> ;
    skos:broader dq-iso-19157:ThematicAccuracy ;
    skos:definition "Accuracy of quantitative attributes"@en ;
    skos:inScheme <https://linked.data.gov.au/def/iso-19157-data-quality-dimension> ;
    skos:prefLabel "Quantitative Attribute Accuracy"@en ;
.

dq-iso-19157:RelativeInternalPositionalAccuracy
    a
        skos:Concept ,
        dqv:Dimension ;
    skos:historyNote "ISO 19157" ;
    rdfs:isDefinedBy <https://www.iso.org/standard/32575.html> ;
    skos:broader dq-iso-19157:PositionalAccuracy ;
    skos:definition "Closeness of the relative positions of features in the scope to their respective relative positions accepted as or being true"@en ;
    skos:inScheme <https://linked.data.gov.au/def/iso-19157-data-quality-dimension> ;
    skos:prefLabel "Relative Internal Positional Accuracy"@en ;
.

dq-iso-19157:Representativity
    a
        skos:Concept ,
        dqv:Dimension ;
    skos:historyNote "ISO 19157" ;
    rdfs:isDefinedBy <https://www.iso.org/standard/32575.html> ;
    skos:broader dq-iso-19157:Metaquality ;
    skos:definition "Degree to which the sample used has produced a result which is representative of the data within the data quality scope "@en ;
    skos:inScheme <https://linked.data.gov.au/def/iso-19157-data-quality-dimension> ;
    skos:prefLabel "Representativity "@en ;
.

dq-iso-19157:TemporalConsistency
    a
        skos:Concept ,
        dqv:Dimension ;
    skos:historyNote "ISO 19157" ;
    rdfs:isDefinedBy <https://www.iso.org/standard/32575.html> ;
    skos:broader dq-iso-19157:TemporalQuality ;
    skos:definition "Correctness of ordered events or sequences, if reported"@en ;
    skos:inScheme <https://linked.data.gov.au/def/iso-19157-data-quality-dimension> ;
    skos:prefLabel "Temporal Consistency"@en ;
.

dq-iso-19157:TemporalValidity
    a
        skos:Concept ,
        dqv:Dimension ;
    skos:historyNote "ISO 19157" ;
    rdfs:isDefinedBy <https://www.iso.org/standard/32575.html> ;
    skos:broader dq-iso-19157:TemporalQuality ;
    skos:definition "Validity of data specified by the scope with respect to time"@en ;
    skos:inScheme <https://linked.data.gov.au/def/iso-19157-data-quality-dimension> ;
    skos:prefLabel "Temporal Validity"@en ;
.

dq-iso-19157:ThematicClassificationCorrectness
    a
        skos:Concept ,
        dqv:Dimension ;
    skos:historyNote "ISO 19157" ;
    rdfs:isDefinedBy <https://www.iso.org/standard/32575.html> ;
    skos:broader dq-iso-19157:ThematicAccuracy ;
    skos:definition "Comparison of the classes assigned to features or their attributes to a universe of discourse"@en ;
    skos:inScheme <https://linked.data.gov.au/def/iso-19157-data-quality-dimension> ;
    skos:prefLabel "Thematic Classification Correctness"@en ;
.

dq-iso-19157:TopologicalConsistency
    a
        skos:Concept ,
        dqv:Dimension ;
    skos:historyNote "ISO 19157" ;
    rdfs:isDefinedBy <https://www.iso.org/standard/32575.html> ;
    skos:broader dq-iso-19157:LogicalConsistency ;
    skos:definition "Correctness of the explicitly encoded topological characteristics of the data set as described by the scope"@en ;
    skos:inScheme <https://linked.data.gov.au/def/iso-19157-data-quality-dimension> ;
    skos:prefLabel "Topological Consistency"@en ;
.

dq-iso-19157:UsabilityElement
    a
        skos:Concept ,
        dqv:Dimension ;
    skos:historyNote "ISO 19157" ;
    rdfs:isDefinedBy <https://www.iso.org/standard/32575.html> ;
    skos:closeMatch dq-iso-25012:compliance ;
    skos:definition "Degree of adherence of a data set to a specific set of requirements"@en ;
    skos:inScheme <https://linked.data.gov.au/def/iso-19157-data-quality-dimension> ;
    skos:prefLabel "Usability Element"@en ;
    skos:topConceptOf <https://linked.data.gov.au/def/iso-19157-data-quality-dimension> ;
.

dq-iso-19157:Completeness
    a
        skos:Concept ,
        dqv:Dimension ;
    skos:historyNote "ISO 19157" ;
    rdfs:isDefinedBy <https://www.iso.org/standard/32575.html> ;
    skos:closeMatch dq-iso-25012:completeness ;
    skos:definition "Presence and absence of features, their attributes and their relationships"@en ;
    skos:inScheme <https://linked.data.gov.au/def/iso-19157-data-quality-dimension> ;
    skos:prefLabel "Completeness (ISO19157)"@en ;
    skos:topConceptOf <https://linked.data.gov.au/def/iso-19157-data-quality-dimension> ;
.

dq-iso-19157:Metaquality
    a
        skos:Concept ,
        dqv:Dimension ;
    skos:historyNote "ISO 19157" ;
    rdfs:isDefinedBy <https://www.iso.org/standard/32575.html> ;
    skos:definition "Information about the reliability of data quality results Use obligation from referencing object"@en ;
    skos:inScheme <https://linked.data.gov.au/def/iso-19157-data-quality-dimension> ;
    skos:prefLabel "Metaquality"@en ;
    skos:topConceptOf <https://linked.data.gov.au/def/iso-19157-data-quality-dimension> ;
.

dq-iso-19157:PositionalAccuracy
    a
        skos:Concept ,
        dqv:Dimension ;
    skos:historyNote "ISO 19157" ;
    rdfs:isDefinedBy <https://www.iso.org/standard/32575.html> ;
    skos:closeMatch dq-iso-25012:accuracy ;
    skos:definition "Accuracy of the position of features"@en ;
    skos:inScheme <https://linked.data.gov.au/def/iso-19157-data-quality-dimension> ;
    skos:prefLabel "Positional Accuracy"@en ;
    skos:topConceptOf <https://linked.data.gov.au/def/iso-19157-data-quality-dimension> ;
.

dq-iso-19157:TemporalQuality
    a
        skos:Concept ,
        dqv:Dimension ;
    skos:historyNote "ISO 19157" ;
    rdfs:isDefinedBy <https://www.iso.org/standard/32575.html> ;
    skos:definition "Accuracy of the temporal attributes and temporal relationships of features"@en ;
    skos:inScheme <https://linked.data.gov.au/def/iso-19157-data-quality-dimension> ;
    skos:prefLabel "Temporal Quality"@en ;
    skos:topConceptOf <https://linked.data.gov.au/def/iso-19157-data-quality-dimension> ;
.

dq-iso-19157:ThematicAccuracy
    a
        skos:Concept ,
        dqv:Dimension ;
    skos:historyNote "ISO 19157" ;
    rdfs:isDefinedBy <https://www.iso.org/standard/32575.html> ;
    skos:closeMatch dq-iso-25012:accuracy ;
    skos:definition "Accuracy of quantitative attributes and the correctness of non-quantitative attributes and of the classifications of features and their relationships"@en ;
    skos:inScheme <https://linked.data.gov.au/def/iso-19157-data-quality-dimension> ;
    skos:prefLabel "Thematic Accuracy"@en ;
    skos:relatedMatch dq-iso-25012:precision ;
    skos:topConceptOf <https://linked.data.gov.au/def/iso-19157-data-quality-dimension> ;
.

dq-iso-19157:LogicalConsistency
    a
        skos:Concept ,
        dqv:Dimension ;
    skos:historyNote "ISO 19157" ;
    rdfs:isDefinedBy <https://www.iso.org/standard/32575.html> ;
    skos:closeMatch dq-iso-25012:consistency ;
    skos:definition "Degree of adherence to logical rules of data structure, attribution and relationships (data structure can be conceptual, logical or physical)"@en ;
    skos:inScheme <https://linked.data.gov.au/def/iso-19157-data-quality-dimension> ;
    skos:prefLabel "Logical Consistency"@en ;
    skos:topConceptOf <https://linked.data.gov.au/def/iso-19157-data-quality-dimension> ;
.

<https://linked.data.gov.au/def/iso-19157-data-quality-dimension>
    a skos:ConceptScheme ;
    dcterms:created "2020-11-16"^^xsd:date ;
    dcterms:creator <https://linked.data.gov.au/org/des> ;
    dcterms:modified "2023-03-10"^^xsd:date ;
    skos:historyNote "ISO 19157" ;
    dcterms:publisher <https://linked.data.gov.au/org/des> ;
    skos:definition "Data quality criteria as defined in ISO19157."@en ;
    skos:hasTopConcept
        dq-iso-19157:Completeness ,
        dq-iso-19157:LogicalConsistency ,
        dq-iso-19157:Metaquality ,
        dq-iso-19157:PositionalAccuracy ,
        dq-iso-19157:TemporalQuality ,
        dq-iso-19157:ThematicAccuracy ,
        dq-iso-19157:UsabilityElement ;
    skos:prefLabel "ISO19157 Data Quality Dimensions"@en ;
.

