PREFIX dcterms: <http://purl.org/dc/terms/>
PREFIX dq-nsw: <https://linked.data.gov.au/def/nsw-quality-dimension/>
PREFIX dqv: <http://www.w3.org/ns/dqv#>
PREFIX rdfs: <http://www.w3.org/2000/01/rdf-schema#>
PREFIX sdo: <http://www.schema.org/>
PREFIX skos: <http://www.w3.org/2004/02/skos/core#>
PREFIX xsd: <http://www.w3.org/2001/XMLSchema#>

dq-nsw:assurance
    a
        skos:Concept ,
        dqv:Dimension ;
    dcterms:provenance "NSW Government Standard for Data Quality Reporting. https://data.nsw.gov.au/data-quality-reporting-tool" ;
    rdfs:isDefinedBy <https://linked.data.gov.au/def/nsw-quality-dimension> ;
    skos:broader dq-nsw:accuracy ;
    skos:definition "This data has been subject to quality assurance processes. ie Checking for errors at each stage of data collection and processing, or verifying data entry and making corrections if necessary."@en ;
    skos:inScheme <https://linked.data.gov.au/def/nsw-quality-dimension> ;
    skos:prefLabel "Data assurance"@en ;
    dqv:inCategory dq-nsw:accuracy ;
.

dq-nsw:authorized
    a
        skos:Concept ,
        dqv:Dimension ;
    dcterms:provenance "NSW Government Standard for Data Quality Reporting. https://data.nsw.gov.au/data-quality-reporting-tool" ;
    rdfs:isDefinedBy <https://linked.data.gov.au/def/nsw-quality-dimension> ;
    skos:broader dq-nsw:institutional-environment ;
    skos:definition "Data collection is mandated or required by a law, regulation or agreement"@en ;
    skos:inScheme <https://linked.data.gov.au/def/nsw-quality-dimension> ;
    skos:prefLabel "Authorized data collection"@en ;
    dqv:inCategory dq-nsw:institutional-environment ;
.

dq-nsw:comparable
    a
        skos:Concept ,
        dqv:Dimension ;
    dcterms:provenance "NSW Government Standard for Data Quality Reporting. https://data.nsw.gov.au/data-quality-reporting-tool" ;
    rdfs:isDefinedBy <https://linked.data.gov.au/def/nsw-quality-dimension> ;
    skos:broader dq-nsw:coherence ;
    skos:definition "Elements within the data can be meaningfully compared."@en ;
    skos:inScheme <https://linked.data.gov.au/def/nsw-quality-dimension> ;
    skos:prefLabel "Elements can be compared"@en ;
    dqv:inCategory dq-nsw:coherence ;
.

dq-nsw:complete
    a
        skos:Concept ,
        dqv:Dimension ;
    dcterms:provenance "NSW Government Standard for Data Quality Reporting. https://data.nsw.gov.au/data-quality-reporting-tool" ;
    rdfs:isDefinedBy <https://linked.data.gov.au/def/nsw-quality-dimension> ;
    skos:broader dq-nsw:accuracy ;
    skos:definition "There are no known gaps in the data. (For example: non-responses, missing records, data not collected.). Or gaps are identified in caveats attached to the dataset or data source."@en ;
    skos:inScheme <https://linked.data.gov.au/def/nsw-quality-dimension> ;
    skos:prefLabel "Data complete"@en ;
    dqv:inCategory dq-nsw:accuracy ;
.

dq-nsw:concepts
    a
        skos:Concept ,
        dqv:Dimension ;
    dcterms:provenance "NSW Government Standard for Data Quality Reporting. https://data.nsw.gov.au/data-quality-reporting-tool" ;
    rdfs:comment "Find out more about concepts used in this dataset and how to understand or interpret the data from the Custodian."@en ;
    rdfs:isDefinedBy <https://linked.data.gov.au/def/nsw-quality-dimension> ;
    skos:broader dq-nsw:interpretability ;
    skos:definition "Information is available to explain concepts, help users correctly interpret the data and understand how it can be used."@en ;
    skos:inScheme <https://linked.data.gov.au/def/nsw-quality-dimension> ;
    skos:prefLabel "Concept explanations"@en ;
    dqv:inCategory dq-nsw:interpretability ;
.

dq-nsw:consistent
    a
        skos:Concept ,
        dqv:Dimension ;
    dcterms:provenance "NSW Government Standard for Data Quality Reporting. https://data.nsw.gov.au/data-quality-reporting-tool" ;
    rdfs:isDefinedBy <https://linked.data.gov.au/def/nsw-quality-dimension> ;
    skos:broader dq-nsw:coherence ;
    skos:definition "This data is generally consistent with similar or related data sources."@en ;
    skos:inScheme <https://linked.data.gov.au/def/nsw-quality-dimension> ;
    skos:prefLabel "Consistent with related datasets"@en ;
    dqv:inCategory dq-nsw:coherence ;
.

dq-nsw:custodian
    a
        skos:Concept ,
        dqv:Dimension ;
    dcterms:provenance "NSW Government Standard for Data Quality Reporting. https://data.nsw.gov.au/data-quality-reporting-tool" ;
    rdfs:isDefinedBy <https://linked.data.gov.au/def/nsw-quality-dimension> ;
    skos:broader dq-nsw:institutional-environment ;
    skos:definition "Agency publishing this data is the recognised data custodian."@en ;
    skos:inScheme <https://linked.data.gov.au/def/nsw-quality-dimension> ;
    skos:prefLabel "Custodian"@en ;
    dqv:inCategory dq-nsw:institutional-environment ;
.

dq-nsw:data-dictionary
    a
        skos:Concept ,
        dqv:Dimension ;
    dcterms:provenance "NSW Government Standard for Data Quality Reporting. https://data.nsw.gov.au/data-quality-reporting-tool" ;
    rdfs:comment "Find out more about the data dictionary from the Custodian."@en ;
    rdfs:isDefinedBy <https://linked.data.gov.au/def/nsw-quality-dimension> ;
    skos:broader dq-nsw:interpretability ;
    skos:definition "A data dictionary is available to explain the meaning of data elements, their origin, format and relationships."@en ;
    skos:inScheme <https://linked.data.gov.au/def/nsw-quality-dimension> ;
    skos:prefLabel "Data dictionary provided"@en ;
    dqv:inCategory dq-nsw:interpretability ;
.

dq-nsw:data-quality-framework
    a
        skos:Concept ,
        dqv:Dimension ;
    dcterms:provenance "NSW Government Standard for Data Quality Reporting. https://data.nsw.gov.au/data-quality-reporting-tool" ;
    rdfs:isDefinedBy <https://linked.data.gov.au/def/nsw-quality-dimension> ;
    skos:broader dq-nsw:institutional-environment ;
    skos:definition "Data is collected and managed according to a data quality framework."@en ;
    skos:inScheme <https://linked.data.gov.au/def/nsw-quality-dimension> ;
    skos:prefLabel "Data quality framework"@en ;
    dqv:inCategory dq-nsw:institutional-environment ;
.

dq-nsw:evaluation
    a
        skos:Concept ,
        dqv:Dimension ;
    dcterms:provenance "NSW Government Standard for Data Quality Reporting. https://data.nsw.gov.au/data-quality-reporting-tool" ;
    rdfs:isDefinedBy <https://linked.data.gov.au/def/nsw-quality-dimension> ;
    skos:broader dq-nsw:interpretability ;
    skos:definition "Information is available to help users evaluate the accuracy of the data and any level of error."@en ;
    skos:inScheme <https://linked.data.gov.au/def/nsw-quality-dimension> ;
    skos:prefLabel "Accuracy evaluation"@en ;
    dqv:inCategory dq-nsw:interpretability ;
.

dq-nsw:governance
    a
        skos:Concept ,
        dqv:Dimension ;
    dcterms:provenance "NSW Government Standard for Data Quality Reporting. https://data.nsw.gov.au/data-quality-reporting-tool" ;
    rdfs:isDefinedBy <https://linked.data.gov.au/def/nsw-quality-dimension> ;
    skos:broader dq-nsw:institutional-environment ;
    skos:definition "Data governance roles and responsibilities are clearly assigned for this dataset or data source."@en ;
    skos:inScheme <https://linked.data.gov.au/def/nsw-quality-dimension> ;
    skos:prefLabel "governance roles"@en ;
    dqv:inCategory dq-nsw:institutional-environment ;
.

dq-nsw:license
    a
        skos:Concept ,
        dqv:Dimension ;
    dcterms:provenance "NSW Government Standard for Data Quality Reporting. https://data.nsw.gov.au/data-quality-reporting-tool" ;
    rdfs:isDefinedBy <https://linked.data.gov.au/def/nsw-quality-dimension> ;
    skos:broader dq-nsw:accessibility ;
    skos:definition "This dataset or data source is available online with an open licence."@en ;
    skos:inScheme <https://linked.data.gov.au/def/nsw-quality-dimension> ;
    skos:prefLabel "Open license"@en ;
    dqv:inCategory dq-nsw:accessibility ;
.

dq-nsw:linked
    a
        skos:Concept ,
        dqv:Dimension ;
    dcterms:provenance "NSW Government Standard for Data Quality Reporting. https://data.nsw.gov.au/data-quality-reporting-tool" ;
    rdfs:isDefinedBy <https://linked.data.gov.au/def/nsw-quality-dimension> ;
    skos:broader dq-nsw:accessibility ;
    skos:definition "This dataset or data source is linked to other data, to provide context."@en ;
    skos:inScheme <https://linked.data.gov.au/def/nsw-quality-dimension> ;
    skos:prefLabel "Links to data and context"@en ;
    dqv:inCategory dq-nsw:accessibility ;
.

dq-nsw:methodology
    a
        skos:Concept ,
        dqv:Dimension ;
    dcterms:provenance "NSW Government Standard for Data Quality Reporting. https://data.nsw.gov.au/data-quality-reporting-tool" ;
    rdfs:isDefinedBy <https://linked.data.gov.au/def/nsw-quality-dimension> ;
    skos:broader dq-nsw:coherence ;
    skos:definition "This dataset is a single collection. It is not impacted by changes in methodology or external events over time. Or this data is part of a time series. There have not been any significant changes in the way data items are defined, classified or counted since the start of the series."@en ;
    skos:inScheme <https://linked.data.gov.au/def/nsw-quality-dimension> ;
    skos:prefLabel "Consistent methodology"@en ;
    dqv:inCategory dq-nsw:coherence ;
.

dq-nsw:no-changes
    a
        skos:Concept ,
        dqv:Dimension ;
    dcterms:provenance "NSW Government Standard for Data Quality Reporting. https://data.nsw.gov.au/data-quality-reporting-tool" ;
    rdfs:isDefinedBy <https://linked.data.gov.au/def/nsw-quality-dimension> ;
    skos:broader dq-nsw:accuracy ;
    skos:definition "There have been no adjustments, changes or other factors that could impact the validity of the data. (For example: weighting, rounding, de-identification of data; changes or flaws in data collection or verification methods.). Or adjustments are identified in caveats attached to the dataset or data source"@en ;
    skos:inScheme <https://linked.data.gov.au/def/nsw-quality-dimension> ;
    skos:prefLabel "No changes or flaws not explained"@en ;
    dqv:inCategory dq-nsw:accuracy ;
.

dq-nsw:no-conflict
    a
        skos:Concept ,
        dqv:Dimension ;
    dcterms:provenance "NSW Government Standard for Data Quality Reporting. https://data.nsw.gov.au/data-quality-reporting-tool" ;
    rdfs:isDefinedBy <https://linked.data.gov.au/def/nsw-quality-dimension> ;
    skos:broader dq-nsw:institutional-environment ;
    skos:definition "Custodian has no commercial interest or conflict of interest in the data – or, has declared any interest in the data."@en ;
    skos:inScheme <https://linked.data.gov.au/def/nsw-quality-dimension> ;
    skos:prefLabel "No commercial interest or conflict"@en ;
    dqv:inCategory dq-nsw:institutional-environment ;
.

dq-nsw:non-proprietary
    a
        skos:Concept ,
        dqv:Dimension ;
    dcterms:provenance "NSW Government Standard for Data Quality Reporting. https://data.nsw.gov.au/data-quality-reporting-tool" ;
    rdfs:isDefinedBy <https://linked.data.gov.au/def/nsw-quality-dimension> ;
    skos:broader dq-nsw:accessibility ;
    skos:definition "This dataset or data source is available in a non-proprietary format."@en ;
    skos:inScheme <https://linked.data.gov.au/def/nsw-quality-dimension> ;
    skos:prefLabel "Non-proprietary format"@en ;
    dqv:inCategory dq-nsw:accessibility ;
.

dq-nsw:open-standards
    a
        skos:Concept ,
        dqv:Dimension ;
    dcterms:provenance "NSW Government Standard for Data Quality Reporting. https://data.nsw.gov.au/data-quality-reporting-tool" ;
    rdfs:isDefinedBy <https://linked.data.gov.au/def/nsw-quality-dimension> ;
    skos:broader dq-nsw:accessibility ;
    skos:definition "This dataset or data source is described using open standards and persistent identifiers."@en ;
    skos:inScheme <https://linked.data.gov.au/def/nsw-quality-dimension> ;
    skos:prefLabel "Open standards"@en ;
    dqv:inCategory dq-nsw:accessibility ;
.

dq-nsw:primary-user
    a
        skos:Concept ,
        dqv:Dimension ;
    dcterms:provenance "NSW Government Standard for Data Quality Reporting. https://data.nsw.gov.au/data-quality-reporting-tool" ;
    rdfs:isDefinedBy <https://linked.data.gov.au/def/nsw-quality-dimension> ;
    skos:broader dq-nsw:accuracy ;
    skos:definition "The data collection met the objectives of the primary user. The data correctly represents what it was designed to measure, monitor or report."@en ;
    skos:inScheme <https://linked.data.gov.au/def/nsw-quality-dimension> ;
    skos:prefLabel "Data met needs of primary user"@en ;
    dqv:inCategory dq-nsw:accuracy ;
.

dq-nsw:revised
    a
        skos:Concept ,
        dqv:Dimension ;
    dcterms:provenance "NSW Government Standard for Data Quality Reporting. https://data.nsw.gov.au/data-quality-reporting-tool" ;
    rdfs:isDefinedBy <https://linked.data.gov.au/def/nsw-quality-dimension> ;
    skos:broader dq-nsw:accuracy ;
    skos:definition "Revision policy: If errors are identified, data is revised and the revision is publicised."@en ;
    skos:inScheme <https://linked.data.gov.au/def/nsw-quality-dimension> ;
    skos:prefLabel "Revised when errors detected"@en ;
    dqv:inCategory dq-nsw:accuracy ;
.

dq-nsw:sources
    a
        skos:Concept ,
        dqv:Dimension ;
    dcterms:provenance "NSW Government Standard for Data Quality Reporting. https://data.nsw.gov.au/data-quality-reporting-tool" ;
    rdfs:comment "Find out more about the primary data sources and methods of data collection from the Custodian (contact details below)."@en ;
    rdfs:isDefinedBy <https://linked.data.gov.au/def/nsw-quality-dimension> ;
    skos:broader dq-nsw:interpretability ;
    skos:definition "Information is available about the primary data sources and methods of data collection. (For example: instruments, forms, instructions.)"@en ;
    skos:inScheme <https://linked.data.gov.au/def/nsw-quality-dimension> ;
    skos:prefLabel "Data sources and methods"@en ;
    dqv:inCategory dq-nsw:interpretability ;
.

dq-nsw:standards
    a
        skos:Concept ,
        dqv:Dimension ;
    dcterms:provenance "NSW Government Standard for Data Quality Reporting. https://data.nsw.gov.au/data-quality-reporting-tool" ;
    rdfs:isDefinedBy <https://linked.data.gov.au/def/nsw-quality-dimension> ;
    skos:broader dq-nsw:coherence ;
    skos:definition "Standard definitions, common concepts, classifications and data recording practices have been used."@en ;
    skos:inScheme <https://linked.data.gov.au/def/nsw-quality-dimension> ;
    skos:prefLabel "Standard definitions and practices"@en ;
    dqv:inCategory dq-nsw:coherence ;
.

dq-nsw:structured
    a
        skos:Concept ,
        dqv:Dimension ;
    dcterms:provenance "NSW Government Standard for Data Quality Reporting. https://data.nsw.gov.au/data-quality-reporting-tool" ;
    rdfs:isDefinedBy <https://linked.data.gov.au/def/nsw-quality-dimension> ;
    skos:broader dq-nsw:accessibility ;
    skos:definition "This dataset or data source is available in a machine-processable, structured format."@en ;
    skos:inScheme <https://linked.data.gov.au/def/nsw-quality-dimension> ;
    skos:prefLabel "Structured data"@en ;
    dqv:inCategory dq-nsw:accessibility ;
.

dq-nsw:technical
    a
        skos:Concept ,
        dqv:Dimension ;
    dcterms:provenance "NSW Government Standard for Data Quality Reporting. https://data.nsw.gov.au/data-quality-reporting-tool" ;
    rdfs:comment "Find out more about ambiguous or technical terms used in the data from the Custodian (contact details below)."@en ;
    rdfs:isDefinedBy <https://linked.data.gov.au/def/nsw-quality-dimension> ;
    skos:broader dq-nsw:interpretability ;
    skos:definition "Information is available to explain ambiguous or technical terms used in the data."@en ;
    skos:inScheme <https://linked.data.gov.au/def/nsw-quality-dimension> ;
    skos:prefLabel "Technical explanations"@en ;
    dqv:inCategory dq-nsw:interpretability ;
.

dq-nsw:time
    a
        skos:Concept ,
        dqv:Dimension ;
    dcterms:provenance "NSW Government Standard for Data Quality Reporting. https://data.nsw.gov.au/data-quality-reporting-tool" ;
    rdfs:isDefinedBy <https://linked.data.gov.au/def/nsw-quality-dimension> ;
    skos:broader dq-nsw:coherence ;
    skos:definition "This data is part of a time series. It is consistent with previous releases. There have been no changes in methodology or external impacts since the last data release."@en ;
    skos:inScheme <https://linked.data.gov.au/def/nsw-quality-dimension> ;
    skos:prefLabel "Consistent over time"@en ;
    dqv:inCategory dq-nsw:coherence ;
.

<https://linked.data.gov.au/def/gsq-alias/des>
    a sdo:Organization ;
    sdo:name "Department of Environment and Science"@en ;
.

dq-nsw:accessibility
    a
        skos:Concept ,
        dqv:Category ;
    dcterms:provenance "NSW Government Standard for Data Quality Reporting. https://data.nsw.gov.au/data-quality-reporting-tool" ;
    rdfs:isDefinedBy <https://linked.data.gov.au/def/nsw-quality-dimension> ;
    skos:definition "A dimension of quality relating to the ease with which data or information can be retrieved, used and understood."@en ;
    skos:inScheme <https://linked.data.gov.au/def/nsw-quality-dimension> ;
    skos:prefLabel "Accessibility"@en ;
.

dq-nsw:accuracy
    a
        skos:Concept ,
        dqv:Category ;
    dcterms:provenance "NSW Government Standard for Data Quality Reporting. https://data.nsw.gov.au/data-quality-reporting-tool" ;
    rdfs:isDefinedBy <https://linked.data.gov.au/def/nsw-quality-dimension> ;
    skos:definition "A dimension of quality relating to the degree to which the data or information correctly describes that which it was designed to measure."@en ;
    skos:inScheme <https://linked.data.gov.au/def/nsw-quality-dimension> ;
    skos:prefLabel "Accuracy"@en ;
.

dq-nsw:coherence
    a
        skos:Concept ,
        dqv:Category ;
    dcterms:provenance "NSW Government Standard for Data Quality Reporting. https://data.nsw.gov.au/data-quality-reporting-tool" ;
    rdfs:isDefinedBy <https://linked.data.gov.au/def/nsw-quality-dimension> ;
    skos:definition "A dimension of quality relating to the degree to which data or information can be compared with itself and other information over time."@en ;
    skos:inScheme <https://linked.data.gov.au/def/nsw-quality-dimension> ;
    skos:prefLabel "Coherence"@en ;
.

dq-nsw:institutional-environment
    a
        skos:Concept ,
        dqv:Category ;
    dcterms:provenance "NSW Government Standard for Data Quality Reporting. https://data.nsw.gov.au/data-quality-reporting-tool" ;
    rdfs:isDefinedBy <https://linked.data.gov.au/def/nsw-quality-dimension> ;
    skos:definition "A dimension of quality relating to the institutional and organisational factors which may have a significant influence on the effectiveness and credibility of the agency producing the data or information."@en ;
    skos:inScheme <https://linked.data.gov.au/def/nsw-quality-dimension> ;
    skos:prefLabel "Institutional Environment"@en ;
.

dq-nsw:interpretability
    a
        skos:Concept ,
        dqv:Category ;
    dcterms:provenance "NSW Government Standard for Data Quality Reporting. https://data.nsw.gov.au/data-quality-reporting-tool" ;
    rdfs:isDefinedBy <https://linked.data.gov.au/def/nsw-quality-dimension> ;
    skos:definition "A dimension of quality relating to the degree to which data or information can be understood, explained and used."@en ;
    skos:inScheme <https://linked.data.gov.au/def/nsw-quality-dimension> ;
    skos:prefLabel "Interpretability"@en ;
.

<https://linked.data.gov.au/def/nsw-quality-dimension>
    a skos:ConceptScheme ;
    dcterms:created "2020-11-16"^^xsd:date ;
    dcterms:creator <https://linked.data.gov.au/def/gsq-alias/des> ;
    dcterms:modified "2023-03-10"^^xsd:date ;
    dcterms:provenance "NSW Government Standard for Data Quality Reporting. https://data.nsw.gov.au/data-quality-reporting-tool" ;
    dcterms:publisher <https://linked.data.gov.au/def/gsq-alias/des> ;
    rdfs:comment "Find out more about the quality assurance processes from the NSW Government Standard for Data Quality Reporting. https://data.nsw.gov.au/data-quality-reporting-tool"@en ;
    rdfs:seeAlso <https://data.nsw.gov.au/data-quality-reporting-tool> ;
    skos:definition "Criteria for a Data Quality Statement as per the New South Wales (NSW) Government. Find out more about the quality assurance processes from the NSW Government Standard for Data Quality Reporting. https://data.nsw.gov.au/data-quality-reporting-tool"@en ;
    skos:hasTopConcept
        dq-nsw:accessibility ,
        dq-nsw:accuracy ,
        dq-nsw:coherence ,
        dq-nsw:institutional-environment ,
        dq-nsw:interpretability ;
    skos:prefLabel "NSW Government Data Quality Dimensions"@en ;
.

