PREFIX dcterms: <http://purl.org/dc/terms/>
PREFIX owl: <http://www.w3.org/2002/07/owl#>
PREFIX quantitykind: <http://qudt.org/vocab/quantitykind/>
PREFIX qudt: <http://qudt.org/schema/qudt/>
PREFIX rdfs: <http://www.w3.org/2000/01/rdf-schema#>
PREFIX skos: <http://www.w3.org/2004/02/skos/core#>
PREFIX unit: <http://qudt.org/vocab/unit/>
PREFIX vaem: <http://www.linkedmodel.org/schema/vaem#>
PREFIX xsd: <http://www.w3.org/2001/XMLSchema#>

quantitykind:AmountOfSubstancePerUnitMass
    a
        qudt:QuantityKind ,
        skos:Concept ;
    skos:historyNote "Derived from QUDT (http://qudt.org/vocab/quantitykind)" ;
    qudt:applicableUnit unit:CentiMOL-PER-KiloGM ;
    rdfs:isDefinedBy <http://qudt.org/2.1/vocab/quantitykind> ;
    skos:broader quantitykind:Concentration ;
    skos:definition "Amount of Substance per Unit of Mass." ;
    skos:inScheme <https://linked.data.gov.au/def/qesd-qkd> ;
    skos:prefLabel "Amount of Substance per Unit Mass"@en ;
.

quantitykind:LengthPercentage
    a
        qudt:QuantityKind ,
        skos:Concept ;
    skos:historyNote "Derived from QUDT (http://qudt.org/vocab/quantitykind)" ;
    qudt:applicableUnit unit:PERCENT ;
    rdfs:isDefinedBy <http://qudt.org/2.1/vocab/quantitykind> ;
    skos:broader quantitykind:DimensionlessRatio ;
    skos:definition "Length Percentage" ;
    skos:inScheme <https://linked.data.gov.au/def/qesd-qkd> ;
    skos:prefLabel "Length Percentage"@en ;
.

quantitykind:LiquidVolume
    a
        qudt:QuantityKind ,
        skos:Concept ;
    skos:historyNote "Derived from QUDT (http://qudt.org/vocab/quantitykind)" ;
    qudt:applicableUnit unit:L ;
    rdfs:isDefinedBy <http://qudt.org/2.1/vocab/quantitykind> ;
    skos:broader quantitykind:Volume ;
    skos:definition "Liquid volume is the volume of a given amount of liquid, that is, the amount of space a liquid takes up. There are a number of different units used to measure liquid volume, but most of them fall under either the metric system of measurement or the Imperial system of measurement." ;
    skos:inScheme <https://linked.data.gov.au/def/qesd-qkd> ;
    skos:prefLabel "Liquid Volume"@en ;
.

quantitykind:PressurePercentage
    a
        qudt:QuantityKind ,
        skos:Concept ;
    skos:historyNote "Derived from QUDT (http://qudt.org/vocab/quantitykind)" ;
    qudt:applicableUnit unit:PERCENT ;
    rdfs:isDefinedBy <http://qudt.org/2.1/vocab/quantitykind> ;
    skos:broader quantitykind:DimensionlessRatio ;
    skos:definition "Pressure Percentage" ;
    skos:inScheme <https://linked.data.gov.au/def/qesd-qkd> ;
    skos:prefLabel "Pressure Percentage"@en ;
.

quantitykind:PressureRatio
    a
        qudt:QuantityKind ,
        skos:Concept ;
    skos:historyNote "Derived from QUDT (http://qudt.org/vocab/quantitykind)" ;
    qudt:applicableUnit unit:PERCENT_RH ;
    rdfs:isDefinedBy <http://qudt.org/2.1/vocab/quantitykind> ;
    skos:broader quantitykind:DimensionlessRatio ;
    skos:definition "Pressure Ratio" ;
    skos:inScheme <https://linked.data.gov.au/def/qesd-qkd> ;
    skos:prefLabel "Pressure Ratio"@en ;
.

quantitykind:TimePercentage
    a
        qudt:QuantityKind ,
        skos:Concept ;
    skos:historyNote "Derived from QUDT (http://qudt.org/vocab/quantitykind)" ;
    qudt:applicableUnit unit:PERCENT ;
    rdfs:isDefinedBy <http://qudt.org/2.1/vocab/quantitykind> ;
    skos:broader quantitykind:DimensionlessRatio ;
    skos:definition "Time Percentage"@en ;
    skos:inScheme <https://linked.data.gov.au/def/qesd-qkd> ;
    skos:prefLabel "Time Percentage"@en ;
.

quantitykind:Voltage
    a
        qudt:QuantityKind ,
        skos:Concept ;
    skos:historyNote "Derived from QUDT (http://qudt.org/vocab/quantitykind)" ;
    qudt:applicableUnit unit:MilliV ;
    rdfs:isDefinedBy <http://qudt.org/2.1/vocab/quantitykind> ;
    skos:broader quantitykind:EnergyPerElectricCharge ;
    skos:definition "Voltage, also referred to as Electric Tension, is the difference between electrical potentials of two points. For an electric field within a medium." ;
    skos:inScheme <https://linked.data.gov.au/def/qesd-qkd> ;
    skos:prefLabel "Voltage"@en ;
.

quantitykind:Absorptance
    a
        qudt:QuantityKind ,
        skos:Concept ;
    skos:historyNote "Derived from QUDT (http://qudt.org/vocab/quantitykind)" ;
    qudt:applicableUnit unit:UNITLESS ;
    rdfs:isDefinedBy <http://qudt.org/2.1/vocab/quantitykind> ;
    skos:definition "Absorptance is the ratio of the radiation absorbed by a surface to that incident upon it. Also known as absorbance." ;
    skos:exactMatch <http://en.wikipedia.org/wiki/Absorbance> ;
    skos:inScheme <https://linked.data.gov.au/def/qesd-qkd> ;
    skos:prefLabel "Absorptance"@en ;
    skos:topConceptOf <https://linked.data.gov.au/def/qesd-qkd> ;
.

quantitykind:ActivityCoefficient
    a
        qudt:QuantityKind ,
        skos:Concept ;
    skos:historyNote "Derived from QUDT (http://qudt.org/vocab/quantitykind)" ;
    qudt:applicableUnit unit:UNITLESS ;
    rdfs:isDefinedBy <http://qudt.org/2.1/vocab/quantitykind> ;
    skos:definition "An Activity Coefficient is a factor used in thermodynamics to account for deviations from ideal behaviour in a mixture of chemical substances. In an ideal mixture, the interactions between each pair of chemical species are the same (or more formally, the enthalpy change of solution is zero) and, as a result, properties of the mixtures can be expressed directly in terms of simple concentrations or partial pressures of the substances present e.g. Raoult's law. Deviations from ideality are accommodated by modifying the concentration by an activity coefficient." ;
    skos:inScheme <https://linked.data.gov.au/def/qesd-qkd> ;
    skos:prefLabel "Activity Coefficient"@en ;
    skos:topConceptOf <https://linked.data.gov.au/def/qesd-qkd> ;
.

quantitykind:AmountOfSubstance
    a
        qudt:QuantityKind ,
        skos:Concept ;
    skos:historyNote "Derived from QUDT (http://qudt.org/vocab/quantitykind)" ;
    qudt:applicableUnit unit:MOL ;
    rdfs:isDefinedBy <http://qudt.org/2.1/vocab/quantitykind> ;
    skos:definition "Amount of Substance is a standards-defined quantity that measures the size of an ensemble of elementary entities, such as atoms, molecules, electrons, and other particles. It is sometimes referred to as chemical amount. The International System of Units (SI) defines the amount of substance to be proportional to the number of elementary entities present. The SI unit for amount of substance is mole. It has the unit symbol mol. The mole is defined as the amount of substance that contains an equal number of elementary entities as there are atoms in 0.012kg of the isotope carbon-12. This number is called Avogadro's number. and has the value 6.02214179(30) times 10 The only other unit of amount of substance in current use is the pound-mole with the symbol lb-mol, which is sometimes used in chemical engineering in the United States. One pound-mole is exactly 453.59237 mol." ;
    skos:inScheme <https://linked.data.gov.au/def/qesd-qkd> ;
    skos:prefLabel "Amount of Substance"@en ;
    skos:topConceptOf <https://linked.data.gov.au/def/qesd-qkd> ;
.

quantitykind:AmountOfSubstanceFractionOfB
    a
        qudt:QuantityKind ,
        skos:Concept ;
    skos:historyNote "Derived from QUDT (http://qudt.org/vocab/quantitykind)" ;
    qudt:applicableUnit unit:UNITLESS ;
    rdfs:isDefinedBy <http://qudt.org/2.1/vocab/quantitykind> ;
    skos:definition "Amount of Substance of Fraction of B is defined as the amount of a constituent divided by the total amount of all constituents in a mixture." ;
    skos:inScheme <https://linked.data.gov.au/def/qesd-qkd> ;
    skos:prefLabel "Amount of Substance of Fraction of B"@en ;
    skos:topConceptOf <https://linked.data.gov.au/def/qesd-qkd> ;
.

quantitykind:Angle
    a
        qudt:QuantityKind ,
        skos:Concept ;
    skos:historyNote "Derived from QUDT (http://qudt.org/vocab/quantitykind)" ;
    qudt:applicableUnit
        unit:DEG ,
        unit:RAD ;
    rdfs:isDefinedBy <http://qudt.org/2.1/vocab/quantitykind> ;
    skos:definition "The abstract notion of angle. Narrow concepts include plane angle and solid angle. While both plane angle and solid angle are dimensionless, they are actually length/length and area/area respectively." ;
    skos:inScheme <https://linked.data.gov.au/def/qesd-qkd> ;
    skos:prefLabel "Angle"@en ;
    skos:topConceptOf <https://linked.data.gov.au/def/qesd-qkd> ;
.

quantitykind:Area
    a
        qudt:QuantityKind ,
        skos:Concept ;
    skos:historyNote "Derived from QUDT (http://qudt.org/vocab/quantitykind)" ;
    qudt:applicableUnit
        unit:CentiM2 ,
        unit:HA ,
        unit:M2 ;
    rdfs:isDefinedBy <http://qudt.org/2.1/vocab/quantitykind> ;
    skos:definition "Area is a quantity expressing the two-dimensional size of a defined part of a surface, typically a region bounded by a closed curve." ;
    skos:inScheme <https://linked.data.gov.au/def/qesd-qkd> ;
    skos:prefLabel "Area"@en ;
    skos:topConceptOf <https://linked.data.gov.au/def/qesd-qkd> ;
.

quantitykind:Conductivity
    a
        qudt:QuantityKind ,
        skos:Concept ;
    skos:historyNote "Derived from QUDT (http://qudt.org/vocab/quantitykind)" ;
    qudt:applicableUnit unit:MicroS-PER-CentiM ;
    rdfs:isDefinedBy <http://qudt.org/2.1/vocab/quantitykind> ;
    skos:definition "Conductivity is a scalar or tensor quantity the product of which by the electric field strength in a medium is equal to the electric current density. For an isotropic medium the conductivity is a scalar quantity; for an anisotropic medium it is a tensor quantity." ;
    skos:inScheme <https://linked.data.gov.au/def/qesd-qkd> ;
    skos:prefLabel "Conductivity"@en ;
    skos:topConceptOf <https://linked.data.gov.au/def/qesd-qkd> ;
.

quantitykind:ElectricConductivity
    a
        qudt:QuantityKind ,
        skos:Concept ;
    skos:historyNote "Derived from QUDT (http://qudt.org/vocab/quantitykind)" ;
    qudt:applicableUnit unit:MicroS ;
    rdfs:isDefinedBy <http://qudt.org/2.1/vocab/quantitykind> ;
    skos:definition "Electric Conductivity or Specific Conductance is a measure of a material's ability to conduct an electric current. When an electrical potential difference is placed across a conductor, its movable charges flow, giving rise to an electric current. The conductivity \\(\\sigma\\) is defined as the ratio of the electric current density (J) to the electric field (E): (J = sigma E). In isotropic materials, conductivity is scalar-valued, however in general, conductivity is a tensor-valued quantity." ;
    skos:inScheme <https://linked.data.gov.au/def/qesd-qkd> ;
    skos:prefLabel "Electric Conductivity"@en ;
    skos:topConceptOf <https://linked.data.gov.au/def/qesd-qkd> ;
.

quantitykind:ExtentOfReaction
    a
        qudt:QuantityKind ,
        skos:Concept ;
    skos:historyNote "Derived from QUDT (http://qudt.org/vocab/quantitykind)" ;
    qudt:applicableUnit unit:MOL ;
    rdfs:isDefinedBy <http://qudt.org/2.1/vocab/quantitykind> ;
    skos:definition "In physical chemistry, the Extent of Reaction is a quantity that measures the extent in which the reaction proceeds." ;
    skos:inScheme <https://linked.data.gov.au/def/qesd-qkd> ;
    skos:prefLabel "Extent of Reaction"@en ;
    skos:topConceptOf <https://linked.data.gov.au/def/qesd-qkd> ;
.

quantitykind:ForcePerArea
    a
        qudt:QuantityKind ,
        skos:Concept ;
    skos:historyNote "Derived from QUDT (http://qudt.org/vocab/quantitykind)" ;
    qudt:applicableUnit unit:HectoPA ;
    rdfs:isDefinedBy <http://qudt.org/2.1/vocab/quantitykind> ;
    skos:definition "The force applied to a unit area of surface; measured in pascals (SI unit) or in dynes (cgs unit)" ;
    skos:inScheme <https://linked.data.gov.au/def/qesd-qkd> ;
    skos:prefLabel "Force Per Area"@en ;
    skos:topConceptOf <https://linked.data.gov.au/def/qesd-qkd> ;
.

quantitykind:IonicStrength
    a
        qudt:QuantityKind ,
        skos:Concept ;
    skos:historyNote "Derived from QUDT (http://qudt.org/vocab/quantitykind)" ;
    qudt:applicableUnit unit:CentiMOL-PER-KiloGM ;
    rdfs:isDefinedBy <http://qudt.org/2.1/vocab/quantitykind> ;
    skos:definition "The Ionic Strength of a solution is a measure of the concentration of ions in that solution." ;
    skos:inScheme <https://linked.data.gov.au/def/qesd-qkd> ;
    skos:prefLabel "Ionic Strength"@en ;
    skos:topConceptOf <https://linked.data.gov.au/def/qesd-qkd> ;
.

quantitykind:Length
    a
        qudt:QuantityKind ,
        skos:Concept ;
    skos:historyNote "Derived from QUDT (http://qudt.org/vocab/quantitykind)" ;
    qudt:applicableUnit
        unit:CentiM ,
        unit:KiloM ,
        unit:M ,
        unit:MicroM ,
        unit:MilliM ;
    rdfs:isDefinedBy <http://qudt.org/2.1/vocab/quantitykind> ;
    skos:definition "In geometric measurements, length most commonly refers to the est dimension of an object. In some contexts, the term length is reserved for a certain dimension of an object along which the length is measured." ;
    skos:inScheme <https://linked.data.gov.au/def/qesd-qkd> ;
    skos:prefLabel "Length"@en ;
    skos:topConceptOf <https://linked.data.gov.au/def/qesd-qkd> ;
.

quantitykind:Mass
    a
        qudt:QuantityKind ,
        skos:Concept ;
    skos:historyNote "Derived from QUDT (http://qudt.org/vocab/quantitykind)" ;
    qudt:applicableUnit
        unit:GM ,
        unit:KiloGM ,
        unit:TONNE ;
    rdfs:isDefinedBy <http://qudt.org/2.1/vocab/quantitykind> ;
    skos:definition "In physics, mass, more specifically inertial mass, can be defined as a quantitative measure of an object's resistance to acceleration. The SI unit of mass is the kilogram (kg)" ;
    skos:inScheme <https://linked.data.gov.au/def/qesd-qkd> ;
    skos:prefLabel "Mass"@en ;
    skos:topConceptOf <https://linked.data.gov.au/def/qesd-qkd> ;
.

quantitykind:MassDensity
    a
        qudt:QuantityKind ,
        skos:Concept ;
    skos:historyNote "Derived from QUDT (http://qudt.org/vocab/quantitykind)" ;
    qudt:applicableUnit
        unit:MicroGM-PER-L ,
        unit:MilliGM-PER-L ;
    rdfs:isDefinedBy <http://qudt.org/2.1/vocab/quantitykind> ;
    skos:definition "The mass density or density of a material is its mass per unit volume." ;
    skos:inScheme <https://linked.data.gov.au/def/qesd-qkd> ;
    skos:prefLabel "Mass Density"@en ;
    skos:topConceptOf <https://linked.data.gov.au/def/qesd-qkd> ;
.

quantitykind:MassFraction
    a
        qudt:QuantityKind ,
        skos:Concept ;
    skos:historyNote "Derived from QUDT (http://qudt.org/vocab/quantitykind)" ;
    qudt:applicableUnit unit:UNITLESS ;
    rdfs:isDefinedBy <http://qudt.org/2.1/vocab/quantitykind> ;
    skos:definition "The Mass Fraction is the fraction of one substance with mass to the mass of the total mixture." ;
    skos:inScheme <https://linked.data.gov.au/def/qesd-qkd> ;
    skos:prefLabel "Mass Fraction"@en ;
    skos:topConceptOf <https://linked.data.gov.au/def/qesd-qkd> ;
.

quantitykind:MassFractionOfDryMatter
    a
        qudt:QuantityKind ,
        skos:Concept ;
    skos:historyNote "Derived from QUDT (http://qudt.org/vocab/quantitykind)" ;
    qudt:applicableUnit unit:UNITLESS ;
    rdfs:isDefinedBy <http://qudt.org/2.1/vocab/quantitykind> ;
    rdfs:seeAlso quantitykind:MassFractionOfWater ;
    skos:definition "Mass Fraction of Dry Matter is one of a number of Concentration quantities defined by ISO 8000." ;
    skos:inScheme <https://linked.data.gov.au/def/qesd-qkd> ;
    skos:prefLabel "Mass Fraction of Dry Matter"@en ;
    skos:topConceptOf <https://linked.data.gov.au/def/qesd-qkd> ;
.

quantitykind:MolalityOfSolute
    a
        qudt:QuantityKind ,
        skos:Concept ;
    skos:historyNote "Derived from QUDT (http://qudt.org/vocab/quantitykind)" ;
    qudt:applicableUnit unit:CentiMOL-PER-KiloGM ;
    rdfs:isDefinedBy <http://qudt.org/2.1/vocab/quantitykind> ;
    skos:definition "The Molality of Solute of a solution is defined as the amount of substance of solute divided by the mass in kg of the solvent." ;
    skos:inScheme <https://linked.data.gov.au/def/qesd-qkd> ;
    skos:prefLabel "Molality of Solute"@en ;
    skos:topConceptOf <https://linked.data.gov.au/def/qesd-qkd> ;
.

quantitykind:MultiplicationFactor
    a
        qudt:QuantityKind ,
        skos:Concept ;
    skos:historyNote "Derived from QUDT (http://qudt.org/vocab/quantitykind)" ;
    qudt:applicableUnit unit:UNITLESS ;
    rdfs:isDefinedBy <http://qudt.org/2.1/vocab/quantitykind> ;
    skos:definition "The Multiplication Factor is the ratio of the total number of fission or fission-dependent neutrons produced in a time interval to the total number of neutrons lost by absorption and leakage during the same interval." ;
    skos:inScheme <https://linked.data.gov.au/def/qesd-qkd> ;
    skos:prefLabel "Multiplication Factor"@en ;
    skos:topConceptOf <https://linked.data.gov.au/def/qesd-qkd> ;
.

quantitykind:Period
    a
        qudt:QuantityKind ,
        skos:Concept ;
    skos:historyNote "Derived from QUDT (http://qudt.org/vocab/quantitykind)" ;
    qudt:applicableUnit unit:SEC ;
    vaem:todo "belongs to SOQ-ISO" ;
    rdfs:isDefinedBy <http://qudt.org/2.1/vocab/quantitykind> ;
    skos:definition "Duration of one cycle of a periodic phenomenon." ;
    skos:inScheme <https://linked.data.gov.au/def/qesd-qkd> ;
    skos:prefLabel "Period"@en ;
    skos:topConceptOf <https://linked.data.gov.au/def/qesd-qkd> ;
.

quantitykind:RelativeHumidity
    a
        qudt:QuantityKind ,
        skos:Concept ;
    skos:historyNote "Derived from QUDT (http://qudt.org/vocab/quantitykind)" ;
    qudt:applicableUnit unit:UNITLESS ;
    rdfs:isDefinedBy <http://qudt.org/2.1/vocab/quantitykind> ;
    rdfs:seeAlso quantitykind:AbsoluteHumidity ;
    skos:altLabel "RH" ;
    skos:definition "Relative Humidity is the ratio of the partial pressure of water vapor in an air-water mixture to the saturated vapor pressure of water at a prescribed temperature. The relative humidity of air depends not only on temperature but also on the pressure of the system of interest. Relative Humidity is also referred to as Relative Partial Pressure. Relative partial pressure is often referred to as RH and expressed in percent." ;
    skos:inScheme <https://linked.data.gov.au/def/qesd-qkd> ;
    skos:prefLabel "Relative Humidity"@en ;
    skos:topConceptOf <https://linked.data.gov.au/def/qesd-qkd> ;
.

quantitykind:RelativeMassDensity
    a
        qudt:QuantityKind ,
        skos:Concept ;
    skos:historyNote "Derived from QUDT (http://qudt.org/vocab/quantitykind)" ;
    qudt:applicableUnit unit:UNITLESS ;
    rdfs:isDefinedBy <http://qudt.org/2.1/vocab/quantitykind> ;
    skos:definition "Relative density, or specific gravity, is the ratio of the density (mass of a unit volume) of a substance to the density of a given reference material." ;
    skos:inScheme <https://linked.data.gov.au/def/qesd-qkd> ;
    skos:prefLabel "Relative Mass Density"@en ;
    skos:topConceptOf <https://linked.data.gov.au/def/qesd-qkd> ;
.

quantitykind:RelativePartialPressure
    a
        qudt:QuantityKind ,
        skos:Concept ;
    skos:historyNote "Derived from QUDT (http://qudt.org/vocab/quantitykind)" ;
    qudt:applicableUnit unit:UNITLESS ;
    rdfs:isDefinedBy <http://qudt.org/2.1/vocab/quantitykind> ;
    skos:altLabel "RH" ;
    skos:definition "Relative partial pressure is often referred to as RH and expressed in percent. Relative Partial Pressure is also referred to as Relative Humidity.  varphi = p / p_sat, where p is partial pressure of vapour,  p_sat is thermodynamic temperature and V is its partial pressure at saturation (at the same temperature). " ;
    skos:inScheme <https://linked.data.gov.au/def/qesd-qkd> ;
    skos:prefLabel "Relative Partial Pressure"@en ;
    skos:topConceptOf <https://linked.data.gov.au/def/qesd-qkd> ;
.

quantitykind:StatisticalWeight
    a
        qudt:QuantityKind ,
        skos:Concept ;
    skos:historyNote "Derived from QUDT (http://qudt.org/vocab/quantitykind)" ;
    qudt:applicableUnit unit:UNITLESS ;
    rdfs:isDefinedBy <http://qudt.org/2.1/vocab/quantitykind> ;
    skos:definition "A Statistical Weight is the relative probability (possibly unnormalized) of a particular feature of a state." ;
    skos:inScheme <https://linked.data.gov.au/def/qesd-qkd> ;
    skos:prefLabel "Statistical Weight"@en ;
    skos:topConceptOf <https://linked.data.gov.au/def/qesd-qkd> ;
.

quantitykind:Temperature
    a
        qudt:QuantityKind ,
        skos:Concept ;
    skos:historyNote "Derived from QUDT (http://qudt.org/vocab/quantitykind)" ;
    qudt:applicableUnit unit:DEG_C ;
    rdfs:isDefinedBy <http://qudt.org/2.1/vocab/quantitykind> ;
    rdfs:seeAlso quantitykind:ThermodynamicTemperature ;
    skos:definition "Temperature is a physical property of matter that quantitatively expresses the common notions of hot and cold. Objects of low temperature are cold, while various degrees of higher temperatures are referred to as warm or hot. Heat spontaneously flows from bodies of a higher temperature to bodies of lower temperature, at a rate that increases with the temperature difference and the thermal conductivity." ;
    skos:inScheme <https://linked.data.gov.au/def/qesd-qkd> ;
    skos:prefLabel "Temperature"@en ;
    skos:topConceptOf <https://linked.data.gov.au/def/qesd-qkd> ;
.

quantitykind:Time
    a
        qudt:QuantityKind ,
        skos:Concept ;
    skos:historyNote "Derived from QUDT (http://qudt.org/vocab/quantitykind)" ;
    qudt:applicableUnit
        unit:DAY ,
        unit:HR ,
        unit:MIN ,
        unit:SEC ,
        unit:YR ;
    rdfs:isDefinedBy <http://qudt.org/2.1/vocab/quantitykind> ;
    skos:definition "Time is a basic component of the measuring system used to sequence events, to compare the durations of events and the intervals between them, and to quantify the motions of objects." ;
    skos:inScheme <https://linked.data.gov.au/def/qesd-qkd> ;
    skos:prefLabel "Time"@en ;
    skos:topConceptOf <https://linked.data.gov.au/def/qesd-qkd> ;
.

quantitykind:Turbidity
    a
        qudt:QuantityKind ,
        skos:Concept ;
    skos:historyNote "Derived from QUDT (http://qudt.org/vocab/quantitykind)" ;
    qudt:applicableUnit unit:NTU ;
    rdfs:isDefinedBy <http://qudt.org/2.1/vocab/quantitykind> ;
    skos:definition "Turbidity is the cloudiness or haziness of a fluid, or of air, caused by individual particles (suspended solids) that are generally invisible to the naked eye, similar to smoke in air. Turbidity in open water is often caused by phytoplankton and the measurement of turbidity is a key test of water quality. The higher the turbidity, the higher the risk of the drinkers developing gastrointestinal diseases, especially for immune-compromised people, because contaminants like virus or bacteria can become attached to the suspended solid. The suspended solids interfere with water disinfection with chlorine because the particles act as shields for the virus and bacteria. Similarly suspended solids can protect bacteria from UV sterilisation of water. Fluids can contain suspended solid matter consisting of particles of many different sizes. While some suspended material will be large enough and heavy enough to settle rapidly to the bottom container if a liquid sample is left to stand (the settleable solids), very small particles will settle only very slowly or not at all if the sample is regularly agitated or the particles are colloidal. These small solid particles cause the liquid to appear turbid." ;
    skos:inScheme <https://linked.data.gov.au/def/qesd-qkd> ;
    skos:prefLabel "Turbidity"@en ;
    skos:topConceptOf <https://linked.data.gov.au/def/qesd-qkd> ;
.

quantitykind:VolumeFlowRate
    a
        qudt:QuantityKind ,
        skos:Concept ;
    skos:historyNote "Derived from QUDT (http://qudt.org/vocab/quantitykind)" ;
    qudt:applicableUnit
        unit:M3-PER-HR ,
        unit:M3-PER-SEC ;
    rdfs:isDefinedBy <http://qudt.org/2.1/vocab/quantitykind> ;
    skos:definition "Volumetric Flow Rate, (also known as volume flow rate, rate of fluid flow or volume velocity) is the volume of fluid which passes through a given surface per unit time." ;
    skos:inScheme <https://linked.data.gov.au/def/qesd-qkd> ;
    skos:prefLabel "Volume Flow Rate"@en ;
    skos:topConceptOf <https://linked.data.gov.au/def/qesd-qkd> ;
.

quantitykind:VolumePerUnitTime
    a
        qudt:QuantityKind ,
        skos:Concept ;
    skos:historyNote "Derived from QUDT (http://qudt.org/vocab/quantitykind)" ;
    qudt:applicableUnit
        unit:M3-PER-HR ,
        unit:M3-PER-SEC ;
    rdfs:isDefinedBy <http://qudt.org/2.1/vocab/quantitykind> ;
    skos:definition "Volume per Unit Time" ;
    skos:inScheme <https://linked.data.gov.au/def/qesd-qkd> ;
    skos:prefLabel "Volume per Unit Time"@en ;
    skos:topConceptOf <https://linked.data.gov.au/def/qesd-qkd> ;
.

quantitykind:Concentration
    a
        qudt:QuantityKind ,
        skos:Concept ;
    skos:historyNote "Derived from QUDT (http://qudt.org/vocab/quantitykind)" ;
    rdfs:isDefinedBy <http://qudt.org/2.1/vocab/quantitykind> ;
    skos:definition "In chemistry, concentration is defined as the abundance of a constituent divided by the total volume of a mixture. Furthermore, in chemistry, four types of mathematical description can be distinguished: mass concentration, molar concentration, number concentration, and volume concentration. The term concentration can be applied to any kind of chemical mixture, but most frequently it refers to solutes in solutions." ;
    skos:inScheme <https://linked.data.gov.au/def/qesd-qkd> ;
    skos:prefLabel "Concentration"@en ;
    skos:topConceptOf <https://linked.data.gov.au/def/qesd-qkd> ;
.

quantitykind:Dimensionless
    a
        qudt:QuantityKind ,
        skos:Concept ;
    skos:historyNote "Derived from QUDT (http://qudt.org/vocab/quantitykind)" ;
    qudt:applicableUnit
        unit:NUM ,
        unit:UNITLESS ;
    rdfs:isDefinedBy <http://qudt.org/2.1/vocab/quantitykind> ;
    skos:definition "In dimensional analysis, a dimensionless quantity or quantity of dimension one is a quantity without an associated physical dimension. It is thus a pure number, and as such always has a dimension of 1. Dimensionless quantities are widely used in mathematics, physics, engineering, economics, and in everyday life (such as in counting). Numerous well-known quantities, such as pi, epsilon, and psi, are dimensionless. By contrast, non-dimensionless quantities are measured in units of length, area, time, etc. Dimensionless quantities are often defined as products or ratios of quantities that are not dimensionless, but whose dimensions cancel out when their powers are multiplied." ;
    skos:inScheme <https://linked.data.gov.au/def/qesd-qkd> ;
    skos:prefLabel "Dimensionless"@en ;
    skos:topConceptOf <https://linked.data.gov.au/def/qesd-qkd> ;
.

quantitykind:EnergyPerElectricCharge
    a
        qudt:QuantityKind ,
        skos:Concept ;
    skos:historyNote "Derived from QUDT (http://qudt.org/vocab/quantitykind)" ;
    qudt:applicableUnit unit:V ;
    rdfs:isDefinedBy <http://qudt.org/2.1/vocab/quantitykind> ;
    skos:definition "Voltage is a representation of the electric potential energy per unit charge. If a unit of electrical charge were placed in a location, the voltage indicates the potential energy of it at that point. In other words, it is a measurement of the energy contained within an electric field, or an electric circuit, at a given point. Voltage is a scalar quantity. The SI unit of voltage is the volt, such that 1 volt = 1 joule/coulomb." ;
    skos:inScheme <https://linked.data.gov.au/def/qesd-qkd> ;
    skos:prefLabel "Energy per electric charge"@en ;
    skos:topConceptOf <https://linked.data.gov.au/def/qesd-qkd> ;
.

quantitykind:Volume
    a
        qudt:QuantityKind ,
        skos:Concept ;
    skos:historyNote "Derived from QUDT (http://qudt.org/vocab/quantitykind)" ;
    qudt:applicableUnit
        unit:CentiM3 ,
        unit:M3 ;
    rdfs:isDefinedBy <http://qudt.org/2.1/vocab/quantitykind> ;
    skos:definition "The volume of a solid object is the three-dimensional concept of how much space it occupies, often quantified numerically. One-dimensional figures (such as lines) and two-dimensional shapes (such as squares) are assigned zero volume in the three-dimensional space." ;
    skos:inScheme <https://linked.data.gov.au/def/qesd-qkd> ;
    skos:prefLabel "Volume"@en ;
    skos:topConceptOf <https://linked.data.gov.au/def/qesd-qkd> ;
.

quantitykind:DimensionlessRatio
    a
        qudt:QuantityKind ,
        skos:Concept ;
    skos:historyNote "Derived from QUDT (http://qudt.org/vocab/quantitykind)" ;
    qudt:applicableUnit
        unit:NUM ,
        unit:PERCENT ,
        unit:UNITLESS ;
    rdfs:isDefinedBy <http://qudt.org/2.1/vocab/quantitykind> ;
    skos:broader quantitykind:Dimensionless ;
    skos:definition "A ratio that has no dimensions." ;
    skos:inScheme <https://linked.data.gov.au/def/qesd-qkd> ;
    skos:prefLabel "Dimensionless Ratio"@en ;
.

<https://linked.data.gov.au/def/qesd-qkd>
    a
        owl:Ontology ,
        skos:ConceptScheme ;
    dcterms:created "2021-04-16"^^xsd:date ;
    dcterms:creator <https://linked.data.gov.au/org/des> ;
    dcterms:modified "2023-03-10"^^xsd:date ;
    skos:historyNote "Derived from QUDT (http://qudt.org/vocab/quantitykind)" ;
    dcterms:publisher <https://linked.data.gov.au/org/des> ;
    skos:definition "This profile of the Quantities, Units, Dimensions & Types ontology and vocabularies lists those elements deemed by the profile creators to be of relevance to Queensland Environmental Science Data (QESD)."@en ;
    skos:editorialNote "The quantity kids from QUDT are a partial copy from the list of items provided from the QUDT public GitHub repositories (https://github.com/qudt/qudt-public-repo). Any quantity kinds created specificly for use in this vocabulary are to be explicitly marked with a source of this scheme. Additions to each term are to include them as an skos:Concept and skos:definition and include them explicitly in this ConceptScheme."@en ;
    skos:hasTopConcept
        quantitykind:Absorptance ,
        quantitykind:ActivityCoefficient ,
        quantitykind:AmountOfSubstance ,
        quantitykind:AmountOfSubstanceFractionOfB ,
        quantitykind:Angle ,
        quantitykind:Area ,
        quantitykind:Concentration ,
        quantitykind:Conductivity ,
        quantitykind:Dimensionless ,
        quantitykind:ElectricConductivity ,
        quantitykind:EnergyPerElectricCharge ,
        quantitykind:ExtentOfReaction ,
        quantitykind:ForcePerArea ,
        quantitykind:IonicStrength ,
        quantitykind:Length ,
        quantitykind:Mass ,
        quantitykind:MassDensity ,
        quantitykind:MassFraction ,
        quantitykind:MassFractionOfDryMatter ,
        quantitykind:MolalityOfSolute ,
        quantitykind:MultiplicationFactor ,
        quantitykind:Period ,
        quantitykind:RelativeHumidity ,
        quantitykind:RelativeMassDensity ,
        quantitykind:RelativePartialPressure ,
        quantitykind:StatisticalWeight ,
        quantitykind:Temperature ,
        quantitykind:Time ,
        quantitykind:Turbidity ,
        quantitykind:Volume ,
        quantitykind:VolumeFlowRate ,
        quantitykind:VolumePerUnitTime ;
    skos:prefLabel "Queensland Environmental Science Data Profile of QUDT Quantity Kinds"@en ;
.

