PREFIX adrss: <http://linked.data.gov.au/def/address-type/>
PREFIX agldwgstatus: <https://linked.data.gov.au/def/reg-statuses/>
PREFIX cs: <http://linked.data.gov.au/def/address-type>
PREFIX dcterms: <http://purl.org/dc/terms/>
PREFIX owl: <http://www.w3.org/2002/07/owl#>
PREFIX rdfs: <http://www.w3.org/2000/01/rdf-schema#>
PREFIX reg: <http://purl.org/linked-data/registry#>
PREFIX sdo: <https://schema.org/>
PREFIX skos: <http://www.w3.org/2004/02/skos/core#>
PREFIX xsd: <http://www.w3.org/2001/XMLSchema#>

adrss:business-address
    a skos:Concept ;
    skos:historyNote "Derived from  Australian Standard AS 4590.1:2017" ;
    rdfs:isDefinedBy cs: ;
    skos:altLabel
        "Company Address"@en ,
        "Office Address"@en ;
    skos:definition "The address of the principal place of business for the client."@en ;
    skos:inScheme cs: ;
    skos:notation "BUS" ;
    skos:prefLabel "Business Address"@en ;
    skos:topConceptOf cs: ;
.

adrss:delivery-address
    a skos:Concept ;
    skos:historyNote "Derived from  Australian Standard AS 4590.1:2017" ;
    rdfs:isDefinedBy cs: ;
    skos:definition "The address used for goods delivery purposes."@en ;
    skos:inScheme cs: ;
    skos:notation "DEL" ;
    skos:prefLabel "Delivery Address"@en ;
    skos:topConceptOf cs: ;
.

adrss:overseas-address
    a skos:Concept ;
    skos:historyNote "Derived from  Australian Standard AS 4590.1:2017" ;
    rdfs:isDefinedBy cs: ;
    skos:definition "The address used by the client when overseas."@en ;
    skos:inScheme cs: ;
    skos:notation "OVS" ;
    skos:prefLabel "Overseas Address"@en ;
    skos:topConceptOf cs: ;
.

adrss:postal-address
    a skos:Concept ;
    skos:historyNote "Derived from  Australian Standard AS 4590.1:2017" ;
    rdfs:isDefinedBy cs: ;
    skos:altLabel "Correspondence Address"@en ;
    skos:definition "The address used by the client for receipt of correspondence."@en ;
    skos:inScheme cs: ;
    skos:notation "POS" ;
    skos:prefLabel "Postal Address"@en ;
    skos:topConceptOf cs: ;
.

adrss:primary-property-address
    a skos:Concept ;
    skos:historyNote "Derived from  Australian Standard AS 4590.1:2017" ;
    rdfs:isDefinedBy cs: ;
    skos:definition "The property address normally used by the client."@en ;
    skos:inScheme cs: ;
    skos:notation "PR" ;
    skos:prefLabel "Primary Property Address"@en ;
    skos:topConceptOf cs: ;
.

adrss:residential-address
    a skos:Concept ;
    skos:historyNote "Derived from  Australian Standard AS 4590.1:2017" ;
    rdfs:isDefinedBy cs: ;
    skos:definition "The address of the principal place of residence for the client."@en ;
    skos:inScheme cs: ;
    skos:notation "RES" ;
    skos:prefLabel "Residential Address"@en ;
    skos:topConceptOf cs: ;
.

adrss:secondary-property-address
    a skos:Concept ;
    skos:historyNote "Derived from  Australian Standard AS 4590.1:2017" ;
    rdfs:isDefinedBy cs: ;
    skos:definition "The address of an additional property attached to the client."@en ;
    skos:inScheme cs: ;
    skos:notation "SEC" ;
    skos:prefLabel "Secondary Property Address"@en ;
    skos:topConceptOf cs: ;
.

<https://linked.data.gov.au/org/gsq>
    a sdo:Organization ;
    sdo:name "Geological Survey of Queensland" ;
    sdo:url "http://www.business.qld.gov.au/industries/mining-energy-water/resources/geoscience-information/gsq"^^xsd:anyURI ;
.

cs:
    a
        owl:Ontology ,
        skos:ConceptScheme ;
    dcterms:created "2020-03-25"^^xsd:date ;
    dcterms:creator <https://linked.data.gov.au/org/gsq> ;
    dcterms:modified "2023-03-16"^^xsd:date ;
    skos:historyNote "Derived from  Australian Standard AS 4590.1:2017" ;
    dcterms:publisher <https://linked.data.gov.au/org/gsq> ;
    reg:status agldwgstatus:stable ;
    skos:definition "The role or use of the address in relation to a party. An address may have more than one purpose."@en ;
    skos:hasTopConcept
        adrss:business-address ,
        adrss:delivery-address ,
        adrss:overseas-address ,
        adrss:postal-address ,
        adrss:primary-property-address ,
        adrss:residential-address ,
        adrss:secondary-property-address ;
    skos:prefLabel "Address Type"@en ;
.

