PREFIX agldwgstatus: <https://linked.data.gov.au/def/reg-statuses/>
PREFIX cs: <http://linked.data.gov.au/def/anzsic-2006>
PREFIX dcterms: <http://purl.org/dc/terms/>
PREFIX icat: <http://linked.data.gov.au/def/anzsic-2006/>
PREFIX owl: <http://www.w3.org/2002/07/owl#>
PREFIX prov: <http://www.w3.org/ns/prov#>
PREFIX rdfs: <http://www.w3.org/2000/01/rdf-schema#>
PREFIX reg: <http://purl.org/linked-data/registry#>
PREFIX sdo: <https://schema.org/>
PREFIX skos: <http://www.w3.org/2004/02/skos/core#>
PREFIX xsd: <http://www.w3.org/2001/XMLSchema#>

icat:A0110
    a skos:Concept ;
    dcterms:source "https://www.abs.gov.au/AUSSTATS/abs@.nsf/DetailsPage/1292.02006%20(Revision%202.0)?OpenDocument"^^xsd:anyURI ;
    rdfs:isDefinedBy cs: ;
    skos:broader icat:A0100 ;
    skos:definition "An individual business entity whose predominant economic activity is Nursery and Floriculture Production."@en ;
    skos:inScheme cs: ;
    skos:notation "A0110" ;
    skos:prefLabel "Nursery and Floriculture Production"@en ;
.

icat:A0120
    a skos:Concept ;
    dcterms:source "https://www.abs.gov.au/AUSSTATS/abs@.nsf/DetailsPage/1292.02006%20(Revision%202.0)?OpenDocument"^^xsd:anyURI ;
    rdfs:isDefinedBy cs: ;
    skos:broader icat:A0100 ;
    skos:definition "An individual business entity whose predominant economic activity is Mushroom and Vegetable Growing."@en ;
    skos:inScheme cs: ;
    skos:notation "A0120" ;
    skos:prefLabel "Mushroom and Vegetable Growing"@en ;
.

icat:A0130
    a skos:Concept ;
    dcterms:source "https://www.abs.gov.au/AUSSTATS/abs@.nsf/DetailsPage/1292.02006%20(Revision%202.0)?OpenDocument"^^xsd:anyURI ;
    rdfs:isDefinedBy cs: ;
    skos:broader icat:A0100 ;
    skos:definition "An individual business entity whose predominant economic activity is Fruit and Tree Nut Growing."@en ;
    skos:inScheme cs: ;
    skos:notation "A0130" ;
    skos:prefLabel "Fruit and Tree Nut Growing"@en ;
.

icat:A0140
    a skos:Concept ;
    dcterms:source "https://www.abs.gov.au/AUSSTATS/abs@.nsf/DetailsPage/1292.02006%20(Revision%202.0)?OpenDocument"^^xsd:anyURI ;
    rdfs:isDefinedBy cs: ;
    skos:broader icat:A0100 ;
    skos:definition "An individual business entity whose predominant economic activity is Sheep, Beef Cattle and Grain Farming."@en ;
    skos:inScheme cs: ;
    skos:notation "A0140" ;
    skos:prefLabel "Sheep, Beef Cattle and Grain Farming"@en ;
.

icat:A0150
    a skos:Concept ;
    dcterms:source "https://www.abs.gov.au/AUSSTATS/abs@.nsf/DetailsPage/1292.02006%20(Revision%202.0)?OpenDocument"^^xsd:anyURI ;
    rdfs:isDefinedBy cs: ;
    skos:broader icat:A0100 ;
    skos:definition "An individual business entity whose predominant economic activity is Other Crop Growing."@en ;
    skos:inScheme cs: ;
    skos:notation "A0150" ;
    skos:prefLabel "Other Crop Growing"@en ;
.

icat:A0160
    a skos:Concept ;
    dcterms:source "https://www.abs.gov.au/AUSSTATS/abs@.nsf/DetailsPage/1292.02006%20(Revision%202.0)?OpenDocument"^^xsd:anyURI ;
    rdfs:isDefinedBy cs: ;
    skos:broader icat:A0100 ;
    skos:definition "An individual business entity whose predominant economic activity is Dairy Cattle Farming."@en ;
    skos:inScheme cs: ;
    skos:notation "A0160" ;
    skos:prefLabel "Dairy Cattle Farming"@en ;
.

icat:A0170
    a skos:Concept ;
    dcterms:source "https://www.abs.gov.au/AUSSTATS/abs@.nsf/DetailsPage/1292.02006%20(Revision%202.0)?OpenDocument"^^xsd:anyURI ;
    rdfs:isDefinedBy cs: ;
    skos:broader icat:A0100 ;
    skos:definition "An individual business entity whose predominant economic activity is Poultry Farming."@en ;
    skos:inScheme cs: ;
    skos:notation "A0170" ;
    skos:prefLabel "Poultry Farming"@en ;
.

icat:A0180
    a skos:Concept ;
    dcterms:source "https://www.abs.gov.au/AUSSTATS/abs@.nsf/DetailsPage/1292.02006%20(Revision%202.0)?OpenDocument"^^xsd:anyURI ;
    rdfs:isDefinedBy cs: ;
    skos:broader icat:A0100 ;
    skos:definition "An individual business entity whose predominant economic activity is Deer Farming."@en ;
    skos:inScheme cs: ;
    skos:notation "A0180" ;
    skos:prefLabel "Deer Farming"@en ;
.

icat:A0190
    a skos:Concept ;
    dcterms:source "https://www.abs.gov.au/AUSSTATS/abs@.nsf/DetailsPage/1292.02006%20(Revision%202.0)?OpenDocument"^^xsd:anyURI ;
    rdfs:isDefinedBy cs: ;
    skos:broader icat:A0100 ;
    skos:definition "An individual business entity whose predominant economic activity is Other Livestock Farming."@en ;
    skos:inScheme cs: ;
    skos:notation "A0190" ;
    skos:prefLabel "Other Livestock Farming"@en ;
.

icat:A0200
    a skos:Concept ;
    dcterms:source "https://www.abs.gov.au/AUSSTATS/abs@.nsf/DetailsPage/1292.02006%20(Revision%202.0)?OpenDocument"^^xsd:anyURI ;
    rdfs:isDefinedBy cs: ;
    skos:broader icat:A0000 ;
    skos:definition "An individual business entity whose predominant economic activity is Aquaculture."@en ;
    skos:inScheme cs: ;
    skos:notation "A0200" ;
    skos:prefLabel "Aquaculture"@en ;
.

icat:A0300
    a skos:Concept ;
    dcterms:source "https://www.abs.gov.au/AUSSTATS/abs@.nsf/DetailsPage/1292.02006%20(Revision%202.0)?OpenDocument"^^xsd:anyURI ;
    rdfs:isDefinedBy cs: ;
    skos:broader icat:A0000 ;
    skos:definition "An individual business entity whose predominant economic activity is Forestry and Logging."@en ;
    skos:inScheme cs: ;
    skos:notation "A0300" ;
    skos:prefLabel "Forestry and Logging"@en ;
.

icat:A0410
    a skos:Concept ;
    dcterms:source "https://www.abs.gov.au/AUSSTATS/abs@.nsf/DetailsPage/1292.02006%20(Revision%202.0)?OpenDocument"^^xsd:anyURI ;
    rdfs:isDefinedBy cs: ;
    skos:broader icat:A0400 ;
    skos:definition "An individual business entity whose predominant economic activity is Fishing."@en ;
    skos:inScheme cs: ;
    skos:notation "A0410" ;
    skos:prefLabel "Fishing"@en ;
.

icat:A0420
    a skos:Concept ;
    dcterms:source "https://www.abs.gov.au/AUSSTATS/abs@.nsf/DetailsPage/1292.02006%20(Revision%202.0)?OpenDocument"^^xsd:anyURI ;
    rdfs:isDefinedBy cs: ;
    skos:broader icat:A0400 ;
    skos:definition "An individual business entity whose predominant economic activity is Hunting and Trapping."@en ;
    skos:inScheme cs: ;
    skos:notation "A0420" ;
    skos:prefLabel "Hunting and Trapping"@en ;
.

icat:A0510
    a skos:Concept ;
    dcterms:source "https://www.abs.gov.au/AUSSTATS/abs@.nsf/DetailsPage/1292.02006%20(Revision%202.0)?OpenDocument"^^xsd:anyURI ;
    rdfs:isDefinedBy cs: ;
    skos:broader icat:A0500 ;
    skos:definition "An individual business entity whose predominant economic activity is Forestry Support Services."@en ;
    skos:inScheme cs: ;
    skos:notation "A0510" ;
    skos:prefLabel "Forestry Support Services"@en ;
.

icat:A0520
    a skos:Concept ;
    dcterms:source "https://www.abs.gov.au/AUSSTATS/abs@.nsf/DetailsPage/1292.02006%20(Revision%202.0)?OpenDocument"^^xsd:anyURI ;
    rdfs:isDefinedBy cs: ;
    skos:broader icat:A0500 ;
    skos:definition "An individual business entity whose predominant economic activity is Agriculture and Fishing Support Services."@en ;
    skos:inScheme cs: ;
    skos:notation "A0520" ;
    skos:prefLabel "Agriculture and Fishing Support Services"@en ;
.

icat:B0700
    a skos:Concept ;
    dcterms:source "https://www.abs.gov.au/AUSSTATS/abs@.nsf/DetailsPage/1292.02006%20(Revision%202.0)?OpenDocument"^^xsd:anyURI ;
    rdfs:isDefinedBy cs: ;
    skos:broader icat:B0000 ;
    skos:definition "An individual business entity whose predominant economic activity is Oil and Gas Extraction."@en ;
    skos:inScheme cs: ;
    skos:notation "B0700" ;
    skos:prefLabel "Oil and Gas Extraction"@en ;
.

icat:B0800
    a skos:Concept ;
    dcterms:source "https://www.abs.gov.au/AUSSTATS/abs@.nsf/DetailsPage/1292.02006%20(Revision%202.0)?OpenDocument"^^xsd:anyURI ;
    rdfs:isDefinedBy cs: ;
    skos:broader icat:B0000 ;
    skos:definition "An individual business entity whose predominant economic activity is Metal Ore Mining."@en ;
    skos:inScheme cs: ;
    skos:notation "B0800" ;
    skos:prefLabel "Metal Ore Mining"@en ;
.

icat:B0910
    a skos:Concept ;
    dcterms:source "https://www.abs.gov.au/AUSSTATS/abs@.nsf/DetailsPage/1292.02006%20(Revision%202.0)?OpenDocument"^^xsd:anyURI ;
    rdfs:isDefinedBy cs: ;
    skos:broader icat:B0900 ;
    skos:definition "An individual business entity whose predominant economic activity is Construction Material Mining."@en ;
    skos:inScheme cs: ;
    skos:notation "B0910" ;
    skos:prefLabel "Construction Material Mining"@en ;
.

icat:B0990
    a skos:Concept ;
    dcterms:source "https://www.abs.gov.au/AUSSTATS/abs@.nsf/DetailsPage/1292.02006%20(Revision%202.0)?OpenDocument"^^xsd:anyURI ;
    rdfs:isDefinedBy cs: ;
    skos:broader icat:B0900 ;
    skos:definition "An individual business entity whose predominant economic activity is Other Non-Metallic Mineral Mining and Quarrying."@en ;
    skos:inScheme cs: ;
    skos:notation "B0990" ;
    skos:prefLabel "Other Non-Metallic Mineral Mining and Quarrying"@en ;
.

icat:B1010
    a skos:Concept ;
    dcterms:source "https://www.abs.gov.au/AUSSTATS/abs@.nsf/DetailsPage/1292.02006%20(Revision%202.0)?OpenDocument"^^xsd:anyURI ;
    rdfs:isDefinedBy cs: ;
    skos:broader icat:B1000 ;
    skos:definition "An individual business entity whose predominant economic activity is Exploration."@en ;
    skos:inScheme cs: ;
    skos:notation "B1010" ;
    skos:prefLabel "Exploration"@en ;
.

icat:B1090
    a skos:Concept ;
    dcterms:source "https://www.abs.gov.au/AUSSTATS/abs@.nsf/DetailsPage/1292.02006%20(Revision%202.0)?OpenDocument"^^xsd:anyURI ;
    rdfs:isDefinedBy cs: ;
    skos:broader icat:B1000 ;
    skos:definition "An individual business entity whose predominant economic activity is Other Mining Support Services."@en ;
    skos:inScheme cs: ;
    skos:notation "B1090" ;
    skos:prefLabel "Other Mining Support Services"@en ;
.

icat:C1110
    a skos:Concept ;
    dcterms:source "https://www.abs.gov.au/AUSSTATS/abs@.nsf/DetailsPage/1292.02006%20(Revision%202.0)?OpenDocument"^^xsd:anyURI ;
    rdfs:isDefinedBy cs: ;
    skos:broader icat:C1100 ;
    skos:definition "An individual business entity whose predominant economic activity is Meat and Meat Product Manufacturing."@en ;
    skos:inScheme cs: ;
    skos:notation "C1110" ;
    skos:prefLabel "Meat and Meat Product Manufacturing"@en ;
.

icat:C1120
    a skos:Concept ;
    dcterms:source "https://www.abs.gov.au/AUSSTATS/abs@.nsf/DetailsPage/1292.02006%20(Revision%202.0)?OpenDocument"^^xsd:anyURI ;
    rdfs:isDefinedBy cs: ;
    skos:broader icat:C1100 ;
    skos:definition "An individual business entity whose predominant economic activity is Seafood Processing."@en ;
    skos:inScheme cs: ;
    skos:notation "C1120" ;
    skos:prefLabel "Seafood Processing"@en ;
.

icat:C1130
    a skos:Concept ;
    dcterms:source "https://www.abs.gov.au/AUSSTATS/abs@.nsf/DetailsPage/1292.02006%20(Revision%202.0)?OpenDocument"^^xsd:anyURI ;
    rdfs:isDefinedBy cs: ;
    skos:broader icat:C1100 ;
    skos:definition "An individual business entity whose predominant economic activity is Dairy Product Manufacturing."@en ;
    skos:inScheme cs: ;
    skos:notation "C1130" ;
    skos:prefLabel "Dairy Product Manufacturing"@en ;
.

icat:C1140
    a skos:Concept ;
    dcterms:source "https://www.abs.gov.au/AUSSTATS/abs@.nsf/DetailsPage/1292.02006%20(Revision%202.0)?OpenDocument"^^xsd:anyURI ;
    rdfs:isDefinedBy cs: ;
    skos:broader icat:C1100 ;
    skos:definition "An individual business entity whose predominant economic activity is Fruit and Vegetable Processing."@en ;
    skos:inScheme cs: ;
    skos:notation "C1140" ;
    skos:prefLabel "Fruit and Vegetable Processing"@en ;
.

icat:C1150
    a skos:Concept ;
    dcterms:source "https://www.abs.gov.au/AUSSTATS/abs@.nsf/DetailsPage/1292.02006%20(Revision%202.0)?OpenDocument"^^xsd:anyURI ;
    rdfs:isDefinedBy cs: ;
    skos:broader icat:C1100 ;
    skos:definition "An individual business entity whose predominant economic activity is Oil and Fat Manufacturing."@en ;
    skos:inScheme cs: ;
    skos:notation "C1150" ;
    skos:prefLabel "Oil and Fat Manufacturing"@en ;
.

icat:C1160
    a skos:Concept ;
    dcterms:source "https://www.abs.gov.au/AUSSTATS/abs@.nsf/DetailsPage/1292.02006%20(Revision%202.0)?OpenDocument"^^xsd:anyURI ;
    rdfs:isDefinedBy cs: ;
    skos:broader icat:C1100 ;
    skos:definition "An individual business entity whose predominant economic activity is Grain Mill and Cereal Product Manufacturing."@en ;
    skos:inScheme cs: ;
    skos:notation "C1160" ;
    skos:prefLabel "Grain Mill and Cereal Product Manufacturing"@en ;
.

icat:C1170
    a skos:Concept ;
    dcterms:source "https://www.abs.gov.au/AUSSTATS/abs@.nsf/DetailsPage/1292.02006%20(Revision%202.0)?OpenDocument"^^xsd:anyURI ;
    rdfs:isDefinedBy cs: ;
    skos:broader icat:C1100 ;
    skos:definition "An individual business entity whose predominant economic activity is Bakery Product Manufacturing."@en ;
    skos:inScheme cs: ;
    skos:notation "C1170" ;
    skos:prefLabel "Bakery Product Manufacturing"@en ;
.

icat:C1180
    a skos:Concept ;
    dcterms:source "https://www.abs.gov.au/AUSSTATS/abs@.nsf/DetailsPage/1292.02006%20(Revision%202.0)?OpenDocument"^^xsd:anyURI ;
    rdfs:isDefinedBy cs: ;
    skos:broader icat:C1100 ;
    skos:definition "An individual business entity whose predominant economic activity is Sugar and Confectionery Manufacturing."@en ;
    skos:inScheme cs: ;
    skos:notation "C1180" ;
    skos:prefLabel "Sugar and Confectionery Manufacturing"@en ;
.

icat:C1190
    a skos:Concept ;
    dcterms:source "https://www.abs.gov.au/AUSSTATS/abs@.nsf/DetailsPage/1292.02006%20(Revision%202.0)?OpenDocument"^^xsd:anyURI ;
    rdfs:isDefinedBy cs: ;
    skos:broader icat:C1100 ;
    skos:definition "An individual business entity whose predominant economic activity is Other Food Product Manufacturing."@en ;
    skos:inScheme cs: ;
    skos:notation "C1190" ;
    skos:prefLabel "Other Food Product Manufacturing"@en ;
.

icat:C1210
    a skos:Concept ;
    dcterms:source "https://www.abs.gov.au/AUSSTATS/abs@.nsf/DetailsPage/1292.02006%20(Revision%202.0)?OpenDocument"^^xsd:anyURI ;
    rdfs:isDefinedBy cs: ;
    skos:broader icat:C1200 ;
    skos:definition "An individual business entity whose predominant economic activity is Beverage Manufacturing."@en ;
    skos:inScheme cs: ;
    skos:notation "C1210" ;
    skos:prefLabel "Beverage Manufacturing"@en ;
.

icat:C1220
    a skos:Concept ;
    dcterms:source "https://www.abs.gov.au/AUSSTATS/abs@.nsf/DetailsPage/1292.02006%20(Revision%202.0)?OpenDocument"^^xsd:anyURI ;
    rdfs:isDefinedBy cs: ;
    skos:broader icat:C1200 ;
    skos:definition "An individual business entity whose predominant economic activity is Cigarette and Tobacco Product Manufacturing."@en ;
    skos:inScheme cs: ;
    skos:notation "C1220" ;
    skos:prefLabel "Cigarette and Tobacco Product Manufacturing"@en ;
.

icat:C1310
    a skos:Concept ;
    dcterms:source "https://www.abs.gov.au/AUSSTATS/abs@.nsf/DetailsPage/1292.02006%20(Revision%202.0)?OpenDocument"^^xsd:anyURI ;
    rdfs:isDefinedBy cs: ;
    skos:broader icat:C1300 ;
    skos:definition "An individual business entity whose predominant economic activity is Textile Manufacturing."@en ;
    skos:inScheme cs: ;
    skos:notation "C1310" ;
    skos:prefLabel "Textile Manufacturing"@en ;
.

icat:C1320
    a skos:Concept ;
    dcterms:source "https://www.abs.gov.au/AUSSTATS/abs@.nsf/DetailsPage/1292.02006%20(Revision%202.0)?OpenDocument"^^xsd:anyURI ;
    rdfs:isDefinedBy cs: ;
    skos:broader icat:C1300 ;
    skos:definition "An individual business entity whose predominant economic activity is Leather Tanning, Fur Dressing and Leather Product Manufacturing."@en ;
    skos:inScheme cs: ;
    skos:notation "C1320" ;
    skos:prefLabel "Leather Tanning, Fur Dressing and Leather Product Manufacturing"@en ;
.

icat:C1330
    a skos:Concept ;
    dcterms:source "https://www.abs.gov.au/AUSSTATS/abs@.nsf/DetailsPage/1292.02006%20(Revision%202.0)?OpenDocument"^^xsd:anyURI ;
    rdfs:isDefinedBy cs: ;
    skos:broader icat:C1300 ;
    skos:definition "An individual business entity whose predominant economic activity is Textile Product Manufacturing."@en ;
    skos:inScheme cs: ;
    skos:notation "C1330" ;
    skos:prefLabel "Textile Product Manufacturing"@en ;
.

icat:C1340
    a skos:Concept ;
    dcterms:source "https://www.abs.gov.au/AUSSTATS/abs@.nsf/DetailsPage/1292.02006%20(Revision%202.0)?OpenDocument"^^xsd:anyURI ;
    rdfs:isDefinedBy cs: ;
    skos:broader icat:C1300 ;
    skos:definition "An individual business entity whose predominant economic activity is Knitted Product Manufacturing."@en ;
    skos:inScheme cs: ;
    skos:notation "C1340" ;
    skos:prefLabel "Knitted Product Manufacturing"@en ;
.

icat:C1350
    a skos:Concept ;
    dcterms:source "https://www.abs.gov.au/AUSSTATS/abs@.nsf/DetailsPage/1292.02006%20(Revision%202.0)?OpenDocument"^^xsd:anyURI ;
    rdfs:isDefinedBy cs: ;
    skos:broader icat:C1300 ;
    skos:definition "An individual business entity whose predominant economic activity is Clothing and Footwear Manufacturing."@en ;
    skos:inScheme cs: ;
    skos:notation "C1350" ;
    skos:prefLabel "Clothing and Footwear Manufacturing"@en ;
.

icat:C1410
    a skos:Concept ;
    dcterms:source "https://www.abs.gov.au/AUSSTATS/abs@.nsf/DetailsPage/1292.02006%20(Revision%202.0)?OpenDocument"^^xsd:anyURI ;
    rdfs:isDefinedBy cs: ;
    skos:broader icat:C1400 ;
    skos:definition "An individual business entity whose predominant economic activity is Log Sawmilling and Timber Dressing."@en ;
    skos:inScheme cs: ;
    skos:notation "C1410" ;
    skos:prefLabel "Log Sawmilling and Timber Dressing"@en ;
.

icat:C1490
    a skos:Concept ;
    dcterms:source "https://www.abs.gov.au/AUSSTATS/abs@.nsf/DetailsPage/1292.02006%20(Revision%202.0)?OpenDocument"^^xsd:anyURI ;
    rdfs:isDefinedBy cs: ;
    skos:broader icat:C1400 ;
    skos:definition "An individual business entity whose predominant economic activity is Other Wood Product Manufacturing."@en ;
    skos:inScheme cs: ;
    skos:notation "C1490" ;
    skos:prefLabel "Other Wood Product Manufacturing"@en ;
.

icat:C1510
    a skos:Concept ;
    dcterms:source "https://www.abs.gov.au/AUSSTATS/abs@.nsf/DetailsPage/1292.02006%20(Revision%202.0)?OpenDocument"^^xsd:anyURI ;
    rdfs:isDefinedBy cs: ;
    skos:broader icat:C1500 ;
    skos:definition "An individual business entity whose predominant economic activity is Pulp, Paper and Paperboard Manufacturing."@en ;
    skos:inScheme cs: ;
    skos:notation "C1510" ;
    skos:prefLabel "Pulp, Paper and Paperboard Manufacturing"@en ;
.

icat:C1520
    a skos:Concept ;
    dcterms:source "https://www.abs.gov.au/AUSSTATS/abs@.nsf/DetailsPage/1292.02006%20(Revision%202.0)?OpenDocument"^^xsd:anyURI ;
    rdfs:isDefinedBy cs: ;
    skos:broader icat:C1500 ;
    skos:definition "An individual business entity whose predominant economic activity is Converted Paper Product Manufacturing."@en ;
    skos:inScheme cs: ;
    skos:notation "C1520" ;
    skos:prefLabel "Converted Paper Product Manufacturing"@en ;
.

icat:C1610
    a skos:Concept ;
    dcterms:source "https://www.abs.gov.au/AUSSTATS/abs@.nsf/DetailsPage/1292.02006%20(Revision%202.0)?OpenDocument"^^xsd:anyURI ;
    rdfs:isDefinedBy cs: ;
    skos:broader icat:C1600 ;
    skos:definition "An individual business entity whose predominant economic activity is Printing and Printing Support Services."@en ;
    skos:inScheme cs: ;
    skos:notation "C1610" ;
    skos:prefLabel "Printing and Printing Support Services"@en ;
.

icat:C1620
    a skos:Concept ;
    dcterms:source "https://www.abs.gov.au/AUSSTATS/abs@.nsf/DetailsPage/1292.02006%20(Revision%202.0)?OpenDocument"^^xsd:anyURI ;
    rdfs:isDefinedBy cs: ;
    skos:broader icat:C1600 ;
    skos:definition "An individual business entity whose predominant economic activity is Reproduction of Recorded Media."@en ;
    skos:inScheme cs: ;
    skos:notation "C1620" ;
    skos:prefLabel "Reproduction of Recorded Media"@en ;
.

icat:C1700
    a skos:Concept ;
    dcterms:source "https://www.abs.gov.au/AUSSTATS/abs@.nsf/DetailsPage/1292.02006%20(Revision%202.0)?OpenDocument"^^xsd:anyURI ;
    rdfs:isDefinedBy cs: ;
    skos:broader icat:C0000 ;
    skos:definition "An individual business entity whose predominant economic activity is Petroleum and Coal Product Manufacturing."@en ;
    skos:inScheme cs: ;
    skos:notation "C1700" ;
    skos:prefLabel "Petroleum and Coal Product Manufacturing"@en ;
.

icat:C1810
    a skos:Concept ;
    dcterms:source "https://www.abs.gov.au/AUSSTATS/abs@.nsf/DetailsPage/1292.02006%20(Revision%202.0)?OpenDocument"^^xsd:anyURI ;
    rdfs:isDefinedBy cs: ;
    skos:broader icat:C1800 ;
    skos:definition "An individual business entity whose predominant economic activity is Basic Chemical Manufacturing."@en ;
    skos:inScheme cs: ;
    skos:notation "C1810" ;
    skos:prefLabel "Basic Chemical Manufacturing"@en ;
.

icat:C1820
    a skos:Concept ;
    dcterms:source "https://www.abs.gov.au/AUSSTATS/abs@.nsf/DetailsPage/1292.02006%20(Revision%202.0)?OpenDocument"^^xsd:anyURI ;
    rdfs:isDefinedBy cs: ;
    skos:broader icat:C1800 ;
    skos:definition "An individual business entity whose predominant economic activity is Basic Polymer Manufacturing."@en ;
    skos:inScheme cs: ;
    skos:notation "C1820" ;
    skos:prefLabel "Basic Polymer Manufacturing"@en ;
.

icat:C1830
    a skos:Concept ;
    dcterms:source "https://www.abs.gov.au/AUSSTATS/abs@.nsf/DetailsPage/1292.02006%20(Revision%202.0)?OpenDocument"^^xsd:anyURI ;
    rdfs:isDefinedBy cs: ;
    skos:broader icat:C1800 ;
    skos:definition "An individual business entity whose predominant economic activity is Fertiliser and Pesticide Manufacturing."@en ;
    skos:inScheme cs: ;
    skos:notation "C1830" ;
    skos:prefLabel "Fertiliser and Pesticide Manufacturing"@en ;
.

icat:C1840
    a skos:Concept ;
    dcterms:source "https://www.abs.gov.au/AUSSTATS/abs@.nsf/DetailsPage/1292.02006%20(Revision%202.0)?OpenDocument"^^xsd:anyURI ;
    rdfs:isDefinedBy cs: ;
    skos:broader icat:C1800 ;
    skos:definition "An individual business entity whose predominant economic activity is Pharmaceutical and Medicinal Product Manufacturing."@en ;
    skos:inScheme cs: ;
    skos:notation "C1840" ;
    skos:prefLabel "Pharmaceutical and Medicinal Product Manufacturing"@en ;
.

icat:C1850
    a skos:Concept ;
    dcterms:source "https://www.abs.gov.au/AUSSTATS/abs@.nsf/DetailsPage/1292.02006%20(Revision%202.0)?OpenDocument"^^xsd:anyURI ;
    rdfs:isDefinedBy cs: ;
    skos:broader icat:C1800 ;
    skos:definition "An individual business entity whose predominant economic activity is Cleaning Compound and Toiletry Preparation Manufacturing."@en ;
    skos:inScheme cs: ;
    skos:notation "C1850" ;
    skos:prefLabel "Cleaning Compound and Toiletry Preparation Manufacturing"@en ;
.

icat:C1890
    a skos:Concept ;
    dcterms:source "https://www.abs.gov.au/AUSSTATS/abs@.nsf/DetailsPage/1292.02006%20(Revision%202.0)?OpenDocument"^^xsd:anyURI ;
    rdfs:isDefinedBy cs: ;
    skos:broader icat:C1800 ;
    skos:definition "An individual business entity whose predominant economic activity is Other Basic Chemical Product Manufacturing."@en ;
    skos:inScheme cs: ;
    skos:notation "C1890" ;
    skos:prefLabel "Other Basic Chemical Product Manufacturing"@en ;
.

icat:C1910
    a skos:Concept ;
    dcterms:source "https://www.abs.gov.au/AUSSTATS/abs@.nsf/DetailsPage/1292.02006%20(Revision%202.0)?OpenDocument"^^xsd:anyURI ;
    rdfs:isDefinedBy cs: ;
    skos:broader icat:C1900 ;
    skos:definition "An individual business entity whose predominant economic activity is Polymer Product Manufacturing."@en ;
    skos:inScheme cs: ;
    skos:notation "C1910" ;
    skos:prefLabel "Polymer Product Manufacturing"@en ;
.

icat:C1920
    a skos:Concept ;
    dcterms:source "https://www.abs.gov.au/AUSSTATS/abs@.nsf/DetailsPage/1292.02006%20(Revision%202.0)?OpenDocument"^^xsd:anyURI ;
    rdfs:isDefinedBy cs: ;
    skos:broader icat:C1900 ;
    skos:definition "An individual business entity whose predominant economic activity is Natural Rubber Product Manufacturing."@en ;
    skos:inScheme cs: ;
    skos:notation "C1920" ;
    skos:prefLabel "Natural Rubber Product Manufacturing"@en ;
.

icat:C2010
    a skos:Concept ;
    dcterms:source "https://www.abs.gov.au/AUSSTATS/abs@.nsf/DetailsPage/1292.02006%20(Revision%202.0)?OpenDocument"^^xsd:anyURI ;
    rdfs:isDefinedBy cs: ;
    skos:broader icat:C2000 ;
    skos:definition "An individual business entity whose predominant economic activity is Glass and Glass Product Manufacturing."@en ;
    skos:inScheme cs: ;
    skos:notation "C2010" ;
    skos:prefLabel "Glass and Glass Product Manufacturing"@en ;
.

icat:C2020
    a skos:Concept ;
    dcterms:source "https://www.abs.gov.au/AUSSTATS/abs@.nsf/DetailsPage/1292.02006%20(Revision%202.0)?OpenDocument"^^xsd:anyURI ;
    rdfs:isDefinedBy cs: ;
    skos:broader icat:C2000 ;
    skos:definition "An individual business entity whose predominant economic activity is Ceramic Product Manufacturing."@en ;
    skos:inScheme cs: ;
    skos:notation "C2020" ;
    skos:prefLabel "Ceramic Product Manufacturing"@en ;
.

icat:C2030
    a skos:Concept ;
    dcterms:source "https://www.abs.gov.au/AUSSTATS/abs@.nsf/DetailsPage/1292.02006%20(Revision%202.0)?OpenDocument"^^xsd:anyURI ;
    rdfs:isDefinedBy cs: ;
    skos:broader icat:C2000 ;
    skos:definition "An individual business entity whose predominant economic activity is Cement, Lime, Plaster and Concrete Product Manufacturing."@en ;
    skos:inScheme cs: ;
    skos:notation "C2030" ;
    skos:prefLabel "Cement, Lime, Plaster and Concrete Product Manufacturing"@en ;
.

icat:C2090
    a skos:Concept ;
    dcterms:source "https://www.abs.gov.au/AUSSTATS/abs@.nsf/DetailsPage/1292.02006%20(Revision%202.0)?OpenDocument"^^xsd:anyURI ;
    rdfs:isDefinedBy cs: ;
    skos:broader icat:C2000 ;
    skos:definition "An individual business entity whose predominant economic activity is Other Non-Metallic Mineral Product Manufacturing."@en ;
    skos:inScheme cs: ;
    skos:notation "C2090" ;
    skos:prefLabel "Other Non-Metallic Mineral Product Manufacturing"@en ;
.

icat:C2110
    a skos:Concept ;
    dcterms:source "https://www.abs.gov.au/AUSSTATS/abs@.nsf/DetailsPage/1292.02006%20(Revision%202.0)?OpenDocument"^^xsd:anyURI ;
    rdfs:isDefinedBy cs: ;
    skos:broader icat:C2100 ;
    skos:definition "An individual business entity whose predominant economic activity is Basic Ferrous Metal Manufacturing."@en ;
    skos:inScheme cs: ;
    skos:notation "C2110" ;
    skos:prefLabel "Basic Ferrous Metal Manufacturing"@en ;
.

icat:C2120
    a skos:Concept ;
    dcterms:source "https://www.abs.gov.au/AUSSTATS/abs@.nsf/DetailsPage/1292.02006%20(Revision%202.0)?OpenDocument"^^xsd:anyURI ;
    rdfs:isDefinedBy cs: ;
    skos:broader icat:C2100 ;
    skos:definition "An individual business entity whose predominant economic activity is Basic Ferrous Metal Product Manufacturing."@en ;
    skos:inScheme cs: ;
    skos:notation "C2120" ;
    skos:prefLabel "Basic Ferrous Metal Product Manufacturing"@en ;
.

icat:C2130
    a skos:Concept ;
    dcterms:source "https://www.abs.gov.au/AUSSTATS/abs@.nsf/DetailsPage/1292.02006%20(Revision%202.0)?OpenDocument"^^xsd:anyURI ;
    rdfs:isDefinedBy cs: ;
    skos:broader icat:C2100 ;
    skos:definition "An individual business entity whose predominant economic activity is Basic Non-Ferrous Metal Manufacturing."@en ;
    skos:inScheme cs: ;
    skos:notation "C2130" ;
    skos:prefLabel "Basic Non-Ferrous Metal Manufacturing"@en ;
.

icat:C2140
    a skos:Concept ;
    dcterms:source "https://www.abs.gov.au/AUSSTATS/abs@.nsf/DetailsPage/1292.02006%20(Revision%202.0)?OpenDocument"^^xsd:anyURI ;
    rdfs:isDefinedBy cs: ;
    skos:broader icat:C2100 ;
    skos:definition "An individual business entity whose predominant economic activity is Basic Non-Ferrous Metal Product Manufacturing."@en ;
    skos:inScheme cs: ;
    skos:notation "C2140" ;
    skos:prefLabel "Basic Non-Ferrous Metal Product Manufacturing"@en ;
.

icat:C2210
    a skos:Concept ;
    dcterms:source "https://www.abs.gov.au/AUSSTATS/abs@.nsf/DetailsPage/1292.02006%20(Revision%202.0)?OpenDocument"^^xsd:anyURI ;
    rdfs:isDefinedBy cs: ;
    skos:broader icat:C2200 ;
    skos:definition "An individual business entity whose predominant economic activity is Iron and Steel Forging."@en ;
    skos:inScheme cs: ;
    skos:notation "C2210" ;
    skos:prefLabel "Iron and Steel Forging"@en ;
.

icat:C2220
    a skos:Concept ;
    dcterms:source "https://www.abs.gov.au/AUSSTATS/abs@.nsf/DetailsPage/1292.02006%20(Revision%202.0)?OpenDocument"^^xsd:anyURI ;
    rdfs:isDefinedBy cs: ;
    skos:broader icat:C2200 ;
    skos:definition "An individual business entity whose predominant economic activity is Structural Metal Product Manufacturing."@en ;
    skos:inScheme cs: ;
    skos:notation "C2220" ;
    skos:prefLabel "Structural Metal Product Manufacturing"@en ;
.

icat:C2230
    a skos:Concept ;
    dcterms:source "https://www.abs.gov.au/AUSSTATS/abs@.nsf/DetailsPage/1292.02006%20(Revision%202.0)?OpenDocument"^^xsd:anyURI ;
    rdfs:isDefinedBy cs: ;
    skos:broader icat:C2200 ;
    skos:definition "An individual business entity whose predominant economic activity is Metal Container Manufacturing."@en ;
    skos:inScheme cs: ;
    skos:notation "C2230" ;
    skos:prefLabel "Metal Container Manufacturing"@en ;
.

icat:C2240
    a skos:Concept ;
    dcterms:source "https://www.abs.gov.au/AUSSTATS/abs@.nsf/DetailsPage/1292.02006%20(Revision%202.0)?OpenDocument"^^xsd:anyURI ;
    rdfs:isDefinedBy cs: ;
    skos:broader icat:C2200 ;
    skos:definition "An individual business entity whose predominant economic activity is Sheet Metal Product Manufacturing (except Metal Structural and Container Products)."@en ;
    skos:inScheme cs: ;
    skos:notation "C2240" ;
    skos:prefLabel "Sheet Metal Product Manufacturing (except Metal Structural and Container Products)"@en ;
.

icat:C2290
    a skos:Concept ;
    dcterms:source "https://www.abs.gov.au/AUSSTATS/abs@.nsf/DetailsPage/1292.02006%20(Revision%202.0)?OpenDocument"^^xsd:anyURI ;
    rdfs:isDefinedBy cs: ;
    skos:broader icat:C2200 ;
    skos:definition "An individual business entity whose predominant economic activity is Other Fabricated Metal Product Manufacturing."@en ;
    skos:inScheme cs: ;
    skos:notation "C2290" ;
    skos:prefLabel "Other Fabricated Metal Product Manufacturing"@en ;
.

icat:C2310
    a skos:Concept ;
    dcterms:source "https://www.abs.gov.au/AUSSTATS/abs@.nsf/DetailsPage/1292.02006%20(Revision%202.0)?OpenDocument"^^xsd:anyURI ;
    rdfs:isDefinedBy cs: ;
    skos:broader icat:C2300 ;
    skos:definition "An individual business entity whose predominant economic activity is Motor Vehicle and Motor Vehicle Part Manufacturing."@en ;
    skos:inScheme cs: ;
    skos:notation "C2310" ;
    skos:prefLabel "Motor Vehicle and Motor Vehicle Part Manufacturing"@en ;
.

icat:C2390
    a skos:Concept ;
    dcterms:source "https://www.abs.gov.au/AUSSTATS/abs@.nsf/DetailsPage/1292.02006%20(Revision%202.0)?OpenDocument"^^xsd:anyURI ;
    rdfs:isDefinedBy cs: ;
    skos:broader icat:C2300 ;
    skos:definition "An individual business entity whose predominant economic activity is Other Transport Equipment Manufacturing."@en ;
    skos:inScheme cs: ;
    skos:notation "C2390" ;
    skos:prefLabel "Other Transport Equipment Manufacturing"@en ;
.

icat:C2410
    a skos:Concept ;
    dcterms:source "https://www.abs.gov.au/AUSSTATS/abs@.nsf/DetailsPage/1292.02006%20(Revision%202.0)?OpenDocument"^^xsd:anyURI ;
    rdfs:isDefinedBy cs: ;
    skos:broader icat:C2400 ;
    skos:definition "An individual business entity whose predominant economic activity is Professional and Scientific Equipment Manufacturing."@en ;
    skos:inScheme cs: ;
    skos:notation "C2410" ;
    skos:prefLabel "Professional and Scientific Equipment Manufacturing"@en ;
.

icat:C2420
    a skos:Concept ;
    dcterms:source "https://www.abs.gov.au/AUSSTATS/abs@.nsf/DetailsPage/1292.02006%20(Revision%202.0)?OpenDocument"^^xsd:anyURI ;
    rdfs:isDefinedBy cs: ;
    skos:broader icat:C2400 ;
    skos:definition "An individual business entity whose predominant economic activity is Computer and Electronic Equipment Manufacturing."@en ;
    skos:inScheme cs: ;
    skos:notation "C2420" ;
    skos:prefLabel "Computer and Electronic Equipment Manufacturing"@en ;
.

icat:C2430
    a skos:Concept ;
    dcterms:source "https://www.abs.gov.au/AUSSTATS/abs@.nsf/DetailsPage/1292.02006%20(Revision%202.0)?OpenDocument"^^xsd:anyURI ;
    rdfs:isDefinedBy cs: ;
    skos:broader icat:C2400 ;
    skos:definition "An individual business entity whose predominant economic activity is Electrical Equipment Manufacturing."@en ;
    skos:inScheme cs: ;
    skos:notation "C2430" ;
    skos:prefLabel "Electrical Equipment Manufacturing"@en ;
.

icat:C2440
    a skos:Concept ;
    dcterms:source "https://www.abs.gov.au/AUSSTATS/abs@.nsf/DetailsPage/1292.02006%20(Revision%202.0)?OpenDocument"^^xsd:anyURI ;
    rdfs:isDefinedBy cs: ;
    skos:broader icat:C2400 ;
    skos:definition "An individual business entity whose predominant economic activity is Domestic Appliance Manufacturing."@en ;
    skos:inScheme cs: ;
    skos:notation "C2440" ;
    skos:prefLabel "Domestic Appliance Manufacturing"@en ;
.

icat:C2450
    a skos:Concept ;
    dcterms:source "https://www.abs.gov.au/AUSSTATS/abs@.nsf/DetailsPage/1292.02006%20(Revision%202.0)?OpenDocument"^^xsd:anyURI ;
    rdfs:isDefinedBy cs: ;
    skos:broader icat:C2400 ;
    skos:definition "An individual business entity whose predominant economic activity is Pump, Compressor, Heating and Ventilation Equipment Manufacturing."@en ;
    skos:inScheme cs: ;
    skos:notation "C2450" ;
    skos:prefLabel "Pump, Compressor, Heating and Ventilation Equipment Manufacturing"@en ;
.

icat:C2460
    a skos:Concept ;
    dcterms:source "https://www.abs.gov.au/AUSSTATS/abs@.nsf/DetailsPage/1292.02006%20(Revision%202.0)?OpenDocument"^^xsd:anyURI ;
    rdfs:isDefinedBy cs: ;
    skos:broader icat:C2400 ;
    skos:definition "An individual business entity whose predominant economic activity is Specialised Machinery and Equipment Manufacturing."@en ;
    skos:inScheme cs: ;
    skos:notation "C2460" ;
    skos:prefLabel "Specialised Machinery and Equipment Manufacturing"@en ;
.

icat:C2490
    a skos:Concept ;
    dcterms:source "https://www.abs.gov.au/AUSSTATS/abs@.nsf/DetailsPage/1292.02006%20(Revision%202.0)?OpenDocument"^^xsd:anyURI ;
    rdfs:isDefinedBy cs: ;
    skos:broader icat:C2400 ;
    skos:definition "An individual business entity whose predominant economic activity is Other Machinery and Equipment Manufacturing."@en ;
    skos:inScheme cs: ;
    skos:notation "C2490" ;
    skos:prefLabel "Other Machinery and Equipment Manufacturing"@en ;
.

icat:C2510
    a skos:Concept ;
    dcterms:source "https://www.abs.gov.au/AUSSTATS/abs@.nsf/DetailsPage/1292.02006%20(Revision%202.0)?OpenDocument"^^xsd:anyURI ;
    rdfs:isDefinedBy cs: ;
    skos:broader icat:C2500 ;
    skos:definition "An individual business entity whose predominant economic activity is Furniture Manufacturing."@en ;
    skos:inScheme cs: ;
    skos:notation "C2510" ;
    skos:prefLabel "Furniture Manufacturing"@en ;
.

icat:C2590
    a skos:Concept ;
    dcterms:source "https://www.abs.gov.au/AUSSTATS/abs@.nsf/DetailsPage/1292.02006%20(Revision%202.0)?OpenDocument"^^xsd:anyURI ;
    rdfs:isDefinedBy cs: ;
    skos:broader icat:C2500 ;
    skos:definition "An individual business entity whose predominant economic activity is Other Manufacturing."@en ;
    skos:inScheme cs: ;
    skos:notation "C2590" ;
    skos:prefLabel "Other Manufacturing"@en ;
.

icat:D2620
    a skos:Concept ;
    dcterms:source "https://www.abs.gov.au/AUSSTATS/abs@.nsf/DetailsPage/1292.02006%20(Revision%202.0)?OpenDocument"^^xsd:anyURI ;
    rdfs:isDefinedBy cs: ;
    skos:broader icat:D2600 ;
    skos:definition "An individual business entity whose predominant economic activity is Electricity Transmission."@en ;
    skos:inScheme cs: ;
    skos:notation "D2620" ;
    skos:prefLabel "Electricity Transmission"@en ;
.

icat:D2630
    a skos:Concept ;
    dcterms:source "https://www.abs.gov.au/AUSSTATS/abs@.nsf/DetailsPage/1292.02006%20(Revision%202.0)?OpenDocument"^^xsd:anyURI ;
    rdfs:isDefinedBy cs: ;
    skos:broader icat:D2600 ;
    skos:definition "An individual business entity whose predominant economic activity is Electricity Distribution."@en ;
    skos:inScheme cs: ;
    skos:notation "D2630" ;
    skos:prefLabel "Electricity Distribution"@en ;
.

icat:D2640
    a skos:Concept ;
    dcterms:source "https://www.abs.gov.au/AUSSTATS/abs@.nsf/DetailsPage/1292.02006%20(Revision%202.0)?OpenDocument"^^xsd:anyURI ;
    rdfs:isDefinedBy cs: ;
    skos:broader icat:D2600 ;
    skos:definition "An individual business entity whose predominant economic activity is On Selling Electricity and Electricity Market Operation."@en ;
    skos:inScheme cs: ;
    skos:notation "D2640" ;
    skos:prefLabel "On Selling Electricity and Electricity Market Operation"@en ;
.

icat:D2700
    a skos:Concept ;
    dcterms:source "https://www.abs.gov.au/AUSSTATS/abs@.nsf/DetailsPage/1292.02006%20(Revision%202.0)?OpenDocument"^^xsd:anyURI ;
    rdfs:isDefinedBy cs: ;
    skos:broader icat:D0000 ;
    skos:definition "An individual business entity whose predominant economic activity is Gas Supply."@en ;
    skos:inScheme cs: ;
    skos:notation "D2700" ;
    skos:prefLabel "Gas Supply"@en ;
.

icat:D2800
    a skos:Concept ;
    dcterms:source "https://www.abs.gov.au/AUSSTATS/abs@.nsf/DetailsPage/1292.02006%20(Revision%202.0)?OpenDocument"^^xsd:anyURI ;
    rdfs:isDefinedBy cs: ;
    skos:broader icat:D0000 ;
    skos:definition "An individual business entity whose predominant economic activity is Water Supply, Sewerage and Drainage Services."@en ;
    skos:inScheme cs: ;
    skos:notation "D2800" ;
    skos:prefLabel "Water Supply, Sewerage and Drainage Services"@en ;
.

icat:D2910
    a skos:Concept ;
    dcterms:source "https://www.abs.gov.au/AUSSTATS/abs@.nsf/DetailsPage/1292.02006%20(Revision%202.0)?OpenDocument"^^xsd:anyURI ;
    rdfs:isDefinedBy cs: ;
    skos:broader icat:D2900 ;
    skos:definition "An individual business entity whose predominant economic activity is Waste Collection Services."@en ;
    skos:inScheme cs: ;
    skos:notation "D2910" ;
    skos:prefLabel "Waste Collection Services"@en ;
.

icat:D2920
    a skos:Concept ;
    dcterms:source "https://www.abs.gov.au/AUSSTATS/abs@.nsf/DetailsPage/1292.02006%20(Revision%202.0)?OpenDocument"^^xsd:anyURI ;
    rdfs:isDefinedBy cs: ;
    skos:broader icat:D2900 ;
    skos:definition "An individual business entity whose predominant economic activity is Waste Treatment, Disposal and Remediation Services."@en ;
    skos:inScheme cs: ;
    skos:notation "D2920" ;
    skos:prefLabel "Waste Treatment, Disposal and Remediation Services"@en ;
.

icat:E3010
    a skos:Concept ;
    dcterms:source "https://www.abs.gov.au/AUSSTATS/abs@.nsf/DetailsPage/1292.02006%20(Revision%202.0)?OpenDocument"^^xsd:anyURI ;
    rdfs:isDefinedBy cs: ;
    skos:broader icat:E3000 ;
    skos:definition "An individual business entity whose predominant economic activity is Residential Building Construction."@en ;
    skos:inScheme cs: ;
    skos:notation "E3010" ;
    skos:prefLabel "Residential Building Construction"@en ;
.

icat:E3020
    a skos:Concept ;
    dcterms:source "https://www.abs.gov.au/AUSSTATS/abs@.nsf/DetailsPage/1292.02006%20(Revision%202.0)?OpenDocument"^^xsd:anyURI ;
    rdfs:isDefinedBy cs: ;
    skos:broader icat:E3000 ;
    skos:definition "An individual business entity whose predominant economic activity is Non-Residential Building Construction."@en ;
    skos:inScheme cs: ;
    skos:notation "E3020" ;
    skos:prefLabel "Non-Residential Building Construction"@en ;
.

icat:E3100
    a skos:Concept ;
    dcterms:source "https://www.abs.gov.au/AUSSTATS/abs@.nsf/DetailsPage/1292.02006%20(Revision%202.0)?OpenDocument"^^xsd:anyURI ;
    rdfs:isDefinedBy cs: ;
    skos:broader icat:E0000 ;
    skos:definition "An individual business entity whose predominant economic activity is Heavy and Civil Engineering Construction."@en ;
    skos:inScheme cs: ;
    skos:notation "E3100" ;
    skos:prefLabel "Heavy and Civil Engineering Construction"@en ;
.

icat:E3210
    a skos:Concept ;
    dcterms:source "https://www.abs.gov.au/AUSSTATS/abs@.nsf/DetailsPage/1292.02006%20(Revision%202.0)?OpenDocument"^^xsd:anyURI ;
    rdfs:isDefinedBy cs: ;
    skos:broader icat:E3200 ;
    skos:definition "An individual business entity whose predominant economic activity is Land Development and Site Preparation Services."@en ;
    skos:inScheme cs: ;
    skos:notation "E3210" ;
    skos:prefLabel "Land Development and Site Preparation Services"@en ;
.

icat:E3220
    a skos:Concept ;
    dcterms:source "https://www.abs.gov.au/AUSSTATS/abs@.nsf/DetailsPage/1292.02006%20(Revision%202.0)?OpenDocument"^^xsd:anyURI ;
    rdfs:isDefinedBy cs: ;
    skos:broader icat:E3200 ;
    skos:definition "An individual business entity whose predominant economic activity is Building Structure Services."@en ;
    skos:inScheme cs: ;
    skos:notation "E3220" ;
    skos:prefLabel "Building Structure Services"@en ;
.

icat:E3230
    a skos:Concept ;
    dcterms:source "https://www.abs.gov.au/AUSSTATS/abs@.nsf/DetailsPage/1292.02006%20(Revision%202.0)?OpenDocument"^^xsd:anyURI ;
    rdfs:isDefinedBy cs: ;
    skos:broader icat:E3200 ;
    skos:definition "An individual business entity whose predominant economic activity is Building Installation Services."@en ;
    skos:inScheme cs: ;
    skos:notation "E3230" ;
    skos:prefLabel "Building Installation Services"@en ;
.

icat:E3240
    a skos:Concept ;
    dcterms:source "https://www.abs.gov.au/AUSSTATS/abs@.nsf/DetailsPage/1292.02006%20(Revision%202.0)?OpenDocument"^^xsd:anyURI ;
    rdfs:isDefinedBy cs: ;
    skos:broader icat:E3200 ;
    skos:definition "An individual business entity whose predominant economic activity is Building Completion Services."@en ;
    skos:inScheme cs: ;
    skos:notation "E3240" ;
    skos:prefLabel "Building Completion Services"@en ;
.

icat:E3290
    a skos:Concept ;
    dcterms:source "https://www.abs.gov.au/AUSSTATS/abs@.nsf/DetailsPage/1292.02006%20(Revision%202.0)?OpenDocument"^^xsd:anyURI ;
    rdfs:isDefinedBy cs: ;
    skos:broader icat:E3200 ;
    skos:definition "An individual business entity whose predominant economic activity is Other Construction Services."@en ;
    skos:inScheme cs: ;
    skos:notation "E3290" ;
    skos:prefLabel "Other Construction Services"@en ;
.

icat:F3310
    a skos:Concept ;
    dcterms:source "https://www.abs.gov.au/AUSSTATS/abs@.nsf/DetailsPage/1292.02006%20(Revision%202.0)?OpenDocument"^^xsd:anyURI ;
    rdfs:isDefinedBy cs: ;
    skos:broader icat:F3300 ;
    skos:definition "An individual business entity whose predominant economic activity is Agricultural Product Wholesaling."@en ;
    skos:inScheme cs: ;
    skos:notation "F3310" ;
    skos:prefLabel "Agricultural Product Wholesaling"@en ;
.

icat:F3320
    a skos:Concept ;
    dcterms:source "https://www.abs.gov.au/AUSSTATS/abs@.nsf/DetailsPage/1292.02006%20(Revision%202.0)?OpenDocument"^^xsd:anyURI ;
    rdfs:isDefinedBy cs: ;
    skos:broader icat:F3300 ;
    skos:definition "An individual business entity whose predominant economic activity is Mineral, Metal and Chemical Wholesaling."@en ;
    skos:inScheme cs: ;
    skos:notation "F3320" ;
    skos:prefLabel "Mineral, Metal and Chemical Wholesaling"@en ;
.

icat:F3330
    a skos:Concept ;
    dcterms:source "https://www.abs.gov.au/AUSSTATS/abs@.nsf/DetailsPage/1292.02006%20(Revision%202.0)?OpenDocument"^^xsd:anyURI ;
    rdfs:isDefinedBy cs: ;
    skos:broader icat:F3300 ;
    skos:definition "An individual business entity whose predominant economic activity is Timber and Hardware Goods Wholesaling."@en ;
    skos:inScheme cs: ;
    skos:notation "F3330" ;
    skos:prefLabel "Timber and Hardware Goods Wholesaling"@en ;
.

icat:F3410
    a skos:Concept ;
    dcterms:source "https://www.abs.gov.au/AUSSTATS/abs@.nsf/DetailsPage/1292.02006%20(Revision%202.0)?OpenDocument"^^xsd:anyURI ;
    rdfs:isDefinedBy cs: ;
    skos:broader icat:F3400 ;
    skos:definition "An individual business entity whose predominant economic activity is Specialised Industrial Machinery and Equipment Wholesaling."@en ;
    skos:inScheme cs: ;
    skos:notation "F3410" ;
    skos:prefLabel "Specialised Industrial Machinery and Equipment Wholesaling"@en ;
.

icat:F3490
    a skos:Concept ;
    dcterms:source "https://www.abs.gov.au/AUSSTATS/abs@.nsf/DetailsPage/1292.02006%20(Revision%202.0)?OpenDocument"^^xsd:anyURI ;
    rdfs:isDefinedBy cs: ;
    skos:broader icat:F3400 ;
    skos:definition "An individual business entity whose predominant economic activity is Other Machinery and Equipment Wholesaling."@en ;
    skos:inScheme cs: ;
    skos:notation "F3490" ;
    skos:prefLabel "Other Machinery and Equipment Wholesaling"@en ;
.

icat:F3500
    a skos:Concept ;
    dcterms:source "https://www.abs.gov.au/AUSSTATS/abs@.nsf/DetailsPage/1292.02006%20(Revision%202.0)?OpenDocument"^^xsd:anyURI ;
    rdfs:isDefinedBy cs: ;
    skos:broader icat:F0000 ;
    skos:definition "An individual business entity whose predominant economic activity is Motor Vehicle and Motor Vehicle Parts Wholesaling."@en ;
    skos:inScheme cs: ;
    skos:notation "F3500" ;
    skos:prefLabel "Motor Vehicle and Motor Vehicle Parts Wholesaling"@en ;
.

icat:F3600
    a skos:Concept ;
    dcterms:source "https://www.abs.gov.au/AUSSTATS/abs@.nsf/DetailsPage/1292.02006%20(Revision%202.0)?OpenDocument"^^xsd:anyURI ;
    rdfs:isDefinedBy cs: ;
    skos:broader icat:F0000 ;
    skos:definition "An individual business entity whose predominant economic activity is Grocery, Liquor and Tobacco Product Wholesaling."@en ;
    skos:inScheme cs: ;
    skos:notation "F3600" ;
    skos:prefLabel "Grocery, Liquor and Tobacco Product Wholesaling"@en ;
.

icat:F3710
    a skos:Concept ;
    dcterms:source "https://www.abs.gov.au/AUSSTATS/abs@.nsf/DetailsPage/1292.02006%20(Revision%202.0)?OpenDocument"^^xsd:anyURI ;
    rdfs:isDefinedBy cs: ;
    skos:broader icat:F3700 ;
    skos:definition "An individual business entity whose predominant economic activity is Textile, Clothing and Footwear Wholesaling."@en ;
    skos:inScheme cs: ;
    skos:notation "F3710" ;
    skos:prefLabel "Textile, Clothing and Footwear Wholesaling"@en ;
.

icat:F3720
    a skos:Concept ;
    dcterms:source "https://www.abs.gov.au/AUSSTATS/abs@.nsf/DetailsPage/1292.02006%20(Revision%202.0)?OpenDocument"^^xsd:anyURI ;
    rdfs:isDefinedBy cs: ;
    skos:broader icat:F3700 ;
    skos:definition "An individual business entity whose predominant economic activity is Pharmaceutical and Toiletry Goods Wholesaling."@en ;
    skos:inScheme cs: ;
    skos:notation "F3720" ;
    skos:prefLabel "Pharmaceutical and Toiletry Goods Wholesaling"@en ;
.

icat:F3730
    a skos:Concept ;
    dcterms:source "https://www.abs.gov.au/AUSSTATS/abs@.nsf/DetailsPage/1292.02006%20(Revision%202.0)?OpenDocument"^^xsd:anyURI ;
    rdfs:isDefinedBy cs: ;
    skos:broader icat:F3700 ;
    skos:definition "An individual business entity whose predominant economic activity is Furniture, Floor Covering and Other Goods Wholesaling."@en ;
    skos:inScheme cs: ;
    skos:notation "F3730" ;
    skos:prefLabel "Furniture, Floor Covering and Other Goods Wholesaling"@en ;
.

icat:F3800
    a skos:Concept ;
    dcterms:source "https://www.abs.gov.au/AUSSTATS/abs@.nsf/DetailsPage/1292.02006%20(Revision%202.0)?OpenDocument"^^xsd:anyURI ;
    rdfs:isDefinedBy cs: ;
    skos:broader icat:F0000 ;
    skos:definition "An individual business entity whose predominant economic activity is Commission-Based Wholesaling."@en ;
    skos:inScheme cs: ;
    skos:notation "F3800" ;
    skos:prefLabel "Commission-Based Wholesaling"@en ;
.

icat:G3910
    a skos:Concept ;
    dcterms:source "https://www.abs.gov.au/AUSSTATS/abs@.nsf/DetailsPage/1292.02006%20(Revision%202.0)?OpenDocument"^^xsd:anyURI ;
    rdfs:isDefinedBy cs: ;
    skos:broader icat:G3900 ;
    skos:definition "An individual business entity whose predominant economic activity is Motor Vehicle Retailing."@en ;
    skos:inScheme cs: ;
    skos:notation "G3910" ;
    skos:prefLabel "Motor Vehicle Retailing"@en ;
.

icat:G3920
    a skos:Concept ;
    dcterms:source "https://www.abs.gov.au/AUSSTATS/abs@.nsf/DetailsPage/1292.02006%20(Revision%202.0)?OpenDocument"^^xsd:anyURI ;
    rdfs:isDefinedBy cs: ;
    skos:broader icat:G3900 ;
    skos:definition "An individual business entity whose predominant economic activity is Motor Vehicle Parts and Tyre Retailing."@en ;
    skos:inScheme cs: ;
    skos:notation "G3920" ;
    skos:prefLabel "Motor Vehicle Parts and Tyre Retailing"@en ;
.

icat:G4000
    a skos:Concept ;
    dcterms:source "https://www.abs.gov.au/AUSSTATS/abs@.nsf/DetailsPage/1292.02006%20(Revision%202.0)?OpenDocument"^^xsd:anyURI ;
    rdfs:isDefinedBy cs: ;
    skos:broader icat:G0000 ;
    skos:definition "An individual business entity whose predominant economic activity is Fuel Retailing."@en ;
    skos:inScheme cs: ;
    skos:notation "G4000" ;
    skos:prefLabel "Fuel Retailing"@en ;
.

icat:G4110
    a skos:Concept ;
    dcterms:source "https://www.abs.gov.au/AUSSTATS/abs@.nsf/DetailsPage/1292.02006%20(Revision%202.0)?OpenDocument"^^xsd:anyURI ;
    rdfs:isDefinedBy cs: ;
    skos:broader icat:G4100 ;
    skos:definition "An individual business entity whose predominant economic activity is Supermarket and Grocery Stores."@en ;
    skos:inScheme cs: ;
    skos:notation "G4110" ;
    skos:prefLabel "Supermarket and Grocery Stores"@en ;
.

icat:G4120
    a skos:Concept ;
    dcterms:source "https://www.abs.gov.au/AUSSTATS/abs@.nsf/DetailsPage/1292.02006%20(Revision%202.0)?OpenDocument"^^xsd:anyURI ;
    rdfs:isDefinedBy cs: ;
    skos:broader icat:G4100 ;
    skos:definition "An individual business entity whose predominant economic activity is Specialised Food Retailing."@en ;
    skos:inScheme cs: ;
    skos:notation "G4120" ;
    skos:prefLabel "Specialised Food Retailing"@en ;
.

icat:G4210
    a skos:Concept ;
    dcterms:source "https://www.abs.gov.au/AUSSTATS/abs@.nsf/DetailsPage/1292.02006%20(Revision%202.0)?OpenDocument"^^xsd:anyURI ;
    rdfs:isDefinedBy cs: ;
    skos:broader icat:G4200 ;
    skos:definition "An individual business entity whose predominant economic activity is Furniture, Floor Coverings, Houseware and Textile Goods Retailing."@en ;
    skos:inScheme cs: ;
    skos:notation "G4210" ;
    skos:prefLabel "Furniture, Floor Coverings, Houseware and Textile Goods Retailing"@en ;
.

icat:G4220
    a skos:Concept ;
    dcterms:source "https://www.abs.gov.au/AUSSTATS/abs@.nsf/DetailsPage/1292.02006%20(Revision%202.0)?OpenDocument"^^xsd:anyURI ;
    rdfs:isDefinedBy cs: ;
    skos:broader icat:G4200 ;
    skos:definition "An individual business entity whose predominant economic activity is Electrical and Electronic Goods Retailing."@en ;
    skos:inScheme cs: ;
    skos:notation "G4220" ;
    skos:prefLabel "Electrical and Electronic Goods Retailing"@en ;
.

icat:G4230
    a skos:Concept ;
    dcterms:source "https://www.abs.gov.au/AUSSTATS/abs@.nsf/DetailsPage/1292.02006%20(Revision%202.0)?OpenDocument"^^xsd:anyURI ;
    rdfs:isDefinedBy cs: ;
    skos:broader icat:G4200 ;
    skos:definition "An individual business entity whose predominant economic activity is Hardware, Building and Garden Supplies Retailing."@en ;
    skos:inScheme cs: ;
    skos:notation "G4230" ;
    skos:prefLabel "Hardware, Building and Garden Supplies Retailing"@en ;
.

icat:G4240
    a skos:Concept ;
    dcterms:source "https://www.abs.gov.au/AUSSTATS/abs@.nsf/DetailsPage/1292.02006%20(Revision%202.0)?OpenDocument"^^xsd:anyURI ;
    rdfs:isDefinedBy cs: ;
    skos:broader icat:G4200 ;
    skos:definition "An individual business entity whose predominant economic activity is Recreational Goods Retailing."@en ;
    skos:inScheme cs: ;
    skos:notation "G4240" ;
    skos:prefLabel "Recreational Goods Retailing"@en ;
.

icat:G4250
    a skos:Concept ;
    dcterms:source "https://www.abs.gov.au/AUSSTATS/abs@.nsf/DetailsPage/1292.02006%20(Revision%202.0)?OpenDocument"^^xsd:anyURI ;
    rdfs:isDefinedBy cs: ;
    skos:broader icat:G4200 ;
    skos:definition "An individual business entity whose predominant economic activity is Clothing, Footwear and Personal Accessory Retailing."@en ;
    skos:inScheme cs: ;
    skos:notation "G4250" ;
    skos:prefLabel "Clothing, Footwear and Personal Accessory Retailing"@en ;
.

icat:G4260
    a skos:Concept ;
    dcterms:source "https://www.abs.gov.au/AUSSTATS/abs@.nsf/DetailsPage/1292.02006%20(Revision%202.0)?OpenDocument"^^xsd:anyURI ;
    rdfs:isDefinedBy cs: ;
    skos:broader icat:G4200 ;
    skos:definition "An individual business entity whose predominant economic activity is Department Stores."@en ;
    skos:inScheme cs: ;
    skos:notation "G4260" ;
    skos:prefLabel "Department Stores"@en ;
.

icat:G4270
    a skos:Concept ;
    dcterms:source "https://www.abs.gov.au/AUSSTATS/abs@.nsf/DetailsPage/1292.02006%20(Revision%202.0)?OpenDocument"^^xsd:anyURI ;
    rdfs:isDefinedBy cs: ;
    skos:broader icat:G4200 ;
    skos:definition "An individual business entity whose predominant economic activity is Pharmaceutical and Other Store-Based Retailing."@en ;
    skos:inScheme cs: ;
    skos:notation "G4270" ;
    skos:prefLabel "Pharmaceutical and Other Store-Based Retailing"@en ;
.

icat:G4310
    a skos:Concept ;
    dcterms:source "https://www.abs.gov.au/AUSSTATS/abs@.nsf/DetailsPage/1292.02006%20(Revision%202.0)?OpenDocument"^^xsd:anyURI ;
    rdfs:isDefinedBy cs: ;
    skos:broader icat:G4300 ;
    skos:definition "An individual business entity whose predominant economic activity is Non-Store Retailing."@en ;
    skos:inScheme cs: ;
    skos:notation "G4310" ;
    skos:prefLabel "Non-Store Retailing"@en ;
.

icat:G4320
    a skos:Concept ;
    dcterms:source "https://www.abs.gov.au/AUSSTATS/abs@.nsf/DetailsPage/1292.02006%20(Revision%202.0)?OpenDocument"^^xsd:anyURI ;
    rdfs:isDefinedBy cs: ;
    skos:broader icat:G4300 ;
    skos:definition "An individual business entity whose predominant economic activity is Retail Commission-Based Buying and/or Selling."@en ;
    skos:inScheme cs: ;
    skos:notation "G4320" ;
    skos:prefLabel "Retail Commission-Based Buying and/or Selling"@en ;
.

icat:H4400
    a skos:Concept ;
    dcterms:source "https://www.abs.gov.au/AUSSTATS/abs@.nsf/DetailsPage/1292.02006%20(Revision%202.0)?OpenDocument"^^xsd:anyURI ;
    rdfs:isDefinedBy cs: ;
    skos:broader icat:H0000 ;
    skos:definition "An individual business entity whose predominant economic activity is Accommodation."@en ;
    skos:inScheme cs: ;
    skos:notation "H4400" ;
    skos:prefLabel "Accommodation"@en ;
.

icat:H4510
    a skos:Concept ;
    dcterms:source "https://www.abs.gov.au/AUSSTATS/abs@.nsf/DetailsPage/1292.02006%20(Revision%202.0)?OpenDocument"^^xsd:anyURI ;
    rdfs:isDefinedBy cs: ;
    skos:broader icat:H4500 ;
    skos:definition "An individual business entity whose predominant economic activity is Cafes, Restaurants and Takeaway Food Services."@en ;
    skos:inScheme cs: ;
    skos:notation "H4510" ;
    skos:prefLabel "Cafes, Restaurants and Takeaway Food Services"@en ;
.

icat:H4520
    a skos:Concept ;
    dcterms:source "https://www.abs.gov.au/AUSSTATS/abs@.nsf/DetailsPage/1292.02006%20(Revision%202.0)?OpenDocument"^^xsd:anyURI ;
    rdfs:isDefinedBy cs: ;
    skos:broader icat:H4500 ;
    skos:definition "An individual business entity whose predominant economic activity is Pubs, Taverns and Bars."@en ;
    skos:inScheme cs: ;
    skos:notation "H4520" ;
    skos:prefLabel "Pubs, Taverns and Bars"@en ;
.

icat:H4530
    a skos:Concept ;
    dcterms:source "https://www.abs.gov.au/AUSSTATS/abs@.nsf/DetailsPage/1292.02006%20(Revision%202.0)?OpenDocument"^^xsd:anyURI ;
    rdfs:isDefinedBy cs: ;
    skos:broader icat:H4500 ;
    skos:definition "An individual business entity whose predominant economic activity is Clubs (Hospitality)."@en ;
    skos:inScheme cs: ;
    skos:notation "H4530" ;
    skos:prefLabel "Clubs (Hospitality)"@en ;
.

icat:I4610
    a skos:Concept ;
    dcterms:source "https://www.abs.gov.au/AUSSTATS/abs@.nsf/DetailsPage/1292.02006%20(Revision%202.0)?OpenDocument"^^xsd:anyURI ;
    rdfs:isDefinedBy cs: ;
    skos:broader icat:I4600 ;
    skos:definition "An individual business entity whose predominant economic activity is Road Freight Transport."@en ;
    skos:inScheme cs: ;
    skos:notation "I4610" ;
    skos:prefLabel "Road Freight Transport"@en ;
.

icat:I4620
    a skos:Concept ;
    dcterms:source "https://www.abs.gov.au/AUSSTATS/abs@.nsf/DetailsPage/1292.02006%20(Revision%202.0)?OpenDocument"^^xsd:anyURI ;
    rdfs:isDefinedBy cs: ;
    skos:broader icat:I4600 ;
    skos:definition "An individual business entity whose predominant economic activity is Road Passenger Transport."@en ;
    skos:inScheme cs: ;
    skos:notation "I4620" ;
    skos:prefLabel "Road Passenger Transport"@en ;
.

icat:I4710
    a skos:Concept ;
    dcterms:source "https://www.abs.gov.au/AUSSTATS/abs@.nsf/DetailsPage/1292.02006%20(Revision%202.0)?OpenDocument"^^xsd:anyURI ;
    rdfs:isDefinedBy cs: ;
    skos:broader icat:I4700 ;
    skos:definition "An individual business entity whose predominant economic activity is Rail Freight Transport."@en ;
    skos:inScheme cs: ;
    skos:notation "I4710" ;
    skos:prefLabel "Rail Freight Transport"@en ;
.

icat:I4720
    a skos:Concept ;
    dcterms:source "https://www.abs.gov.au/AUSSTATS/abs@.nsf/DetailsPage/1292.02006%20(Revision%202.0)?OpenDocument"^^xsd:anyURI ;
    rdfs:isDefinedBy cs: ;
    skos:broader icat:I4700 ;
    skos:definition "An individual business entity whose predominant economic activity is Rail Passenger Transport."@en ;
    skos:inScheme cs: ;
    skos:notation "I4720" ;
    skos:prefLabel "Rail Passenger Transport"@en ;
.

icat:I4810
    a skos:Concept ;
    dcterms:source "https://www.abs.gov.au/AUSSTATS/abs@.nsf/DetailsPage/1292.02006%20(Revision%202.0)?OpenDocument"^^xsd:anyURI ;
    rdfs:isDefinedBy cs: ;
    skos:broader icat:I4800 ;
    skos:definition "An individual business entity whose predominant economic activity is Water Freight Transport."@en ;
    skos:inScheme cs: ;
    skos:notation "I4810" ;
    skos:prefLabel "Water Freight Transport"@en ;
.

icat:I4820
    a skos:Concept ;
    dcterms:source "https://www.abs.gov.au/AUSSTATS/abs@.nsf/DetailsPage/1292.02006%20(Revision%202.0)?OpenDocument"^^xsd:anyURI ;
    rdfs:isDefinedBy cs: ;
    skos:broader icat:I4800 ;
    skos:definition "An individual business entity whose predominant economic activity is Water Passenger Transport."@en ;
    skos:inScheme cs: ;
    skos:notation "I4820" ;
    skos:prefLabel "Water Passenger Transport"@en ;
.

icat:I4900
    a skos:Concept ;
    dcterms:source "https://www.abs.gov.au/AUSSTATS/abs@.nsf/DetailsPage/1292.02006%20(Revision%202.0)?OpenDocument"^^xsd:anyURI ;
    rdfs:isDefinedBy cs: ;
    skos:broader icat:I0000 ;
    skos:definition "An individual business entity whose predominant economic activity is Air and Space Transport."@en ;
    skos:inScheme cs: ;
    skos:notation "I4900" ;
    skos:prefLabel "Air and Space Transport"@en ;
.

icat:I5010
    a skos:Concept ;
    dcterms:source "https://www.abs.gov.au/AUSSTATS/abs@.nsf/DetailsPage/1292.02006%20(Revision%202.0)?OpenDocument"^^xsd:anyURI ;
    rdfs:isDefinedBy cs: ;
    skos:broader icat:I5000 ;
    skos:definition "An individual business entity whose predominant economic activity is Scenic and Sightseeing Transport."@en ;
    skos:inScheme cs: ;
    skos:notation "I5010" ;
    skos:prefLabel "Scenic and Sightseeing Transport"@en ;
.

icat:I5020
    a skos:Concept ;
    dcterms:source "https://www.abs.gov.au/AUSSTATS/abs@.nsf/DetailsPage/1292.02006%20(Revision%202.0)?OpenDocument"^^xsd:anyURI ;
    rdfs:isDefinedBy cs: ;
    skos:broader icat:I5000 ;
    skos:definition "An individual business entity whose predominant economic activity is Pipeline and Other Transport."@en ;
    skos:inScheme cs: ;
    skos:notation "I5020" ;
    skos:prefLabel "Pipeline and Other Transport"@en ;
.

icat:I5100
    a skos:Concept ;
    dcterms:source "https://www.abs.gov.au/AUSSTATS/abs@.nsf/DetailsPage/1292.02006%20(Revision%202.0)?OpenDocument"^^xsd:anyURI ;
    rdfs:isDefinedBy cs: ;
    skos:broader icat:I0000 ;
    skos:definition "An individual business entity whose predominant economic activity is Postal and Courier Pick-up and Delivery Services."@en ;
    skos:inScheme cs: ;
    skos:notation "I5100" ;
    skos:prefLabel "Postal and Courier Pick-up and Delivery Services"@en ;
.

icat:I5210
    a skos:Concept ;
    dcterms:source "https://www.abs.gov.au/AUSSTATS/abs@.nsf/DetailsPage/1292.02006%20(Revision%202.0)?OpenDocument"^^xsd:anyURI ;
    rdfs:isDefinedBy cs: ;
    skos:broader icat:I5200 ;
    skos:definition "An individual business entity whose predominant economic activity is Water Transport Support Services."@en ;
    skos:inScheme cs: ;
    skos:notation "I5210" ;
    skos:prefLabel "Water Transport Support Services"@en ;
.

icat:I5220
    a skos:Concept ;
    dcterms:source "https://www.abs.gov.au/AUSSTATS/abs@.nsf/DetailsPage/1292.02006%20(Revision%202.0)?OpenDocument"^^xsd:anyURI ;
    rdfs:isDefinedBy cs: ;
    skos:broader icat:I5200 ;
    skos:definition "An individual business entity whose predominant economic activity is Airport Operations and Other Air Transport Support Services."@en ;
    skos:inScheme cs: ;
    skos:notation "I5220" ;
    skos:prefLabel "Airport Operations and Other Air Transport Support Services"@en ;
.

icat:I5290
    a skos:Concept ;
    dcterms:source "https://www.abs.gov.au/AUSSTATS/abs@.nsf/DetailsPage/1292.02006%20(Revision%202.0)?OpenDocument"^^xsd:anyURI ;
    rdfs:isDefinedBy cs: ;
    skos:broader icat:I5200 ;
    skos:definition "An individual business entity whose predominant economic activity is Other Transport Support Services."@en ;
    skos:inScheme cs: ;
    skos:notation "I5290" ;
    skos:prefLabel "Other Transport Support Services"@en ;
.

icat:I5300
    a skos:Concept ;
    dcterms:source "https://www.abs.gov.au/AUSSTATS/abs@.nsf/DetailsPage/1292.02006%20(Revision%202.0)?OpenDocument"^^xsd:anyURI ;
    rdfs:isDefinedBy cs: ;
    skos:broader icat:I0000 ;
    skos:definition "An individual business entity whose predominant economic activity is Warehousing and Storage Services."@en ;
    skos:inScheme cs: ;
    skos:notation "I5300" ;
    skos:prefLabel "Warehousing and Storage Services"@en ;
.

icat:J5410
    a skos:Concept ;
    dcterms:source "https://www.abs.gov.au/AUSSTATS/abs@.nsf/DetailsPage/1292.02006%20(Revision%202.0)?OpenDocument"^^xsd:anyURI ;
    rdfs:isDefinedBy cs: ;
    skos:broader icat:J5400 ;
    skos:definition "An individual business entity whose predominant economic activity is Newspaper, Periodical, Book and Directory Publishing."@en ;
    skos:inScheme cs: ;
    skos:notation "J5410" ;
    skos:prefLabel "Newspaper, Periodical, Book and Directory Publishing"@en ;
.

icat:J5420
    a skos:Concept ;
    dcterms:source "https://www.abs.gov.au/AUSSTATS/abs@.nsf/DetailsPage/1292.02006%20(Revision%202.0)?OpenDocument"^^xsd:anyURI ;
    rdfs:isDefinedBy cs: ;
    skos:broader icat:J5400 ;
    skos:definition "An individual business entity whose predominant economic activity is Software Publishing."@en ;
    skos:inScheme cs: ;
    skos:notation "J5420" ;
    skos:prefLabel "Software Publishing"@en ;
.

icat:J5510
    a skos:Concept ;
    dcterms:source "https://www.abs.gov.au/AUSSTATS/abs@.nsf/DetailsPage/1292.02006%20(Revision%202.0)?OpenDocument"^^xsd:anyURI ;
    rdfs:isDefinedBy cs: ;
    skos:broader icat:J5500 ;
    skos:definition "An individual business entity whose predominant economic activity is Motion Picture and Video Activities."@en ;
    skos:inScheme cs: ;
    skos:notation "J5510" ;
    skos:prefLabel "Motion Picture and Video Activities"@en ;
.

icat:J5520
    a skos:Concept ;
    dcterms:source "https://www.abs.gov.au/AUSSTATS/abs@.nsf/DetailsPage/1292.02006%20(Revision%202.0)?OpenDocument"^^xsd:anyURI ;
    rdfs:isDefinedBy cs: ;
    skos:broader icat:J5500 ;
    skos:definition "An individual business entity whose predominant economic activity is Sound Recording and Music Publishing."@en ;
    skos:inScheme cs: ;
    skos:notation "J5520" ;
    skos:prefLabel "Sound Recording and Music Publishing"@en ;
.

icat:J5610
    a skos:Concept ;
    dcterms:source "https://www.abs.gov.au/AUSSTATS/abs@.nsf/DetailsPage/1292.02006%20(Revision%202.0)?OpenDocument"^^xsd:anyURI ;
    rdfs:isDefinedBy cs: ;
    skos:broader icat:J5600 ;
    skos:definition "An individual business entity whose predominant economic activity is Radio Broadcasting."@en ;
    skos:inScheme cs: ;
    skos:notation "J5610" ;
    skos:prefLabel "Radio Broadcasting"@en ;
.

icat:J5620
    a skos:Concept ;
    dcterms:source "https://www.abs.gov.au/AUSSTATS/abs@.nsf/DetailsPage/1292.02006%20(Revision%202.0)?OpenDocument"^^xsd:anyURI ;
    rdfs:isDefinedBy cs: ;
    skos:broader icat:J5600 ;
    skos:definition "An individual business entity whose predominant economic activity is Television Broadcasting."@en ;
    skos:inScheme cs: ;
    skos:notation "J5620" ;
    skos:prefLabel "Television Broadcasting"@en ;
.

icat:J5700
    a skos:Concept ;
    dcterms:source "https://www.abs.gov.au/AUSSTATS/abs@.nsf/DetailsPage/1292.02006%20(Revision%202.0)?OpenDocument"^^xsd:anyURI ;
    rdfs:isDefinedBy cs: ;
    skos:broader icat:J0000 ;
    skos:definition "An individual business entity whose predominant economic activity is Internet Publishing and Broadcasting."@en ;
    skos:inScheme cs: ;
    skos:notation "J5700" ;
    skos:prefLabel "Internet Publishing and Broadcasting"@en ;
.

icat:J5800
    a skos:Concept ;
    dcterms:source "https://www.abs.gov.au/AUSSTATS/abs@.nsf/DetailsPage/1292.02006%20(Revision%202.0)?OpenDocument"^^xsd:anyURI ;
    rdfs:isDefinedBy cs: ;
    skos:broader icat:J0000 ;
    skos:definition "An individual business entity whose predominant economic activity is Telecommunications Services."@en ;
    skos:inScheme cs: ;
    skos:notation "J5800" ;
    skos:prefLabel "Telecommunications Services"@en ;
.

icat:J5910
    a skos:Concept ;
    dcterms:source "https://www.abs.gov.au/AUSSTATS/abs@.nsf/DetailsPage/1292.02006%20(Revision%202.0)?OpenDocument"^^xsd:anyURI ;
    rdfs:isDefinedBy cs: ;
    skos:broader icat:J5900 ;
    skos:definition "An individual business entity whose predominant economic activity is Internet Service Providers and Web Search Portals."@en ;
    skos:inScheme cs: ;
    skos:notation "J5910" ;
    skos:prefLabel "Internet Service Providers and Web Search Portals"@en ;
.

icat:J5920
    a skos:Concept ;
    dcterms:source "https://www.abs.gov.au/AUSSTATS/abs@.nsf/DetailsPage/1292.02006%20(Revision%202.0)?OpenDocument"^^xsd:anyURI ;
    rdfs:isDefinedBy cs: ;
    skos:broader icat:J5900 ;
    skos:definition "An individual business entity whose predominant economic activity is Data Processing, Web Hosting and Electronic Information Storage Services."@en ;
    skos:inScheme cs: ;
    skos:notation "J5920" ;
    skos:prefLabel "Data Processing, Web Hosting and Electronic Information Storage Services"@en ;
.

icat:J6010
    a skos:Concept ;
    dcterms:source "https://www.abs.gov.au/AUSSTATS/abs@.nsf/DetailsPage/1292.02006%20(Revision%202.0)?OpenDocument"^^xsd:anyURI ;
    rdfs:isDefinedBy cs: ;
    skos:broader icat:J6000 ;
    skos:definition "An individual business entity whose predominant economic activity is Libraries and Archives."@en ;
    skos:inScheme cs: ;
    skos:notation "J6010" ;
    skos:prefLabel "Libraries and Archives"@en ;
.

icat:J6020
    a skos:Concept ;
    dcterms:source "https://www.abs.gov.au/AUSSTATS/abs@.nsf/DetailsPage/1292.02006%20(Revision%202.0)?OpenDocument"^^xsd:anyURI ;
    rdfs:isDefinedBy cs: ;
    skos:broader icat:J6000 ;
    skos:definition "An individual business entity whose predominant economic activity is Other Information Services."@en ;
    skos:inScheme cs: ;
    skos:notation "J6020" ;
    skos:prefLabel "Other Information Services"@en ;
.

icat:K6210
    a skos:Concept ;
    dcterms:source "https://www.abs.gov.au/AUSSTATS/abs@.nsf/DetailsPage/1292.02006%20(Revision%202.0)?OpenDocument"^^xsd:anyURI ;
    rdfs:isDefinedBy cs: ;
    skos:broader icat:K6200 ;
    skos:definition "An individual business entity whose predominant economic activity is Central Banking."@en ;
    skos:inScheme cs: ;
    skos:notation "K6210" ;
    skos:prefLabel "Central Banking"@en ;
.

icat:K6220
    a skos:Concept ;
    dcterms:source "https://www.abs.gov.au/AUSSTATS/abs@.nsf/DetailsPage/1292.02006%20(Revision%202.0)?OpenDocument"^^xsd:anyURI ;
    rdfs:isDefinedBy cs: ;
    skos:broader icat:K6200 ;
    skos:definition "An individual business entity whose predominant economic activity is Depository Financial Intermediation."@en ;
    skos:inScheme cs: ;
    skos:notation "K6220" ;
    skos:prefLabel "Depository Financial Intermediation"@en ;
.

icat:K6230
    a skos:Concept ;
    dcterms:source "https://www.abs.gov.au/AUSSTATS/abs@.nsf/DetailsPage/1292.02006%20(Revision%202.0)?OpenDocument"^^xsd:anyURI ;
    rdfs:isDefinedBy cs: ;
    skos:broader icat:K6200 ;
    skos:definition "An individual business entity whose predominant economic activity is Non-Depository Financing."@en ;
    skos:inScheme cs: ;
    skos:notation "K6230" ;
    skos:prefLabel "Non-Depository Financing"@en ;
.

icat:K6240
    a skos:Concept ;
    dcterms:source "https://www.abs.gov.au/AUSSTATS/abs@.nsf/DetailsPage/1292.02006%20(Revision%202.0)?OpenDocument"^^xsd:anyURI ;
    rdfs:isDefinedBy cs: ;
    skos:broader icat:K6200 ;
    skos:definition "An individual business entity whose predominant economic activity is Financial Asset Investing."@en ;
    skos:inScheme cs: ;
    skos:notation "K6240" ;
    skos:prefLabel "Financial Asset Investing"@en ;
.

icat:K6310
    a skos:Concept ;
    dcterms:source "https://www.abs.gov.au/AUSSTATS/abs@.nsf/DetailsPage/1292.02006%20(Revision%202.0)?OpenDocument"^^xsd:anyURI ;
    rdfs:isDefinedBy cs: ;
    skos:broader icat:K6300 ;
    skos:definition "An individual business entity whose predominant economic activity is Life Insurance."@en ;
    skos:inScheme cs: ;
    skos:notation "K6310" ;
    skos:prefLabel "Life Insurance"@en ;
.

icat:K6320
    a skos:Concept ;
    dcterms:source "https://www.abs.gov.au/AUSSTATS/abs@.nsf/DetailsPage/1292.02006%20(Revision%202.0)?OpenDocument"^^xsd:anyURI ;
    rdfs:isDefinedBy cs: ;
    skos:broader icat:K6300 ;
    skos:definition "An individual business entity whose predominant economic activity is Health and General Insurance."@en ;
    skos:inScheme cs: ;
    skos:notation "K6320" ;
    skos:prefLabel "Health and General Insurance"@en ;
.

icat:K6330
    a skos:Concept ;
    dcterms:source "https://www.abs.gov.au/AUSSTATS/abs@.nsf/DetailsPage/1292.02006%20(Revision%202.0)?OpenDocument"^^xsd:anyURI ;
    rdfs:isDefinedBy cs: ;
    skos:broader icat:K6300 ;
    skos:definition "An individual business entity whose predominant economic activity is Superannuation Funds."@en ;
    skos:inScheme cs: ;
    skos:notation "K6330" ;
    skos:prefLabel "Superannuation Funds"@en ;
.

icat:K6410
    a skos:Concept ;
    dcterms:source "https://www.abs.gov.au/AUSSTATS/abs@.nsf/DetailsPage/1292.02006%20(Revision%202.0)?OpenDocument"^^xsd:anyURI ;
    rdfs:isDefinedBy cs: ;
    skos:broader icat:K6400 ;
    skos:definition "An individual business entity whose predominant economic activity is Auxiliary Finance and Investment Services."@en ;
    skos:inScheme cs: ;
    skos:notation "K6410" ;
    skos:prefLabel "Auxiliary Finance and Investment Services"@en ;
.

icat:K6420
    a skos:Concept ;
    dcterms:source "https://www.abs.gov.au/AUSSTATS/abs@.nsf/DetailsPage/1292.02006%20(Revision%202.0)?OpenDocument"^^xsd:anyURI ;
    rdfs:isDefinedBy cs: ;
    skos:broader icat:K6400 ;
    skos:definition "An individual business entity whose predominant economic activity is Auxiliary Insurance Services."@en ;
    skos:inScheme cs: ;
    skos:notation "K6420" ;
    skos:prefLabel "Auxiliary Insurance Services"@en ;
.

icat:L6610
    a skos:Concept ;
    dcterms:source "https://www.abs.gov.au/AUSSTATS/abs@.nsf/DetailsPage/1292.02006%20(Revision%202.0)?OpenDocument"^^xsd:anyURI ;
    rdfs:isDefinedBy cs: ;
    skos:broader icat:L6600 ;
    skos:definition "An individual business entity whose predominant economic activity is Motor Vehicle and Transport Equipment Rental and Hiring."@en ;
    skos:inScheme cs: ;
    skos:notation "L6610" ;
    skos:prefLabel "Motor Vehicle and Transport Equipment Rental and Hiring"@en ;
.

icat:L6620
    a skos:Concept ;
    dcterms:source "https://www.abs.gov.au/AUSSTATS/abs@.nsf/DetailsPage/1292.02006%20(Revision%202.0)?OpenDocument"^^xsd:anyURI ;
    rdfs:isDefinedBy cs: ;
    skos:broader icat:L6600 ;
    skos:definition "An individual business entity whose predominant economic activity is Farm Animal and Bloodstock Leasing."@en ;
    skos:inScheme cs: ;
    skos:notation "L6620" ;
    skos:prefLabel "Farm Animal and Bloodstock Leasing"@en ;
.

icat:L6630
    a skos:Concept ;
    dcterms:source "https://www.abs.gov.au/AUSSTATS/abs@.nsf/DetailsPage/1292.02006%20(Revision%202.0)?OpenDocument"^^xsd:anyURI ;
    rdfs:isDefinedBy cs: ;
    skos:broader icat:L6600 ;
    skos:definition "An individual business entity whose predominant economic activity is Other Goods and Equipment Rental and Hiring."@en ;
    skos:inScheme cs: ;
    skos:notation "L6630" ;
    skos:prefLabel "Other Goods and Equipment Rental and Hiring"@en ;
.

icat:L6640
    a skos:Concept ;
    dcterms:source "https://www.abs.gov.au/AUSSTATS/abs@.nsf/DetailsPage/1292.02006%20(Revision%202.0)?OpenDocument"^^xsd:anyURI ;
    rdfs:isDefinedBy cs: ;
    skos:broader icat:L6600 ;
    skos:definition "An individual business entity whose predominant economic activity is Non-Financial Intangible Assets (Except Copyrights) Leasing."@en ;
    skos:inScheme cs: ;
    skos:notation "L6640" ;
    skos:prefLabel "Non-Financial Intangible Assets (Except Copyrights) Leasing"@en ;
.

icat:L6710
    a skos:Concept ;
    dcterms:source "https://www.abs.gov.au/AUSSTATS/abs@.nsf/DetailsPage/1292.02006%20(Revision%202.0)?OpenDocument"^^xsd:anyURI ;
    rdfs:isDefinedBy cs: ;
    skos:broader icat:L6700 ;
    skos:definition "An individual business entity whose predominant economic activity is Property Operators."@en ;
    skos:inScheme cs: ;
    skos:notation "L6710" ;
    skos:prefLabel "Property Operators"@en ;
.

icat:L6720
    a skos:Concept ;
    dcterms:source "https://www.abs.gov.au/AUSSTATS/abs@.nsf/DetailsPage/1292.02006%20(Revision%202.0)?OpenDocument"^^xsd:anyURI ;
    rdfs:isDefinedBy cs: ;
    skos:broader icat:L6700 ;
    skos:definition "An individual business entity whose predominant economic activity is Real Estate Services."@en ;
    skos:inScheme cs: ;
    skos:notation "L6720" ;
    skos:prefLabel "Real Estate Services"@en ;
.

icat:M6910
    a skos:Concept ;
    dcterms:source "https://www.abs.gov.au/AUSSTATS/abs@.nsf/DetailsPage/1292.02006%20(Revision%202.0)?OpenDocument"^^xsd:anyURI ;
    rdfs:isDefinedBy cs: ;
    skos:broader icat:M6900 ;
    skos:definition "An individual business entity whose predominant economic activity is Scientific Research Services."@en ;
    skos:inScheme cs: ;
    skos:notation "M6910" ;
    skos:prefLabel "Scientific Research Services"@en ;
.

icat:M6920
    a skos:Concept ;
    dcterms:source "https://www.abs.gov.au/AUSSTATS/abs@.nsf/DetailsPage/1292.02006%20(Revision%202.0)?OpenDocument"^^xsd:anyURI ;
    rdfs:isDefinedBy cs: ;
    skos:broader icat:M6900 ;
    skos:definition "An individual business entity whose predominant economic activity is Architectural, Engineering and Technical Services."@en ;
    skos:inScheme cs: ;
    skos:notation "M6920" ;
    skos:prefLabel "Architectural, Engineering and Technical Services"@en ;
.

icat:M6930
    a skos:Concept ;
    dcterms:source "https://www.abs.gov.au/AUSSTATS/abs@.nsf/DetailsPage/1292.02006%20(Revision%202.0)?OpenDocument"^^xsd:anyURI ;
    rdfs:isDefinedBy cs: ;
    skos:broader icat:M6900 ;
    skos:definition "An individual business entity whose predominant economic activity is Legal and Accounting Services."@en ;
    skos:inScheme cs: ;
    skos:notation "M6930" ;
    skos:prefLabel "Legal and Accounting Services"@en ;
.

icat:M6940
    a skos:Concept ;
    dcterms:source "https://www.abs.gov.au/AUSSTATS/abs@.nsf/DetailsPage/1292.02006%20(Revision%202.0)?OpenDocument"^^xsd:anyURI ;
    rdfs:isDefinedBy cs: ;
    skos:broader icat:M6900 ;
    skos:definition "An individual business entity whose predominant economic activity is Advertising Services."@en ;
    skos:inScheme cs: ;
    skos:notation "M6940" ;
    skos:prefLabel "Advertising Services"@en ;
.

icat:M6950
    a skos:Concept ;
    dcterms:source "https://www.abs.gov.au/AUSSTATS/abs@.nsf/DetailsPage/1292.02006%20(Revision%202.0)?OpenDocument"^^xsd:anyURI ;
    rdfs:isDefinedBy cs: ;
    skos:broader icat:M6900 ;
    skos:definition "An individual business entity whose predominant economic activity is Market Research and Statistical Services."@en ;
    skos:inScheme cs: ;
    skos:notation "M6950" ;
    skos:prefLabel "Market Research and Statistical Services"@en ;
.

icat:M6960
    a skos:Concept ;
    dcterms:source "https://www.abs.gov.au/AUSSTATS/abs@.nsf/DetailsPage/1292.02006%20(Revision%202.0)?OpenDocument"^^xsd:anyURI ;
    rdfs:isDefinedBy cs: ;
    skos:broader icat:M6900 ;
    skos:definition "An individual business entity whose predominant economic activity is Management and Related Consulting Services."@en ;
    skos:inScheme cs: ;
    skos:notation "M6960" ;
    skos:prefLabel "Management and Related Consulting Services"@en ;
.

icat:M6970
    a skos:Concept ;
    dcterms:source "https://www.abs.gov.au/AUSSTATS/abs@.nsf/DetailsPage/1292.02006%20(Revision%202.0)?OpenDocument"^^xsd:anyURI ;
    rdfs:isDefinedBy cs: ;
    skos:broader icat:M6900 ;
    skos:definition "An individual business entity whose predominant economic activity is Veterinary Services."@en ;
    skos:inScheme cs: ;
    skos:notation "M6970" ;
    skos:prefLabel "Veterinary Services"@en ;
.

icat:M6990
    a skos:Concept ;
    dcterms:source "https://www.abs.gov.au/AUSSTATS/abs@.nsf/DetailsPage/1292.02006%20(Revision%202.0)?OpenDocument"^^xsd:anyURI ;
    rdfs:isDefinedBy cs: ;
    skos:broader icat:M6900 ;
    skos:definition "An individual business entity whose predominant economic activity is Other Professional, Scientific and Technical Services."@en ;
    skos:inScheme cs: ;
    skos:notation "M6990" ;
    skos:prefLabel "Other Professional, Scientific and Technical Services"@en ;
.

icat:M7000
    a skos:Concept ;
    dcterms:source "https://www.abs.gov.au/AUSSTATS/abs@.nsf/DetailsPage/1292.02006%20(Revision%202.0)?OpenDocument"^^xsd:anyURI ;
    rdfs:isDefinedBy cs: ;
    skos:broader icat:M0000 ;
    skos:definition "An individual business entity whose predominant economic activity is Computer System Design and Related Services."@en ;
    skos:inScheme cs: ;
    skos:notation "M7000" ;
    skos:prefLabel "Computer System Design and Related Services"@en ;
.

icat:N7210
    a skos:Concept ;
    dcterms:source "https://www.abs.gov.au/AUSSTATS/abs@.nsf/DetailsPage/1292.02006%20(Revision%202.0)?OpenDocument"^^xsd:anyURI ;
    rdfs:isDefinedBy cs: ;
    skos:broader icat:N7200 ;
    skos:definition "An individual business entity whose predominant economic activity is Employment Services."@en ;
    skos:inScheme cs: ;
    skos:notation "N7210" ;
    skos:prefLabel "Employment Services"@en ;
.

icat:N7220
    a skos:Concept ;
    dcterms:source "https://www.abs.gov.au/AUSSTATS/abs@.nsf/DetailsPage/1292.02006%20(Revision%202.0)?OpenDocument"^^xsd:anyURI ;
    rdfs:isDefinedBy cs: ;
    skos:broader icat:N7200 ;
    skos:definition "An individual business entity whose predominant economic activity is Travel Agency and Tour Arrangement Services."@en ;
    skos:inScheme cs: ;
    skos:notation "N7220" ;
    skos:prefLabel "Travel Agency and Tour Arrangement Services"@en ;
.

icat:N7290
    a skos:Concept ;
    dcterms:source "https://www.abs.gov.au/AUSSTATS/abs@.nsf/DetailsPage/1292.02006%20(Revision%202.0)?OpenDocument"^^xsd:anyURI ;
    rdfs:isDefinedBy cs: ;
    skos:broader icat:N7200 ;
    skos:definition "An individual business entity whose predominant economic activity is Other Administrative Services."@en ;
    skos:inScheme cs: ;
    skos:notation "N7290" ;
    skos:prefLabel "Other Administrative Services"@en ;
.

icat:N7310
    a skos:Concept ;
    dcterms:source "https://www.abs.gov.au/AUSSTATS/abs@.nsf/DetailsPage/1292.02006%20(Revision%202.0)?OpenDocument"^^xsd:anyURI ;
    rdfs:isDefinedBy cs: ;
    skos:broader icat:N7300 ;
    skos:definition "An individual business entity whose predominant economic activity is Building Cleaning, Pest Control and Gardening Services."@en ;
    skos:inScheme cs: ;
    skos:notation "N7310" ;
    skos:prefLabel "Building Cleaning, Pest Control and Gardening Services"@en ;
.

icat:N7320
    a skos:Concept ;
    dcterms:source "https://www.abs.gov.au/AUSSTATS/abs@.nsf/DetailsPage/1292.02006%20(Revision%202.0)?OpenDocument"^^xsd:anyURI ;
    rdfs:isDefinedBy cs: ;
    skos:broader icat:N7300 ;
    skos:definition "An individual business entity whose predominant economic activity is Packaging Services."@en ;
    skos:inScheme cs: ;
    skos:notation "N7320" ;
    skos:prefLabel "Packaging Services"@en ;
.

icat:O7510
    a skos:Concept ;
    dcterms:source "https://www.abs.gov.au/AUSSTATS/abs@.nsf/DetailsPage/1292.02006%20(Revision%202.0)?OpenDocument"^^xsd:anyURI ;
    rdfs:isDefinedBy cs: ;
    skos:broader icat:O7500 ;
    skos:definition "An individual business entity whose predominant economic activity is Central Government Administration."@en ;
    skos:inScheme cs: ;
    skos:notation "O7510" ;
    skos:prefLabel "Central Government Administration"@en ;
.

icat:O7520
    a skos:Concept ;
    dcterms:source "https://www.abs.gov.au/AUSSTATS/abs@.nsf/DetailsPage/1292.02006%20(Revision%202.0)?OpenDocument"^^xsd:anyURI ;
    rdfs:isDefinedBy cs: ;
    skos:broader icat:O7500 ;
    skos:definition "An individual business entity whose predominant economic activity is State Government Administration."@en ;
    skos:inScheme cs: ;
    skos:notation "O7520" ;
    skos:prefLabel "State Government Administration"@en ;
.

icat:O7530
    a skos:Concept ;
    dcterms:source "https://www.abs.gov.au/AUSSTATS/abs@.nsf/DetailsPage/1292.02006%20(Revision%202.0)?OpenDocument"^^xsd:anyURI ;
    rdfs:isDefinedBy cs: ;
    skos:broader icat:O7500 ;
    skos:definition "An individual business entity whose predominant economic activity is Local Government Administration."@en ;
    skos:inScheme cs: ;
    skos:notation "O7530" ;
    skos:prefLabel "Local Government Administration"@en ;
.

icat:O7540
    a skos:Concept ;
    dcterms:source "https://www.abs.gov.au/AUSSTATS/abs@.nsf/DetailsPage/1292.02006%20(Revision%202.0)?OpenDocument"^^xsd:anyURI ;
    rdfs:isDefinedBy cs: ;
    skos:broader icat:O7500 ;
    skos:definition "An individual business entity whose predominant economic activity is Justice."@en ;
    skos:inScheme cs: ;
    skos:notation "O7540" ;
    skos:prefLabel "Justice"@en ;
.

icat:O7550
    a skos:Concept ;
    dcterms:source "https://www.abs.gov.au/AUSSTATS/abs@.nsf/DetailsPage/1292.02006%20(Revision%202.0)?OpenDocument"^^xsd:anyURI ;
    rdfs:isDefinedBy cs: ;
    skos:broader icat:O7500 ;
    skos:definition "An individual business entity whose predominant economic activity is Government Representation."@en ;
    skos:inScheme cs: ;
    skos:notation "O7550" ;
    skos:prefLabel "Government Representation"@en ;
.

icat:O7600
    a skos:Concept ;
    dcterms:source "https://www.abs.gov.au/AUSSTATS/abs@.nsf/DetailsPage/1292.02006%20(Revision%202.0)?OpenDocument"^^xsd:anyURI ;
    rdfs:isDefinedBy cs: ;
    skos:broader icat:O0000 ;
    skos:definition "An individual business entity whose predominant economic activity is Defence."@en ;
    skos:inScheme cs: ;
    skos:notation "O7600" ;
    skos:prefLabel "Defence"@en ;
.

icat:O7710
    a skos:Concept ;
    dcterms:source "https://www.abs.gov.au/AUSSTATS/abs@.nsf/DetailsPage/1292.02006%20(Revision%202.0)?OpenDocument"^^xsd:anyURI ;
    rdfs:isDefinedBy cs: ;
    skos:broader icat:O7700 ;
    skos:definition "An individual business entity whose predominant economic activity is Public Order and Safety Services."@en ;
    skos:inScheme cs: ;
    skos:notation "O7710" ;
    skos:prefLabel "Public Order and Safety Services"@en ;
.

icat:O7720
    a skos:Concept ;
    dcterms:source "https://www.abs.gov.au/AUSSTATS/abs@.nsf/DetailsPage/1292.02006%20(Revision%202.0)?OpenDocument"^^xsd:anyURI ;
    rdfs:isDefinedBy cs: ;
    skos:broader icat:O7700 ;
    skos:definition "An individual business entity whose predominant economic activity is Regulatory Services."@en ;
    skos:inScheme cs: ;
    skos:notation "O7720" ;
    skos:prefLabel "Regulatory Services"@en ;
.

icat:P8010
    a skos:Concept ;
    dcterms:source "https://www.abs.gov.au/AUSSTATS/abs@.nsf/DetailsPage/1292.02006%20(Revision%202.0)?OpenDocument"^^xsd:anyURI ;
    rdfs:isDefinedBy cs: ;
    skos:broader icat:P8000 ;
    skos:definition "An individual business entity whose predominant economic activity is Preschool Education."@en ;
    skos:inScheme cs: ;
    skos:notation "P8010" ;
    skos:prefLabel "Preschool Education"@en ;
.

icat:P8020
    a skos:Concept ;
    dcterms:source "https://www.abs.gov.au/AUSSTATS/abs@.nsf/DetailsPage/1292.02006%20(Revision%202.0)?OpenDocument"^^xsd:anyURI ;
    rdfs:isDefinedBy cs: ;
    skos:broader icat:P8000 ;
    skos:definition "An individual business entity whose predominant economic activity is School Education."@en ;
    skos:inScheme cs: ;
    skos:notation "P8020" ;
    skos:prefLabel "School Education"@en ;
.

icat:P8100
    a skos:Concept ;
    dcterms:source "https://www.abs.gov.au/AUSSTATS/abs@.nsf/DetailsPage/1292.02006%20(Revision%202.0)?OpenDocument"^^xsd:anyURI ;
    rdfs:isDefinedBy cs: ;
    skos:broader icat:P0000 ;
    skos:definition "An individual business entity whose predominant economic activity is Tertiary Education."@en ;
    skos:inScheme cs: ;
    skos:notation "P8100" ;
    skos:prefLabel "Tertiary Education"@en ;
.

icat:P8220
    a skos:Concept ;
    dcterms:source "https://www.abs.gov.au/AUSSTATS/abs@.nsf/DetailsPage/1292.02006%20(Revision%202.0)?OpenDocument"^^xsd:anyURI ;
    rdfs:isDefinedBy cs: ;
    skos:broader icat:P8200 ;
    skos:definition "An individual business entity whose predominant economic activity is Educational Support Services."@en ;
    skos:inScheme cs: ;
    skos:notation "P8220" ;
    skos:prefLabel "Educational Support Services"@en ;
.

icat:Q8400
    a skos:Concept ;
    dcterms:source "https://www.abs.gov.au/AUSSTATS/abs@.nsf/DetailsPage/1292.02006%20(Revision%202.0)?OpenDocument"^^xsd:anyURI ;
    rdfs:isDefinedBy cs: ;
    skos:broader icat:Q0000 ;
    skos:definition "An individual business entity whose predominant economic activity is Hospitals."@en ;
    skos:inScheme cs: ;
    skos:notation "Q8400" ;
    skos:prefLabel "Hospitals"@en ;
.

icat:Q8510
    a skos:Concept ;
    dcterms:source "https://www.abs.gov.au/AUSSTATS/abs@.nsf/DetailsPage/1292.02006%20(Revision%202.0)?OpenDocument"^^xsd:anyURI ;
    rdfs:isDefinedBy cs: ;
    skos:broader icat:Q8500 ;
    skos:definition "An individual business entity whose predominant economic activity is Medical Services."@en ;
    skos:inScheme cs: ;
    skos:notation "Q8510" ;
    skos:prefLabel "Medical Services"@en ;
.

icat:Q8520
    a skos:Concept ;
    dcterms:source "https://www.abs.gov.au/AUSSTATS/abs@.nsf/DetailsPage/1292.02006%20(Revision%202.0)?OpenDocument"^^xsd:anyURI ;
    rdfs:isDefinedBy cs: ;
    skos:broader icat:Q8500 ;
    skos:definition "An individual business entity whose predominant economic activity is Pathology and Diagnostic Imaging Services."@en ;
    skos:inScheme cs: ;
    skos:notation "Q8520" ;
    skos:prefLabel "Pathology and Diagnostic Imaging Services"@en ;
.

icat:Q8530
    a skos:Concept ;
    dcterms:source "https://www.abs.gov.au/AUSSTATS/abs@.nsf/DetailsPage/1292.02006%20(Revision%202.0)?OpenDocument"^^xsd:anyURI ;
    rdfs:isDefinedBy cs: ;
    skos:broader icat:Q8500 ;
    skos:definition "An individual business entity whose predominant economic activity is Allied Health Services."@en ;
    skos:inScheme cs: ;
    skos:notation "Q8530" ;
    skos:prefLabel "Allied Health Services"@en ;
.

icat:Q8590
    a skos:Concept ;
    dcterms:source "https://www.abs.gov.au/AUSSTATS/abs@.nsf/DetailsPage/1292.02006%20(Revision%202.0)?OpenDocument"^^xsd:anyURI ;
    rdfs:isDefinedBy cs: ;
    skos:broader icat:Q8500 ;
    skos:definition "An individual business entity whose predominant economic activity is Other Health Care Services."@en ;
    skos:inScheme cs: ;
    skos:notation "Q8590" ;
    skos:prefLabel "Other Health Care Services"@en ;
.

icat:Q8600
    a skos:Concept ;
    dcterms:source "https://www.abs.gov.au/AUSSTATS/abs@.nsf/DetailsPage/1292.02006%20(Revision%202.0)?OpenDocument"^^xsd:anyURI ;
    rdfs:isDefinedBy cs: ;
    skos:broader icat:Q0000 ;
    skos:definition "An individual business entity whose predominant economic activity is Residential Care Services."@en ;
    skos:inScheme cs: ;
    skos:notation "Q8600" ;
    skos:prefLabel "Residential Care Services"@en ;
.

icat:Q8710
    a skos:Concept ;
    dcterms:source "https://www.abs.gov.au/AUSSTATS/abs@.nsf/DetailsPage/1292.02006%20(Revision%202.0)?OpenDocument"^^xsd:anyURI ;
    rdfs:isDefinedBy cs: ;
    skos:broader icat:Q8700 ;
    skos:definition "An individual business entity whose predominant economic activity is Child Care Services."@en ;
    skos:inScheme cs: ;
    skos:notation "Q8710" ;
    skos:prefLabel "Child Care Services"@en ;
.

icat:Q8790
    a skos:Concept ;
    dcterms:source "https://www.abs.gov.au/AUSSTATS/abs@.nsf/DetailsPage/1292.02006%20(Revision%202.0)?OpenDocument"^^xsd:anyURI ;
    rdfs:isDefinedBy cs: ;
    skos:broader icat:Q8700 ;
    skos:definition "An individual business entity whose predominant economic activity is Other Social Assistance Services."@en ;
    skos:inScheme cs: ;
    skos:notation "Q8790" ;
    skos:prefLabel "Other Social Assistance Services"@en ;
.

icat:R8910
    a skos:Concept ;
    dcterms:source "https://www.abs.gov.au/AUSSTATS/abs@.nsf/DetailsPage/1292.02006%20(Revision%202.0)?OpenDocument"^^xsd:anyURI ;
    rdfs:isDefinedBy cs: ;
    skos:broader icat:R8900 ;
    skos:definition "An individual business entity whose predominant economic activity is Museum Operation."@en ;
    skos:inScheme cs: ;
    skos:notation "R8910" ;
    skos:prefLabel "Museum Operation"@en ;
.

icat:R8920
    a skos:Concept ;
    dcterms:source "https://www.abs.gov.au/AUSSTATS/abs@.nsf/DetailsPage/1292.02006%20(Revision%202.0)?OpenDocument"^^xsd:anyURI ;
    rdfs:isDefinedBy cs: ;
    skos:broader icat:R8900 ;
    skos:definition "An individual business entity whose predominant economic activity is Parks and Gardens Operations."@en ;
    skos:inScheme cs: ;
    skos:notation "R8920" ;
    skos:prefLabel "Parks and Gardens Operations"@en ;
.

icat:R9000
    a skos:Concept ;
    dcterms:source "https://www.abs.gov.au/AUSSTATS/abs@.nsf/DetailsPage/1292.02006%20(Revision%202.0)?OpenDocument"^^xsd:anyURI ;
    rdfs:isDefinedBy cs: ;
    skos:broader icat:R0000 ;
    skos:definition "An individual business entity whose predominant economic activity is Creative and Performing Arts Activities."@en ;
    skos:inScheme cs: ;
    skos:notation "R9000" ;
    skos:prefLabel "Creative and Performing Arts Activities"@en ;
.

icat:R9110
    a skos:Concept ;
    dcterms:source "https://www.abs.gov.au/AUSSTATS/abs@.nsf/DetailsPage/1292.02006%20(Revision%202.0)?OpenDocument"^^xsd:anyURI ;
    rdfs:isDefinedBy cs: ;
    skos:broader icat:R9100 ;
    skos:definition "An individual business entity whose predominant economic activity is Sports and Physical Recreation Activities."@en ;
    skos:inScheme cs: ;
    skos:notation "R9110" ;
    skos:prefLabel "Sports and Physical Recreation Activities"@en ;
.

icat:R9120
    a skos:Concept ;
    dcterms:source "https://www.abs.gov.au/AUSSTATS/abs@.nsf/DetailsPage/1292.02006%20(Revision%202.0)?OpenDocument"^^xsd:anyURI ;
    rdfs:isDefinedBy cs: ;
    skos:broader icat:R9100 ;
    skos:definition "An individual business entity whose predominant economic activity is Horse and Dog Racing Activities."@en ;
    skos:inScheme cs: ;
    skos:notation "R9120" ;
    skos:prefLabel "Horse and Dog Racing Activities"@en ;
.

icat:R9130
    a skos:Concept ;
    dcterms:source "https://www.abs.gov.au/AUSSTATS/abs@.nsf/DetailsPage/1292.02006%20(Revision%202.0)?OpenDocument"^^xsd:anyURI ;
    rdfs:isDefinedBy cs: ;
    skos:broader icat:R9100 ;
    skos:definition "An individual business entity whose predominant economic activity is Amusement and Other Recreation Activities."@en ;
    skos:inScheme cs: ;
    skos:notation "R9130" ;
    skos:prefLabel "Amusement and Other Recreation Activities"@en ;
.

icat:R9200
    a skos:Concept ;
    dcterms:source "https://www.abs.gov.au/AUSSTATS/abs@.nsf/DetailsPage/1292.02006%20(Revision%202.0)?OpenDocument"^^xsd:anyURI ;
    rdfs:isDefinedBy cs: ;
    skos:broader icat:R0000 ;
    skos:definition "An individual business entity whose predominant economic activity is Gambling Activities."@en ;
    skos:inScheme cs: ;
    skos:notation "R9200" ;
    skos:prefLabel "Gambling Activities"@en ;
.

icat:S9410
    a skos:Concept ;
    dcterms:source "https://www.abs.gov.au/AUSSTATS/abs@.nsf/DetailsPage/1292.02006%20(Revision%202.0)?OpenDocument"^^xsd:anyURI ;
    rdfs:isDefinedBy cs: ;
    skos:broader icat:S9400 ;
    skos:definition "An individual business entity whose predominant economic activity is Automotive Repair and Maintenance."@en ;
    skos:inScheme cs: ;
    skos:notation "S9410" ;
    skos:prefLabel "Automotive Repair and Maintenance"@en ;
.

icat:S9420
    a skos:Concept ;
    dcterms:source "https://www.abs.gov.au/AUSSTATS/abs@.nsf/DetailsPage/1292.02006%20(Revision%202.0)?OpenDocument"^^xsd:anyURI ;
    rdfs:isDefinedBy cs: ;
    skos:broader icat:S9400 ;
    skos:definition "An individual business entity whose predominant economic activity is Machinery and Equipment Repair and Maintenance."@en ;
    skos:inScheme cs: ;
    skos:notation "S9420" ;
    skos:prefLabel "Machinery and Equipment Repair and Maintenance"@en ;
.

icat:S9490
    a skos:Concept ;
    dcterms:source "https://www.abs.gov.au/AUSSTATS/abs@.nsf/DetailsPage/1292.02006%20(Revision%202.0)?OpenDocument"^^xsd:anyURI ;
    rdfs:isDefinedBy cs: ;
    skos:broader icat:S9400 ;
    skos:definition "An individual business entity whose predominant economic activity is Other Repair and Maintenance."@en ;
    skos:inScheme cs: ;
    skos:notation "S9490" ;
    skos:prefLabel "Other Repair and Maintenance"@en ;
.

icat:S9510
    a skos:Concept ;
    dcterms:source "https://www.abs.gov.au/AUSSTATS/abs@.nsf/DetailsPage/1292.02006%20(Revision%202.0)?OpenDocument"^^xsd:anyURI ;
    rdfs:isDefinedBy cs: ;
    skos:broader icat:S9500 ;
    skos:definition "An individual business entity whose predominant economic activity is Personal Care Services."@en ;
    skos:inScheme cs: ;
    skos:notation "S9510" ;
    skos:prefLabel "Personal Care Services"@en ;
.

icat:S9520
    a skos:Concept ;
    dcterms:source "https://www.abs.gov.au/AUSSTATS/abs@.nsf/DetailsPage/1292.02006%20(Revision%202.0)?OpenDocument"^^xsd:anyURI ;
    rdfs:isDefinedBy cs: ;
    skos:broader icat:S9500 ;
    skos:definition "An individual business entity whose predominant economic activity is Funeral, Crematorium and Cemetery Services."@en ;
    skos:inScheme cs: ;
    skos:notation "S9520" ;
    skos:prefLabel "Funeral, Crematorium and Cemetery Services"@en ;
.

icat:S9530
    a skos:Concept ;
    dcterms:source "https://www.abs.gov.au/AUSSTATS/abs@.nsf/DetailsPage/1292.02006%20(Revision%202.0)?OpenDocument"^^xsd:anyURI ;
    rdfs:isDefinedBy cs: ;
    skos:broader icat:S9500 ;
    skos:definition "An individual business entity whose predominant economic activity is Other Personal Services."@en ;
    skos:inScheme cs: ;
    skos:notation "S9530" ;
    skos:prefLabel "Other Personal Services"@en ;
.

icat:S9540
    a skos:Concept ;
    dcterms:source "https://www.abs.gov.au/AUSSTATS/abs@.nsf/DetailsPage/1292.02006%20(Revision%202.0)?OpenDocument"^^xsd:anyURI ;
    rdfs:isDefinedBy cs: ;
    skos:broader icat:S9500 ;
    skos:definition "An individual business entity whose predominant economic activity is Religious Services."@en ;
    skos:inScheme cs: ;
    skos:notation "S9540" ;
    skos:prefLabel "Religious Services"@en ;
.

icat:S9550
    a skos:Concept ;
    dcterms:source "https://www.abs.gov.au/AUSSTATS/abs@.nsf/DetailsPage/1292.02006%20(Revision%202.0)?OpenDocument"^^xsd:anyURI ;
    rdfs:isDefinedBy cs: ;
    skos:broader icat:S9500 ;
    skos:definition "An individual business entity whose predominant economic activity is Civic, Professional and Other Interest Group Services."@en ;
    skos:inScheme cs: ;
    skos:notation "S9550" ;
    skos:prefLabel "Civic, Professional and Other Interest Group Services"@en ;
.

icat:S9600
    a skos:Concept ;
    dcterms:source "https://www.abs.gov.au/AUSSTATS/abs@.nsf/DetailsPage/1292.02006%20(Revision%202.0)?OpenDocument"^^xsd:anyURI ;
    rdfs:isDefinedBy cs: ;
    skos:broader icat:S0000 ;
    skos:definition "An individual business entity whose predominant economic activity is Private Households Employing Staff and Undifferentiated Goods and Service Producing Activities of Households for Own Use."@en ;
    skos:inScheme cs: ;
    skos:notation "S9600" ;
    skos:prefLabel "Private Households Employing Staff and Undifferentiated Goods and Service Producing Activities of Households for Own Use"@en ;
.

icat:coal-buyer
    a skos:Collection ;
    skos:definition "Industry categorisations as applicable to coal sales."@en ;
    skos:member
        icat:B0600 ,
        icat:C0000 ,
        icat:C2100 ,
        icat:D2610 ,
        icat:X9800 ,
        icat:X9900 ;
    skos:prefLabel "Coal Buyer Industry"@en ;
    prov:wasDerivedFrom cs: ;
.

icat:B0600
    a skos:Concept ;
    dcterms:source "https://www.abs.gov.au/AUSSTATS/abs@.nsf/DetailsPage/1292.02006%20(Revision%202.0)?OpenDocument"^^xsd:anyURI ;
    rdfs:isDefinedBy cs: ;
    skos:altLabel "Coal Mine"@en ;
    skos:broader icat:B0000 ;
    skos:definition "An individual business entity whose predominant economic activity is Coal Mining."@en ;
    skos:inScheme cs: ;
    skos:notation "B0600" ;
    skos:prefLabel "Coal Mining"@en ;
.

icat:D2610
    a skos:Concept ;
    dcterms:source "https://www.abs.gov.au/AUSSTATS/abs@.nsf/DetailsPage/1292.02006%20(Revision%202.0)?OpenDocument"^^xsd:anyURI ;
    rdfs:isDefinedBy cs: ;
    skos:broader icat:D2600 ;
    skos:definition "An individual business entity whose predominant economic activity is Electricity Generation."@en ;
    skos:inScheme cs: ;
    skos:notation "D2610" ;
    skos:prefLabel "Electricity Generation"@en ;
.

icat:P8200
    a skos:Concept ;
    dcterms:source "https://www.abs.gov.au/AUSSTATS/abs@.nsf/DetailsPage/1292.02006%20(Revision%202.0)?OpenDocument"^^xsd:anyURI ;
    rdfs:isDefinedBy cs: ;
    skos:broader icat:P0000 ;
    skos:definition "An individual business entity whose predominant economic activity is Adult, Community and Other Education."@en ;
    skos:inScheme cs: ;
    skos:notation "P8200" ;
    skos:prefLabel "Adult, Community and Other Education"@en ;
.

icat:X9800
    a skos:Concept ;
    dcterms:source "https://www.abs.gov.au/AUSSTATS/abs@.nsf/DetailsPage/1292.02006%20(Revision%202.0)?OpenDocument"^^xsd:anyURI ;
    rdfs:isDefinedBy cs: ;
    skos:altLabel
        "Other"@en ,
        "Other Industry"@en ;
    skos:broader icat:X0000 ;
    skos:definition "An individual business entity whose predominant economic activity is unspecified or is not available for selection with provided list. This typically applies to a known industrial classification that is not relevant to a high degree of specificity in a specific use case."@en ;
    skos:inScheme cs: ;
    skos:notation "X9800" ;
    skos:prefLabel "Unspecified Industry"@en ;
.

icat:X9900
    a skos:Concept ;
    dcterms:source "https://www.abs.gov.au/AUSSTATS/abs@.nsf/DetailsPage/1292.02006%20(Revision%202.0)?OpenDocument"^^xsd:anyURI ;
    rdfs:isDefinedBy cs: ;
    skos:altLabel "Unknown Industry"@en ;
    skos:broader icat:X0000 ;
    skos:definition "An individual business entity whose predominant economic activity is unknown."@en ;
    skos:inScheme cs: ;
    skos:notation "X9900" ;
    skos:prefLabel "Unknown"@en ;
.

icat:A0400
    a skos:Concept ;
    dcterms:source "https://www.abs.gov.au/AUSSTATS/abs@.nsf/DetailsPage/1292.02006%20(Revision%202.0)?OpenDocument"^^xsd:anyURI ;
    rdfs:isDefinedBy cs: ;
    skos:broader icat:A0000 ;
    skos:definition "An individual business entity whose predominant economic activity is Fishing, Hunting and Trapping."@en ;
    skos:inScheme cs: ;
    skos:notation "A0400" ;
    skos:prefLabel "Fishing, Hunting and Trapping"@en ;
.

icat:A0500
    a skos:Concept ;
    dcterms:source "https://www.abs.gov.au/AUSSTATS/abs@.nsf/DetailsPage/1292.02006%20(Revision%202.0)?OpenDocument"^^xsd:anyURI ;
    rdfs:isDefinedBy cs: ;
    skos:broader icat:A0000 ;
    skos:definition "An individual business entity whose predominant economic activity is Agriculture, Forestry and Fishing Support Services."@en ;
    skos:inScheme cs: ;
    skos:notation "A0500" ;
    skos:prefLabel "Agriculture, Forestry and Fishing Support Services"@en ;
.

icat:B0900
    a skos:Concept ;
    dcterms:source "https://www.abs.gov.au/AUSSTATS/abs@.nsf/DetailsPage/1292.02006%20(Revision%202.0)?OpenDocument"^^xsd:anyURI ;
    rdfs:isDefinedBy cs: ;
    skos:broader icat:B0000 ;
    skos:definition "An individual business entity whose predominant economic activity is Non-Metallic Mineral Mining and Quarrying."@en ;
    skos:inScheme cs: ;
    skos:notation "B0900" ;
    skos:prefLabel "Non-Metallic Mineral Mining and Quarrying"@en ;
.

icat:B1000
    a skos:Concept ;
    dcterms:source "https://www.abs.gov.au/AUSSTATS/abs@.nsf/DetailsPage/1292.02006%20(Revision%202.0)?OpenDocument"^^xsd:anyURI ;
    rdfs:isDefinedBy cs: ;
    skos:broader icat:B0000 ;
    skos:definition "An individual business entity whose predominant economic activity is Exploration and Other Mining Support Services."@en ;
    skos:inScheme cs: ;
    skos:notation "B1000" ;
    skos:prefLabel "Exploration and Other Mining Support Services"@en ;
.

icat:C1200
    a skos:Concept ;
    dcterms:source "https://www.abs.gov.au/AUSSTATS/abs@.nsf/DetailsPage/1292.02006%20(Revision%202.0)?OpenDocument"^^xsd:anyURI ;
    rdfs:isDefinedBy cs: ;
    skos:broader icat:C0000 ;
    skos:definition "An individual business entity whose predominant economic activity is Beverage and Tobacco Product Manufacturing."@en ;
    skos:inScheme cs: ;
    skos:notation "C1200" ;
    skos:prefLabel "Beverage and Tobacco Product Manufacturing"@en ;
.

icat:C1400
    a skos:Concept ;
    dcterms:source "https://www.abs.gov.au/AUSSTATS/abs@.nsf/DetailsPage/1292.02006%20(Revision%202.0)?OpenDocument"^^xsd:anyURI ;
    rdfs:isDefinedBy cs: ;
    skos:broader icat:C0000 ;
    skos:definition "An individual business entity whose predominant economic activity is Wood Product Manufacturing."@en ;
    skos:inScheme cs: ;
    skos:notation "C1400" ;
    skos:prefLabel "Wood Product Manufacturing"@en ;
.

icat:C1500
    a skos:Concept ;
    dcterms:source "https://www.abs.gov.au/AUSSTATS/abs@.nsf/DetailsPage/1292.02006%20(Revision%202.0)?OpenDocument"^^xsd:anyURI ;
    rdfs:isDefinedBy cs: ;
    skos:broader icat:C0000 ;
    skos:definition "An individual business entity whose predominant economic activity is Pulp, Paper and Converted Paper Product Manufacturing."@en ;
    skos:inScheme cs: ;
    skos:notation "C1500" ;
    skos:prefLabel "Pulp, Paper and Converted Paper Product Manufacturing"@en ;
.

icat:C1600
    a skos:Concept ;
    dcterms:source "https://www.abs.gov.au/AUSSTATS/abs@.nsf/DetailsPage/1292.02006%20(Revision%202.0)?OpenDocument"^^xsd:anyURI ;
    rdfs:isDefinedBy cs: ;
    skos:broader icat:C0000 ;
    skos:definition "An individual business entity whose predominant economic activity is Printing (including the Reproduction of Recorded Media)."@en ;
    skos:inScheme cs: ;
    skos:notation "C1600" ;
    skos:prefLabel "Printing (including the Reproduction of Recorded Media)"@en ;
.

icat:C1900
    a skos:Concept ;
    dcterms:source "https://www.abs.gov.au/AUSSTATS/abs@.nsf/DetailsPage/1292.02006%20(Revision%202.0)?OpenDocument"^^xsd:anyURI ;
    rdfs:isDefinedBy cs: ;
    skos:broader icat:C0000 ;
    skos:definition "An individual business entity whose predominant economic activity is Polymer Product and Rubber Product Manufacturing."@en ;
    skos:inScheme cs: ;
    skos:notation "C1900" ;
    skos:prefLabel "Polymer Product and Rubber Product Manufacturing"@en ;
.

icat:C2300
    a skos:Concept ;
    dcterms:source "https://www.abs.gov.au/AUSSTATS/abs@.nsf/DetailsPage/1292.02006%20(Revision%202.0)?OpenDocument"^^xsd:anyURI ;
    rdfs:isDefinedBy cs: ;
    skos:broader icat:C0000 ;
    skos:definition "An individual business entity whose predominant economic activity is Transport Equipment Manufacturing."@en ;
    skos:inScheme cs: ;
    skos:notation "C2300" ;
    skos:prefLabel "Transport Equipment Manufacturing"@en ;
.

icat:C2500
    a skos:Concept ;
    dcterms:source "https://www.abs.gov.au/AUSSTATS/abs@.nsf/DetailsPage/1292.02006%20(Revision%202.0)?OpenDocument"^^xsd:anyURI ;
    rdfs:isDefinedBy cs: ;
    skos:broader icat:C0000 ;
    skos:definition "An individual business entity whose predominant economic activity is Furniture and Other Manufacturing."@en ;
    skos:inScheme cs: ;
    skos:notation "C2500" ;
    skos:prefLabel "Furniture and Other Manufacturing"@en ;
.

icat:D2900
    a skos:Concept ;
    dcterms:source "https://www.abs.gov.au/AUSSTATS/abs@.nsf/DetailsPage/1292.02006%20(Revision%202.0)?OpenDocument"^^xsd:anyURI ;
    rdfs:isDefinedBy cs: ;
    skos:broader icat:D0000 ;
    skos:definition "An individual business entity whose predominant economic activity is Waste Collection, Treatment and Disposal Services."@en ;
    skos:inScheme cs: ;
    skos:notation "D2900" ;
    skos:prefLabel "Waste Collection, Treatment and Disposal Services"@en ;
.

icat:E3000
    a skos:Concept ;
    dcterms:source "https://www.abs.gov.au/AUSSTATS/abs@.nsf/DetailsPage/1292.02006%20(Revision%202.0)?OpenDocument"^^xsd:anyURI ;
    rdfs:isDefinedBy cs: ;
    skos:broader icat:E0000 ;
    skos:definition "An individual business entity whose predominant economic activity is Building Construction."@en ;
    skos:inScheme cs: ;
    skos:notation "E3000" ;
    skos:prefLabel "Building Construction"@en ;
.

icat:F3400
    a skos:Concept ;
    dcterms:source "https://www.abs.gov.au/AUSSTATS/abs@.nsf/DetailsPage/1292.02006%20(Revision%202.0)?OpenDocument"^^xsd:anyURI ;
    rdfs:isDefinedBy cs: ;
    skos:broader icat:F0000 ;
    skos:definition "An individual business entity whose predominant economic activity is Machinery and Equipment Wholesaling."@en ;
    skos:inScheme cs: ;
    skos:notation "F3400" ;
    skos:prefLabel "Machinery and Equipment Wholesaling"@en ;
.

icat:G3900
    a skos:Concept ;
    dcterms:source "https://www.abs.gov.au/AUSSTATS/abs@.nsf/DetailsPage/1292.02006%20(Revision%202.0)?OpenDocument"^^xsd:anyURI ;
    rdfs:isDefinedBy cs: ;
    skos:broader icat:G0000 ;
    skos:definition "An individual business entity whose predominant economic activity is Motor Vehicle and Motor Vehicle Parts Retailing."@en ;
    skos:inScheme cs: ;
    skos:notation "G3900" ;
    skos:prefLabel "Motor Vehicle and Motor Vehicle Parts Retailing"@en ;
.

icat:G4100
    a skos:Concept ;
    dcterms:source "https://www.abs.gov.au/AUSSTATS/abs@.nsf/DetailsPage/1292.02006%20(Revision%202.0)?OpenDocument"^^xsd:anyURI ;
    rdfs:isDefinedBy cs: ;
    skos:broader icat:G0000 ;
    skos:definition "An individual business entity whose predominant economic activity is Food Retailing."@en ;
    skos:inScheme cs: ;
    skos:notation "G4100" ;
    skos:prefLabel "Food Retailing"@en ;
.

icat:G4300
    a skos:Concept ;
    dcterms:source "https://www.abs.gov.au/AUSSTATS/abs@.nsf/DetailsPage/1292.02006%20(Revision%202.0)?OpenDocument"^^xsd:anyURI ;
    rdfs:isDefinedBy cs: ;
    skos:broader icat:G0000 ;
    skos:definition "An individual business entity whose predominant economic activity is Non-Store Retailing and Retail Commission-Based Buying and/or Selling."@en ;
    skos:inScheme cs: ;
    skos:notation "G4300" ;
    skos:prefLabel "Non-Store Retailing and Retail Commission-Based Buying and/or Selling"@en ;
.

icat:I4600
    a skos:Concept ;
    dcterms:source "https://www.abs.gov.au/AUSSTATS/abs@.nsf/DetailsPage/1292.02006%20(Revision%202.0)?OpenDocument"^^xsd:anyURI ;
    rdfs:isDefinedBy cs: ;
    skos:broader icat:I0000 ;
    skos:definition "An individual business entity whose predominant economic activity is Road Transport."@en ;
    skos:inScheme cs: ;
    skos:notation "I4600" ;
    skos:prefLabel "Road Transport"@en ;
.

icat:I4700
    a skos:Concept ;
    dcterms:source "https://www.abs.gov.au/AUSSTATS/abs@.nsf/DetailsPage/1292.02006%20(Revision%202.0)?OpenDocument"^^xsd:anyURI ;
    rdfs:isDefinedBy cs: ;
    skos:broader icat:I0000 ;
    skos:definition "An individual business entity whose predominant economic activity is Rail Transport."@en ;
    skos:inScheme cs: ;
    skos:notation "I4700" ;
    skos:prefLabel "Rail Transport"@en ;
.

icat:I4800
    a skos:Concept ;
    dcterms:source "https://www.abs.gov.au/AUSSTATS/abs@.nsf/DetailsPage/1292.02006%20(Revision%202.0)?OpenDocument"^^xsd:anyURI ;
    rdfs:isDefinedBy cs: ;
    skos:broader icat:I0000 ;
    skos:definition "An individual business entity whose predominant economic activity is Water Transport."@en ;
    skos:inScheme cs: ;
    skos:notation "I4800" ;
    skos:prefLabel "Water Transport"@en ;
.

icat:I5000
    a skos:Concept ;
    dcterms:source "https://www.abs.gov.au/AUSSTATS/abs@.nsf/DetailsPage/1292.02006%20(Revision%202.0)?OpenDocument"^^xsd:anyURI ;
    rdfs:isDefinedBy cs: ;
    skos:broader icat:I0000 ;
    skos:definition "An individual business entity whose predominant economic activity is Other Transport."@en ;
    skos:inScheme cs: ;
    skos:notation "I5000" ;
    skos:prefLabel "Other Transport"@en ;
.

icat:J5400
    a skos:Concept ;
    dcterms:source "https://www.abs.gov.au/AUSSTATS/abs@.nsf/DetailsPage/1292.02006%20(Revision%202.0)?OpenDocument"^^xsd:anyURI ;
    rdfs:isDefinedBy cs: ;
    skos:broader icat:J0000 ;
    skos:definition "An individual business entity whose predominant economic activity is Publishing (except Internet and Music Publishing)."@en ;
    skos:inScheme cs: ;
    skos:notation "J5400" ;
    skos:prefLabel "Publishing (except Internet and Music Publishing)"@en ;
.

icat:J5500
    a skos:Concept ;
    dcterms:source "https://www.abs.gov.au/AUSSTATS/abs@.nsf/DetailsPage/1292.02006%20(Revision%202.0)?OpenDocument"^^xsd:anyURI ;
    rdfs:isDefinedBy cs: ;
    skos:broader icat:J0000 ;
    skos:definition "An individual business entity whose predominant economic activity is Motion Picture and Sound Recording Activities."@en ;
    skos:inScheme cs: ;
    skos:notation "J5500" ;
    skos:prefLabel "Motion Picture and Sound Recording Activities"@en ;
.

icat:J5600
    a skos:Concept ;
    dcterms:source "https://www.abs.gov.au/AUSSTATS/abs@.nsf/DetailsPage/1292.02006%20(Revision%202.0)?OpenDocument"^^xsd:anyURI ;
    rdfs:isDefinedBy cs: ;
    skos:broader icat:J0000 ;
    skos:definition "An individual business entity whose predominant economic activity is Broadcasting (except Internet)."@en ;
    skos:inScheme cs: ;
    skos:notation "J5600" ;
    skos:prefLabel "Broadcasting (except Internet)"@en ;
.

icat:J5900
    a skos:Concept ;
    dcterms:source "https://www.abs.gov.au/AUSSTATS/abs@.nsf/DetailsPage/1292.02006%20(Revision%202.0)?OpenDocument"^^xsd:anyURI ;
    rdfs:isDefinedBy cs: ;
    skos:broader icat:J0000 ;
    skos:definition "An individual business entity whose predominant economic activity is Internet Service Providers, Web Search Portals and Data Processing Services."@en ;
    skos:inScheme cs: ;
    skos:notation "J5900" ;
    skos:prefLabel "Internet Service Providers, Web Search Portals and Data Processing Services"@en ;
.

icat:J6000
    a skos:Concept ;
    dcterms:source "https://www.abs.gov.au/AUSSTATS/abs@.nsf/DetailsPage/1292.02006%20(Revision%202.0)?OpenDocument"^^xsd:anyURI ;
    rdfs:isDefinedBy cs: ;
    skos:broader icat:J0000 ;
    skos:definition "An individual business entity whose predominant economic activity is Library and Other Information Services."@en ;
    skos:inScheme cs: ;
    skos:notation "J6000" ;
    skos:prefLabel "Library and Other Information Services"@en ;
.

icat:K6400
    a skos:Concept ;
    dcterms:source "https://www.abs.gov.au/AUSSTATS/abs@.nsf/DetailsPage/1292.02006%20(Revision%202.0)?OpenDocument"^^xsd:anyURI ;
    rdfs:isDefinedBy cs: ;
    skos:broader icat:K0000 ;
    skos:definition "An individual business entity whose predominant economic activity is Auxiliary Finance and Insurance Services."@en ;
    skos:inScheme cs: ;
    skos:notation "K6400" ;
    skos:prefLabel "Auxiliary Finance and Insurance Services"@en ;
.

icat:L6700
    a skos:Concept ;
    dcterms:source "https://www.abs.gov.au/AUSSTATS/abs@.nsf/DetailsPage/1292.02006%20(Revision%202.0)?OpenDocument"^^xsd:anyURI ;
    rdfs:isDefinedBy cs: ;
    skos:broader icat:L0000 ;
    skos:definition "An individual business entity whose predominant economic activity is Property Operators and Real Estate Services."@en ;
    skos:inScheme cs: ;
    skos:notation "L6700" ;
    skos:prefLabel "Property Operators and Real Estate Services"@en ;
.

icat:N7300
    a skos:Concept ;
    dcterms:source "https://www.abs.gov.au/AUSSTATS/abs@.nsf/DetailsPage/1292.02006%20(Revision%202.0)?OpenDocument"^^xsd:anyURI ;
    rdfs:isDefinedBy cs: ;
    skos:broader icat:N0000 ;
    skos:definition "An individual business entity whose predominant economic activity is Building Cleaning, Pest Control and Other Support Services."@en ;
    skos:inScheme cs: ;
    skos:notation "N7300" ;
    skos:prefLabel "Building Cleaning, Pest Control and Other Support Services"@en ;
.

icat:O7700
    a skos:Concept ;
    dcterms:source "https://www.abs.gov.au/AUSSTATS/abs@.nsf/DetailsPage/1292.02006%20(Revision%202.0)?OpenDocument"^^xsd:anyURI ;
    rdfs:isDefinedBy cs: ;
    skos:broader icat:O0000 ;
    skos:definition "An individual business entity whose predominant economic activity is Public Order, Safety and Regulatory Services."@en ;
    skos:inScheme cs: ;
    skos:notation "O7700" ;
    skos:prefLabel "Public Order, Safety and Regulatory Services"@en ;
.

icat:P8000
    a skos:Concept ;
    dcterms:source "https://www.abs.gov.au/AUSSTATS/abs@.nsf/DetailsPage/1292.02006%20(Revision%202.0)?OpenDocument"^^xsd:anyURI ;
    rdfs:isDefinedBy cs: ;
    skos:broader icat:P0000 ;
    skos:definition "An individual business entity whose predominant economic activity is Preschool and School Education."@en ;
    skos:inScheme cs: ;
    skos:notation "P8000" ;
    skos:prefLabel "Preschool and School Education"@en ;
.

icat:Q8700
    a skos:Concept ;
    dcterms:source "https://www.abs.gov.au/AUSSTATS/abs@.nsf/DetailsPage/1292.02006%20(Revision%202.0)?OpenDocument"^^xsd:anyURI ;
    rdfs:isDefinedBy cs: ;
    skos:broader icat:Q0000 ;
    skos:definition "An individual business entity whose predominant economic activity is Social Assistance Services."@en ;
    skos:inScheme cs: ;
    skos:notation "Q8700" ;
    skos:prefLabel "Social Assistance Services"@en ;
.

icat:R8900
    a skos:Concept ;
    dcterms:source "https://www.abs.gov.au/AUSSTATS/abs@.nsf/DetailsPage/1292.02006%20(Revision%202.0)?OpenDocument"^^xsd:anyURI ;
    rdfs:isDefinedBy cs: ;
    skos:broader icat:R0000 ;
    skos:definition "An individual business entity whose predominant economic activity is Heritage Activities."@en ;
    skos:inScheme cs: ;
    skos:notation "R8900" ;
    skos:prefLabel "Heritage Activities"@en ;
.

<https://linked.data.gov.au/org/gsq>
    a sdo:Organization ;
    sdo:name "Geological Survey of Queensland" ;
    sdo:url "https://www.business.qld.gov.au/industries/mining-energy-water/resources/geoscience-information/gsq"^^xsd:anyURI ;
.

icat:F3300
    a skos:Concept ;
    dcterms:source "https://www.abs.gov.au/AUSSTATS/abs@.nsf/DetailsPage/1292.02006%20(Revision%202.0)?OpenDocument"^^xsd:anyURI ;
    rdfs:isDefinedBy cs: ;
    skos:broader icat:F0000 ;
    skos:definition "An individual business entity whose predominant economic activity is Basic Material Wholesaling."@en ;
    skos:inScheme cs: ;
    skos:notation "F3300" ;
    skos:prefLabel "Basic Material Wholesaling"@en ;
.

icat:F3700
    a skos:Concept ;
    dcterms:source "https://www.abs.gov.au/AUSSTATS/abs@.nsf/DetailsPage/1292.02006%20(Revision%202.0)?OpenDocument"^^xsd:anyURI ;
    rdfs:isDefinedBy cs: ;
    skos:broader icat:F0000 ;
    skos:definition "An individual business entity whose predominant economic activity is Other Goods Wholesaling."@en ;
    skos:inScheme cs: ;
    skos:notation "F3700" ;
    skos:prefLabel "Other Goods Wholesaling"@en ;
.

icat:H0000
    a skos:Concept ;
    dcterms:source "https://www.abs.gov.au/AUSSTATS/abs@.nsf/DetailsPage/1292.02006%20(Revision%202.0)?OpenDocument"^^xsd:anyURI ;
    rdfs:isDefinedBy cs: ;
    skos:definition "An individual business entity whose predominant economic activity is Accommodation and Food Services."@en ;
    skos:inScheme cs: ;
    skos:notation "H0000" ;
    skos:prefLabel "Accommodation and Food Services"@en ;
    skos:topConceptOf cs: ;
.

icat:H4500
    a skos:Concept ;
    dcterms:source "https://www.abs.gov.au/AUSSTATS/abs@.nsf/DetailsPage/1292.02006%20(Revision%202.0)?OpenDocument"^^xsd:anyURI ;
    rdfs:isDefinedBy cs: ;
    skos:broader icat:H0000 ;
    skos:definition "An individual business entity whose predominant economic activity is Food and Beverage Services."@en ;
    skos:inScheme cs: ;
    skos:notation "H4500" ;
    skos:prefLabel "Food and Beverage Services"@en ;
.

icat:I5200
    a skos:Concept ;
    dcterms:source "https://www.abs.gov.au/AUSSTATS/abs@.nsf/DetailsPage/1292.02006%20(Revision%202.0)?OpenDocument"^^xsd:anyURI ;
    rdfs:isDefinedBy cs: ;
    skos:broader icat:I0000 ;
    skos:definition "An individual business entity whose predominant economic activity is Transport Support Services."@en ;
    skos:inScheme cs: ;
    skos:notation "I5200" ;
    skos:prefLabel "Transport Support Services"@en ;
.

icat:K6300
    a skos:Concept ;
    dcterms:source "https://www.abs.gov.au/AUSSTATS/abs@.nsf/DetailsPage/1292.02006%20(Revision%202.0)?OpenDocument"^^xsd:anyURI ;
    rdfs:isDefinedBy cs: ;
    skos:broader icat:K0000 ;
    skos:definition "An individual business entity whose predominant economic activity is Insurance and Superannuation Funds."@en ;
    skos:inScheme cs: ;
    skos:notation "K6300" ;
    skos:prefLabel "Insurance and Superannuation Funds"@en ;
.

icat:L0000
    a skos:Concept ;
    dcterms:source "https://www.abs.gov.au/AUSSTATS/abs@.nsf/DetailsPage/1292.02006%20(Revision%202.0)?OpenDocument"^^xsd:anyURI ;
    rdfs:isDefinedBy cs: ;
    skos:definition "An individual business entity whose predominant economic activity is Rental, Hiring and Real Estate Services."@en ;
    skos:inScheme cs: ;
    skos:notation "L0000" ;
    skos:prefLabel "Rental, Hiring and Real Estate Services"@en ;
    skos:topConceptOf cs: ;
.

icat:M0000
    a skos:Concept ;
    dcterms:source "https://www.abs.gov.au/AUSSTATS/abs@.nsf/DetailsPage/1292.02006%20(Revision%202.0)?OpenDocument"^^xsd:anyURI ;
    rdfs:isDefinedBy cs: ;
    skos:definition "An individual business entity whose predominant economic activity is Professional, Scientific and Technical Services."@en ;
    skos:inScheme cs: ;
    skos:notation "M0000" ;
    skos:prefLabel "Professional, Scientific and Technical Services"@en ;
    skos:topConceptOf cs: ;
.

icat:N0000
    a skos:Concept ;
    dcterms:source "https://www.abs.gov.au/AUSSTATS/abs@.nsf/DetailsPage/1292.02006%20(Revision%202.0)?OpenDocument"^^xsd:anyURI ;
    rdfs:isDefinedBy cs: ;
    skos:definition "An individual business entity whose predominant economic activity is Administrative and Support Services."@en ;
    skos:inScheme cs: ;
    skos:notation "N0000" ;
    skos:prefLabel "Administrative and Support Services"@en ;
    skos:topConceptOf cs: ;
.

icat:N7200
    a skos:Concept ;
    dcterms:source "https://www.abs.gov.au/AUSSTATS/abs@.nsf/DetailsPage/1292.02006%20(Revision%202.0)?OpenDocument"^^xsd:anyURI ;
    rdfs:isDefinedBy cs: ;
    skos:broader icat:N0000 ;
    skos:definition "An individual business entity whose predominant economic activity is Administrative Services."@en ;
    skos:inScheme cs: ;
    skos:notation "N7200" ;
    skos:prefLabel "Administrative Services"@en ;
.

icat:R9100
    a skos:Concept ;
    dcterms:source "https://www.abs.gov.au/AUSSTATS/abs@.nsf/DetailsPage/1292.02006%20(Revision%202.0)?OpenDocument"^^xsd:anyURI ;
    rdfs:isDefinedBy cs: ;
    skos:broader icat:R0000 ;
    skos:definition "An individual business entity whose predominant economic activity is Sports and Recreation Activities."@en ;
    skos:inScheme cs: ;
    skos:notation "R9100" ;
    skos:prefLabel "Sports and Recreation Activities"@en ;
.

icat:S9400
    a skos:Concept ;
    dcterms:source "https://www.abs.gov.au/AUSSTATS/abs@.nsf/DetailsPage/1292.02006%20(Revision%202.0)?OpenDocument"^^xsd:anyURI ;
    rdfs:isDefinedBy cs: ;
    skos:broader icat:S0000 ;
    skos:definition "An individual business entity whose predominant economic activity is Repair and Maintenance."@en ;
    skos:inScheme cs: ;
    skos:notation "S9400" ;
    skos:prefLabel "Repair and Maintenance"@en ;
.

icat:X0000
    a skos:Concept ;
    dcterms:source "https://www.abs.gov.au/AUSSTATS/abs@.nsf/DetailsPage/1292.02006%20(Revision%202.0)?OpenDocument"^^xsd:anyURI ;
    rdfs:isDefinedBy cs: ;
    skos:definition "An individual business entity whose predominant economic activity is Undefined Industry."@en ;
    skos:inScheme cs: ;
    skos:notation "X0000" ;
    skos:prefLabel "Undefined Industry"@en ;
    skos:topConceptOf cs: ;
.

icat:C2000
    a skos:Concept ;
    dcterms:source "https://www.abs.gov.au/AUSSTATS/abs@.nsf/DetailsPage/1292.02006%20(Revision%202.0)?OpenDocument"^^xsd:anyURI ;
    rdfs:isDefinedBy cs: ;
    skos:broader icat:C0000 ;
    skos:definition "An individual business entity whose predominant economic activity is Non-Metallic Mineral Product Manufacturing."@en ;
    skos:inScheme cs: ;
    skos:notation "C2000" ;
    skos:prefLabel "Non-Metallic Mineral Product Manufacturing"@en ;
.

icat:D2600
    a skos:Concept ;
    dcterms:source "https://www.abs.gov.au/AUSSTATS/abs@.nsf/DetailsPage/1292.02006%20(Revision%202.0)?OpenDocument"^^xsd:anyURI ;
    rdfs:isDefinedBy cs: ;
    skos:broader icat:D0000 ;
    skos:definition "An individual business entity whose predominant economic activity is Electricity Supply."@en ;
    skos:inScheme cs: ;
    skos:notation "D2600" ;
    skos:prefLabel "Electricity Supply"@en ;
.

icat:E0000
    a skos:Concept ;
    dcterms:source "https://www.abs.gov.au/AUSSTATS/abs@.nsf/DetailsPage/1292.02006%20(Revision%202.0)?OpenDocument"^^xsd:anyURI ;
    rdfs:isDefinedBy cs: ;
    skos:definition "An individual business entity whose predominant economic activity is Construction."@en ;
    skos:inScheme cs: ;
    skos:notation "E0000" ;
    skos:prefLabel "Construction"@en ;
    skos:topConceptOf cs: ;
.

icat:K0000
    a skos:Concept ;
    dcterms:source "https://www.abs.gov.au/AUSSTATS/abs@.nsf/DetailsPage/1292.02006%20(Revision%202.0)?OpenDocument"^^xsd:anyURI ;
    rdfs:isDefinedBy cs: ;
    skos:definition "An individual business entity whose predominant economic activity is Financial and Insurance Services."@en ;
    skos:inScheme cs: ;
    skos:notation "K0000" ;
    skos:prefLabel "Financial and Insurance Services"@en ;
    skos:topConceptOf cs: ;
.

icat:K6200
    a skos:Concept ;
    dcterms:source "https://www.abs.gov.au/AUSSTATS/abs@.nsf/DetailsPage/1292.02006%20(Revision%202.0)?OpenDocument"^^xsd:anyURI ;
    rdfs:isDefinedBy cs: ;
    skos:broader icat:K0000 ;
    skos:definition "An individual business entity whose predominant economic activity is Finance."@en ;
    skos:inScheme cs: ;
    skos:notation "K6200" ;
    skos:prefLabel "Finance"@en ;
.

icat:L6600
    a skos:Concept ;
    dcterms:source "https://www.abs.gov.au/AUSSTATS/abs@.nsf/DetailsPage/1292.02006%20(Revision%202.0)?OpenDocument"^^xsd:anyURI ;
    rdfs:isDefinedBy cs: ;
    skos:broader icat:L0000 ;
    skos:definition "An individual business entity whose predominant economic activity is Rental and Hiring Services (except Real Estate)."@en ;
    skos:inScheme cs: ;
    skos:notation "L6600" ;
    skos:prefLabel "Rental and Hiring Services (except Real Estate)"@en ;
.

icat:O0000
    a skos:Concept ;
    dcterms:source "https://www.abs.gov.au/AUSSTATS/abs@.nsf/DetailsPage/1292.02006%20(Revision%202.0)?OpenDocument"^^xsd:anyURI ;
    rdfs:isDefinedBy cs: ;
    skos:definition "An individual business entity whose predominant economic activity is Public Administration and Safety."@en ;
    skos:inScheme cs: ;
    skos:notation "O0000" ;
    skos:prefLabel "Public Administration and Safety"@en ;
    skos:topConceptOf cs: ;
.

icat:P0000
    a skos:Concept ;
    dcterms:source "https://www.abs.gov.au/AUSSTATS/abs@.nsf/DetailsPage/1292.02006%20(Revision%202.0)?OpenDocument"^^xsd:anyURI ;
    rdfs:isDefinedBy cs: ;
    skos:definition "An individual business entity whose predominant economic activity is Education and Training."@en ;
    skos:inScheme cs: ;
    skos:notation "P0000" ;
    skos:prefLabel "Education and Training"@en ;
    skos:topConceptOf cs: ;
.

icat:Q8500
    a skos:Concept ;
    dcterms:source "https://www.abs.gov.au/AUSSTATS/abs@.nsf/DetailsPage/1292.02006%20(Revision%202.0)?OpenDocument"^^xsd:anyURI ;
    rdfs:isDefinedBy cs: ;
    skos:broader icat:Q0000 ;
    skos:definition "An individual business entity whose predominant economic activity is Medical and Other Health Care Services."@en ;
    skos:inScheme cs: ;
    skos:notation "Q8500" ;
    skos:prefLabel "Medical and Other Health Care Services"@en ;
.

icat:S0000
    a skos:Concept ;
    dcterms:source "https://www.abs.gov.au/AUSSTATS/abs@.nsf/DetailsPage/1292.02006%20(Revision%202.0)?OpenDocument"^^xsd:anyURI ;
    rdfs:isDefinedBy cs: ;
    skos:definition "An individual business entity whose predominant economic activity is Other Services."@en ;
    skos:inScheme cs: ;
    skos:notation "S0000" ;
    skos:prefLabel "Other Services"@en ;
    skos:topConceptOf cs: ;
.

icat:C1300
    a skos:Concept ;
    dcterms:source "https://www.abs.gov.au/AUSSTATS/abs@.nsf/DetailsPage/1292.02006%20(Revision%202.0)?OpenDocument"^^xsd:anyURI ;
    rdfs:isDefinedBy cs: ;
    skos:broader icat:C0000 ;
    skos:definition "An individual business entity whose predominant economic activity is Textile, Leather, Clothing and Footwear Manufacturing."@en ;
    skos:inScheme cs: ;
    skos:notation "C1300" ;
    skos:prefLabel "Textile, Leather, Clothing and Footwear Manufacturing"@en ;
.

icat:C2100
    a skos:Concept ;
    dcterms:source "https://www.abs.gov.au/AUSSTATS/abs@.nsf/DetailsPage/1292.02006%20(Revision%202.0)?OpenDocument"^^xsd:anyURI ;
    rdfs:isDefinedBy cs: ;
    skos:altLabel "Metal Processing"@en ;
    skos:broader icat:C0000 ;
    skos:definition "An individual business entity whose predominant economic activity is Primary Metal and Metal Product Manufacturing."@en ;
    skos:inScheme cs: ;
    skos:notation "C2100" ;
    skos:prefLabel "Primary Metal and Metal Product Manufacturing"@en ;
.

icat:C2200
    a skos:Concept ;
    dcterms:source "https://www.abs.gov.au/AUSSTATS/abs@.nsf/DetailsPage/1292.02006%20(Revision%202.0)?OpenDocument"^^xsd:anyURI ;
    rdfs:isDefinedBy cs: ;
    skos:broader icat:C0000 ;
    skos:definition "An individual business entity whose predominant economic activity is Fabricated Metal Product Manufacturing."@en ;
    skos:inScheme cs: ;
    skos:notation "C2200" ;
    skos:prefLabel "Fabricated Metal Product Manufacturing"@en ;
.

icat:D0000
    a skos:Concept ;
    dcterms:source "https://www.abs.gov.au/AUSSTATS/abs@.nsf/DetailsPage/1292.02006%20(Revision%202.0)?OpenDocument"^^xsd:anyURI ;
    rdfs:isDefinedBy cs: ;
    skos:definition "An individual business entity whose predominant economic activity is Electricity, Gas, Water and Waste Services."@en ;
    skos:inScheme cs: ;
    skos:notation "D0000" ;
    skos:prefLabel "Electricity, Gas, Water and Waste Services"@en ;
    skos:topConceptOf cs: ;
.

icat:E3200
    a skos:Concept ;
    dcterms:source "https://www.abs.gov.au/AUSSTATS/abs@.nsf/DetailsPage/1292.02006%20(Revision%202.0)?OpenDocument"^^xsd:anyURI ;
    rdfs:isDefinedBy cs: ;
    skos:broader icat:E0000 ;
    skos:definition "An individual business entity whose predominant economic activity is Construction Services."@en ;
    skos:inScheme cs: ;
    skos:notation "E3200" ;
    skos:prefLabel "Construction Services"@en ;
.

icat:O7500
    a skos:Concept ;
    dcterms:source "https://www.abs.gov.au/AUSSTATS/abs@.nsf/DetailsPage/1292.02006%20(Revision%202.0)?OpenDocument"^^xsd:anyURI ;
    rdfs:isDefinedBy cs: ;
    skos:broader icat:O0000 ;
    skos:definition "An individual business entity whose predominant economic activity is Public Administration."@en ;
    skos:inScheme cs: ;
    skos:notation "O7500" ;
    skos:prefLabel "Public Administration"@en ;
.

icat:Q0000
    a skos:Concept ;
    dcterms:source "https://www.abs.gov.au/AUSSTATS/abs@.nsf/DetailsPage/1292.02006%20(Revision%202.0)?OpenDocument"^^xsd:anyURI ;
    rdfs:isDefinedBy cs: ;
    skos:definition "An individual business entity whose predominant economic activity is Health Care and Social Assistance."@en ;
    skos:inScheme cs: ;
    skos:notation "Q0000" ;
    skos:prefLabel "Health Care and Social Assistance"@en ;
    skos:topConceptOf cs: ;
.

icat:R0000
    a skos:Concept ;
    dcterms:source "https://www.abs.gov.au/AUSSTATS/abs@.nsf/DetailsPage/1292.02006%20(Revision%202.0)?OpenDocument"^^xsd:anyURI ;
    rdfs:isDefinedBy cs: ;
    skos:definition "An individual business entity whose predominant economic activity is Arts and Recreation Services."@en ;
    skos:inScheme cs: ;
    skos:notation "R0000" ;
    skos:prefLabel "Arts and Recreation Services"@en ;
    skos:topConceptOf cs: ;
.

icat:S9500
    a skos:Concept ;
    dcterms:source "https://www.abs.gov.au/AUSSTATS/abs@.nsf/DetailsPage/1292.02006%20(Revision%202.0)?OpenDocument"^^xsd:anyURI ;
    rdfs:isDefinedBy cs: ;
    skos:broader icat:S0000 ;
    skos:definition "An individual business entity whose predominant economic activity is Personal and Other Services."@en ;
    skos:inScheme cs: ;
    skos:notation "S9500" ;
    skos:prefLabel "Personal and Other Services"@en ;
.

icat:A0000
    a skos:Concept ;
    dcterms:source "https://www.abs.gov.au/AUSSTATS/abs@.nsf/DetailsPage/1292.02006%20(Revision%202.0)?OpenDocument"^^xsd:anyURI ;
    rdfs:isDefinedBy cs: ;
    skos:definition "An individual business entity whose predominant economic activity is Agriculture, Forestry and Fishing."@en ;
    skos:inScheme cs: ;
    skos:notation "A0000" ;
    skos:prefLabel "Agriculture, Forestry and Fishing"@en ;
    skos:topConceptOf cs: ;
.

icat:B0000
    a skos:Concept ;
    dcterms:source "https://www.abs.gov.au/AUSSTATS/abs@.nsf/DetailsPage/1292.02006%20(Revision%202.0)?OpenDocument"^^xsd:anyURI ;
    rdfs:isDefinedBy cs: ;
    skos:definition "An individual business entity whose predominant economic activity is Mining."@en ;
    skos:inScheme cs: ;
    skos:notation "B0000" ;
    skos:prefLabel "Mining"@en ;
    skos:topConceptOf cs: ;
.

icat:C1800
    a skos:Concept ;
    dcterms:source "https://www.abs.gov.au/AUSSTATS/abs@.nsf/DetailsPage/1292.02006%20(Revision%202.0)?OpenDocument"^^xsd:anyURI ;
    rdfs:isDefinedBy cs: ;
    skos:broader icat:C0000 ;
    skos:definition "An individual business entity whose predominant economic activity is Basic Chemical and Chemical Product Manufacturing."@en ;
    skos:inScheme cs: ;
    skos:notation "C1800" ;
    skos:prefLabel "Basic Chemical and Chemical Product Manufacturing"@en ;
.

icat:G0000
    a skos:Concept ;
    dcterms:source "https://www.abs.gov.au/AUSSTATS/abs@.nsf/DetailsPage/1292.02006%20(Revision%202.0)?OpenDocument"^^xsd:anyURI ;
    rdfs:isDefinedBy cs: ;
    skos:definition "An individual business entity whose predominant economic activity is Retail Trade."@en ;
    skos:inScheme cs: ;
    skos:notation "G0000" ;
    skos:prefLabel "Retail Trade"@en ;
    skos:topConceptOf cs: ;
.

icat:C2400
    a skos:Concept ;
    dcterms:source "https://www.abs.gov.au/AUSSTATS/abs@.nsf/DetailsPage/1292.02006%20(Revision%202.0)?OpenDocument"^^xsd:anyURI ;
    rdfs:isDefinedBy cs: ;
    skos:broader icat:C0000 ;
    skos:definition "An individual business entity whose predominant economic activity is Machinery and Equipment Manufacturing."@en ;
    skos:inScheme cs: ;
    skos:notation "C2400" ;
    skos:prefLabel "Machinery and Equipment Manufacturing"@en ;
.

icat:F0000
    a skos:Concept ;
    dcterms:source "https://www.abs.gov.au/AUSSTATS/abs@.nsf/DetailsPage/1292.02006%20(Revision%202.0)?OpenDocument"^^xsd:anyURI ;
    rdfs:isDefinedBy cs: ;
    skos:definition "An individual business entity whose predominant economic activity is Wholesale Trade."@en ;
    skos:inScheme cs: ;
    skos:notation "F0000" ;
    skos:prefLabel "Wholesale Trade"@en ;
    skos:topConceptOf cs: ;
.

icat:G4200
    a skos:Concept ;
    dcterms:source "https://www.abs.gov.au/AUSSTATS/abs@.nsf/DetailsPage/1292.02006%20(Revision%202.0)?OpenDocument"^^xsd:anyURI ;
    rdfs:isDefinedBy cs: ;
    skos:broader icat:G0000 ;
    skos:definition "An individual business entity whose predominant economic activity is Other Store-Based Retailing."@en ;
    skos:inScheme cs: ;
    skos:notation "G4200" ;
    skos:prefLabel "Other Store-Based Retailing"@en ;
.

icat:J0000
    a skos:Concept ;
    dcterms:source "https://www.abs.gov.au/AUSSTATS/abs@.nsf/DetailsPage/1292.02006%20(Revision%202.0)?OpenDocument"^^xsd:anyURI ;
    rdfs:isDefinedBy cs: ;
    skos:definition "An individual business entity whose predominant economic activity is Information Media and Telecommunications."@en ;
    skos:inScheme cs: ;
    skos:notation "J0000" ;
    skos:prefLabel "Information Media and Telecommunications"@en ;
    skos:topConceptOf cs: ;
.

icat:M6900
    a skos:Concept ;
    dcterms:source "https://www.abs.gov.au/AUSSTATS/abs@.nsf/DetailsPage/1292.02006%20(Revision%202.0)?OpenDocument"^^xsd:anyURI ;
    rdfs:isDefinedBy cs: ;
    skos:broader icat:M0000 ;
    skos:definition "An individual business entity whose predominant economic activity is Professional, Scientific and Technical Services (Except Computer System Design and Related Services)."@en ;
    skos:inScheme cs: ;
    skos:notation "M6900" ;
    skos:prefLabel "Professional, Scientific and Technical Services (Except Computer System Design and Related Services)"@en ;
.

icat:A0100
    a skos:Concept ;
    dcterms:source "https://www.abs.gov.au/AUSSTATS/abs@.nsf/DetailsPage/1292.02006%20(Revision%202.0)?OpenDocument"^^xsd:anyURI ;
    rdfs:isDefinedBy cs: ;
    skos:broader icat:A0000 ;
    skos:definition "An individual business entity whose predominant economic activity is Agriculture."@en ;
    skos:inScheme cs: ;
    skos:notation "A0100" ;
    skos:prefLabel "Agriculture"@en ;
.

icat:C1100
    a skos:Concept ;
    dcterms:source "https://www.abs.gov.au/AUSSTATS/abs@.nsf/DetailsPage/1292.02006%20(Revision%202.0)?OpenDocument"^^xsd:anyURI ;
    rdfs:isDefinedBy cs: ;
    skos:broader icat:C0000 ;
    skos:definition "An individual business entity whose predominant economic activity is Food Product Manufacturing."@en ;
    skos:inScheme cs: ;
    skos:notation "C1100" ;
    skos:prefLabel "Food Product Manufacturing"@en ;
.

icat:I0000
    a skos:Concept ;
    dcterms:source "https://www.abs.gov.au/AUSSTATS/abs@.nsf/DetailsPage/1292.02006%20(Revision%202.0)?OpenDocument"^^xsd:anyURI ;
    rdfs:isDefinedBy cs: ;
    skos:definition "An individual business entity whose predominant economic activity is Transport, Postal and Warehousing."@en ;
    skos:inScheme cs: ;
    skos:notation "I0000" ;
    skos:prefLabel "Transport, Postal and Warehousing"@en ;
    skos:topConceptOf cs: ;
.

icat:C0000
    a skos:Concept ;
    dcterms:source "https://www.abs.gov.au/AUSSTATS/abs@.nsf/DetailsPage/1292.02006%20(Revision%202.0)?OpenDocument"^^xsd:anyURI ;
    rdfs:isDefinedBy cs: ;
    skos:altLabel "Other Processing"@en ;
    skos:definition "An individual business entity whose predominant economic activity is Manufacturing."@en ;
    skos:inScheme cs: ;
    skos:notation "C0000" ;
    skos:prefLabel "Manufacturing"@en ;
    skos:topConceptOf cs: ;
.

cs:
    a
        owl:Ontology ,
        skos:ConceptScheme ;
    dcterms:created "2020-02-17"^^xsd:date ;
    dcterms:creator <https://linked.data.gov.au/org/gsq> ;
    dcterms:modified "2023-03-16"^^xsd:date ;
    dcterms:publisher <https://linked.data.gov.au/org/gsq> ;
    dcterms:source "https://www.abs.gov.au/AUSSTATS/abs@.nsf/DetailsPage/1292.02006%20(Revision%202.0)?OpenDocument"^^xsd:anyURI ;
    reg:status agldwgstatus:stable ;
    skos:definition """An industrial classification organises data about business units. It provides a standard framework under which business units carrying out similar production activities can be grouped together, with each resultant group referred to as an industry.\r
    An individual business entity is assigned to an industry based on its predominant economic activity. The term business entity is used in its widest sense to include any organisation undertaking productive activities, including companies, non-profit organisations, government departments and enterprises. ANZSIC has four hierarchic levels: Divisions (the broadest level), Subdivisions, Groups and Classes (the finest level).\r
    At the Divisional level, the main purpose is to provide a limited number of categories which provide a broad overall picture of the economy and are suitable for the publication of summary tables in official statistics. The Subdivision, Group and Class levels provide increasingly detailed dissections of these categories for the compilation of more specific and detailed statistics."""@en ;
    skos:hasTopConcept
        icat:A0000 ,
        icat:B0000 ,
        icat:C0000 ,
        icat:D0000 ,
        icat:E0000 ,
        icat:F0000 ,
        icat:G0000 ,
        icat:H0000 ,
        icat:I0000 ,
        icat:J0000 ,
        icat:K0000 ,
        icat:L0000 ,
        icat:M0000 ,
        icat:N0000 ,
        icat:O0000 ,
        icat:P0000 ,
        icat:Q0000 ,
        icat:R0000 ,
        icat:S0000 ,
        icat:X0000 ;
    skos:prefLabel "Australian and New Zealand Standard Industrial Classification 2006 - Codes and Titles"@en ;
.

