PREFIX aac: <http://linked.data.gov.au/def/australian-phone-area-codes/>
PREFIX agldwgstatus: <https://linked.data.gov.au/def/reg-statuses/>
PREFIX cs: <http://linked.data.gov.au/def/australian-phone-area-codes>
PREFIX dcterms: <http://purl.org/dc/terms/>
PREFIX owl: <http://www.w3.org/2002/07/owl#>
PREFIX rdfs: <http://www.w3.org/2000/01/rdf-schema#>
PREFIX reg: <http://purl.org/linked-data/registry#>
PREFIX sdo: <https://schema.org/>
PREFIX skos: <http://www.w3.org/2004/02/skos/core#>
PREFIX xsd: <http://www.w3.org/2001/XMLSchema#>

aac:02
    a skos:Concept ;
    dcterms:provenance "Derived from Australian Standard AS 4590.1:2017 citing The Australian Communications Media Authority (ACMA) Telecommunications Numbering Plan 2015." ;
    rdfs:isDefinedBy cs: ;
    skos:altLabel "(02)"@en ;
    skos:definition "The Australian telephone area code for New South Wales and the Australian Captial Territory. (ACMA)"@en ;
    skos:inScheme cs: ;
    skos:prefLabel "02"@en ;
    skos:topConceptOf cs: ;
.

aac:03
    a skos:Concept ;
    dcterms:provenance "Derived from Australian Standard AS 4590.1:2017 citing The Australian Communications Media Authority (ACMA) Telecommunications Numbering Plan 2015." ;
    rdfs:isDefinedBy cs: ;
    skos:altLabel "(03)"@en ;
    skos:definition "The Australian telephone area code for Victoria and Tasmania. (ACMA)"@en ;
    skos:inScheme cs: ;
    skos:prefLabel "03"@en ;
    skos:topConceptOf cs: ;
.

aac:07
    a skos:Concept ;
    dcterms:provenance "Derived from Australian Standard AS 4590.1:2017 citing The Australian Communications Media Authority (ACMA) Telecommunications Numbering Plan 2015." ;
    rdfs:isDefinedBy cs: ;
    skos:altLabel "(07)"@en ;
    skos:definition "The Australian telephone area code for Queensland. (ACMA)"@en ;
    skos:inScheme cs: ;
    skos:prefLabel "07"@en ;
    skos:topConceptOf cs: ;
.

aac:08
    a skos:Concept ;
    dcterms:provenance "Derived from Australian Standard AS 4590.1:2017 citing The Australian Communications Media Authority (ACMA) Telecommunications Numbering Plan 2015." ;
    rdfs:isDefinedBy cs: ;
    skos:altLabel "(08)"@en ;
    skos:definition "The Australian telephone area code for South Australia and Western Australia, including Christmas Island  and Cocos (Keeling) Islands. (ACMA)"@en ;
    skos:inScheme cs: ;
    skos:prefLabel "08"@en ;
    skos:topConceptOf cs: ;
.

<https://linked.data.gov.au/org/gsq>
    a sdo:Organization ;
    sdo:name "Geological Survey of Queensland" ;
    sdo:url "http://www.business.qld.gov.au/industries/mining-energy-water/resources/geoscience-information/gsq"^^xsd:anyURI ;
.

cs:
    a
        owl:Ontology ,
        skos:ConceptScheme ;
    dcterms:created "2020-03-25"^^xsd:date ;
    dcterms:creator <https://linked.data.gov.au/org/gsq> ;
    dcterms:modified "2023-03-16"^^xsd:date ;
    dcterms:provenance "Derived from Australian Standard AS 4590.1:2017 citing The Australian Communications Media Authority (ACMA) Telecommunications Numbering Plan 2015." ;
    dcterms:publisher <https://linked.data.gov.au/org/gsq> ;
    reg:status agldwgstatus:stable ;
    skos:definition "A two-digit-prefix code denoting the area in Australia to which a fixed telephone is registered."@en ;
    skos:hasTopConcept
        aac:02 ,
        aac:03 ,
        aac:07 ,
        aac:08 ;
    skos:prefLabel "Australian Telephone Area Codes"@en ;
.

