PREFIX agldwgstatus: <https://linked.data.gov.au/def/reg-statuses/>
PREFIX bhsp: <http://linked.data.gov.au/def/borehole-start-point/>
PREFIX cs: <http://linked.data.gov.au/def/borehole-start-point>
PREFIX dcterms: <http://purl.org/dc/terms/>
PREFIX owl: <http://www.w3.org/2002/07/owl#>
PREFIX rdfs: <http://www.w3.org/2000/01/rdf-schema#>
PREFIX reg: <http://purl.org/linked-data/registry#>
PREFIX sdo: <https://schema.org/>
PREFIX skos: <http://www.w3.org/2004/02/skos/core#>
PREFIX xsd: <http://www.w3.org/2001/XMLSchema#>

bhsp:from-pre-existing-hole
    a skos:Concept ;
    dcterms:provenance "Derived from the 201109 version of CGI Borehole start point list" ;
    rdfs:isDefinedBy cs: ;
    skos:definition "Indicates that the borehole was drilled from a pre-existing hole."@en ;
    skos:exactMatch <http://resource.geosciml.org/classifier/cgi/boreholestartpoint/0002> ;
    skos:inScheme cs: ;
    skos:prefLabel "From pre-existing hole"@en ;
    skos:topConceptOf cs: ;
.

bhsp:natural-ground-surface
    a skos:Concept ;
    dcterms:provenance "Derived from the 201109 version of CGI Borehole start point list" ;
    rdfs:isDefinedBy cs: ;
    skos:definition "Indicates that the borehole was drilled from the natural ground surface."@en ;
    skos:exactMatch <http://resource.geosciml.org/classifier/cgi/boreholestartpoint/0003> ;
    skos:inScheme cs: ;
    skos:prefLabel "Natural ground surface"@en ;
    skos:topConceptOf cs: ;
.

bhsp:offshore
    a skos:Concept ;
    dcterms:provenance "Derived from the 201109 version of CGI Borehole start point list" ;
    rdfs:isDefinedBy cs: ;
    skos:definition "Indicates that the borehole was drilled from an offshore platform, such as a petroleum platform or a marine research vessel."@en ;
    skos:exactMatch <http://resource.geosciml.org/classifier/cgi/boreholestartpoint/0005> ;
    skos:inScheme cs: ;
    skos:prefLabel "Offshore"@en ;
    skos:topConceptOf cs: ;
.

bhsp:open-pit-floor-or-wall
    a skos:Concept ;
    dcterms:provenance "Derived from the 201109 version of CGI Borehole start point list" ;
    rdfs:isDefinedBy cs: ;
    skos:definition "Indicates that the borehole was drilled from an open pit floor or open pit wall."@en ;
    skos:exactMatch <http://resource.geosciml.org/classifier/cgi/boreholestartpoint/0004> ;
    skos:inScheme cs: ;
    skos:prefLabel "Open pit floor or wall"@en ;
    skos:topConceptOf cs: ;
.

bhsp:underground
    a skos:Concept ;
    dcterms:provenance "Derived from the 201109 version of CGI Borehole start point list" ;
    rdfs:isDefinedBy cs: ;
    skos:definition "Indicates that the borehole was drilled from an underground location."@en ;
    skos:exactMatch <http://resource.geosciml.org/classifier/cgi/boreholestartpoint/0001> ;
    skos:inScheme cs: ;
    skos:prefLabel "Underground"@en ;
    skos:topConceptOf cs: ;
.

<https://linked.data.gov.au/org/gsq>
    a sdo:Organization ;
    sdo:name "Geological Survey of Queensland" ;
    sdo:url "http://www.business.qld.gov.au/industries/mining-energy-water/resources/geoscience-information/gsq"^^xsd:anyURI ;
.

cs:
    a
        owl:Ontology ,
        skos:ConceptScheme ;
    dcterms:created "2020-04-02"^^xsd:date ;
    dcterms:creator <https://linked.data.gov.au/org/gsq> ;
    dcterms:modified "2023-03-16"^^xsd:date ;
    dcterms:provenance "Derived from the 201109 version of CGI Borehole start point list" ;
    dcterms:publisher <https://linked.data.gov.au/org/gsq> ;
    reg:status agldwgstatus:stable ;
    skos:definition "Indicates the nature of the borehole start point location."@en ;
    skos:hasTopConcept
        bhsp:from-pre-existing-hole ,
        bhsp:natural-ground-surface ,
        bhsp:offshore ,
        bhsp:open-pit-floor-or-wall ,
        bhsp:underground ;
    skos:prefLabel "Borehole Start Point"@en ;
.

