PREFIX agldwgstatus: <https://linked.data.gov.au/def/reg-statuses/>
PREFIX bhd: <http://linked.data.gov.au/def/borehole-design/>
PREFIX cs: <http://linked.data.gov.au/def/borehole-design>
PREFIX dcterms: <http://purl.org/dc/terms/>
PREFIX owl: <http://www.w3.org/2002/07/owl#>
PREFIX reg: <http://purl.org/linked-data/registry#>
PREFIX sdo: <https://schema.org/>
PREFIX skos: <http://www.w3.org/2004/02/skos/core#>
PREFIX xsd: <http://www.w3.org/2001/XMLSchema#>

bhd:deviated
    a skos:Concept ;
    dcterms:provenance "Developed by the Geological Survey of Queensland." ;
    skos:altLabel "Directional"@en ;
    skos:definition "A borehole drilled with geosteering equipment with the intent of controlling inclination and/or azimuth on a specified trajectory to intersect a target or targets."@en ;
    skos:inScheme cs: ;
    skos:prefLabel "Deviated"@en ;
    skos:topConceptOf cs: ;
.

bhd:inclineddown
    a skos:Concept ;
    dcterms:provenance "Developed by the Geological Survey of Queensland." ;
    skos:altLabel "Inclined"@en ;
    skos:definition "A borehole drilled without geosteering equipment at a non-vertical angle at or below horizontal."@en ;
    skos:inScheme cs: ;
    skos:prefLabel "Inclined Down"@en ;
    skos:topConceptOf cs: ;
.

bhd:inclinedup
    a skos:Concept ;
    dcterms:provenance "Developed by the Geological Survey of Queensland." ;
    skos:definition "A borehole drilled without geosteering equipment at a non-vertical angle above horizontal."@en ;
    skos:inScheme cs: ;
    skos:prefLabel "Inclined Up"@en ;
    skos:topConceptOf cs: ;
.

bhd:lateral
    a skos:Concept ;
    dcterms:provenance "Developed by the Geological Survey of Queensland." ;
    skos:altLabel "Horizontal"@en ;
    skos:definition "A borehole drilled with geosteering equipment with the intent of controlling the trajectory to drill laterally within a targeted stratigraphic interval or intervals."@en ;
    skos:inScheme cs: ;
    skos:prefLabel "Lateral"@en ;
    skos:topConceptOf cs: ;
.

bhd:vertical
    a skos:Concept ;
    dcterms:provenance "Developed by the Geological Survey of Queensland." ;
    skos:definition "A borehole drilled in a vertical downward direction with the intent of maintaining a vertical trajectory."@en ;
    skos:inScheme cs: ;
    skos:prefLabel "Vertical"@en ;
    skos:topConceptOf cs: ;
.

<https://linked.data.gov.au/org/gsq>
    a sdo:Organization ;
    sdo:name "Geological Survey of Queensland" ;
    sdo:url "http://www.business.qld.gov.au/industries/mining-energy-water/resources/geoscience-information/gsq"^^xsd:anyURI ;
.

cs:
    a
        owl:Ontology ,
        skos:ConceptScheme ;
    dcterms:created "2019-10-03T16:24:51"^^xsd:dateTime ;
    dcterms:creator <https://linked.data.gov.au/org/gsq> ;
    dcterms:modified "2023-03-16"^^xsd:date ;
    dcterms:provenance "Developed by the Geological Survey of Queensland." ;
    dcterms:publisher <https://linked.data.gov.au/org/gsq> ;
    reg:status agldwgstatus:stable ;
    skos:definition "A description of the intended configuration and trajectory of a borehole."@en ;
    skos:hasTopConcept
        bhd:deviated ,
        bhd:inclineddown ,
        bhd:inclinedup ,
        bhd:lateral ,
        bhd:vertical ;
    skos:prefLabel "Borehole Design"@en ;
.

