PREFIX agldwgstatus: <https://linked.data.gov.au/def/reg-statuses/>
PREFIX bhfunc: <http://linked.data.gov.au/def/borehole-sub-purpose/>
PREFIX cs: <http://linked.data.gov.au/def/borehole-sub-purpose>
PREFIX dcterms: <http://purl.org/dc/terms/>
PREFIX owl: <http://www.w3.org/2002/07/owl#>
PREFIX rdfs: <http://www.w3.org/2000/01/rdf-schema#>
PREFIX reg: <http://purl.org/linked-data/registry#>
PREFIX sdo: <https://schema.org/>
PREFIX skos: <http://www.w3.org/2004/02/skos/core#>
PREFIX xsd: <http://www.w3.org/2001/XMLSchema#>

bhfunc:acid-leachate-testing
    a skos:Concept ;
    skos:historyNote "Compiled by the Geological Survey of Queensland" ;
    rdfs:isDefinedBy cs: ;
    skos:broader bhfunc:environmental ;
    skos:definition "A well or bore drilled to recover strata samples for their use in acid leachate testing."@en ;
    skos:inScheme cs: ;
    skos:prefLabel "acid leachate testing"@en ;
.

bhfunc:ballast
    a skos:Concept ;
    skos:historyNote "Compiled by the Geological Survey of Queensland" ;
    rdfs:isDefinedBy cs: ;
    skos:broader bhfunc:service ;
    skos:definition "A well or bore through which ballast is transported to and from mine workings."@en ;
    skos:inScheme cs: ;
    skos:prefLabel "ballast"@en ;
.

bhfunc:cement
    a skos:Concept ;
    skos:historyNote "Compiled by the Geological Survey of Queensland" ;
    rdfs:isDefinedBy cs: ;
    skos:broader bhfunc:service ;
    skos:definition "A well or bore through which cement is transported to and from mine workings."@en ;
    skos:inScheme cs: ;
    skos:prefLabel "cement"@en ;
.

bhfunc:chemical-flood
    a skos:Concept ;
    skos:historyNote "Compiled by the Geological Survey of Queensland" ;
    rdfs:isDefinedBy cs: ;
    skos:broader bhfunc:stimulation ;
    skos:definition "The introduction of chemicals to either increase the receptiveness of a petroleum system to other improved recovery techniques, or to improve recovery in its own right."@en ;
    skos:inScheme cs: ;
    skos:prefLabel "Chemical Flood"@en ;
.

bhfunc:compliance-gas-testing
    a skos:Concept ;
    skos:historyNote "Compiled by the Geological Survey of Queensland" ;
    rdfs:isDefinedBy cs: ;
    skos:broader bhfunc:gas-management ;
    skos:definition "Gas content testing in drainage areas to ensure remaining gas content is below the mining threshold."@en ;
    skos:inScheme cs: ;
    skos:prefLabel "compliance gas testing"@en ;
.

bhfunc:controlled-pressure-well
    a skos:Concept ;
    skos:historyNote "Compiled by the Geological Survey of Queensland" ;
    rdfs:isDefinedBy cs: ;
    skos:broader bhfunc:gas-management ;
    skos:definition "A well drilled to provide a mechanism for the control of pressure in a system."@en ;
    skos:inScheme cs: ;
    skos:prefLabel "controlled pressure well"@en ;
.

bhfunc:electricity
    a skos:Concept ;
    skos:historyNote "Compiled by the Geological Survey of Queensland" ;
    rdfs:isDefinedBy cs: ;
    skos:broader bhfunc:service ;
    skos:definition "A well or bore through which electricity is provided to mine workings."@en ;
    skos:inScheme cs: ;
    skos:prefLabel "electricity"@en ;
.

bhfunc:end-of-borehole-well
    a skos:Concept ;
    skos:historyNote "Compiled by the Geological Survey of Queensland" ;
    rdfs:isDefinedBy cs: ;
    skos:broader bhfunc:gas-management ;
    skos:definition "A well drilled to be intersected by a ranging well."@en ;
    skos:inScheme cs: ;
    skos:prefLabel "end of borehole well"@en ;
.

bhfunc:extensometer
    a skos:Concept ;
    skos:historyNote "Compiled by the Geological Survey of Queensland" ;
    rdfs:isDefinedBy cs: ;
    skos:broader bhfunc:geotech ;
    skos:definition "A well or bore drilled to facilitate strain measurements and tensile tests through the use of an extensometer."@en ;
    skos:inScheme cs: ;
    skos:prefLabel "extensometer"@en ;
.

bhfunc:fault-delineation
    a skos:Concept ;
    skos:historyNote "Compiled by the Geological Survey of Queensland" ;
    rdfs:isDefinedBy cs: ;
    skos:broader bhfunc:structure ;
    skos:definition "Borehole drilled to define a fault structure."@en ;
    skos:inScheme cs: ;
    skos:prefLabel "fault delineation"@en ;
.

bhfunc:fire-flood
    a skos:Concept ;
    skos:historyNote "Compiled by the Geological Survey of Queensland" ;
    rdfs:isDefinedBy cs: ;
    skos:broader bhfunc:stimulation ;
    skos:definition "The ignition of a petroleum system to inject heat, improving recovery through the reduction of viscosity, displacement by combustion products and more beneficial pressure gradients."@en ;
    skos:inScheme cs: ;
    skos:prefLabel "Fire Flood"@en ;
.

bhfunc:gas-drainage-undifferentiated
    a skos:Concept ;
    skos:historyNote "Compiled by the Geological Survey of Queensland" ;
    rdfs:isDefinedBy cs: ;
    skos:broader bhfunc:gas-management ;
    skos:definition "A well or bore drilled to remove gas from a subsurface system without any intent for commercialisation."@en ;
    skos:inScheme cs: ;
    skos:prefLabel "gas drainage undifferentiated"@en ;
.

bhfunc:gas-flood
    a skos:Concept ;
    skos:historyNote "Compiled by the Geological Survey of Queensland" ;
    rdfs:isDefinedBy cs: ;
    skos:broader bhfunc:stimulation ;
    skos:definition "The introduction of a gas to a petroleum system to improve recovery through displacement and more beneficial pressure gradients."@en ;
    skos:inScheme cs: ;
    skos:prefLabel "Gas Flood"@en ;
.

bhfunc:geotechnical-properties
    a skos:Concept ;
    skos:historyNote "Compiled by the Geological Survey of Queensland" ;
    rdfs:isDefinedBy cs: ;
    skos:broader bhfunc:geotech ;
    skos:definition "A borehole drilled to obtain strata core for geotechnical rock property testing."@en ;
    skos:inScheme cs: ;
    skos:prefLabel "geotechnical properties"@en ;
.

bhfunc:goaf-drainage
    a skos:Concept ;
    skos:historyNote "Compiled by the Geological Survey of Queensland" ;
    rdfs:isDefinedBy cs: ;
    skos:broader bhfunc:gas-management ;
    skos:definition "A well or bore drilled to remove fluids and or dangerous gases from the goaf."@en ;
    skos:inScheme cs: ;
    skos:prefLabel "goaf drainage"@en ;
.

bhfunc:intrusion-delineation
    a skos:Concept ;
    skos:historyNote "Compiled by the Geological Survey of Queensland" ;
    rdfs:isDefinedBy cs: ;
    skos:broader bhfunc:structure ;
    skos:definition "Borehole drilled to define an intrusion."@en ;
    skos:inScheme cs: ;
    skos:prefLabel "intrusion delineation"@en ;
.

bhfunc:large-diameter
    a skos:Concept ;
    skos:historyNote "Compiled by the Geological Survey of Queensland" ;
    rdfs:isDefinedBy cs: ;
    skos:broader bhfunc:coal-quality ;
    skos:definition "Large diameter tests for coal physical properties and washability"@en ;
    skos:inScheme cs: ;
    skos:prefLabel "large diameter"@en ;
.

bhfunc:limit-of-oxidation
    a skos:Concept ;
    skos:historyNote "Compiled by the Geological Survey of Queensland" ;
    rdfs:isDefinedBy cs: ;
    skos:broader bhfunc:resource-assessment ;
    skos:definition "Borehole drilled to obtain samples to determine the amount of oxidation of any coal seam by either visual and tactile or coal analysis methods."@en ;
    skos:inScheme cs: ;
    skos:notation "LOX" ;
    skos:prefLabel "Limit of Oxidation"@en ;
.

bhfunc:mineral-ore-body-assessment
    a skos:Concept ;
    skos:historyNote "Compiled by the Geological Survey of Queensland" ;
    rdfs:isDefinedBy cs: ;
    skos:broader bhfunc:resource-assessment ;
    skos:definition "A well drilled to delineate a mineral ore deposit and/or define physical properties such as grade and quality"@en ;
    skos:inScheme cs: ;
    skos:prefLabel "Mineral Ore Body Assessment"@en ;
.

bhfunc:multi-channel-vibrating-wire-piezometer
    a skos:Concept ;
    skos:historyNote "Compiled by the Geological Survey of Queensland" ;
    rdfs:isDefinedBy cs: ;
    skos:broader bhfunc:observation ;
    skos:definition "A well or bore drilled to provide a location in which Multi-Channel Vibrating Wire Piezometer can be used to register changes in fluid pressure."@en ;
    skos:inScheme cs: ;
    skos:prefLabel "multi-channel vibrating wire piezometer"@en ;
.

bhfunc:nested-standpipe-piezometer
    a skos:Concept ;
    skos:historyNote "Compiled by the Geological Survey of Queensland" ;
    rdfs:isDefinedBy cs: ;
    skos:broader bhfunc:observation ;
    skos:definition "A well or bore drilled to provide a location in which Nested Standpipe Piezometer can be used to register changes in fluid pressure."@en ;
    skos:inScheme cs: ;
    skos:prefLabel "nested standpipe piezometer"@en ;
.

bhfunc:nitrogen
    a skos:Concept ;
    skos:historyNote "Compiled by the Geological Survey of Queensland" ;
    rdfs:isDefinedBy cs: ;
    skos:broader bhfunc:service ;
    skos:definition "A well or bore through which nitrogen is transported to and from mine workings."@en ;
    skos:inScheme cs: ;
    skos:prefLabel "nitrogen"@en ;
.

bhfunc:penetrometer
    a skos:Concept ;
    skos:historyNote "Compiled by the Geological Survey of Queensland" ;
    rdfs:isDefinedBy cs: ;
    skos:broader bhfunc:geotech ;
    skos:definition "A well or bore drilled to facilitate strength measurements through the use of a penetrometer."@en ;
    skos:inScheme cs: ;
    skos:prefLabel "penetrometer"@en ;
.

bhfunc:pggd-functions
    a skos:Collection ;
    skos:historyNote "Compiled by the Geological Survey of Queensland" ;
    skos:definition "The functions of boreholes specific to petroleum, greenhouse gas, and geothermal wells and bores i.e. those that require a statutory notification in Queensland regulation."@en ;
    skos:member
        bhfunc:disposal ,
        bhfunc:heat-flow ,
        bhfunc:observation ,
        bhfunc:petroleum-injection ,
        bhfunc:petroleum-prod-test ,
        bhfunc:petroleum-production ,
        bhfunc:petroleum-reservoir-characterisation ,
        bhfunc:stimulation ,
        bhfunc:stratigraphic ,
        bhfunc:water-injection ,
        bhfunc:water-supply ;
    skos:prefLabel "Petroleum Borehole Functions"@en ;
.

bhfunc:plug
    a skos:Concept ;
    skos:historyNote "Compiled by the Geological Survey of Queensland" ;
    rdfs:isDefinedBy cs: ;
    skos:broader bhfunc:service ;
    skos:definition "Plug hole"@en ;
    skos:inScheme cs: ;
    skos:prefLabel "plug"@en ;
.

bhfunc:primary-hydraulic-fracturing
    a skos:Concept ;
    skos:historyNote "Compiled by the Geological Survey of Queensland" ;
    rdfs:isDefinedBy cs: ;
    skos:broader bhfunc:geotech ;
    skos:definition "A well or bore drilled to facilitate the introduction of a liquid solution to a system, under significant pressure, to introduce fractures into strata."@en ;
    skos:inScheme cs: ;
    skos:prefLabel "primary hydraulic fracturing"@en ;
.

bhfunc:ranging-well
    a skos:Concept ;
    skos:historyNote "Compiled by the Geological Survey of Queensland" ;
    rdfs:isDefinedBy cs: ;
    skos:broader bhfunc:gas-management ;
    skos:definition "A well drilled to intersect with another well."@en ;
    skos:inScheme cs: ;
    skos:prefLabel "ranging well"@en ;
.

bhfunc:refuge
    a skos:Concept ;
    skos:historyNote "Compiled by the Geological Survey of Queensland" ;
    rdfs:isDefinedBy cs: ;
    skos:broader bhfunc:service ;
    skos:definition "A well or bore which provides access to, for ventilation or rescue, a refuge."@en ;
    skos:inScheme cs: ;
    skos:prefLabel "refuge"@en ;
.

bhfunc:slim-core-testing
    a skos:Concept ;
    skos:historyNote "Compiled by the Geological Survey of Queensland" ;
    rdfs:isDefinedBy cs: ;
    skos:broader bhfunc:coal-quality ;
    skos:definition "Slim core testing for basic coal quality"@en ;
    skos:inScheme cs: ;
    skos:prefLabel "slim core testing"@en ;
.

bhfunc:spontaneous-combustion-testing
    a skos:Concept ;
    skos:historyNote "Compiled by the Geological Survey of Queensland" ;
    rdfs:isDefinedBy cs: ;
    skos:broader bhfunc:coal-quality ;
    skos:definition "Borehole Drilled to obtains samples for spontaneous combustion testing"@en ;
    skos:inScheme cs: ;
    skos:prefLabel "spontaneous combustion testing"@en ;
.

bhfunc:standpipe-piezometer
    a skos:Concept ;
    skos:historyNote "Compiled by the Geological Survey of Queensland" ;
    rdfs:isDefinedBy cs: ;
    skos:broader bhfunc:observation ;
    skos:definition "A well or bore drilled to provide a location in which Standpipe Piezometer can be used to register changes in fluid pressure."@en ;
    skos:inScheme cs: ;
    skos:prefLabel "standpipe piezometer"@en ;
.

bhfunc:steam-flood
    a skos:Concept ;
    skos:historyNote "Compiled by the Geological Survey of Queensland" ;
    rdfs:isDefinedBy cs: ;
    skos:altLabel
        "CSS"@en ,
        "Cyclic Steam Stimulation"@en ,
        "SAGD"@en ,
        "Steam Assisted Gravity Drainage"@en ;
    skos:broader bhfunc:stimulation ;
    skos:definition "The injection of steam into a petroleum system to improve recovery through the reduction of viscosity, displacement and more beneficial pressure gradients."@en ;
    skos:inScheme cs: ;
    skos:prefLabel "Steam Flood"@en ;
.

bhfunc:stone-dust
    a skos:Concept ;
    skos:historyNote "Compiled by the Geological Survey of Queensland" ;
    rdfs:isDefinedBy cs: ;
    skos:broader bhfunc:service ;
    skos:definition "A well or bore through which stone dust is transported to and from mine workings."@en ;
    skos:inScheme cs: ;
    skos:prefLabel "stone dust"@en ;
.

bhfunc:stress-test-cell-over-stress-overcore
    a skos:Concept ;
    skos:historyNote "Compiled by the Geological Survey of Queensland" ;
    rdfs:isDefinedBy cs: ;
    skos:broader bhfunc:geotech ;
    skos:definition "A well or bore drilled to facilitate the installation and subsequent retrieval of (Through overcoring) a stress cell."@en ;
    skos:inScheme cs: ;
    skos:prefLabel "stress test cell / stress overcore"@en ;
.

bhfunc:stygofauna-monitoring
    a skos:Concept ;
    skos:historyNote "Compiled by the Geological Survey of Queensland" ;
    rdfs:isDefinedBy cs: ;
    skos:broader bhfunc:environmental ;
    skos:definition "A well or bore drilled to facilitate the monitoring of the population, biodiversity and overall 'health' parameters of stygofauna."@en ;
    skos:inScheme cs: ;
    skos:prefLabel "stygofauna monitoring"@en ;
.

bhfunc:surface-to-in-seam-well
    a skos:Concept ;
    skos:historyNote "Compiled by the Geological Survey of Queensland" ;
    rdfs:isDefinedBy cs: ;
    skos:broader bhfunc:petroleum-production ;
    skos:definition "A well drilled to laterally intersect and drain hydrocarbons from a subsurface system."@en ;
    skos:inScheme cs: ;
    skos:prefLabel "surface to in-seam well"@en ;
.

bhfunc:tiltmeter
    a skos:Concept ;
    skos:historyNote "Compiled by the Geological Survey of Queensland" ;
    rdfs:isDefinedBy cs: ;
    skos:broader bhfunc:geotech ;
    skos:definition "A well or bore drilled to facilitate the installation of a tiltmeter."@en ;
    skos:inScheme cs: ;
    skos:prefLabel "tiltmeter"@en ;
.

bhfunc:underground-in-seam-gas-riser
    a skos:Concept ;
    skos:historyNote "Compiled by the Geological Survey of Queensland" ;
    rdfs:isDefinedBy cs: ;
    skos:broader bhfunc:gas-management ;
    skos:definition "A well drilled to improve the transport of gas away from a coal seam."@en ;
    skos:inScheme cs: ;
    skos:prefLabel "underground in-seam gas-riser"@en ;
.

bhfunc:vertical-production-well
    a skos:Concept ;
    skos:historyNote "Compiled by the Geological Survey of Queensland" ;
    rdfs:isDefinedBy cs: ;
    skos:broader bhfunc:petroleum-production ;
    skos:definition "A vertical well drilled to drain hydrocarbons from a subsurface system."@en ;
    skos:inScheme cs: ;
    skos:prefLabel "vertical production well"@en ;
.

bhfunc:vibrating-wire-piezometer
    a skos:Concept ;
    skos:historyNote "Compiled by the Geological Survey of Queensland" ;
    rdfs:isDefinedBy cs: ;
    skos:broader bhfunc:observation ;
    skos:definition "A well or bore drilled to provide a location in which Vibrating Wire Piezometer can be used to register changes in fluid pressure."@en ;
    skos:inScheme cs: ;
    skos:prefLabel "vibrating wire piezometer"@en ;
.

bhfunc:virgin-gas-testing
    a skos:Concept ;
    skos:historyNote "Compiled by the Geological Survey of Queensland" ;
    rdfs:isDefinedBy cs: ;
    skos:broader bhfunc:gas-management ;
    skos:definition "Gas content testing in areas not subject to gas drainage."@en ;
    skos:inScheme cs: ;
    skos:prefLabel "virgin gas testing"@en ;
.

bhfunc:water-flood
    a skos:Concept ;
    skos:historyNote "Compiled by the Geological Survey of Queensland" ;
    rdfs:isDefinedBy cs: ;
    skos:broader bhfunc:stimulation ;
    skos:definition "The introduction of liquid water to a petroleum system to improve recovery through displacement and more beneficial pressure gradients."@en ;
    skos:inScheme cs: ;
    skos:prefLabel "Water Flood"@en ;
.

bhfunc:blasthole
    a skos:Concept ;
    skos:historyNote "Compiled by the Geological Survey of Queensland" ;
    rdfs:isDefinedBy cs: ;
    skos:definition "A well or bore drilled to facilitate the installation and subsequent detonation of explosives, pulverising material and throwing it away from the wall or face, reducing the effort required to advance the face or recover and remove materials."@en ;
    skos:inScheme cs: ;
    skos:prefLabel "Blasthole"@en ;
    skos:topConceptOf cs: ;
.

bhfunc:heat-flow
    a skos:Concept ;
    skos:historyNote "Compiled by the Geological Survey of Queensland" ;
    rdfs:isDefinedBy cs: ;
    skos:altLabel "Heat flow"@en ;
    skos:broader bhfunc:resource-assessment ;
    skos:definition "purposely drilled to directly measure downhole temperature gradient as well as collecting core samples (to measure thermal conductivity of formations intersected), then to be able to calculate / determine heat flow in the drilled section of the borehole."@en ;
    skos:inScheme cs: ;
    skos:prefLabel "Geothermal heat flow"@en ;
.

bhfunc:investigation
    a skos:Concept ;
    skos:historyNote "Compiled by the Geological Survey of Queensland" ;
    rdfs:isDefinedBy cs: ;
    skos:definition "A well drilled with scant or nil prior knowledge of the geology of an area to identify the presence of any lithologic, structural, hydrological, geochemical, or other geologic properties of interest."@en ;
    skos:inScheme cs: ;
    skos:prefLabel "Investigation"@en ;
    skos:topConceptOf cs: ;
.

bhfunc:petroleum-prod-test
    a skos:Concept ;
    skos:historyNote "Compiled by the Geological Survey of Queensland" ;
    rdfs:isDefinedBy cs: ;
    skos:broader bhfunc:resource-assessment ;
    skos:definition "A well drilled primarily to test the ability of a target reservoir to  produce hydrocarbons, and to measure production parameters such as flow rates, well interference, pressure decline etc."@en ;
    skos:inScheme cs: ;
    skos:prefLabel "Petroleum Production Testing"@en ;
.

bhfunc:petroleum-reservoir-characterisation
    a skos:Concept ;
    skos:historyNote "Compiled by the Geological Survey of Queensland" ;
    rdfs:isDefinedBy cs: ;
    skos:broader bhfunc:resource-assessment ;
    skos:definition "A well drilled to determine how to develop a hydrocarbon field most efficiently or quantify reservoir characteristics such as pay zone thickness, porosity, permeability, saturation, fluid column heights, and the presence of cap rock. Most commonly associated with the Appraisal stage of the resource lifecycle."@en ;
    skos:inScheme cs: ;
    skos:prefLabel "Petroleum Resource Characterisation"@en ;
.

bhfunc:disposal
    a skos:Concept ;
    skos:historyNote "Compiled by the Geological Survey of Queensland" ;
    rdfs:isDefinedBy cs: ;
    skos:definition "A well in which fluids are injected rather than produced, where the primary objective is to dispose of fluid into an isolated formation."@en ;
    skos:inScheme cs: ;
    skos:prefLabel "Disposal"@en ;
    skos:topConceptOf cs: ;
.

bhfunc:petroleum-injection
    a skos:Concept ;
    skos:historyNote "Compiled by the Geological Survey of Queensland" ;
    rdfs:isDefinedBy cs: ;
    skos:altLabel "Petroleum Storage"@en ;
    skos:definition "A well in which hydrocarbons are injected rather than produced, the primary objective typically to store gas in a high quality reservoir for later production to maintain consistent rates of gas supply."@en ;
    skos:inScheme cs: ;
    skos:prefLabel "Petroleum Injection"@en ;
    skos:topConceptOf cs: ;
.

bhfunc:stratigraphic
    a skos:Concept ;
    skos:historyNote "Compiled by the Geological Survey of Queensland" ;
    rdfs:isDefinedBy cs: ;
    skos:definition "A well determining the lithological intervals present at a location. Typically to determine on the presence, location and extent of a potential resource. Most commonly associated with the Exploration stage of the resource lifecycle."@en ;
    skos:inScheme cs: ;
    skos:notation "STRAT" ;
    skos:prefLabel "Stratigraphic"@en ;
    skos:topConceptOf cs: ;
.

bhfunc:water-injection
    a skos:Concept ;
    skos:historyNote "Compiled by the Geological Survey of Queensland" ;
    rdfs:isDefinedBy cs: ;
    skos:altLabel "Water Storage"@en ;
    skos:definition "A well in which water is injected rather than produced, where the primary objective is to store water in a reservoir or aquifer for later production."@en ;
    skos:inScheme cs: ;
    skos:prefLabel "Water Injection"@en ;
    skos:topConceptOf cs: ;
.

bhfunc:water-supply
    a skos:Concept ;
    skos:historyNote "Compiled by the Geological Survey of Queensland" ;
    rdfs:isDefinedBy cs: ;
    skos:altLabel
        "Production Water Bore"@en ,
        "Water Production"@en ;
    skos:definition "A well drilled to drain water from an aquifer."@en ;
    skos:inScheme cs: ;
    skos:prefLabel "Water Supply"@en ;
    skos:topConceptOf cs: ;
.

<https://linked.data.gov.au/org/gsq>
    a sdo:Organization ;
    sdo:name "Geological Survey of Queensland" ;
    sdo:url "http://www.business.qld.gov.au/industries/mining-energy-water/resources/geoscience-information/gsq"^^xsd:anyURI ;
.

bhfunc:coal-quality
    a skos:Concept ;
    skos:historyNote "Compiled by the Geological Survey of Queensland" ;
    rdfs:isDefinedBy cs: ;
    skos:broader bhfunc:resource-assessment ;
    skos:definition "Borehole drilled to obtain samples for laboratory testing and coal analysis."@en ;
    skos:inScheme cs: ;
    skos:prefLabel "Coal Quality"@en ;
.

bhfunc:environmental
    a skos:Concept ;
    skos:historyNote "Compiled by the Geological Survey of Queensland" ;
    rdfs:isDefinedBy cs: ;
    skos:definition "Borehole drilled to obtain samples of strata for laboratory analysis of parameters which may impact on the environment."@en ;
    skos:inScheme cs: ;
    skos:prefLabel "Environmental"@en ;
    skos:topConceptOf cs: ;
.

bhfunc:structure
    a skos:Concept ;
    skos:historyNote "Compiled by the Geological Survey of Queensland" ;
    rdfs:isDefinedBy cs: ;
    skos:definition "Borehole drilled to investigate the attitude of strata and the impact of any tectonic features."@en ;
    skos:inScheme cs: ;
    skos:prefLabel "Structure"@en ;
    skos:topConceptOf cs: ;
.

bhfunc:petroleum-production
    a skos:Concept ;
    skos:historyNote "Compiled by the Geological Survey of Queensland" ;
    rdfs:isDefinedBy cs: ;
    skos:definition "A well drilled to drain hydrocarbons from an oil or gas field, including during the degasification of a coal seam."@en ;
    skos:inScheme cs: ;
    skos:prefLabel "Petroleum Production"@en ;
    skos:topConceptOf cs: ;
.

bhfunc:observation
    a skos:Concept ;
    skos:historyNote "Compiled by the Geological Survey of Queensland" ;
    rdfs:isDefinedBy cs: ;
    skos:definition "Borehole drilled to investigate water level or for piezometer installation."@en ;
    skos:inScheme cs: ;
    skos:prefLabel "Observation"@en ;
    skos:topConceptOf cs: ;
.

bhfunc:geotech
    a skos:Concept ;
    skos:historyNote "Compiled by the Geological Survey of Queensland" ;
    rdfs:isDefinedBy cs: ;
    skos:definition "A borehole drilled to investigate the geotechnical properties of the strata and provide samples for mechanical testing."@en ;
    skos:inScheme cs: ;
    skos:prefLabel "Geotech"@en ;
    skos:topConceptOf cs: ;
.

bhfunc:resource-assessment
    a skos:Concept ;
    skos:historyNote "Compiled by the Geological Survey of Queensland" ;
    rdfs:isDefinedBy cs: ;
    skos:definition "A well determining the geological properties of a resource specific to the type of commodity. This may include quantification of volume, grade, porosity, permeability, quality, or ease-of-extraction."@en ;
    skos:inScheme cs: ;
    skos:prefLabel "Resource Assessment"@en ;
    skos:topConceptOf cs: ;
.

bhfunc:stimulation
    a skos:Concept ;
    skos:historyNote "Compiled by the Geological Survey of Queensland" ;
    rdfs:isDefinedBy cs: ;
    skos:definition "A well drilled to enhance the production of a fluid from an offset production well. Typically to maintain reservoir pressure, to overcome to low permeability or high viscosity fluids in petroleum systems, or to introduce additional fluid in geothermal systems."@en ;
    skos:inScheme cs: ;
    skos:prefLabel "Stimulation"@en ;
    skos:topConceptOf cs: ;
.

bhfunc:service
    a skos:Concept ;
    skos:historyNote "Compiled by the Geological Survey of Queensland" ;
    rdfs:isDefinedBy cs: ;
    skos:definition "Borehole drilled to provide a conduit or access to and from mine workings for equipment or materials."@en ;
    skos:inScheme cs: ;
    skos:prefLabel "Service"@en ;
    skos:topConceptOf cs: ;
.

bhfunc:gas-management
    a skos:Concept ;
    skos:historyNote "Compiled by the Geological Survey of Queensland" ;
    rdfs:isDefinedBy cs: ;
    skos:definition "Borehole drilled for gas analysis and management. Typical applications include exploration, management of gas in coal mines, compliance and greenhouse gas emissions."@en ;
    skos:inScheme cs: ;
    skos:prefLabel "Gas Management"@en ;
    skos:topConceptOf cs: ;
.

cs:
    a
        owl:Ontology ,
        skos:ConceptScheme ;
    dcterms:created "2020-01-23"^^xsd:date ;
    dcterms:creator <https://linked.data.gov.au/org/gsq> ;
    dcterms:modified "2023-03-16"^^xsd:date ;
    skos:historyNote "Compiled by the Geological Survey of Queensland" ;
    dcterms:publisher <https://linked.data.gov.au/org/gsq> ;
    reg:status agldwgstatus:stable ;
    skos:definition "The intended function of a borehole."@en ;
    skos:hasTopConcept
        bhfunc:blasthole ,
        bhfunc:disposal ,
        bhfunc:environmental ,
        bhfunc:gas-management ,
        bhfunc:geotech ,
        bhfunc:investigation ,
        bhfunc:observation ,
        bhfunc:petroleum-injection ,
        bhfunc:petroleum-production ,
        bhfunc:resource-assessment ,
        bhfunc:service ,
        bhfunc:stimulation ,
        bhfunc:stratigraphic ,
        bhfunc:structure ,
        bhfunc:water-injection ,
        bhfunc:water-supply ;
    skos:prefLabel "Borehole Sub-Purpose"@en ;
.

