PREFIX agldwgstatus: <https://linked.data.gov.au/def/reg-statuses/>
PREFIX cs: <http://linked.data.gov.au/def/depth-reference>
PREFIX dcterms: <http://purl.org/dc/terms/>
PREFIX drd: <http://linked.data.gov.au/def/depth-reference/>
PREFIX owl: <http://www.w3.org/2002/07/owl#>
PREFIX rdfs: <http://www.w3.org/2000/01/rdf-schema#>
PREFIX reg: <http://purl.org/linked-data/registry#>
PREFIX sdo: <https://schema.org/>
PREFIX skos: <http://www.w3.org/2004/02/skos/core#>
PREFIX xsd: <http://www.w3.org/2001/XMLSchema#>

drd:absolute
    a skos:Collection ;
    dcterms:provenance "Defined here" ;
    skos:definition "A fixed plane or point that describes an absolute reference for depth observations."@en ;
    skos:member
        drd:australian-height-datum ,
        drd:mean-sea-level ,
        drd:metres-sub-sea ;
    skos:prefLabel "Absolute"@en ;
.

drd:borehole
    a skos:Collection ;
    dcterms:provenance "Defined here" ;
    skos:definition "A point to which measurements are referenced to in a borehole."@en ;
    skos:member
        drd:drill-collar ,
        drd:ground-level ,
        drd:kelly-bushing ,
        drd:rotary-table ,
        drd:water-bottom ,
        drd:well-head ;
    skos:prefLabel "Borehole"@en ;
.

drd:seismic
    a skos:Collection ;
    dcterms:provenance "Defined here" ;
    skos:definition "A reference relating to time based measurements and datasets, such as seismic surveys. Reported in a unit of measure of time."@en ;
    skos:member drd:seismic-reference-datum ;
    skos:prefLabel "Seismic"@en ;
.

drd:site
    a skos:Collection ;
    dcterms:provenance "Defined here" ;
    skos:definition "A generic reference point for sites, samples, observations, or surveys."@en ;
    skos:member
        drd:ground-level ,
        drd:water-bottom ;
    skos:prefLabel "Site"@en ;
.

drd:australian-height-datum
    a skos:Concept ;
    dcterms:provenance "Compiled by the Geological Survey of Queensland" ;
    rdfs:isDefinedBy cs: ;
    skos:definition "The Australian Height Datum is a vertical datum in Australia.In 1971 the mean sea level for 1966-1968 was assigned the value of 0.000m on the Australian Height Datum at thirty tide gauges around the coast of the Australian continent."@en ;
    skos:inScheme cs: ;
    skos:notation "AHD" ;
    skos:prefLabel "Australian Height Datum"@en ;
    skos:topConceptOf cs: ;
.

drd:drill-collar
    a skos:Concept ;
    dcterms:provenance "Compiled by the Geological Survey of Queensland" ;
    rdfs:isDefinedBy cs: ;
    skos:definition "A component of a drillstring that provides weight on bit for drilling. Drill collars are thick-walled tubular pieces machined from solid bars of steel or alloy. Source: Schlumberger Oilfield Glossary"@en ;
    skos:inScheme cs: ;
    skos:notation "DC" ;
    skos:prefLabel "Drill Collar"@en ;
    skos:topConceptOf cs: ;
.

drd:kelly-bushing
    a skos:Concept ;
    dcterms:provenance "Compiled by the Geological Survey of Queensland" ;
    rdfs:isDefinedBy cs: ;
    skos:altLabel "Kelly Bushing (KB)"@en ;
    skos:definition "An adapter that serves to connect the rotary table to the kelly (A long square or hexagonal steel bar with a hole drilled through the middle for a fluid path).Source: Schlumberger Oilfield Glossary"@en ;
    skos:inScheme cs: ;
    skos:notation "KB" ;
    skos:prefLabel "Kelly Bushing"@en ;
    skos:topConceptOf cs: ;
.

drd:mean-sea-level
    a skos:Concept ;
    dcterms:provenance "Compiled by the Geological Survey of Queensland" ;
    rdfs:isDefinedBy cs: ;
    skos:definition "The elevation (on the ground) or altitude (in the air) of an object, relative to the average sea level."@en ;
    skos:inScheme cs: ;
    skos:notation "MSL" ;
    skos:prefLabel "Mean Sea Level"@en ;
    skos:topConceptOf cs: ;
.

drd:metres-sub-sea
    a skos:Concept ;
    dcterms:provenance "Compiled by the Geological Survey of Queensland" ;
    rdfs:isDefinedBy cs: ;
    skos:definition "The distance below mean sea level, the inverse of measurements to Mean Sea Level."@en ;
    skos:inScheme cs: ;
    skos:notation "MSS" ;
    skos:prefLabel "Metres Sub-Sea"@en ;
    skos:topConceptOf cs: ;
.

drd:rotary-table
    a skos:Concept ;
    dcterms:provenance "Compiled by the Geological Survey of Queensland" ;
    rdfs:isDefinedBy cs: ;
    skos:altLabel "Rotary Table (RT)"@en ;
    skos:definition "The revolving or spinning section of the drillfloor that provides power to turn the drillstring in a clockwise direction (as viewed from above).Source: Schlumberger Oilfield Glossary"@en ;
    skos:inScheme cs: ;
    skos:notation "RT" ;
    skos:prefLabel "Rotary Table"@en ;
    skos:topConceptOf cs: ;
.

drd:seismic-reference-datum
    a skos:Concept ;
    dcterms:provenance "Compiled by the Geological Survey of Queensland" ;
    rdfs:isDefinedBy cs: ;
    skos:definition "The SRD is a plane that sits above the highest elevation in the data. In a land project with a seismic reference datum set, the SRD will have a time of 0 ms. All time data, e.g. seismic and velocities, will start at this datum."@en ;
    skos:inScheme cs: ;
    skos:notation "SRD" ;
    skos:prefLabel "Seismic Reference Datum"@en ;
    skos:topConceptOf cs: ;
.

drd:well-head
    a skos:Concept ;
    dcterms:provenance "Compiled by the Geological Survey of Queensland" ;
    rdfs:isDefinedBy cs: ;
    skos:altLabel
        "Well head (WH)"@en ,
        "Wellhead"@en ;
    skos:definition "A wellhead is the component at the surface of an oil or gas well that provides the structural and pressure-containing interface for the drilling and production equipment. Iolation valves and choke equipment control the flow of well fluids during production. Elevation is typically equivalent to the valve or outlet point from which samples are extracted."@en ;
    skos:inScheme cs: ;
    skos:notation "WH" ;
    skos:prefLabel "Well Head"@en ;
    skos:topConceptOf cs: ;
.

<https://linked.data.gov.au/org/gsq>
    a sdo:Organization ;
    sdo:name "Geological Survey of Queensland" ;
    sdo:url "http://www.business.qld.gov.au/industries/mining-energy-water/resources/geoscience-information/gsq"^^xsd:anyURI ;
.

drd:ground-level
    a skos:Concept ;
    dcterms:provenance "Compiled by the Geological Survey of Queensland" ;
    rdfs:isDefinedBy cs: ;
    skos:altLabel "Ground Level (GL)"@en ;
    skos:definition "Ground level elevation without additional equipment"@en ;
    skos:inScheme cs: ;
    skos:notation "GL" ;
    skos:prefLabel "Ground Level"@en ;
    skos:topConceptOf cs: ;
.

drd:water-bottom
    a skos:Concept ;
    dcterms:provenance "Compiled by the Geological Survey of Queensland" ;
    rdfs:isDefinedBy cs: ;
    skos:definition "The depth of the interface between water and solid substrate, such as the sea bed or the bottom of a terrestrial body of water."@en ;
    skos:inScheme cs: ;
    skos:notation "WB" ;
    skos:prefLabel "Water Bottom"@en ;
    skos:topConceptOf cs: ;
.

cs:
    a
        owl:Ontology ,
        skos:ConceptScheme ;
    dcterms:created "2020-01-21T11:03:47"^^xsd:dateTime ;
    dcterms:creator <https://linked.data.gov.au/org/gsq> ;
    dcterms:modified "2023-03-16"^^xsd:date ;
    dcterms:provenance "Compiled by the Geological Survey of Queensland" ;
    dcterms:publisher <https://linked.data.gov.au/org/gsq> ;
    reg:status agldwgstatus:stable ;
    skos:definition "The point or level from which all depths are measured and referenced to for an entity or activity. Typically relative to a common global or regional reference datum such as the Australian Height Datum (AHD)."@en ;
    skos:hasTopConcept
        drd:australian-height-datum ,
        drd:drill-collar ,
        drd:ground-level ,
        drd:kelly-bushing ,
        drd:mean-sea-level ,
        drd:metres-sub-sea ,
        drd:rotary-table ,
        drd:seismic-reference-datum ,
        drd:water-bottom ,
        drd:well-head ;
    skos:prefLabel "Depth Reference"@en ;
.

