PREFIX agldwgstatus: <https://linked.data.gov.au/def/reg-statuses/>
PREFIX cs: <http://linked.data.gov.au/def/geo-product-form>
PREFIX dcterms: <http://purl.org/dc/terms/>
PREFIX gcpf: <http://linked.data.gov.au/def/geo-product-form/>
PREFIX owl: <http://www.w3.org/2002/07/owl#>
PREFIX rdfs: <http://www.w3.org/2000/01/rdf-schema#>
PREFIX reg: <http://purl.org/linked-data/registry#>
PREFIX sdo: <https://schema.org/>
PREFIX skos: <http://www.w3.org/2004/02/skos/core#>
PREFIX xsd: <http://www.w3.org/2001/XMLSchema#>

gcpf:carbonate-ore
    a skos:Concept ;
    dcterms:provenance "Derived by the Geological Survey of Queensland to describe the forms in which geo-commodities are produced and sold by miners, fossickers, and extractive industries." ;
    rdfs:isDefinedBy cs: ;
    skos:altLabel "Carbonate Ore"@en ;
    skos:broader gcpf:ore ;
    skos:definition "A mixture of ore minerals and gangue from which at least one of the metals can be extracted at a profit where the primary economic mineral is a carbonate."@en ;
    skos:inScheme cs: ;
    skos:prefLabel "Ore (Carbonate)"@en ;
.

gcpf:sulphide-ore
    a skos:Concept ;
    dcterms:provenance "Derived by the Geological Survey of Queensland to describe the forms in which geo-commodities are produced and sold by miners, fossickers, and extractive industries." ;
    rdfs:isDefinedBy cs: ;
    skos:altLabel
        "Ore (Sulfide)"@en ,
        "Sulfide Ore"@en ,
        "Sulphide Ore"@en ;
    skos:broader gcpf:ore ;
    skos:definition "A mixture of ore minerals and gangue from which at least one of the metals can be extracted at a profit where the primary economic mineral is a carbonate."@en ;
    skos:inScheme cs: ;
    skos:prefLabel "Ore (Sulphide)"@en ;
.

gcpf:alluvial
    a skos:Concept ;
    dcterms:provenance "Derived by the Geological Survey of Queensland to describe the forms in which geo-commodities are produced and sold by miners, fossickers, and extractive industries." ;
    rdfs:isDefinedBy cs: ;
    skos:definition "A metallic product consisting of the commodity in its natural alluvial state separated from its host material or as unconsolidated sediment hosting the target commodity."@en ;
    skos:inScheme cs: ;
    skos:prefLabel "Alluvial Metal"@en ;
    skos:topConceptOf cs: ;
.

gcpf:bulk-metal
    a skos:Concept ;
    dcterms:provenance "Derived by the Geological Survey of Queensland to describe the forms in which geo-commodities are produced and sold by miners, fossickers, and extractive industries." ;
    rdfs:isDefinedBy cs: ;
    skos:definition "A product of processed and refined or undifferentiated metal(s)."@en ;
    skos:inScheme cs: ;
    skos:prefLabel "Bulk Metal"@en ;
    skos:topConceptOf cs: ;
.

gcpf:bullion
    a skos:Concept ;
    dcterms:provenance "Derived by the Geological Survey of Queensland to describe the forms in which geo-commodities are produced and sold by miners, fossickers, and extractive industries." ;
    rdfs:isDefinedBy cs: ;
    skos:definition "Metal formed into bars or ingots. Typically of high purity. source: https://www.sec.gov/"@en ;
    skos:inScheme cs: ;
    skos:prefLabel "Bullion"@en ;
    skos:topConceptOf cs: ;
.

gcpf:cathode
    a skos:Concept ;
    dcterms:provenance "Derived by the Geological Survey of Queensland to describe the forms in which geo-commodities are produced and sold by miners, fossickers, and extractive industries." ;
    rdfs:isDefinedBy cs: ;
    skos:definition "A metal plate, produced by electrolytic refining, which is melted into commercial shapes such as wirebars, billets, ingots, etc. source:https://www.sec.gov/"@en ;
    skos:inScheme cs: ;
    skos:prefLabel "Cathode"@en ;
    skos:topConceptOf cs: ;
.

gcpf:clay
    a skos:Concept ;
    dcterms:provenance "Derived by the Geological Survey of Queensland to describe the forms in which geo-commodities are produced and sold by miners, fossickers, and extractive industries." ;
    rdfs:isDefinedBy cs: ;
    skos:definition "A broad category of clay-grade clastic-sediments, used as a commodity for thier physical or chemical properties."@en ;
    skos:inScheme cs: ;
    skos:prefLabel "Clay"@en ;
    skos:topConceptOf cs: ;
.

gcpf:concentrate
    a skos:Concept ;
    dcterms:provenance "Derived by the Geological Survey of Queensland to describe the forms in which geo-commodities are produced and sold by miners, fossickers, and extractive industries." ;
    rdfs:isDefinedBy cs: ;
    skos:definition "Metal concentrates are produced by the beneficiation, or upgrading, of ore. For example a typical copper ore would be 0.7% to 2% copper, a typical copper concentrate would grade around 25% to 35% copper."@en ;
    skos:inScheme cs: ;
    skos:prefLabel "Metal Concentrate"@en ;
    skos:topConceptOf cs: ;
.

gcpf:construction
    a skos:Concept ;
    dcterms:provenance "Derived by the Geological Survey of Queensland to describe the forms in which geo-commodities are produced and sold by miners, fossickers, and extractive industries." ;
    rdfs:isDefinedBy cs: ;
    skos:definition "A broad category of particulate products used as materials for construction, landscaping, infrastructure. Excludes cut and fabricated dimension stone."@en ;
    skos:inScheme cs: ;
    skos:prefLabel "Construction and Extractive"@en ;
    skos:topConceptOf cs: ;
.

gcpf:dimension-stone
    a skos:Concept ;
    dcterms:provenance "Derived by the Geological Survey of Queensland to describe the forms in which geo-commodities are produced and sold by miners, fossickers, and extractive industries." ;
    rdfs:isDefinedBy cs: ;
    skos:definition "Dimension stone is natural stone or rock that has been selected and fabricated (i.e., trimmed, cut, drilled, ground, or other) to specific sizes or shapes."@en ;
    skos:inScheme cs: ;
    skos:prefLabel "Dimension Stone"@en ;
    skos:topConceptOf cs: ;
.

gcpf:fuel
    a skos:Concept ;
    dcterms:provenance "Derived by the Geological Survey of Queensland to describe the forms in which geo-commodities are produced and sold by miners, fossickers, and extractive industries." ;
    rdfs:isDefinedBy cs: ;
    skos:definition "A mined or extracted combustible product that is used primarily as a source of thermal energy for heating, transport, or power generation; or as a reducing agent in the manufacture, refining, and metallurgy of saleable metals and alloys."@en ;
    skos:inScheme cs: ;
    skos:prefLabel "Coal"@en ;
    skos:topConceptOf cs: ;
.

gcpf:gemstone
    a skos:Concept ;
    dcterms:provenance "Derived by the Geological Survey of Queensland to describe the forms in which geo-commodities are produced and sold by miners, fossickers, and extractive industries." ;
    rdfs:isDefinedBy cs: ;
    skos:altLabel
        "Gem"@en ,
        "Jewel"@en ,
        "Precious Stone"@en ;
    skos:definition "A gemstone or gem (also called a precious or semi-precious stone, a fine gem, or jewel) is a piece of mineral, which, in cut and polished form, is used to make jewelry or other adornments"@en ;
    skos:inScheme cs: ;
    skos:prefLabel "Gemstone"@en ;
    skos:topConceptOf cs: ;
.

gcpf:non-metal
    a skos:Concept ;
    dcterms:provenance "Derived by the Geological Survey of Queensland to describe the forms in which geo-commodities are produced and sold by miners, fossickers, and extractive industries." ;
    rdfs:isDefinedBy cs: ;
    skos:definition "Minerals, metalloids, non-metals and rocks used in industrial, manufacturing, agricultural, horticultural or other processes for thier physical or chemical properties, rather than any specific metal content. Distinguished by usage from gemstones, constructive aggregates, and dimension stone. For example, this category includes industrial diamonds but not gemstone diamonds, and includes limestone as an industrial product for agriculture or as a reagent in cement making, but not as a dimension (building) stone or as limestone aggregate used as a construction material. This category includes silica sand for foundries, filters, glass-making, and ceramics, but not sand for use as a construction aggregate."@en ;
    skos:inScheme cs: ;
    skos:prefLabel "Mineral and Non-Metal"@en ;
    skos:topConceptOf cs: ;
.

gcpf:sulphate
    a skos:Concept ;
    dcterms:provenance "Derived by the Geological Survey of Queensland to describe the forms in which geo-commodities are produced and sold by miners, fossickers, and extractive industries." ;
    rdfs:isDefinedBy cs: ;
    skos:altLabel "Sulfate"@en ;
    skos:definition "A sulphate salt of a metallic commodity. Most commonly encountered as a form of copper."@en ;
    skos:inScheme cs: ;
    skos:prefLabel "Sulphate"@en ;
    skos:topConceptOf cs: ;
.

<https://linked.data.gov.au/org/gsq>
    a sdo:Organization ;
    sdo:name "Geological Survey of Queensland" ;
    sdo:url "https://www.business.qld.gov.au/industries/mining-energy-water/resources/geoscience-information/gsq"^^xsd:anyURI ;
.

gcpf:ore
    a skos:Concept ;
    dcterms:provenance "Derived by the Geological Survey of Queensland to describe the forms in which geo-commodities are produced and sold by miners, fossickers, and extractive industries." ;
    rdfs:isDefinedBy cs: ;
    skos:definition "A mixture of ore minerals and gangue from which at least one of the contained metals can be extracted at a profit."@en ;
    skos:inScheme cs: ;
    skos:prefLabel "Ore"@en ;
    skos:topConceptOf cs: ;
.

cs:
    a
        owl:Ontology ,
        skos:ConceptScheme ;
    dcterms:created "2021-07-29"^^xsd:date ;
    dcterms:creator <https://linked.data.gov.au/org/gsq> ;
    dcterms:modified "2023-03-16"^^xsd:date ;
    dcterms:provenance "Derived by the Geological Survey of Queensland to describe the forms in which geo-commodities are produced and sold by miners, fossickers, and extractive industries." ;
    dcterms:publisher <https://linked.data.gov.au/org/gsq> ;
    reg:status agldwgstatus:stable ;
    skos:definition "The forms of geo-commodities as produced and sold by miners, quarries, fossickers and other extractive operations. The form of a metallic commodity may imply levels and methods of processing and refinement from raw material such as ore, to partially refined concentrates, to highly processed and refined bullion."@en ;
    skos:hasTopConcept
        gcpf:alluvial ,
        gcpf:bulk-metal ,
        gcpf:bullion ,
        gcpf:cathode ,
        gcpf:clay ,
        gcpf:concentrate ,
        gcpf:construction ,
        gcpf:dimension-stone ,
        gcpf:fuel ,
        gcpf:gemstone ,
        gcpf:non-metal ,
        gcpf:ore ,
        gcpf:sulphate ;
    skos:prefLabel "Geoscience Commodity Product Forms"@en ;
.

