PREFIX agldwgstatus: <https://linked.data.gov.au/def/reg-statuses/>
PREFIX cs: <http://linked.data.gov.au/def/geoadminfeatures>
PREFIX dcterms: <http://purl.org/dc/terms/>
PREFIX geoad: <http://linked.data.gov.au/def/geoadminfeatures/>
PREFIX owl: <http://www.w3.org/2002/07/owl#>
PREFIX rdfs: <http://www.w3.org/2000/01/rdf-schema#>
PREFIX reg: <http://purl.org/linked-data/registry#>
PREFIX skos: <http://www.w3.org/2004/02/skos/core#>
PREFIX xsd: <http://www.w3.org/2001/XMLSchema#>

geoad:Abbieglassie8443
    a skos:Concept ;
    skos:historyNote "Compiled by the Geological Survey of Queensland" ;
    skos:broader geoad:MapSeries ;
    skos:definition "Map sheet for Abbieglassie at 1:100 000 scale. The first two digits define a longitude band 0.5 degree wide and the second two digits a latitude band 0.5 degree wide."@en ;
    skos:inScheme cs: ;
    skos:notation "8443" ;
    skos:prefLabel "Abbieglassie:8443"@en ;
.

geoad:AbbotPoint8558
    a skos:Concept ;
    skos:historyNote "Compiled by the Geological Survey of Queensland" ;
    skos:broader geoad:MapSeries ;
    skos:definition "Map sheet for Abbot Point at 1:100 000 scale. The first two digits define a longitude band 0.5 degree wide and the second two digits a latitude band 0.5 degree wide."@en ;
    skos:inScheme cs: ;
    skos:notation "8558" ;
    skos:prefLabel "Abbot Point:8558"@en ;
.

geoad:Aberfoyle7954
    a skos:Concept ;
    skos:historyNote "Compiled by the Geological Survey of Queensland" ;
    skos:broader geoad:MapSeries ;
    skos:definition "Map sheet for Aberfoyle at 1:100 000 scale. The first two digits define a longitude band 0.5 degree wide and the second two digits a latitude band 0.5 degree wide."@en ;
    skos:inScheme cs: ;
    skos:notation "7954" ;
    skos:prefLabel "Aberfoyle:7954"@en ;
.

geoad:AbingdonDowns7562
    a skos:Concept ;
    skos:historyNote "Compiled by the Geological Survey of Queensland" ;
    skos:broader geoad:MapSeries ;
    skos:definition "Map sheet for Abingdon Downs at 1:100 000 scale. The first two digits define a longitude band 0.5 degree wide and the second two digits a latitude band 0.5 degree wide."@en ;
    skos:inScheme cs: ;
    skos:notation "7562" ;
    skos:prefLabel "Abingdon Downs:7562"@en ;
.

geoad:AbuddaLakes6551
    a skos:Concept ;
    skos:historyNote "Compiled by the Geological Survey of Queensland" ;
    skos:broader geoad:MapSeries ;
    skos:definition "Map sheet for Abudda Lakes at 1:100 000 scale. The first two digits define a longitude band 0.5 degree wide and the second two digits a latitude band 0.5 degree wide."@en ;
    skos:inScheme cs: ;
    skos:notation "6551" ;
    skos:prefLabel "Abudda Lakes:6551"@en ;
.

geoad:Adavale7846
    a skos:Concept ;
    skos:historyNote "Compiled by the Geological Survey of Queensland" ;
    skos:broader geoad:MapSeries ;
    skos:definition "Map sheet for Adavale at 1:100 000 scale. The first two digits define a longitude band 0.5 degree wide and the second two digits a latitude band 0.5 degree wide."@en ;
    skos:inScheme cs: ;
    skos:notation "7846" ;
    skos:prefLabel "Adavale:7846"@en ;
.

geoad:Agnew7373
    a skos:Concept ;
    skos:historyNote "Compiled by the Geological Survey of Queensland" ;
    skos:broader geoad:MapSeries ;
    skos:definition "Map sheet for Agnew at 1:100 000 scale. The first two digits define a longitude band 0.5 degree wide and the second two digits a latitude band 0.5 degree wide."@en ;
    skos:inScheme cs: ;
    skos:notation "7373" ;
    skos:prefLabel "Agnew:7373"@en ;
.

geoad:Albro8252
    a skos:Concept ;
    skos:historyNote "Compiled by the Geological Survey of Queensland" ;
    skos:broader geoad:MapSeries ;
    skos:definition "Map sheet for Albro at 1:100 000 scale. The first two digits define a longitude band 0.5 degree wide and the second two digits a latitude band 0.5 degree wide."@en ;
    skos:inScheme cs: ;
    skos:notation "8252" ;
    skos:prefLabel "Albro:8252"@en ;
.

geoad:Alcala7058
    a skos:Concept ;
    skos:historyNote "Compiled by the Geological Survey of Queensland" ;
    skos:broader geoad:MapSeries ;
    skos:definition "Map sheet for Alcala at 1:100 000 scale. The first two digits define a longitude band 0.5 degree wide and the second two digits a latitude band 0.5 degree wide."@en ;
    skos:inScheme cs: ;
    skos:notation "7058" ;
    skos:prefLabel "Alcala:7058"@en ;
.

geoad:Allora9241
    a skos:Concept ;
    skos:historyNote "Compiled by the Geological Survey of Queensland" ;
    skos:broader geoad:MapSeries ;
    skos:definition "Map sheet for Allora at 1:100 000 scale. The first two digits define a longitude band 0.5 degree wide and the second two digits a latitude band 0.5 degree wide."@en ;
    skos:inScheme cs: ;
    skos:notation "9241" ;
    skos:prefLabel "Allora:9241"@en ;
.

geoad:Alpha8250
    a skos:Concept ;
    skos:historyNote "Compiled by the Geological Survey of Queensland" ;
    skos:broader geoad:MapSeries ;
    skos:definition "Map sheet for Alpha at 1:100 000 scale. The first two digits define a longitude band 0.5 degree wide and the second two digits a latitude band 0.5 degree wide."@en ;
    skos:inScheme cs: ;
    skos:notation "8250" ;
    skos:prefLabel "Alpha:8250"@en ;
.

geoad:Alsace6858
    a skos:Concept ;
    skos:historyNote "Compiled by the Geological Survey of Queensland" ;
    skos:broader geoad:MapSeries ;
    skos:definition "Map sheet for Alsace at 1:100 000 scale. The first two digits define a longitude band 0.5 degree wide and the second two digits a latitude band 0.5 degree wide."@en ;
    skos:inScheme cs: ;
    skos:notation "6858" ;
    skos:prefLabel "Alsace:6858"@en ;
.

geoad:AltonDowns6645
    a skos:Concept ;
    skos:historyNote "Compiled by the Geological Survey of Queensland" ;
    skos:broader geoad:MapSeries ;
    skos:definition "Map sheet for Alton Downs at 1:100 000 scale. The first two digits define a longitude band 0.5 degree wide and the second two digits a latitude band 0.5 degree wide."@en ;
    skos:inScheme cs: ;
    skos:notation "6645" ;
    skos:prefLabel "Alton Downs:6645"@en ;
.

geoad:Ambathala7946
    a skos:Concept ;
    skos:historyNote "Compiled by the Geological Survey of Queensland" ;
    skos:broader geoad:MapSeries ;
    skos:definition "Map sheet for Ambathala at 1:100 000 scale. The first two digits define a longitude band 0.5 degree wide and the second two digits a latitude band 0.5 degree wide."@en ;
    skos:inScheme cs: ;
    skos:notation "7946" ;
    skos:prefLabel "Ambathala:7946"@en ;
.

geoad:Anakie8450
    a skos:Concept ;
    skos:historyNote "Compiled by the Geological Survey of Queensland" ;
    skos:broader geoad:MapSeries ;
    skos:definition "Map sheet for Anakie at 1:100 000 scale. The first two digits define a longitude band 0.5 degree wide and the second two digits a latitude band 0.5 degree wide."@en ;
    skos:inScheme cs: ;
    skos:notation "8450" ;
    skos:prefLabel "Anakie:8450"@en ;
.

geoad:Angellala8245
    a skos:Concept ;
    skos:historyNote "Compiled by the Geological Survey of Queensland" ;
    skos:broader geoad:MapSeries ;
    skos:definition "Map sheet for Angellala at 1:100 000 scale. The first two digits define a longitude band 0.5 degree wide and the second two digits a latitude band 0.5 degree wide."@en ;
    skos:inScheme cs: ;
    skos:notation "8245" ;
    skos:prefLabel "Angellala:8245"@en ;
.

geoad:Aramac7952
    a skos:Concept ;
    skos:historyNote "Compiled by the Geological Survey of Queensland" ;
    skos:broader geoad:MapSeries ;
    skos:definition "Map sheet for Aramac at 1:100 000 scale. The first two digits define a longitude band 0.5 degree wide and the second two digits a latitude band 0.5 degree wide."@en ;
    skos:inScheme cs: ;
    skos:notation "7952" ;
    skos:prefLabel "Aramac:7952"@en ;
.

geoad:Arcadia8647
    a skos:Concept ;
    skos:historyNote "Compiled by the Geological Survey of Queensland" ;
    skos:broader geoad:MapSeries ;
    skos:definition "Map sheet for Arcadia at 1:100 000 scale. The first two digits define a longitude band 0.5 degree wide and the second two digits a latitude band 0.5 degree wide."@en ;
    skos:inScheme cs: ;
    skos:notation "8647" ;
    skos:prefLabel "Arcadia:8647"@en ;
.

geoad:ArcherRiver7270
    a skos:Concept ;
    skos:historyNote "Compiled by the Geological Survey of Queensland" ;
    skos:broader geoad:MapSeries ;
    skos:definition "Map sheet for Archer River at 1:100 000 scale. The first two digits define a longitude band 0.5 degree wide and the second two digits a latitude band 0.5 degree wide."@en ;
    skos:inScheme cs: ;
    skos:notation "7270" ;
    skos:prefLabel "Archer River:7270"@en ;
.

geoad:Ardmore6754
    a skos:Concept ;
    skos:historyNote "Compiled by the Geological Survey of Queensland" ;
    skos:broader geoad:MapSeries ;
    skos:definition "Map sheet for Ardmore at 1:100 000 scale. The first two digits define a longitude band 0.5 degree wide and the second two digits a latitude band 0.5 degree wide."@en ;
    skos:inScheme cs: ;
    skos:notation "6754" ;
    skos:prefLabel "Ardmore:6754"@en ;
.

geoad:Arno7648
    a skos:Concept ;
    skos:historyNote "Compiled by the Geological Survey of Queensland" ;
    skos:broader geoad:MapSeries ;
    skos:definition "Map sheet for Arno at 1:100 000 scale. The first two digits define a longitude band 0.5 degree wide and the second two digits a latitude band 0.5 degree wide."@en ;
    skos:inScheme cs: ;
    skos:notation "7648" ;
    skos:prefLabel "Arno:7648"@en ;
.

geoad:Arrabury7144
    a skos:Concept ;
    skos:historyNote "Compiled by the Geological Survey of Queensland" ;
    skos:broader geoad:MapSeries ;
    skos:definition "Map sheet for Arrabury at 1:100 000 scale. The first two digits define a longitude band 0.5 degree wide and the second two digits a latitude band 0.5 degree wide."@en ;
    skos:inScheme cs: ;
    skos:notation "7144" ;
    skos:prefLabel "Arrabury:7144"@en ;
.

geoad:Arrilalah7650
    a skos:Concept ;
    skos:historyNote "Compiled by the Geological Survey of Queensland" ;
    skos:broader geoad:MapSeries ;
    skos:definition "Map sheet for Arrilalah at 1:100 000 scale. The first two digits define a longitude band 0.5 degree wide and the second two digits a latitude band 0.5 degree wide."@en ;
    skos:inScheme cs: ;
    skos:notation "7650" ;
    skos:prefLabel "Arrilalah:7650"@en ;
.

geoad:Artracoona6939
    a skos:Concept ;
    skos:historyNote "Compiled by the Geological Survey of Queensland" ;
    skos:broader geoad:MapSeries ;
    skos:definition "Map sheet for Artracoona at 1:100 000 scale. The first two digits define a longitude band 0.5 degree wide and the second two digits a latitude band 0.5 degree wide."@en ;
    skos:inScheme cs: ;
    skos:notation "6939" ;
    skos:prefLabel "Artracoona:6939"@en ;
.

geoad:ArtubIslet7576
    a skos:Concept ;
    skos:historyNote "Compiled by the Geological Survey of Queensland" ;
    skos:broader geoad:MapSeries ;
    skos:definition "Map sheet for Artub Islet at 1:100 000 scale. The first two digits define a longitude band 0.5 degree wide and the second two digits a latitude band 0.5 degree wide."@en ;
    skos:inScheme cs: ;
    skos:notation "7576" ;
    skos:prefLabel "Artub Islet:7576"@en ;
.

geoad:Ashford9139
    a skos:Concept ;
    skos:historyNote "Compiled by the Geological Survey of Queensland" ;
    skos:broader geoad:MapSeries ;
    skos:definition "Map sheet for Ashford at 1:100 000 scale. The first two digits define a longitude band 0.5 degree wide and the second two digits a latitude band 0.5 degree wide."@en ;
    skos:inScheme cs: ;
    skos:notation "9139" ;
    skos:prefLabel "Ashford:9139"@en ;
.

geoad:Atherton7963
    a skos:Concept ;
    skos:historyNote "Compiled by the Geological Survey of Queensland" ;
    skos:broader geoad:MapSeries ;
    skos:definition "Map sheet for Atherton at 1:100 000 scale. The first two digits define a longitude band 0.5 degree wide and the second two digits a latitude band 0.5 degree wide."@en ;
    skos:inScheme cs: ;
    skos:notation "7963" ;
    skos:prefLabel "Atherton:7963"@en ;
.

geoad:Auburn9046
    a skos:Concept ;
    skos:historyNote "Compiled by the Geological Survey of Queensland" ;
    skos:broader geoad:MapSeries ;
    skos:definition "Map sheet for Auburn at 1:100 000 scale. The first two digits define a longitude band 0.5 degree wide and the second two digits a latitude band 0.5 degree wide."@en ;
    skos:inScheme cs: ;
    skos:notation "9046" ;
    skos:prefLabel "Auburn:9046"@en ;
.

geoad:Augathella8246
    a skos:Concept ;
    skos:historyNote "Compiled by the Geological Survey of Queensland" ;
    skos:broader geoad:MapSeries ;
    skos:definition "Map sheet for Augathella at 1:100 000 scale. The first two digits define a longitude band 0.5 degree wide and the second two digits a latitude band 0.5 degree wide."@en ;
    skos:inScheme cs: ;
    skos:notation "8246" ;
    skos:prefLabel "Augathella:8246"@en ;
.

geoad:AugustusDowns6860
    a skos:Concept ;
    skos:historyNote "Compiled by the Geological Survey of Queensland" ;
    skos:broader geoad:MapSeries ;
    skos:definition "Map sheet for Augustus Downs at 1:100 000 scale. The first two digits define a longitude band 0.5 degree wide and the second two digits a latitude band 0.5 degree wide."@en ;
    skos:inScheme cs: ;
    skos:notation "6860" ;
    skos:prefLabel "Augustus Downs:6860"@en ;
.

geoad:Aurukun7271
    a skos:Concept ;
    skos:historyNote "Compiled by the Geological Survey of Queensland" ;
    skos:broader geoad:MapSeries ;
    skos:definition "Map sheet for Aurukun at 1:100 000 scale. The first two digits define a longitude band 0.5 degree wide and the second two digits a latitude band 0.5 degree wide."@en ;
    skos:inScheme cs: ;
    skos:notation "7271" ;
    skos:prefLabel "Aurukun:7271"@en ;
.

geoad:Authoringa8244
    a skos:Concept ;
    skos:historyNote "Compiled by the Geological Survey of Queensland" ;
    skos:broader geoad:MapSeries ;
    skos:definition "Map sheet for Authoringa at 1:100 000 scale. The first two digits define a longitude band 0.5 degree wide and the second two digits a latitude band 0.5 degree wide."@en ;
    skos:inScheme cs: ;
    skos:notation "8244" ;
    skos:prefLabel "Authoringa:8244"@en ;
.

geoad:Ayr8358
    a skos:Concept ;
    skos:historyNote "Compiled by the Geological Survey of Queensland" ;
    skos:broader geoad:MapSeries ;
    skos:definition "Map sheet for Ayr at 1:100 000 scale. The first two digits define a longitude band 0.5 degree wide and the second two digits a latitude band 0.5 degree wide."@en ;
    skos:inScheme cs: ;
    skos:notation "8358" ;
    skos:prefLabel "Ayr:8358"@en ;
.

geoad:AyrshireDowns7454
    a skos:Concept ;
    skos:historyNote "Compiled by the Geological Survey of Queensland" ;
    skos:broader geoad:MapSeries ;
    skos:definition "Map sheet for Ayrshire Downs at 1:100 000 scale. The first two digits define a longitude band 0.5 degree wide and the second two digits a latitude band 0.5 degree wide."@en ;
    skos:inScheme cs: ;
    skos:notation "7454" ;
    skos:prefLabel "Ayrshire Downs:7454"@en ;
.

geoad:Badalia6752
    a skos:Concept ;
    skos:historyNote "Compiled by the Geological Survey of Queensland" ;
    skos:broader geoad:MapSeries ;
    skos:definition "Map sheet for Badalia at 1:100 000 scale. The first two digits define a longitude band 0.5 degree wide and the second two digits a latitude band 0.5 degree wide."@en ;
    skos:inScheme cs: ;
    skos:notation "6752" ;
    skos:prefLabel "Badalia:6752"@en ;
.

geoad:Bajool9050
    a skos:Concept ;
    skos:historyNote "Compiled by the Geological Survey of Queensland" ;
    skos:broader geoad:MapSeries ;
    skos:definition "Map sheet for Bajool at 1:100 000 scale. The first two digits define a longitude band 0.5 degree wide and the second two digits a latitude band 0.5 degree wide."@en ;
    skos:inScheme cs: ;
    skos:notation "9050" ;
    skos:prefLabel "Bajool:9050"@en ;
.

geoad:Ballina9640
    a skos:Concept ;
    skos:historyNote "Compiled by the Geological Survey of Queensland" ;
    skos:broader geoad:MapSeries ;
    skos:definition "Map sheet for Ballina at 1:100 000 scale. The first two digits define a longitude band 0.5 degree wide and the second two digits a latitude band 0.5 degree wide."@en ;
    skos:inScheme cs: ;
    skos:notation "9640" ;
    skos:prefLabel "Ballina:9640"@en ;
.

geoad:BallysLagoon6663
    a skos:Concept ;
    skos:historyNote "Compiled by the Geological Survey of Queensland" ;
    skos:broader geoad:MapSeries ;
    skos:definition "Map sheet for Ballys Lagoon at 1:100 000 scale. The first two digits define a longitude band 0.5 degree wide and the second two digits a latitude band 0.5 degree wide."@en ;
    skos:inScheme cs: ;
    skos:notation "6663" ;
    skos:prefLabel "Ballys Lagoon:6663"@en ;
.

geoad:Banana8949
    a skos:Concept ;
    skos:historyNote "Compiled by the Geological Survey of Queensland" ;
    skos:broader geoad:MapSeries ;
    skos:definition "Map sheet for Banana at 1:100 000 scale. The first two digits define a longitude band 0.5 degree wide and the second two digits a latitude band 0.5 degree wide."@en ;
    skos:inScheme cs: ;
    skos:notation "8949" ;
    skos:prefLabel "Banana:8949"@en ;
.

geoad:Barakula9045
    a skos:Concept ;
    skos:historyNote "Compiled by the Geological Survey of Queensland" ;
    skos:broader geoad:MapSeries ;
    skos:definition "Map sheet for Barakula at 1:100 000 scale. The first two digits define a longitude band 0.5 degree wide and the second two digits a latitude band 0.5 degree wide."@en ;
    skos:inScheme cs: ;
    skos:notation "9045" ;
    skos:prefLabel "Barakula:9045"@en ;
.

geoad:Baralaba8849
    a skos:Concept ;
    skos:historyNote "Compiled by the Geological Survey of Queensland" ;
    skos:broader geoad:MapSeries ;
    skos:definition "Map sheet for Baralaba at 1:100 000 scale. The first two digits define a longitude band 0.5 degree wide and the second two digits a latitude band 0.5 degree wide."@en ;
    skos:inScheme cs: ;
    skos:notation "8849" ;
    skos:prefLabel "Baralaba:8849"@en ;
.

geoad:Barcaldine7950
    a skos:Concept ;
    skos:historyNote "Compiled by the Geological Survey of Queensland" ;
    skos:broader geoad:MapSeries ;
    skos:definition "Map sheet for Barcaldine at 1:100 000 scale. The first two digits define a longitude band 0.5 degree wide and the second two digits a latitude band 0.5 degree wide."@en ;
    skos:inScheme cs: ;
    skos:notation "7950" ;
    skos:prefLabel "Barcaldine:7950"@en ;
.

geoad:Barcoonia7543
    a skos:Concept ;
    skos:historyNote "Compiled by the Geological Survey of Queensland" ;
    skos:broader geoad:MapSeries ;
    skos:definition "Map sheet for Barcoonia at 1:100 000 scale. The first two digits define a longitude band 0.5 degree wide and the second two digits a latitude band 0.5 degree wide."@en ;
    skos:inScheme cs: ;
    skos:notation "7543" ;
    skos:prefLabel "Barcoonia:7543"@en ;
.

geoad:BarringtonPeak6650
    a skos:Concept ;
    skos:historyNote "Compiled by the Geological Survey of Queensland" ;
    skos:broader geoad:MapSeries ;
    skos:definition "Map sheet for Barrington Peak at 1:100 000 scale. The first two digits define a longitude band 0.5 degree wide and the second two digits a latitude band 0.5 degree wide."@en ;
    skos:inScheme cs: ;
    skos:notation "6650" ;
    skos:prefLabel "Barrington Peak:6650"@en ;
.

geoad:Barrolka7245
    a skos:Concept ;
    skos:historyNote "Compiled by the Geological Survey of Queensland" ;
    skos:broader geoad:MapSeries ;
    skos:definition "Map sheet for Barrolka at 1:100 000 scale. The first two digits define a longitude band 0.5 degree wide and the second two digits a latitude band 0.5 degree wide."@en ;
    skos:inScheme cs: ;
    skos:notation "7245" ;
    skos:prefLabel "Barrolka:7245"@en ;
.

geoad:BartleFrere8063
    a skos:Concept ;
    skos:historyNote "Compiled by the Geological Survey of Queensland" ;
    skos:broader geoad:MapSeries ;
    skos:definition "Map sheet for Bartle Frere at 1:100 000 scale. The first two digits define a longitude band 0.5 degree wide and the second two digits a latitude band 0.5 degree wide."@en ;
    skos:inScheme cs: ;
    skos:notation "8063" ;
    skos:prefLabel "Bartle Frere:8063"@en ;
.

geoad:Baryulah7242
    a skos:Concept ;
    skos:historyNote "Compiled by the Geological Survey of Queensland" ;
    skos:broader geoad:MapSeries ;
    skos:definition "Map sheet for Baryulah at 1:100 000 scale. The first two digits define a longitude band 0.5 degree wide and the second two digits a latitude band 0.5 degree wide."@en ;
    skos:inScheme cs: ;
    skos:notation "7242" ;
    skos:prefLabel "Baryulah:7242"@en ;
.

geoad:BataviaDowns7472
    a skos:Concept ;
    skos:historyNote "Compiled by the Geological Survey of Queensland" ;
    skos:broader geoad:MapSeries ;
    skos:definition "Map sheet for Batavia Downs at 1:100 000 scale. The first two digits define a longitude band 0.5 degree wide and the second two digits a latitude band 0.5 degree wide."@en ;
    skos:inScheme cs: ;
    skos:notation "7472" ;
    skos:prefLabel "Batavia Downs:7472"@en ;
.

geoad:BathurstRange7769
    a skos:Concept ;
    skos:historyNote "Compiled by the Geological Survey of Queensland" ;
    skos:broader geoad:MapSeries ;
    skos:definition "Map sheet for Bathurst Range at 1:100 000 scale. The first two digits define a longitude band 0.5 degree wide and the second two digits a latitude band 0.5 degree wide."@en ;
    skos:inScheme cs: ;
    skos:notation "7769" ;
    skos:prefLabel "Bathurst Range:7769"@en ;
.

geoad:BattleCamp7867
    a skos:Concept ;
    skos:historyNote "Compiled by the Geological Survey of Queensland" ;
    skos:broader geoad:MapSeries ;
    skos:definition "Map sheet for Battle Camp at 1:100 000 scale. The first two digits define a longitude band 0.5 degree wide and the second two digits a latitude band 0.5 degree wide."@en ;
    skos:inScheme cs: ;
    skos:notation "7867" ;
    skos:prefLabel "Battle Camp:7867"@en ;
.

geoad:Bauhinia8748
    a skos:Concept ;
    skos:historyNote "Compiled by the Geological Survey of Queensland" ;
    skos:broader geoad:MapSeries ;
    skos:definition "Map sheet for Bauhinia at 1:100 000 scale. The first two digits define a longitude band 0.5 degree wide and the second two digits a latitude band 0.5 degree wide."@en ;
    skos:inScheme cs: ;
    skos:notation "8748" ;
    skos:prefLabel "Bauhinia:8748"@en ;
.

geoad:Bayfield9052
    a skos:Concept ;
    skos:historyNote "Compiled by the Geological Survey of Queensland" ;
    skos:broader geoad:MapSeries ;
    skos:definition "Map sheet for Bayfield at 1:100 000 scale. The first two digits define a longitude band 0.5 degree wide and the second two digits a latitude band 0.5 degree wide."@en ;
    skos:inScheme cs: ;
    skos:notation "9052" ;
    skos:prefLabel "Bayfield:9052"@en ;
.

geoad:Bedourie6749
    a skos:Concept ;
    skos:historyNote "Compiled by the Geological Survey of Queensland" ;
    skos:broader geoad:MapSeries ;
    skos:definition "Map sheet for Bedourie at 1:100 000 scale. The first two digits define a longitude band 0.5 degree wide and the second two digits a latitude band 0.5 degree wide."@en ;
    skos:inScheme cs: ;
    skos:notation "6749" ;
    skos:prefLabel "Bedourie:6749"@en ;
.

geoad:Beechal7843
    a skos:Concept ;
    skos:historyNote "Compiled by the Geological Survey of Queensland" ;
    skos:broader geoad:MapSeries ;
    skos:definition "Map sheet for Beechal at 1:100 000 scale. The first two digits define a longitude band 0.5 degree wide and the second two digits a latitude band 0.5 degree wide."@en ;
    skos:inScheme cs: ;
    skos:notation "7843" ;
    skos:prefLabel "Beechal:7843"@en ;
.

geoad:Beenleigh9542
    a skos:Concept ;
    skos:historyNote "Compiled by the Geological Survey of Queensland" ;
    skos:broader geoad:MapSeries ;
    skos:definition "Map sheet for Beenleigh at 1:100 000 scale. The first two digits define a longitude band 0.5 degree wide and the second two digits a latitude band 0.5 degree wide."@en ;
    skos:inScheme cs: ;
    skos:notation "9542" ;
    skos:prefLabel "Beenleigh:9542"@en ;
.

geoad:Bellevue7764
    a skos:Concept ;
    skos:historyNote "Compiled by the Geological Survey of Queensland" ;
    skos:broader geoad:MapSeries ;
    skos:definition "Map sheet for Bellevue at 1:100 000 scale. The first two digits define a longitude band 0.5 degree wide and the second two digits a latitude band 0.5 degree wide."@en ;
    skos:inScheme cs: ;
    skos:notation "7764" ;
    skos:prefLabel "Bellevue:7764"@en ;
.

geoad:Bellfield7559
    a skos:Concept ;
    skos:historyNote "Compiled by the Geological Survey of Queensland" ;
    skos:broader geoad:MapSeries ;
    skos:definition "Map sheet for Bellfield at 1:100 000 scale. The first two digits define a longitude band 0.5 degree wide and the second two digits a latitude band 0.5 degree wide."@en ;
    skos:inScheme cs: ;
    skos:notation "7559" ;
    skos:prefLabel "Bellfield:7559"@en ;
.

geoad:Bendena8242
    a skos:Concept ;
    skos:historyNote "Compiled by the Geological Survey of Queensland" ;
    skos:broader geoad:MapSeries ;
    skos:definition "Map sheet for Bendena at 1:100 000 scale. The first two digits define a longitude band 0.5 degree wide and the second two digits a latitude band 0.5 degree wide."@en ;
    skos:inScheme cs: ;
    skos:notation "8242" ;
    skos:prefLabel "Bendena:8242"@en ;
.

geoad:Bensbach7179
    a skos:Concept ;
    skos:historyNote "Compiled by the Geological Survey of Queensland" ;
    skos:broader geoad:MapSeries ;
    skos:definition "Map sheet for Bensbach at 1:100 000 scale. The first two digits define a longitude band 0.5 degree wide and the second two digits a latitude band 0.5 degree wide."@en ;
    skos:inScheme cs: ;
    skos:notation "7179" ;
    skos:prefLabel "Bensbach:7179"@en ;
.

geoad:BerawinniaDowns7639
    a skos:Concept ;
    skos:historyNote "Compiled by the Geological Survey of Queensland" ;
    skos:broader geoad:MapSeries ;
    skos:definition "Map sheet for Berawinnia Downs at 1:100 000 scale. The first two digits define a longitude band 0.5 degree wide and the second two digits a latitude band 0.5 degree wide."@en ;
    skos:inScheme cs: ;
    skos:notation "7639" ;
    skos:prefLabel "Berawinnia Downs:7639"@en ;
.

geoad:Betoota7046
    a skos:Concept ;
    skos:historyNote "Compiled by the Geological Survey of Queensland" ;
    skos:broader geoad:MapSeries ;
    skos:definition "Map sheet for Betoota at 1:100 000 scale. The first two digits define a longitude band 0.5 degree wide and the second two digits a latitude band 0.5 degree wide."@en ;
    skos:inScheme cs: ;
    skos:notation "7046" ;
    skos:prefLabel "Betoota:7046"@en ;
.

geoad:Bidgel8742
    a skos:Concept ;
    skos:historyNote "Compiled by the Geological Survey of Queensland" ;
    skos:broader geoad:MapSeries ;
    skos:definition "Map sheet for Bidgel at 1:100 000 scale. The first two digits define a longitude band 0.5 degree wide and the second two digits a latitude band 0.5 degree wide."@en ;
    skos:inScheme cs: ;
    skos:notation "8742" ;
    skos:prefLabel "Bidgel:8742"@en ;
.

geoad:Biggenden9346
    a skos:Concept ;
    skos:historyNote "Compiled by the Geological Survey of Queensland" ;
    skos:broader geoad:MapSeries ;
    skos:definition "Map sheet for Biggenden at 1:100 000 scale. The first two digits define a longitude band 0.5 degree wide and the second two digits a latitude band 0.5 degree wide."@en ;
    skos:inScheme cs: ;
    skos:notation "9346" ;
    skos:prefLabel "Biggenden:9346"@en ;
.

geoad:Biloela9049
    a skos:Concept ;
    skos:historyNote "Compiled by the Geological Survey of Queensland" ;
    skos:broader geoad:MapSeries ;
    skos:definition "Map sheet for Biloela at 1:100 000 scale. The first two digits define a longitude band 0.5 degree wide and the second two digits a latitude band 0.5 degree wide."@en ;
    skos:inScheme cs: ;
    skos:notation "9049" ;
    skos:prefLabel "Biloela:9049"@en ;
.

geoad:Bilpamorea6847
    a skos:Concept ;
    skos:historyNote "Compiled by the Geological Survey of Queensland" ;
    skos:broader geoad:MapSeries ;
    skos:definition "Map sheet for Bilpamorea at 1:100 000 scale. The first two digits define a longitude band 0.5 degree wide and the second two digits a latitude band 0.5 degree wide."@en ;
    skos:inScheme cs: ;
    skos:notation "6847" ;
    skos:prefLabel "Bilpamorea:6847"@en ;
.

geoad:Bimerah7649
    a skos:Concept ;
    skos:historyNote "Compiled by the Geological Survey of Queensland" ;
    skos:broader geoad:MapSeries ;
    skos:definition "Map sheet for Bimerah at 1:100 000 scale. The first two digits define a longitude band 0.5 degree wide and the second two digits a latitude band 0.5 degree wide."@en ;
    skos:inScheme cs: ;
    skos:notation "7649" ;
    skos:prefLabel "Bimerah:7649"@en ;
.

geoad:Birdsville6746
    a skos:Concept ;
    skos:historyNote "Compiled by the Geological Survey of Queensland" ;
    skos:broader geoad:MapSeries ;
    skos:definition "Map sheet for Birdsville at 1:100 000 scale. The first two digits define a longitude band 0.5 degree wide and the second two digits a latitude band 0.5 degree wide."@en ;
    skos:inScheme cs: ;
    skos:notation "6746" ;
    skos:prefLabel "Birdsville:6746"@en ;
.

geoad:Blackall7949
    a skos:Concept ;
    skos:historyNote "Compiled by the Geological Survey of Queensland" ;
    skos:broader geoad:MapSeries ;
    skos:definition "Map sheet for Blackall at 1:100 000 scale. The first two digits define a longitude band 0.5 degree wide and the second two digits a latitude band 0.5 degree wide."@en ;
    skos:inScheme cs: ;
    skos:notation "7949" ;
    skos:prefLabel "Blackall:7949"@en ;
.

geoad:Blackbull7262
    a skos:Concept ;
    skos:historyNote "Compiled by the Geological Survey of Queensland" ;
    skos:broader geoad:MapSeries ;
    skos:definition "Map sheet for Blackbull at 1:100 000 scale. The first two digits define a longitude band 0.5 degree wide and the second two digits a latitude band 0.5 degree wide."@en ;
    skos:inScheme cs: ;
    skos:notation "7262" ;
    skos:prefLabel "Blackbull:7262"@en ;
.

geoad:Blackdown7663
    a skos:Concept ;
    skos:historyNote "Compiled by the Geological Survey of Queensland" ;
    skos:broader geoad:MapSeries ;
    skos:definition "Map sheet for Blackdown at 1:100 000 scale. The first two digits define a longitude band 0.5 degree wide and the second two digits a latitude band 0.5 degree wide."@en ;
    skos:inScheme cs: ;
    skos:notation "7663" ;
    skos:prefLabel "Blackdown:7663"@en ;
.

geoad:Bogantungan8350
    a skos:Concept ;
    skos:historyNote "Compiled by the Geological Survey of Queensland" ;
    skos:broader geoad:MapSeries ;
    skos:definition "Map sheet for Bogantungan at 1:100 000 scale. The first two digits define a longitude band 0.5 degree wide and the second two digits a latitude band 0.5 degree wide."@en ;
    skos:inScheme cs: ;
    skos:notation "8350" ;
    skos:prefLabel "Bogantungan:8350"@en ;
.

geoad:Bogie8457
    a skos:Concept ;
    skos:historyNote "Compiled by the Geological Survey of Queensland" ;
    skos:broader geoad:MapSeries ;
    skos:definition "Map sheet for Bogie at 1:100 000 scale. The first two digits define a longitude band 0.5 degree wide and the second two digits a latitude band 0.5 degree wide."@en ;
    skos:inScheme cs: ;
    skos:notation "8457" ;
    skos:prefLabel "Bogie:8457"@en ;
.

geoad:Boigu7379
    a skos:Concept ;
    skos:historyNote "Compiled by the Geological Survey of Queensland" ;
    skos:broader geoad:MapSeries ;
    skos:definition "Map sheet for Boigu at 1:100 000 scale. The first two digits define a longitude band 0.5 degree wide and the second two digits a latitude band 0.5 degree wide."@en ;
    skos:inScheme cs: ;
    skos:notation "7379" ;
    skos:prefLabel "Boigu:7379"@en ;
.

geoad:Bollard7040
    a skos:Concept ;
    skos:historyNote "Compiled by the Geological Survey of Queensland" ;
    skos:broader geoad:MapSeries ;
    skos:definition "Map sheet for Bollard at 1:100 000 scale. The first two digits define a longitude band 0.5 degree wide and the second two digits a latitude band 0.5 degree wide."@en ;
    skos:inScheme cs: ;
    skos:notation "7040" ;
    skos:prefLabel "Bollard:7040"@en ;
.

geoad:Bollon8341
    a skos:Concept ;
    skos:historyNote "Compiled by the Geological Survey of Queensland" ;
    skos:broader geoad:MapSeries ;
    skos:definition "Map sheet for Bollon at 1:100 000 scale. The first two digits define a longitude band 0.5 degree wide and the second two digits a latitude band 0.5 degree wide."@en ;
    skos:inScheme cs: ;
    skos:notation "8341" ;
    skos:prefLabel "Bollon:8341"@en ;
.

geoad:Bombandy8653
    a skos:Concept ;
    skos:historyNote "Compiled by the Geological Survey of Queensland" ;
    skos:broader geoad:MapSeries ;
    skos:definition "Map sheet for Bombandy at 1:100 000 scale. The first two digits define a longitude band 0.5 degree wide and the second two digits a latitude band 0.5 degree wide."@en ;
    skos:inScheme cs: ;
    skos:notation "8653" ;
    skos:prefLabel "Bombandy:8653"@en ;
.

geoad:Bonalbo9440
    a skos:Concept ;
    skos:historyNote "Compiled by the Geological Survey of Queensland" ;
    skos:broader geoad:MapSeries ;
    skos:definition "Map sheet for Bonalbo at 1:100 000 scale. The first two digits define a longitude band 0.5 degree wide and the second two digits a latitude band 0.5 degree wide."@en ;
    skos:inScheme cs: ;
    skos:notation "9440" ;
    skos:prefLabel "Bonalbo:9440"@en ;
.

geoad:BonnaVonna8241
    a skos:Concept ;
    skos:historyNote "Compiled by the Geological Survey of Queensland" ;
    skos:broader geoad:MapSeries ;
    skos:definition "Map sheet for Bonna Vonna at 1:100 000 scale. The first two digits define a longitude band 0.5 degree wide and the second two digits a latitude band 0.5 degree wide."@en ;
    skos:inScheme cs: ;
    skos:notation "8241" ;
    skos:prefLabel "Bonna Vonna:8241"@en ;
.

geoad:BonusDowns8444
    a skos:Concept ;
    skos:historyNote "Compiled by the Geological Survey of Queensland" ;
    skos:broader geoad:MapSeries ;
    skos:definition "Map sheet for Bonus Downs at 1:100 000 scale. The first two digits define a longitude band 0.5 degree wide and the second two digits a latitude band 0.5 degree wide."@en ;
    skos:inScheme cs: ;
    skos:notation "8444" ;
    skos:prefLabel "Bonus Downs:8444"@en ;
.

geoad:Boobara7942
    a skos:Concept ;
    skos:historyNote "Compiled by the Geological Survey of Queensland" ;
    skos:broader geoad:MapSeries ;
    skos:definition "Map sheet for Boobara at 1:100 000 scale. The first two digits define a longitude band 0.5 degree wide and the second two digits a latitude band 0.5 degree wide."@en ;
    skos:inScheme cs: ;
    skos:notation "7942" ;
    skos:prefLabel "Boobara:7942"@en ;
.

geoad:BoobyIsland7276
    a skos:Concept ;
    skos:historyNote "Compiled by the Geological Survey of Queensland" ;
    skos:broader geoad:MapSeries ;
    skos:definition "Map sheet for Booby Island at 1:100 000 scale. The first two digits define a longitude band 0.5 degree wide and the second two digits a latitude band 0.5 degree wide."@en ;
    skos:inScheme cs: ;
    skos:notation "7276" ;
    skos:prefLabel "Booby Island:7276"@en ;
.

geoad:Boolba8542
    a skos:Concept ;
    skos:historyNote "Compiled by the Geological Survey of Queensland" ;
    skos:broader geoad:MapSeries ;
    skos:definition "Map sheet for Boolba at 1:100 000 scale. The first two digits define a longitude band 0.5 degree wide and the second two digits a latitude band 0.5 degree wide."@en ;
    skos:inScheme cs: ;
    skos:notation "8542" ;
    skos:prefLabel "Boolba:8542"@en ;
.

geoad:Boomi8840
    a skos:Concept ;
    skos:historyNote "Compiled by the Geological Survey of Queensland" ;
    skos:broader geoad:MapSeries ;
    skos:definition "Map sheet for Boomi at 1:100 000 scale. The first two digits define a longitude band 0.5 degree wide and the second two digits a latitude band 0.5 degree wide."@en ;
    skos:inScheme cs: ;
    skos:notation "8840" ;
    skos:prefLabel "Boomi:8840"@en ;
.

geoad:Boonderoo7757
    a skos:Concept ;
    skos:historyNote "Compiled by the Geological Survey of Queensland" ;
    skos:broader geoad:MapSeries ;
    skos:definition "Map sheet for Boonderoo at 1:100 000 scale. The first two digits define a longitude band 0.5 degree wide and the second two digits a latitude band 0.5 degree wide."@en ;
    skos:inScheme cs: ;
    skos:notation "7757" ;
    skos:prefLabel "Boonderoo:7757"@en ;
.

geoad:Boondooma9145
    a skos:Concept ;
    skos:historyNote "Compiled by the Geological Survey of Queensland" ;
    skos:broader geoad:MapSeries ;
    skos:definition "Map sheet for Boondooma at 1:100 000 scale. The first two digits define a longitude band 0.5 degree wide and the second two digits a latitude band 0.5 degree wide."@en ;
    skos:inScheme cs: ;
    skos:notation "9145" ;
    skos:prefLabel "Boondooma:9145"@en ;
.

geoad:Boongoondoo8052
    a skos:Concept ;
    skos:historyNote "Compiled by the Geological Survey of Queensland" ;
    skos:broader geoad:MapSeries ;
    skos:definition "Map sheet for Boongoondoo at 1:100 000 scale. The first two digits define a longitude band 0.5 degree wide and the second two digits a latitude band 0.5 degree wide."@en ;
    skos:inScheme cs: ;
    skos:notation "8052" ;
    skos:prefLabel "Boongoondoo:8052"@en ;
.

geoad:Boulia6852
    a skos:Concept ;
    skos:historyNote "Compiled by the Geological Survey of Queensland" ;
    skos:broader geoad:MapSeries ;
    skos:definition "Map sheet for Boulia at 1:100 000 scale. The first two digits define a longitude band 0.5 degree wide and the second two digits a latitude band 0.5 degree wide."@en ;
    skos:inScheme cs: ;
    skos:notation "6852" ;
    skos:prefLabel "Boulia:6852"@en ;
.

geoad:Bowalli7643
    a skos:Concept ;
    skos:historyNote "Compiled by the Geological Survey of Queensland" ;
    skos:broader geoad:MapSeries ;
    skos:definition "Map sheet for Bowalli at 1:100 000 scale. The first two digits define a longitude band 0.5 degree wide and the second two digits a latitude band 0.5 degree wide."@en ;
    skos:inScheme cs: ;
    skos:notation "7643" ;
    skos:prefLabel "Bowalli:7643"@en ;
.

geoad:Bowen8557
    a skos:Concept ;
    skos:historyNote "Compiled by the Geological Survey of Queensland" ;
    skos:broader geoad:MapSeries ;
    skos:definition "Map sheet for Bowen at 1:100 000 scale. The first two digits define a longitude band 0.5 degree wide and the second two digits a latitude band 0.5 degree wide."@en ;
    skos:inScheme cs: ;
    skos:notation "8557" ;
    skos:prefLabel "Bowen:8557"@en ;
.

geoad:Bowie8054
    a skos:Concept ;
    skos:historyNote "Compiled by the Geological Survey of Queensland" ;
    skos:broader geoad:MapSeries ;
    skos:definition "Map sheet for Bowie at 1:100 000 scale. The first two digits define a longitude band 0.5 degree wide and the second two digits a latitude band 0.5 degree wide."@en ;
    skos:inScheme cs: ;
    skos:notation "8054" ;
    skos:prefLabel "Bowie:8054"@en ;
.

geoad:BowlingGreenBay8359
    a skos:Concept ;
    skos:historyNote "Compiled by the Geological Survey of Queensland" ;
    skos:broader geoad:MapSeries ;
    skos:definition "Map sheet for Bowling Green Bay at 1:100 000 scale. The first two digits define a longitude band 0.5 degree wide and the second two digits a latitude band 0.5 degree wide."@en ;
    skos:inScheme cs: ;
    skos:notation "8359" ;
    skos:prefLabel "Bowling Green Bay:8359"@en ;
.

geoad:Bowthorn6561
    a skos:Concept ;
    skos:historyNote "Compiled by the Geological Survey of Queensland" ;
    skos:broader geoad:MapSeries ;
    skos:definition "Map sheet for Bowthorn at 1:100 000 scale. The first two digits define a longitude band 0.5 degree wide and the second two digits a latitude band 0.5 degree wide."@en ;
    skos:inScheme cs: ;
    skos:notation "6561" ;
    skos:prefLabel "Bowthorn:6561"@en ;
.

geoad:Bowyer7951
    a skos:Concept ;
    skos:historyNote "Compiled by the Geological Survey of Queensland" ;
    skos:broader geoad:MapSeries ;
    skos:definition "Map sheet for Bowyer at 1:100 000 scale. The first two digits define a longitude band 0.5 degree wide and the second two digits a latitude band 0.5 degree wide."@en ;
    skos:inScheme cs: ;
    skos:notation "7951" ;
    skos:prefLabel "Bowyer:7951"@en ;
.

geoad:Boxwood6840
    a skos:Concept ;
    skos:historyNote "Compiled by the Geological Survey of Queensland" ;
    skos:broader geoad:MapSeries ;
    skos:definition "Map sheet for Boxwood at 1:100 000 scale. The first two digits define a longitude band 0.5 degree wide and the second two digits a latitude band 0.5 degree wide."@en ;
    skos:inScheme cs: ;
    skos:notation "6840" ;
    skos:prefLabel "Boxwood:6840"@en ;
.

geoad:BoydongIsland7575
    a skos:Concept ;
    skos:historyNote "Compiled by the Geological Survey of Queensland" ;
    skos:broader geoad:MapSeries ;
    skos:definition "Map sheet for Boydong Island at 1:100 000 scale. The first two digits define a longitude band 0.5 degree wide and the second two digits a latitude band 0.5 degree wide."@en ;
    skos:inScheme cs: ;
    skos:notation "7575" ;
    skos:prefLabel "Boydong Island:7575"@en ;
.

geoad:BradleyCreek7752
    a skos:Concept ;
    skos:historyNote "Compiled by the Geological Survey of Queensland" ;
    skos:broader geoad:MapSeries ;
    skos:definition "Map sheet for Bradley Creek at 1:100 000 scale. The first two digits define a longitude band 0.5 degree wide and the second two digits a latitude band 0.5 degree wide."@en ;
    skos:inScheme cs: ;
    skos:notation "7752" ;
    skos:prefLabel "Bradley Creek:7752"@en ;
.

geoad:BrambleCay7679
    a skos:Concept ;
    skos:historyNote "Compiled by the Geological Survey of Queensland" ;
    skos:broader geoad:MapSeries ;
    skos:definition "Map sheet for Bramble Cay at 1:100 000 scale. The first two digits define a longitude band 0.5 degree wide and the second two digits a latitude band 0.5 degree wide."@en ;
    skos:inScheme cs: ;
    skos:notation "7679" ;
    skos:prefLabel "Bramble Cay:7679"@en ;
.

geoad:Bransby7341
    a skos:Concept ;
    skos:historyNote "Compiled by the Geological Survey of Queensland" ;
    skos:broader geoad:MapSeries ;
    skos:definition "Map sheet for Bransby at 1:100 000 scale. The first two digits define a longitude band 0.5 degree wide and the second two digits a latitude band 0.5 degree wide."@en ;
    skos:inScheme cs: ;
    skos:notation "7341" ;
    skos:prefLabel "Bransby:7341"@en ;
.

geoad:Breadalbane6850
    a skos:Concept ;
    skos:historyNote "Compiled by the Geological Survey of Queensland" ;
    skos:broader geoad:MapSeries ;
    skos:definition "Map sheet for Breadalbane at 1:100 000 scale. The first two digits define a longitude band 0.5 degree wide and the second two digits a latitude band 0.5 degree wide."@en ;
    skos:inScheme cs: ;
    skos:notation "6850" ;
    skos:prefLabel "Breadalbane:6850"@en ;
.

geoad:BrightonDowns7251
    a skos:Concept ;
    skos:historyNote "Compiled by the Geological Survey of Queensland" ;
    skos:broader geoad:MapSeries ;
    skos:definition "Map sheet for Brighton Downs at 1:100 000 scale. The first two digits define a longitude band 0.5 degree wide and the second two digits a latitude band 0.5 degree wide."@en ;
    skos:inScheme cs: ;
    skos:notation "7251" ;
    skos:prefLabel "Brighton Downs:7251"@en ;
.

geoad:Brindingabba7839
    a skos:Concept ;
    skos:historyNote "Compiled by the Geological Survey of Queensland" ;
    skos:broader geoad:MapSeries ;
    skos:definition "Map sheet for Brindingabba at 1:100 000 scale. The first two digits define a longitude band 0.5 degree wide and the second two digits a latitude band 0.5 degree wide."@en ;
    skos:inScheme cs: ;
    skos:notation "7839" ;
    skos:prefLabel "Brindingabba:7839"@en ;
.

geoad:Brisbane9543
    a skos:Concept ;
    skos:historyNote "Compiled by the Geological Survey of Queensland" ;
    skos:broader geoad:MapSeries ;
    skos:definition "Map sheet for Brisbane at 1:100 000 scale. The first two digits define a longitude band 0.5 degree wide and the second two digits a latitude band 0.5 degree wide."@en ;
    skos:inScheme cs: ;
    skos:notation "9543" ;
    skos:prefLabel "Brisbane:9543"@en ;
.

geoad:BrownCreek7161
    a skos:Concept ;
    skos:historyNote "Compiled by the Geological Survey of Queensland" ;
    skos:broader geoad:MapSeries ;
    skos:definition "Map sheet for Brown Creek at 1:100 000 scale. The first two digits define a longitude band 0.5 degree wide and the second two digits a latitude band 0.5 degree wide."@en ;
    skos:inScheme cs: ;
    skos:notation "7161" ;
    skos:prefLabel "Brown Creek:7161"@en ;
.

geoad:BuckinghamDowns6853
    a skos:Concept ;
    skos:historyNote "Compiled by the Geological Survey of Queensland" ;
    skos:broader geoad:MapSeries ;
    skos:definition "Map sheet for Buckingham Downs at 1:100 000 scale. The first two digits define a longitude band 0.5 degree wide and the second two digits a latitude band 0.5 degree wide."@en ;
    skos:inScheme cs: ;
    skos:notation "6853" ;
    skos:prefLabel "Buckingham Downs:6853"@en ;
.

geoad:Budgerygar7647
    a skos:Concept ;
    skos:historyNote "Compiled by the Geological Survey of Queensland" ;
    skos:broader geoad:MapSeries ;
    skos:definition "Map sheet for Budgerygar at 1:100 000 scale. The first two digits define a longitude band 0.5 degree wide and the second two digits a latitude band 0.5 degree wide."@en ;
    skos:inScheme cs: ;
    skos:notation "7647" ;
    skos:prefLabel "Budgerygar:7647"@en ;
.

geoad:Bulgroo7646
    a skos:Concept ;
    skos:historyNote "Compiled by the Geological Survey of Queensland" ;
    skos:broader geoad:MapSeries ;
    skos:definition "Map sheet for Bulgroo at 1:100 000 scale. The first two digits define a longitude band 0.5 degree wide and the second two digits a latitude band 0.5 degree wide."@en ;
    skos:inScheme cs: ;
    skos:notation "7646" ;
    skos:prefLabel "Bulgroo:7646"@en ;
.

geoad:Bulimba7564
    a skos:Concept ;
    skos:historyNote "Compiled by the Geological Survey of Queensland" ;
    skos:broader geoad:MapSeries ;
    skos:definition "Map sheet for Bulimba at 1:100 000 scale. The first two digits define a longitude band 0.5 degree wide and the second two digits a latitude band 0.5 degree wide."@en ;
    skos:inScheme cs: ;
    skos:notation "7564" ;
    skos:prefLabel "Bulimba:7564"@en ;
.

geoad:Bullecourt6556
    a skos:Concept ;
    skos:historyNote "Compiled by the Geological Survey of Queensland" ;
    skos:broader geoad:MapSeries ;
    skos:definition "Map sheet for Bullecourt at 1:100 000 scale. The first two digits define a longitude band 0.5 degree wide and the second two digits a latitude band 0.5 degree wide."@en ;
    skos:inScheme cs: ;
    skos:notation "6556" ;
    skos:prefLabel "Bullecourt:6556"@en ;
.

geoad:Bulliwallah8254
    a skos:Concept ;
    skos:historyNote "Compiled by the Geological Survey of Queensland" ;
    skos:broader geoad:MapSeries ;
    skos:definition "Map sheet for Bulliwallah at 1:100 000 scale. The first two digits define a longitude band 0.5 degree wide and the second two digits a latitude band 0.5 degree wide."@en ;
    skos:inScheme cs: ;
    skos:notation "8254" ;
    skos:prefLabel "Bulliwallah:8254"@en ;
.

geoad:BullockCreek7862
    a skos:Concept ;
    skos:historyNote "Compiled by the Geological Survey of Queensland" ;
    skos:broader geoad:MapSeries ;
    skos:definition "Map sheet for Bullock Creek at 1:100 000 scale. The first two digits define a longitude band 0.5 degree wide and the second two digits a latitude band 0.5 degree wide."@en ;
    skos:inScheme cs: ;
    skos:notation "7862" ;
    skos:prefLabel "Bullock Creek:7862"@en ;
.

geoad:Bulloo7440
    a skos:Concept ;
    skos:historyNote "Compiled by the Geological Survey of Queensland" ;
    skos:broader geoad:MapSeries ;
    skos:definition "Map sheet for Bulloo at 1:100 000 scale. The first two digits define a longitude band 0.5 degree wide and the second two digits a latitude band 0.5 degree wide."@en ;
    skos:inScheme cs: ;
    skos:notation "7440" ;
    skos:prefLabel "Bulloo:7440"@en ;
.

geoad:Bunarba8739
    a skos:Concept ;
    skos:historyNote "Compiled by the Geological Survey of Queensland" ;
    skos:broader geoad:MapSeries ;
    skos:definition "Map sheet for Bunarba at 1:100 000 scale. The first two digits define a longitude band 0.5 degree wide and the second two digits a latitude band 0.5 degree wide."@en ;
    skos:inScheme cs: ;
    skos:notation "8739" ;
    skos:prefLabel "Bunarba:8739"@en ;
.

geoad:BuncheedaSwamp7244
    a skos:Concept ;
    skos:historyNote "Compiled by the Geological Survey of Queensland" ;
    skos:broader geoad:MapSeries ;
    skos:definition "Map sheet for Buncheeda Swamp at 1:100 000 scale. The first two digits define a longitude band 0.5 degree wide and the second two digits a latitude band 0.5 degree wide."@en ;
    skos:inScheme cs: ;
    skos:notation "7244" ;
    skos:prefLabel "Buncheeda Swamp:7244"@en ;
.

geoad:Bundaberg9348
    a skos:Concept ;
    skos:historyNote "Compiled by the Geological Survey of Queensland" ;
    skos:broader geoad:MapSeries ;
    skos:definition "Map sheet for Bundaberg at 1:100 000 scale. The first two digits define a longitude band 0.5 degree wide and the second two digits a latitude band 0.5 degree wide."@en ;
    skos:inScheme cs: ;
    skos:notation "9348" ;
    skos:prefLabel "Bundaberg:9348"@en ;
.

geoad:Bundaleer8240
    a skos:Concept ;
    skos:historyNote "Compiled by the Geological Survey of Queensland" ;
    skos:broader geoad:MapSeries ;
    skos:definition "Map sheet for Bundaleer at 1:100 000 scale. The first two digits define a longitude band 0.5 degree wide and the second two digits a latitude band 0.5 degree wide."@en ;
    skos:inScheme cs: ;
    skos:notation "8240" ;
    skos:prefLabel "Bundaleer:8240"@en ;
.

geoad:Bungaban8946
    a skos:Concept ;
    skos:historyNote "Compiled by the Geological Survey of Queensland" ;
    skos:broader geoad:MapSeries ;
    skos:definition "Map sheet for Bungaban at 1:100 000 scale. The first two digits define a longitude band 0.5 degree wide and the second two digits a latitude band 0.5 degree wide."@en ;
    skos:inScheme cs: ;
    skos:notation "8946" ;
    skos:prefLabel "Bungaban:8946"@en ;
.

geoad:Bungunya8841
    a skos:Concept ;
    skos:historyNote "Compiled by the Geological Survey of Queensland" ;
    skos:broader geoad:MapSeries ;
    skos:definition "Map sheet for Bungunya at 1:100 000 scale. The first two digits define a longitude band 0.5 degree wide and the second two digits a latitude band 0.5 degree wide."@en ;
    skos:inScheme cs: ;
    skos:notation "8841" ;
    skos:prefLabel "Bungunya:8841"@en ;
.

geoad:Burges7859
    a skos:Concept ;
    skos:historyNote "Compiled by the Geological Survey of Queensland" ;
    skos:broader geoad:MapSeries ;
    skos:definition "Map sheet for Burges at 1:100 000 scale. The first two digits define a longitude band 0.5 degree wide and the second two digits a latitude band 0.5 degree wide."@en ;
    skos:inScheme cs: ;
    skos:notation "7859" ;
    skos:prefLabel "Burges:7859"@en ;
.

geoad:Burgorah8642
    a skos:Concept ;
    skos:historyNote "Compiled by the Geological Survey of Queensland" ;
    skos:broader geoad:MapSeries ;
    skos:definition "Map sheet for Burgorah at 1:100 000 scale. The first two digits define a longitude band 0.5 degree wide and the second two digits a latitude band 0.5 degree wide."@en ;
    skos:inScheme cs: ;
    skos:notation "8642" ;
    skos:prefLabel "Burgorah:8642"@en ;
.

geoad:Burketown6862
    a skos:Concept ;
    skos:historyNote "Compiled by the Geological Survey of Queensland" ;
    skos:broader geoad:MapSeries ;
    skos:definition "Map sheet for Burketown at 1:100 000 scale. The first two digits define a longitude band 0.5 degree wide and the second two digits a latitude band 0.5 degree wide."@en ;
    skos:inScheme cs: ;
    skos:notation "6862" ;
    skos:prefLabel "Burketown:6862"@en ;
.

geoad:Burrenbar8740
    a skos:Concept ;
    skos:historyNote "Compiled by the Geological Survey of Queensland" ;
    skos:broader geoad:MapSeries ;
    skos:definition "Map sheet for Burrenbar at 1:100 000 scale. The first two digits define a longitude band 0.5 degree wide and the second two digits a latitude band 0.5 degree wide."@en ;
    skos:inScheme cs: ;
    skos:notation "8740" ;
    skos:prefLabel "Burrenbar:8740"@en ;
.

geoad:Burruna7039
    a skos:Concept ;
    skos:historyNote "Compiled by the Geological Survey of Queensland" ;
    skos:broader geoad:MapSeries ;
    skos:definition "Map sheet for Burruna at 1:100 000 scale. The first two digits define a longitude band 0.5 degree wide and the second two digits a latitude band 0.5 degree wide."@en ;
    skos:inScheme cs: ;
    skos:notation "7039" ;
    skos:prefLabel "Burruna:7039"@en ;
.

geoad:Busthinia8050
    a skos:Concept ;
    skos:historyNote "Compiled by the Geological Survey of Queensland" ;
    skos:broader geoad:MapSeries ;
    skos:definition "Map sheet for Busthinia at 1:100 000 scale. The first two digits define a longitude band 0.5 degree wide and the second two digits a latitude band 0.5 degree wide."@en ;
    skos:inScheme cs: ;
    skos:notation "8050" ;
    skos:prefLabel "Busthinia:8050"@en ;
.

geoad:ButchersHill7866
    a skos:Concept ;
    skos:historyNote "Compiled by the Geological Survey of Queensland" ;
    skos:broader geoad:MapSeries ;
    skos:definition "Map sheet for Butchers Hill at 1:100 000 scale. The first two digits define a longitude band 0.5 degree wide and the second two digits a latitude band 0.5 degree wide."@en ;
    skos:inScheme cs: ;
    skos:notation "7866" ;
    skos:prefLabel "Butchers Hill:7866"@en ;
.

geoad:Byerwen8455
    a skos:Concept ;
    skos:historyNote "Compiled by the Geological Survey of Queensland" ;
    skos:broader geoad:MapSeries ;
    skos:definition "Map sheet for Byerwen at 1:100 000 scale. The first two digits define a longitude band 0.5 degree wide and the second two digits a latitude band 0.5 degree wide."@en ;
    skos:inScheme cs: ;
    skos:notation "8455" ;
    skos:prefLabel "Byerwen:8455"@en ;
.

geoad:Bygombo6747
    a skos:Concept ;
    skos:historyNote "Compiled by the Geological Survey of Queensland" ;
    skos:broader geoad:MapSeries ;
    skos:definition "Map sheet for Bygombo at 1:100 000 scale. The first two digits define a longitude band 0.5 degree wide and the second two digits a latitude band 0.5 degree wide."@en ;
    skos:inScheme cs: ;
    skos:notation "6747" ;
    skos:prefLabel "Bygombo:6747"@en ;
.

geoad:Caboolture9443
    a skos:Concept ;
    skos:historyNote "Compiled by the Geological Survey of Queensland" ;
    skos:broader geoad:MapSeries ;
    skos:definition "Map sheet for Caboolture at 1:100 000 scale. The first two digits define a longitude band 0.5 degree wide and the second two digits a latitude band 0.5 degree wide."@en ;
    skos:inScheme cs: ;
    skos:notation "9443" ;
    skos:prefLabel "Caboolture:9443"@en ;
.

geoad:Cadelga6945
    a skos:Concept ;
    skos:historyNote "Compiled by the Geological Survey of Queensland" ;
    skos:broader geoad:MapSeries ;
    skos:definition "Map sheet for Cadelga at 1:100 000 scale. The first two digits define a longitude band 0.5 degree wide and the second two digits a latitude band 0.5 degree wide."@en ;
    skos:inScheme cs: ;
    skos:notation "6945" ;
    skos:prefLabel "Cadelga:6945"@en ;
.

geoad:Cairns8064
    a skos:Concept ;
    skos:historyNote "Compiled by the Geological Survey of Queensland" ;
    skos:broader geoad:MapSeries ;
    skos:definition "Map sheet for Cairns at 1:100 000 scale. The first two digits define a longitude band 0.5 degree wide and the second two digits a latitude band 0.5 degree wide."@en ;
    skos:inScheme cs: ;
    skos:notation "8064" ;
    skos:prefLabel "Cairns:8064"@en ;
.

geoad:Caiwarro7840
    a skos:Concept ;
    skos:historyNote "Compiled by the Geological Survey of Queensland" ;
    skos:broader geoad:MapSeries ;
    skos:definition "Map sheet for Caiwarro at 1:100 000 scale. The first two digits define a longitude band 0.5 degree wide and the second two digits a latitude band 0.5 degree wide."@en ;
    skos:inScheme cs: ;
    skos:notation "7840" ;
    skos:prefLabel "Caiwarro:7840"@en ;
.

geoad:Caldervale8247
    a skos:Concept ;
    skos:historyNote "Compiled by the Geological Survey of Queensland" ;
    skos:broader geoad:MapSeries ;
    skos:definition "Map sheet for Caldervale at 1:100 000 scale. The first two digits define a longitude band 0.5 degree wide and the second two digits a latitude band 0.5 degree wide."@en ;
    skos:inScheme cs: ;
    skos:notation "8247" ;
    skos:prefLabel "Caldervale:8247"@en ;
.

geoad:Caledonia7953
    a skos:Concept ;
    skos:historyNote "Compiled by the Geological Survey of Queensland" ;
    skos:broader geoad:MapSeries ;
    skos:definition "Map sheet for Caledonia at 1:100 000 scale. The first two digits define a longitude band 0.5 degree wide and the second two digits a latitude band 0.5 degree wide."@en ;
    skos:inScheme cs: ;
    skos:notation "7953" ;
    skos:prefLabel "Caledonia:7953"@en ;
.

geoad:Calen8656
    a skos:Concept ;
    skos:historyNote "Compiled by the Geological Survey of Queensland" ;
    skos:broader geoad:MapSeries ;
    skos:definition "Map sheet for Calen at 1:100 000 scale. The first two digits define a longitude band 0.5 degree wide and the second two digits a latitude band 0.5 degree wide."@en ;
    skos:inScheme cs: ;
    skos:notation "8656" ;
    skos:prefLabel "Calen:8656"@en ;
.

geoad:Calliope9149
    a skos:Concept ;
    skos:historyNote "Compiled by the Geological Survey of Queensland" ;
    skos:broader geoad:MapSeries ;
    skos:definition "Map sheet for Calliope at 1:100 000 scale. The first two digits define a longitude band 0.5 degree wide and the second two digits a latitude band 0.5 degree wide."@en ;
    skos:inScheme cs: ;
    skos:notation "9149" ;
    skos:prefLabel "Calliope:9149"@en ;
.

geoad:Caloundra9544
    a skos:Concept ;
    skos:historyNote "Compiled by the Geological Survey of Queensland" ;
    skos:broader geoad:MapSeries ;
    skos:definition "Map sheet for Caloundra at 1:100 000 scale. The first two digits define a longitude band 0.5 degree wide and the second two digits a latitude band 0.5 degree wide."@en ;
    skos:inScheme cs: ;
    skos:notation "9544" ;
    skos:prefLabel "Caloundra:9544"@en ;
.

geoad:CameronDowns7755
    a skos:Concept ;
    skos:historyNote "Compiled by the Geological Survey of Queensland" ;
    skos:broader geoad:MapSeries ;
    skos:definition "Map sheet for Cameron Downs at 1:100 000 scale. The first two digits define a longitude band 0.5 degree wide and the second two digits a latitude band 0.5 degree wide."@en ;
    skos:inScheme cs: ;
    skos:notation "7755" ;
    skos:prefLabel "Cameron Downs:7755"@en ;
.

geoad:Camooweal6558
    a skos:Concept ;
    skos:historyNote "Compiled by the Geological Survey of Queensland" ;
    skos:broader geoad:MapSeries ;
    skos:definition "Map sheet for Camooweal at 1:100 000 scale. The first two digits define a longitude band 0.5 degree wide and the second two digits a latitude band 0.5 degree wide."@en ;
    skos:inScheme cs: ;
    skos:notation "6558" ;
    skos:prefLabel "Camooweal:6558"@en ;
.

geoad:Canary6951
    a skos:Concept ;
    skos:historyNote "Compiled by the Geological Survey of Queensland" ;
    skos:broader geoad:MapSeries ;
    skos:definition "Map sheet for Canary at 1:100 000 scale. The first two digits define a longitude band 0.5 degree wide and the second two digits a latitude band 0.5 degree wide."@en ;
    skos:inScheme cs: ;
    skos:notation "6951" ;
    skos:prefLabel "Canary:6951"@en ;
.

geoad:Canobie7059
    a skos:Concept ;
    skos:historyNote "Compiled by the Geological Survey of Queensland" ;
    skos:broader geoad:MapSeries ;
    skos:definition "Map sheet for Canobie at 1:100 000 scale. The first two digits define a longitude band 0.5 degree wide and the second two digits a latitude band 0.5 degree wide."@en ;
    skos:inScheme cs: ;
    skos:notation "7059" ;
    skos:prefLabel "Canobie:7059"@en ;
.

geoad:Canterbury7247
    a skos:Concept ;
    skos:historyNote "Compiled by the Geological Survey of Queensland" ;
    skos:broader geoad:MapSeries ;
    skos:definition "Map sheet for Canterbury at 1:100 000 scale. The first two digits define a longitude band 0.5 degree wide and the second two digits a latitude band 0.5 degree wide."@en ;
    skos:inScheme cs: ;
    skos:notation "7247" ;
    skos:prefLabel "Canterbury:7247"@en ;
.

geoad:CapeCapricorn9151
    a skos:Concept ;
    skos:historyNote "Compiled by the Geological Survey of Queensland" ;
    skos:broader geoad:MapSeries ;
    skos:definition "Map sheet for Cape Capricorn at 1:100 000 scale. The first two digits define a longitude band 0.5 degree wide and the second two digits a latitude band 0.5 degree wide."@en ;
    skos:inScheme cs: ;
    skos:notation "9151" ;
    skos:prefLabel "Cape Capricorn:9151"@en ;
.

geoad:CapeDirection7672
    a skos:Concept ;
    skos:historyNote "Compiled by the Geological Survey of Queensland" ;
    skos:broader geoad:MapSeries ;
    skos:definition "Map sheet for Cape Direction at 1:100 000 scale. The first two digits define a longitude band 0.5 degree wide and the second two digits a latitude band 0.5 degree wide."@en ;
    skos:inScheme cs: ;
    skos:notation "7672" ;
    skos:prefLabel "Cape Direction:7672"@en ;
.

geoad:CapeFlattery7968
    a skos:Concept ;
    skos:historyNote "Compiled by the Geological Survey of Queensland" ;
    skos:broader geoad:MapSeries ;
    skos:definition "Map sheet for Cape Flattery at 1:100 000 scale. The first two digits define a longitude band 0.5 degree wide and the second two digits a latitude band 0.5 degree wide."@en ;
    skos:inScheme cs: ;
    skos:notation "7968" ;
    skos:prefLabel "Cape Flattery:7968"@en ;
.

geoad:CapeGrenville7574
    a skos:Concept ;
    skos:historyNote "Compiled by the Geological Survey of Queensland" ;
    skos:broader geoad:MapSeries ;
    skos:definition "Map sheet for Cape Grenville at 1:100 000 scale. The first two digits define a longitude band 0.5 degree wide and the second two digits a latitude band 0.5 degree wide."@en ;
    skos:inScheme cs: ;
    skos:notation "7574" ;
    skos:prefLabel "Cape Grenville:7574"@en ;
.

geoad:CapeKeerweer7170
    a skos:Concept ;
    skos:historyNote "Compiled by the Geological Survey of Queensland" ;
    skos:broader geoad:MapSeries ;
    skos:definition "Map sheet for Cape Keerweer at 1:100 000 scale. The first two digits define a longitude band 0.5 degree wide and the second two digits a latitude band 0.5 degree wide."@en ;
    skos:inScheme cs: ;
    skos:notation "7170" ;
    skos:prefLabel "Cape Keerweer:7170"@en ;
.

geoad:CapeMelville7869
    a skos:Concept ;
    skos:historyNote "Compiled by the Geological Survey of Queensland" ;
    skos:broader geoad:MapSeries ;
    skos:definition "Map sheet for Cape Melville at 1:100 000 scale. The first two digits define a longitude band 0.5 degree wide and the second two digits a latitude band 0.5 degree wide."@en ;
    skos:inScheme cs: ;
    skos:notation "7869" ;
    skos:prefLabel "Cape Melville:7869"@en ;
.

geoad:CapeSidmouth7671
    a skos:Concept ;
    skos:historyNote "Compiled by the Geological Survey of Queensland" ;
    skos:broader geoad:MapSeries ;
    skos:definition "Map sheet for Cape Sidmouth at 1:100 000 scale. The first two digits define a longitude band 0.5 degree wide and the second two digits a latitude band 0.5 degree wide."@en ;
    skos:inScheme cs: ;
    skos:notation "7671" ;
    skos:prefLabel "Cape Sidmouth:7671"@en ;
.

geoad:CapeUpstart8458
    a skos:Concept ;
    skos:historyNote "Compiled by the Geological Survey of Queensland" ;
    skos:broader geoad:MapSeries ;
    skos:definition "Map sheet for Cape Upstart at 1:100 000 scale. The first two digits define a longitude band 0.5 degree wide and the second two digits a latitude band 0.5 degree wide."@en ;
    skos:inScheme cs: ;
    skos:notation "8458" ;
    skos:prefLabel "Cape Upstart:8458"@en ;
.

geoad:CapeVanDiemen6864
    a skos:Concept ;
    skos:historyNote "Compiled by the Geological Survey of Queensland" ;
    skos:broader geoad:MapSeries ;
    skos:definition "Map sheet for Cape Van Diemen at 1:100 000 scale. The first two digits define a longitude band 0.5 degree wide and the second two digits a latitude band 0.5 degree wide."@en ;
    skos:inScheme cs: ;
    skos:notation "6864" ;
    skos:prefLabel "Cape Van Diemen:6864"@en ;
.

geoad:CapeWeymouth7572
    a skos:Concept ;
    skos:historyNote "Compiled by the Geological Survey of Queensland" ;
    skos:broader geoad:MapSeries ;
    skos:definition "Map sheet for Cape Weymouth at 1:100 000 scale. The first two digits define a longitude band 0.5 degree wide and the second two digits a latitude band 0.5 degree wide."@en ;
    skos:inScheme cs: ;
    skos:notation "7572" ;
    skos:prefLabel "Cape Weymouth:7572"@en ;
.

geoad:CapeYork7476
    a skos:Concept ;
    skos:historyNote "Compiled by the Geological Survey of Queensland" ;
    skos:broader geoad:MapSeries ;
    skos:definition "Map sheet for Cape York at 1:100 000 scale. The first two digits define a longitude band 0.5 degree wide and the second two digits a latitude band 0.5 degree wide."@en ;
    skos:inScheme cs: ;
    skos:notation "7476" ;
    skos:prefLabel "Cape York:7476"@en ;
.

geoad:Capella8551
    a skos:Concept ;
    skos:historyNote "Compiled by the Geological Survey of Queensland" ;
    skos:broader geoad:MapSeries ;
    skos:definition "Map sheet for Capella at 1:100 000 scale. The first two digits define a longitude band 0.5 degree wide and the second two digits a latitude band 0.5 degree wide."@en ;
    skos:inScheme cs: ;
    skos:notation "8551" ;
    skos:prefLabel "Capella:8551"@en ;
.

geoad:Carandotta6654
    a skos:Concept ;
    skos:historyNote "Compiled by the Geological Survey of Queensland" ;
    skos:broader geoad:MapSeries ;
    skos:definition "Map sheet for Carandotta at 1:100 000 scale. The first two digits define a longitude band 0.5 degree wide and the second two digits a latitude band 0.5 degree wide."@en ;
    skos:inScheme cs: ;
    skos:notation "6654" ;
    skos:prefLabel "Carandotta:6654"@en ;
.

geoad:Cardwell8161
    a skos:Concept ;
    skos:historyNote "Compiled by the Geological Survey of Queensland" ;
    skos:broader geoad:MapSeries ;
    skos:definition "Map sheet for Cardwell at 1:100 000 scale. The first two digits define a longitude band 0.5 degree wide and the second two digits a latitude band 0.5 degree wide."@en ;
    skos:inScheme cs: ;
    skos:notation "8161" ;
    skos:prefLabel "Cardwell:8161"@en ;
.

geoad:Carmila8754
    a skos:Concept ;
    skos:historyNote "Compiled by the Geological Survey of Queensland" ;
    skos:broader geoad:MapSeries ;
    skos:definition "Map sheet for Carmila at 1:100 000 scale. The first two digits define a longitude band 0.5 degree wide and the second two digits a latitude band 0.5 degree wide."@en ;
    skos:inScheme cs: ;
    skos:notation "8754" ;
    skos:prefLabel "Carmila:8754"@en ;
.

geoad:Carwell8248
    a skos:Concept ;
    skos:historyNote "Compiled by the Geological Survey of Queensland" ;
    skos:broader geoad:MapSeries ;
    skos:definition "Map sheet for Carwell at 1:100 000 scale. The first two digits define a longitude band 0.5 degree wide and the second two digits a latitude band 0.5 degree wide."@en ;
    skos:inScheme cs: ;
    skos:notation "8248" ;
    skos:prefLabel "Carwell:8248"@en ;
.

geoad:Cashmere7961
    a skos:Concept ;
    skos:historyNote "Compiled by the Geological Survey of Queensland" ;
    skos:broader geoad:MapSeries ;
    skos:definition "Map sheet for Cashmere at 1:100 000 scale. The first two digits define a longitude band 0.5 degree wide and the second two digits a latitude band 0.5 degree wide."@en ;
    skos:inScheme cs: ;
    skos:notation "7961" ;
    skos:prefLabel "Cashmere:7961"@en ;
.

geoad:Cassilis7555
    a skos:Concept ;
    skos:historyNote "Compiled by the Geological Survey of Queensland" ;
    skos:broader geoad:MapSeries ;
    skos:definition "Map sheet for Cassilis at 1:100 000 scale. The first two digits define a longitude band 0.5 degree wide and the second two digits a latitude band 0.5 degree wide."@en ;
    skos:inScheme cs: ;
    skos:notation "7555" ;
    skos:prefLabel "Cassilis:7555"@en ;
.

geoad:Cathua7248
    a skos:Concept ;
    skos:historyNote "Compiled by the Geological Survey of Queensland" ;
    skos:broader geoad:MapSeries ;
    skos:definition "Map sheet for Cathua at 1:100 000 scale. The first two digits define a longitude band 0.5 degree wide and the second two digits a latitude band 0.5 degree wide."@en ;
    skos:inScheme cs: ;
    skos:notation "7248" ;
    skos:prefLabel "Cathua:7248"@en ;
.

geoad:Charleville8145
    a skos:Concept ;
    skos:historyNote "Compiled by the Geological Survey of Queensland" ;
    skos:broader geoad:MapSeries ;
    skos:definition "Map sheet for Charleville at 1:100 000 scale. The first two digits define a longitude band 0.5 degree wide and the second two digits a latitude band 0.5 degree wide."@en ;
    skos:inScheme cs: ;
    skos:notation "8145" ;
    skos:prefLabel "Charleville:8145"@en ;
.

geoad:ChartersTowers8157
    a skos:Concept ;
    skos:historyNote "Compiled by the Geological Survey of Queensland" ;
    skos:broader geoad:MapSeries ;
    skos:definition "Map sheet for Charters Towers at 1:100 000 scale. The first two digits define a longitude band 0.5 degree wide and the second two digits a latitude band 0.5 degree wide."@en ;
    skos:inScheme cs: ;
    skos:notation "8157" ;
    skos:prefLabel "Charters Towers:8157"@en ;
.

geoad:Cheepie7944
    a skos:Concept ;
    skos:historyNote "Compiled by the Geological Survey of Queensland" ;
    skos:broader geoad:MapSeries ;
    skos:definition "Map sheet for Cheepie at 1:100 000 scale. The first two digits define a longitude band 0.5 degree wide and the second two digits a latitude band 0.5 degree wide."@en ;
    skos:inScheme cs: ;
    skos:notation "7944" ;
    skos:prefLabel "Cheepie:7944"@en ;
.

geoad:Cheshire8149
    a skos:Concept ;
    skos:historyNote "Compiled by the Geological Survey of Queensland" ;
    skos:broader geoad:MapSeries ;
    skos:definition "Map sheet for Cheshire at 1:100 000 scale. The first two digits define a longitude band 0.5 degree wide and the second two digits a latitude band 0.5 degree wide."@en ;
    skos:inScheme cs: ;
    skos:notation "8149" ;
    skos:prefLabel "Cheshire:8149"@en ;
.

geoad:Chesterton8347
    a skos:Concept ;
    skos:historyNote "Compiled by the Geological Survey of Queensland" ;
    skos:broader geoad:MapSeries ;
    skos:definition "Map sheet for Chesterton at 1:100 000 scale. The first two digits define a longitude band 0.5 degree wide and the second two digits a latitude band 0.5 degree wide."@en ;
    skos:inScheme cs: ;
    skos:notation "8347" ;
    skos:prefLabel "Chesterton:8347"@en ;
.

geoad:Childers9347
    a skos:Concept ;
    skos:historyNote "Compiled by the Geological Survey of Queensland" ;
    skos:broader geoad:MapSeries ;
    skos:definition "Map sheet for Childers at 1:100 000 scale. The first two digits define a longitude band 0.5 degree wide and the second two digits a latitude band 0.5 degree wide."@en ;
    skos:inScheme cs: ;
    skos:notation "9347" ;
    skos:prefLabel "Childers:9347"@en ;
.

geoad:Chillagoe7863
    a skos:Concept ;
    skos:historyNote "Compiled by the Geological Survey of Queensland" ;
    skos:broader geoad:MapSeries ;
    skos:definition "Map sheet for Chillagoe at 1:100 000 scale. The first two digits define a longitude band 0.5 degree wide and the second two digits a latitude band 0.5 degree wide."@en ;
    skos:inScheme cs: ;
    skos:notation "7863" ;
    skos:prefLabel "Chillagoe:7863"@en ;
.

geoad:Chinchilla9044
    a skos:Concept ;
    skos:historyNote "Compiled by the Geological Survey of Queensland" ;
    skos:broader geoad:MapSeries ;
    skos:definition "Map sheet for Chinchilla at 1:100 000 scale. The first two digits define a longitude band 0.5 degree wide and the second two digits a latitude band 0.5 degree wide."@en ;
    skos:inScheme cs: ;
    skos:notation "9044" ;
    skos:prefLabel "Chinchilla:9044"@en ;
.

geoad:ChristmasCreek6843
    a skos:Concept ;
    skos:historyNote "Compiled by the Geological Survey of Queensland" ;
    skos:broader geoad:MapSeries ;
    skos:definition "Map sheet for Christmas Creek at 1:100 000 scale. The first two digits define a longitude band 0.5 degree wide and the second two digits a latitude band 0.5 degree wide."@en ;
    skos:inScheme cs: ;
    skos:notation "6843" ;
    skos:prefLabel "Christmas Creek:6843"@en ;
.

geoad:ChudleighPark7758
    a skos:Concept ;
    skos:historyNote "Compiled by the Geological Survey of Queensland" ;
    skos:broader geoad:MapSeries ;
    skos:definition "Map sheet for Chudleigh Park at 1:100 000 scale. The first two digits define a longitude band 0.5 degree wide and the second two digits a latitude band 0.5 degree wide."@en ;
    skos:inScheme cs: ;
    skos:notation "7758" ;
    skos:prefLabel "Chudleigh Park:7758"@en ;
.

geoad:Claraville7260
    a skos:Concept ;
    skos:historyNote "Compiled by the Geological Survey of Queensland" ;
    skos:broader geoad:MapSeries ;
    skos:definition "Map sheet for Claraville at 1:100 000 scale. The first two digits define a longitude band 0.5 degree wide and the second two digits a latitude band 0.5 degree wide."@en ;
    skos:inScheme cs: ;
    skos:notation "7260" ;
    skos:prefLabel "Claraville:7260"@en ;
.

geoad:ClarkeRiver7959
    a skos:Concept ;
    skos:historyNote "Compiled by the Geological Survey of Queensland" ;
    skos:broader geoad:MapSeries ;
    skos:definition "Map sheet for Clarke River at 1:100 000 scale. The first two digits define a longitude band 0.5 degree wide and the second two digits a latitude band 0.5 degree wide."@en ;
    skos:inScheme cs: ;
    skos:notation "7959" ;
    skos:prefLabel "Clarke River:7959"@en ;
.

geoad:Clayton6539
    a skos:Concept ;
    skos:historyNote "Compiled by the Geological Survey of Queensland" ;
    skos:broader geoad:MapSeries ;
    skos:definition "Map sheet for Clayton at 1:100 000 scale. The first two digits define a longitude band 0.5 degree wide and the second two digits a latitude band 0.5 degree wide."@en ;
    skos:inScheme cs: ;
    skos:notation "6539" ;
    skos:prefLabel "Clayton:6539"@en ;
.

geoad:Clermont8452
    a skos:Concept ;
    skos:historyNote "Compiled by the Geological Survey of Queensland" ;
    skos:broader geoad:MapSeries ;
    skos:definition "Map sheet for Clermont at 1:100 000 scale. The first two digits define a longitude band 0.5 degree wide and the second two digits a latitude band 0.5 degree wide."@en ;
    skos:inScheme cs: ;
    skos:notation "8452" ;
    skos:prefLabel "Clermont:8452"@en ;
.

geoad:CliffdaleCreek6664
    a skos:Concept ;
    skos:historyNote "Compiled by the Geological Survey of Queensland" ;
    skos:broader geoad:MapSeries ;
    skos:definition "Map sheet for Cliffdale Creek at 1:100 000 scale. The first two digits define a longitude band 0.5 degree wide and the second two digits a latitude band 0.5 degree wide."@en ;
    skos:inScheme cs: ;
    skos:notation "6664" ;
    skos:prefLabel "Cliffdale Creek:6664"@en ;
.

geoad:Clive9239
    a skos:Concept ;
    skos:historyNote "Compiled by the Geological Survey of Queensland" ;
    skos:broader geoad:MapSeries ;
    skos:definition "Map sheet for Clive at 1:100 000 scale. The first two digits define a longitude band 0.5 degree wide and the second two digits a latitude band 0.5 degree wide."@en ;
    skos:inScheme cs: ;
    skos:notation "9239" ;
    skos:prefLabel "Clive:9239"@en ;
.

geoad:Clonagh7057
    a skos:Concept ;
    skos:historyNote "Compiled by the Geological Survey of Queensland" ;
    skos:broader geoad:MapSeries ;
    skos:definition "Map sheet for Clonagh at 1:100 000 scale. The first two digits define a longitude band 0.5 degree wide and the second two digits a latitude band 0.5 degree wide."@en ;
    skos:inScheme cs: ;
    skos:notation "7057" ;
    skos:prefLabel "Clonagh:7057"@en ;
.

geoad:Cloncurry7056
    a skos:Concept ;
    skos:historyNote "Compiled by the Geological Survey of Queensland" ;
    skos:broader geoad:MapSeries ;
    skos:definition "Map sheet for Cloncurry at 1:100 000 scale. The first two digits define a longitude band 0.5 degree wide and the second two digits a latitude band 0.5 degree wide."@en ;
    skos:inScheme cs: ;
    skos:notation "7056" ;
    skos:prefLabel "Cloncurry:7056"@en ;
.

geoad:Coalbrook7557
    a skos:Concept ;
    skos:historyNote "Compiled by the Geological Survey of Queensland" ;
    skos:broader geoad:MapSeries ;
    skos:definition "Map sheet for Coalbrook at 1:100 000 scale. The first two digits define a longitude band 0.5 degree wide and the second two digits a latitude band 0.5 degree wide."@en ;
    skos:inScheme cs: ;
    skos:notation "7557" ;
    skos:prefLabel "Coalbrook:7557"@en ;
.

geoad:Coaldale9439
    a skos:Concept ;
    skos:historyNote "Compiled by the Geological Survey of Queensland" ;
    skos:broader geoad:MapSeries ;
    skos:definition "Map sheet for Coaldale at 1:100 000 scale. The first two digits define a longitude band 0.5 degree wide and the second two digits a latitude band 0.5 degree wide."@en ;
    skos:inScheme cs: ;
    skos:notation "9439" ;
    skos:prefLabel "Coaldale:9439"@en ;
.

geoad:CoconutIsland7577
    a skos:Concept ;
    skos:historyNote "Compiled by the Geological Survey of Queensland" ;
    skos:broader geoad:MapSeries ;
    skos:definition "Map sheet for Coconut Island at 1:100 000 scale. The first two digits define a longitude band 0.5 degree wide and the second two digits a latitude band 0.5 degree wide."@en ;
    skos:inScheme cs: ;
    skos:notation "7577" ;
    skos:prefLabel "Coconut Island:7577"@en ;
.

geoad:Coen7570
    a skos:Concept ;
    skos:historyNote "Compiled by the Geological Survey of Queensland" ;
    skos:broader geoad:MapSeries ;
    skos:definition "Map sheet for Coen at 1:100 000 scale. The first two digits define a longitude band 0.5 degree wide and the second two digits a latitude band 0.5 degree wide."@en ;
    skos:inScheme cs: ;
    skos:notation "7570" ;
    skos:prefLabel "Coen:7570"@en ;
.

geoad:Cogoon8643
    a skos:Concept ;
    skos:historyNote "Compiled by the Geological Survey of Queensland" ;
    skos:broader geoad:MapSeries ;
    skos:definition "Map sheet for Cogoon at 1:100 000 scale. The first two digits define a longitude band 0.5 degree wide and the second two digits a latitude band 0.5 degree wide."@en ;
    skos:inScheme cs: ;
    skos:notation "8643" ;
    skos:prefLabel "Cogoon:8643"@en ;
.

geoad:Collabara7847
    a skos:Concept ;
    skos:historyNote "Compiled by the Geological Survey of Queensland" ;
    skos:broader geoad:MapSeries ;
    skos:definition "Map sheet for Collabara at 1:100 000 scale. The first two digits define a longitude band 0.5 degree wide and the second two digits a latitude band 0.5 degree wide."@en ;
    skos:inScheme cs: ;
    skos:notation "7847" ;
    skos:prefLabel "Collabara:7847"@en ;
.

geoad:Collinsville8456
    a skos:Concept ;
    skos:historyNote "Compiled by the Geological Survey of Queensland" ;
    skos:broader geoad:MapSeries ;
    skos:definition "Map sheet for Collinsville at 1:100 000 scale. The first two digits define a longitude band 0.5 degree wide and the second two digits a latitude band 0.5 degree wide."@en ;
    skos:inScheme cs: ;
    skos:notation "8456" ;
    skos:prefLabel "Collinsville:8456"@en ;
.

geoad:Comet8650
    a skos:Concept ;
    skos:historyNote "Compiled by the Geological Survey of Queensland" ;
    skos:broader geoad:MapSeries ;
    skos:definition "Map sheet for Comet at 1:100 000 scale. The first two digits define a longitude band 0.5 degree wide and the second two digits a latitude band 0.5 degree wide."@en ;
    skos:inScheme cs: ;
    skos:notation "8650" ;
    skos:prefLabel "Comet:8650"@en ;
.

geoad:Congie7644
    a skos:Concept ;
    skos:historyNote "Compiled by the Geological Survey of Queensland" ;
    skos:broader geoad:MapSeries ;
    skos:definition "Map sheet for Congie at 1:100 000 scale. The first two digits define a longitude band 0.5 degree wide and the second two digits a latitude band 0.5 degree wide."@en ;
    skos:inScheme cs: ;
    skos:notation "7644" ;
    skos:prefLabel "Congie:7644"@en ;
.

geoad:Conjuboy7860
    a skos:Concept ;
    skos:historyNote "Compiled by the Geological Survey of Queensland" ;
    skos:broader geoad:MapSeries ;
    skos:definition "Map sheet for Conjuboy at 1:100 000 scale. The first two digits define a longitude band 0.5 degree wide and the second two digits a latitude band 0.5 degree wide."@en ;
    skos:inScheme cs: ;
    skos:notation "7860" ;
    skos:prefLabel "Conjuboy:7860"@en ;
.

geoad:Connemara7349
    a skos:Concept ;
    skos:historyNote "Compiled by the Geological Survey of Queensland" ;
    skos:broader geoad:MapSeries ;
    skos:definition "Map sheet for Connemara at 1:100 000 scale. The first two digits define a longitude band 0.5 degree wide and the second two digits a latitude band 0.5 degree wide."@en ;
    skos:inScheme cs: ;
    skos:notation "7349" ;
    skos:prefLabel "Connemara:7349"@en ;
.

geoad:ConnorsRange8753
    a skos:Concept ;
    skos:historyNote "Compiled by the Geological Survey of Queensland" ;
    skos:broader geoad:MapSeries ;
    skos:definition "Map sheet for Connors Range at 1:100 000 scale. The first two digits define a longitude band 0.5 degree wide and the second two digits a latitude band 0.5 degree wide."@en ;
    skos:inScheme cs: ;
    skos:notation "8753" ;
    skos:prefLabel "Connors Range:8753"@en ;
.

geoad:Consuelo8548
    a skos:Concept ;
    skos:historyNote "Compiled by the Geological Survey of Queensland" ;
    skos:broader geoad:MapSeries ;
    skos:definition "Map sheet for Consuelo at 1:100 000 scale. The first two digits define a longitude band 0.5 degree wide and the second two digits a latitude band 0.5 degree wide."@en ;
    skos:inScheme cs: ;
    skos:notation "8548" ;
    skos:prefLabel "Consuelo:8548"@en ;
.

geoad:Cooktown7967
    a skos:Concept ;
    skos:historyNote "Compiled by the Geological Survey of Queensland" ;
    skos:broader geoad:MapSeries ;
    skos:definition "Map sheet for Cooktown at 1:100 000 scale. The first two digits define a longitude band 0.5 degree wide and the second two digits a latitude band 0.5 degree wide."@en ;
    skos:inScheme cs: ;
    skos:notation "7967" ;
    skos:prefLabel "Cooktown:7967"@en ;
.

geoad:Coolullah6958
    a skos:Concept ;
    skos:historyNote "Compiled by the Geological Survey of Queensland" ;
    skos:broader geoad:MapSeries ;
    skos:definition "Map sheet for Coolullah at 1:100 000 scale. The first two digits define a longitude band 0.5 degree wide and the second two digits a latitude band 0.5 degree wide."@en ;
    skos:inScheme cs: ;
    skos:notation "6958" ;
    skos:prefLabel "Coolullah:6958"@en ;
.

geoad:Coomburra8340
    a skos:Concept ;
    skos:historyNote "Compiled by the Geological Survey of Queensland" ;
    skos:broader geoad:MapSeries ;
    skos:definition "Map sheet for Coomburra at 1:100 000 scale. The first two digits define a longitude band 0.5 degree wide and the second two digits a latitude band 0.5 degree wide."@en ;
    skos:inScheme cs: ;
    skos:notation "8340" ;
    skos:prefLabel "Coomburra:8340"@en ;
.

geoad:Coongie6943
    a skos:Concept ;
    skos:historyNote "Compiled by the Geological Survey of Queensland" ;
    skos:broader geoad:MapSeries ;
    skos:definition "Map sheet for Coongie at 1:100 000 scale. The first two digits define a longitude band 0.5 degree wide and the second two digits a latitude band 0.5 degree wide."@en ;
    skos:inScheme cs: ;
    skos:notation "6943" ;
    skos:prefLabel "Coongie:6943"@en ;
.

geoad:Coongoola8042
    a skos:Concept ;
    skos:historyNote "Compiled by the Geological Survey of Queensland" ;
    skos:broader geoad:MapSeries ;
    skos:definition "Map sheet for Coongoola at 1:100 000 scale. The first two digits define a longitude band 0.5 degree wide and the second two digits a latitude band 0.5 degree wide."@en ;
    skos:inScheme cs: ;
    skos:notation "8042" ;
    skos:prefLabel "Coongoola:8042"@en ;
.

geoad:CooperPoint8163
    a skos:Concept ;
    skos:historyNote "Compiled by the Geological Survey of Queensland" ;
    skos:broader geoad:MapSeries ;
    skos:definition "Map sheet for Cooper Point at 1:100 000 scale. The first two digits define a longitude band 0.5 degree wide and the second two digits a latitude band 0.5 degree wide."@en ;
    skos:inScheme cs: ;
    skos:notation "8163" ;
    skos:prefLabel "Cooper Point:8163"@en ;
.

geoad:Coorabulka6950
    a skos:Concept ;
    skos:historyNote "Compiled by the Geological Survey of Queensland" ;
    skos:broader geoad:MapSeries ;
    skos:definition "Map sheet for Coorabulka at 1:100 000 scale. The first two digits define a longitude band 0.5 degree wide and the second two digits a latitude band 0.5 degree wide."@en ;
    skos:inScheme cs: ;
    skos:notation "6950" ;
    skos:prefLabel "Coorabulka:6950"@en ;
.

geoad:Cooroorah8651
    a skos:Concept ;
    skos:historyNote "Compiled by the Geological Survey of Queensland" ;
    skos:broader geoad:MapSeries ;
    skos:definition "Map sheet for Cooroorah at 1:100 000 scale. The first two digits define a longitude band 0.5 degree wide and the second two digits a latitude band 0.5 degree wide."@en ;
    skos:inScheme cs: ;
    skos:notation "8651" ;
    skos:prefLabel "Cooroorah:8651"@en ;
.

geoad:Cooryanna6639
    a skos:Concept ;
    skos:historyNote "Compiled by the Geological Survey of Queensland" ;
    skos:broader geoad:MapSeries ;
    skos:definition "Map sheet for Cooryanna at 1:100 000 scale. The first two digits define a longitude band 0.5 degree wide and the second two digits a latitude band 0.5 degree wide."@en ;
    skos:inScheme cs: ;
    skos:notation "6639" ;
    skos:prefLabel "Cooryanna:6639"@en ;
.

geoad:Coralie7261
    a skos:Concept ;
    skos:historyNote "Compiled by the Geological Survey of Queensland" ;
    skos:broader geoad:MapSeries ;
    skos:definition "Map sheet for Coralie at 1:100 000 scale. The first two digits define a longitude band 0.5 degree wide and the second two digits a latitude band 0.5 degree wide."@en ;
    skos:inScheme cs: ;
    skos:notation "7261" ;
    skos:prefLabel "Coralie:7261"@en ;
.

geoad:Cordillo7044
    a skos:Concept ;
    skos:historyNote "Compiled by the Geological Survey of Queensland" ;
    skos:broader geoad:MapSeries ;
    skos:definition "Map sheet for Cordillo at 1:100 000 scale. The first two digits define a longitude band 0.5 degree wide and the second two digits a latitude band 0.5 degree wide."@en ;
    skos:inScheme cs: ;
    skos:notation "7044" ;
    skos:prefLabel "Cordillo:7044"@en ;
.

geoad:Cotherstone8552
    a skos:Concept ;
    skos:historyNote "Compiled by the Geological Survey of Queensland" ;
    skos:broader geoad:MapSeries ;
    skos:definition "Map sheet for Cotherstone at 1:100 000 scale. The first two digits define a longitude band 0.5 degree wide and the second two digits a latitude band 0.5 degree wide."@en ;
    skos:inScheme cs: ;
    skos:notation "8552" ;
    skos:prefLabel "Cotherstone:8552"@en ;
.

geoad:Cowarie6542
    a skos:Concept ;
    skos:historyNote "Compiled by the Geological Survey of Queensland" ;
    skos:broader geoad:MapSeries ;
    skos:definition "Map sheet for Cowarie at 1:100 000 scale. The first two digits define a longitude band 0.5 degree wide and the second two digits a latitude band 0.5 degree wide."@en ;
    skos:inScheme cs: ;
    skos:notation "6542" ;
    skos:prefLabel "Cowarie:6542"@en ;
.

geoad:Cracow8947
    a skos:Concept ;
    skos:historyNote "Compiled by the Geological Survey of Queensland" ;
    skos:broader geoad:MapSeries ;
    skos:definition "Map sheet for Cracow at 1:100 000 scale. The first two digits define a longitude band 0.5 degree wide and the second two digits a latitude band 0.5 degree wide."@en ;
    skos:inScheme cs: ;
    skos:notation "8947" ;
    skos:prefLabel "Cracow:8947"@en ;
.

geoad:CrookedCreek7463
    a skos:Concept ;
    skos:historyNote "Compiled by the Geological Survey of Queensland" ;
    skos:broader geoad:MapSeries ;
    skos:definition "Map sheet for Crooked Creek at 1:100 000 scale. The first two digits define a longitude band 0.5 degree wide and the second two digits a latitude band 0.5 degree wide."@en ;
    skos:inScheme cs: ;
    skos:notation "7463" ;
    skos:prefLabel "Crooked Creek:7463"@en ;
.

geoad:CroppaCreek8939
    a skos:Concept ;
    skos:historyNote "Compiled by the Geological Survey of Queensland" ;
    skos:broader geoad:MapSeries ;
    skos:definition "Map sheet for Croppa Creek at 1:100 000 scale. The first two digits define a longitude band 0.5 degree wide and the second two digits a latitude band 0.5 degree wide."@en ;
    skos:inScheme cs: ;
    skos:notation "8939" ;
    skos:prefLabel "Croppa Creek:8939"@en ;
.

geoad:CrosbieCreek7467
    a skos:Concept ;
    skos:historyNote "Compiled by the Geological Survey of Queensland" ;
    skos:broader geoad:MapSeries ;
    skos:definition "Map sheet for Crosbie Creek at 1:100 000 scale. The first two digits define a longitude band 0.5 degree wide and the second two digits a latitude band 0.5 degree wide."@en ;
    skos:inScheme cs: ;
    skos:notation "7467" ;
    skos:prefLabel "Crosbie Creek:7467"@en ;
.

geoad:Croydon7361
    a skos:Concept ;
    skos:historyNote "Compiled by the Geological Survey of Queensland" ;
    skos:broader geoad:MapSeries ;
    skos:definition "Map sheet for Croydon at 1:100 000 scale. The first two digits define a longitude band 0.5 degree wide and the second two digits a latitude band 0.5 degree wide."@en ;
    skos:inScheme cs: ;
    skos:notation "7361" ;
    skos:prefLabel "Croydon:7361"@en ;
.

geoad:Culloden7753
    a skos:Concept ;
    skos:historyNote "Compiled by the Geological Survey of Queensland" ;
    skos:broader geoad:MapSeries ;
    skos:definition "Map sheet for Culloden at 1:100 000 scale. The first two digits define a longitude band 0.5 degree wide and the second two digits a latitude band 0.5 degree wide."@en ;
    skos:inScheme cs: ;
    skos:notation "7753" ;
    skos:prefLabel "Culloden:7753"@en ;
.

geoad:CumberlandIslands8756
    a skos:Concept ;
    skos:historyNote "Compiled by the Geological Survey of Queensland" ;
    skos:broader geoad:MapSeries ;
    skos:definition "Map sheet for Cumberland Islands at 1:100 000 scale. The first two digits define a longitude band 0.5 degree wide and the second two digits a latitude band 0.5 degree wide."@en ;
    skos:inScheme cs: ;
    skos:notation "8756" ;
    skos:prefLabel "Cumberland Islands:8756"@en ;
.

geoad:Cungelella8348
    a skos:Concept ;
    skos:historyNote "Compiled by the Geological Survey of Queensland" ;
    skos:broader geoad:MapSeries ;
    skos:definition "Map sheet for Cungelella at 1:100 000 scale. The first two digits define a longitude band 0.5 degree wide and the second two digits a latitude band 0.5 degree wide."@en ;
    skos:inScheme cs: ;
    skos:notation "8348" ;
    skos:prefLabel "Cungelella:8348"@en ;
.

geoad:Cunnamulla8041
    a skos:Concept ;
    skos:historyNote "Compiled by the Geological Survey of Queensland" ;
    skos:broader geoad:MapSeries ;
    skos:definition "Map sheet for Cunnamulla at 1:100 000 scale. The first two digits define a longitude band 0.5 degree wide and the second two digits a latitude band 0.5 degree wide."@en ;
    skos:inScheme cs: ;
    skos:notation "8041" ;
    skos:prefLabel "Cunnamulla:8041"@en ;
.

geoad:CurlewIsland8854
    a skos:Concept ;
    skos:historyNote "Compiled by the Geological Survey of Queensland" ;
    skos:broader geoad:MapSeries ;
    skos:definition "Map sheet for Curlew Island at 1:100 000 scale. The first two digits define a longitude band 0.5 degree wide and the second two digits a latitude band 0.5 degree wide."@en ;
    skos:inScheme cs: ;
    skos:notation "8854" ;
    skos:prefLabel "Curlew Island:8854"@en ;
.

geoad:Currawilla7147
    a skos:Concept ;
    skos:historyNote "Compiled by the Geological Survey of Queensland" ;
    skos:broader geoad:MapSeries ;
    skos:definition "Map sheet for Currawilla at 1:100 000 scale. The first two digits define a longitude band 0.5 degree wide and the second two digits a latitude band 0.5 degree wide."@en ;
    skos:inScheme cs: ;
    skos:notation "7147" ;
    skos:prefLabel "Currawilla:7147"@en ;
.

geoad:Dagworth7354
    a skos:Concept ;
    skos:historyNote "Compiled by the Geological Survey of Queensland" ;
    skos:broader geoad:MapSeries ;
    skos:definition "Map sheet for Dagworth at 1:100 000 scale. The first two digits define a longitude band 0.5 degree wide and the second two digits a latitude band 0.5 degree wide."@en ;
    skos:inScheme cs: ;
    skos:notation "7354" ;
    skos:prefLabel "Dagworth:7354"@en ;
.

geoad:Dajarra6854
    a skos:Concept ;
    skos:historyNote "Compiled by the Geological Survey of Queensland" ;
    skos:broader geoad:MapSeries ;
    skos:definition "Map sheet for Dajarra at 1:100 000 scale. The first two digits define a longitude band 0.5 degree wide and the second two digits a latitude band 0.5 degree wide."@en ;
    skos:inScheme cs: ;
    skos:notation "6854" ;
    skos:prefLabel "Dajarra:6854"@en ;
.

geoad:Dalby9143
    a skos:Concept ;
    skos:historyNote "Compiled by the Geological Survey of Queensland" ;
    skos:broader geoad:MapSeries ;
    skos:definition "Map sheet for Dalby at 1:100 000 scale. The first two digits define a longitude band 0.5 degree wide and the second two digits a latitude band 0.5 degree wide."@en ;
    skos:inScheme cs: ;
    skos:notation "9143" ;
    skos:prefLabel "Dalby:9143"@en ;
.

geoad:Dalgonally7157
    a skos:Concept ;
    skos:historyNote "Compiled by the Geological Survey of Queensland" ;
    skos:broader geoad:MapSeries ;
    skos:definition "Map sheet for Dalgonally at 1:100 000 scale. The first two digits define a longitude band 0.5 degree wide and the second two digits a latitude band 0.5 degree wide."@en ;
    skos:inScheme cs: ;
    skos:notation "7157" ;
    skos:prefLabel "Dalgonally:7157"@en ;
.

geoad:Daralingie6941
    a skos:Concept ;
    skos:historyNote "Compiled by the Geological Survey of Queensland" ;
    skos:broader geoad:MapSeries ;
    skos:definition "Map sheet for Daralingie at 1:100 000 scale. The first two digits define a longitude band 0.5 degree wide and the second two digits a latitude band 0.5 degree wide."@en ;
    skos:inScheme cs: ;
    skos:notation "6941" ;
    skos:prefLabel "Daralingie:6941"@en ;
.

geoad:DarnleyIsland7678
    a skos:Concept ;
    skos:historyNote "Compiled by the Geological Survey of Queensland" ;
    skos:broader geoad:MapSeries ;
    skos:definition "Map sheet for Darnley Island at 1:100 000 scale. The first two digits define a longitude band 0.5 degree wide and the second two digits a latitude band 0.5 degree wide."@en ;
    skos:inScheme cs: ;
    skos:notation "7678" ;
    skos:prefLabel "Darnley Island:7678"@en ;
.

geoad:Daru7579
    a skos:Concept ;
    skos:historyNote "Compiled by the Geological Survey of Queensland" ;
    skos:broader geoad:MapSeries ;
    skos:definition "Map sheet for Daru at 1:100 000 scale. The first two digits define a longitude band 0.5 degree wide and the second two digits a latitude band 0.5 degree wide."@en ;
    skos:inScheme cs: ;
    skos:notation "7579" ;
    skos:prefLabel "Daru:7579"@en ;
.

geoad:DavenportDowns7149
    a skos:Concept ;
    skos:historyNote "Compiled by the Geological Survey of Queensland" ;
    skos:broader geoad:MapSeries ;
    skos:definition "Map sheet for Davenport Downs at 1:100 000 scale. The first two digits define a longitude band 0.5 degree wide and the second two digits a latitude band 0.5 degree wide."@en ;
    skos:inScheme cs: ;
    skos:notation "7149" ;
    skos:prefLabel "Davenport Downs:7149"@en ;
.

geoad:DeliveranceIsland7278
    a skos:Concept ;
    skos:historyNote "Compiled by the Geological Survey of Queensland" ;
    skos:broader geoad:MapSeries ;
    skos:definition "Map sheet for Deliverance Island at 1:100 000 scale. The first two digits define a longitude band 0.5 degree wide and the second two digits a latitude band 0.5 degree wide."@en ;
    skos:inScheme cs: ;
    skos:notation "7278" ;
    skos:prefLabel "Deliverance Island:7278"@en ;
.

geoad:Diamantina6744
    a skos:Concept ;
    skos:historyNote "Compiled by the Geological Survey of Queensland" ;
    skos:broader geoad:MapSeries ;
    skos:definition "Map sheet for Diamantina at 1:100 000 scale. The first two digits define a longitude band 0.5 degree wide and the second two digits a latitude band 0.5 degree wide."@en ;
    skos:inScheme cs: ;
    skos:notation "6744" ;
    skos:prefLabel "Diamantina:6744"@en ;
.

geoad:DiamantinaLakes7150
    a skos:Concept ;
    skos:historyNote "Compiled by the Geological Survey of Queensland" ;
    skos:broader geoad:MapSeries ;
    skos:definition "Map sheet for Diamantina Lakes at 1:100 000 scale. The first two digits define a longitude band 0.5 degree wide and the second two digits a latitude band 0.5 degree wide."@en ;
    skos:inScheme cs: ;
    skos:notation "7150" ;
    skos:prefLabel "Diamantina Lakes:7150"@en ;
.

geoad:DiamondBog6841
    a skos:Concept ;
    skos:historyNote "Compiled by the Geological Survey of Queensland" ;
    skos:broader geoad:MapSeries ;
    skos:definition "Map sheet for Diamond Bog at 1:100 000 scale. The first two digits define a longitude band 0.5 degree wide and the second two digits a latitude band 0.5 degree wide."@en ;
    skos:inScheme cs: ;
    skos:notation "6841" ;
    skos:prefLabel "Diamond Bog:6841"@en ;
.

geoad:DigbyPeaks6953
    a skos:Concept ;
    skos:historyNote "Compiled by the Geological Survey of Queensland" ;
    skos:broader geoad:MapSeries ;
    skos:definition "Map sheet for Digby Peaks at 1:100 000 scale. The first two digits define a longitude band 0.5 degree wide and the second two digits a latitude band 0.5 degree wide."@en ;
    skos:inScheme cs: ;
    skos:notation "6953" ;
    skos:prefLabel "Digby Peaks:6953"@en ;
.

geoad:DinahIsland7165
    a skos:Concept ;
    skos:historyNote "Compiled by the Geological Survey of Queensland" ;
    skos:broader geoad:MapSeries ;
    skos:definition "Map sheet for Dinah Island at 1:100 000 scale. The first two digits define a longitude band 0.5 degree wide and the second two digits a latitude band 0.5 degree wide."@en ;
    skos:inScheme cs: ;
    skos:notation "7165" ;
    skos:prefLabel "Dinah Island:7165"@en ;
.

geoad:Dingo8750
    a skos:Concept ;
    skos:historyNote "Compiled by the Geological Survey of Queensland" ;
    skos:broader geoad:MapSeries ;
    skos:definition "Map sheet for Dingo at 1:100 000 scale. The first two digits define a longitude band 0.5 degree wide and the second two digits a latitude band 0.5 degree wide."@en ;
    skos:inScheme cs: ;
    skos:notation "8750" ;
    skos:prefLabel "Dingo:8750"@en ;
.

geoad:Dirranbandi8540
    a skos:Concept ;
    skos:historyNote "Compiled by the Geological Survey of Queensland" ;
    skos:broader geoad:MapSeries ;
    skos:definition "Map sheet for Dirranbandi at 1:100 000 scale. The first two digits define a longitude band 0.5 degree wide and the second two digits a latitude band 0.5 degree wide."@en ;
    skos:inScheme cs: ;
    skos:notation "8540" ;
    skos:prefLabel "Dirranbandi:8540"@en ;
.

geoad:Dixie7567
    a skos:Concept ;
    skos:historyNote "Compiled by the Geological Survey of Queensland" ;
    skos:broader geoad:MapSeries ;
    skos:definition "Map sheet for Dixie at 1:100 000 scale. The first two digits define a longitude band 0.5 degree wide and the second two digits a latitude band 0.5 degree wide."@en ;
    skos:inScheme cs: ;
    skos:notation "7567" ;
    skos:prefLabel "Dixie:7567"@en ;
.

geoad:DonorsHill7060
    a skos:Concept ;
    skos:historyNote "Compiled by the Geological Survey of Queensland" ;
    skos:broader geoad:MapSeries ;
    skos:definition "Map sheet for Donors Hill at 1:100 000 scale. The first two digits define a longitude band 0.5 degree wide and the second two digits a latitude band 0.5 degree wide."@en ;
    skos:inScheme cs: ;
    skos:notation "7060" ;
    skos:prefLabel "Donors Hill:7060"@en ;
.

geoad:Doomadgee6662
    a skos:Concept ;
    skos:historyNote "Compiled by the Geological Survey of Queensland" ;
    skos:broader geoad:MapSeries ;
    skos:definition "Map sheet for Doomadgee at 1:100 000 scale. The first two digits define a longitude band 0.5 degree wide and the second two digits a latitude band 0.5 degree wide."@en ;
    skos:inScheme cs: ;
    skos:notation "6662" ;
    skos:prefLabel "Doomadgee:6662"@en ;
.

geoad:Dotswood8158
    a skos:Concept ;
    skos:historyNote "Compiled by the Geological Survey of Queensland" ;
    skos:broader geoad:MapSeries ;
    skos:definition "Map sheet for Dotswood at 1:100 000 scale. The first two digits define a longitude band 0.5 degree wide and the second two digits a latitude band 0.5 degree wide."@en ;
    skos:inScheme cs: ;
    skos:notation "8158" ;
    skos:prefLabel "Dotswood:8158"@en ;
.

geoad:DoubleLagoon7163
    a skos:Concept ;
    skos:historyNote "Compiled by the Geological Survey of Queensland" ;
    skos:broader geoad:MapSeries ;
    skos:definition "Map sheet for Double Lagoon at 1:100 000 scale. The first two digits define a longitude band 0.5 degree wide and the second two digits a latitude band 0.5 degree wide."@en ;
    skos:inScheme cs: ;
    skos:notation "7163" ;
    skos:prefLabel "Double Lagoon:7163"@en ;
.

geoad:Drake9340
    a skos:Concept ;
    skos:historyNote "Compiled by the Geological Survey of Queensland" ;
    skos:broader geoad:MapSeries ;
    skos:definition "Map sheet for Drake at 1:100 000 scale. The first two digits define a longitude band 0.5 degree wide and the second two digits a latitude band 0.5 degree wide."@en ;
    skos:inScheme cs: ;
    skos:notation "9340" ;
    skos:prefLabel "Drake:9340"@en ;
.

geoad:Duaringa8850
    a skos:Concept ;
    skos:historyNote "Compiled by the Geological Survey of Queensland" ;
    skos:broader geoad:MapSeries ;
    skos:definition "Map sheet for Duaringa at 1:100 000 scale. The first two digits define a longitude band 0.5 degree wide and the second two digits a latitude band 0.5 degree wide."@en ;
    skos:inScheme cs: ;
    skos:notation "8850" ;
    skos:prefLabel "Duaringa:8850"@en ;
.

geoad:Duchess6855
    a skos:Concept ;
    skos:historyNote "Compiled by the Geological Survey of Queensland" ;
    skos:broader geoad:MapSeries ;
    skos:definition "Map sheet for Duchess at 1:100 000 scale. The first two digits define a longitude band 0.5 degree wide and the second two digits a latitude band 0.5 degree wide."@en ;
    skos:inScheme cs: ;
    skos:notation "6855" ;
    skos:prefLabel "Duchess:6855"@en ;
.

geoad:Dulacca8844
    a skos:Concept ;
    skos:historyNote "Compiled by the Geological Survey of Queensland" ;
    skos:broader geoad:MapSeries ;
    skos:definition "Map sheet for Dulacca at 1:100 000 scale. The first two digits define a longitude band 0.5 degree wide and the second two digits a latitude band 0.5 degree wide."@en ;
    skos:inScheme cs: ;
    skos:notation "8844" ;
    skos:prefLabel "Dulacca:8844"@en ;
.

geoad:Dullingari7041
    a skos:Concept ;
    skos:historyNote "Compiled by the Geological Survey of Queensland" ;
    skos:broader geoad:MapSeries ;
    skos:definition "Map sheet for Dullingari at 1:100 000 scale. The first two digits define a longitude band 0.5 degree wide and the second two digits a latitude band 0.5 degree wide."@en ;
    skos:inScheme cs: ;
    skos:notation "7041" ;
    skos:prefLabel "Dullingari:7041"@en ;
.

geoad:Dunbar7365
    a skos:Concept ;
    skos:historyNote "Compiled by the Geological Survey of Queensland" ;
    skos:broader geoad:MapSeries ;
    skos:definition "Map sheet for Dunbar at 1:100 000 scale. The first two digits define a longitude band 0.5 degree wide and the second two digits a latitude band 0.5 degree wide."@en ;
    skos:inScheme cs: ;
    skos:notation "7365" ;
    skos:prefLabel "Dunbar:7365"@en ;
.

geoad:Dundoo7842
    a skos:Concept ;
    skos:historyNote "Compiled by the Geological Survey of Queensland" ;
    skos:broader geoad:MapSeries ;
    skos:definition "Map sheet for Dundoo at 1:100 000 scale. The first two digits define a longitude band 0.5 degree wide and the second two digits a latitude band 0.5 degree wide."@en ;
    skos:inScheme cs: ;
    skos:notation "7842" ;
    skos:prefLabel "Dundoo:7842"@en ;
.

geoad:Dunrobin8152
    a skos:Concept ;
    skos:historyNote "Compiled by the Geological Survey of Queensland" ;
    skos:broader geoad:MapSeries ;
    skos:definition "Map sheet for Dunrobin at 1:100 000 scale. The first two digits define a longitude band 0.5 degree wide and the second two digits a latitude band 0.5 degree wide."@en ;
    skos:inScheme cs: ;
    skos:notation "8152" ;
    skos:prefLabel "Dunrobin:8152"@en ;
.

geoad:Dunumbral8539
    a skos:Concept ;
    skos:historyNote "Compiled by the Geological Survey of Queensland" ;
    skos:broader geoad:MapSeries ;
    skos:definition "Map sheet for Dunumbral at 1:100 000 scale. The first two digits define a longitude band 0.5 degree wide and the second two digits a latitude band 0.5 degree wide."@en ;
    skos:inScheme cs: ;
    skos:notation "8539" ;
    skos:prefLabel "Dunumbral:8539"@en ;
.

geoad:DurhamDowns7243
    a skos:Concept ;
    skos:historyNote "Compiled by the Geological Survey of Queensland" ;
    skos:broader geoad:MapSeries ;
    skos:definition "Map sheet for Durham Downs at 1:100 000 scale. The first two digits define a longitude band 0.5 degree wide and the second two digits a latitude band 0.5 degree wide."@en ;
    skos:inScheme cs: ;
    skos:notation "7243" ;
    skos:prefLabel "Durham Downs:7243"@en ;
.

geoad:Durrie6946
    a skos:Concept ;
    skos:historyNote "Compiled by the Geological Survey of Queensland" ;
    skos:broader geoad:MapSeries ;
    skos:definition "Map sheet for Durrie at 1:100 000 scale. The first two digits define a longitude band 0.5 degree wide and the second two digits a latitude band 0.5 degree wide."@en ;
    skos:inScheme cs: ;
    skos:notation "6946" ;
    skos:prefLabel "Durrie:6946"@en ;
.

geoad:DuttonRiver7657
    a skos:Concept ;
    skos:historyNote "Compiled by the Geological Survey of Queensland" ;
    skos:broader geoad:MapSeries ;
    skos:definition "Map sheet for Dutton River at 1:100 000 scale. The first two digits define a longitude band 0.5 degree wide and the second two digits a latitude band 0.5 degree wide."@en ;
    skos:inScheme cs: ;
    skos:notation "7657" ;
    skos:prefLabel "Dutton River:7657"@en ;
.

geoad:DynevorDowns7741
    a skos:Concept ;
    skos:historyNote "Compiled by the Geological Survey of Queensland" ;
    skos:broader geoad:MapSeries ;
    skos:definition "Map sheet for Dynevor Downs at 1:100 000 scale. The first two digits define a longitude band 0.5 degree wide and the second two digits a latitude band 0.5 degree wide."@en ;
    skos:inScheme cs: ;
    skos:notation "7741" ;
    skos:prefLabel "Dynevor Downs:7741"@en ;
.

geoad:Ebagoola7569
    a skos:Concept ;
    skos:historyNote "Compiled by the Geological Survey of Queensland" ;
    skos:broader geoad:MapSeries ;
    skos:definition "Map sheet for Ebagoola at 1:100 000 scale. The first two digits define a longitude band 0.5 degree wide and the second two digits a latitude band 0.5 degree wide."@en ;
    skos:inScheme cs: ;
    skos:notation "7569" ;
    skos:prefLabel "Ebagoola:7569"@en ;
.

geoad:EchoCreek7363
    a skos:Concept ;
    skos:historyNote "Compiled by the Geological Survey of Queensland" ;
    skos:broader geoad:MapSeries ;
    skos:definition "Map sheet for Echo Creek at 1:100 000 scale. The first two digits define a longitude band 0.5 degree wide and the second two digits a latitude band 0.5 degree wide."@en ;
    skos:inScheme cs: ;
    skos:notation "7363" ;
    skos:prefLabel "Echo Creek:7363"@en ;
.

geoad:EdwardRiver7268
    a skos:Concept ;
    skos:historyNote "Compiled by the Geological Survey of Queensland" ;
    skos:broader geoad:MapSeries ;
    skos:definition "Map sheet for Edward River at 1:100 000 scale. The first two digits define a longitude band 0.5 degree wide and the second two digits a latitude band 0.5 degree wide."@en ;
    skos:inScheme cs: ;
    skos:notation "7268" ;
    skos:prefLabel "Edward River:7268"@en ;
.

geoad:Edwinstowe8151
    a skos:Concept ;
    skos:historyNote "Compiled by the Geological Survey of Queensland" ;
    skos:broader geoad:MapSeries ;
    skos:definition "Map sheet for Edwinstowe at 1:100 000 scale. The first two digits define a longitude band 0.5 degree wide and the second two digits a latitude band 0.5 degree wide."@en ;
    skos:inScheme cs: ;
    skos:notation "8151" ;
    skos:prefLabel "Edwinstowe:8151"@en ;
.

geoad:Eidsvold9147
    a skos:Concept ;
    skos:historyNote "Compiled by the Geological Survey of Queensland" ;
    skos:broader geoad:MapSeries ;
    skos:definition "Map sheet for Eidsvold at 1:100 000 scale. The first two digits define a longitude band 0.5 degree wide and the second two digits a latitude band 0.5 degree wide."@en ;
    skos:inScheme cs: ;
    skos:notation "9147" ;
    skos:prefLabel "Eidsvold:9147"@en ;
.

geoad:Einasleigh7760
    a skos:Concept ;
    skos:historyNote "Compiled by the Geological Survey of Queensland" ;
    skos:broader geoad:MapSeries ;
    skos:definition "Map sheet for Einasleigh at 1:100 000 scale. The first two digits define a longitude band 0.5 degree wide and the second two digits a latitude band 0.5 degree wide."@en ;
    skos:inScheme cs: ;
    skos:notation "7760" ;
    skos:prefLabel "Einasleigh:7760"@en ;
.

geoad:ElRita7154
    a skos:Concept ;
    skos:historyNote "Compiled by the Geological Survey of Queensland" ;
    skos:broader geoad:MapSeries ;
    skos:definition "Map sheet for El Rita at 1:100 000 scale. The first two digits define a longitude band 0.5 degree wide and the second two digits a latitude band 0.5 degree wide."@en ;
    skos:inScheme cs: ;
    skos:notation "7154" ;
    skos:prefLabel "El Rita:7154"@en ;
.

geoad:ElizabethRiver6865
    a skos:Concept ;
    skos:historyNote "Compiled by the Geological Survey of Queensland" ;
    skos:broader geoad:MapSeries ;
    skos:definition "Map sheet for Elizabeth River at 1:100 000 scale. The first two digits define a longitude band 0.5 degree wide and the second two digits a latitude band 0.5 degree wide."@en ;
    skos:inScheme cs: ;
    skos:notation "6865" ;
    skos:prefLabel "Elizabeth River:6865"@en ;
.

geoad:ElizabethSprings7051
    a skos:Concept ;
    skos:historyNote "Compiled by the Geological Survey of Queensland" ;
    skos:broader geoad:MapSeries ;
    skos:definition "Map sheet for Elizabeth Springs at 1:100 000 scale. The first two digits define a longitude band 0.5 degree wide and the second two digits a latitude band 0.5 degree wide."@en ;
    skos:inScheme cs: ;
    skos:notation "7051" ;
    skos:prefLabel "Elizabeth Springs:7051"@en ;
.

geoad:Elmina8243
    a skos:Concept ;
    skos:historyNote "Compiled by the Geological Survey of Queensland" ;
    skos:broader geoad:MapSeries ;
    skos:definition "Map sheet for Elmina at 1:100 000 scale. The first two digits define a longitude band 0.5 degree wide and the second two digits a latitude band 0.5 degree wide."@en ;
    skos:inScheme cs: ;
    skos:notation "8243" ;
    skos:prefLabel "Elmina:8243"@en ;
.

geoad:Emerald8550
    a skos:Concept ;
    skos:historyNote "Compiled by the Geological Survey of Queensland" ;
    skos:broader geoad:MapSeries ;
    skos:definition "Map sheet for Emerald at 1:100 000 scale. The first two digits define a longitude band 0.5 degree wide and the second two digits a latitude band 0.5 degree wide."@en ;
    skos:inScheme cs: ;
    skos:notation "8550" ;
    skos:prefLabel "Emerald:8550"@en ;
.

geoad:Enngonia8039
    a skos:Concept ;
    skos:historyNote "Compiled by the Geological Survey of Queensland" ;
    skos:broader geoad:MapSeries ;
    skos:definition "Map sheet for Enngonia at 1:100 000 scale. The first two digits define a longitude band 0.5 degree wide and the second two digits a latitude band 0.5 degree wide."@en ;
    skos:inScheme cs: ;
    skos:notation "8039" ;
    skos:prefLabel "Enngonia:8039"@en ;
.

geoad:EppingForest8253
    a skos:Concept ;
    skos:historyNote "Compiled by the Geological Survey of Queensland" ;
    skos:broader geoad:MapSeries ;
    skos:definition "Map sheet for Epping Forest at 1:100 000 scale. The first two digits define a longitude band 0.5 degree wide and the second two digits a latitude band 0.5 degree wide."@en ;
    skos:inScheme cs: ;
    skos:notation "8253" ;
    skos:prefLabel "Epping Forest:8253"@en ;
.

geoad:Epsilon7141
    a skos:Concept ;
    skos:historyNote "Compiled by the Geological Survey of Queensland" ;
    skos:broader geoad:MapSeries ;
    skos:definition "Map sheet for Epsilon at 1:100 000 scale. The first two digits define a longitude band 0.5 degree wide and the second two digits a latitude band 0.5 degree wide."@en ;
    skos:inScheme cs: ;
    skos:notation "7141" ;
    skos:prefLabel "Epsilon:7141"@en ;
.

geoad:Eromanga7544
    a skos:Concept ;
    skos:historyNote "Compiled by the Geological Survey of Queensland" ;
    skos:broader geoad:MapSeries ;
    skos:definition "Map sheet for Eromanga at 1:100 000 scale. The first two digits define a longitude band 0.5 degree wide and the second two digits a latitude band 0.5 degree wide."@en ;
    skos:inScheme cs: ;
    skos:notation "7544" ;
    skos:prefLabel "Eromanga:7544"@en ;
.

geoad:Escott6762
    a skos:Concept ;
    skos:historyNote "Compiled by the Geological Survey of Queensland" ;
    skos:broader geoad:MapSeries ;
    skos:definition "Map sheet for Escott at 1:100 000 scale. The first two digits define a longitude band 0.5 degree wide and the second two digits a latitude band 0.5 degree wide."@en ;
    skos:inScheme cs: ;
    skos:notation "6762" ;
    skos:prefLabel "Escott:6762"@en ;
.

geoad:Esk9343
    a skos:Concept ;
    skos:historyNote "Compiled by the Geological Survey of Queensland" ;
    skos:broader geoad:MapSeries ;
    skos:definition "Map sheet for Esk at 1:100 000 scale. The first two digits define a longitude band 0.5 degree wide and the second two digits a latitude band 0.5 degree wide."@en ;
    skos:inScheme cs: ;
    skos:notation "9343" ;
    skos:prefLabel "Esk:9343"@en ;
.

geoad:Esmeralda7460
    a skos:Concept ;
    skos:historyNote "Compiled by the Geological Survey of Queensland" ;
    skos:broader geoad:MapSeries ;
    skos:definition "Map sheet for Esmeralda at 1:100 000 scale. The first two digits define a longitude band 0.5 degree wide and the second two digits a latitude band 0.5 degree wide."@en ;
    skos:inScheme cs: ;
    skos:notation "7460" ;
    skos:prefLabel "Esmeralda:7460"@en ;
.

geoad:Etamunbanie6845
    a skos:Concept ;
    skos:historyNote "Compiled by the Geological Survey of Queensland" ;
    skos:broader geoad:MapSeries ;
    skos:definition "Map sheet for Etamunbanie at 1:100 000 scale. The first two digits define a longitude band 0.5 degree wide and the second two digits a latitude band 0.5 degree wide."@en ;
    skos:inScheme cs: ;
    skos:notation "6845" ;
    skos:prefLabel "Etamunbanie:6845"@en ;
.

geoad:Etheldale7458
    a skos:Concept ;
    skos:historyNote "Compiled by the Geological Survey of Queensland" ;
    skos:broader geoad:MapSeries ;
    skos:definition "Map sheet for Etheldale at 1:100 000 scale. The first two digits define a longitude band 0.5 degree wide and the second two digits a latitude band 0.5 degree wide."@en ;
    skos:inScheme cs: ;
    skos:notation "7458" ;
    skos:prefLabel "Etheldale:7458"@en ;
.

geoad:Eulo7941
    a skos:Concept ;
    skos:historyNote "Compiled by the Geological Survey of Queensland" ;
    skos:broader geoad:MapSeries ;
    skos:definition "Map sheet for Eulo at 1:100 000 scale. The first two digits define a longitude band 0.5 degree wide and the second two digits a latitude band 0.5 degree wide."@en ;
    skos:inScheme cs: ;
    skos:notation "7941" ;
    skos:prefLabel "Eulo:7941"@en ;
.

geoad:Eulolo7255
    a skos:Concept ;
    skos:historyNote "Compiled by the Geological Survey of Queensland" ;
    skos:broader geoad:MapSeries ;
    skos:definition "Map sheet for Eulolo at 1:100 000 scale. The first two digits define a longitude band 0.5 degree wide and the second two digits a latitude band 0.5 degree wide."@en ;
    skos:inScheme cs: ;
    skos:notation "7255" ;
    skos:prefLabel "Eulolo:7255"@en ;
.

geoad:Ewan8059
    a skos:Concept ;
    skos:historyNote "Compiled by the Geological Survey of Queensland" ;
    skos:broader geoad:MapSeries ;
    skos:definition "Map sheet for Ewan at 1:100 000 scale. The first two digits define a longitude band 0.5 degree wide and the second two digits a latitude band 0.5 degree wide."@en ;
    skos:inScheme cs: ;
    skos:notation "8059" ;
    skos:prefLabel "Ewan:8059"@en ;
.

geoad:Fermoy7551
    a skos:Concept ;
    skos:historyNote "Compiled by the Geological Survey of Queensland" ;
    skos:broader geoad:MapSeries ;
    skos:definition "Map sheet for Fermoy at 1:100 000 scale. The first two digits define a longitude band 0.5 degree wide and the second two digits a latitude band 0.5 degree wide."@en ;
    skos:inScheme cs: ;
    skos:notation "7551" ;
    skos:prefLabel "Fermoy:7551"@en ;
.

geoad:FinucaneRange7153
    a skos:Concept ;
    skos:historyNote "Compiled by the Geological Survey of Queensland" ;
    skos:broader geoad:MapSeries ;
    skos:definition "Map sheet for Finucane Range at 1:100 000 scale. The first two digits define a longitude band 0.5 degree wide and the second two digits a latitude band 0.5 degree wide."@en ;
    skos:inScheme cs: ;
    skos:notation "7153" ;
    skos:prefLabel "Finucane Range:7153"@en ;
.

geoad:Flinton8842
    a skos:Concept ;
    skos:historyNote "Compiled by the Geological Survey of Queensland" ;
    skos:broader geoad:MapSeries ;
    skos:definition "Map sheet for Flinton at 1:100 000 scale. The first two digits define a longitude band 0.5 degree wide and the second two digits a latitude band 0.5 degree wide."@en ;
    skos:inScheme cs: ;
    skos:notation "8842" ;
    skos:prefLabel "Flinton:8842"@en ;
.

geoad:ForestHome7561
    a skos:Concept ;
    skos:historyNote "Compiled by the Geological Survey of Queensland" ;
    skos:broader geoad:MapSeries ;
    skos:definition "Map sheet for Forest Home at 1:100 000 scale. The first two digits define a longitude band 0.5 degree wide and the second two digits a latitude band 0.5 degree wide."@en ;
    skos:inScheme cs: ;
    skos:notation "7561" ;
    skos:prefLabel "Forest Home:7561"@en ;
.

geoad:ForestVale8446
    a skos:Concept ;
    skos:historyNote "Compiled by the Geological Survey of Queensland" ;
    skos:broader geoad:MapSeries ;
    skos:definition "Map sheet for Forest Vale at 1:100 000 scale. The first two digits define a longitude band 0.5 degree wide and the second two digits a latitude band 0.5 degree wide."@en ;
    skos:inScheme cs: ;
    skos:notation "8446" ;
    skos:prefLabel "Forest Vale:8446"@en ;
.

geoad:Forsayth7660
    a skos:Concept ;
    skos:historyNote "Compiled by the Geological Survey of Queensland" ;
    skos:broader geoad:MapSeries ;
    skos:definition "Map sheet for Forsayth at 1:100 000 scale. The first two digits define a longitude band 0.5 degree wide and the second two digits a latitude band 0.5 degree wide."@en ;
    skos:inScheme cs: ;
    skos:notation "7660" ;
    skos:prefLabel "Forsayth:7660"@en ;
.

geoad:FortGrey7139
    a skos:Concept ;
    skos:historyNote "Compiled by the Geological Survey of Queensland" ;
    skos:broader geoad:MapSeries ;
    skos:definition "Map sheet for Fort Grey at 1:100 000 scale. The first two digits define a longitude band 0.5 degree wide and the second two digits a latitude band 0.5 degree wide."@en ;
    skos:inScheme cs: ;
    skos:notation "7139" ;
    skos:prefLabel "Fort Grey:7139"@en ;
.

geoad:Frankfield8353
    a skos:Concept ;
    skos:historyNote "Compiled by the Geological Survey of Queensland" ;
    skos:broader geoad:MapSeries ;
    skos:definition "Map sheet for Frankfield at 1:100 000 scale. The first two digits define a longitude band 0.5 degree wide and the second two digits a latitude band 0.5 degree wide."@en ;
    skos:inScheme cs: ;
    skos:notation "8353" ;
    skos:prefLabel "Frankfield:8353"@en ;
.

geoad:GabbaIsland7478
    a skos:Concept ;
    skos:historyNote "Compiled by the Geological Survey of Queensland" ;
    skos:broader geoad:MapSeries ;
    skos:definition "Map sheet for Gabba Island at 1:100 000 scale. The first two digits define a longitude band 0.5 degree wide and the second two digits a latitude band 0.5 degree wide."@en ;
    skos:inScheme cs: ;
    skos:notation "7478" ;
    skos:prefLabel "Gabba Island:7478"@en ;
.

geoad:Galbraith7265
    a skos:Concept ;
    skos:historyNote "Compiled by the Geological Survey of Queensland" ;
    skos:broader geoad:MapSeries ;
    skos:definition "Map sheet for Galbraith at 1:100 000 scale. The first two digits define a longitude band 0.5 degree wide and the second two digits a latitude band 0.5 degree wide."@en ;
    skos:inScheme cs: ;
    skos:notation "7265" ;
    skos:prefLabel "Galbraith:7265"@en ;
.

geoad:Galilee8053
    a skos:Concept ;
    skos:historyNote "Compiled by the Geological Survey of Queensland" ;
    skos:broader geoad:MapSeries ;
    skos:definition "Map sheet for Galilee at 1:100 000 scale. The first two digits define a longitude band 0.5 degree wide and the second two digits a latitude band 0.5 degree wide."@en ;
    skos:inScheme cs: ;
    skos:notation "8053" ;
    skos:prefLabel "Galilee:8053"@en ;
.

geoad:Galloway7662
    a skos:Concept ;
    skos:historyNote "Compiled by the Geological Survey of Queensland" ;
    skos:broader geoad:MapSeries ;
    skos:definition "Map sheet for Galloway at 1:100 000 scale. The first two digits define a longitude band 0.5 degree wide and the second two digits a latitude band 0.5 degree wide."@en ;
    skos:inScheme cs: ;
    skos:notation "7662" ;
    skos:prefLabel "Galloway:7662"@en ;
.

geoad:Garfield8051
    a skos:Concept ;
    skos:historyNote "Compiled by the Geological Survey of Queensland" ;
    skos:broader geoad:MapSeries ;
    skos:definition "Map sheet for Garfield at 1:100 000 scale. The first two digits define a longitude band 0.5 degree wide and the second two digits a latitude band 0.5 degree wide."@en ;
    skos:inScheme cs: ;
    skos:notation "8051" ;
    skos:prefLabel "Garfield:8051"@en ;
.

geoad:Gason6643
    a skos:Concept ;
    skos:historyNote "Compiled by the Geological Survey of Queensland" ;
    skos:broader geoad:MapSeries ;
    skos:definition "Map sheet for Gason at 1:100 000 scale. The first two digits define a longitude band 0.5 degree wide and the second two digits a latitude band 0.5 degree wide."@en ;
    skos:inScheme cs: ;
    skos:notation "6643" ;
    skos:prefLabel "Gason:6643"@en ;
.

geoad:Gayndah9246
    a skos:Concept ;
    skos:historyNote "Compiled by the Geological Survey of Queensland" ;
    skos:broader geoad:MapSeries ;
    skos:definition "Map sheet for Gayndah at 1:100 000 scale. The first two digits define a longitude band 0.5 degree wide and the second two digits a latitude band 0.5 degree wide."@en ;
    skos:inScheme cs: ;
    skos:notation "9246" ;
    skos:prefLabel "Gayndah:9246"@en ;
.

geoad:Georgetown7661
    a skos:Concept ;
    skos:historyNote "Compiled by the Geological Survey of Queensland" ;
    skos:broader geoad:MapSeries ;
    skos:definition "Map sheet for Georgetown at 1:100 000 scale. The first two digits define a longitude band 0.5 degree wide and the second two digits a latitude band 0.5 degree wide."@en ;
    skos:inScheme cs: ;
    skos:notation "7661" ;
    skos:prefLabel "Georgetown:7661"@en ;
.

geoad:Gerara8139
    a skos:Concept ;
    skos:historyNote "Compiled by the Geological Survey of Queensland" ;
    skos:broader geoad:MapSeries ;
    skos:definition "Map sheet for Gerara at 1:100 000 scale. The first two digits define a longitude band 0.5 degree wide and the second two digits a latitude band 0.5 degree wide."@en ;
    skos:inScheme cs: ;
    skos:notation "8139" ;
    skos:prefLabel "Gerara:8139"@en ;
.

geoad:Ghinghinda8847
    a skos:Concept ;
    skos:historyNote "Compiled by the Geological Survey of Queensland" ;
    skos:broader geoad:MapSeries ;
    skos:definition "Map sheet for Ghinghinda at 1:100 000 scale. The first two digits define a longitude band 0.5 degree wide and the second two digits a latitude band 0.5 degree wide."@en ;
    skos:inScheme cs: ;
    skos:notation "8847" ;
    skos:prefLabel "Ghinghinda:8847"@en ;
.

geoad:Gidgealpa6942
    a skos:Concept ;
    skos:historyNote "Compiled by the Geological Survey of Queensland" ;
    skos:broader geoad:MapSeries ;
    skos:definition "Map sheet for Gidgealpa at 1:100 000 scale. The first two digits define a longitude band 0.5 degree wide and the second two digits a latitude band 0.5 degree wide."@en ;
    skos:inScheme cs: ;
    skos:notation "6942" ;
    skos:prefLabel "Gidgealpa:6942"@en ;
.

geoad:GilbertRiver7461
    a skos:Concept ;
    skos:historyNote "Compiled by the Geological Survey of Queensland" ;
    skos:broader geoad:MapSeries ;
    skos:definition "Map sheet for Gilbert River at 1:100 000 scale. The first two digits define a longitude band 0.5 degree wide and the second two digits a latitude band 0.5 degree wide."@en ;
    skos:inScheme cs: ;
    skos:notation "7461" ;
    skos:prefLabel "Gilbert River:7461"@en ;
.

geoad:Gilberton7659
    a skos:Concept ;
    skos:historyNote "Compiled by the Geological Survey of Queensland" ;
    skos:broader geoad:MapSeries ;
    skos:definition "Map sheet for Gilberton at 1:100 000 scale. The first two digits define a longitude band 0.5 degree wide and the second two digits a latitude band 0.5 degree wide."@en ;
    skos:inScheme cs: ;
    skos:notation "7659" ;
    skos:prefLabel "Gilberton:7659"@en ;
.

geoad:Gladstone9150
    a skos:Concept ;
    skos:historyNote "Compiled by the Geological Survey of Queensland" ;
    skos:broader geoad:MapSeries ;
    skos:definition "Map sheet for Gladstone at 1:100 000 scale. The first two digits define a longitude band 0.5 degree wide and the second two digits a latitude band 0.5 degree wide."@en ;
    skos:inScheme cs: ;
    skos:notation "9150" ;
    skos:prefLabel "Gladstone:9150"@en ;
.

geoad:Glanworth8047
    a skos:Concept ;
    skos:historyNote "Compiled by the Geological Survey of Queensland" ;
    skos:broader geoad:MapSeries ;
    skos:definition "Map sheet for Glanworth at 1:100 000 scale. The first two digits define a longitude band 0.5 degree wide and the second two digits a latitude band 0.5 degree wide."@en ;
    skos:inScheme cs: ;
    skos:notation "8047" ;
    skos:prefLabel "Glanworth:8047"@en ;
.

geoad:Glenara7747
    a skos:Concept ;
    skos:historyNote "Compiled by the Geological Survey of Queensland" ;
    skos:broader geoad:MapSeries ;
    skos:definition "Map sheet for Glenara at 1:100 000 scale. The first two digits define a longitude band 0.5 degree wide and the second two digits a latitude band 0.5 degree wide."@en ;
    skos:inScheme cs: ;
    skos:notation "7747" ;
    skos:prefLabel "Glenara:7747"@en ;
.

geoad:Glendon8356
    a skos:Concept ;
    skos:historyNote "Compiled by the Geological Survey of Queensland" ;
    skos:broader geoad:MapSeries ;
    skos:definition "Map sheet for Glendon at 1:100 000 scale. The first two digits define a longitude band 0.5 degree wide and the second two digits a latitude band 0.5 degree wide."@en ;
    skos:inScheme cs: ;
    skos:notation "8356" ;
    skos:prefLabel "Glendon:8356"@en ;
.

geoad:Glenhaughton8747
    a skos:Concept ;
    skos:historyNote "Compiled by the Geological Survey of Queensland" ;
    skos:broader geoad:MapSeries ;
    skos:definition "Map sheet for Glenhaughton at 1:100 000 scale. The first two digits define a longitude band 0.5 degree wide and the second two digits a latitude band 0.5 degree wide."@en ;
    skos:inScheme cs: ;
    skos:notation "8747" ;
    skos:prefLabel "Glenhaughton:8747"@en ;
.

geoad:Glenlyon7455
    a skos:Concept ;
    skos:historyNote "Compiled by the Geological Survey of Queensland" ;
    skos:broader geoad:MapSeries ;
    skos:definition "Map sheet for Glenlyon at 1:100 000 scale. The first two digits define a longitude band 0.5 degree wide and the second two digits a latitude band 0.5 degree wide."@en ;
    skos:inScheme cs: ;
    skos:notation "7455" ;
    skos:prefLabel "Glenlyon:7455"@en ;
.

geoad:Glenormiston6652
    a skos:Concept ;
    skos:historyNote "Compiled by the Geological Survey of Queensland" ;
    skos:broader geoad:MapSeries ;
    skos:definition "Map sheet for Glenormiston at 1:100 000 scale. The first two digits define a longitude band 0.5 degree wide and the second two digits a latitude band 0.5 degree wide."@en ;
    skos:inScheme cs: ;
    skos:notation "6652" ;
    skos:prefLabel "Glenormiston:6652"@en ;
.

geoad:Glenusk8049
    a skos:Concept ;
    skos:historyNote "Compiled by the Geological Survey of Queensland" ;
    skos:broader geoad:MapSeries ;
    skos:definition "Map sheet for Glenusk at 1:100 000 scale. The first two digits define a longitude band 0.5 degree wide and the second two digits a latitude band 0.5 degree wide."@en ;
    skos:inScheme cs: ;
    skos:notation "8049" ;
    skos:prefLabel "Glenusk:8049"@en ;
.

geoad:GnallanAGeaCreek6549
    a skos:Concept ;
    skos:historyNote "Compiled by the Geological Survey of Queensland" ;
    skos:broader geoad:MapSeries ;
    skos:definition "Map sheet for Gnallan A Gea Creek at 1:100 000 scale. The first two digits define a longitude band 0.5 degree wide and the second two digits a latitude band 0.5 degree wide."@en ;
    skos:inScheme cs: ;
    skos:notation "6549" ;
    skos:prefLabel "Gnallan A Gea Creek:6549"@en ;
.

geoad:GoaCreek6655
    a skos:Concept ;
    skos:historyNote "Compiled by the Geological Survey of Queensland" ;
    skos:broader geoad:MapSeries ;
    skos:definition "Map sheet for Goa Creek at 1:100 000 scale. The first two digits define a longitude band 0.5 degree wide and the second two digits a latitude band 0.5 degree wide."@en ;
    skos:inScheme cs: ;
    skos:notation "6655" ;
    skos:prefLabel "Goa Creek:6655"@en ;
.

geoad:Goodar8941
    a skos:Concept ;
    skos:historyNote "Compiled by the Geological Survey of Queensland" ;
    skos:broader geoad:MapSeries ;
    skos:definition "Map sheet for Goodar at 1:100 000 scale. The first two digits define a longitude band 0.5 degree wide and the second two digits a latitude band 0.5 degree wide."@en ;
    skos:inScheme cs: ;
    skos:notation "8941" ;
    skos:prefLabel "Goodar:8941"@en ;
.

geoad:Goodooga8339
    a skos:Concept ;
    skos:historyNote "Compiled by the Geological Survey of Queensland" ;
    skos:broader geoad:MapSeries ;
    skos:definition "Map sheet for Goodooga at 1:100 000 scale. The first two digits define a longitude band 0.5 degree wide and the second two digits a latitude band 0.5 degree wide."@en ;
    skos:inScheme cs: ;
    skos:notation "8339" ;
    skos:prefLabel "Goodooga:8339"@en ;
.

geoad:Goodwood6952
    a skos:Concept ;
    skos:historyNote "Compiled by the Geological Survey of Queensland" ;
    skos:broader geoad:MapSeries ;
    skos:definition "Map sheet for Goodwood at 1:100 000 scale. The first two digits define a longitude band 0.5 degree wide and the second two digits a latitude band 0.5 degree wide."@en ;
    skos:inScheme cs: ;
    skos:notation "6952" ;
    skos:prefLabel "Goodwood:6952"@en ;
.

geoad:Goomeri9345
    a skos:Concept ;
    skos:historyNote "Compiled by the Geological Survey of Queensland" ;
    skos:broader geoad:MapSeries ;
    skos:definition "Map sheet for Goomeri at 1:100 000 scale. The first two digits define a longitude band 0.5 degree wide and the second two digits a latitude band 0.5 degree wide."@en ;
    skos:inScheme cs: ;
    skos:notation "9345" ;
    skos:prefLabel "Goomeri:9345"@en ;
.

geoad:Goonamillera6646
    a skos:Concept ;
    skos:historyNote "Compiled by the Geological Survey of Queensland" ;
    skos:broader geoad:MapSeries ;
    skos:definition "Map sheet for Goonamillera at 1:100 000 scale. The first two digits define a longitude band 0.5 degree wide and the second two digits a latitude band 0.5 degree wide."@en ;
    skos:inScheme cs: ;
    skos:notation "6646" ;
    skos:prefLabel "Goonamillera:6646"@en ;
.

geoad:Goondiwindi8940
    a skos:Concept ;
    skos:historyNote "Compiled by the Geological Survey of Queensland" ;
    skos:broader geoad:MapSeries ;
    skos:definition "Map sheet for Goondiwindi at 1:100 000 scale. The first two digits define a longitude band 0.5 degree wide and the second two digits a latitude band 0.5 degree wide."@en ;
    skos:inScheme cs: ;
    skos:notation "8940" ;
    skos:prefLabel "Goondiwindi:8940"@en ;
.

geoad:Goyder6644
    a skos:Concept ;
    skos:historyNote "Compiled by the Geological Survey of Queensland" ;
    skos:broader geoad:MapSeries ;
    skos:definition "Map sheet for Goyder at 1:100 000 scale. The first two digits define a longitude band 0.5 degree wide and the second two digits a latitude band 0.5 degree wide."@en ;
    skos:inScheme cs: ;
    skos:notation "6644" ;
    skos:prefLabel "Goyder:6644"@en ;
.

geoad:Gregory6740
    a skos:Concept ;
    skos:historyNote "Compiled by the Geological Survey of Queensland" ;
    skos:broader geoad:MapSeries ;
    skos:definition "Map sheet for Gregory at 1:100 000 scale. The first two digits define a longitude band 0.5 degree wide and the second two digits a latitude band 0.5 degree wide."@en ;
    skos:inScheme cs: ;
    skos:notation "6740" ;
    skos:prefLabel "Gregory:6740"@en ;
.

geoad:GregoryDowns6760
    a skos:Concept ;
    skos:historyNote "Compiled by the Geological Survey of Queensland" ;
    skos:broader geoad:MapSeries ;
    skos:definition "Map sheet for Gregory Downs at 1:100 000 scale. The first two digits define a longitude band 0.5 degree wide and the second two digits a latitude band 0.5 degree wide."@en ;
    skos:inScheme cs: ;
    skos:notation "6760" ;
    skos:prefLabel "Gregory Downs:6760"@en ;
.

geoad:GrosvenorDowns8553
    a skos:Concept ;
    skos:historyNote "Compiled by the Geological Survey of Queensland" ;
    skos:broader geoad:MapSeries ;
    skos:definition "Map sheet for Grosvenor Downs at 1:100 000 scale. The first two digits define a longitude band 0.5 degree wide and the second two digits a latitude band 0.5 degree wide."@en ;
    skos:inScheme cs: ;
    skos:notation "8553" ;
    skos:prefLabel "Grosvenor Downs:8553"@en ;
.

geoad:Guluguba8945
    a skos:Concept ;
    skos:historyNote "Compiled by the Geological Survey of Queensland" ;
    skos:broader geoad:MapSeries ;
    skos:definition "Map sheet for Guluguba at 1:100 000 scale. The first two digits define a longitude band 0.5 degree wide and the second two digits a latitude band 0.5 degree wide."@en ;
    skos:inScheme cs: ;
    skos:notation "8945" ;
    skos:prefLabel "Guluguba:8945"@en ;
.

geoad:Gumbardo7845
    a skos:Concept ;
    skos:historyNote "Compiled by the Geological Survey of Queensland" ;
    skos:broader geoad:MapSeries ;
    skos:definition "Map sheet for Gumbardo at 1:100 000 scale. The first two digits define a longitude band 0.5 degree wide and the second two digits a latitude band 0.5 degree wide."@en ;
    skos:inScheme cs: ;
    skos:notation "7845" ;
    skos:prefLabel "Gumbardo:7845"@en ;
.

geoad:Gunjulla8354
    a skos:Concept ;
    skos:historyNote "Compiled by the Geological Survey of Queensland" ;
    skos:broader geoad:MapSeries ;
    skos:definition "Map sheet for Gunjulla at 1:100 000 scale. The first two digits define a longitude band 0.5 degree wide and the second two digits a latitude band 0.5 degree wide."@en ;
    skos:inScheme cs: ;
    skos:notation "8354" ;
    skos:prefLabel "Gunjulla:8354"@en ;
.

geoad:Gympie9445
    a skos:Concept ;
    skos:historyNote "Compiled by the Geological Survey of Queensland" ;
    skos:broader geoad:MapSeries ;
    skos:definition "Map sheet for Gympie at 1:100 000 scale. The first two digits define a longitude band 0.5 degree wide and the second two digits a latitude band 0.5 degree wide."@en ;
    skos:inScheme cs: ;
    skos:notation "9445" ;
    skos:prefLabel "Gympie:9445"@en ;
.

geoad:Haddon7045
    a skos:Concept ;
    skos:historyNote "Compiled by the Geological Survey of Queensland" ;
    skos:broader geoad:MapSeries ;
    skos:definition "Map sheet for Haddon at 1:100 000 scale. The first two digits define a longitude band 0.5 degree wide and the second two digits a latitude band 0.5 degree wide."@en ;
    skos:inScheme cs: ;
    skos:notation "7045" ;
    skos:prefLabel "Haddon:7045"@en ;
.

geoad:HaddonCorner7146
    a skos:Concept ;
    skos:historyNote "Compiled by the Geological Survey of Queensland" ;
    skos:broader geoad:MapSeries ;
    skos:definition "Map sheet for Haddon Corner at 1:100 000 scale. The first two digits define a longitude band 0.5 degree wide and the second two digits a latitude band 0.5 degree wide."@en ;
    skos:inScheme cs: ;
    skos:notation "7146" ;
    skos:prefLabel "Haddon Corner:7146"@en ;
.

geoad:HamiltonDowns7355
    a skos:Concept ;
    skos:historyNote "Compiled by the Geological Survey of Queensland" ;
    skos:broader geoad:MapSeries ;
    skos:definition "Map sheet for Hamilton Downs at 1:100 000 scale. The first two digits define a longitude band 0.5 degree wide and the second two digits a latitude band 0.5 degree wide."@en ;
    skos:inScheme cs: ;
    skos:notation "7355" ;
    skos:prefLabel "Hamilton Downs:7355"@en ;
.

geoad:Hampstead7658
    a skos:Concept ;
    skos:historyNote "Compiled by the Geological Survey of Queensland" ;
    skos:broader geoad:MapSeries ;
    skos:definition "Map sheet for Hampstead at 1:100 000 scale. The first two digits define a longitude band 0.5 degree wide and the second two digits a latitude band 0.5 degree wide."@en ;
    skos:inScheme cs: ;
    skos:notation "7658" ;
    skos:prefLabel "Hampstead:7658"@en ;
.

geoad:HappyValley9547
    a skos:Concept ;
    skos:historyNote "Compiled by the Geological Survey of Queensland" ;
    skos:broader geoad:MapSeries ;
    skos:definition "Map sheet for Happy Valley at 1:100 000 scale. The first two digits define a longitude band 0.5 degree wide and the second two digits a latitude band 0.5 degree wide."@en ;
    skos:inScheme cs: ;
    skos:notation "9547" ;
    skos:prefLabel "Happy Valley:9547"@en ;
.

geoad:Harrybrandt8554
    a skos:Concept ;
    skos:historyNote "Compiled by the Geological Survey of Queensland" ;
    skos:broader geoad:MapSeries ;
    skos:definition "Map sheet for Harrybrandt at 1:100 000 scale. The first two digits define a longitude band 0.5 degree wide and the second two digits a latitude band 0.5 degree wide."@en ;
    skos:inScheme cs: ;
    skos:notation "8554" ;
    skos:prefLabel "Harrybrandt:8554"@en ;
.

geoad:HarvestHome8256
    a skos:Concept ;
    skos:historyNote "Compiled by the Geological Survey of Queensland" ;
    skos:broader geoad:MapSeries ;
    skos:definition "Map sheet for Harvest Home at 1:100 000 scale. The first two digits define a longitude band 0.5 degree wide and the second two digits a latitude band 0.5 degree wide."@en ;
    skos:inScheme cs: ;
    skos:notation "8256" ;
    skos:prefLabel "Harvest Home:8256"@en ;
.

geoad:Headingly6555
    a skos:Concept ;
    skos:historyNote "Compiled by the Geological Survey of Queensland" ;
    skos:broader geoad:MapSeries ;
    skos:definition "Map sheet for Headingly at 1:100 000 scale. The first two digits define a longitude band 0.5 degree wide and the second two digits a latitude band 0.5 degree wide."@en ;
    skos:inScheme cs: ;
    skos:notation "6555" ;
    skos:prefLabel "Headingly:6555"@en ;
.

geoad:Hebel8440
    a skos:Concept ;
    skos:historyNote "Compiled by the Geological Survey of Queensland" ;
    skos:broader geoad:MapSeries ;
    skos:definition "Map sheet for Hebel at 1:100 000 scale. The first two digits define a longitude band 0.5 degree wide and the second two digits a latitude band 0.5 degree wide."@en ;
    skos:inScheme cs: ;
    skos:notation "8440" ;
    skos:prefLabel "Hebel:8440"@en ;
.

geoad:HedleysCreek6562
    a skos:Concept ;
    skos:historyNote "Compiled by the Geological Survey of Queensland" ;
    skos:broader geoad:MapSeries ;
    skos:definition "Map sheet for Hedleys Creek at 1:100 000 scale. The first two digits define a longitude band 0.5 degree wide and the second two digits a latitude band 0.5 degree wide."@en ;
    skos:inScheme cs: ;
    skos:notation "6562" ;
    skos:prefLabel "Hedleys Creek:6562"@en ;
.

geoad:Helenvale7966
    a skos:Concept ;
    skos:historyNote "Compiled by the Geological Survey of Queensland" ;
    skos:broader geoad:MapSeries ;
    skos:definition "Map sheet for Helenvale at 1:100 000 scale. The first two digits define a longitude band 0.5 degree wide and the second two digits a latitude band 0.5 degree wide."@en ;
    skos:inScheme cs: ;
    skos:notation "7966" ;
    skos:prefLabel "Helenvale:7966"@en ;
.

geoad:Helidon9342
    a skos:Concept ;
    skos:historyNote "Compiled by the Geological Survey of Queensland" ;
    skos:broader geoad:MapSeries ;
    skos:definition "Map sheet for Helidon at 1:100 000 scale. The first two digits define a longitude band 0.5 degree wide and the second two digits a latitude band 0.5 degree wide."@en ;
    skos:inScheme cs: ;
    skos:notation "9342" ;
    skos:prefLabel "Helidon:9342"@en ;
.

geoad:HerbertDowns6751
    a skos:Concept ;
    skos:historyNote "Compiled by the Geological Survey of Queensland" ;
    skos:broader geoad:MapSeries ;
    skos:definition "Map sheet for Herbert Downs at 1:100 000 scale. The first two digits define a longitude band 0.5 degree wide and the second two digits a latitude band 0.5 degree wide."@en ;
    skos:inScheme cs: ;
    skos:notation "6751" ;
    skos:prefLabel "Herbert Downs:6751"@en ;
.

geoad:HeronIsland9251
    a skos:Concept ;
    skos:historyNote "Compiled by the Geological Survey of Queensland" ;
    skos:broader geoad:MapSeries ;
    skos:definition "Map sheet for Heron Island at 1:100 000 scale. The first two digits define a longitude band 0.5 degree wide and the second two digits a latitude band 0.5 degree wide."@en ;
    skos:inScheme cs: ;
    skos:notation "9251" ;
    skos:prefLabel "Heron Island:9251"@en ;
.

geoad:HighPeakIsland9054
    a skos:Concept ;
    skos:historyNote "Compiled by the Geological Survey of Queensland" ;
    skos:broader geoad:MapSeries ;
    skos:definition "Map sheet for High Peak Island at 1:100 000 scale. The first two digits define a longitude band 0.5 degree wide and the second two digits a latitude band 0.5 degree wide."@en ;
    skos:inScheme cs: ;
    skos:notation "9054" ;
    skos:prefLabel "High Peak Island:9054"@en ;
.

geoad:Highbury7565
    a skos:Concept ;
    skos:historyNote "Compiled by the Geological Survey of Queensland" ;
    skos:broader geoad:MapSeries ;
    skos:definition "Map sheet for Highbury at 1:100 000 scale. The first two digits define a longitude band 0.5 degree wide and the second two digits a latitude band 0.5 degree wide."@en ;
    skos:inScheme cs: ;
    skos:notation "7565" ;
    skos:prefLabel "Highbury:7565"@en ;
.

geoad:Hillalong8555
    a skos:Concept ;
    skos:historyNote "Compiled by the Geological Survey of Queensland" ;
    skos:broader geoad:MapSeries ;
    skos:definition "Map sheet for Hillalong at 1:100 000 scale. The first two digits define a longitude band 0.5 degree wide and the second two digits a latitude band 0.5 degree wide."@en ;
    skos:inScheme cs: ;
    skos:notation "8555" ;
    skos:prefLabel "Hillalong:8555"@en ;
.

geoad:Hillgrove8058
    a skos:Concept ;
    skos:historyNote "Compiled by the Geological Survey of Queensland" ;
    skos:broader geoad:MapSeries ;
    skos:definition "Map sheet for Hillgrove at 1:100 000 scale. The first two digits define a longitude band 0.5 degree wide and the second two digits a latitude band 0.5 degree wide."@en ;
    skos:inScheme cs: ;
    skos:notation "8058" ;
    skos:prefLabel "Hillgrove:8058"@en ;
.

geoad:HillsRange7252
    a skos:Concept ;
    skos:historyNote "Compiled by the Geological Survey of Queensland" ;
    skos:broader geoad:MapSeries ;
    skos:definition "Map sheet for Hills Range at 1:100 000 scale. The first two digits define a longitude band 0.5 degree wide and the second two digits a latitude band 0.5 degree wide."@en ;
    skos:inScheme cs: ;
    skos:notation "7252" ;
    skos:prefLabel "Hills Range:7252"@en ;
.

geoad:Hoganthulla8346
    a skos:Concept ;
    skos:historyNote "Compiled by the Geological Survey of Queensland" ;
    skos:broader geoad:MapSeries ;
    skos:definition "Map sheet for Hoganthulla at 1:100 000 scale. The first two digits define a longitude band 0.5 degree wide and the second two digits a latitude band 0.5 degree wide."@en ;
    skos:inScheme cs: ;
    skos:notation "8346" ;
    skos:prefLabel "Hoganthulla:8346"@en ;
.

geoad:Holroyd7269
    a skos:Concept ;
    skos:historyNote "Compiled by the Geological Survey of Queensland" ;
    skos:broader geoad:MapSeries ;
    skos:definition "Map sheet for Holroyd at 1:100 000 scale. The first two digits define a longitude band 0.5 degree wide and the second two digits a latitude band 0.5 degree wide."@en ;
    skos:inScheme cs: ;
    skos:notation "7269" ;
    skos:prefLabel "Holroyd:7269"@en ;
.

geoad:Homeboin8342
    a skos:Concept ;
    skos:historyNote "Compiled by the Geological Survey of Queensland" ;
    skos:broader geoad:MapSeries ;
    skos:definition "Map sheet for Homeboin at 1:100 000 scale. The first two digits define a longitude band 0.5 degree wide and the second two digits a latitude band 0.5 degree wide."@en ;
    skos:inScheme cs: ;
    skos:notation "8342" ;
    skos:prefLabel "Homeboin:8342"@en ;
.

geoad:Homestead8057
    a skos:Concept ;
    skos:historyNote "Compiled by the Geological Survey of Queensland" ;
    skos:broader geoad:MapSeries ;
    skos:definition "Map sheet for Homestead at 1:100 000 scale. The first two digits define a longitude band 0.5 degree wide and the second two digits a latitude band 0.5 degree wide."@en ;
    skos:inScheme cs: ;
    skos:notation "8057" ;
    skos:prefLabel "Homestead:8057"@en ;
.

geoad:HornetBank8746
    a skos:Concept ;
    skos:historyNote "Compiled by the Geological Survey of Queensland" ;
    skos:broader geoad:MapSeries ;
    skos:definition "Map sheet for Hornet Bank at 1:100 000 scale. The first two digits define a longitude band 0.5 degree wide and the second two digits a latitude band 0.5 degree wide."@en ;
    skos:inScheme cs: ;
    skos:notation "8746" ;
    skos:prefLabel "Hornet Bank:8746"@en ;
.

geoad:HoskynIsland9350
    a skos:Concept ;
    skos:historyNote "Compiled by the Geological Survey of Queensland" ;
    skos:broader geoad:MapSeries ;
    skos:definition "Map sheet for Hoskyn Island at 1:100 000 scale. The first two digits define a longitude band 0.5 degree wide and the second two digits a latitude band 0.5 degree wide."@en ;
    skos:inScheme cs: ;
    skos:notation "9350" ;
    skos:prefLabel "Hoskyn Island:9350"@en ;
.

geoad:HotspurIsland8955
    a skos:Concept ;
    skos:historyNote "Compiled by the Geological Survey of Queensland" ;
    skos:broader geoad:MapSeries ;
    skos:definition "Map sheet for Hotspur Island at 1:100 000 scale. The first two digits define a longitude band 0.5 degree wide and the second two digits a latitude band 0.5 degree wide."@en ;
    skos:inScheme cs: ;
    skos:notation "8955" ;
    skos:prefLabel "Hotspur Island:8955"@en ;
.

geoad:Hughenden7756
    a skos:Concept ;
    skos:historyNote "Compiled by the Geological Survey of Queensland" ;
    skos:broader geoad:MapSeries ;
    skos:definition "Map sheet for Hughenden at 1:100 000 scale. The first two digits define a longitude band 0.5 degree wide and the second two digits a latitude band 0.5 degree wide."@en ;
    skos:inScheme cs: ;
    skos:notation "7756" ;
    skos:prefLabel "Hughenden:7756"@en ;
.

geoad:Humeburn7943
    a skos:Concept ;
    skos:historyNote "Compiled by the Geological Survey of Queensland" ;
    skos:broader geoad:MapSeries ;
    skos:definition "Map sheet for Humeburn at 1:100 000 scale. The first two digits define a longitude band 0.5 degree wide and the second two digits a latitude band 0.5 degree wide."@en ;
    skos:inScheme cs: ;
    skos:notation "7943" ;
    skos:prefLabel "Humeburn:7943"@en ;
.

geoad:Hungerford7740
    a skos:Concept ;
    skos:historyNote "Compiled by the Geological Survey of Queensland" ;
    skos:broader geoad:MapSeries ;
    skos:definition "Map sheet for Hungerford at 1:100 000 scale. The first two digits define a longitude band 0.5 degree wide and the second two digits a latitude band 0.5 degree wide."@en ;
    skos:inScheme cs: ;
    skos:notation "7740" ;
    skos:prefLabel "Hungerford:7740"@en ;
.

geoad:Iffley7160
    a skos:Concept ;
    skos:historyNote "Compiled by the Geological Survey of Queensland" ;
    skos:broader geoad:MapSeries ;
    skos:definition "Map sheet for Iffley at 1:100 000 scale. The first two digits define a longitude band 0.5 degree wide and the second two digits a latitude band 0.5 degree wide."@en ;
    skos:inScheme cs: ;
    skos:notation "7160" ;
    skos:prefLabel "Iffley:7160"@en ;
.

geoad:Ilfracombe7851
    a skos:Concept ;
    skos:historyNote "Compiled by the Geological Survey of Queensland" ;
    skos:broader geoad:MapSeries ;
    skos:definition "Map sheet for Ilfracombe at 1:100 000 scale. The first two digits define a longitude band 0.5 degree wide and the second two digits a latitude band 0.5 degree wide."@en ;
    skos:inScheme cs: ;
    skos:notation "7851" ;
    skos:prefLabel "Ilfracombe:7851"@en ;
.

geoad:Ingham8160
    a skos:Concept ;
    skos:historyNote "Compiled by the Geological Survey of Queensland" ;
    skos:broader geoad:MapSeries ;
    skos:definition "Map sheet for Ingham at 1:100 000 scale. The first two digits define a longitude band 0.5 degree wide and the second two digits a latitude band 0.5 degree wide."@en ;
    skos:inScheme cs: ;
    skos:notation "8160" ;
    skos:prefLabel "Ingham:8160"@en ;
.

geoad:Inglewood9141
    a skos:Concept ;
    skos:historyNote "Compiled by the Geological Survey of Queensland" ;
    skos:broader geoad:MapSeries ;
    skos:definition "Map sheet for Inglewood at 1:100 000 scale. The first two digits define a longitude band 0.5 degree wide and the second two digits a latitude band 0.5 degree wide."@en ;
    skos:inScheme cs: ;
    skos:notation "9141" ;
    skos:prefLabel "Inglewood:9141"@en ;
.

geoad:Injune8646
    a skos:Concept ;
    skos:historyNote "Compiled by the Geological Survey of Queensland" ;
    skos:broader geoad:MapSeries ;
    skos:definition "Map sheet for Injune at 1:100 000 scale. The first two digits define a longitude band 0.5 degree wide and the second two digits a latitude band 0.5 degree wide."@en ;
    skos:inScheme cs: ;
    skos:notation "8646" ;
    skos:prefLabel "Injune:8646"@en ;
.

geoad:Innamincka7042
    a skos:Concept ;
    skos:historyNote "Compiled by the Geological Survey of Queensland" ;
    skos:broader geoad:MapSeries ;
    skos:definition "Map sheet for Innamincka at 1:100 000 scale. The first two digits define a longitude band 0.5 degree wide and the second two digits a latitude band 0.5 degree wide."@en ;
    skos:inScheme cs: ;
    skos:notation "7042" ;
    skos:prefLabel "Innamincka:7042"@en ;
.

geoad:Innisfail8162
    a skos:Concept ;
    skos:historyNote "Compiled by the Geological Survey of Queensland" ;
    skos:broader geoad:MapSeries ;
    skos:definition "Map sheet for Innisfail at 1:100 000 scale. The first two digits define a longitude band 0.5 degree wide and the second two digits a latitude band 0.5 degree wide."@en ;
    skos:inScheme cs: ;
    skos:notation "8162" ;
    skos:prefLabel "Innisfail:8162"@en ;
.

geoad:Ipswich9442
    a skos:Concept ;
    skos:historyNote "Compiled by the Geological Survey of Queensland" ;
    skos:broader geoad:MapSeries ;
    skos:definition "Map sheet for Ipswich at 1:100 000 scale. The first two digits define a longitude band 0.5 degree wide and the second two digits a latitude band 0.5 degree wide."@en ;
    skos:inScheme cs: ;
    skos:notation "9442" ;
    skos:prefLabel "Ipswich:9442"@en ;
.

geoad:Isisford7749
    a skos:Concept ;
    skos:historyNote "Compiled by the Geological Survey of Queensland" ;
    skos:broader geoad:MapSeries ;
    skos:definition "Map sheet for Isisford at 1:100 000 scale. The first two digits define a longitude band 0.5 degree wide and the second two digits a latitude band 0.5 degree wide."@en ;
    skos:inScheme cs: ;
    skos:notation "7749" ;
    skos:prefLabel "Isisford:7749"@en ;
.

geoad:Jandowae9144
    a skos:Concept ;
    skos:historyNote "Compiled by the Geological Survey of Queensland" ;
    skos:broader geoad:MapSeries ;
    skos:definition "Map sheet for Jandowae at 1:100 000 scale. The first two digits define a longitude band 0.5 degree wide and the second two digits a latitude band 0.5 degree wide."@en ;
    skos:inScheme cs: ;
    skos:notation "9144" ;
    skos:prefLabel "Jandowae:9144"@en ;
.

geoad:JeannieRiver7868
    a skos:Concept ;
    skos:historyNote "Compiled by the Geological Survey of Queensland" ;
    skos:broader geoad:MapSeries ;
    skos:definition "Map sheet for Jeannie River at 1:100 000 scale. The first two digits define a longitude band 0.5 degree wide and the second two digits a latitude band 0.5 degree wide."@en ;
    skos:inScheme cs: ;
    skos:notation "7868" ;
    skos:prefLabel "Jeannie River:7868"@en ;
.

geoad:JeddaCreek7666
    a skos:Concept ;
    skos:historyNote "Compiled by the Geological Survey of Queensland" ;
    skos:broader geoad:MapSeries ;
    skos:definition "Map sheet for Jedda Creek at 1:100 000 scale. The first two digits define a longitude band 0.5 degree wide and the second two digits a latitude band 0.5 degree wide."@en ;
    skos:inScheme cs: ;
    skos:notation "7666" ;
    skos:prefLabel "Jedda Creek:7666"@en ;
.

geoad:Jericho8150
    a skos:Concept ;
    skos:historyNote "Compiled by the Geological Survey of Queensland" ;
    skos:broader geoad:MapSeries ;
    skos:definition "Map sheet for Jericho at 1:100 000 scale. The first two digits define a longitude band 0.5 degree wide and the second two digits a latitude band 0.5 degree wide."@en ;
    skos:inScheme cs: ;
    skos:notation "8150" ;
    skos:prefLabel "Jericho:8150"@en ;
.

geoad:JohnHills7353
    a skos:Concept ;
    skos:historyNote "Compiled by the Geological Survey of Queensland" ;
    skos:broader geoad:MapSeries ;
    skos:definition "Map sheet for John Hills at 1:100 000 scale. The first two digits define a longitude band 0.5 degree wide and the second two digits a latitude band 0.5 degree wide."@en ;
    skos:inScheme cs: ;
    skos:notation "7353" ;
    skos:prefLabel "John Hills:7353"@en ;
.

geoad:JuliaCreek7256
    a skos:Concept ;
    skos:historyNote "Compiled by the Geological Survey of Queensland" ;
    skos:broader geoad:MapSeries ;
    skos:definition "Map sheet for Julia Creek at 1:100 000 scale. The first two digits define a longitude band 0.5 degree wide and the second two digits a latitude band 0.5 degree wide."@en ;
    skos:inScheme cs: ;
    skos:notation "7256" ;
    skos:prefLabel "Julia Creek:7256"@en ;
.

geoad:Jundah7548
    a skos:Concept ;
    skos:historyNote "Compiled by the Geological Survey of Queensland" ;
    skos:broader geoad:MapSeries ;
    skos:definition "Map sheet for Jundah at 1:100 000 scale. The first two digits define a longitude band 0.5 degree wide and the second two digits a latitude band 0.5 degree wide."@en ;
    skos:inScheme cs: ;
    skos:notation "7548" ;
    skos:prefLabel "Jundah:7548"@en ;
.

geoad:Kalinga7667
    a skos:Concept ;
    skos:historyNote "Compiled by the Geological Survey of Queensland" ;
    skos:broader geoad:MapSeries ;
    skos:definition "Map sheet for Kalinga at 1:100 000 scale. The first two digits define a longitude band 0.5 degree wide and the second two digits a latitude band 0.5 degree wide."@en ;
    skos:inScheme cs: ;
    skos:notation "7667" ;
    skos:prefLabel "Kalinga:7667"@en ;
.

geoad:Kalkah7568
    a skos:Concept ;
    skos:historyNote "Compiled by the Geological Survey of Queensland" ;
    skos:broader geoad:MapSeries ;
    skos:definition "Map sheet for Kalkah at 1:100 000 scale. The first two digits define a longitude band 0.5 degree wide and the second two digits a latitude band 0.5 degree wide."@en ;
    skos:inScheme cs: ;
    skos:notation "7568" ;
    skos:prefLabel "Kalkah:7568"@en ;
.

geoad:Kamileroi6959
    a skos:Concept ;
    skos:historyNote "Compiled by the Geological Survey of Queensland" ;
    skos:broader geoad:MapSeries ;
    skos:definition "Map sheet for Kamileroi at 1:100 000 scale. The first two digits define a longitude band 0.5 degree wide and the second two digits a latitude band 0.5 degree wide."@en ;
    skos:inScheme cs: ;
    skos:notation "6959" ;
    skos:prefLabel "Kamileroi:6959"@en ;
.

geoad:KangarooHills8060
    a skos:Concept ;
    skos:historyNote "Compiled by the Geological Survey of Queensland" ;
    skos:broader geoad:MapSeries ;
    skos:definition "Map sheet for Kangaroo Hills at 1:100 000 scale. The first two digits define a longitude band 0.5 degree wide and the second two digits a latitude band 0.5 degree wide."@en ;
    skos:inScheme cs: ;
    skos:notation "8060" ;
    skos:prefLabel "Kangaroo Hills:8060"@en ;
.

geoad:Kanowana6842
    a skos:Concept ;
    skos:historyNote "Compiled by the Geological Survey of Queensland" ;
    skos:broader geoad:MapSeries ;
    skos:definition "Map sheet for Kanowana at 1:100 000 scale. The first two digits define a longitude band 0.5 degree wide and the second two digits a latitude band 0.5 degree wide."@en ;
    skos:inScheme cs: ;
    skos:notation "6842" ;
    skos:prefLabel "Kanowana:6842"@en ;
.

geoad:Karumba7063
    a skos:Concept ;
    skos:historyNote "Compiled by the Geological Survey of Queensland" ;
    skos:broader geoad:MapSeries ;
    skos:definition "Map sheet for Karumba at 1:100 000 scale. The first two digits define a longitude band 0.5 degree wide and the second two digits a latitude band 0.5 degree wide."@en ;
    skos:inScheme cs: ;
    skos:notation "7063" ;
    skos:prefLabel "Karumba:7063"@en ;
.

geoad:Katandra7654
    a skos:Concept ;
    skos:historyNote "Compiled by the Geological Survey of Queensland" ;
    skos:broader geoad:MapSeries ;
    skos:definition "Map sheet for Katandra at 1:100 000 scale. The first two digits define a longitude band 0.5 degree wide and the second two digits a latitude band 0.5 degree wide."@en ;
    skos:inScheme cs: ;
    skos:notation "7654" ;
    skos:prefLabel "Katandra:7654"@en ;
.

geoad:Keeroongooloo7446
    a skos:Concept ;
    skos:historyNote "Compiled by the Geological Survey of Queensland" ;
    skos:broader geoad:MapSeries ;
    skos:definition "Map sheet for Keeroongooloo at 1:100 000 scale. The first two digits define a longitude band 0.5 degree wide and the second two digits a latitude band 0.5 degree wide."@en ;
    skos:inScheme cs: ;
    skos:notation "7446" ;
    skos:prefLabel "Keeroongooloo:7446"@en ;
.

geoad:KendallRiver7369
    a skos:Concept ;
    skos:historyNote "Compiled by the Geological Survey of Queensland" ;
    skos:broader geoad:MapSeries ;
    skos:definition "Map sheet for Kendall River at 1:100 000 scale. The first two digits define a longitude band 0.5 degree wide and the second two digits a latitude band 0.5 degree wide."@en ;
    skos:inScheme cs: ;
    skos:notation "7369" ;
    skos:prefLabel "Kendall River:7369"@en ;
.

geoad:KennedyBend7767
    a skos:Concept ;
    skos:historyNote "Compiled by the Geological Survey of Queensland" ;
    skos:broader geoad:MapSeries ;
    skos:definition "Map sheet for Kennedy Bend at 1:100 000 scale. The first two digits define a longitude band 0.5 degree wide and the second two digits a latitude band 0.5 degree wide."@en ;
    skos:inScheme cs: ;
    skos:notation "7767" ;
    skos:prefLabel "Kennedy Bend:7767"@en ;
.

geoad:KennedyGap6757
    a skos:Concept ;
    skos:historyNote "Compiled by the Geological Survey of Queensland" ;
    skos:broader geoad:MapSeries ;
    skos:definition "Map sheet for Kennedy Gap at 1:100 000 scale. The first two digits define a longitude band 0.5 degree wide and the second two digits a latitude band 0.5 degree wide."@en ;
    skos:inScheme cs: ;
    skos:notation "6757" ;
    skos:prefLabel "Kennedy Gap:6757"@en ;
.

geoad:Kihee7443
    a skos:Concept ;
    skos:historyNote "Compiled by the Geological Survey of Queensland" ;
    skos:broader geoad:MapSeries ;
    skos:definition "Map sheet for Kihee at 1:100 000 scale. The first two digits define a longitude band 0.5 degree wide and the second two digits a latitude band 0.5 degree wide."@en ;
    skos:inScheme cs: ;
    skos:notation "7443" ;
    skos:prefLabel "Kihee:7443"@en ;
.

geoad:Kilcowera7640
    a skos:Concept ;
    skos:historyNote "Compiled by the Geological Survey of Queensland" ;
    skos:broader geoad:MapSeries ;
    skos:definition "Map sheet for Kilcowera at 1:100 000 scale. The first two digits define a longitude band 0.5 degree wide and the second two digits a latitude band 0.5 degree wide."@en ;
    skos:inScheme cs: ;
    skos:notation "7640" ;
    skos:prefLabel "Kilcowera:7640"@en ;
.

geoad:Kilcummin8453
    a skos:Concept ;
    skos:historyNote "Compiled by the Geological Survey of Queensland" ;
    skos:broader geoad:MapSeries ;
    skos:definition "Map sheet for Kilcummin at 1:100 000 scale. The first two digits define a longitude band 0.5 degree wide and the second two digits a latitude band 0.5 degree wide."@en ;
    skos:inScheme cs: ;
    skos:notation "8453" ;
    skos:prefLabel "Kilcummin:8453"@en ;
.

geoad:Kilterry7357
    a skos:Concept ;
    skos:historyNote "Compiled by the Geological Survey of Queensland" ;
    skos:broader geoad:MapSeries ;
    skos:definition "Map sheet for Kilterry at 1:100 000 scale. The first two digits define a longitude band 0.5 degree wide and the second two digits a latitude band 0.5 degree wide."@en ;
    skos:inScheme cs: ;
    skos:notation "7357" ;
    skos:prefLabel "Kilterry:7357"@en ;
.

geoad:Kingaroy9244
    a skos:Concept ;
    skos:historyNote "Compiled by the Geological Survey of Queensland" ;
    skos:broader geoad:MapSeries ;
    skos:definition "Map sheet for Kingaroy at 1:100 000 scale. The first two digits define a longitude band 0.5 degree wide and the second two digits a latitude band 0.5 degree wide."@en ;
    skos:inScheme cs: ;
    skos:notation "9244" ;
    skos:prefLabel "Kingaroy:9244"@en ;
.

geoad:KingfishLagoon7465
    a skos:Concept ;
    skos:historyNote "Compiled by the Geological Survey of Queensland" ;
    skos:broader geoad:MapSeries ;
    skos:definition "Map sheet for Kingfish Lagoon at 1:100 000 scale. The first two digits define a longitude band 0.5 degree wide and the second two digits a latitude band 0.5 degree wide."@en ;
    skos:inScheme cs: ;
    skos:notation "7465" ;
    skos:prefLabel "Kingfish Lagoon:7465"@en ;
.

geoad:Kirrama8061
    a skos:Concept ;
    skos:historyNote "Compiled by the Geological Survey of Queensland" ;
    skos:broader geoad:MapSeries ;
    skos:definition "Map sheet for Kirrama at 1:100 000 scale. The first two digits define a longitude band 0.5 degree wide and the second two digits a latitude band 0.5 degree wide."@en ;
    skos:inScheme cs: ;
    skos:notation "8061" ;
    skos:prefLabel "Kirrama:8061"@en ;
.

geoad:Kittakittaooloo6541
    a skos:Concept ;
    skos:historyNote "Compiled by the Geological Survey of Queensland" ;
    skos:broader geoad:MapSeries ;
    skos:definition "Map sheet for Kittakittaooloo at 1:100 000 scale. The first two digits define a longitude band 0.5 degree wide and the second two digits a latitude band 0.5 degree wide."@en ;
    skos:inScheme cs: ;
    skos:notation "6541" ;
    skos:prefLabel "Kittakittaooloo:6541"@en ;
.

geoad:Kogan9043
    a skos:Concept ;
    skos:historyNote "Compiled by the Geological Survey of Queensland" ;
    skos:broader geoad:MapSeries ;
    skos:definition "Map sheet for Kogan at 1:100 000 scale. The first two digits define a longitude band 0.5 degree wide and the second two digits a latitude band 0.5 degree wide."@en ;
    skos:inScheme cs: ;
    skos:notation "9043" ;
    skos:prefLabel "Kogan:9043"@en ;
.

geoad:Koolatah7366
    a skos:Concept ;
    skos:historyNote "Compiled by the Geological Survey of Queensland" ;
    skos:broader geoad:MapSeries ;
    skos:definition "Map sheet for Koolatah at 1:100 000 scale. The first two digits define a longitude band 0.5 degree wide and the second two digits a latitude band 0.5 degree wide."@en ;
    skos:inScheme cs: ;
    skos:notation "7366" ;
    skos:prefLabel "Koolatah:7366"@en ;
.

geoad:Koomarinna6544
    a skos:Concept ;
    skos:historyNote "Compiled by the Geological Survey of Queensland" ;
    skos:broader geoad:MapSeries ;
    skos:definition "Map sheet for Koomarinna at 1:100 000 scale. The first two digits define a longitude band 0.5 degree wide and the second two digits a latitude band 0.5 degree wide."@en ;
    skos:inScheme cs: ;
    skos:notation "6544" ;
    skos:prefLabel "Koomarinna:6544"@en ;
.

geoad:Kopperamanna6640
    a skos:Concept ;
    skos:historyNote "Compiled by the Geological Survey of Queensland" ;
    skos:broader geoad:MapSeries ;
    skos:definition "Map sheet for Kopperamanna at 1:100 000 scale. The first two digits define a longitude band 0.5 degree wide and the second two digits a latitude band 0.5 degree wide."@en ;
    skos:inScheme cs: ;
    skos:notation "6640" ;
    skos:prefLabel "Kopperamanna:6640"@en ;
.

geoad:Kungie7940
    a skos:Concept ;
    skos:historyNote "Compiled by the Geological Survey of Queensland" ;
    skos:broader geoad:MapSeries ;
    skos:definition "Map sheet for Kungie at 1:100 000 scale. The first two digits define a longitude band 0.5 degree wide and the second two digits a latitude band 0.5 degree wide."@en ;
    skos:inScheme cs: ;
    skos:notation "7940" ;
    skos:prefLabel "Kungie:7940"@en ;
.

geoad:Kynuna7254
    a skos:Concept ;
    skos:historyNote "Compiled by the Geological Survey of Queensland" ;
    skos:broader geoad:MapSeries ;
    skos:definition "Map sheet for Kynuna at 1:100 000 scale. The first two digits define a longitude band 0.5 degree wide and the second two digits a latitude band 0.5 degree wide."@en ;
    skos:inScheme cs: ;
    skos:notation "7254" ;
    skos:prefLabel "Kynuna:7254"@en ;
.

geoad:LagunaBay9545
    a skos:Concept ;
    skos:historyNote "Compiled by the Geological Survey of Queensland" ;
    skos:broader geoad:MapSeries ;
    skos:definition "Map sheet for Laguna Bay at 1:100 000 scale. The first two digits define a longitude band 0.5 degree wide and the second two digits a latitude band 0.5 degree wide."@en ;
    skos:inScheme cs: ;
    skos:notation "9545" ;
    skos:prefLabel "Laguna Bay:9545"@en ;
.

geoad:LakeDartmouth7945
    a skos:Concept ;
    skos:historyNote "Compiled by the Geological Survey of Queensland" ;
    skos:broader geoad:MapSeries ;
    skos:definition "Map sheet for Lake Dartmouth at 1:100 000 scale. The first two digits define a longitude band 0.5 degree wide and the second two digits a latitude band 0.5 degree wide."@en ;
    skos:inScheme cs: ;
    skos:notation "7945" ;
    skos:prefLabel "Lake Dartmouth:7945"@en ;
.

geoad:LakeHope6741
    a skos:Concept ;
    skos:historyNote "Compiled by the Geological Survey of Queensland" ;
    skos:broader geoad:MapSeries ;
    skos:definition "Map sheet for Lake Hope at 1:100 000 scale. The first two digits define a longitude band 0.5 degree wide and the second two digits a latitude band 0.5 degree wide."@en ;
    skos:inScheme cs: ;
    skos:notation "6741" ;
    skos:prefLabel "Lake Hope:6741"@en ;
.

geoad:LakeKatherine6653
    a skos:Concept ;
    skos:historyNote "Compiled by the Geological Survey of Queensland" ;
    skos:broader geoad:MapSeries ;
    skos:definition "Map sheet for Lake Katherine at 1:100 000 scale. The first two digits define a longitude band 0.5 degree wide and the second two digits a latitude band 0.5 degree wide."@en ;
    skos:inScheme cs: ;
    skos:notation "6653" ;
    skos:prefLabel "Lake Katherine:6653"@en ;
.

geoad:LakePoeppel6545
    a skos:Concept ;
    skos:historyNote "Compiled by the Geological Survey of Queensland" ;
    skos:broader geoad:MapSeries ;
    skos:definition "Map sheet for Lake Poeppel at 1:100 000 scale. The first two digits define a longitude band 0.5 degree wide and the second two digits a latitude band 0.5 degree wide."@en ;
    skos:inScheme cs: ;
    skos:notation "6545" ;
    skos:prefLabel "Lake Poeppel:6545"@en ;
.

geoad:LakePure7143
    a skos:Concept ;
    skos:historyNote "Compiled by the Geological Survey of Queensland" ;
    skos:broader geoad:MapSeries ;
    skos:definition "Map sheet for Lake Pure at 1:100 000 scale. The first two digits define a longitude band 0.5 degree wide and the second two digits a latitude band 0.5 degree wide."@en ;
    skos:inScheme cs: ;
    skos:notation "7143" ;
    skos:prefLabel "Lake Pure:7143"@en ;
.

geoad:LakeTorquinie6648
    a skos:Concept ;
    skos:historyNote "Compiled by the Geological Survey of Queensland" ;
    skos:broader geoad:MapSeries ;
    skos:definition "Map sheet for Lake Torquinie at 1:100 000 scale. The first two digits define a longitude band 0.5 degree wide and the second two digits a latitude band 0.5 degree wide."@en ;
    skos:inScheme cs: ;
    skos:notation "6648" ;
    skos:prefLabel "Lake Torquinie:6648"@en ;
.

geoad:LakeYammaYamma7145
    a skos:Concept ;
    skos:historyNote "Compiled by the Geological Survey of Queensland" ;
    skos:broader geoad:MapSeries ;
    skos:definition "Map sheet for Lake Yamma Yamma at 1:100 000 scale. The first two digits define a longitude band 0.5 degree wide and the second two digits a latitude band 0.5 degree wide."@en ;
    skos:inScheme cs: ;
    skos:notation "7145" ;
    skos:prefLabel "Lake Yamma Yamma:7145"@en ;
.

geoad:Lakefield7768
    a skos:Concept ;
    skos:historyNote "Compiled by the Geological Survey of Queensland" ;
    skos:broader geoad:MapSeries ;
    skos:definition "Map sheet for Lakefield at 1:100 000 scale. The first two digits define a longitude band 0.5 degree wide and the second two digits a latitude band 0.5 degree wide."@en ;
    skos:inScheme cs: ;
    skos:notation "7768" ;
    skos:prefLabel "Lakefield:7768"@en ;
.

geoad:Lammermoor7855
    a skos:Concept ;
    skos:historyNote "Compiled by the Geological Survey of Queensland" ;
    skos:broader geoad:MapSeries ;
    skos:definition "Map sheet for Lammermoor at 1:100 000 scale. The first two digits define a longitude band 0.5 degree wide and the second two digits a latitude band 0.5 degree wide."@en ;
    skos:inScheme cs: ;
    skos:notation "7855" ;
    skos:prefLabel "Lammermoor:7855"@en ;
.

geoad:LangloCrossing8045
    a skos:Concept ;
    skos:historyNote "Compiled by the Geological Survey of Queensland" ;
    skos:broader geoad:MapSeries ;
    skos:definition "Map sheet for Langlo Crossing at 1:100 000 scale. The first two digits define a longitude band 0.5 degree wide and the second two digits a latitude band 0.5 degree wide."@en ;
    skos:inScheme cs: ;
    skos:notation "8045" ;
    skos:prefLabel "Langlo Crossing:8045"@en ;
.

geoad:Lansdowne8147
    a skos:Concept ;
    skos:historyNote "Compiled by the Geological Survey of Queensland" ;
    skos:broader geoad:MapSeries ;
    skos:definition "Map sheet for Lansdowne at 1:100 000 scale. The first two digits define a longitude band 0.5 degree wide and the second two digits a latitude band 0.5 degree wide."@en ;
    skos:inScheme cs: ;
    skos:notation "8147" ;
    skos:prefLabel "Lansdowne:8147"@en ;
.

geoad:Laura7766
    a skos:Concept ;
    skos:historyNote "Compiled by the Geological Survey of Queensland" ;
    skos:broader geoad:MapSeries ;
    skos:definition "Map sheet for Laura at 1:100 000 scale. The first two digits define a longitude band 0.5 degree wide and the second two digits a latitude band 0.5 degree wide."@en ;
    skos:inScheme cs: ;
    skos:notation "7766" ;
    skos:prefLabel "Laura:7766"@en ;
.

geoad:LawnHill6660
    a skos:Concept ;
    skos:historyNote "Compiled by the Geological Survey of Queensland" ;
    skos:broader geoad:MapSeries ;
    skos:definition "Map sheet for Lawn Hill at 1:100 000 scale. The first two digits define a longitude band 0.5 degree wide and the second two digits a latitude band 0.5 degree wide."@en ;
    skos:inScheme cs: ;
    skos:notation "6660" ;
    skos:prefLabel "Lawn Hill:6660"@en ;
.

geoad:LesliePeak6753
    a skos:Concept ;
    skos:historyNote "Compiled by the Geological Survey of Queensland" ;
    skos:broader geoad:MapSeries ;
    skos:definition "Map sheet for Leslie Peak at 1:100 000 scale. The first two digits define a longitude band 0.5 degree wide and the second two digits a latitude band 0.5 degree wide."@en ;
    skos:inScheme cs: ;
    skos:notation "6753" ;
    skos:prefLabel "Leslie Peak:6753"@en ;
.

geoad:LightningRidge8439
    a skos:Concept ;
    skos:historyNote "Compiled by the Geological Survey of Queensland" ;
    skos:broader geoad:MapSeries ;
    skos:definition "Map sheet for Lightning Ridge at 1:100 000 scale. The first two digits define a longitude band 0.5 degree wide and the second two digits a latitude band 0.5 degree wide."@en ;
    skos:inScheme cs: ;
    skos:notation "8439" ;
    skos:prefLabel "Lightning Ridge:8439"@en ;
.

geoad:LindaDowns6553
    a skos:Concept ;
    skos:historyNote "Compiled by the Geological Survey of Queensland" ;
    skos:broader geoad:MapSeries ;
    skos:definition "Map sheet for Linda Downs at 1:100 000 scale. The first two digits define a longitude band 0.5 degree wide and the second two digits a latitude band 0.5 degree wide."@en ;
    skos:inScheme cs: ;
    skos:notation "6553" ;
    skos:prefLabel "Linda Downs:6553"@en ;
.

geoad:LindemanIsland8757
    a skos:Concept ;
    skos:historyNote "Compiled by the Geological Survey of Queensland" ;
    skos:broader geoad:MapSeries ;
    skos:definition "Map sheet for Lindeman Island at 1:100 000 scale. The first two digits define a longitude band 0.5 degree wide and the second two digits a latitude band 0.5 degree wide."@en ;
    skos:inScheme cs: ;
    skos:notation "8757" ;
    skos:prefLabel "Lindeman Island:8757"@en ;
.

geoad:Lismore9540
    a skos:Concept ;
    skos:historyNote "Compiled by the Geological Survey of Queensland" ;
    skos:broader geoad:MapSeries ;
    skos:definition "Map sheet for Lismore at 1:100 000 scale. The first two digits define a longitude band 0.5 degree wide and the second two digits a latitude band 0.5 degree wide."@en ;
    skos:inScheme cs: ;
    skos:notation "9540" ;
    skos:prefLabel "Lismore:9540"@en ;
.

geoad:ListowelDowns7947
    a skos:Concept ;
    skos:historyNote "Compiled by the Geological Survey of Queensland" ;
    skos:broader geoad:MapSeries ;
    skos:definition "Map sheet for Listowel Downs at 1:100 000 scale. The first two digits define a longitude band 0.5 degree wide and the second two digits a latitude band 0.5 degree wide."@en ;
    skos:inScheme cs: ;
    skos:notation "7947" ;
    skos:prefLabel "Listowel Downs:7947"@en ;
.

geoad:Lochiel7348
    a skos:Concept ;
    skos:historyNote "Compiled by the Geological Survey of Queensland" ;
    skos:broader geoad:MapSeries ;
    skos:definition "Map sheet for Lochiel at 1:100 000 scale. The first two digits define a longitude band 0.5 degree wide and the second two digits a latitude band 0.5 degree wide."@en ;
    skos:inScheme cs: ;
    skos:notation "7348" ;
    skos:prefLabel "Lochiel:7348"@en ;
.

geoad:LockhartRiver7571
    a skos:Concept ;
    skos:historyNote "Compiled by the Geological Survey of Queensland" ;
    skos:broader geoad:MapSeries ;
    skos:definition "Map sheet for Lockhart River at 1:100 000 scale. The first two digits define a longitude band 0.5 degree wide and the second two digits a latitude band 0.5 degree wide."@en ;
    skos:inScheme cs: ;
    skos:notation "7571" ;
    skos:prefLabel "Lockhart River:7571"@en ;
.

geoad:Loddon8044
    a skos:Concept ;
    skos:historyNote "Compiled by the Geological Survey of Queensland" ;
    skos:broader geoad:MapSeries ;
    skos:definition "Map sheet for Loddon at 1:100 000 scale. The first two digits define a longitude band 0.5 degree wide and the second two digits a latitude band 0.5 degree wide."@en ;
    skos:inScheme cs: ;
    skos:notation "8044" ;
    skos:prefLabel "Loddon:8044"@en ;
.

geoad:Lolworth7957
    a skos:Concept ;
    skos:historyNote "Compiled by the Geological Survey of Queensland" ;
    skos:broader geoad:MapSeries ;
    skos:definition "Map sheet for Lolworth at 1:100 000 scale. The first two digits define a longitude band 0.5 degree wide and the second two digits a latitude band 0.5 degree wide."@en ;
    skos:inScheme cs: ;
    skos:notation "7957" ;
    skos:prefLabel "Lolworth:7957"@en ;
.

geoad:Longreach7751
    a skos:Concept ;
    skos:historyNote "Compiled by the Geological Survey of Queensland" ;
    skos:broader geoad:MapSeries ;
    skos:definition "Map sheet for Longreach at 1:100 000 scale. The first two digits define a longitude band 0.5 degree wide and the second two digits a latitude band 0.5 degree wide."@en ;
    skos:inScheme cs: ;
    skos:notation "7751" ;
    skos:prefLabel "Longreach:7751"@en ;
.

geoad:LouLouPark8153
    a skos:Concept ;
    skos:historyNote "Compiled by the Geological Survey of Queensland" ;
    skos:broader geoad:MapSeries ;
    skos:definition "Map sheet for Lou Lou Park at 1:100 000 scale. The first two digits define a longitude band 0.5 degree wide and the second two digits a latitude band 0.5 degree wide."@en ;
    skos:inScheme cs: ;
    skos:notation "8153" ;
    skos:prefLabel "Lou Lou Park:8153"@en ;
.

geoad:LowareahPoint6765
    a skos:Concept ;
    skos:historyNote "Compiled by the Geological Survey of Queensland" ;
    skos:broader geoad:MapSeries ;
    skos:definition "Map sheet for Lowareah Point at 1:100 000 scale. The first two digits define a longitude band 0.5 degree wide and the second two digits a latitude band 0.5 degree wide."@en ;
    skos:inScheme cs: ;
    skos:notation "6765" ;
    skos:prefLabel "Lowareah Point:6765"@en ;
.

geoad:Lucknow7052
    a skos:Concept ;
    skos:historyNote "Compiled by the Geological Survey of Queensland" ;
    skos:broader geoad:MapSeries ;
    skos:definition "Map sheet for Lucknow at 1:100 000 scale. The first two digits define a longitude band 0.5 degree wide and the second two digits a latitude band 0.5 degree wide."@en ;
    skos:inScheme cs: ;
    skos:notation "7052" ;
    skos:prefLabel "Lucknow:7052"@en ;
.

geoad:LudgateHill7854
    a skos:Concept ;
    skos:historyNote "Compiled by the Geological Survey of Queensland" ;
    skos:broader geoad:MapSeries ;
    skos:definition "Map sheet for Ludgate Hill at 1:100 000 scale. The first two digits define a longitude band 0.5 degree wide and the second two digits a latitude band 0.5 degree wide."@en ;
    skos:inScheme cs: ;
    skos:notation "7854" ;
    skos:prefLabel "Ludgate Hill:7854"@en ;
.

geoad:Lyndbrook7762
    a skos:Concept ;
    skos:historyNote "Compiled by the Geological Survey of Queensland" ;
    skos:broader geoad:MapSeries ;
    skos:definition "Map sheet for Lyndbrook at 1:100 000 scale. The first two digits define a longitude band 0.5 degree wide and the second two digits a latitude band 0.5 degree wide."@en ;
    skos:inScheme cs: ;
    skos:notation "7762" ;
    skos:prefLabel "Lyndbrook:7762"@en ;
.

geoad:Lyndhurst7759
    a skos:Concept ;
    skos:historyNote "Compiled by the Geological Survey of Queensland" ;
    skos:broader geoad:MapSeries ;
    skos:definition "Map sheet for Lyndhurst at 1:100 000 scale. The first two digits define a longitude band 0.5 degree wide and the second two digits a latitude band 0.5 degree wide."@en ;
    skos:inScheme cs: ;
    skos:notation "7759" ;
    skos:prefLabel "Lyndhurst:7759"@en ;
.

geoad:MabuiagIsland7378
    a skos:Concept ;
    skos:historyNote "Compiled by the Geological Survey of Queensland" ;
    skos:broader geoad:MapSeries ;
    skos:definition "Map sheet for Mabuiag Island at 1:100 000 scale. The first two digits define a longitude band 0.5 degree wide and the second two digits a latitude band 0.5 degree wide."@en ;
    skos:inScheme cs: ;
    skos:notation "7378" ;
    skos:prefLabel "Mabuiag Island:7378"@en ;
.

geoad:Macaroni7164
    a skos:Concept ;
    skos:historyNote "Compiled by the Geological Survey of Queensland" ;
    skos:broader geoad:MapSeries ;
    skos:definition "Map sheet for Macaroni at 1:100 000 scale. The first two digits define a longitude band 0.5 degree wide and the second two digits a latitude band 0.5 degree wide."@en ;
    skos:inScheme cs: ;
    skos:notation "7164" ;
    skos:prefLabel "Macaroni:7164"@en ;
.

geoad:MacartneyRange7151
    a skos:Concept ;
    skos:historyNote "Compiled by the Geological Survey of Queensland" ;
    skos:broader geoad:MapSeries ;
    skos:definition "Map sheet for Macartney Range at 1:100 000 scale. The first two digits define a longitude band 0.5 degree wide and the second two digits a latitude band 0.5 degree wide."@en ;
    skos:inScheme cs: ;
    skos:notation "7151" ;
    skos:prefLabel "Macartney Range:7151"@en ;
.

geoad:Machattie6848
    a skos:Concept ;
    skos:historyNote "Compiled by the Geological Survey of Queensland" ;
    skos:broader geoad:MapSeries ;
    skos:definition "Map sheet for Machattie at 1:100 000 scale. The first two digits define a longitude band 0.5 degree wide and the second two digits a latitude band 0.5 degree wide."@en ;
    skos:inScheme cs: ;
    skos:notation "6848" ;
    skos:prefLabel "Machattie:6848"@en ;
.

geoad:Mackay8755
    a skos:Concept ;
    skos:historyNote "Compiled by the Geological Survey of Queensland" ;
    skos:broader geoad:MapSeries ;
    skos:definition "Map sheet for Mackay at 1:100 000 scale. The first two digits define a longitude band 0.5 degree wide and the second two digits a latitude band 0.5 degree wide."@en ;
    skos:inScheme cs: ;
    skos:notation "8755" ;
    skos:prefLabel "Mackay:8755"@en ;
.

geoad:Mackunda7152
    a skos:Concept ;
    skos:historyNote "Compiled by the Geological Survey of Queensland" ;
    skos:broader geoad:MapSeries ;
    skos:definition "Map sheet for Mackunda at 1:100 000 scale. The first two digits define a longitude band 0.5 degree wide and the second two digits a latitude band 0.5 degree wide."@en ;
    skos:inScheme cs: ;
    skos:notation "7152" ;
    skos:prefLabel "Mackunda:7152"@en ;
.

geoad:Magowra7062
    a skos:Concept ;
    skos:historyNote "Compiled by the Geological Survey of Queensland" ;
    skos:broader geoad:MapSeries ;
    skos:definition "Map sheet for Magowra at 1:100 000 scale. The first two digits define a longitude band 0.5 degree wide and the second two digits a latitude band 0.5 degree wide."@en ;
    skos:inScheme cs: ;
    skos:notation "7062" ;
    skos:prefLabel "Magowra:7062"@en ;
.

geoad:Mahrigong7653
    a skos:Concept ;
    skos:historyNote "Compiled by the Geological Survey of Queensland" ;
    skos:broader geoad:MapSeries ;
    skos:definition "Map sheet for Mahrigong at 1:100 000 scale. The first two digits define a longitude band 0.5 degree wide and the second two digits a latitude band 0.5 degree wide."@en ;
    skos:inScheme cs: ;
    skos:notation "7653" ;
    skos:prefLabel "Mahrigong:7653"@en ;
.

geoad:Malagarga7345
    a skos:Concept ;
    skos:historyNote "Compiled by the Geological Survey of Queensland" ;
    skos:broader geoad:MapSeries ;
    skos:definition "Map sheet for Malagarga at 1:100 000 scale. The first two digits define a longitude band 0.5 degree wide and the second two digits a latitude band 0.5 degree wide."@en ;
    skos:inScheme cs: ;
    skos:notation "7345" ;
    skos:prefLabel "Malagarga:7345"@en ;
.

geoad:Malbon6955
    a skos:Concept ;
    skos:historyNote "Compiled by the Geological Survey of Queensland" ;
    skos:broader geoad:MapSeries ;
    skos:definition "Map sheet for Malbon at 1:100 000 scale. The first two digits define a longitude band 0.5 degree wide and the second two digits a latitude band 0.5 degree wide."@en ;
    skos:inScheme cs: ;
    skos:notation "6955" ;
    skos:prefLabel "Malbon:6955"@en ;
.

geoad:Malpas7358
    a skos:Concept ;
    skos:historyNote "Compiled by the Geological Survey of Queensland" ;
    skos:broader geoad:MapSeries ;
    skos:definition "Map sheet for Malpas at 1:100 000 scale. The first two digits define a longitude band 0.5 degree wide and the second two digits a latitude band 0.5 degree wide."@en ;
    skos:inScheme cs: ;
    skos:notation "7358" ;
    skos:prefLabel "Malpas:7358"@en ;
.

geoad:MammothMines6758
    a skos:Concept ;
    skos:historyNote "Compiled by the Geological Survey of Queensland" ;
    skos:broader geoad:MapSeries ;
    skos:definition "Map sheet for Mammoth Mines at 1:100 000 scale. The first two digits define a longitude band 0.5 degree wide and the second two digits a latitude band 0.5 degree wide."@en ;
    skos:inScheme cs: ;
    skos:notation "6758" ;
    skos:prefLabel "Mammoth Mines:6758"@en ;
.

geoad:Maneroo7651
    a skos:Concept ;
    skos:historyNote "Compiled by the Geological Survey of Queensland" ;
    skos:broader geoad:MapSeries ;
    skos:definition "Map sheet for Maneroo at 1:100 000 scale. The first two digits define a longitude band 0.5 degree wide and the second two digits a latitude band 0.5 degree wide."@en ;
    skos:inScheme cs: ;
    skos:notation "7651" ;
    skos:prefLabel "Maneroo:7651"@en ;
.

geoad:MantuanDowns8349
    a skos:Concept ;
    skos:historyNote "Compiled by the Geological Survey of Queensland" ;
    skos:broader geoad:MapSeries ;
    skos:definition "Map sheet for Mantuan Downs at 1:100 000 scale. The first two digits define a longitude band 0.5 degree wide and the second two digits a latitude band 0.5 degree wide."@en ;
    skos:inScheme cs: ;
    skos:notation "8349" ;
    skos:prefLabel "Mantuan Downs:8349"@en ;
.

geoad:Manuka7554
    a skos:Concept ;
    skos:historyNote "Compiled by the Geological Survey of Queensland" ;
    skos:broader geoad:MapSeries ;
    skos:definition "Map sheet for Manuka at 1:100 000 scale. The first two digits define a longitude band 0.5 degree wide and the second two digits a latitude band 0.5 degree wide."@en ;
    skos:inScheme cs: ;
    skos:notation "7554" ;
    skos:prefLabel "Manuka:7554"@en ;
.

geoad:Mapoon7274
    a skos:Concept ;
    skos:historyNote "Compiled by the Geological Survey of Queensland" ;
    skos:broader geoad:MapSeries ;
    skos:definition "Map sheet for Mapoon at 1:100 000 scale. The first two digits define a longitude band 0.5 degree wide and the second two digits a latitude band 0.5 degree wide."@en ;
    skos:inScheme cs: ;
    skos:notation "7274" ;
    skos:prefLabel "Mapoon:7274"@en ;
.

geoad:Marathon7656
    a skos:Concept ;
    skos:historyNote "Compiled by the Geological Survey of Queensland" ;
    skos:broader geoad:MapSeries ;
    skos:definition "Map sheet for Marathon at 1:100 000 scale. The first two digits define a longitude band 0.5 degree wide and the second two digits a latitude band 0.5 degree wide."@en ;
    skos:inScheme cs: ;
    skos:notation "7656" ;
    skos:prefLabel "Marathon:7656"@en ;
.

geoad:Marduroo6849
    a skos:Concept ;
    skos:historyNote "Compiled by the Geological Survey of Queensland" ;
    skos:broader geoad:MapSeries ;
    skos:definition "Map sheet for Marduroo at 1:100 000 scale. The first two digits define a longitude band 0.5 degree wide and the second two digits a latitude band 0.5 degree wide."@en ;
    skos:inScheme cs: ;
    skos:notation "6849" ;
    skos:prefLabel "Marduroo:6849"@en ;
.

geoad:Mari7279
    a skos:Concept ;
    skos:historyNote "Compiled by the Geological Survey of Queensland" ;
    skos:broader geoad:MapSeries ;
    skos:definition "Map sheet for Mari at 1:100 000 scale. The first two digits define a longitude band 0.5 degree wide and the second two digits a latitude band 0.5 degree wide."@en ;
    skos:inScheme cs: ;
    skos:notation "7279" ;
    skos:prefLabel "Mari:7279"@en ;
.

geoad:MarinaPlains7668
    a skos:Concept ;
    skos:historyNote "Compiled by the Geological Survey of Queensland" ;
    skos:broader geoad:MapSeries ;
    skos:definition "Map sheet for Marina Plains at 1:100 000 scale. The first two digits define a longitude band 0.5 degree wide and the second two digits a latitude band 0.5 degree wide."@en ;
    skos:inScheme cs: ;
    skos:notation "7668" ;
    skos:prefLabel "Marina Plains:7668"@en ;
.

geoad:MarionDowns6851
    a skos:Concept ;
    skos:historyNote "Compiled by the Geological Survey of Queensland" ;
    skos:broader geoad:MapSeries ;
    skos:definition "Map sheet for Marion Downs at 1:100 000 scale. The first two digits define a longitude band 0.5 degree wide and the second two digits a latitude band 0.5 degree wide."@en ;
    skos:inScheme cs: ;
    skos:notation "6851" ;
    skos:prefLabel "Marion Downs:6851"@en ;
.

geoad:Marlborough8852
    a skos:Concept ;
    skos:historyNote "Compiled by the Geological Survey of Queensland" ;
    skos:broader geoad:MapSeries ;
    skos:definition "Map sheet for Marlborough at 1:100 000 scale. The first two digits define a longitude band 0.5 degree wide and the second two digits a latitude band 0.5 degree wide."@en ;
    skos:inScheme cs: ;
    skos:notation "8852" ;
    skos:prefLabel "Marlborough:8852"@en ;
.

geoad:Marraba6956
    a skos:Concept ;
    skos:historyNote "Compiled by the Geological Survey of Queensland" ;
    skos:broader geoad:MapSeries ;
    skos:definition "Map sheet for Marraba at 1:100 000 scale. The first two digits define a longitude band 0.5 degree wide and the second two digits a latitude band 0.5 degree wide."@en ;
    skos:inScheme cs: ;
    skos:notation "6956" ;
    skos:prefLabel "Marraba:6956"@en ;
.

geoad:MaryKathleen6856
    a skos:Concept ;
    skos:historyNote "Compiled by the Geological Survey of Queensland" ;
    skos:broader geoad:MapSeries ;
    skos:definition "Map sheet for Mary Kathleen at 1:100 000 scale. The first two digits define a longitude band 0.5 degree wide and the second two digits a latitude band 0.5 degree wide."@en ;
    skos:inScheme cs: ;
    skos:notation "6856" ;
    skos:prefLabel "Mary Kathleen:6856"@en ;
.

geoad:Maryborough9446
    a skos:Concept ;
    skos:historyNote "Compiled by the Geological Survey of Queensland" ;
    skos:broader geoad:MapSeries ;
    skos:definition "Map sheet for Maryborough at 1:100 000 scale. The first two digits define a longitude band 0.5 degree wide and the second two digits a latitude band 0.5 degree wide."@en ;
    skos:inScheme cs: ;
    skos:notation "9446" ;
    skos:prefLabel "Maryborough:9446"@en ;
.

geoad:Maryvale7958
    a skos:Concept ;
    skos:historyNote "Compiled by the Geological Survey of Queensland" ;
    skos:broader geoad:MapSeries ;
    skos:definition "Map sheet for Maryvale at 1:100 000 scale. The first two digits define a longitude band 0.5 degree wide and the second two digits a latitude band 0.5 degree wide."@en ;
    skos:inScheme cs: ;
    skos:notation "7958" ;
    skos:prefLabel "Maryvale:7958"@en ;
.

geoad:MassacreInlet6564
    a skos:Concept ;
    skos:historyNote "Compiled by the Geological Survey of Queensland" ;
    skos:broader geoad:MapSeries ;
    skos:definition "Map sheet for Massacre Inlet at 1:100 000 scale. The first two digits define a longitude band 0.5 degree wide and the second two digits a latitude band 0.5 degree wide."@en ;
    skos:inScheme cs: ;
    skos:notation "6564" ;
    skos:prefLabel "Massacre Inlet:6564"@en ;
.

geoad:Maxwelton7456
    a skos:Concept ;
    skos:historyNote "Compiled by the Geological Survey of Queensland" ;
    skos:broader geoad:MapSeries ;
    skos:definition "Map sheet for Maxwelton at 1:100 000 scale. The first two digits define a longitude band 0.5 degree wide and the second two digits a latitude band 0.5 degree wide."@en ;
    skos:inScheme cs: ;
    skos:notation "7456" ;
    skos:prefLabel "Maxwelton:7456"@en ;
.

geoad:Mayneside7450
    a skos:Concept ;
    skos:historyNote "Compiled by the Geological Survey of Queensland" ;
    skos:broader geoad:MapSeries ;
    skos:definition "Map sheet for Mayneside at 1:100 000 scale. The first two digits define a longitude band 0.5 degree wide and the second two digits a latitude band 0.5 degree wide."@en ;
    skos:inScheme cs: ;
    skos:notation "7450" ;
    skos:prefLabel "Mayneside:7450"@en ;
.

geoad:Maytown7765
    a skos:Concept ;
    skos:historyNote "Compiled by the Geological Survey of Queensland" ;
    skos:broader geoad:MapSeries ;
    skos:definition "Map sheet for Maytown at 1:100 000 scale. The first two digits define a longitude band 0.5 degree wide and the second two digits a latitude band 0.5 degree wide."@en ;
    skos:inScheme cs: ;
    skos:notation "7765" ;
    skos:prefLabel "Maytown:7765"@en ;
.

geoad:Mckinlay7155
    a skos:Concept ;
    skos:historyNote "Compiled by the Geological Survey of Queensland" ;
    skos:broader geoad:MapSeries ;
    skos:definition "Map sheet for Mckinlay at 1:100 000 scale. The first two digits define a longitude band 0.5 degree wide and the second two digits a latitude band 0.5 degree wide."@en ;
    skos:inScheme cs: ;
    skos:notation "7155" ;
    skos:prefLabel "Mckinlay:7155"@en ;
.

geoad:Meandarra8843
    a skos:Concept ;
    skos:historyNote "Compiled by the Geological Survey of Queensland" ;
    skos:broader geoad:MapSeries ;
    skos:definition "Map sheet for Meandarra at 1:100 000 scale. The first two digits define a longitude band 0.5 degree wide and the second two digits a latitude band 0.5 degree wide."@en ;
    skos:inScheme cs: ;
    skos:notation "8843" ;
    skos:prefLabel "Meandarra:8843"@en ;
.

geoad:Mekaree7848
    a skos:Concept ;
    skos:historyNote "Compiled by the Geological Survey of Queensland" ;
    skos:broader geoad:MapSeries ;
    skos:definition "Map sheet for Mekaree at 1:100 000 scale. The first two digits define a longitude band 0.5 degree wide and the second two digits a latitude band 0.5 degree wide."@en ;
    skos:inScheme cs: ;
    skos:notation "7848" ;
    skos:prefLabel "Mekaree:7848"@en ;
.

geoad:Merabooka7249
    a skos:Concept ;
    skos:historyNote "Compiled by the Geological Survey of Queensland" ;
    skos:broader geoad:MapSeries ;
    skos:definition "Map sheet for Merabooka at 1:100 000 scale. The first two digits define a longitude band 0.5 degree wide and the second two digits a latitude band 0.5 degree wide."@en ;
    skos:inScheme cs: ;
    skos:notation "7249" ;
    skos:prefLabel "Merabooka:7249"@en ;
.

geoad:Merapah7370
    a skos:Concept ;
    skos:historyNote "Compiled by the Geological Survey of Queensland" ;
    skos:broader geoad:MapSeries ;
    skos:definition "Map sheet for Merapah at 1:100 000 scale. The first two digits define a longitude band 0.5 degree wide and the second two digits a latitude band 0.5 degree wide."@en ;
    skos:inScheme cs: ;
    skos:notation "7370" ;
    skos:prefLabel "Merapah:7370"@en ;
.

geoad:Merluna7371
    a skos:Concept ;
    skos:historyNote "Compiled by the Geological Survey of Queensland" ;
    skos:broader geoad:MapSeries ;
    skos:definition "Map sheet for Merluna at 1:100 000 scale. The first two digits define a longitude band 0.5 degree wide and the second two digits a latitude band 0.5 degree wide."@en ;
    skos:inScheme cs: ;
    skos:notation "7371" ;
    skos:prefLabel "Merluna:7371"@en ;
.

geoad:MiddlePoint6962
    a skos:Concept ;
    skos:historyNote "Compiled by the Geological Survey of Queensland" ;
    skos:broader geoad:MapSeries ;
    skos:definition "Map sheet for Middle Point at 1:100 000 scale. The first two digits define a longitude band 0.5 degree wide and the second two digits a latitude band 0.5 degree wide."@en ;
    skos:inScheme cs: ;
    skos:notation "6962" ;
    skos:prefLabel "Middle Point:6962"@en ;
.

geoad:Middleton7253
    a skos:Concept ;
    skos:historyNote "Compiled by the Geological Survey of Queensland" ;
    skos:broader geoad:MapSeries ;
    skos:definition "Map sheet for Middleton at 1:100 000 scale. The first two digits define a longitude band 0.5 degree wide and the second two digits a latitude band 0.5 degree wide."@en ;
    skos:inScheme cs: ;
    skos:notation "7253" ;
    skos:prefLabel "Middleton:7253"@en ;
.

geoad:Miles8944
    a skos:Concept ;
    skos:historyNote "Compiled by the Geological Survey of Queensland" ;
    skos:broader geoad:MapSeries ;
    skos:definition "Map sheet for Miles at 1:100 000 scale. The first two digits define a longitude band 0.5 degree wide and the second two digits a latitude band 0.5 degree wide."@en ;
    skos:inScheme cs: ;
    skos:notation "8944" ;
    skos:prefLabel "Miles:8944"@en ;
.

geoad:Milgarra7061
    a skos:Concept ;
    skos:historyNote "Compiled by the Geological Survey of Queensland" ;
    skos:broader geoad:MapSeries ;
    skos:definition "Map sheet for Milgarra at 1:100 000 scale. The first two digits define a longitude band 0.5 degree wide and the second two digits a latitude band 0.5 degree wide."@en ;
    skos:inScheme cs: ;
    skos:notation "7061" ;
    skos:prefLabel "Milgarra:7061"@en ;
.

geoad:Millmerran9142
    a skos:Concept ;
    skos:historyNote "Compiled by the Geological Survey of Queensland" ;
    skos:broader geoad:MapSeries ;
    skos:definition "Map sheet for Millmerran at 1:100 000 scale. The first two digits define a longitude band 0.5 degree wide and the second two digits a latitude band 0.5 degree wide."@en ;
    skos:inScheme cs: ;
    skos:notation "9142" ;
    skos:prefLabel "Millmerran:9142"@en ;
.

geoad:Millungera7258
    a skos:Concept ;
    skos:historyNote "Compiled by the Geological Survey of Queensland" ;
    skos:broader geoad:MapSeries ;
    skos:definition "Map sheet for Millungera at 1:100 000 scale. The first two digits define a longitude band 0.5 degree wide and the second two digits a latitude band 0.5 degree wide."@en ;
    skos:inScheme cs: ;
    skos:notation "7258" ;
    skos:prefLabel "Millungera:7258"@en ;
.

geoad:Milo7746
    a skos:Concept ;
    skos:historyNote "Compiled by the Geological Survey of Queensland" ;
    skos:broader geoad:MapSeries ;
    skos:definition "Map sheet for Milo at 1:100 000 scale. The first two digits define a longitude band 0.5 degree wide and the second two digits a latitude band 0.5 degree wide."@en ;
    skos:inScheme cs: ;
    skos:notation "7746" ;
    skos:prefLabel "Milo:7746"@en ;
.

geoad:Milray8056
    a skos:Concept ;
    skos:historyNote "Compiled by the Geological Survey of Queensland" ;
    skos:broader geoad:MapSeries ;
    skos:definition "Map sheet for Milray at 1:100 000 scale. The first two digits define a longitude band 0.5 degree wide and the second two digits a latitude band 0.5 degree wide."@en ;
    skos:inScheme cs: ;
    skos:notation "8056" ;
    skos:prefLabel "Milray:8056"@en ;
.

geoad:Mingela8258
    a skos:Concept ;
    skos:historyNote "Compiled by the Geological Survey of Queensland" ;
    skos:broader geoad:MapSeries ;
    skos:definition "Map sheet for Mingela at 1:100 000 scale. The first two digits define a longitude band 0.5 degree wide and the second two digits a latitude band 0.5 degree wide."@en ;
    skos:inScheme cs: ;
    skos:notation "8258" ;
    skos:prefLabel "Mingela:8258"@en ;
.

geoad:Mirani8655
    a skos:Concept ;
    skos:historyNote "Compiled by the Geological Survey of Queensland" ;
    skos:broader geoad:MapSeries ;
    skos:definition "Map sheet for Mirani at 1:100 000 scale. The first two digits define a longitude band 0.5 degree wide and the second two digits a latitude band 0.5 degree wide."@en ;
    skos:inScheme cs: ;
    skos:notation "8655" ;
    skos:prefLabel "Mirani:8655"@en ;
.

geoad:MiriamVale9249
    a skos:Concept ;
    skos:historyNote "Compiled by the Geological Survey of Queensland" ;
    skos:broader geoad:MapSeries ;
    skos:definition "Map sheet for Miriam Vale at 1:100 000 scale. The first two digits define a longitude band 0.5 degree wide and the second two digits a latitude band 0.5 degree wide."@en ;
    skos:inScheme cs: ;
    skos:notation "9249" ;
    skos:prefLabel "Miriam Vale:9249"@en ;
.

geoad:MirraMitta6642
    a skos:Concept ;
    skos:historyNote "Compiled by the Geological Survey of Queensland" ;
    skos:broader geoad:MapSeries ;
    skos:definition "Map sheet for Mirra Mitta at 1:100 000 scale. The first two digits define a longitude band 0.5 degree wide and the second two digits a latitude band 0.5 degree wide."@en ;
    skos:inScheme cs: ;
    skos:notation "6642" ;
    skos:prefLabel "Mirra Mitta:6642"@en ;
.

geoad:MirricaBore6550
    a skos:Concept ;
    skos:historyNote "Compiled by the Geological Survey of Queensland" ;
    skos:broader geoad:MapSeries ;
    skos:definition "Map sheet for Mirrica Bore at 1:100 000 scale. The first two digits define a longitude band 0.5 degree wide and the second two digits a latitude band 0.5 degree wide."@en ;
    skos:inScheme cs: ;
    skos:notation "6550" ;
    skos:prefLabel "Mirrica Bore:6550"@en ;
.

geoad:Mitchell8445
    a skos:Concept ;
    skos:historyNote "Compiled by the Geological Survey of Queensland" ;
    skos:broader geoad:MapSeries ;
    skos:definition "Map sheet for Mitchell at 1:100 000 scale. The first two digits define a longitude band 0.5 degree wide and the second two digits a latitude band 0.5 degree wide."@en ;
    skos:inScheme cs: ;
    skos:notation "8445" ;
    skos:prefLabel "Mitchell:8445"@en ;
.

geoad:MitchellCreek9349
    a skos:Concept ;
    skos:historyNote "Compiled by the Geological Survey of Queensland" ;
    skos:broader geoad:MapSeries ;
    skos:definition "Map sheet for Mitchell Creek at 1:100 000 scale. The first two digits define a longitude band 0.5 degree wide and the second two digits a latitude band 0.5 degree wide."@en ;
    skos:inScheme cs: ;
    skos:notation "9349" ;
    skos:prefLabel "Mitchell Creek:9349"@en ;
.

geoad:MitchellRiver7267
    a skos:Concept ;
    skos:historyNote "Compiled by the Geological Survey of Queensland" ;
    skos:broader geoad:MapSeries ;
    skos:definition "Map sheet for Mitchell River at 1:100 000 scale. The first two digits define a longitude band 0.5 degree wide and the second two digits a latitude band 0.5 degree wide."@en ;
    skos:inScheme cs: ;
    skos:notation "7267" ;
    skos:prefLabel "Mitchell River:7267"@en ;
.

geoad:MoaIsland7377
    a skos:Concept ;
    skos:historyNote "Compiled by the Geological Survey of Queensland" ;
    skos:broader geoad:MapSeries ;
    skos:definition "Map sheet for Moa Island at 1:100 000 scale. The first two digits define a longitude band 0.5 degree wide and the second two digits a latitude band 0.5 degree wide."@en ;
    skos:inScheme cs: ;
    skos:notation "7377" ;
    skos:prefLabel "Moa Island:7377"@en ;
.

geoad:MogilMogil8639
    a skos:Concept ;
    skos:historyNote "Compiled by the Geological Survey of Queensland" ;
    skos:broader geoad:MapSeries ;
    skos:definition "Map sheet for Mogil Mogil at 1:100 000 scale. The first two digits define a longitude band 0.5 degree wide and the second two digits a latitude band 0.5 degree wide."@en ;
    skos:inScheme cs: ;
    skos:notation "8639" ;
    skos:prefLabel "Mogil Mogil:8639"@en ;
.

geoad:Monkira7048
    a skos:Concept ;
    skos:historyNote "Compiled by the Geological Survey of Queensland" ;
    skos:broader geoad:MapSeries ;
    skos:definition "Map sheet for Monkira at 1:100 000 scale. The first two digits define a longitude band 0.5 degree wide and the second two digits a latitude band 0.5 degree wide."@en ;
    skos:inScheme cs: ;
    skos:notation "7048" ;
    skos:prefLabel "Monkira:7048"@en ;
.

geoad:Monteagle8352
    a skos:Concept ;
    skos:historyNote "Compiled by the Geological Survey of Queensland" ;
    skos:broader geoad:MapSeries ;
    skos:definition "Map sheet for Monteagle at 1:100 000 scale. The first two digits define a longitude band 0.5 degree wide and the second two digits a latitude band 0.5 degree wide."@en ;
    skos:inScheme cs: ;
    skos:notation "8352" ;
    skos:prefLabel "Monteagle:8352"@en ;
.

geoad:Montecollina6839
    a skos:Concept ;
    skos:historyNote "Compiled by the Geological Survey of Queensland" ;
    skos:broader geoad:MapSeries ;
    skos:definition "Map sheet for Montecollina at 1:100 000 scale. The first two digits define a longitude band 0.5 degree wide and the second two digits a latitude band 0.5 degree wide."@en ;
    skos:inScheme cs: ;
    skos:notation "6839" ;
    skos:prefLabel "Montecollina:6839"@en ;
.

geoad:Monto9148
    a skos:Concept ;
    skos:historyNote "Compiled by the Geological Survey of Queensland" ;
    skos:broader geoad:MapSeries ;
    skos:definition "Map sheet for Monto at 1:100 000 scale. The first two digits define a longitude band 0.5 degree wide and the second two digits a latitude band 0.5 degree wide."@en ;
    skos:inScheme cs: ;
    skos:notation "9148" ;
    skos:prefLabel "Monto:9148"@en ;
.

geoad:Moonie8942
    a skos:Concept ;
    skos:historyNote "Compiled by the Geological Survey of Queensland" ;
    skos:broader geoad:MapSeries ;
    skos:definition "Map sheet for Moonie at 1:100 000 scale. The first two digits define a longitude band 0.5 degree wide and the second two digits a latitude band 0.5 degree wide."@en ;
    skos:inScheme cs: ;
    skos:notation "8942" ;
    skos:prefLabel "Moonie:8942"@en ;
.

geoad:Mooraberree7047
    a skos:Concept ;
    skos:historyNote "Compiled by the Geological Survey of Queensland" ;
    skos:broader geoad:MapSeries ;
    skos:definition "Map sheet for Mooraberree at 1:100 000 scale. The first two digits define a longitude band 0.5 degree wide and the second two digits a latitude band 0.5 degree wide."@en ;
    skos:inScheme cs: ;
    skos:notation "7047" ;
    skos:prefLabel "Mooraberree:7047"@en ;
.

geoad:Moree8839
    a skos:Concept ;
    skos:historyNote "Compiled by the Geological Survey of Queensland" ;
    skos:broader geoad:MapSeries ;
    skos:definition "Map sheet for Moree at 1:100 000 scale. The first two digits define a longitude band 0.5 degree wide and the second two digits a latitude band 0.5 degree wide."@en ;
    skos:inScheme cs: ;
    skos:notation "8839" ;
    skos:prefLabel "Moree:8839"@en ;
.

geoad:Moreton7473
    a skos:Concept ;
    skos:historyNote "Compiled by the Geological Survey of Queensland" ;
    skos:broader geoad:MapSeries ;
    skos:definition "Map sheet for Moreton at 1:100 000 scale. The first two digits define a longitude band 0.5 degree wide and the second two digits a latitude band 0.5 degree wide."@en ;
    skos:inScheme cs: ;
    skos:notation "7473" ;
    skos:prefLabel "Moreton:7473"@en ;
.

geoad:Mornington6764
    a skos:Concept ;
    skos:historyNote "Compiled by the Geological Survey of Queensland" ;
    skos:broader geoad:MapSeries ;
    skos:definition "Map sheet for Mornington at 1:100 000 scale. The first two digits define a longitude band 0.5 degree wide and the second two digits a latitude band 0.5 degree wide."@en ;
    skos:inScheme cs: ;
    skos:notation "6764" ;
    skos:prefLabel "Mornington:6764"@en ;
.

geoad:Morven8345
    a skos:Concept ;
    skos:historyNote "Compiled by the Geological Survey of Queensland" ;
    skos:broader geoad:MapSeries ;
    skos:definition "Map sheet for Morven at 1:100 000 scale. The first two digits define a longitude band 0.5 degree wide and the second two digits a latitude band 0.5 degree wide."@en ;
    skos:inScheme cs: ;
    skos:notation "8345" ;
    skos:prefLabel "Morven:8345"@en ;
.

geoad:Mossman7965
    a skos:Concept ;
    skos:historyNote "Compiled by the Geological Survey of Queensland" ;
    skos:broader geoad:MapSeries ;
    skos:definition "Map sheet for Mossman at 1:100 000 scale. The first two digits define a longitude band 0.5 degree wide and the second two digits a latitude band 0.5 degree wide."@en ;
    skos:inScheme cs: ;
    skos:notation "7965" ;
    skos:prefLabel "Mossman:7965"@en ;
.

geoad:MountAngelay7055
    a skos:Concept ;
    skos:historyNote "Compiled by the Geological Survey of Queensland" ;
    skos:broader geoad:MapSeries ;
    skos:definition "Map sheet for Mount Angelay at 1:100 000 scale. The first two digits define a longitude band 0.5 degree wide and the second two digits a latitude band 0.5 degree wide."@en ;
    skos:inScheme cs: ;
    skos:notation "7055" ;
    skos:prefLabel "Mount Angelay:7055"@en ;
.

geoad:MountBluffkin8752
    a skos:Concept ;
    skos:historyNote "Compiled by the Geological Survey of Queensland" ;
    skos:broader geoad:MapSeries ;
    skos:definition "Map sheet for Mount Bluffkin at 1:100 000 scale. The first two digits define a longitude band 0.5 degree wide and the second two digits a latitude band 0.5 degree wide."@en ;
    skos:inScheme cs: ;
    skos:notation "8752" ;
    skos:prefLabel "Mount Bluffkin:8752"@en ;
.

geoad:MountCoolon8355
    a skos:Concept ;
    skos:historyNote "Compiled by the Geological Survey of Queensland" ;
    skos:broader geoad:MapSeries ;
    skos:definition "Map sheet for Mount Coolon at 1:100 000 scale. The first two digits define a longitude band 0.5 degree wide and the second two digits a latitude band 0.5 degree wide."@en ;
    skos:inScheme cs: ;
    skos:notation "8355" ;
    skos:prefLabel "Mount Coolon:8355"@en ;
.

geoad:MountCuttiguree6948
    a skos:Concept ;
    skos:historyNote "Compiled by the Geological Survey of Queensland" ;
    skos:broader geoad:MapSeries ;
    skos:definition "Map sheet for Mount Cuttiguree at 1:100 000 scale. The first two digits define a longitude band 0.5 degree wide and the second two digits a latitude band 0.5 degree wide."@en ;
    skos:inScheme cs: ;
    skos:notation "6948" ;
    skos:prefLabel "Mount Cuttiguree:6948"@en ;
.

geoad:MountEdwardGraves7250
    a skos:Concept ;
    skos:historyNote "Compiled by the Geological Survey of Queensland" ;
    skos:broader geoad:MapSeries ;
    skos:definition "Map sheet for Mount Edward Graves at 1:100 000 scale. The first two digits define a longitude band 0.5 degree wide and the second two digits a latitude band 0.5 degree wide."@en ;
    skos:inScheme cs: ;
    skos:notation "7250" ;
    skos:prefLabel "Mount Edward Graves:7250"@en ;
.

geoad:MountHowe8547
    a skos:Concept ;
    skos:historyNote "Compiled by the Geological Survey of Queensland" ;
    skos:broader geoad:MapSeries ;
    skos:definition "Map sheet for Mount Howe at 1:100 000 scale. The first two digits define a longitude band 0.5 degree wide and the second two digits a latitude band 0.5 degree wide."@en ;
    skos:inScheme cs: ;
    skos:notation "8547" ;
    skos:prefLabel "Mount Howe:8547"@en ;
.

geoad:MountHowitt7344
    a skos:Concept ;
    skos:historyNote "Compiled by the Geological Survey of Queensland" ;
    skos:broader geoad:MapSeries ;
    skos:definition "Map sheet for Mount Howitt at 1:100 000 scale. The first two digits define a longitude band 0.5 degree wide and the second two digits a latitude band 0.5 degree wide."@en ;
    skos:inScheme cs: ;
    skos:notation "7344" ;
    skos:prefLabel "Mount Howitt:7344"@en ;
.

geoad:MountIsa6756
    a skos:Concept ;
    skos:historyNote "Compiled by the Geological Survey of Queensland" ;
    skos:broader geoad:MapSeries ;
    skos:definition "Map sheet for Mount Isa at 1:100 000 scale. The first two digits define a longitude band 0.5 degree wide and the second two digits a latitude band 0.5 degree wide."@en ;
    skos:inScheme cs: ;
    skos:notation "6756" ;
    skos:prefLabel "Mount Isa:6756"@en ;
.

geoad:MountLindesay9441
    a skos:Concept ;
    skos:historyNote "Compiled by the Geological Survey of Queensland" ;
    skos:broader geoad:MapSeries ;
    skos:definition "Map sheet for Mount Lindesay at 1:100 000 scale. The first two digits define a longitude band 0.5 degree wide and the second two digits a latitude band 0.5 degree wide."@en ;
    skos:inScheme cs: ;
    skos:notation "9441" ;
    skos:prefLabel "Mount Lindesay:9441"@en ;
.

geoad:MountMerlin6954
    a skos:Concept ;
    skos:historyNote "Compiled by the Geological Survey of Queensland" ;
    skos:broader geoad:MapSeries ;
    skos:definition "Map sheet for Mount Merlin at 1:100 000 scale. The first two digits define a longitude band 0.5 degree wide and the second two digits a latitude band 0.5 degree wide."@en ;
    skos:inScheme cs: ;
    skos:notation "6954" ;
    skos:prefLabel "Mount Merlin:6954"@en ;
.

geoad:MountMorgan8950
    a skos:Concept ;
    skos:historyNote "Compiled by the Geological Survey of Queensland" ;
    skos:broader geoad:MapSeries ;
    skos:definition "Map sheet for Mount Morgan at 1:100 000 scale. The first two digits define a longitude band 0.5 degree wide and the second two digits a latitude band 0.5 degree wide."@en ;
    skos:inScheme cs: ;
    skos:notation "8950" ;
    skos:prefLabel "Mount Morgan:8950"@en ;
.

geoad:MountMorris8046
    a skos:Concept ;
    skos:historyNote "Compiled by the Geological Survey of Queensland" ;
    skos:broader geoad:MapSeries ;
    skos:definition "Map sheet for Mount Morris at 1:100 000 scale. The first two digits define a longitude band 0.5 degree wide and the second two digits a latitude band 0.5 degree wide."@en ;
    skos:inScheme cs: ;
    skos:notation "8046" ;
    skos:prefLabel "Mount Morris:8046"@en ;
.

geoad:MountMulgrave7665
    a skos:Concept ;
    skos:historyNote "Compiled by the Geological Survey of Queensland" ;
    skos:broader geoad:MapSeries ;
    skos:definition "Map sheet for Mount Mulgrave at 1:100 000 scale. The first two digits define a longitude band 0.5 degree wide and the second two digits a latitude band 0.5 degree wide."@en ;
    skos:inScheme cs: ;
    skos:notation "7665" ;
    skos:prefLabel "Mount Mulgrave:7665"@en ;
.

geoad:MountMulligan7864
    a skos:Concept ;
    skos:historyNote "Compiled by the Geological Survey of Queensland" ;
    skos:broader geoad:MapSeries ;
    skos:definition "Map sheet for Mount Mulligan at 1:100 000 scale. The first two digits define a longitude band 0.5 degree wide and the second two digits a latitude band 0.5 degree wide."@en ;
    skos:inScheme cs: ;
    skos:notation "7864" ;
    skos:prefLabel "Mount Mulligan:7864"@en ;
.

geoad:MountNorman7558
    a skos:Concept ;
    skos:historyNote "Compiled by the Geological Survey of Queensland" ;
    skos:broader geoad:MapSeries ;
    skos:definition "Map sheet for Mount Norman at 1:100 000 scale. The first two digits define a longitude band 0.5 degree wide and the second two digits a latitude band 0.5 degree wide."@en ;
    skos:inScheme cs: ;
    skos:notation "7558" ;
    skos:prefLabel "Mount Norman:7558"@en ;
.

geoad:MountOscar6661
    a skos:Concept ;
    skos:historyNote "Compiled by the Geological Survey of Queensland" ;
    skos:broader geoad:MapSeries ;
    skos:definition "Map sheet for Mount Oscar at 1:100 000 scale. The first two digits define a longitude band 0.5 degree wide and the second two digits a latitude band 0.5 degree wide."@en ;
    skos:inScheme cs: ;
    skos:notation "6661" ;
    skos:prefLabel "Mount Oscar:6661"@en ;
.

geoad:MountOxide6759
    a skos:Concept ;
    skos:historyNote "Compiled by the Geological Survey of Queensland" ;
    skos:broader geoad:MapSeries ;
    skos:definition "Map sheet for Mount Oxide at 1:100 000 scale. The first two digits define a longitude band 0.5 degree wide and the second two digits a latitude band 0.5 degree wide."@en ;
    skos:inScheme cs: ;
    skos:notation "6759" ;
    skos:prefLabel "Mount Oxide:6759"@en ;
.

geoad:MountPerry9247
    a skos:Concept ;
    skos:historyNote "Compiled by the Geological Survey of Queensland" ;
    skos:broader geoad:MapSeries ;
    skos:definition "Map sheet for Mount Perry at 1:100 000 scale. The first two digits define a longitude band 0.5 degree wide and the second two digits a latitude band 0.5 degree wide."@en ;
    skos:inScheme cs: ;
    skos:notation "9247" ;
    skos:prefLabel "Mount Perry:9247"@en ;
.

geoad:MountRouse7445
    a skos:Concept ;
    skos:historyNote "Compiled by the Geological Survey of Queensland" ;
    skos:broader geoad:MapSeries ;
    skos:definition "Map sheet for Mount Rouse at 1:100 000 scale. The first two digits define a longitude band 0.5 degree wide and the second two digits a latitude band 0.5 degree wide."@en ;
    skos:inScheme cs: ;
    skos:notation "7445" ;
    skos:prefLabel "Mount Rouse:7445"@en ;
.

geoad:MountSurprise7761
    a skos:Concept ;
    skos:historyNote "Compiled by the Geological Survey of Queensland" ;
    skos:broader geoad:MapSeries ;
    skos:definition "Map sheet for Mount Surprise at 1:100 000 scale. The first two digits define a longitude band 0.5 degree wide and the second two digits a latitude band 0.5 degree wide."@en ;
    skos:inScheme cs: ;
    skos:notation "7761" ;
    skos:prefLabel "Mount Surprise:7761"@en ;
.

geoad:MountTarley6750
    a skos:Concept ;
    skos:historyNote "Compiled by the Geological Survey of Queensland" ;
    skos:broader geoad:MapSeries ;
    skos:definition "Map sheet for Mount Tarley at 1:100 000 scale. The first two digits define a longitude band 0.5 degree wide and the second two digits a latitude band 0.5 degree wide."@en ;
    skos:inScheme cs: ;
    skos:notation "6750" ;
    skos:prefLabel "Mount Tarley:6750"@en ;
.

geoad:MountTutah8154
    a skos:Concept ;
    skos:historyNote "Compiled by the Geological Survey of Queensland" ;
    skos:broader geoad:MapSeries ;
    skos:definition "Map sheet for Mount Tutah at 1:100 000 scale. The first two digits define a longitude band 0.5 degree wide and the second two digits a latitude band 0.5 degree wide."@en ;
    skos:inScheme cs: ;
    skos:notation "8154" ;
    skos:prefLabel "Mount Tutah:8154"@en ;
.

geoad:MountWhelan6651
    a skos:Concept ;
    skos:historyNote "Compiled by the Geological Survey of Queensland" ;
    skos:broader geoad:MapSeries ;
    skos:definition "Map sheet for Mount Whelan at 1:100 000 scale. The first two digits define a longitude band 0.5 degree wide and the second two digits a latitude band 0.5 degree wide."@en ;
    skos:inScheme cs: ;
    skos:notation "6651" ;
    skos:prefLabel "Mount Whelan:6651"@en ;
.

geoad:MountWoneeala6949
    a skos:Concept ;
    skos:historyNote "Compiled by the Geological Survey of Queensland" ;
    skos:broader geoad:MapSeries ;
    skos:definition "Map sheet for Mount Woneeala at 1:100 000 scale. The first two digits define a longitude band 0.5 degree wide and the second two digits a latitude band 0.5 degree wide."@en ;
    skos:inScheme cs: ;
    skos:notation "6949" ;
    skos:prefLabel "Mount Woneeala:6949"@en ;
.

geoad:Moura8848
    a skos:Concept ;
    skos:historyNote "Compiled by the Geological Survey of Queensland" ;
    skos:broader geoad:MapSeries ;
    skos:definition "Map sheet for Moura at 1:100 000 scale. The first two digits define a longitude band 0.5 degree wide and the second two digits a latitude band 0.5 degree wide."@en ;
    skos:inScheme cs: ;
    skos:notation "8848" ;
    skos:prefLabel "Moura:8848"@en ;
.

geoad:Muckadilla8544
    a skos:Concept ;
    skos:historyNote "Compiled by the Geological Survey of Queensland" ;
    skos:broader geoad:MapSeries ;
    skos:definition "Map sheet for Muckadilla at 1:100 000 scale. The first two digits define a longitude band 0.5 degree wide and the second two digits a latitude band 0.5 degree wide."@en ;
    skos:inScheme cs: ;
    skos:notation "8544" ;
    skos:prefLabel "Muckadilla:8544"@en ;
.

geoad:Mudloo6548
    a skos:Concept ;
    skos:historyNote "Compiled by the Geological Survey of Queensland" ;
    skos:broader geoad:MapSeries ;
    skos:definition "Map sheet for Mudloo at 1:100 000 scale. The first two digits define a longitude band 0.5 degree wide and the second two digits a latitude band 0.5 degree wide."@en ;
    skos:inScheme cs: ;
    skos:notation "6548" ;
    skos:prefLabel "Mudloo:6548"@en ;
.

geoad:Muggleton8745
    a skos:Concept ;
    skos:historyNote "Compiled by the Geological Survey of Queensland" ;
    skos:broader geoad:MapSeries ;
    skos:definition "Map sheet for Muggleton at 1:100 000 scale. The first two digits define a longitude band 0.5 degree wide and the second two digits a latitude band 0.5 degree wide."@en ;
    skos:inScheme cs: ;
    skos:notation "8745" ;
    skos:prefLabel "Muggleton:8745"@en ;
.

geoad:Mulka6641
    a skos:Concept ;
    skos:historyNote "Compiled by the Geological Survey of Queensland" ;
    skos:broader geoad:MapSeries ;
    skos:definition "Map sheet for Mulka at 1:100 000 scale. The first two digits define a longitude band 0.5 degree wide and the second two digits a latitude band 0.5 degree wide."@en ;
    skos:inScheme cs: ;
    skos:notation "6641" ;
    skos:prefLabel "Mulka:6641"@en ;
.

geoad:Muncoonie6647
    a skos:Concept ;
    skos:historyNote "Compiled by the Geological Survey of Queensland" ;
    skos:broader geoad:MapSeries ;
    skos:definition "Map sheet for Muncoonie at 1:100 000 scale. The first two digits define a longitude band 0.5 degree wide and the second two digits a latitude band 0.5 degree wide."@en ;
    skos:inScheme cs: ;
    skos:notation "6647" ;
    skos:prefLabel "Muncoonie:6647"@en ;
.

geoad:Mundubbera9146
    a skos:Concept ;
    skos:historyNote "Compiled by the Geological Survey of Queensland" ;
    skos:broader geoad:MapSeries ;
    skos:definition "Map sheet for Mundubbera at 1:100 000 scale. The first two digits define a longitude band 0.5 degree wide and the second two digits a latitude band 0.5 degree wide."@en ;
    skos:inScheme cs: ;
    skos:notation "9146" ;
    skos:prefLabel "Mundubbera:9146"@en ;
.

geoad:Mungana7763
    a skos:Concept ;
    skos:historyNote "Compiled by the Geological Survey of Queensland" ;
    skos:broader geoad:MapSeries ;
    skos:definition "Map sheet for Mungana at 1:100 000 scale. The first two digits define a longitude band 0.5 degree wide and the second two digits a latitude band 0.5 degree wide."@en ;
    skos:inScheme cs: ;
    skos:notation "7763" ;
    skos:prefLabel "Mungana:7763"@en ;
.

geoad:Murgon9245
    a skos:Concept ;
    skos:historyNote "Compiled by the Geological Survey of Queensland" ;
    skos:broader geoad:MapSeries ;
    skos:definition "Map sheet for Murgon at 1:100 000 scale. The first two digits define a longitude band 0.5 degree wide and the second two digits a latitude band 0.5 degree wide."@en ;
    skos:inScheme cs: ;
    skos:notation "9245" ;
    skos:prefLabel "Murgon:9245"@en ;
.

geoad:Murraturley6748
    a skos:Concept ;
    skos:historyNote "Compiled by the Geological Survey of Queensland" ;
    skos:broader geoad:MapSeries ;
    skos:definition "Map sheet for Murraturley at 1:100 000 scale. The first two digits define a longitude band 0.5 degree wide and the second two digits a latitude band 0.5 degree wide."@en ;
    skos:inScheme cs: ;
    skos:notation "6748" ;
    skos:prefLabel "Murraturley:6748"@en ;
.

geoad:MurrayIslands7778
    a skos:Concept ;
    skos:historyNote "Compiled by the Geological Survey of Queensland" ;
    skos:broader geoad:MapSeries ;
    skos:definition "Map sheet for Murray Islands at 1:100 000 scale. The first two digits define a longitude band 0.5 degree wide and the second two digits a latitude band 0.5 degree wide."@en ;
    skos:inScheme cs: ;
    skos:notation "7778" ;
    skos:prefLabel "Murray Islands:7778"@en ;
.

geoad:Murweh8143
    a skos:Concept ;
    skos:historyNote "Compiled by the Geological Survey of Queensland" ;
    skos:broader geoad:MapSeries ;
    skos:definition "Map sheet for Murweh at 1:100 000 scale. The first two digits define a longitude band 0.5 degree wide and the second two digits a latitude band 0.5 degree wide."@en ;
    skos:inScheme cs: ;
    skos:notation "8143" ;
    skos:prefLabel "Murweh:8143"@en ;
.

geoad:Murwillumbah9541
    a skos:Concept ;
    skos:historyNote "Compiled by the Geological Survey of Queensland" ;
    skos:broader geoad:MapSeries ;
    skos:definition "Map sheet for Murwillumbah at 1:100 000 scale. The first two digits define a longitude band 0.5 degree wide and the second two digits a latitude band 0.5 degree wide."@en ;
    skos:inScheme cs: ;
    skos:notation "9541" ;
    skos:prefLabel "Murwillumbah:9541"@en ;
.

geoad:Musselbrook6560
    a skos:Concept ;
    skos:historyNote "Compiled by the Geological Survey of Queensland" ;
    skos:broader geoad:MapSeries ;
    skos:definition "Map sheet for Musselbrook at 1:100 000 scale. The first two digits define a longitude band 0.5 degree wide and the second two digits a latitude band 0.5 degree wide."@en ;
    skos:inScheme cs: ;
    skos:notation "6560" ;
    skos:prefLabel "Musselbrook:6560"@en ;
.

geoad:Muttaburra7852
    a skos:Concept ;
    skos:historyNote "Compiled by the Geological Survey of Queensland" ;
    skos:broader geoad:MapSeries ;
    skos:definition "Map sheet for Muttaburra at 1:100 000 scale. The first two digits define a longitude band 0.5 degree wide and the second two digits a latitude band 0.5 degree wide."@en ;
    skos:inScheme cs: ;
    skos:notation "7852" ;
    skos:prefLabel "Muttaburra:7852"@en ;
.

geoad:Myally6859
    a skos:Concept ;
    skos:historyNote "Compiled by the Geological Survey of Queensland" ;
    skos:broader geoad:MapSeries ;
    skos:definition "Map sheet for Myally at 1:100 000 scale. The first two digits define a longitude band 0.5 degree wide and the second two digits a latitude band 0.5 degree wide."@en ;
    skos:inScheme cs: ;
    skos:notation "6859" ;
    skos:prefLabel "Myally:6859"@en ;
.

geoad:Naccowlah7342
    a skos:Concept ;
    skos:historyNote "Compiled by the Geological Survey of Queensland" ;
    skos:broader geoad:MapSeries ;
    skos:definition "Map sheet for Naccowlah at 1:100 000 scale. The first two digits define a longitude band 0.5 degree wide and the second two digits a latitude band 0.5 degree wide."@en ;
    skos:inScheme cs: ;
    skos:notation "7342" ;
    skos:prefLabel "Naccowlah:7342"@en ;
.

geoad:Nambour9444
    a skos:Concept ;
    skos:historyNote "Compiled by the Geological Survey of Queensland" ;
    skos:broader geoad:MapSeries ;
    skos:definition "Map sheet for Nambour at 1:100 000 scale. The first two digits define a longitude band 0.5 degree wide and the second two digits a latitude band 0.5 degree wide."@en ;
    skos:inScheme cs: ;
    skos:notation "9444" ;
    skos:prefLabel "Nambour:9444"@en ;
.

geoad:Nanango9344
    a skos:Concept ;
    skos:historyNote "Compiled by the Geological Survey of Queensland" ;
    skos:broader geoad:MapSeries ;
    skos:definition "Map sheet for Nanango at 1:100 000 scale. The first two digits define a longitude band 0.5 degree wide and the second two digits a latitude band 0.5 degree wide."@en ;
    skos:inScheme cs: ;
    skos:notation "9344" ;
    skos:prefLabel "Nanango:9344"@en ;
.

geoad:Nandowrie8449
    a skos:Concept ;
    skos:historyNote "Compiled by the Geological Survey of Queensland" ;
    skos:broader geoad:MapSeries ;
    skos:definition "Map sheet for Nandowrie at 1:100 000 scale. The first two digits define a longitude band 0.5 degree wide and the second two digits a latitude band 0.5 degree wide."@en ;
    skos:inScheme cs: ;
    skos:notation "8449" ;
    skos:prefLabel "Nandowrie:8449"@en ;
.

geoad:Nappamerry7142
    a skos:Concept ;
    skos:historyNote "Compiled by the Geological Survey of Queensland" ;
    skos:broader geoad:MapSeries ;
    skos:definition "Map sheet for Nappamerry at 1:100 000 scale. The first two digits define a longitude band 0.5 degree wide and the second two digits a latitude band 0.5 degree wide."@en ;
    skos:inScheme cs: ;
    skos:notation "7142" ;
    skos:prefLabel "Nappamerry:7142"@en ;
.

geoad:Naryilco7240
    a skos:Concept ;
    skos:historyNote "Compiled by the Geological Survey of Queensland" ;
    skos:broader geoad:MapSeries ;
    skos:definition "Map sheet for Naryilco at 1:100 000 scale. The first two digits define a longitude band 0.5 degree wide and the second two digits a latitude band 0.5 degree wide."@en ;
    skos:inScheme cs: ;
    skos:notation "7240" ;
    skos:prefLabel "Naryilco:7240"@en ;
.

geoad:NassauRiver7166
    a skos:Concept ;
    skos:historyNote "Compiled by the Geological Survey of Queensland" ;
    skos:broader geoad:MapSeries ;
    skos:definition "Map sheet for Nassau River at 1:100 000 scale. The first two digits define a longitude band 0.5 degree wide and the second two digits a latitude band 0.5 degree wide."@en ;
    skos:inScheme cs: ;
    skos:notation "7166" ;
    skos:prefLabel "Nassau River:7166"@en ;
.

geoad:NatalDowns8155
    a skos:Concept ;
    skos:historyNote "Compiled by the Geological Survey of Queensland" ;
    skos:broader geoad:MapSeries ;
    skos:definition "Map sheet for Natal Downs at 1:100 000 scale. The first two digits define a longitude band 0.5 degree wide and the second two digits a latitude band 0.5 degree wide."@en ;
    skos:inScheme cs: ;
    skos:notation "8155" ;
    skos:prefLabel "Natal Downs:8155"@en ;
.

geoad:Nebo8654
    a skos:Concept ;
    skos:historyNote "Compiled by the Geological Survey of Queensland" ;
    skos:broader geoad:MapSeries ;
    skos:definition "Map sheet for Nebo at 1:100 000 scale. The first two digits define a longitude band 0.5 degree wide and the second two digits a latitude band 0.5 degree wide."@en ;
    skos:inScheme cs: ;
    skos:notation "8654" ;
    skos:prefLabel "Nebo:8654"@en ;
.

geoad:NeeyambaHill6552
    a skos:Concept ;
    skos:historyNote "Compiled by the Geological Survey of Queensland" ;
    skos:broader geoad:MapSeries ;
    skos:definition "Map sheet for Neeyamba Hill at 1:100 000 scale. The first two digits define a longitude band 0.5 degree wide and the second two digits a latitude band 0.5 degree wide."@en ;
    skos:inScheme cs: ;
    skos:notation "6552" ;
    skos:prefLabel "Neeyamba Hill:6552"@en ;
.

geoad:Nelia7356
    a skos:Concept ;
    skos:historyNote "Compiled by the Geological Survey of Queensland" ;
    skos:broader geoad:MapSeries ;
    skos:definition "Map sheet for Nelia at 1:100 000 scale. The first two digits define a longitude band 0.5 degree wide and the second two digits a latitude band 0.5 degree wide."@en ;
    skos:inScheme cs: ;
    skos:notation "7356" ;
    skos:prefLabel "Nelia:7356"@en ;
.

geoad:NeumayerValley6961
    a skos:Concept ;
    skos:historyNote "Compiled by the Geological Survey of Queensland" ;
    skos:broader geoad:MapSeries ;
    skos:definition "Map sheet for Neumayer Valley at 1:100 000 scale. The first two digits define a longitude band 0.5 degree wide and the second two digits a latitude band 0.5 degree wide."@en ;
    skos:inScheme cs: ;
    skos:notation "6961" ;
    skos:prefLabel "Neumayer Valley:6961"@en ;
.

geoad:Nickavilla7745
    a skos:Concept ;
    skos:historyNote "Compiled by the Geological Survey of Queensland" ;
    skos:broader geoad:MapSeries ;
    skos:definition "Map sheet for Nickavilla at 1:100 000 scale. The first two digits define a longitude band 0.5 degree wide and the second two digits a latitude band 0.5 degree wide."@en ;
    skos:inScheme cs: ;
    skos:notation "7745" ;
    skos:prefLabel "Nickavilla:7745"@en ;
.

geoad:Noccundra7442
    a skos:Concept ;
    skos:historyNote "Compiled by the Geological Survey of Queensland" ;
    skos:broader geoad:MapSeries ;
    skos:definition "Map sheet for Noccundra at 1:100 000 scale. The first two digits define a longitude band 0.5 degree wide and the second two digits a latitude band 0.5 degree wide."@en ;
    skos:inScheme cs: ;
    skos:notation "7442" ;
    skos:prefLabel "Noccundra:7442"@en ;
.

geoad:Noorama8140
    a skos:Concept ;
    skos:historyNote "Compiled by the Geological Survey of Queensland" ;
    skos:broader geoad:MapSeries ;
    skos:definition "Map sheet for Noorama at 1:100 000 scale. The first two digits define a longitude band 0.5 degree wide and the second two digits a latitude band 0.5 degree wide."@en ;
    skos:inScheme cs: ;
    skos:notation "8140" ;
    skos:prefLabel "Noorama:8140"@en ;
.

geoad:NooyeahDowns7641
    a skos:Concept ;
    skos:historyNote "Compiled by the Geological Survey of Queensland" ;
    skos:broader geoad:MapSeries ;
    skos:definition "Map sheet for Nooyeah Downs at 1:100 000 scale. The first two digits define a longitude band 0.5 degree wide and the second two digits a latitude band 0.5 degree wide."@en ;
    skos:inScheme cs: ;
    skos:notation "7641" ;
    skos:prefLabel "Nooyeah Downs:7641"@en ;
.

geoad:Norfolk6559
    a skos:Concept ;
    skos:historyNote "Compiled by the Geological Survey of Queensland" ;
    skos:broader geoad:MapSeries ;
    skos:definition "Map sheet for Norfolk at 1:100 000 scale. The first two digits define a longitude band 0.5 degree wide and the second two digits a latitude band 0.5 degree wide."@en ;
    skos:inScheme cs: ;
    skos:notation "6559" ;
    skos:prefLabel "Norfolk:6559"@en ;
.

geoad:Normanton7162
    a skos:Concept ;
    skos:historyNote "Compiled by the Geological Survey of Queensland" ;
    skos:broader geoad:MapSeries ;
    skos:definition "Map sheet for Normanton at 1:100 000 scale. The first two digits define a longitude band 0.5 degree wide and the second two digits a latitude band 0.5 degree wide."@en ;
    skos:inScheme cs: ;
    skos:notation "7162" ;
    skos:prefLabel "Normanton:7162"@en ;
.

geoad:NorthHead7560
    a skos:Concept ;
    skos:historyNote "Compiled by the Geological Survey of Queensland" ;
    skos:broader geoad:MapSeries ;
    skos:definition "Map sheet for North Head at 1:100 000 scale. The first two digits define a longitude band 0.5 degree wide and the second two digits a latitude band 0.5 degree wide."@en ;
    skos:inScheme cs: ;
    skos:notation "7560" ;
    skos:prefLabel "North Head:7560"@en ;
.

geoad:NorthamptonDowns8048
    a skos:Concept ;
    skos:historyNote "Compiled by the Geological Survey of Queensland" ;
    skos:broader geoad:MapSeries ;
    skos:definition "Map sheet for Northampton Downs at 1:100 000 scale. The first two digits define a longitude band 0.5 degree wide and the second two digits a latitude band 0.5 degree wide."@en ;
    skos:inScheme cs: ;
    skos:notation "8048" ;
    skos:prefLabel "Northampton Downs:8048"@en ;
.

geoad:Numil7158
    a skos:Concept ;
    skos:historyNote "Compiled by the Geological Survey of Queensland" ;
    skos:broader geoad:MapSeries ;
    skos:definition "Map sheet for Numil at 1:100 000 scale. The first two digits define a longitude band 0.5 degree wide and the second two digits a latitude band 0.5 degree wide."@en ;
    skos:inScheme cs: ;
    skos:notation "7158" ;
    skos:prefLabel "Numil:7158"@en ;
.

geoad:Oakey9243
    a skos:Concept ;
    skos:historyNote "Compiled by the Geological Survey of Queensland" ;
    skos:broader geoad:MapSeries ;
    skos:definition "Map sheet for Oakey at 1:100 000 scale. The first two digits define a longitude band 0.5 degree wide and the second two digits a latitude band 0.5 degree wide."@en ;
    skos:inScheme cs: ;
    skos:notation "9243" ;
    skos:prefLabel "Oakey:9243"@en ;
.

geoad:Oakhampton7850
    a skos:Concept ;
    skos:historyNote "Compiled by the Geological Survey of Queensland" ;
    skos:broader geoad:MapSeries ;
    skos:definition "Map sheet for Oakhampton at 1:100 000 scale. The first two digits define a longitude band 0.5 degree wide and the second two digits a latitude band 0.5 degree wide."@en ;
    skos:inScheme cs: ;
    skos:notation "7850" ;
    skos:prefLabel "Oakhampton:7850"@en ;
.

geoad:Oakwood8146
    a skos:Concept ;
    skos:historyNote "Compiled by the Geological Survey of Queensland" ;
    skos:broader geoad:MapSeries ;
    skos:definition "Map sheet for Oakwood at 1:100 000 scale. The first two digits define a longitude band 0.5 degree wide and the second two digits a latitude band 0.5 degree wide."@en ;
    skos:inScheme cs: ;
    skos:notation "8146" ;
    skos:prefLabel "Oakwood:8146"@en ;
.

geoad:Oban6755
    a skos:Concept ;
    skos:historyNote "Compiled by the Geological Survey of Queensland" ;
    skos:broader geoad:MapSeries ;
    skos:definition "Map sheet for Oban at 1:100 000 scale. The first two digits define a longitude band 0.5 degree wide and the second two digits a latitude band 0.5 degree wide."@en ;
    skos:inScheme cs: ;
    skos:notation "6755" ;
    skos:prefLabel "Oban:6755"@en ;
.

geoad:OffshoreMap7277
    a skos:Concept ;
    skos:historyNote "Compiled by the Geological Survey of Queensland" ;
    skos:broader geoad:MapSeries ;
    skos:definition "Map sheet for Offshore Map at 1:100 000 scale. The first two digits define a longitude band 0.5 degree wide and the second two digits a latitude band 0.5 degree wide."@en ;
    skos:inScheme cs: ;
    skos:notation "7277" ;
    skos:prefLabel "Offshore Map:7277"@en ;
.

geoad:OffshoreMap7673
    a skos:Concept ;
    skos:historyNote "Compiled by the Geological Survey of Queensland" ;
    skos:broader geoad:MapSeries ;
    skos:definition "Map sheet for Offshore Map at 1:100 000 scale. The first two digits define a longitude band 0.5 degree wide and the second two digits a latitude band 0.5 degree wide."@en ;
    skos:inScheme cs: ;
    skos:notation "7673" ;
    skos:prefLabel "Offshore Map:7673"@en ;
.

geoad:OffshoreMap7674
    a skos:Concept ;
    skos:historyNote "Compiled by the Geological Survey of Queensland" ;
    skos:broader geoad:MapSeries ;
    skos:definition "Map sheet for Offshore Map at 1:100 000 scale. The first two digits define a longitude band 0.5 degree wide and the second two digits a latitude band 0.5 degree wide."@en ;
    skos:inScheme cs: ;
    skos:notation "7674" ;
    skos:prefLabel "Offshore Map:7674"@en ;
.

geoad:OffshoreMap7675
    a skos:Concept ;
    skos:historyNote "Compiled by the Geological Survey of Queensland" ;
    skos:broader geoad:MapSeries ;
    skos:definition "Map sheet for Offshore Map at 1:100 000 scale. The first two digits define a longitude band 0.5 degree wide and the second two digits a latitude band 0.5 degree wide."@en ;
    skos:inScheme cs: ;
    skos:notation "7675" ;
    skos:prefLabel "Offshore Map:7675"@en ;
.

geoad:OffshoreMap7676
    a skos:Concept ;
    skos:historyNote "Compiled by the Geological Survey of Queensland" ;
    skos:broader geoad:MapSeries ;
    skos:definition "Map sheet for Offshore Map at 1:100 000 scale. The first two digits define a longitude band 0.5 degree wide and the second two digits a latitude band 0.5 degree wide."@en ;
    skos:inScheme cs: ;
    skos:notation "7676" ;
    skos:prefLabel "Offshore Map:7676"@en ;
.

geoad:OffshoreMap7677
    a skos:Concept ;
    skos:historyNote "Compiled by the Geological Survey of Queensland" ;
    skos:broader geoad:MapSeries ;
    skos:definition "Map sheet for Offshore Map at 1:100 000 scale. The first two digits define a longitude band 0.5 degree wide and the second two digits a latitude band 0.5 degree wide."@en ;
    skos:inScheme cs: ;
    skos:notation "7677" ;
    skos:prefLabel "Offshore Map:7677"@en ;
.

geoad:OffshoreMap7770
    a skos:Concept ;
    skos:historyNote "Compiled by the Geological Survey of Queensland" ;
    skos:broader geoad:MapSeries ;
    skos:definition "Map sheet for Offshore Map at 1:100 000 scale. The first two digits define a longitude band 0.5 degree wide and the second two digits a latitude band 0.5 degree wide."@en ;
    skos:inScheme cs: ;
    skos:notation "7770" ;
    skos:prefLabel "Offshore Map:7770"@en ;
.

geoad:OffshoreMap7771
    a skos:Concept ;
    skos:historyNote "Compiled by the Geological Survey of Queensland" ;
    skos:broader geoad:MapSeries ;
    skos:definition "Map sheet for Offshore Map at 1:100 000 scale. The first two digits define a longitude band 0.5 degree wide and the second two digits a latitude band 0.5 degree wide."@en ;
    skos:inScheme cs: ;
    skos:notation "7771" ;
    skos:prefLabel "Offshore Map:7771"@en ;
.

geoad:OffshoreMap7773
    a skos:Concept ;
    skos:historyNote "Compiled by the Geological Survey of Queensland" ;
    skos:broader geoad:MapSeries ;
    skos:definition "Map sheet for Offshore Map at 1:100 000 scale. The first two digits define a longitude band 0.5 degree wide and the second two digits a latitude band 0.5 degree wide."@en ;
    skos:inScheme cs: ;
    skos:notation "7773" ;
    skos:prefLabel "Offshore Map:7773"@en ;
.

geoad:OffshoreMap7774
    a skos:Concept ;
    skos:historyNote "Compiled by the Geological Survey of Queensland" ;
    skos:broader geoad:MapSeries ;
    skos:definition "Map sheet for Offshore Map at 1:100 000 scale. The first two digits define a longitude band 0.5 degree wide and the second two digits a latitude band 0.5 degree wide."@en ;
    skos:inScheme cs: ;
    skos:notation "7774" ;
    skos:prefLabel "Offshore Map:7774"@en ;
.

geoad:OffshoreMap7775
    a skos:Concept ;
    skos:historyNote "Compiled by the Geological Survey of Queensland" ;
    skos:broader geoad:MapSeries ;
    skos:definition "Map sheet for Offshore Map at 1:100 000 scale. The first two digits define a longitude band 0.5 degree wide and the second two digits a latitude band 0.5 degree wide."@en ;
    skos:inScheme cs: ;
    skos:notation "7775" ;
    skos:prefLabel "Offshore Map:7775"@en ;
.

geoad:OffshoreMap7777
    a skos:Concept ;
    skos:historyNote "Compiled by the Geological Survey of Queensland" ;
    skos:broader geoad:MapSeries ;
    skos:definition "Map sheet for Offshore Map at 1:100 000 scale. The first two digits define a longitude band 0.5 degree wide and the second two digits a latitude band 0.5 degree wide."@en ;
    skos:inScheme cs: ;
    skos:notation "7777" ;
    skos:prefLabel "Offshore Map:7777"@en ;
.

geoad:OffshoreMap7779
    a skos:Concept ;
    skos:historyNote "Compiled by the Geological Survey of Queensland" ;
    skos:broader geoad:MapSeries ;
    skos:definition "Map sheet for Offshore Map at 1:100 000 scale. The first two digits define a longitude band 0.5 degree wide and the second two digits a latitude band 0.5 degree wide."@en ;
    skos:inScheme cs: ;
    skos:notation "7779" ;
    skos:prefLabel "Offshore Map:7779"@en ;
.

geoad:OffshoreMap7870
    a skos:Concept ;
    skos:historyNote "Compiled by the Geological Survey of Queensland" ;
    skos:broader geoad:MapSeries ;
    skos:definition "Map sheet for Offshore Map at 1:100 000 scale. The first two digits define a longitude band 0.5 degree wide and the second two digits a latitude band 0.5 degree wide."@en ;
    skos:inScheme cs: ;
    skos:notation "7870" ;
    skos:prefLabel "Offshore Map:7870"@en ;
.

geoad:OffshoreMap8068
    a skos:Concept ;
    skos:historyNote "Compiled by the Geological Survey of Queensland" ;
    skos:broader geoad:MapSeries ;
    skos:definition "Map sheet for Offshore Map at 1:100 000 scale. The first two digits define a longitude band 0.5 degree wide and the second two digits a latitude band 0.5 degree wide."@en ;
    skos:inScheme cs: ;
    skos:notation "8068" ;
    skos:prefLabel "Offshore Map:8068"@en ;
.

geoad:OffshoreMap8956
    a skos:Concept ;
    skos:historyNote "Compiled by the Geological Survey of Queensland" ;
    skos:broader geoad:MapSeries ;
    skos:definition "Map sheet for Offshore Map at 1:100 000 scale. The first two digits define a longitude band 0.5 degree wide and the second two digits a latitude band 0.5 degree wide."@en ;
    skos:inScheme cs: ;
    skos:notation "8956" ;
    skos:prefLabel "Offshore Map:8956"@en ;
.

geoad:OffshoreMap9448
    a skos:Concept ;
    skos:historyNote "Compiled by the Geological Survey of Queensland" ;
    skos:broader geoad:MapSeries ;
    skos:definition "Map sheet for Offshore Map at 1:100 000 scale. The first two digits define a longitude band 0.5 degree wide and the second two digits a latitude band 0.5 degree wide."@en ;
    skos:inScheme cs: ;
    skos:notation "9448" ;
    skos:prefLabel "Offshore Map:9448"@en ;
.

geoad:OliveDowns7239
    a skos:Concept ;
    skos:historyNote "Compiled by the Geological Survey of Queensland" ;
    skos:broader geoad:MapSeries ;
    skos:definition "Map sheet for Olive Downs at 1:100 000 scale. The first two digits define a longitude band 0.5 degree wide and the second two digits a latitude band 0.5 degree wide."@en ;
    skos:inScheme cs: ;
    skos:notation "7239" ;
    skos:prefLabel "Olive Downs:7239"@en ;
.

geoad:Oorindi7156
    a skos:Concept ;
    skos:historyNote "Compiled by the Geological Survey of Queensland" ;
    skos:broader geoad:MapSeries ;
    skos:definition "Map sheet for Oorindi at 1:100 000 scale. The first two digits define a longitude band 0.5 degree wide and the second two digits a latitude band 0.5 degree wide."@en ;
    skos:inScheme cs: ;
    skos:notation "7156" ;
    skos:prefLabel "Oorindi:7156"@en ;
.

geoad:Opalton7451
    a skos:Concept ;
    skos:historyNote "Compiled by the Geological Survey of Queensland" ;
    skos:broader geoad:MapSeries ;
    skos:definition "Map sheet for Opalton at 1:100 000 scale. The first two digits define a longitude band 0.5 degree wide and the second two digits a latitude band 0.5 degree wide."@en ;
    skos:inScheme cs: ;
    skos:notation "7451" ;
    skos:prefLabel "Opalton:7451"@en ;
.

geoad:Orallo8645
    a skos:Concept ;
    skos:historyNote "Compiled by the Geological Survey of Queensland" ;
    skos:broader geoad:MapSeries ;
    skos:definition "Map sheet for Orallo at 1:100 000 scale. The first two digits define a longitude band 0.5 degree wide and the second two digits a latitude band 0.5 degree wide."@en ;
    skos:inScheme cs: ;
    skos:notation "8645" ;
    skos:prefLabel "Orallo:8645"@en ;
.

geoad:OrfordBay7475
    a skos:Concept ;
    skos:historyNote "Compiled by the Geological Survey of Queensland" ;
    skos:broader geoad:MapSeries ;
    skos:definition "Map sheet for Orford Bay at 1:100 000 scale. The first two digits define a longitude band 0.5 degree wide and the second two digits a latitude band 0.5 degree wide."@en ;
    skos:inScheme cs: ;
    skos:notation "7475" ;
    skos:prefLabel "Orford Bay:7475"@en ;
.

geoad:Orientos7241
    a skos:Concept ;
    skos:historyNote "Compiled by the Geological Survey of Queensland" ;
    skos:broader geoad:MapSeries ;
    skos:definition "Map sheet for Orientos at 1:100 000 scale. The first two digits define a longitude band 0.5 degree wide and the second two digits a latitude band 0.5 degree wide."@en ;
    skos:inScheme cs: ;
    skos:notation "7241" ;
    skos:prefLabel "Orientos:7241"@en ;
.

geoad:Pajingo8156
    a skos:Concept ;
    skos:historyNote "Compiled by the Geological Survey of Queensland" ;
    skos:broader geoad:MapSeries ;
    skos:definition "Map sheet for Pajingo at 1:100 000 scale. The first two digits define a longitude band 0.5 degree wide and the second two digits a latitude band 0.5 degree wide."@en ;
    skos:inScheme cs: ;
    skos:notation "8156" ;
    skos:prefLabel "Pajingo:8156"@en ;
.

geoad:Palankarinna6540
    a skos:Concept ;
    skos:historyNote "Compiled by the Geological Survey of Queensland" ;
    skos:broader geoad:MapSeries ;
    skos:definition "Map sheet for Palankarinna at 1:100 000 scale. The first two digits define a longitude band 0.5 degree wide and the second two digits a latitude band 0.5 degree wide."@en ;
    skos:inScheme cs: ;
    skos:notation "6540" ;
    skos:prefLabel "Palankarinna:6540"@en ;
.

geoad:PalmIslands8260
    a skos:Concept ;
    skos:historyNote "Compiled by the Geological Survey of Queensland" ;
    skos:broader geoad:MapSeries ;
    skos:definition "Map sheet for Palm Islands at 1:100 000 scale. The first two digits define a longitude band 0.5 degree wide and the second two digits a latitude band 0.5 degree wide."@en ;
    skos:inScheme cs: ;
    skos:notation "8260" ;
    skos:prefLabel "Palm Islands:8260"@en ;
.

geoad:Palparara7148
    a skos:Concept ;
    skos:historyNote "Compiled by the Geological Survey of Queensland" ;
    skos:broader geoad:MapSeries ;
    skos:definition "Map sheet for Palparara at 1:100 000 scale. The first two digits define a longitude band 0.5 degree wide and the second two digits a latitude band 0.5 degree wide."@en ;
    skos:inScheme cs: ;
    skos:notation "7148" ;
    skos:prefLabel "Palparara:7148"@en ;
.

geoad:PandanusCreek7464
    a skos:Concept ;
    skos:historyNote "Compiled by the Geological Survey of Queensland" ;
    skos:broader geoad:MapSeries ;
    skos:definition "Map sheet for Pandanus Creek at 1:100 000 scale. The first two digits define a longitude band 0.5 degree wide and the second two digits a latitude band 0.5 degree wide."@en ;
    skos:inScheme cs: ;
    skos:notation "7464" ;
    skos:prefLabel "Pandanus Creek:7464"@en ;
.

geoad:PandiePandie6745
    a skos:Concept ;
    skos:historyNote "Compiled by the Geological Survey of Queensland" ;
    skos:broader geoad:MapSeries ;
    skos:definition "Map sheet for Pandie Pandie at 1:100 000 scale. The first two digits define a longitude band 0.5 degree wide and the second two digits a latitude band 0.5 degree wide."@en ;
    skos:inScheme cs: ;
    skos:notation "6745" ;
    skos:prefLabel "Pandie Pandie:6745"@en ;
.

geoad:ParadiseCreek7367
    a skos:Concept ;
    skos:historyNote "Compiled by the Geological Survey of Queensland" ;
    skos:broader geoad:MapSeries ;
    skos:definition "Map sheet for Paradise Creek at 1:100 000 scale. The first two digits define a longitude band 0.5 degree wide and the second two digits a latitude band 0.5 degree wide."@en ;
    skos:inScheme cs: ;
    skos:notation "7367" ;
    skos:prefLabel "Paradise Creek:7367"@en ;
.

geoad:Patchawara7043
    a skos:Concept ;
    skos:historyNote "Compiled by the Geological Survey of Queensland" ;
    skos:broader geoad:MapSeries ;
    skos:definition "Map sheet for Patchawara at 1:100 000 scale. The first two digits define a longitude band 0.5 degree wide and the second two digits a latitude band 0.5 degree wide."@en ;
    skos:inScheme cs: ;
    skos:notation "7043" ;
    skos:prefLabel "Patchawara:7043"@en ;
.

geoad:Pathraootara6543
    a skos:Concept ;
    skos:historyNote "Compiled by the Geological Survey of Queensland" ;
    skos:broader geoad:MapSeries ;
    skos:definition "Map sheet for Pathraootara at 1:100 000 scale. The first two digits define a longitude band 0.5 degree wide and the second two digits a latitude band 0.5 degree wide."@en ;
    skos:inScheme cs: ;
    skos:notation "6543" ;
    skos:prefLabel "Pathraootara:6543"@en ;
.

geoad:Peleenah7049
    a skos:Concept ;
    skos:historyNote "Compiled by the Geological Survey of Queensland" ;
    skos:broader geoad:MapSeries ;
    skos:definition "Map sheet for Peleenah at 1:100 000 scale. The first two digits define a longitude band 0.5 degree wide and the second two digits a latitude band 0.5 degree wide."@en ;
    skos:inScheme cs: ;
    skos:notation "7049" ;
    skos:prefLabel "Peleenah:7049"@en ;
.

geoad:Pelham7459
    a skos:Concept ;
    skos:historyNote "Compiled by the Geological Survey of Queensland" ;
    skos:broader geoad:MapSeries ;
    skos:definition "Map sheet for Pelham at 1:100 000 scale. The first two digits define a longitude band 0.5 degree wide and the second two digits a latitude band 0.5 degree wide."@en ;
    skos:inScheme cs: ;
    skos:notation "7459" ;
    skos:prefLabel "Pelham:7459"@en ;
.

geoad:PeninsulaRange9053
    a skos:Concept ;
    skos:historyNote "Compiled by the Geological Survey of Queensland" ;
    skos:broader geoad:MapSeries ;
    skos:definition "Map sheet for Peninsula Range at 1:100 000 scale. The first two digits define a longitude band 0.5 degree wide and the second two digits a latitude band 0.5 degree wide."@en ;
    skos:inScheme cs: ;
    skos:notation "9053" ;
    skos:prefLabel "Peninsula Range:9053"@en ;
.

geoad:PennefatherRiver7273
    a skos:Concept ;
    skos:historyNote "Compiled by the Geological Survey of Queensland" ;
    skos:broader geoad:MapSeries ;
    skos:definition "Map sheet for Pennefather River at 1:100 000 scale. The first two digits define a longitude band 0.5 degree wide and the second two digits a latitude band 0.5 degree wide."@en ;
    skos:inScheme cs: ;
    skos:notation "7273" ;
    skos:prefLabel "Pennefather River:7273"@en ;
.

geoad:Pentland7956
    a skos:Concept ;
    skos:historyNote "Compiled by the Geological Survey of Queensland" ;
    skos:broader geoad:MapSeries ;
    skos:definition "Map sheet for Pentland at 1:100 000 scale. The first two digits define a longitude band 0.5 degree wide and the second two digits a latitude band 0.5 degree wide."@en ;
    skos:inScheme cs: ;
    skos:notation "7956" ;
    skos:prefLabel "Pentland:7956"@en ;
.

geoad:PercyIsles8954
    a skos:Concept ;
    skos:historyNote "Compiled by the Geological Survey of Queensland" ;
    skos:broader geoad:MapSeries ;
    skos:definition "Map sheet for Percy Isles at 1:100 000 scale. The first two digits define a longitude band 0.5 degree wide and the second two digits a latitude band 0.5 degree wide."@en ;
    skos:inScheme cs: ;
    skos:notation "8954" ;
    skos:prefLabel "Percy Isles:8954"@en ;
.

geoad:Perigundi6742
    a skos:Concept ;
    skos:historyNote "Compiled by the Geological Survey of Queensland" ;
    skos:broader geoad:MapSeries ;
    skos:definition "Map sheet for Perigundi at 1:100 000 scale. The first two digits define a longitude band 0.5 degree wide and the second two digits a latitude band 0.5 degree wide."@en ;
    skos:inScheme cs: ;
    skos:notation "6742" ;
    skos:prefLabel "Perigundi:6742"@en ;
.

geoad:PetersLagoon7466
    a skos:Concept ;
    skos:historyNote "Compiled by the Geological Survey of Queensland" ;
    skos:broader geoad:MapSeries ;
    skos:definition "Map sheet for Peters Lagoon at 1:100 000 scale. The first two digits define a longitude band 0.5 degree wide and the second two digits a latitude band 0.5 degree wide."@en ;
    skos:inScheme cs: ;
    skos:notation "7466" ;
    skos:prefLabel "Peters Lagoon:7466"@en ;
.

geoad:Pialba9447
    a skos:Concept ;
    skos:historyNote "Compiled by the Geological Survey of Queensland" ;
    skos:broader geoad:MapSeries ;
    skos:definition "Map sheet for Pialba at 1:100 000 scale. The first two digits define a longitude band 0.5 degree wide and the second two digits a latitude band 0.5 degree wide."@en ;
    skos:inScheme cs: ;
    skos:notation "9447" ;
    skos:prefLabel "Pialba:9447"@en ;
.

geoad:Pinidary7542
    a skos:Concept ;
    skos:historyNote "Compiled by the Geological Survey of Queensland" ;
    skos:broader geoad:MapSeries ;
    skos:definition "Map sheet for Pinidary at 1:100 000 scale. The first two digits define a longitude band 0.5 degree wide and the second two digits a latitude band 0.5 degree wide."@en ;
    skos:inScheme cs: ;
    skos:notation "7542" ;
    skos:prefLabel "Pinidary:7542"@en ;
.

geoad:Pitteroo7441
    a skos:Concept ;
    skos:historyNote "Compiled by the Geological Survey of Queensland" ;
    skos:broader geoad:MapSeries ;
    skos:definition "Map sheet for Pitteroo at 1:100 000 scale. The first two digits define a longitude band 0.5 degree wide and the second two digits a latitude band 0.5 degree wide."@en ;
    skos:inScheme cs: ;
    skos:notation "7441" ;
    skos:prefLabel "Pitteroo:7441"@en ;
.

geoad:PlevnaDowns7444
    a skos:Concept ;
    skos:historyNote "Compiled by the Geological Survey of Queensland" ;
    skos:broader geoad:MapSeries ;
    skos:definition "Map sheet for Plevna Downs at 1:100 000 scale. The first two digits define a longitude band 0.5 degree wide and the second two digits a latitude band 0.5 degree wide."@en ;
    skos:inScheme cs: ;
    skos:notation "7444" ;
    skos:prefLabel "Plevna Downs:7444"@en ;
.

geoad:PoeppelCorner6546
    a skos:Concept ;
    skos:historyNote "Compiled by the Geological Survey of Queensland" ;
    skos:broader geoad:MapSeries ;
    skos:definition "Map sheet for Poeppel Corner at 1:100 000 scale. The first two digits define a longitude band 0.5 degree wide and the second two digits a latitude band 0.5 degree wide."@en ;
    skos:inScheme cs: ;
    skos:notation "6546" ;
    skos:prefLabel "Poeppel Corner:6546"@en ;
.

geoad:PointLookout9643
    a skos:Concept ;
    skos:historyNote "Compiled by the Geological Survey of Queensland" ;
    skos:broader geoad:MapSeries ;
    skos:definition "Map sheet for Point Lookout at 1:100 000 scale. The first two digits define a longitude band 0.5 degree wide and the second two digits a latitude band 0.5 degree wide."@en ;
    skos:inScheme cs: ;
    skos:notation "9643" ;
    skos:prefLabel "Point Lookout:9643"@en ;
.

geoad:PointParker6763
    a skos:Concept ;
    skos:historyNote "Compiled by the Geological Survey of Queensland" ;
    skos:broader geoad:MapSeries ;
    skos:definition "Map sheet for Point Parker at 1:100 000 scale. The first two digits define a longitude band 0.5 degree wide and the second two digits a latitude band 0.5 degree wide."@en ;
    skos:inScheme cs: ;
    skos:notation "6763" ;
    skos:prefLabel "Point Parker:6763"@en ;
.

geoad:PortlandDowns7849
    a skos:Concept ;
    skos:historyNote "Compiled by the Geological Survey of Queensland" ;
    skos:broader geoad:MapSeries ;
    skos:definition "Map sheet for Portland Downs at 1:100 000 scale. The first two digits define a longitude band 0.5 degree wide and the second two digits a latitude band 0.5 degree wide."@en ;
    skos:inScheme cs: ;
    skos:notation "7849" ;
    skos:prefLabel "Portland Downs:7849"@en ;
.

geoad:Potosi7853
    a skos:Concept ;
    skos:historyNote "Compiled by the Geological Survey of Queensland" ;
    skos:broader geoad:MapSeries ;
    skos:definition "Map sheet for Potosi at 1:100 000 scale. The first two digits define a longitude band 0.5 degree wide and the second two digits a latitude band 0.5 degree wide."@en ;
    skos:inScheme cs: ;
    skos:notation "7853" ;
    skos:prefLabel "Potosi:7853"@en ;
.

geoad:Prairie7856
    a skos:Concept ;
    skos:historyNote "Compiled by the Geological Survey of Queensland" ;
    skos:broader geoad:MapSeries ;
    skos:definition "Map sheet for Prairie at 1:100 000 scale. The first two digits define a longitude band 0.5 degree wide and the second two digits a latitude band 0.5 degree wide."@en ;
    skos:inScheme cs: ;
    skos:notation "7856" ;
    skos:prefLabel "Prairie:7856"@en ;
.

geoad:PrincessCharlotteBay7669
    a skos:Concept ;
    skos:historyNote "Compiled by the Geological Survey of Queensland" ;
    skos:broader geoad:MapSeries ;
    skos:definition "Map sheet for Princess Charlotte Bay at 1:100 000 scale. The first two digits define a longitude band 0.5 degree wide and the second two digits a latitude band 0.5 degree wide."@en ;
    skos:inScheme cs: ;
    skos:notation "7669" ;
    skos:prefLabel "Princess Charlotte Bay:7669"@en ;
.

geoad:Princhester8952
    a skos:Concept ;
    skos:historyNote "Compiled by the Geological Survey of Queensland" ;
    skos:broader geoad:MapSeries ;
    skos:definition "Map sheet for Princhester at 1:100 000 scale. The first two digits define a longitude band 0.5 degree wide and the second two digits a latitude band 0.5 degree wide."@en ;
    skos:inScheme cs: ;
    skos:notation "8952" ;
    skos:prefLabel "Princhester:8952"@en ;
.

geoad:Proserpine8657
    a skos:Concept ;
    skos:historyNote "Compiled by the Geological Survey of Queensland" ;
    skos:broader geoad:MapSeries ;
    skos:definition "Map sheet for Proserpine at 1:100 000 scale. The first two digits define a longitude band 0.5 degree wide and the second two digits a latitude band 0.5 degree wide."@en ;
    skos:inScheme cs: ;
    skos:notation "8657" ;
    skos:prefLabel "Proserpine:8657"@en ;
.

geoad:Prospect7360
    a skos:Concept ;
    skos:historyNote "Compiled by the Geological Survey of Queensland" ;
    skos:broader geoad:MapSeries ;
    skos:definition "Map sheet for Prospect at 1:100 000 scale. The first two digits define a longitude band 0.5 degree wide and the second two digits a latitude band 0.5 degree wide."@en ;
    skos:inScheme cs: ;
    skos:notation "7360" ;
    skos:prefLabel "Prospect:7360"@en ;
.

geoad:Prospector6857
    a skos:Concept ;
    skos:historyNote "Compiled by the Geological Survey of Queensland" ;
    skos:broader geoad:MapSeries ;
    skos:definition "Map sheet for Prospector at 1:100 000 scale. The first two digits define a longitude band 0.5 degree wide and the second two digits a latitude band 0.5 degree wide."@en ;
    skos:inScheme cs: ;
    skos:notation "6857" ;
    skos:prefLabel "Prospector:6857"@en ;
.

geoad:PrudhoeIsland8855
    a skos:Concept ;
    skos:historyNote "Compiled by the Geological Survey of Queensland" ;
    skos:broader geoad:MapSeries ;
    skos:definition "Map sheet for Prudhoe Island at 1:100 000 scale. The first two digits define a longitude band 0.5 degree wide and the second two digits a latitude band 0.5 degree wide."@en ;
    skos:inScheme cs: ;
    skos:notation "8855" ;
    skos:prefLabel "Prudhoe Island:8855"@en ;
.

geoad:Punjaub6761
    a skos:Concept ;
    skos:historyNote "Compiled by the Geological Survey of Queensland" ;
    skos:broader geoad:MapSeries ;
    skos:definition "Map sheet for Punjaub at 1:100 000 scale. The first two digits define a longitude band 0.5 degree wide and the second two digits a latitude band 0.5 degree wide."@en ;
    skos:inScheme cs: ;
    skos:notation "6761" ;
    skos:prefLabel "Punjaub:6761"@en ;
.

geoad:Quamby6957
    a skos:Concept ;
    skos:historyNote "Compiled by the Geological Survey of Queensland" ;
    skos:broader geoad:MapSeries ;
    skos:definition "Map sheet for Quamby at 1:100 000 scale. The first two digits define a longitude band 0.5 degree wide and the second two digits a latitude band 0.5 degree wide."@en ;
    skos:inScheme cs: ;
    skos:notation "6957" ;
    skos:prefLabel "Quamby:6957"@en ;
.

geoad:Quilpie7744
    a skos:Concept ;
    skos:historyNote "Compiled by the Geological Survey of Queensland" ;
    skos:broader geoad:MapSeries ;
    skos:definition "Map sheet for Quilpie at 1:100 000 scale. The first two digits define a longitude band 0.5 degree wide and the second two digits a latitude band 0.5 degree wide."@en ;
    skos:inScheme cs: ;
    skos:notation "7744" ;
    skos:prefLabel "Quilpie:7744"@en ;
.

geoad:RainbowPlain6944
    a skos:Concept ;
    skos:historyNote "Compiled by the Geological Survey of Queensland" ;
    skos:broader geoad:MapSeries ;
    skos:definition "Map sheet for Rainbow Plain at 1:100 000 scale. The first two digits define a longitude band 0.5 degree wide and the second two digits a latitude band 0.5 degree wide."@en ;
    skos:inScheme cs: ;
    skos:notation "6944" ;
    skos:prefLabel "Rainbow Plain:6944"@en ;
.

geoad:Ravenshoe7962
    a skos:Concept ;
    skos:historyNote "Compiled by the Geological Survey of Queensland" ;
    skos:broader geoad:MapSeries ;
    skos:definition "Map sheet for Ravenshoe at 1:100 000 scale. The first two digits define a longitude band 0.5 degree wide and the second two digits a latitude band 0.5 degree wide."@en ;
    skos:inScheme cs: ;
    skos:notation "7962" ;
    skos:prefLabel "Ravenshoe:7962"@en ;
.

geoad:Ravenswood8257
    a skos:Concept ;
    skos:historyNote "Compiled by the Geological Survey of Queensland" ;
    skos:broader geoad:MapSeries ;
    skos:definition "Map sheet for Ravenswood at 1:100 000 scale. The first two digits define a longitude band 0.5 degree wide and the second two digits a latitude band 0.5 degree wide."@en ;
    skos:inScheme cs: ;
    skos:notation "8257" ;
    skos:prefLabel "Ravenswood:8257"@en ;
.

geoad:Rawbelle9047
    a skos:Concept ;
    skos:historyNote "Compiled by the Geological Survey of Queensland" ;
    skos:broader geoad:MapSeries ;
    skos:definition "Map sheet for Rawbelle at 1:100 000 scale. The first two digits define a longitude band 0.5 degree wide and the second two digits a latitude band 0.5 degree wide."@en ;
    skos:inScheme cs: ;
    skos:notation "9047" ;
    skos:prefLabel "Rawbelle:9047"@en ;
.

geoad:Ray7645
    a skos:Concept ;
    skos:historyNote "Compiled by the Geological Survey of Queensland" ;
    skos:broader geoad:MapSeries ;
    skos:definition "Map sheet for Ray at 1:100 000 scale. The first two digits define a longitude band 0.5 degree wide and the second two digits a latitude band 0.5 degree wide."@en ;
    skos:inScheme cs: ;
    skos:notation "7645" ;
    skos:prefLabel "Ray:7645"@en ;
.

geoad:RedRiver7563
    a skos:Concept ;
    skos:historyNote "Compiled by the Geological Survey of Queensland" ;
    skos:broader geoad:MapSeries ;
    skos:definition "Map sheet for Red River at 1:100 000 scale. The first two digits define a longitude band 0.5 degree wide and the second two digits a latitude band 0.5 degree wide."@en ;
    skos:inScheme cs: ;
    skos:notation "7563" ;
    skos:prefLabel "Red River:7563"@en ;
.

geoad:RennelIsland7578
    a skos:Concept ;
    skos:historyNote "Compiled by the Geological Survey of Queensland" ;
    skos:broader geoad:MapSeries ;
    skos:definition "Map sheet for Rennel Island at 1:100 000 scale. The first two digits define a longitude band 0.5 degree wide and the second two digits a latitude band 0.5 degree wide."@en ;
    skos:inScheme cs: ;
    skos:notation "7578" ;
    skos:prefLabel "Rennel Island:7578"@en ;
.

geoad:Retreat7547
    a skos:Concept ;
    skos:historyNote "Compiled by the Geological Survey of Queensland" ;
    skos:broader geoad:MapSeries ;
    skos:definition "Map sheet for Retreat at 1:100 000 scale. The first two digits define a longitude band 0.5 degree wide and the second two digits a latitude band 0.5 degree wide."@en ;
    skos:inScheme cs: ;
    skos:notation "7547" ;
    skos:prefLabel "Retreat:7547"@en ;
.

geoad:Richmond7556
    a skos:Concept ;
    skos:historyNote "Compiled by the Geological Survey of Queensland" ;
    skos:broader geoad:MapSeries ;
    skos:definition "Map sheet for Richmond at 1:100 000 scale. The first two digits define a longitude band 0.5 degree wide and the second two digits a latitude band 0.5 degree wide."@en ;
    skos:inScheme cs: ;
    skos:notation "7556" ;
    skos:prefLabel "Richmond:7556"@en ;
.

geoad:Ridgelands8951
    a skos:Concept ;
    skos:historyNote "Compiled by the Geological Survey of Queensland" ;
    skos:broader geoad:MapSeries ;
    skos:definition "Map sheet for Ridgelands at 1:100 000 scale. The first two digits define a longitude band 0.5 degree wide and the second two digits a latitude band 0.5 degree wide."@en ;
    skos:inScheme cs: ;
    skos:notation "8951" ;
    skos:prefLabel "Ridgelands:8951"@en ;
.

geoad:Rimbanda7652
    a skos:Concept ;
    skos:historyNote "Compiled by the Geological Survey of Queensland" ;
    skos:broader geoad:MapSeries ;
    skos:definition "Map sheet for Rimbanda at 1:100 000 scale. The first two digits define a longitude band 0.5 degree wide and the second two digits a latitude band 0.5 degree wide."@en ;
    skos:inScheme cs: ;
    skos:notation "7652" ;
    skos:prefLabel "Rimbanda:7652"@en ;
.

geoad:Riversleigh6659
    a skos:Concept ;
    skos:historyNote "Compiled by the Geological Survey of Queensland" ;
    skos:broader geoad:MapSeries ;
    skos:definition "Map sheet for Riversleigh at 1:100 000 scale. The first two digits define a longitude band 0.5 degree wide and the second two digits a latitude band 0.5 degree wide."@en ;
    skos:inScheme cs: ;
    skos:notation "6659" ;
    skos:prefLabel "Riversleigh:6659"@en ;
.

geoad:Rockhampton9051
    a skos:Concept ;
    skos:historyNote "Compiled by the Geological Survey of Queensland" ;
    skos:broader geoad:MapSeries ;
    skos:definition "Map sheet for Rockhampton at 1:100 000 scale. The first two digits define a longitude band 0.5 degree wide and the second two digits a latitude band 0.5 degree wide."@en ;
    skos:inScheme cs: ;
    skos:notation "9051" ;
    skos:prefLabel "Rockhampton:9051"@en ;
.

geoad:RoddsBay9250
    a skos:Concept ;
    skos:historyNote "Compiled by the Geological Survey of Queensland" ;
    skos:broader geoad:MapSeries ;
    skos:definition "Map sheet for Rodds Bay at 1:100 000 scale. The first two digits define a longitude band 0.5 degree wide and the second two digits a latitude band 0.5 degree wide."@en ;
    skos:inScheme cs: ;
    skos:notation "9250" ;
    skos:prefLabel "Rodds Bay:9250"@en ;
.

geoad:Rokeby7470
    a skos:Concept ;
    skos:historyNote "Compiled by the Geological Survey of Queensland" ;
    skos:broader geoad:MapSeries ;
    skos:definition "Map sheet for Rokeby at 1:100 000 scale. The first two digits define a longitude band 0.5 degree wide and the second two digits a latitude band 0.5 degree wide."@en ;
    skos:inScheme cs: ;
    skos:notation "7470" ;
    skos:prefLabel "Rokeby:7470"@en ;
.

geoad:Rolleston8649
    a skos:Concept ;
    skos:historyNote "Compiled by the Geological Survey of Queensland" ;
    skos:broader geoad:MapSeries ;
    skos:definition "Map sheet for Rolleston at 1:100 000 scale. The first two digits define a longitude band 0.5 degree wide and the second two digits a latitude band 0.5 degree wide."@en ;
    skos:inScheme cs: ;
    skos:notation "8649" ;
    skos:prefLabel "Rolleston:8649"@en ;
.

geoad:Rollingstone8159
    a skos:Concept ;
    skos:historyNote "Compiled by the Geological Survey of Queensland" ;
    skos:broader geoad:MapSeries ;
    skos:definition "Map sheet for Rollingstone at 1:100 000 scale. The first two digits define a longitude band 0.5 degree wide and the second two digits a latitude band 0.5 degree wide."@en ;
    skos:inScheme cs: ;
    skos:notation "8159" ;
    skos:prefLabel "Rollingstone:8159"@en ;
.

geoad:Roma8644
    a skos:Concept ;
    skos:historyNote "Compiled by the Geological Survey of Queensland" ;
    skos:broader geoad:MapSeries ;
    skos:definition "Map sheet for Roma at 1:100 000 scale. The first two digits define a longitude band 0.5 degree wide and the second two digits a latitude band 0.5 degree wide."@en ;
    skos:inScheme cs: ;
    skos:notation "8644" ;
    skos:prefLabel "Roma:8644"@en ;
.

geoad:Rookwood8851
    a skos:Concept ;
    skos:historyNote "Compiled by the Geological Survey of Queensland" ;
    skos:broader geoad:MapSeries ;
    skos:definition "Map sheet for Rookwood at 1:100 000 scale. The first two digits define a longitude band 0.5 degree wide and the second two digits a latitude band 0.5 degree wide."@en ;
    skos:inScheme cs: ;
    skos:notation "8851" ;
    skos:prefLabel "Rookwood:8851"@en ;
.

geoad:Roseberth6846
    a skos:Concept ;
    skos:historyNote "Compiled by the Geological Survey of Queensland" ;
    skos:broader geoad:MapSeries ;
    skos:definition "Map sheet for Roseberth at 1:100 000 scale. The first two digits define a longitude band 0.5 degree wide and the second two digits a latitude band 0.5 degree wide."@en ;
    skos:inScheme cs: ;
    skos:notation "6846" ;
    skos:prefLabel "Roseberth:6846"@en ;
.

geoad:Rosebrook7351
    a skos:Concept ;
    skos:historyNote "Compiled by the Geological Survey of Queensland" ;
    skos:broader geoad:MapSeries ;
    skos:definition "Map sheet for Rosebrook at 1:100 000 scale. The first two digits define a longitude band 0.5 degree wide and the second two digits a latitude band 0.5 degree wide."@en ;
    skos:inScheme cs: ;
    skos:notation "7351" ;
    skos:prefLabel "Rosebrook:7351"@en ;
.

geoad:Rosedale9248
    a skos:Concept ;
    skos:historyNote "Compiled by the Geological Survey of Queensland" ;
    skos:broader geoad:MapSeries ;
    skos:definition "Map sheet for Rosedale at 1:100 000 scale. The first two digits define a longitude band 0.5 degree wide and the second two digits a latitude band 0.5 degree wide."@en ;
    skos:inScheme cs: ;
    skos:notation "9248" ;
    skos:prefLabel "Rosedale:9248"@en ;
.

geoad:Rubyvale8451
    a skos:Concept ;
    skos:historyNote "Compiled by the Geological Survey of Queensland" ;
    skos:broader geoad:MapSeries ;
    skos:definition "Map sheet for Rubyvale at 1:100 000 scale. The first two digits define a longitude band 0.5 degree wide and the second two digits a latitude band 0.5 degree wide."@en ;
    skos:inScheme cs: ;
    skos:notation "8451" ;
    skos:prefLabel "Rubyvale:8451"@en ;
.

geoad:Rumula7964
    a skos:Concept ;
    skos:historyNote "Compiled by the Geological Survey of Queensland" ;
    skos:broader geoad:MapSeries ;
    skos:definition "Map sheet for Rumula at 1:100 000 scale. The first two digits define a longitude band 0.5 degree wide and the second two digits a latitude band 0.5 degree wide."@en ;
    skos:inScheme cs: ;
    skos:notation "7964" ;
    skos:prefLabel "Rumula:7964"@en ;
.

geoad:Runnymede7457
    a skos:Concept ;
    skos:historyNote "Compiled by the Geological Survey of Queensland" ;
    skos:broader geoad:MapSeries ;
    skos:definition "Map sheet for Runnymede at 1:100 000 scale. The first two digits define a longitude band 0.5 degree wide and the second two digits a latitude band 0.5 degree wide."@en ;
    skos:inScheme cs: ;
    skos:notation "7457" ;
    skos:prefLabel "Runnymede:7457"@en ;
.

geoad:RutlandPlains7266
    a skos:Concept ;
    skos:historyNote "Compiled by the Geological Survey of Queensland" ;
    skos:broader geoad:MapSeries ;
    skos:definition "Map sheet for Rutland Plains at 1:100 000 scale. The first two digits define a longitude band 0.5 degree wide and the second two digits a latitude band 0.5 degree wide."@en ;
    skos:inScheme cs: ;
    skos:notation "7266" ;
    skos:prefLabel "Rutland Plains:7266"@en ;
.

geoad:Saibai7479
    a skos:Concept ;
    skos:historyNote "Compiled by the Geological Survey of Queensland" ;
    skos:broader geoad:MapSeries ;
    skos:definition "Map sheet for Saibai at 1:100 000 scale. The first two digits define a longitude band 0.5 degree wide and the second two digits a latitude band 0.5 degree wide."@en ;
    skos:inScheme cs: ;
    skos:notation "7479" ;
    skos:prefLabel "Saibai:7479"@en ;
.

geoad:SassieIsland7477
    a skos:Concept ;
    skos:historyNote "Compiled by the Geological Survey of Queensland" ;
    skos:broader geoad:MapSeries ;
    skos:definition "Map sheet for Sassie Island at 1:100 000 scale. The first two digits define a longitude band 0.5 degree wide and the second two digits a latitude band 0.5 degree wide."@en ;
    skos:inScheme cs: ;
    skos:notation "7477" ;
    skos:prefLabel "Sassie Island:7477"@en ;
.

geoad:SavannahDowns7259
    a skos:Concept ;
    skos:historyNote "Compiled by the Geological Survey of Queensland" ;
    skos:broader geoad:MapSeries ;
    skos:definition "Map sheet for Savannah Downs at 1:100 000 scale. The first two digits define a longitude band 0.5 degree wide and the second two digits a latitude band 0.5 degree wide."@en ;
    skos:inScheme cs: ;
    skos:notation "7259" ;
    skos:prefLabel "Savannah Downs:7259"@en ;
.

geoad:Scartwater8255
    a skos:Concept ;
    skos:historyNote "Compiled by the Geological Survey of Queensland" ;
    skos:broader geoad:MapSeries ;
    skos:definition "Map sheet for Scartwater at 1:100 000 scale. The first two digits define a longitude band 0.5 degree wide and the second two digits a latitude band 0.5 degree wide."@en ;
    skos:inScheme cs: ;
    skos:notation "8255" ;
    skos:prefLabel "Scartwater:8255"@en ;
.

geoad:Scawfell8856
    a skos:Concept ;
    skos:historyNote "Compiled by the Geological Survey of Queensland" ;
    skos:broader geoad:MapSeries ;
    skos:definition "Map sheet for Scawfell at 1:100 000 scale. The first two digits define a longitude band 0.5 degree wide and the second two digits a latitude band 0.5 degree wide."@en ;
    skos:inScheme cs: ;
    skos:notation "8856" ;
    skos:prefLabel "Scawfell:8856"@en ;
.

geoad:Scoria9048
    a skos:Concept ;
    skos:historyNote "Compiled by the Geological Survey of Queensland" ;
    skos:broader geoad:MapSeries ;
    skos:definition "Map sheet for Scoria at 1:100 000 scale. The first two digits define a longitude band 0.5 degree wide and the second two digits a latitude band 0.5 degree wide."@en ;
    skos:inScheme cs: ;
    skos:notation "9048" ;
    skos:prefLabel "Scoria:9048"@en ;
.

geoad:Selwyn7054
    a skos:Concept ;
    skos:historyNote "Compiled by the Geological Survey of Queensland" ;
    skos:broader geoad:MapSeries ;
    skos:definition "Map sheet for Selwyn at 1:100 000 scale. The first two digits define a longitude band 0.5 degree wide and the second two digits a latitude band 0.5 degree wide."@en ;
    skos:inScheme cs: ;
    skos:notation "7054" ;
    skos:prefLabel "Selwyn:7054"@en ;
.

geoad:ShelburneBay7474
    a skos:Concept ;
    skos:historyNote "Compiled by the Geological Survey of Queensland" ;
    skos:broader geoad:MapSeries ;
    skos:definition "Map sheet for Shelburne Bay at 1:100 000 scale. The first two digits define a longitude band 0.5 degree wide and the second two digits a latitude band 0.5 degree wide."@en ;
    skos:inScheme cs: ;
    skos:notation "7474" ;
    skos:prefLabel "Shelburne Bay:7474"@en ;
.

geoad:Shoalwater8953
    a skos:Concept ;
    skos:historyNote "Compiled by the Geological Survey of Queensland" ;
    skos:broader geoad:MapSeries ;
    skos:definition "Map sheet for Shoalwater at 1:100 000 scale. The first two digits define a longitude band 0.5 degree wide and the second two digits a latitude band 0.5 degree wide."@en ;
    skos:inScheme cs: ;
    skos:notation "8953" ;
    skos:prefLabel "Shoalwater:8953"@en ;
.

geoad:SilverPlains7670
    a skos:Concept ;
    skos:historyNote "Compiled by the Geological Survey of Queensland" ;
    skos:broader geoad:MapSeries ;
    skos:definition "Map sheet for Silver Plains at 1:100 000 scale. The first two digits define a longitude band 0.5 degree wide and the second two digits a latitude band 0.5 degree wide."@en ;
    skos:inScheme cs: ;
    skos:notation "7670" ;
    skos:prefLabel "Silver Plains:7670"@en ;
.

geoad:SkardonRiver7374
    a skos:Concept ;
    skos:historyNote "Compiled by the Geological Survey of Queensland" ;
    skos:broader geoad:MapSeries ;
    skos:definition "Map sheet for Skardon River at 1:100 000 scale. The first two digits define a longitude band 0.5 degree wide and the second two digits a latitude band 0.5 degree wide."@en ;
    skos:inScheme cs: ;
    skos:notation "7374" ;
    skos:prefLabel "Skardon River:7374"@en ;
.

geoad:SouthGalway7346
    a skos:Concept ;
    skos:historyNote "Compiled by the Geological Survey of Queensland" ;
    skos:broader geoad:MapSeries ;
    skos:definition "Map sheet for South Galway at 1:100 000 scale. The first two digits define a longitude band 0.5 degree wide and the second two digits a latitude band 0.5 degree wide."@en ;
    skos:inScheme cs: ;
    skos:notation "7346" ;
    skos:prefLabel "South Galway:7346"@en ;
.

geoad:SouthPalmerRiver7865
    a skos:Concept ;
    skos:historyNote "Compiled by the Geological Survey of Queensland" ;
    skos:broader geoad:MapSeries ;
    skos:definition "Map sheet for South Palmer River at 1:100 000 scale. The first two digits define a longitude band 0.5 degree wide and the second two digits a latitude band 0.5 degree wide."@en ;
    skos:inScheme cs: ;
    skos:notation "7865" ;
    skos:prefLabel "South Palmer River:7865"@en ;
.

geoad:Springfield7546
    a skos:Concept ;
    skos:historyNote "Compiled by the Geological Survey of Queensland" ;
    skos:broader geoad:MapSeries ;
    skos:definition "Map sheet for Springfield at 1:100 000 scale. The first two digits define a longitude band 0.5 degree wide and the second two digits a latitude band 0.5 degree wide."@en ;
    skos:inScheme cs: ;
    skos:notation "7546" ;
    skos:prefLabel "Springfield:7546"@en ;
.

geoad:Springsure8549
    a skos:Concept ;
    skos:historyNote "Compiled by the Geological Survey of Queensland" ;
    skos:broader geoad:MapSeries ;
    skos:definition "Map sheet for Springsure at 1:100 000 scale. The first two digits define a longitude band 0.5 degree wide and the second two digits a latitude band 0.5 degree wide."@en ;
    skos:inScheme cs: ;
    skos:notation "8549" ;
    skos:prefLabel "Springsure:8549"@en ;
.

geoad:Springvale7050
    a skos:Concept ;
    skos:historyNote "Compiled by the Geological Survey of Queensland" ;
    skos:broader geoad:MapSeries ;
    skos:definition "Map sheet for Springvale at 1:100 000 scale. The first two digits define a longitude band 0.5 degree wide and the second two digits a latitude band 0.5 degree wide."@en ;
    skos:inScheme cs: ;
    skos:notation "7050" ;
    skos:prefLabel "Springvale:7050"@en ;
.

geoad:StGeorge8641
    a skos:Concept ;
    skos:historyNote "Compiled by the Geological Survey of Queensland" ;
    skos:broader geoad:MapSeries ;
    skos:definition "Map sheet for St George at 1:100 000 scale. The first two digits define a longitude band 0.5 degree wide and the second two digits a latitude band 0.5 degree wide."@en ;
    skos:inScheme cs: ;
    skos:notation "8641" ;
    skos:prefLabel "St George:8641"@en ;
.

geoad:StLawrence8853
    a skos:Concept ;
    skos:historyNote "Compiled by the Geological Survey of Queensland" ;
    skos:broader geoad:MapSeries ;
    skos:definition "Map sheet for St Lawrence at 1:100 000 scale. The first two digits define a longitude band 0.5 degree wide and the second two digits a latitude band 0.5 degree wide."@en ;
    skos:inScheme cs: ;
    skos:notation "8853" ;
    skos:prefLabel "St Lawrence:8853"@en ;
.

geoad:StRonans7861
    a skos:Concept ;
    skos:historyNote "Compiled by the Geological Survey of Queensland" ;
    skos:broader geoad:MapSeries ;
    skos:definition "Map sheet for St Ronans at 1:100 000 scale. The first two digits define a longitude band 0.5 degree wide and the second two digits a latitude band 0.5 degree wide."@en ;
    skos:inScheme cs: ;
    skos:notation "7861" ;
    skos:prefLabel "St Ronans:7861"@en ;
.

geoad:StaatenRiver7364
    a skos:Concept ;
    skos:historyNote "Compiled by the Geological Survey of Queensland" ;
    skos:broader geoad:MapSeries ;
    skos:definition "Map sheet for Staaten River at 1:100 000 scale. The first two digits define a longitude band 0.5 degree wide and the second two digits a latitude band 0.5 degree wide."@en ;
    skos:inScheme cs: ;
    skos:notation "7364" ;
    skos:prefLabel "Staaten River:7364"@en ;
.

geoad:Stamford7655
    a skos:Concept ;
    skos:historyNote "Compiled by the Geological Survey of Queensland" ;
    skos:broader geoad:MapSeries ;
    skos:definition "Map sheet for Stamford at 1:100 000 scale. The first two digits define a longitude band 0.5 degree wide and the second two digits a latitude band 0.5 degree wide."@en ;
    skos:inScheme cs: ;
    skos:notation "7655" ;
    skos:prefLabel "Stamford:7655"@en ;
.

geoad:Stanthorpe9240
    a skos:Concept ;
    skos:historyNote "Compiled by the Geological Survey of Queensland" ;
    skos:broader geoad:MapSeries ;
    skos:definition "Map sheet for Stanthorpe at 1:100 000 scale. The first two digits define a longitude band 0.5 degree wide and the second two digits a latitude band 0.5 degree wide."@en ;
    skos:inScheme cs: ;
    skos:notation "9240" ;
    skos:prefLabel "Stanthorpe:9240"@en ;
.

geoad:Stirling7263
    a skos:Concept ;
    skos:historyNote "Compiled by the Geological Survey of Queensland" ;
    skos:broader geoad:MapSeries ;
    skos:definition "Map sheet for Stirling at 1:100 000 scale. The first two digits define a longitude band 0.5 degree wide and the second two digits a latitude band 0.5 degree wide."@en ;
    skos:inScheme cs: ;
    skos:notation "7263" ;
    skos:prefLabel "Stirling:7263"@en ;
.

geoad:Stonehenge7549
    a skos:Concept ;
    skos:historyNote "Compiled by the Geological Survey of Queensland" ;
    skos:broader geoad:MapSeries ;
    skos:definition "Map sheet for Stonehenge at 1:100 000 scale. The first two digits define a longitude band 0.5 degree wide and the second two digits a latitude band 0.5 degree wide."@en ;
    skos:inScheme cs: ;
    skos:notation "7549" ;
    skos:prefLabel "Stonehenge:7549"@en ;
.

geoad:Strathalbyn8357
    a skos:Concept ;
    skos:historyNote "Compiled by the Geological Survey of Queensland" ;
    skos:broader geoad:MapSeries ;
    skos:definition "Map sheet for Strathalbyn at 1:100 000 scale. The first two digits define a longitude band 0.5 degree wide and the second two digits a latitude band 0.5 degree wide."@en ;
    skos:inScheme cs: ;
    skos:notation "8357" ;
    skos:prefLabel "Strathalbyn:8357"@en ;
.

geoad:Strathburn7469
    a skos:Concept ;
    skos:historyNote "Compiled by the Geological Survey of Queensland" ;
    skos:broader geoad:MapSeries ;
    skos:definition "Map sheet for Strathburn at 1:100 000 scale. The first two digits define a longitude band 0.5 degree wide and the second two digits a latitude band 0.5 degree wide."@en ;
    skos:inScheme cs: ;
    skos:notation "7469" ;
    skos:prefLabel "Strathburn:7469"@en ;
.

geoad:Strathconan8751
    a skos:Concept ;
    skos:historyNote "Compiled by the Geological Survey of Queensland" ;
    skos:broader geoad:MapSeries ;
    skos:definition "Map sheet for Strathconan at 1:100 000 scale. The first two digits define a longitude band 0.5 degree wide and the second two digits a latitude band 0.5 degree wide."@en ;
    skos:inScheme cs: ;
    skos:notation "8751" ;
    skos:prefLabel "Strathconan:8751"@en ;
.

geoad:Strathgordon7368
    a skos:Concept ;
    skos:historyNote "Compiled by the Geological Survey of Queensland" ;
    skos:broader geoad:MapSeries ;
    skos:definition "Map sheet for Strathgordon at 1:100 000 scale. The first two digits define a longitude band 0.5 degree wide and the second two digits a latitude band 0.5 degree wide."@en ;
    skos:inScheme cs: ;
    skos:notation "7368" ;
    skos:prefLabel "Strathgordon:7368"@en ;
.

geoad:Strathleven7566
    a skos:Concept ;
    skos:historyNote "Compiled by the Geological Survey of Queensland" ;
    skos:broader geoad:MapSeries ;
    skos:definition "Map sheet for Strathleven at 1:100 000 scale. The first two digits define a longitude band 0.5 degree wide and the second two digits a latitude band 0.5 degree wide."@en ;
    skos:inScheme cs: ;
    skos:notation "7566" ;
    skos:prefLabel "Strathleven:7566"@en ;
.

geoad:Strathmay7468
    a skos:Concept ;
    skos:historyNote "Compiled by the Geological Survey of Queensland" ;
    skos:broader geoad:MapSeries ;
    skos:definition "Map sheet for Strathmay at 1:100 000 scale. The first two digits define a longitude band 0.5 degree wide and the second two digits a latitude band 0.5 degree wide."@en ;
    skos:inScheme cs: ;
    skos:notation "7468" ;
    skos:prefLabel "Strathmay:7468"@en ;
.

geoad:Strathmore7462
    a skos:Concept ;
    skos:historyNote "Compiled by the Geological Survey of Queensland" ;
    skos:broader geoad:MapSeries ;
    skos:definition "Map sheet for Strathmore at 1:100 000 scale. The first two digits define a longitude band 0.5 degree wide and the second two digits a latitude band 0.5 degree wide."@en ;
    skos:inScheme cs: ;
    skos:notation "7462" ;
    skos:prefLabel "Strathmore:7462"@en ;
.

geoad:Struan8543
    a skos:Concept ;
    skos:historyNote "Compiled by the Geological Survey of Queensland" ;
    skos:broader geoad:MapSeries ;
    skos:definition "Map sheet for Struan at 1:100 000 scale. The first two digits define a longitude band 0.5 degree wide and the second two digits a latitude band 0.5 degree wide."@en ;
    skos:inScheme cs: ;
    skos:notation "8543" ;
    skos:prefLabel "Struan:8543"@en ;
.

geoad:Surat8743
    a skos:Concept ;
    skos:historyNote "Compiled by the Geological Survey of Queensland" ;
    skos:broader geoad:MapSeries ;
    skos:definition "Map sheet for Surat at 1:100 000 scale. The first two digits define a longitude band 0.5 degree wide and the second two digits a latitude band 0.5 degree wide."@en ;
    skos:inScheme cs: ;
    skos:notation "8743" ;
    skos:prefLabel "Surat:8743"@en ;
.

geoad:Surbiton8251
    a skos:Concept ;
    skos:historyNote "Compiled by the Geological Survey of Queensland" ;
    skos:broader geoad:MapSeries ;
    skos:definition "Map sheet for Surbiton at 1:100 000 scale. The first two digits define a longitude band 0.5 degree wide and the second two digits a latitude band 0.5 degree wide."@en ;
    skos:inScheme cs: ;
    skos:notation "8251" ;
    skos:prefLabel "Surbiton:8251"@en ;
.

geoad:SweersIsland6863
    a skos:Concept ;
    skos:historyNote "Compiled by the Geological Survey of Queensland" ;
    skos:broader geoad:MapSeries ;
    skos:definition "Map sheet for Sweers Island at 1:100 000 scale. The first two digits define a longitude band 0.5 degree wide and the second two digits a latitude band 0.5 degree wide."@en ;
    skos:inScheme cs: ;
    skos:notation "6863" ;
    skos:prefLabel "Sweers Island:6863"@en ;
.

geoad:Talawanta6960
    a skos:Concept ;
    skos:historyNote "Compiled by the Geological Survey of Queensland" ;
    skos:broader geoad:MapSeries ;
    skos:definition "Map sheet for Talawanta at 1:100 000 scale. The first two digits define a longitude band 0.5 degree wide and the second two digits a latitude band 0.5 degree wide."@en ;
    skos:inScheme cs: ;
    skos:notation "6960" ;
    skos:prefLabel "Talawanta:6960"@en ;
.

geoad:Taldora7159
    a skos:Concept ;
    skos:historyNote "Compiled by the Geological Survey of Queensland" ;
    skos:broader geoad:MapSeries ;
    skos:definition "Map sheet for Taldora at 1:100 000 scale. The first two digits define a longitude band 0.5 degree wide and the second two digits a latitude band 0.5 degree wide."@en ;
    skos:inScheme cs: ;
    skos:notation "7159" ;
    skos:prefLabel "Taldora:7159"@en ;
.

geoad:Talleranie6743
    a skos:Concept ;
    skos:historyNote "Compiled by the Geological Survey of Queensland" ;
    skos:broader geoad:MapSeries ;
    skos:definition "Map sheet for Talleranie at 1:100 000 scale. The first two digits define a longitude band 0.5 degree wide and the second two digits a latitude band 0.5 degree wide."@en ;
    skos:inScheme cs: ;
    skos:notation "6743" ;
    skos:prefLabel "Talleranie:6743"@en ;
.

geoad:Talwood8741
    a skos:Concept ;
    skos:historyNote "Compiled by the Geological Survey of Queensland" ;
    skos:broader geoad:MapSeries ;
    skos:definition "Map sheet for Talwood at 1:100 000 scale. The first two digits define a longitude band 0.5 degree wide and the second two digits a latitude band 0.5 degree wide."@en ;
    skos:inScheme cs: ;
    skos:notation "8741" ;
    skos:prefLabel "Talwood:8741"@en ;
.

geoad:Talyealye7739
    a skos:Concept ;
    skos:historyNote "Compiled by the Geological Survey of Queensland" ;
    skos:broader geoad:MapSeries ;
    skos:definition "Map sheet for Talyealye at 1:100 000 scale. The first two digits define a longitude band 0.5 degree wide and the second two digits a latitude band 0.5 degree wide."@en ;
    skos:inScheme cs: ;
    skos:notation "7739" ;
    skos:prefLabel "Talyealye:7739"@en ;
.

geoad:Tambo8148
    a skos:Concept ;
    skos:historyNote "Compiled by the Geological Survey of Queensland" ;
    skos:broader geoad:MapSeries ;
    skos:definition "Map sheet for Tambo at 1:100 000 scale. The first two digits define a longitude band 0.5 degree wide and the second two digits a latitude band 0.5 degree wide."@en ;
    skos:inScheme cs: ;
    skos:notation "8148" ;
    skos:prefLabel "Tambo:8148"@en ;
.

geoad:Tanbar7246
    a skos:Concept ;
    skos:historyNote "Compiled by the Geological Survey of Queensland" ;
    skos:broader geoad:MapSeries ;
    skos:definition "Map sheet for Tanbar at 1:100 000 scale. The first two digits define a longitude band 0.5 degree wide and the second two digits a latitude band 0.5 degree wide."@en ;
    skos:inScheme cs: ;
    skos:notation "7246" ;
    skos:prefLabel "Tanbar:7246"@en ;
.

geoad:Tangorin7754
    a skos:Concept ;
    skos:historyNote "Compiled by the Geological Survey of Queensland" ;
    skos:broader geoad:MapSeries ;
    skos:definition "Map sheet for Tangorin at 1:100 000 scale. The first two digits define a longitude band 0.5 degree wide and the second two digits a latitude band 0.5 degree wide."@en ;
    skos:inScheme cs: ;
    skos:notation "7754" ;
    skos:prefLabel "Tangorin:7754"@en ;
.

geoad:Tara8943
    a skos:Concept ;
    skos:historyNote "Compiled by the Geological Survey of Queensland" ;
    skos:broader geoad:MapSeries ;
    skos:definition "Map sheet for Tara at 1:100 000 scale. The first two digits define a longitude band 0.5 degree wide and the second two digits a latitude band 0.5 degree wide."@en ;
    skos:inScheme cs: ;
    skos:notation "8943" ;
    skos:prefLabel "Tara:8943"@en ;
.

geoad:Taroom8846
    a skos:Concept ;
    skos:historyNote "Compiled by the Geological Survey of Queensland" ;
    skos:broader geoad:MapSeries ;
    skos:definition "Map sheet for Taroom at 1:100 000 scale. The first two digits define a longitude band 0.5 degree wide and the second two digits a latitude band 0.5 degree wide."@en ;
    skos:inScheme cs: ;
    skos:notation "8846" ;
    skos:prefLabel "Taroom:8846"@en ;
.

geoad:TempleBay7573
    a skos:Concept ;
    skos:historyNote "Compiled by the Geological Survey of Queensland" ;
    skos:broader geoad:MapSeries ;
    skos:definition "Map sheet for Temple Bay at 1:100 000 scale. The first two digits define a longitude band 0.5 degree wide and the second two digits a latitude band 0.5 degree wide."@en ;
    skos:inScheme cs: ;
    skos:notation "7573" ;
    skos:prefLabel "Temple Bay:7573"@en ;
.

geoad:Templeton6656
    a skos:Concept ;
    skos:historyNote "Compiled by the Geological Survey of Queensland" ;
    skos:broader geoad:MapSeries ;
    skos:definition "Map sheet for Templeton at 1:100 000 scale. The first two digits define a longitude band 0.5 degree wide and the second two digits a latitude band 0.5 degree wide."@en ;
    skos:inScheme cs: ;
    skos:notation "6656" ;
    skos:prefLabel "Templeton:6656"@en ;
.

geoad:Tenterfield9339
    a skos:Concept ;
    skos:historyNote "Compiled by the Geological Survey of Queensland" ;
    skos:broader geoad:MapSeries ;
    skos:definition "Map sheet for Tenterfield at 1:100 000 scale. The first two digits define a longitude band 0.5 degree wide and the second two digits a latitude band 0.5 degree wide."@en ;
    skos:inScheme cs: ;
    skos:notation "9339" ;
    skos:prefLabel "Tenterfield:9339"@en ;
.

geoad:Teriwa6649
    a skos:Concept ;
    skos:historyNote "Compiled by the Geological Survey of Queensland" ;
    skos:broader geoad:MapSeries ;
    skos:definition "Map sheet for Teriwa at 1:100 000 scale. The first two digits define a longitude band 0.5 degree wide and the second two digits a latitude band 0.5 degree wide."@en ;
    skos:inScheme cs: ;
    skos:notation "6649" ;
    skos:prefLabel "Teriwa:6649"@en ;
.

geoad:TerrickTerrick7948
    a skos:Concept ;
    skos:historyNote "Compiled by the Geological Survey of Queensland" ;
    skos:broader geoad:MapSeries ;
    skos:definition "Map sheet for Terrick Terrick at 1:100 000 scale. The first two digits define a longitude band 0.5 degree wide and the second two digits a latitude band 0.5 degree wide."@en ;
    skos:inScheme cs: ;
    skos:notation "7948" ;
    skos:prefLabel "Terrick Terrick:7948"@en ;
.

geoad:Texas9140
    a skos:Concept ;
    skos:historyNote "Compiled by the Geological Survey of Queensland" ;
    skos:broader geoad:MapSeries ;
    skos:definition "Map sheet for Texas at 1:100 000 scale. The first two digits define a longitude band 0.5 degree wide and the second two digits a latitude band 0.5 degree wide."@en ;
    skos:inScheme cs: ;
    skos:notation "9140" ;
    skos:prefLabel "Texas:9140"@en ;
.

geoad:Thallon8640
    a skos:Concept ;
    skos:historyNote "Compiled by the Geological Survey of Queensland" ;
    skos:broader geoad:MapSeries ;
    skos:definition "Map sheet for Thallon at 1:100 000 scale. The first two digits define a longitude band 0.5 degree wide and the second two digits a latitude band 0.5 degree wide."@en ;
    skos:inScheme cs: ;
    skos:notation "8640" ;
    skos:prefLabel "Thallon:8640"@en ;
.

geoad:Thargomindah7642
    a skos:Concept ;
    skos:historyNote "Compiled by the Geological Survey of Queensland" ;
    skos:broader geoad:MapSeries ;
    skos:definition "Map sheet for Thargomindah at 1:100 000 scale. The first two digits define a longitude band 0.5 degree wide and the second two digits a latitude band 0.5 degree wide."@en ;
    skos:inScheme cs: ;
    skos:notation "7642" ;
    skos:prefLabel "Thargomindah:7642"@en ;
.

geoad:Theodore8948
    a skos:Concept ;
    skos:historyNote "Compiled by the Geological Survey of Queensland" ;
    skos:broader geoad:MapSeries ;
    skos:definition "Map sheet for Theodore at 1:100 000 scale. The first two digits define a longitude band 0.5 degree wide and the second two digits a latitude band 0.5 degree wide."@en ;
    skos:inScheme cs: ;
    skos:notation "8948" ;
    skos:prefLabel "Theodore:8948"@en ;
.

geoad:Thuringowa7541
    a skos:Concept ;
    skos:historyNote "Compiled by the Geological Survey of Queensland" ;
    skos:broader geoad:MapSeries ;
    skos:definition "Map sheet for Thuringowa at 1:100 000 scale. The first two digits define a longitude band 0.5 degree wide and the second two digits a latitude band 0.5 degree wide."@en ;
    skos:inScheme cs: ;
    skos:notation "7541" ;
    skos:prefLabel "Thuringowa:7541"@en ;
.

geoad:ThurlooDowns7539
    a skos:Concept ;
    skos:historyNote "Compiled by the Geological Survey of Queensland" ;
    skos:broader geoad:MapSeries ;
    skos:definition "Map sheet for Thurloo Downs at 1:100 000 scale. The first two digits define a longitude band 0.5 degree wide and the second two digits a latitude band 0.5 degree wide."@en ;
    skos:inScheme cs: ;
    skos:notation "7539" ;
    skos:prefLabel "Thurloo Downs:7539"@en ;
.

geoad:ThursdayIsland7376
    a skos:Concept ;
    skos:historyNote "Compiled by the Geological Survey of Queensland" ;
    skos:broader geoad:MapSeries ;
    skos:definition "Map sheet for Thursday Island at 1:100 000 scale. The first two digits define a longitude band 0.5 degree wide and the second two digits a latitude band 0.5 degree wide."@en ;
    skos:inScheme cs: ;
    skos:notation "7376" ;
    skos:prefLabel "Thursday Island:7376"@en ;
.

geoad:Thylungra7545
    a skos:Concept ;
    skos:historyNote "Compiled by the Geological Survey of Queensland" ;
    skos:broader geoad:MapSeries ;
    skos:definition "Map sheet for Thylungra at 1:100 000 scale. The first two digits define a longitude band 0.5 degree wide and the second two digits a latitude band 0.5 degree wide."@en ;
    skos:inScheme cs: ;
    skos:notation "7545" ;
    skos:prefLabel "Thylungra:7545"@en ;
.

geoad:Tibooburra7339
    a skos:Concept ;
    skos:historyNote "Compiled by the Geological Survey of Queensland" ;
    skos:broader geoad:MapSeries ;
    skos:definition "Map sheet for Tibooburra at 1:100 000 scale. The first two digits define a longitude band 0.5 degree wide and the second two digits a latitude band 0.5 degree wide."@en ;
    skos:inScheme cs: ;
    skos:notation "7339" ;
    skos:prefLabel "Tibooburra:7339"@en ;
.

geoad:Tickalara7340
    a skos:Concept ;
    skos:historyNote "Compiled by the Geological Survey of Queensland" ;
    skos:broader geoad:MapSeries ;
    skos:definition "Map sheet for Tickalara at 1:100 000 scale. The first two digits define a longitude band 0.5 degree wide and the second two digits a latitude band 0.5 degree wide."@en ;
    skos:inScheme cs: ;
    skos:notation "7340" ;
    skos:prefLabel "Tickalara:7340"@en ;
.

geoad:TingaTingana6940
    a skos:Concept ;
    skos:historyNote "Compiled by the Geological Survey of Queensland" ;
    skos:broader geoad:MapSeries ;
    skos:definition "Map sheet for Tinga Tingana at 1:100 000 scale. The first two digits define a longitude band 0.5 degree wide and the second two digits a latitude band 0.5 degree wide."@en ;
    skos:inScheme cs: ;
    skos:notation "6940" ;
    skos:prefLabel "Tinga Tingana:6940"@en ;
.

geoad:TitherooCreek7540
    a skos:Concept ;
    skos:historyNote "Compiled by the Geological Survey of Queensland" ;
    skos:broader geoad:MapSeries ;
    skos:definition "Map sheet for Titheroo Creek at 1:100 000 scale. The first two digits define a longitude band 0.5 degree wide and the second two digits a latitude band 0.5 degree wide."@en ;
    skos:inScheme cs: ;
    skos:notation "7540" ;
    skos:prefLabel "Titheroo Creek:7540"@en ;
.

geoad:Tongowoko7439
    a skos:Concept ;
    skos:historyNote "Compiled by the Geological Survey of Queensland" ;
    skos:broader geoad:MapSeries ;
    skos:definition "Map sheet for Tongowoko at 1:100 000 scale. The first two digits define a longitude band 0.5 degree wide and the second two digits a latitude band 0.5 degree wide."@en ;
    skos:inScheme cs: ;
    skos:notation "7439" ;
    skos:prefLabel "Tongowoko:7439"@en ;
.

geoad:Tongy8343
    a skos:Concept ;
    skos:historyNote "Compiled by the Geological Survey of Queensland" ;
    skos:broader geoad:MapSeries ;
    skos:definition "Map sheet for Tongy at 1:100 000 scale. The first two digits define a longitude band 0.5 degree wide and the second two digits a latitude band 0.5 degree wide."@en ;
    skos:inScheme cs: ;
    skos:notation "8343" ;
    skos:prefLabel "Tongy:8343"@en ;
.

geoad:Tonkoro7350
    a skos:Concept ;
    skos:historyNote "Compiled by the Geological Survey of Queensland" ;
    skos:broader geoad:MapSeries ;
    skos:definition "Map sheet for Tonkoro at 1:100 000 scale. The first two digits define a longitude band 0.5 degree wide and the second two digits a latitude band 0.5 degree wide."@en ;
    skos:inScheme cs: ;
    skos:notation "7350" ;
    skos:prefLabel "Tonkoro:7350"@en ;
.

geoad:Toolebuc7053
    a skos:Concept ;
    skos:historyNote "Compiled by the Geological Survey of Queensland" ;
    skos:broader geoad:MapSeries ;
    skos:definition "Map sheet for Toolebuc at 1:100 000 scale. The first two digits define a longitude band 0.5 degree wide and the second two digits a latitude band 0.5 degree wide."@en ;
    skos:inScheme cs: ;
    skos:notation "7053" ;
    skos:prefLabel "Toolebuc:7053"@en ;
.

geoad:Toompine7743
    a skos:Concept ;
    skos:historyNote "Compiled by the Geological Survey of Queensland" ;
    skos:broader geoad:MapSeries ;
    skos:definition "Map sheet for Toompine at 1:100 000 scale. The first two digits define a longitude band 0.5 degree wide and the second two digits a latitude band 0.5 degree wide."@en ;
    skos:inScheme cs: ;
    skos:notation "7743" ;
    skos:prefLabel "Toompine:7743"@en ;
.

geoad:Tooncatchyin6739
    a skos:Concept ;
    skos:historyNote "Compiled by the Geological Survey of Queensland" ;
    skos:broader geoad:MapSeries ;
    skos:definition "Map sheet for Tooncatchyin at 1:100 000 scale. The first two digits define a longitude band 0.5 degree wide and the second two digits a latitude band 0.5 degree wide."@en ;
    skos:inScheme cs: ;
    skos:notation "6739" ;
    skos:prefLabel "Tooncatchyin:6739"@en ;
.

geoad:Toowoomba9242
    a skos:Concept ;
    skos:historyNote "Compiled by the Geological Survey of Queensland" ;
    skos:broader geoad:MapSeries ;
    skos:definition "Map sheet for Toowoomba at 1:100 000 scale. The first two digits define a longitude band 0.5 degree wide and the second two digits a latitude band 0.5 degree wide."@en ;
    skos:inScheme cs: ;
    skos:notation "9242" ;
    skos:prefLabel "Toowoomba:9242"@en ;
.

geoad:Townsville8259
    a skos:Concept ;
    skos:historyNote "Compiled by the Geological Survey of Queensland" ;
    skos:broader geoad:MapSeries ;
    skos:definition "Map sheet for Townsville at 1:100 000 scale. The first two digits define a longitude band 0.5 degree wide and the second two digits a latitude band 0.5 degree wide."@en ;
    skos:inScheme cs: ;
    skos:notation "8259" ;
    skos:prefLabel "Townsville:8259"@en ;
.

geoad:Trenton7359
    a skos:Concept ;
    skos:historyNote "Compiled by the Geological Survey of Queensland" ;
    skos:broader geoad:MapSeries ;
    skos:definition "Map sheet for Trenton at 1:100 000 scale. The first two digits define a longitude band 0.5 degree wide and the second two digits a latitude band 0.5 degree wide."@en ;
    skos:inScheme cs: ;
    skos:notation "7359" ;
    skos:prefLabel "Trenton:7359"@en ;
.

geoad:Trewalla7448
    a skos:Concept ;
    skos:historyNote "Compiled by the Geological Survey of Queensland" ;
    skos:broader geoad:MapSeries ;
    skos:definition "Map sheet for Trewalla at 1:100 000 scale. The first two digits define a longitude band 0.5 degree wide and the second two digits a latitude band 0.5 degree wide."@en ;
    skos:inScheme cs: ;
    skos:notation "7448" ;
    skos:prefLabel "Trewalla:7448"@en ;
.

geoad:TroopersBluff8249
    a skos:Concept ;
    skos:historyNote "Compiled by the Geological Survey of Queensland" ;
    skos:broader geoad:MapSeries ;
    skos:definition "Map sheet for Troopers Bluff at 1:100 000 scale. The first two digits define a longitude band 0.5 degree wide and the second two digits a latitude band 0.5 degree wide."@en ;
    skos:inScheme cs: ;
    skos:notation "8249" ;
    skos:prefLabel "Troopers Bluff:8249"@en ;
.

geoad:Tualta7140
    a skos:Concept ;
    skos:historyNote "Compiled by the Geological Survey of Queensland" ;
    skos:broader geoad:MapSeries ;
    skos:definition "Map sheet for Tualta at 1:100 000 scale. The first two digits define a longitude band 0.5 degree wide and the second two digits a latitude band 0.5 degree wide."@en ;
    skos:inScheme cs: ;
    skos:notation "7140" ;
    skos:prefLabel "Tualta:7140"@en ;
.

geoad:Tuen8040
    a skos:Concept ;
    skos:historyNote "Compiled by the Geological Survey of Queensland" ;
    skos:broader geoad:MapSeries ;
    skos:definition "Map sheet for Tuen at 1:100 000 scale. The first two digits define a longitude band 0.5 degree wide and the second two digits a latitude band 0.5 degree wide."@en ;
    skos:inScheme cs: ;
    skos:notation "8040" ;
    skos:prefLabel "Tuen:8040"@en ;
.

geoad:Tully8062
    a skos:Concept ;
    skos:historyNote "Compiled by the Geological Survey of Queensland" ;
    skos:broader geoad:MapSeries ;
    skos:definition "Map sheet for Tully at 1:100 000 scale. The first two digits define a longitude band 0.5 degree wide and the second two digits a latitude band 0.5 degree wide."@en ;
    skos:inScheme cs: ;
    skos:notation "8062" ;
    skos:prefLabel "Tully:8062"@en ;
.

geoad:Tulmur7352
    a skos:Concept ;
    skos:historyNote "Compiled by the Geological Survey of Queensland" ;
    skos:broader geoad:MapSeries ;
    skos:definition "Map sheet for Tulmur at 1:100 000 scale. The first two digits define a longitude band 0.5 degree wide and the second two digits a latitude band 0.5 degree wide."@en ;
    skos:inScheme cs: ;
    skos:notation "7352" ;
    skos:prefLabel "Tulmur:7352"@en ;
.

geoad:TuruCay7178
    a skos:Concept ;
    skos:historyNote "Compiled by the Geological Survey of Queensland" ;
    skos:broader geoad:MapSeries ;
    skos:definition "Map sheet for Turu Cay at 1:100 000 scale. The first two digits define a longitude band 0.5 degree wide and the second two digits a latitude band 0.5 degree wide."@en ;
    skos:inScheme cs: ;
    skos:notation "7178" ;
    skos:prefLabel "Turu Cay:7178"@en ;
.

geoad:TweedHeads9641
    a skos:Concept ;
    skos:historyNote "Compiled by the Geological Survey of Queensland" ;
    skos:broader geoad:MapSeries ;
    skos:definition "Map sheet for Tweed Heads at 1:100 000 scale. The first two digits define a longitude band 0.5 degree wide and the second two digits a latitude band 0.5 degree wide."@en ;
    skos:inScheme cs: ;
    skos:notation "9641" ;
    skos:prefLabel "Tweed Heads:9641"@en ;
.

geoad:Ularunda8344
    a skos:Concept ;
    skos:historyNote "Compiled by the Geological Survey of Queensland" ;
    skos:broader geoad:MapSeries ;
    skos:definition "Map sheet for Ularunda at 1:100 000 scale. The first two digits define a longitude band 0.5 degree wide and the second two digits a latitude band 0.5 degree wide."@en ;
    skos:inScheme cs: ;
    skos:notation "8344" ;
    skos:prefLabel "Ularunda:8344"@en ;
.

geoad:Undilla6658
    a skos:Concept ;
    skos:historyNote "Compiled by the Geological Survey of Queensland" ;
    skos:broader geoad:MapSeries ;
    skos:definition "Map sheet for Undilla at 1:100 000 scale. The first two digits define a longitude band 0.5 degree wide and the second two digits a latitude band 0.5 degree wide."@en ;
    skos:inScheme cs: ;
    skos:notation "6658" ;
    skos:prefLabel "Undilla:6658"@en ;
.

geoad:Urandangi6554
    a skos:Concept ;
    skos:historyNote "Compiled by the Geological Survey of Queensland" ;
    skos:broader geoad:MapSeries ;
    skos:definition "Map sheet for Urandangi at 1:100 000 scale. The first two digits define a longitude band 0.5 degree wide and the second two digits a latitude band 0.5 degree wide."@en ;
    skos:inScheme cs: ;
    skos:notation "6554" ;
    skos:prefLabel "Urandangi:6554"@en ;
.

geoad:Urannah8556
    a skos:Concept ;
    skos:historyNote "Compiled by the Geological Survey of Queensland" ;
    skos:broader geoad:MapSeries ;
    skos:definition "Map sheet for Urannah at 1:100 000 scale. The first two digits define a longitude band 0.5 degree wide and the second two digits a latitude band 0.5 degree wide."@en ;
    skos:inScheme cs: ;
    skos:notation "8556" ;
    skos:prefLabel "Urannah:8556"@en ;
.

geoad:ValleyOfLagoons7960
    a skos:Concept ;
    skos:historyNote "Compiled by the Geological Survey of Queensland" ;
    skos:broader geoad:MapSeries ;
    skos:definition "Map sheet for Valley Of Lagoons at 1:100 000 scale. The first two digits define a longitude band 0.5 degree wide and the second two digits a latitude band 0.5 degree wide."@en ;
    skos:inScheme cs: ;
    skos:notation "7960" ;
    skos:prefLabel "Valley Of Lagoons:7960"@en ;
.

geoad:Vandyke8448
    a skos:Concept ;
    skos:historyNote "Compiled by the Geological Survey of Queensland" ;
    skos:broader geoad:MapSeries ;
    skos:definition "Map sheet for Vandyke at 1:100 000 scale. The first two digits define a longitude band 0.5 degree wide and the second two digits a latitude band 0.5 degree wide."@en ;
    skos:inScheme cs: ;
    skos:notation "8448" ;
    skos:prefLabel "Vandyke:8448"@en ;
.

geoad:Vanrook7264
    a skos:Concept ;
    skos:historyNote "Compiled by the Geological Survey of Queensland" ;
    skos:broader geoad:MapSeries ;
    skos:definition "Map sheet for Vanrook at 1:100 000 scale. The first two digits define a longitude band 0.5 degree wide and the second two digits a latitude band 0.5 degree wide."@en ;
    skos:inScheme cs: ;
    skos:notation "7264" ;
    skos:prefLabel "Vanrook:7264"@en ;
.

geoad:Vergemont7550
    a skos:Concept ;
    skos:historyNote "Compiled by the Geological Survey of Queensland" ;
    skos:broader geoad:MapSeries ;
    skos:definition "Map sheet for Vergemont at 1:100 000 scale. The first two digits define a longitude band 0.5 degree wide and the second two digits a latitude band 0.5 degree wide."@en ;
    skos:inScheme cs: ;
    skos:notation "7550" ;
    skos:prefLabel "Vergemont:7550"@en ;
.

geoad:Vindex7552
    a skos:Concept ;
    skos:historyNote "Compiled by the Geological Survey of Queensland" ;
    skos:broader geoad:MapSeries ;
    skos:definition "Map sheet for Vindex at 1:100 000 scale. The first two digits define a longitude band 0.5 degree wide and the second two digits a latitude band 0.5 degree wide."@en ;
    skos:inScheme cs: ;
    skos:notation "7552" ;
    skos:prefLabel "Vindex:7552"@en ;
.

geoad:VrilyaPoint7375
    a skos:Concept ;
    skos:historyNote "Compiled by the Geological Survey of Queensland" ;
    skos:broader geoad:MapSeries ;
    skos:definition "Map sheet for Vrilya Point at 1:100 000 scale. The first two digits define a longitude band 0.5 degree wide and the second two digits a latitude band 0.5 degree wide."@en ;
    skos:inScheme cs: ;
    skos:notation "7375" ;
    skos:prefLabel "Vrilya Point:7375"@en ;
.

geoad:WaarWaar9042
    a skos:Concept ;
    skos:historyNote "Compiled by the Geological Survey of Queensland" ;
    skos:broader geoad:MapSeries ;
    skos:definition "Map sheet for Waar Waar at 1:100 000 scale. The first two digits define a longitude band 0.5 degree wide and the second two digits a latitude band 0.5 degree wide."@en ;
    skos:inScheme cs: ;
    skos:notation "9042" ;
    skos:prefLabel "Waar Waar:9042"@en ;
.

geoad:WaddyPoint9548
    a skos:Concept ;
    skos:historyNote "Compiled by the Geological Survey of Queensland" ;
    skos:broader geoad:MapSeries ;
    skos:definition "Map sheet for Waddy Point at 1:100 000 scale. The first two digits define a longitude band 0.5 degree wide and the second two digits a latitude band 0.5 degree wide."@en ;
    skos:inScheme cs: ;
    skos:notation "9548" ;
    skos:prefLabel "Waddy Point:9548"@en ;
.

geoad:Wallabadah7362
    a skos:Concept ;
    skos:historyNote "Compiled by the Geological Survey of Queensland" ;
    skos:broader geoad:MapSeries ;
    skos:definition "Map sheet for Wallabadah at 1:100 000 scale. The first two digits define a longitude band 0.5 degree wide and the second two digits a latitude band 0.5 degree wide."@en ;
    skos:inScheme cs: ;
    skos:notation "7362" ;
    skos:prefLabel "Wallabadah:7362"@en ;
.

geoad:Walsh7664
    a skos:Concept ;
    skos:historyNote "Compiled by the Geological Survey of Queensland" ;
    skos:broader geoad:MapSeries ;
    skos:definition "Map sheet for Walsh at 1:100 000 scale. The first two digits define a longitude band 0.5 degree wide and the second two digits a latitude band 0.5 degree wide."@en ;
    skos:inScheme cs: ;
    skos:notation "7664" ;
    skos:prefLabel "Walsh:7664"@en ;
.

geoad:WandoVale7858
    a skos:Concept ;
    skos:historyNote "Compiled by the Geological Survey of Queensland" ;
    skos:broader geoad:MapSeries ;
    skos:definition "Map sheet for Wando Vale at 1:100 000 scale. The first two digits define a longitude band 0.5 degree wide and the second two digits a latitude band 0.5 degree wide."@en ;
    skos:inScheme cs: ;
    skos:notation "7858" ;
    skos:prefLabel "Wando Vale:7858"@en ;
.

geoad:Wandoan8845
    a skos:Concept ;
    skos:historyNote "Compiled by the Geological Survey of Queensland" ;
    skos:broader geoad:MapSeries ;
    skos:definition "Map sheet for Wandoan at 1:100 000 scale. The first two digits define a longitude band 0.5 degree wide and the second two digits a latitude band 0.5 degree wide."@en ;
    skos:inScheme cs: ;
    skos:notation "8845" ;
    skos:prefLabel "Wandoan:8845"@en ;
.

geoad:Wantata6947
    a skos:Concept ;
    skos:historyNote "Compiled by the Geological Survey of Queensland" ;
    skos:broader geoad:MapSeries ;
    skos:definition "Map sheet for Wantata at 1:100 000 scale. The first two digits define a longitude band 0.5 degree wide and the second two digits a latitude band 0.5 degree wide."@en ;
    skos:inScheme cs: ;
    skos:notation "6947" ;
    skos:prefLabel "Wantata:6947"@en ;
.

geoad:Warbreccan7449
    a skos:Concept ;
    skos:historyNote "Compiled by the Geological Survey of Queensland" ;
    skos:broader geoad:MapSeries ;
    skos:definition "Map sheet for Warbreccan at 1:100 000 scale. The first two digits define a longitude band 0.5 degree wide and the second two digits a latitude band 0.5 degree wide."@en ;
    skos:inScheme cs: ;
    skos:notation "7449" ;
    skos:prefLabel "Warbreccan:7449"@en ;
.

geoad:Warnambool7452
    a skos:Concept ;
    skos:historyNote "Compiled by the Geological Survey of Queensland" ;
    skos:broader geoad:MapSeries ;
    skos:definition "Map sheet for Warnambool at 1:100 000 scale. The first two digits define a longitude band 0.5 degree wide and the second two digits a latitude band 0.5 degree wide."@en ;
    skos:inScheme cs: ;
    skos:notation "7452" ;
    skos:prefLabel "Warnambool:7452"@en ;
.

geoad:Waroonga8545
    a skos:Concept ;
    skos:historyNote "Compiled by the Geological Survey of Queensland" ;
    skos:broader geoad:MapSeries ;
    skos:definition "Map sheet for Waroonga at 1:100 000 scale. The first two digits define a longitude band 0.5 degree wide and the second two digits a latitude band 0.5 degree wide."@en ;
    skos:inScheme cs: ;
    skos:notation "8545" ;
    skos:prefLabel "Waroonga:8545"@en ;
.

geoad:Warrinilla8648
    a skos:Concept ;
    skos:historyNote "Compiled by the Geological Survey of Queensland" ;
    skos:broader geoad:MapSeries ;
    skos:definition "Map sheet for Warrinilla at 1:100 000 scale. The first two digits define a longitude band 0.5 degree wide and the second two digits a latitude band 0.5 degree wide."@en ;
    skos:inScheme cs: ;
    skos:notation "8648" ;
    skos:prefLabel "Warrinilla:8648"@en ;
.

geoad:Warrong8447
    a skos:Concept ;
    skos:historyNote "Compiled by the Geological Survey of Queensland" ;
    skos:broader geoad:MapSeries ;
    skos:definition "Map sheet for Warrong at 1:100 000 scale. The first two digits define a longitude band 0.5 degree wide and the second two digits a latitude band 0.5 degree wide."@en ;
    skos:inScheme cs: ;
    skos:notation "8447" ;
    skos:prefLabel "Warrong:8447"@en ;
.

geoad:Warwick9341
    a skos:Concept ;
    skos:historyNote "Compiled by the Geological Survey of Queensland" ;
    skos:broader geoad:MapSeries ;
    skos:definition "Map sheet for Warwick at 1:100 000 scale. The first two digits define a longitude band 0.5 degree wide and the second two digits a latitude band 0.5 degree wide."@en ;
    skos:inScheme cs: ;
    skos:notation "9341" ;
    skos:prefLabel "Warwick:9341"@en ;
.

geoad:WebbLake7955
    a skos:Concept ;
    skos:historyNote "Compiled by the Geological Survey of Queensland" ;
    skos:broader geoad:MapSeries ;
    skos:definition "Map sheet for Webb Lake at 1:100 000 scale. The first two digits define a longitude band 0.5 degree wide and the second two digits a latitude band 0.5 degree wide."@en ;
    skos:inScheme cs: ;
    skos:notation "7955" ;
    skos:prefLabel "Webb Lake:7955"@en ;
.

geoad:Weelamurra8141
    a skos:Concept ;
    skos:historyNote "Compiled by the Geological Survey of Queensland" ;
    skos:broader geoad:MapSeries ;
    skos:definition "Map sheet for Weelamurra at 1:100 000 scale. The first two digits define a longitude band 0.5 degree wide and the second two digits a latitude band 0.5 degree wide."@en ;
    skos:inScheme cs: ;
    skos:notation "8141" ;
    skos:prefLabel "Weelamurra:8141"@en ;
.

geoad:Weilmoringle8239
    a skos:Concept ;
    skos:historyNote "Compiled by the Geological Survey of Queensland" ;
    skos:broader geoad:MapSeries ;
    skos:definition "Map sheet for Weilmoringle at 1:100 000 scale. The first two digits define a longitude band 0.5 degree wide and the second two digits a latitude band 0.5 degree wide."@en ;
    skos:inScheme cs: ;
    skos:notation "8239" ;
    skos:prefLabel "Weilmoringle:8239"@en ;
.

geoad:Weipa7272
    a skos:Concept ;
    skos:historyNote "Compiled by the Geological Survey of Queensland" ;
    skos:broader geoad:MapSeries ;
    skos:definition "Map sheet for Weipa at 1:100 000 scale. The first two digits define a longitude band 0.5 degree wide and the second two digits a latitude band 0.5 degree wide."@en ;
    skos:inScheme cs: ;
    skos:notation "7272" ;
    skos:prefLabel "Weipa:7272"@en ;
.

geoad:Wellshot7750
    a skos:Concept ;
    skos:historyNote "Compiled by the Geological Survey of Queensland" ;
    skos:broader geoad:MapSeries ;
    skos:definition "Map sheet for Wellshot at 1:100 000 scale. The first two digits define a longitude band 0.5 degree wide and the second two digits a latitude band 0.5 degree wide."@en ;
    skos:inScheme cs: ;
    skos:notation "7750" ;
    skos:prefLabel "Wellshot:7750"@en ;
.

geoad:Wenlock7471
    a skos:Concept ;
    skos:historyNote "Compiled by the Geological Survey of Queensland" ;
    skos:broader geoad:MapSeries ;
    skos:definition "Map sheet for Wenlock at 1:100 000 scale. The first two digits define a longitude band 0.5 degree wide and the second two digits a latitude band 0.5 degree wide."@en ;
    skos:inScheme cs: ;
    skos:notation "7471" ;
    skos:prefLabel "Wenlock:7471"@en ;
.

geoad:WerieEla7742
    a skos:Concept ;
    skos:historyNote "Compiled by the Geological Survey of Queensland" ;
    skos:broader geoad:MapSeries ;
    skos:definition "Map sheet for Werie Ela at 1:100 000 scale. The first two digits define a longitude band 0.5 degree wide and the second two digits a latitude band 0.5 degree wide."@en ;
    skos:inScheme cs: ;
    skos:notation "7742" ;
    skos:prefLabel "Werie Ela:7742"@en ;
.

geoad:Wernadinga6861
    a skos:Concept ;
    skos:historyNote "Compiled by the Geological Survey of Queensland" ;
    skos:broader geoad:MapSeries ;
    skos:definition "Map sheet for Wernadinga at 1:100 000 scale. The first two digits define a longitude band 0.5 degree wide and the second two digits a latitude band 0.5 degree wide."@en ;
    skos:inScheme cs: ;
    skos:notation "6861" ;
    skos:prefLabel "Wernadinga:6861"@en ;
.

geoad:Westgate8144
    a skos:Concept ;
    skos:historyNote "Compiled by the Geological Survey of Queensland" ;
    skos:broader geoad:MapSeries ;
    skos:definition "Map sheet for Westgate at 1:100 000 scale. The first two digits define a longitude band 0.5 degree wide and the second two digits a latitude band 0.5 degree wide."@en ;
    skos:inScheme cs: ;
    skos:notation "8144" ;
    skos:prefLabel "Westgate:8144"@en ;
.

geoad:Westmoreland6563
    a skos:Concept ;
    skos:historyNote "Compiled by the Geological Survey of Queensland" ;
    skos:broader geoad:MapSeries ;
    skos:definition "Map sheet for Westmoreland at 1:100 000 scale. The first two digits define a longitude band 0.5 degree wide and the second two digits a latitude band 0.5 degree wide."@en ;
    skos:inScheme cs: ;
    skos:notation "6563" ;
    skos:prefLabel "Westmoreland:6563"@en ;
.

geoad:WhiteMountains7857
    a skos:Concept ;
    skos:historyNote "Compiled by the Geological Survey of Queensland" ;
    skos:broader geoad:MapSeries ;
    skos:definition "Map sheet for White Mountains at 1:100 000 scale. The first two digits define a longitude band 0.5 degree wide and the second two digits a latitude band 0.5 degree wide."@en ;
    skos:inScheme cs: ;
    skos:notation "7857" ;
    skos:prefLabel "White Mountains:7857"@en ;
.

geoad:Whitula7347
    a skos:Concept ;
    skos:historyNote "Compiled by the Geological Survey of Queensland" ;
    skos:broader geoad:MapSeries ;
    skos:definition "Map sheet for Whitula at 1:100 000 scale. The first two digits define a longitude band 0.5 degree wide and the second two digits a latitude band 0.5 degree wide."@en ;
    skos:inScheme cs: ;
    skos:notation "7347" ;
    skos:prefLabel "Whitula:7347"@en ;
.

geoad:Whyenbah8541
    a skos:Concept ;
    skos:historyNote "Compiled by the Geological Survey of Queensland" ;
    skos:broader geoad:MapSeries ;
    skos:definition "Map sheet for Whyenbah at 1:100 000 scale. The first two digits define a longitude band 0.5 degree wide and the second two digits a latitude band 0.5 degree wide."@en ;
    skos:inScheme cs: ;
    skos:notation "8541" ;
    skos:prefLabel "Whyenbah:8541"@en ;
.

geoad:WideBay9546
    a skos:Concept ;
    skos:historyNote "Compiled by the Geological Survey of Queensland" ;
    skos:broader geoad:MapSeries ;
    skos:definition "Map sheet for Wide Bay at 1:100 000 scale. The first two digits define a longitude band 0.5 degree wide and the second two digits a latitude band 0.5 degree wide."@en ;
    skos:inScheme cs: ;
    skos:notation "9546" ;
    skos:prefLabel "Wide Bay:9546"@en ;
.

geoad:Wierbolla8442
    a skos:Concept ;
    skos:historyNote "Compiled by the Geological Survey of Queensland" ;
    skos:broader geoad:MapSeries ;
    skos:definition "Map sheet for Wierbolla at 1:100 000 scale. The first two digits define a longitude band 0.5 degree wide and the second two digits a latitude band 0.5 degree wide."@en ;
    skos:inScheme cs: ;
    skos:notation "8442" ;
    skos:prefLabel "Wierbolla:8442"@en ;
.

geoad:Winbin7844
    a skos:Concept ;
    skos:historyNote "Compiled by the Geological Survey of Queensland" ;
    skos:broader geoad:MapSeries ;
    skos:definition "Map sheet for Winbin at 1:100 000 scale. The first two digits define a longitude band 0.5 degree wide and the second two digits a latitude band 0.5 degree wide."@en ;
    skos:inScheme cs: ;
    skos:notation "7844" ;
    skos:prefLabel "Winbin:7844"@en ;
.

geoad:WindeyersHill8652
    a skos:Concept ;
    skos:historyNote "Compiled by the Geological Survey of Queensland" ;
    skos:broader geoad:MapSeries ;
    skos:definition "Map sheet for Windeyers Hill at 1:100 000 scale. The first two digits define a longitude band 0.5 degree wide and the second two digits a latitude band 0.5 degree wide."@en ;
    skos:inScheme cs: ;
    skos:notation "8652" ;
    skos:prefLabel "Windeyers Hill:8652"@en ;
.

geoad:Windorah7447
    a skos:Concept ;
    skos:historyNote "Compiled by the Geological Survey of Queensland" ;
    skos:broader geoad:MapSeries ;
    skos:definition "Map sheet for Windorah at 1:100 000 scale. The first two digits define a longitude band 0.5 degree wide and the second two digits a latitude band 0.5 degree wide."@en ;
    skos:inScheme cs: ;
    skos:notation "7447" ;
    skos:prefLabel "Windorah:7447"@en ;
.

geoad:Winton7553
    a skos:Concept ;
    skos:historyNote "Compiled by the Geological Survey of Queensland" ;
    skos:broader geoad:MapSeries ;
    skos:definition "Map sheet for Winton at 1:100 000 scale. The first two digits define a longitude band 0.5 degree wide and the second two digits a latitude band 0.5 degree wide."@en ;
    skos:inScheme cs: ;
    skos:notation "7553" ;
    skos:prefLabel "Winton:7553"@en ;
.

geoad:Wokingham7453
    a skos:Concept ;
    skos:historyNote "Compiled by the Geological Survey of Queensland" ;
    skos:broader geoad:MapSeries ;
    skos:definition "Map sheet for Wokingham at 1:100 000 scale. The first two digits define a longitude band 0.5 degree wide and the second two digits a latitude band 0.5 degree wide."@en ;
    skos:inScheme cs: ;
    skos:notation "7453" ;
    skos:prefLabel "Wokingham:7453"@en ;
.

geoad:Womblebank8546
    a skos:Concept ;
    skos:historyNote "Compiled by the Geological Survey of Queensland" ;
    skos:broader geoad:MapSeries ;
    skos:definition "Map sheet for Womblebank at 1:100 000 scale. The first two digits define a longitude band 0.5 degree wide and the second two digits a latitude band 0.5 degree wide."@en ;
    skos:inScheme cs: ;
    skos:notation "8546" ;
    skos:prefLabel "Womblebank:8546"@en ;
.

geoad:Woodburn9539
    a skos:Concept ;
    skos:historyNote "Compiled by the Geological Survey of Queensland" ;
    skos:broader geoad:MapSeries ;
    skos:definition "Map sheet for Woodburn at 1:100 000 scale. The first two digits define a longitude band 0.5 degree wide and the second two digits a latitude band 0.5 degree wide."@en ;
    skos:inScheme cs: ;
    skos:notation "9539" ;
    skos:prefLabel "Woodburn:9539"@en ;
.

geoad:Woomanooka7343
    a skos:Concept ;
    skos:historyNote "Compiled by the Geological Survey of Queensland" ;
    skos:broader geoad:MapSeries ;
    skos:definition "Map sheet for Woomanooka at 1:100 000 scale. The first two digits define a longitude band 0.5 degree wide and the second two digits a latitude band 0.5 degree wide."@en ;
    skos:inScheme cs: ;
    skos:notation "7343" ;
    skos:prefLabel "Woomanooka:7343"@en ;
.

geoad:Woorabinda8749
    a skos:Concept ;
    skos:historyNote "Compiled by the Geological Survey of Queensland" ;
    skos:broader geoad:MapSeries ;
    skos:definition "Map sheet for Woorabinda at 1:100 000 scale. The first two digits define a longitude band 0.5 degree wide and the second two digits a latitude band 0.5 degree wide."@en ;
    skos:inScheme cs: ;
    skos:notation "8749" ;
    skos:prefLabel "Woorabinda:8749"@en ;
.

geoad:Wooroona6557
    a skos:Concept ;
    skos:historyNote "Compiled by the Geological Survey of Queensland" ;
    skos:broader geoad:MapSeries ;
    skos:definition "Map sheet for Wooroona at 1:100 000 scale. The first two digits define a longitude band 0.5 degree wide and the second two digits a latitude band 0.5 degree wide."@en ;
    skos:inScheme cs: ;
    skos:notation "6557" ;
    skos:prefLabel "Wooroona:6557"@en ;
.

geoad:Wyaga9041
    a skos:Concept ;
    skos:historyNote "Compiled by the Geological Survey of Queensland" ;
    skos:broader geoad:MapSeries ;
    skos:definition "Map sheet for Wyaga at 1:100 000 scale. The first two digits define a longitude band 0.5 degree wide and the second two digits a latitude band 0.5 degree wide."@en ;
    skos:inScheme cs: ;
    skos:notation "9041" ;
    skos:prefLabel "Wyaga:9041"@en ;
.

geoad:Wyaldra7257
    a skos:Concept ;
    skos:historyNote "Compiled by the Geological Survey of Queensland" ;
    skos:broader geoad:MapSeries ;
    skos:definition "Map sheet for Wyaldra at 1:100 000 scale. The first two digits define a longitude band 0.5 degree wide and the second two digits a latitude band 0.5 degree wide."@en ;
    skos:inScheme cs: ;
    skos:notation "7257" ;
    skos:prefLabel "Wyaldra:7257"@en ;
.

geoad:Wyandra8043
    a skos:Concept ;
    skos:historyNote "Compiled by the Geological Survey of Queensland" ;
    skos:broader geoad:MapSeries ;
    skos:definition "Map sheet for Wyandra at 1:100 000 scale. The first two digits define a longitude band 0.5 degree wide and the second two digits a latitude band 0.5 degree wide."@en ;
    skos:inScheme cs: ;
    skos:notation "8043" ;
    skos:prefLabel "Wyandra:8043"@en ;
.

geoad:Wyena8454
    a skos:Concept ;
    skos:historyNote "Compiled by the Geological Survey of Queensland" ;
    skos:broader geoad:MapSeries ;
    skos:definition "Map sheet for Wyena at 1:100 000 scale. The first two digits define a longitude band 0.5 degree wide and the second two digits a latitude band 0.5 degree wide."@en ;
    skos:inScheme cs: ;
    skos:notation "8454" ;
    skos:prefLabel "Wyena:8454"@en ;
.

geoad:Yallaroi9039
    a skos:Concept ;
    skos:historyNote "Compiled by the Geological Survey of Queensland" ;
    skos:broader geoad:MapSeries ;
    skos:definition "Map sheet for Yallaroi at 1:100 000 scale. The first two digits define a longitude band 0.5 degree wide and the second two digits a latitude band 0.5 degree wide."@en ;
    skos:inScheme cs: ;
    skos:notation "9039" ;
    skos:prefLabel "Yallaroi:9039"@en ;
.

geoad:Yaluma6547
    a skos:Concept ;
    skos:historyNote "Compiled by the Geological Survey of Queensland" ;
    skos:broader geoad:MapSeries ;
    skos:definition "Map sheet for Yaluma at 1:100 000 scale. The first two digits define a longitude band 0.5 degree wide and the second two digits a latitude band 0.5 degree wide."@en ;
    skos:inScheme cs: ;
    skos:notation "6547" ;
    skos:prefLabel "Yaluma:6547"@en ;
.

geoad:Yamma8441
    a skos:Concept ;
    skos:historyNote "Compiled by the Geological Survey of Queensland" ;
    skos:broader geoad:MapSeries ;
    skos:definition "Map sheet for Yamma at 1:100 000 scale. The first two digits define a longitude band 0.5 degree wide and the second two digits a latitude band 0.5 degree wide."@en ;
    skos:inScheme cs: ;
    skos:notation "8441" ;
    skos:prefLabel "Yamma:8441"@en ;
.

geoad:Yaniabulla7939
    a skos:Concept ;
    skos:historyNote "Compiled by the Geological Survey of Queensland" ;
    skos:broader geoad:MapSeries ;
    skos:definition "Map sheet for Yaniabulla at 1:100 000 scale. The first two digits define a longitude band 0.5 degree wide and the second two digits a latitude band 0.5 degree wide."@en ;
    skos:inScheme cs: ;
    skos:notation "7939" ;
    skos:prefLabel "Yaniabulla:7939"@en ;
.

geoad:Yaraka7748
    a skos:Concept ;
    skos:historyNote "Compiled by the Geological Survey of Queensland" ;
    skos:broader geoad:MapSeries ;
    skos:definition "Map sheet for Yaraka at 1:100 000 scale. The first two digits define a longitude band 0.5 degree wide and the second two digits a latitude band 0.5 degree wide."@en ;
    skos:inScheme cs: ;
    skos:notation "7748" ;
    skos:prefLabel "Yaraka:7748"@en ;
.

geoad:Yarmouth8142
    a skos:Concept ;
    skos:historyNote "Compiled by the Geological Survey of Queensland" ;
    skos:broader geoad:MapSeries ;
    skos:definition "Map sheet for Yarmouth at 1:100 000 scale. The first two digits define a longitude band 0.5 degree wide and the second two digits a latitude band 0.5 degree wide."@en ;
    skos:inScheme cs: ;
    skos:notation "8142" ;
    skos:prefLabel "Yarmouth:8142"@en ;
.

geoad:Yarrowmere8055
    a skos:Concept ;
    skos:historyNote "Compiled by the Geological Survey of Queensland" ;
    skos:broader geoad:MapSeries ;
    skos:definition "Map sheet for Yarrowmere at 1:100 000 scale. The first two digits define a longitude band 0.5 degree wide and the second two digits a latitude band 0.5 degree wide."@en ;
    skos:inScheme cs: ;
    skos:notation "8055" ;
    skos:prefLabel "Yarrowmere:8055"@en ;
.

geoad:Yelvertoft6657
    a skos:Concept ;
    skos:historyNote "Compiled by the Geological Survey of Queensland" ;
    skos:broader geoad:MapSeries ;
    skos:definition "Map sheet for Yelvertoft at 1:100 000 scale. The first two digits define a longitude band 0.5 degree wide and the second two digits a latitude band 0.5 degree wide."@en ;
    skos:inScheme cs: ;
    skos:notation "6657" ;
    skos:prefLabel "Yelvertoft:6657"@en ;
.

geoad:Yeriecoola6844
    a skos:Concept ;
    skos:historyNote "Compiled by the Geological Survey of Queensland" ;
    skos:broader geoad:MapSeries ;
    skos:definition "Map sheet for Yeriecoola at 1:100 000 scale. The first two digits define a longitude band 0.5 degree wide and the second two digits a latitude band 0.5 degree wide."@en ;
    skos:inScheme cs: ;
    skos:notation "6844" ;
    skos:prefLabel "Yeriecoola:6844"@en ;
.

geoad:Yetman9040
    a skos:Concept ;
    skos:historyNote "Compiled by the Geological Survey of Queensland" ;
    skos:broader geoad:MapSeries ;
    skos:definition "Map sheet for Yetman at 1:100 000 scale. The first two digits define a longitude band 0.5 degree wide and the second two digits a latitude band 0.5 degree wide."@en ;
    skos:inScheme cs: ;
    skos:notation "9040" ;
    skos:prefLabel "Yetman:9040"@en ;
.

geoad:YorkDowns7372
    a skos:Concept ;
    skos:historyNote "Compiled by the Geological Survey of Queensland" ;
    skos:broader geoad:MapSeries ;
    skos:definition "Map sheet for York Downs at 1:100 000 scale. The first two digits define a longitude band 0.5 degree wide and the second two digits a latitude band 0.5 degree wide."@en ;
    skos:inScheme cs: ;
    skos:notation "7372" ;
    skos:prefLabel "York Downs:7372"@en ;
.

geoad:Yowah7841
    a skos:Concept ;
    skos:historyNote "Compiled by the Geological Survey of Queensland" ;
    skos:broader geoad:MapSeries ;
    skos:definition "Map sheet for Yowah at 1:100 000 scale. The first two digits define a longitude band 0.5 degree wide and the second two digits a latitude band 0.5 degree wide."@en ;
    skos:inScheme cs: ;
    skos:notation "7841" ;
    skos:prefLabel "Yowah:7841"@en ;
.

geoad:Yuleba8744
    a skos:Concept ;
    skos:historyNote "Compiled by the Geological Survey of Queensland" ;
    skos:broader geoad:MapSeries ;
    skos:definition "Map sheet for Yuleba at 1:100 000 scale. The first two digits define a longitude band 0.5 degree wide and the second two digits a latitude band 0.5 degree wide."@en ;
    skos:inScheme cs: ;
    skos:notation "8744" ;
    skos:prefLabel "Yuleba:8744"@en ;
.

geoad:ZigZag8351
    a skos:Concept ;
    skos:historyNote "Compiled by the Geological Survey of Queensland" ;
    skos:broader geoad:MapSeries ;
    skos:definition "Map sheet for Zig Zag at 1:100 000 scale. The first two digits define a longitude band 0.5 degree wide and the second two digits a latitude band 0.5 degree wide."@en ;
    skos:inScheme cs: ;
    skos:notation "8351" ;
    skos:prefLabel "Zig Zag:8351"@en ;
.

geoad:Block
    a skos:Concept ;
    skos:historyNote "Compiled by the Geological Survey of Queensland" ;
    rdfs:isDefinedBy cs: ;
    skos:definition "A Block is an administrative division of the State of Queensland that is used for tenure management. A Block is defined as five minutes of latitude by five minutes of longitude. Blocks are grouped by 1:1,000,000 map sheet areas, the names of which provide the containing Blocks with a four letter prefix (e.g. Clermont 1:1,000,000 provides CLER). Each sheet area contains 3456 Blocks, with the Blocks numbered between 1 and 3456 inclusive. A Block is divided into 25 Sub-Blocks."@en ;
    skos:inScheme cs: ;
    skos:prefLabel "Block"@en ;
.

geoad:Permit
    a skos:Concept ;
    skos:historyNote "Compiled by the Geological Survey of Queensland" ;
    rdfs:isDefinedBy cs: ;
    skos:definition "Permits are a license granted over a spatial region within the State of Queensland. Permits govern the activities which can be conducted upon them. Activities include exploration, development, and extraction of a specific commodity or commodities."@en ;
    skos:inScheme cs: ;
    skos:prefLabel "Permit"@en ;
.

geoad:SubBlock
    a skos:Concept ;
    skos:historyNote "Compiled by the Geological Survey of Queensland" ;
    rdfs:isDefinedBy cs: ;
    skos:definition "A Sub-Block is an administrative sub-division of a Block. Each Block is divided into 25 Sub-Blocks. A Sub-Block is defined as one minute of latitude by one minute of longitude. The Sub-Blocks are prefixed with their corresponding Block name and are labelled from A to Z, excluding I. Labels are allocated from left to right, top to bottom, starting from the northwest corner."@en ;
    skos:inScheme cs: ;
    skos:prefLabel "Sub-Block"@en ;
.

geoad:MapSeries
    a skos:Concept ;
    skos:historyNote "Compiled by the Geological Survey of Queensland" ;
    rdfs:isDefinedBy cs: ;
    skos:definition "A map series is a group of topographic or thematic maps or charts usually having the same scale and cartographic specifications, and with each sheet appropriately identified by its publisher as belonging to the same series. Map series occur when an area is to be covered by a map that, due to its scale, must be spread over several sheets. Nevertheless, the individual sheets of a map series can also be used quite independently, as they generally have full map surround details and legends. If a publisher produces several map series at different scales, then these series are called scale series."@en ;
    skos:inScheme cs: ;
    skos:prefLabel "Map Series"@en ;
.

cs:
    a
        owl:Ontology ,
        skos:ConceptScheme ;
    dcterms:created "2019-12-04"^^xsd:date ;
    dcterms:creator <https://linked.data.gov.au/org/gsq> ;
    dcterms:modified "2023-03-16"^^xsd:date ;
    skos:historyNote "Compiled by the Geological Survey of Queensland" ;
    dcterms:publisher <https://linked.data.gov.au/org/gsq> ;
    reg:status agldwgstatus:stable ;
    owl:imports <http://www.opengis.net/ont/geosparql> ;
    skos:definition "This vocabulary lists types of geological administrative features relevant to the duties of the Geological Survey of Queensland. An Administrative Feature is a geo:Feature that is defined by adminstrative processes such as legislation, regulation, policy or procedure."@en ;
    skos:hasTopConcept
        geoad:Block ,
        geoad:MapSeries ,
        geoad:Permit ,
        geoad:SubBlock ;
    skos:prefLabel "GeoAdmin Features"@en ;
.

