PREFIX agldwgstatus: <https://linked.data.gov.au/def/reg-statuses/>
PREFIX cs: <http://linked.data.gov.au/def/geological-properties>
PREFIX dcterms: <http://purl.org/dc/terms/>
PREFIX gprp: <http://linked.data.gov.au/def/geological-properties/>
PREFIX owl: <http://www.w3.org/2002/07/owl#>
PREFIX rdfs: <http://www.w3.org/2000/01/rdf-schema#>
PREFIX reg: <http://purl.org/linked-data/registry#>
PREFIX sdo: <https://schema.org/>
PREFIX skos: <http://www.w3.org/2004/02/skos/core#>
PREFIX xsd: <http://www.w3.org/2001/XMLSchema#>

gprp:AgeAbsoluteMax
    a skos:Concept ;
    dcterms:provenance "Construction by the GSQ. Initial version derived from rock unit properties" ;
    rdfs:isDefinedBy cs: ;
    skos:altLabel "Max Age"@en ;
    skos:broader gprp:AgeAbsolute ;
    skos:definition "The numeric age of the oldest chronological layer or section of a geological feature."@en ;
    skos:inScheme cs: ;
    skos:prefLabel "Maximum Absolute Age"@en ;
.

gprp:AgeAbsoluteMin
    a skos:Concept ;
    dcterms:provenance "Construction by the GSQ. Initial version derived from rock unit properties" ;
    rdfs:isDefinedBy cs: ;
    skos:altLabel "Min Age"@en ;
    skos:broader gprp:AgeAbsolute ;
    skos:definition "The numeric age of the youngest chronological layer or section of a geological feature."@en ;
    skos:inScheme cs: ;
    skos:prefLabel "Minimum Absolute Age"@en ;
.

gprp:AgeChronoLower
    a skos:Concept ;
    dcterms:provenance "Construction by the GSQ. Initial version derived from rock unit properties" ;
    rdfs:isDefinedBy cs: ;
    skos:altLabel "Age From"@en ;
    skos:broader gprp:AgeChrono ;
    skos:definition "The named age of the lowest and oldest chronological layer or section of a geological feature as per the international chronostratigraphic chart."@en ;
    skos:inScheme cs: ;
    skos:prefLabel "Lower Age"@en ;
.

gprp:AgeChronoUpper
    a skos:Concept ;
    dcterms:provenance "Construction by the GSQ. Initial version derived from rock unit properties" ;
    rdfs:isDefinedBy cs: ;
    skos:altLabel "Age To"@en ;
    skos:broader gprp:AgeChrono ;
    skos:definition "The age of the upper-most and youngest chronological layer or section of a geological feature as per the international chronostratigraphic chart."@en ;
    skos:inScheme cs: ;
    skos:prefLabel "Upper Age"@en ;
.

gprp:ResourceProspectivity
    a skos:Concept ;
    dcterms:provenance "Construction by the GSQ. Initial version derived from rock unit properties" ;
    rdfs:isDefinedBy cs: ;
    skos:definition "The potential or maturity of a resource accumulation (Mineral Occurrence, Coal Deposit, Petroleum Play) to be progressed to economic development. The progress from discovery or lead, to prospect, to opportunity. Related to the resource project lifecycle."@en ;
    skos:inScheme cs: ;
    skos:prefLabel "Resource Prospectivity"@en ;
    skos:topConceptOf cs: ;
.

gprp:ThicknessAtTypeSection
    a skos:Concept ;
    dcterms:provenance "Construction by the GSQ. Initial version derived from rock unit properties" ;
    rdfs:isDefinedBy cs: ;
    skos:broader gprp:Thickness ;
    skos:definition "The thickness of the feature at the type section of representative site."@en ;
    skos:inScheme cs: ;
    skos:prefLabel "Type Section Thickness"@en ;
.

gprp:ThicknessAverage
    a skos:Concept ;
    dcterms:provenance "Construction by the GSQ. Initial version derived from rock unit properties" ;
    rdfs:isDefinedBy cs: ;
    skos:broader gprp:Thickness ;
    skos:definition "The average thickness of the feature."@en ;
    skos:inScheme cs: ;
    skos:prefLabel "Average Thickness"@en ;
.

gprp:ThicknessMax
    a skos:Concept ;
    dcterms:provenance "Construction by the GSQ. Initial version derived from rock unit properties" ;
    rdfs:isDefinedBy cs: ;
    skos:broader gprp:Thickness ;
    skos:definition "The maximum thickness of the feature."@en ;
    skos:inScheme cs: ;
    skos:prefLabel "Maximum Thickness"@en ;
.

gprp:ThicknessMin
    a skos:Concept ;
    dcterms:provenance "Construction by the GSQ. Initial version derived from rock unit properties" ;
    rdfs:isDefinedBy cs: ;
    skos:broader gprp:Thickness ;
    skos:definition "The minimum thickness of the feature."@en ;
    skos:inScheme cs: ;
    skos:prefLabel "Minimum Thickness"@en ;
.

gprp:DepthMax
    a skos:Concept ;
    dcterms:provenance "Construction by the GSQ. Initial version derived from rock unit properties" ;
    rdfs:isDefinedBy cs: ;
    skos:altLabel "Max Depth"@en ;
    skos:definition "The maximum depth of a geological feature. This may be to underlying 'basement' rock or a defined boundary. Traditionally this is measured in distance (feet, metres, miles, kilometres) or time from seismic acquisition techniques represented as 1-way or 2-way time (seconds, milliseconds)"@en ;
    skos:inScheme cs: ;
    skos:prefLabel "Maximum Depth"@en ;
.

gprp:DominantElement
    a skos:Concept ;
    dcterms:provenance "Construction by the GSQ. Initial version derived from rock unit properties" ;
    rdfs:isDefinedBy cs: ;
    skos:definition "The most prevalent element present in the geological feature."@en ;
    skos:inScheme cs: ;
    skos:prefLabel "Dominant Element"@en ;
    skos:topConceptOf cs: ;
.

gprp:DominantMineral
    a skos:Concept ;
    dcterms:provenance "Construction by the GSQ. Initial version derived from rock unit properties" ;
    rdfs:isDefinedBy cs: ;
    skos:definition "The most prevalent mineral species present in the geological feature."@en ;
    skos:inScheme cs: ;
    skos:prefLabel "Dominant Mineral"@en ;
    skos:topConceptOf cs: ;
.

gprp:DominantRock
    a skos:Concept ;
    dcterms:provenance "Construction by the GSQ. Initial version derived from rock unit properties" ;
    rdfs:isDefinedBy cs: ;
    skos:definition "The most prevalent rock type present in the geological feature."@en ;
    skos:inScheme cs: ;
    skos:prefLabel "Dominant Rock"@en ;
    skos:topConceptOf cs: ;
.

gprp:Extent
    a skos:Concept ;
    dcterms:provenance "Construction by the GSQ. Initial version derived from rock unit properties" ;
    rdfs:isDefinedBy cs: ;
    skos:altLabel "Area"@en ;
    skos:definition "The spatial extent or area covered by a feature at the surface of the Earth."@en ;
    skos:inScheme cs: ;
    skos:prefLabel "Extent"@en ;
    skos:topConceptOf cs: ;
.

gprp:RockUnitRank
    a skos:Concept ;
    dcterms:provenance "Construction by the GSQ. Initial version derived from rock unit properties" ;
    rdfs:isDefinedBy cs: ;
    skos:definition "The rank of a rock unit in as defined by its type, extent, and relationships to other rock units. For example, in stratigraphic rock units: Supergroup, group, subgroup, formation, member, bed, and in igneous rock units: Supersuite, suite etc."@en ;
    skos:inScheme cs: ;
    skos:prefLabel "Rock Unit Rank"@en ;
    skos:topConceptOf cs: ;
.

gprp:TypeLocality
    a skos:Concept ;
    dcterms:provenance "Construction by the GSQ. Initial version derived from rock unit properties" ;
    rdfs:isDefinedBy cs: ;
    skos:definition "The location of the type section or representative site. This may be a property name, outcrop name, coordinates, or associated geomorpholgical feature."@en ;
    skos:inScheme cs: ;
    skos:prefLabel "Type Locality"@en ;
    skos:scopeNote "The locality is used as the defining site that pertains to the feature description."@en ;
    skos:topConceptOf cs: ;
.

<https://linked.data.gov.au/org/gsq>
    a sdo:Organization ;
    sdo:name "Geological Survey of Queensland" ;
    sdo:url "https://www.business.qld.gov.au/industries/mining-energy-water/resources/geoscience-information/gsq"^^xsd:anyURI ;
.

gprp:AgeAbsolute
    a skos:Concept ;
    dcterms:provenance "Construction by the GSQ. Initial version derived from rock unit properties" ;
    rdfs:isDefinedBy cs: ;
    skos:definition "The numeric age of the geological feature, typically represented in thousands, millions, or billions of years, with millions of years (MA) being the most common."@en ;
    skos:inScheme cs: ;
    skos:prefLabel "Absolute Age"@en ;
    skos:topConceptOf cs: ;
.

gprp:AgeChrono
    a skos:Concept ;
    dcterms:provenance "Construction by the GSQ. Initial version derived from rock unit properties" ;
    rdfs:isDefinedBy cs: ;
    skos:definition "The named age of the geological feature as per the international chronostratigraphic chart."@en ;
    skos:inScheme cs: ;
    skos:prefLabel "Chronological Age"@en ;
    skos:topConceptOf cs: ;
.

gprp:Thickness
    a skos:Concept ;
    dcterms:provenance "Construction by the GSQ. Initial version derived from rock unit properties" ;
    rdfs:isDefinedBy cs: ;
    skos:definition "The thickness of the geological feature."@en ;
    skos:inScheme cs: ;
    skos:prefLabel "Thickness"@en ;
    skos:scopeNote "This unspecified level categorisation should only be used where the thickness is not at the type location and not numerically specific (average, maximuim, or minimum)."@en ;
    skos:topConceptOf cs: ;
.

cs:
    a
        owl:Ontology ,
        skos:ConceptScheme ;
    dcterms:created "2022-09-13"^^xsd:date ;
    dcterms:creator <https://linked.data.gov.au/org/gsq> ;
    dcterms:modified "2023-03-16"^^xsd:date ;
    dcterms:provenance "Construction by the GSQ. Initial version derived from rock unit properties" ;
    dcterms:publisher <https://linked.data.gov.au/org/gsq> ;
    reg:status agldwgstatus:stable ;
    skos:definition "The geological properties that can be interpreted or concluded about a geological feature based on the analysis of observations and results of that feature."@en ;
    skos:hasTopConcept
        gprp:AgeAbsolute ,
        gprp:AgeChrono ,
        gprp:DepthMax ,
        gprp:DominantElement ,
        gprp:DominantMineral ,
        gprp:DominantRock ,
        gprp:Extent ,
        gprp:RockUnitRank ,
        gprp:Thickness ,
        gprp:TypeLocality ;
    skos:prefLabel "Geological Properties"@en ;
.

