PREFIX agldwgstatus: <https://linked.data.gov.au/def/reg-statuses/>
PREFIX cs: <http://linked.data.gov.au/def/geological-observation-method>
PREFIX dcterms: <http://purl.org/dc/terms/>
PREFIX obsmh: <http://linked.data.gov.au/def/geological-observation-method/>
PREFIX owl: <http://www.w3.org/2002/07/owl#>
PREFIX rdfs: <http://www.w3.org/2000/01/rdf-schema#>
PREFIX reg: <http://purl.org/linked-data/registry#>
PREFIX sdo: <https://schema.org/>
PREFIX skos: <http://www.w3.org/2004/02/skos/core#>
PREFIX xsd: <http://www.w3.org/2001/XMLSchema#>

obsmh:electrical-methods
    a skos:Collection ;
    skos:historyNote "Compiled by the Geological Survey of Queensland" ;
    skos:definition "The classification of methods used in electrical geophysical survey acquisition."@en ;
    skos:member
        obsmh:cr ,
        obsmh:dcr ,
        obsmh:ert ,
        obsmh:ip ,
        obsmh:sp ,
        obsmh:ves ;
    skos:prefLabel "Electrical Geophysical Methods"@en ;
.

obsmh:em-methods
    a skos:Collection ;
    skos:historyNote "Compiled by the Geological Survey of Queensland" ;
    skos:definition "The classification of methods used in electromagnetic geophysical survey acquisition."@en ;
    skos:member
        obsmh:flem ,
        obsmh:gpr ,
        obsmh:mlem ,
        obsmh:sam ,
        obsmh:tem ;
    skos:prefLabel "Electromagnetic Geophysical Methods"@en ;
.

obsmh:mt-methods
    a skos:Collection ;
    skos:historyNote "Compiled by the Geological Survey of Queensland" ;
    skos:definition "The classification of methods used in magnetotelluric geophysical survey acquisition."@en ;
    skos:member
        obsmh:amt ,
        obsmh:bbmt ,
        obsmh:csem ,
        obsmh:lpmt ;
    skos:prefLabel "Magnetotelluric Methods"@en ;
.

obsmh:seismic-methods
    a skos:Collection ;
    skos:historyNote "Compiled by the Geological Survey of Queensland" ;
    skos:definition "The classification of tools used as an energy source that generate a seismic signal for use in seismic survey acquisition."@en ;
    skos:member
        obsmh:accelerated-weight-drop ,
        obsmh:air-gun ,
        obsmh:boomer ,
        obsmh:dynamite ,
        obsmh:firearm ,
        obsmh:hammer ,
        obsmh:hydraulic-oil-impactor ,
        obsmh:noise-source ,
        obsmh:plasma-sound-source ,
        obsmh:vibroseis ,
        obsmh:wacker ,
        obsmh:water-gun ,
        obsmh:weight-drop ;
    skos:prefLabel "Seismic Methods"@en ;
.

obsmh:spatial-methods
    a skos:Collection ;
    skos:historyNote "Compiled by the Geological Survey of Queensland" ;
    skos:definition "The classification of methods used in spatial survey acquisition."@en ;
    skos:member
        obsmh:laser-altimetry ,
        obsmh:lidar ,
        obsmh:radar ,
        obsmh:sar ;
    skos:prefLabel "Spatial Methods"@en ;
.

obsmh:spectral-methods
    a skos:Collection ;
    skos:historyNote "Compiled by the Geological Survey of Queensland" ;
    skos:definition "The classification of methods used in spectral survey acquisition."@en ;
    skos:member
        obsmh:imaging-radiometer ,
        obsmh:interferometer ,
        obsmh:radiometer ,
        obsmh:spectrometer ,
        obsmh:spectroradiometer ,
        obsmh:xrd ,
        obsmh:xrf ;
    skos:prefLabel "Spectral Methods"@en ;
.

obsmh:direct
    a skos:Concept ;
    skos:historyNote "Compiled by the Geological Survey of Queensland" ;
    rdfs:isDefinedBy cs: ;
    skos:altLabel "Human Observed"@en ;
    skos:definition "An observation method whereby the observation is made directly by a human."@en ;
    skos:inScheme cs: ;
    skos:prefLabel "Direct Observation"@en ;
    skos:topConceptOf cs: ;
.

obsmh:imaging-radiometer
    a skos:Concept ;
    skos:historyNote "Compiled by the Geological Survey of Queensland" ;
    rdfs:isDefinedBy cs: ;
    skos:broader obsmh:radiometer ;
    skos:definition "A radiometer that has a scanning capability to provide a two-dimensional array of pixels from which an image may be produced. Scanning can be performed mechanically or electronically by using an array of detectors. Source:NASA EarthData"@en ;
    skos:inScheme cs: ;
    skos:prefLabel "Imaging Radiometry"@en ;
.

obsmh:interferometer
    a skos:Concept ;
    skos:historyNote "Compiled by the Geological Survey of Queensland" ;
    rdfs:isDefinedBy cs: ;
    skos:broader obsmh:passive-spectral ;
    skos:definition "A family of techniques in which waves, usually electromagnetic waves, are superimposed, causing the phenomenon of interference, which is used to extract information."@en ;
    skos:inScheme cs: ;
    skos:prefLabel "Interferometry"@en ;
.

obsmh:laser-altimetry
    a skos:Concept ;
    skos:historyNote "Compiled by the Geological Survey of Queensland" ;
    rdfs:isDefinedBy cs: ;
    skos:altLabel "laser altimeter"@en ;
    skos:definition "Laser altimetry is a group of active remote sensing techniques in which laser pulses are emitted and  are reflected from the ground surface; part of the reflected radiation returns to the sensor; then, the distance from the ground surface can be calculated considering the speed of light ."@en ;
    skos:inScheme cs: ;
    skos:prefLabel "Laser Altimetry"@en ;
    skos:topConceptOf cs: ;
.

obsmh:lidar
    a skos:Concept ;
    skos:historyNote "Compiled by the Geological Survey of Queensland" ;
    rdfs:isDefinedBy cs: ;
    skos:altLabel
        "3-D laser scanning"@en ,
        "LADAR"@en ,
        "Laser Ranging"@en ,
        "laser imaging, detection, and ranging"@en ,
        "light detection and ranging"@en ;
    skos:definition "A method for measuring distances (ranging) by illuminating the target with laser light and measuring the reflection with a sensor.."@en ;
    skos:inScheme cs: ;
    skos:prefLabel "LIDAR"@en ;
    skos:topConceptOf cs: ;
.

obsmh:sar
    a skos:Concept ;
    skos:historyNote "Compiled by the Geological Survey of Queensland" ;
    rdfs:isDefinedBy cs: ;
    skos:altLabel "SAR"@en ;
    skos:broader obsmh:radar ;
    skos:definition "A form of radar that is used to create two-dimensional images or three-dimensional reconstructions of objects, such as landscapes.[1] SAR uses the motion of the radar antenna over a target region to provide finer spatial resolution than conventional beam-scanning radars."@en ;
    skos:inScheme cs: ;
    skos:prefLabel "Synthetic-Aperture Radar"@en ;
.

obsmh:spectrometer
    a skos:Concept ;
    skos:historyNote "Compiled by the Geological Survey of Queensland" ;
    rdfs:isDefinedBy cs: ;
    skos:altLabel "Spectrometer"@en ;
    skos:broader obsmh:passive-spectral ;
    skos:definition "A device that is designed to detect, measure, and analyze the spectral content of incident electromagnetic radiation. Conventional imaging spectrometers use gratings or prisms to disperse the radiation for spectral discrimination. Source:NASA EarthData"@en ;
    skos:inScheme cs: ;
    skos:prefLabel "Spectrometry"@en ;
.

obsmh:spectroradiometer
    a skos:Concept ;
    skos:historyNote "Compiled by the Geological Survey of Queensland" ;
    rdfs:isDefinedBy cs: ;
    skos:altLabel "Spectroradiometer"@en ;
    skos:broader obsmh:passive-spectral ;
    skos:definition "A radiometer that measures the intensity of radiation in multiple wavelength bands (i.e., multispectral). Many times the bands are of high-spectral resolution, designed for remotely sensing specific geophysical parameters. Source:NASA EarthData"@en ;
    skos:inScheme cs: ;
    skos:prefLabel "Spectroradiometry"@en ;
.

obsmh:xrd
    a skos:Concept ;
    skos:historyNote "Compiled by the Geological Survey of Queensland" ;
    rdfs:isDefinedBy cs: ;
    skos:altLabel "XRD"@en ;
    skos:broader obsmh:active-spectral ;
    skos:definition "A non-destructive technique for identifying and quantifying the mineralogy of crystalline compounds in rocks, soils and particulates. Monochromatic X-rays are projected onto a crystalline material at an angle (θ) and diffraction occurs when the distance traveled by the rays reflected from successive planes differs by an integer(n) of wavelengths (λ). Every mineral or compound has a characteristic X-ray diffraction pattern whose 'fingerprint'. Source:British Geological Survey"@en ;
    skos:inScheme cs: ;
    skos:prefLabel "X-ray diffraction"@en ;
.

obsmh:xrf
    a skos:Concept ;
    skos:historyNote "Compiled by the Geological Survey of Queensland" ;
    rdfs:isDefinedBy cs: ;
    skos:altLabel "XRF"@en ;
    skos:broader obsmh:active-spectral ;
    skos:definition "A non-destructive analytical technique used to determine the elemental composition of materials. XRF analyzers determine the chemistry of a sample by measuring the fluorescent (or secondary) X-ray emitted from a sample when it is excited by a primary X-ray source. Source:ThermoFisher Scientific"@en ;
    skos:inScheme cs: ;
    skos:prefLabel "X-ray fluorescence"@en ;
.

obsmh:accelerated-weight-drop
    a skos:Concept ;
    skos:historyNote "Compiled by the Geological Survey of Queensland" ;
    rdfs:isDefinedBy cs: ;
    skos:altLabel "AWD"@en ;
    skos:definition "A mass, or striker, is held above the impact point on the ground surface. The mass is then released and propelled into the impact point to generate a seismic pulse."@en ;
    skos:inScheme cs: ;
    skos:prefLabel "Accelerated Weight Drop"@en ;
    skos:topConceptOf cs: ;
.

obsmh:air-gun
    a skos:Concept ;
    skos:historyNote "Compiled by the Geological Survey of Queensland" ;
    rdfs:isDefinedBy cs: ;
    skos:altLabel "Air Pulse"@en ;
    skos:definition "Metal cylinders through which high pressure air is forced through and into the water column. The injection of air into the water creates a pressure pulse that travels through the water and into the subsurface. It is common to have multiple airguns firing at once to create an array."@en ;
    skos:inScheme cs: ;
    skos:prefLabel "Air Gun"@en ;
    skos:topConceptOf cs: ;
.

obsmh:amt
    a skos:Concept ;
    skos:historyNote "Compiled by the Geological Survey of Queensland" ;
    rdfs:isDefinedBy cs: ;
    skos:altLabel
        "A.M.T"@en ,
        "AMT"@en ;
    skos:definition "A higher-frequency magnetotelluric technique for shallower investigations. AMT has less depth penetration than MT but commonly take approximately one hour to perform whereas deep AMT measurements during low-signal strength periods may take up to 24 hours."@en ;
    skos:inScheme cs: ;
    skos:prefLabel "Audio-magnetotellurics"@en ;
    skos:topConceptOf cs: ;
.

obsmh:bbmt
    a skos:Concept ;
    skos:historyNote "Compiled by the Geological Survey of Queensland" ;
    rdfs:isDefinedBy cs: ;
    skos:altLabel
        "B.B.M.T"@en ,
        "BBMT"@en ,
        "W.B.M.T."@en ,
        "WBMT"@en ,
        "Wide band magnetotellurics"@en ;
    skos:definition "A magnetotellurics technique combining long-period and audio magentotelluric frequencies to create a broadband electrical signal."@en ;
    skos:inScheme cs: ;
    skos:prefLabel "Broadband magnetotellurics"@en ;
    skos:topConceptOf cs: ;
.

obsmh:boomer
    a skos:Concept ;
    skos:historyNote "Compiled by the Geological Survey of Queensland" ;
    rdfs:isDefinedBy cs: ;
    skos:altLabel
        "Bang Box"@en ,
        "Boomers"@en ;
    skos:definition "Energy is stored in capacitors and discharges through a flat spiral coil with no spark. A copper plate adjacent to the coil flexes away from the coil as the capacitors are discharged. This flexing is transmitted into the water as the seismic pulse. Boomers are towed in a floating sled behind a survey vessel."@en ;
    skos:inScheme cs: ;
    skos:prefLabel "Boomer"@en ;
    skos:topConceptOf cs: ;
.

obsmh:cr
    a skos:Concept ;
    skos:historyNote "Compiled by the Geological Survey of Queensland" ;
    rdfs:isDefinedBy cs: ;
    skos:altLabel
        "C.C."@en ,
        "C.R."@en ,
        "CC"@en ,
        "CR"@en ,
        "Complex Conductivity"@en ,
        "S.I.P."@en ,
        "SIP"@en ,
        "Spectral Induced Polarisation"@en ,
        "Spectral Induced Polarization"@en ;
    skos:definition "A geophysical survey technique and an extension of the induced polarization (IP) method that measures the frequency-dependent (i.e. spectral) complex impedance, equivalent to the amount of resistance and phase shift between electric current and voltage."@en ;
    skos:inScheme cs: ;
    skos:prefLabel "Complex Resistivity"@en ;
    skos:topConceptOf cs: ;
.

obsmh:csem
    a skos:Concept ;
    skos:historyNote "Compiled by the Geological Survey of Queensland" ;
    rdfs:isDefinedBy cs: ;
    skos:altLabel
        "Audio-frequency Magnetotellurics"@en ,
        "C.S.A.M.T."@en ,
        "C.S.E.M"@en ,
        "C.S.M.T."@en ,
        "CSAMT"@en ,
        "CSEM"@en ,
        "CSMT"@en ,
        "Controlled source audio-frequency Magnetotellurics"@en ,
        "Controlled source electromagnetics"@en ;
    skos:definition "A low-impact, ground geophysical survey method transmitting a controlled electric signal at a suite of frequencies into the ground from one location (transmitter site) and measuring the received electric and magnetic fields in the area of interest (receiver site)."@en ;
    skos:inScheme cs: ;
    skos:prefLabel "Controlled source magnetotellurics"@en ;
    skos:topConceptOf cs: ;
.

obsmh:dcr
    a skos:Concept ;
    skos:historyNote "Compiled by the Geological Survey of Queensland" ;
    rdfs:isDefinedBy cs: ;
    skos:altLabel
        "D.C.R."@en ,
        "DCR"@en ,
        "Direct Current Resistivity"@en ;
    skos:definition "An electircal geophysical method where an electrical current is injected into the earth. The current path depends upon the variation of conductivity or equivalently, its reciprocal, the electrical resistivity."@en ;
    skos:inScheme cs: ;
    skos:prefLabel "DC Resistivity"@en ;
    skos:topConceptOf cs: ;
.

obsmh:dynamite
    a skos:Concept ;
    skos:historyNote "Compiled by the Geological Survey of Queensland" ;
    rdfs:isDefinedBy cs: ;
    skos:definition "An explosive consisting of nitroglycerine mixed with an absorbent material and typically moulded into sticks. A stick is placed into a shallow borehole and detonated to generate a seismic pulse."@en ;
    skos:inScheme cs: ;
    skos:prefLabel "Dynamite"@en ;
    skos:topConceptOf cs: ;
.

obsmh:ert
    a skos:Concept ;
    skos:historyNote "Compiled by the Geological Survey of Queensland" ;
    rdfs:isDefinedBy cs: ;
    skos:altLabel
        "E.R.I."@en ,
        "E.R.T."@en ,
        "ERI"@en ,
        "ERT"@en ,
        "Electrical Resistivity Imaging"@en ;
    skos:definition "A geophysical technique for imaging sub-surface structures from electrical resistivity measurements made at the surface, or by electrodes in one or more boreholes. "@en ;
    skos:inScheme cs: ;
    skos:prefLabel "Electrical Resistivity Tomography"@en ;
    skos:topConceptOf cs: ;
.

obsmh:firearm
    a skos:Concept ;
    skos:historyNote "Compiled by the Geological Survey of Queensland" ;
    rdfs:isDefinedBy cs: ;
    skos:altLabel
        "Betsy Gun"@en ,
        "Pistol"@en ,
        "Shotgun"@en ;
    skos:definition "A gunpowder-based firearm is discharged in a shallow borehole to generate a seismic pulse."@en ;
    skos:inScheme cs: ;
    skos:prefLabel "Firearm"@en ;
    skos:topConceptOf cs: ;
.

obsmh:flem
    a skos:Concept ;
    skos:historyNote "Compiled by the Geological Survey of Queensland" ;
    rdfs:isDefinedBy cs: ;
    skos:altLabel
        "F.L.E.M."@en ,
        "FLEM"@en ;
    skos:definition "A non-destructive testing tool for mapping sub-surface changes in electrical conductivity. At a specified station, or sounding location, a transmitted EM field is generated by a transmitter coil to induce an electrical current in the subsurface. In a fixed-loop survey a large transmitter loop is placed in a fixed position and measurements are made along a survey line at a series of receiver positions. The induced subsurface secondary field which is created by the induced subsurface electrical current is detected by the EM receiver. The MLEM equipment measures the conductivity value with time at the sounding location. Sources:Draig Geoscience & University of Queensland"@en ;
    skos:inScheme cs: ;
    skos:prefLabel "Fixed-Loop Electromagnetics"@en ;
    skos:topConceptOf cs: ;
.

obsmh:gpr
    a skos:Concept ;
    skos:historyNote "Compiled by the Geological Survey of Queensland" ;
    rdfs:isDefinedBy cs: ;
    skos:altLabel
        "G.P.R."@en ,
        "GPR"@en ,
        "Ground Probing Radar"@en ;
    skos:definition "A geophysical method that uses radar pulses to image the subsurface. "@en ;
    skos:inScheme cs: ;
    skos:prefLabel "Ground Penetrating Radar"@en ;
    skos:topConceptOf cs: ;
.

obsmh:hammer
    a skos:Concept ;
    skos:historyNote "Compiled by the Geological Survey of Queensland" ;
    rdfs:isDefinedBy cs: ;
    skos:altLabel
        "Sledge Hammer"@en ,
        "Sledgehammer"@en ;
    skos:definition "A large hand-held hammer is used to strike a metal plate on the ground surface to generate a seismic pulse."@en ;
    skos:inScheme cs: ;
    skos:prefLabel "Hammer"@en ;
    skos:topConceptOf cs: ;
.

obsmh:hydraulic-oil-impactor
    a skos:Concept ;
    skos:historyNote "Compiled by the Geological Survey of Queensland" ;
    rdfs:isDefinedBy cs: ;
    skos:definition "The transmission of energy wave vibrations into earth strata surrounding a borehole. A hydraulic oscillator acts as a piston and is regulated by a high pressure hydraulic fluid flow into and out of upper and lower chambers surrounding the piston. The device impacts the surrounding strata in the borehole to generate a series of seismic pulses."@en ;
    skos:inScheme cs: ;
    skos:prefLabel "Hydraulic Oil Impactor"@en ;
    skos:topConceptOf cs: ;
.

obsmh:ip
    a skos:Concept ;
    skos:historyNote "Compiled by the Geological Survey of Queensland" ;
    rdfs:isDefinedBy cs: ;
    skos:altLabel
        "I.P."@en ,
        "IP"@en ,
        "Induced Polarization"@en ;
    skos:definition "A geophysical imaging technique used to identify the electrical chargeability of subsurface materials."@en ;
    skos:inScheme cs: ;
    skos:prefLabel "Induced Polarisation"@en ;
    skos:topConceptOf cs: ;
.

obsmh:lpmt
    a skos:Concept ;
    skos:historyNote "Compiled by the Geological Survey of Queensland" ;
    rdfs:isDefinedBy cs: ;
    skos:altLabel
        "L.M.T."@en ,
        "L.P.M.T"@en ,
        "LMT"@en ,
        "LPMT"@en ;
    skos:definition "A magnetotelluric survey method that uses a low frequency (below 1-10Hz) electric signal over an extended period"@en ;
    skos:inScheme cs: ;
    skos:prefLabel "Long Period Magnetotellurics"@en ;
    skos:topConceptOf cs: ;
.

obsmh:mlem
    a skos:Concept ;
    skos:historyNote "Compiled by the Geological Survey of Queensland" ;
    rdfs:isDefinedBy cs: ;
    skos:altLabel
        "M.L.E.M."@en ,
        "MLEM"@en ;
    skos:definition "A non-destructive testing tool for mapping sub-surface changes in electrical conductivity. At a specified station, or sounding location, a transmitted EM field is generated by a transmitter coil to induce an electrical current in the subsurface. In a moving loop survey the transmitter and receiver are moved simultaneously along a survey line. The induced subsurface secondary field which is created by the induced subsurface electrical current is detected by the EM receiver. The MLEM equipment measures the conductivity value with time at the sounding location. Sources:Draig Geoscience & University of Queensland"@en ;
    skos:inScheme cs: ;
    skos:prefLabel "Moving-Loop Electromagnetics"@en ;
    skos:topConceptOf cs: ;
.

obsmh:noise-source
    a skos:Concept ;
    skos:historyNote "Compiled by the Geological Survey of Queensland" ;
    rdfs:isDefinedBy cs: ;
    skos:altLabel "Passive Source"@en ;
    skos:definition "The ambient vibrations transmitted in the ground. Measurements are typically taken over relatively long timeframes."@en ;
    skos:inScheme cs: ;
    skos:prefLabel "Noise Source"@en ;
    skos:topConceptOf cs: ;
.

obsmh:plasma-sound-source
    a skos:Concept ;
    skos:historyNote "Compiled by the Geological Survey of Queensland" ;
    rdfs:isDefinedBy cs: ;
    skos:altLabel
        "Spark Gap"@en ,
        "Spark Gap Sound Source"@en ,
        "Sparker"@en ,
        "Sparkers"@en ;
    skos:definition "An electric charge is stored in a large high-voltage bank of capacitors and then released in an arc across electrodes in the water. The underwater spark discharge produces a high-pressure plasma and vapor bubble, which expands and displaces the surrounding water. The resulting implosion of water to fill the cavity generates a seismic pulse."@en ;
    skos:inScheme cs: ;
    skos:prefLabel "Plasma Sound Source"@en ;
    skos:topConceptOf cs: ;
.

obsmh:radar
    a skos:Concept ;
    skos:historyNote "Compiled by the Geological Survey of Queensland" ;
    rdfs:isDefinedBy cs: ;
    skos:altLabel "Radar Imaging"@en ;
    skos:definition "An application of radar which is used to create two-dimensional images, typically of landscapes. Imaging radar provides its light to illuminate an area on the ground and take a picture at radio wavelengths. It uses an antenna and digital computer storage to record its images.."@en ;
    skos:inScheme cs: ;
    skos:prefLabel "Imaging Radar"@en ;
    skos:topConceptOf cs: ;
.

obsmh:radiometer
    a skos:Concept ;
    skos:historyNote "Compiled by the Geological Survey of Queensland" ;
    rdfs:isDefinedBy cs: ;
    skos:broader obsmh:passive-spectral ;
    skos:definition "An instrument that quantitatively measures the intensity of electromagnetic radiation in some bands within the spectrum. Usually, a radiometer is further identified by the portion of the spectrum it covers; for example, visible, infrared, or microwave. Source:NASA EarthData"@en ;
    skos:inScheme cs: ;
    skos:prefLabel "Radiometry"@en ;
.

obsmh:sam
    a skos:Concept ;
    skos:historyNote "Compiled by the Geological Survey of Queensland" ;
    rdfs:isDefinedBy cs: ;
    skos:altLabel
        "S.A.M."@en ,
        "SAM"@en ;
    skos:definition "A Gap GeoPhysics proprietary survey technique which requires a geophysical transmitter to transmit a precisely controlled signal into either an inductive transmit loop or a grounded dipole in order to induce secondary fields in sub-surface conductors. "@en ;
    skos:inScheme cs: ;
    skos:prefLabel "Sub-Audio Magnetics"@en ;
    skos:topConceptOf cs: ;
.

obsmh:sp
    a skos:Concept ;
    skos:historyNote "Compiled by the Geological Survey of Queensland" ;
    rdfs:isDefinedBy cs: ;
    skos:altLabel
        "S.P."@en ,
        "SP"@en ,
        "Self Potential"@en ;
    skos:definition "A naturally occurring electric potential difference in the Earth, measured by an electrode relative to a fixed reference electrode."@en ;
    skos:inScheme cs: ;
    skos:prefLabel "Spontaneous Potential "@en ;
    skos:topConceptOf cs: ;
.

obsmh:tem
    a skos:Concept ;
    skos:historyNote "Compiled by the Geological Survey of Queensland" ;
    rdfs:isDefinedBy cs: ;
    skos:altLabel
        "T.D.E.M"@en ,
        "T.E.M."@en ,
        "TDEM"@en ,
        "TEM"@en ,
        "Time-domain electromagnetics"@en ;
    skos:definition "A geophysical exploration technique in which electric and magnetic fields are induced by transient pulses of electric current and the subsequent decay response measured."@en ;
    skos:inScheme cs: ;
    skos:prefLabel "Transient Electromagnetics"@en ;
    skos:topConceptOf cs: ;
.

obsmh:ves
    a skos:Concept ;
    skos:historyNote "Compiled by the Geological Survey of Queensland" ;
    rdfs:isDefinedBy cs: ;
    skos:altLabel
        "V.E.S."@en ,
        "VES"@en ;
    skos:definition "A 1-D geophysical method for investigation of a geological medium. The method is based on the estimation of the electrical conductivity or resistivity of the medium by measurement of electrical field voltage of induced by distant grounded electrodes"@en ;
    skos:inScheme cs: ;
    skos:prefLabel "Vertical Electrical Sounding"@en ;
    skos:topConceptOf cs: ;
.

obsmh:vibroseis
    a skos:Concept ;
    skos:historyNote "Compiled by the Geological Survey of Queensland" ;
    rdfs:isDefinedBy cs: ;
    skos:altLabel "Vibrator"@en ;
    skos:definition "A vehicle-mounted system that holds a large mass to the ground surface which is then oscillated to generate vibrations."@en ;
    skos:inScheme cs: ;
    skos:prefLabel "Vibroseis"@en ;
    skos:topConceptOf cs: ;
.

obsmh:wacker
    a skos:Concept ;
    skos:historyNote "Compiled by the Geological Survey of Queensland" ;
    rdfs:isDefinedBy cs: ;
    skos:altLabel
        "Compactor"@en ,
        "Mini-SOSIE"@en ,
        "Rammer"@en ,
        "SOSIE"@en ,
        "Sozie"@en ,
        "Wacker Packer"@en ,
        "Whacker"@en ;
    skos:definition "A vibration-rammer, similar to a large jackhammer with a flat-plated bottom, repeatedly strikes the ground to generate a series of seismic pulses. Engine speed is used to vary the striking rate, resulting in a random impulse transmission."@en ;
    skos:inScheme cs: ;
    skos:prefLabel "Wacker"@en ;
    skos:topConceptOf cs: ;
.

obsmh:water-gun
    a skos:Concept ;
    skos:historyNote "Compiled by the Geological Survey of Queensland" ;
    rdfs:isDefinedBy cs: ;
    skos:definition "A piston mechanism forces compressed air into the surrounding water and displaces it. The resulting implosion of water to fill the cavity generates a seismic pulse."@en ;
    skos:inScheme cs: ;
    skos:prefLabel "Water Gun"@en ;
    skos:topConceptOf cs: ;
.

<https://linked.data.gov.au/org/gsq>
    a sdo:Organization ;
    sdo:name "Geological Survey of Queensland" ;
    sdo:url "http://www.business.qld.gov.au/industries/mining-energy-water/resources/geoscience-information/gsq"^^xsd:anyURI ;
.

obsmh:weight-drop
    a skos:Concept ;
    skos:historyNote "Compiled by the Geological Survey of Queensland" ;
    rdfs:isDefinedBy cs: ;
    skos:definition "A mass, or striker, is held above the impact point on the ground surface. The mass is then released under the force of gravity with no additional forces applied. The mass strikes the impact point to generate a seismic pulse."@en ;
    skos:inScheme cs: ;
    skos:prefLabel "Weight Drop"@en ;
    skos:topConceptOf cs: ;
.

obsmh:active-spectral
    a skos:Concept ;
    skos:historyNote "Compiled by the Geological Survey of Queensland" ;
    rdfs:isDefinedBy cs: ;
    skos:definition "Spectral methods that use their own source of energy to illuminate the objects they observe. An active sensor emits radiation in the direction of the target to be investigated."@en ;
    skos:inScheme cs: ;
    skos:prefLabel "Active Spectroscopy"@en ;
    skos:topConceptOf cs: ;
.

obsmh:passive-spectral
    a skos:Concept ;
    skos:historyNote "Compiled by the Geological Survey of Queensland" ;
    rdfs:isDefinedBy cs: ;
    skos:definition "Spectral methods that detect natural energy (radiation) that is emitted or reflected by the object or scene being observed. Reflected sunlight is the most common source of radiation measured by passive sensors."@en ;
    skos:inScheme cs: ;
    skos:prefLabel "Passive Spectroscopy"@en ;
    skos:topConceptOf cs: ;
.

cs:
    a
        owl:Ontology ,
        skos:ConceptScheme ;
    dcterms:created "2020-02-10"^^xsd:date ;
    dcterms:creator <https://linked.data.gov.au/org/gsq> ;
    dcterms:modified "2024-02-06"^^xsd:date ;
    skos:historyNote "Compiled by the Geological Survey of Queensland" ;
    dcterms:publisher <https://linked.data.gov.au/org/gsq> ;
    reg:status agldwgstatus:stable ;
    skos:definition "The method of collection used in an observation."@en ;
    skos:hasTopConcept
        obsmh:accelerated-weight-drop ,
        obsmh:active-spectral ,
        obsmh:air-gun ,
        obsmh:amt ,
        obsmh:bbmt ,
        obsmh:boomer ,
        obsmh:cr ,
        obsmh:csem ,
        obsmh:dcr ,
        obsmh:direct ,
        obsmh:dynamite ,
        obsmh:ert ,
        obsmh:firearm ,
        obsmh:flem ,
        obsmh:gpr ,
        obsmh:hammer ,
        obsmh:hydraulic-oil-impactor ,
        obsmh:ip ,
        obsmh:laser-altimetry ,
        obsmh:lidar ,
        obsmh:lpmt ,
        obsmh:mlem ,
        obsmh:noise-source ,
        obsmh:passive-spectral ,
        obsmh:plasma-sound-source ,
        obsmh:radar ,
        obsmh:sam ,
        obsmh:sar ,
        obsmh:sp ,
        obsmh:tem ,
        obsmh:ves ,
        obsmh:vibroseis ,
        obsmh:wacker ,
        obsmh:water-gun ,
        obsmh:weight-drop ;
    skos:prefLabel "Observation Method"@en ;
.

