PREFIX agldwgstatus: <https://linked.data.gov.au/def/reg-statuses/>
PREFIX cs: <http://linked.data.gov.au/def/geological-observation-type>
PREFIX dcterms: <http://purl.org/dc/terms/>
PREFIX obstp: <http://linked.data.gov.au/def/geological-observation-type/>
PREFIX owl: <http://www.w3.org/2002/07/owl#>
PREFIX rdfs: <http://www.w3.org/2000/01/rdf-schema#>
PREFIX reg: <http://purl.org/linked-data/registry#>
PREFIX sdo: <https://schema.org/>
PREFIX skos: <http://www.w3.org/2004/02/skos/core#>
PREFIX xsd: <http://www.w3.org/2001/XMLSchema#>

obstp:borehole-obs
    a skos:Collection ;
    skos:historyNote "Compiled by the Geological Survey of Queensland" ;
    skos:definition "The observation types pertinent to borehole observations."@en ;
    skos:member
        obstp:auger-hole-description ,
        obstp:cement-int ,
        obstp:coal-seam-properties ,
        obstp:coal-type ,
        obstp:depths-of-supergene-alteration ,
        obstp:directional ,
        obstp:drilling-int ,
        obstp:fossils ,
        obstp:lith-int ,
        obstp:mineralogical-components ,
        obstp:miscellaneous-observation ,
        obstp:perf-int ,
        obstp:photographic ,
        obstp:physical ,
        obstp:regolith-observations ,
        obstp:reservoir-int ,
        obstp:rock-classification ,
        obstp:sedimentary-lithofacies ,
        obstp:sedimentary-structures ,
        obstp:strat-int ,
        obstp:tubular-int ,
        obstp:velocity-survey ,
        obstp:weathering-features ,
        obstp:well-completion-int ;
    skos:prefLabel "Borehole Observations"@en ;
.

obstp:sample-obs
    a skos:Collection ;
    skos:historyNote "Compiled by the Geological Survey of Queensland" ;
    skos:definition "The observation types pertinent to samples."@en ;
    skos:member
        obstp:alteration ,
        obstp:coal-seam-properties ,
        obstp:coal-type ,
        obstp:coherance ,
        obstp:fabric ,
        obstp:fossils ,
        obstp:geochemical-signature ,
        obstp:hylogger ,
        obstp:hyperspectral ,
        obstp:igneous-structures ,
        obstp:internal-sequences ,
        obstp:magnetic ,
        obstp:metamorphic-structures ,
        obstp:metamorphic-type ,
        obstp:metamorphism ,
        obstp:mineral-deposit-expression ,
        obstp:mineral-deposit-form ,
        obstp:mineralogical-components ,
        obstp:miscellaneous-observation ,
        obstp:multispectral ,
        obstp:ore-textures ,
        obstp:panchromatic ,
        obstp:photographic ,
        obstp:physical ,
        obstp:quartz-textures ,
        obstp:radiometric ,
        obstp:regolith-observations ,
        obstp:rock-classification ,
        obstp:sedimentary-lithofacies ,
        obstp:sedimentary-structures ,
        obstp:tectonic-structures ,
        obstp:textures ,
        obstp:weathering-features ,
        obstp:younging ;
    skos:prefLabel "Sample Observations"@en ;
.

obstp:seismic-obs
    a skos:Collection ;
    skos:historyNote "Compiled by the Geological Survey of Queensland" ;
    skos:definition "The observation types pertinent to seismic surveys."@en ;
    skos:member
        obstp:seismic-2d ,
        obstp:seismic-3d ,
        obstp:seismic-4d ,
        obstp:seismic-passive ;
    skos:prefLabel "Seismic Observations"@en ;
.

obstp:site-obs
    a skos:Collection ;
    skos:historyNote "Compiled by the Geological Survey of Queensland" ;
    skos:definition "The observation types pertinent to sites."@en ;
    skos:member
        obstp:alteration ,
        obstp:auger-hole-description ,
        obstp:coal-seam-properties ,
        obstp:coal-type ,
        obstp:coherance ,
        obstp:depths-of-supergene-alteration ,
        obstp:electrical ,
        obstp:electromagnetic ,
        obstp:fabric ,
        obstp:fossils ,
        obstp:geochemical-signature ,
        obstp:geothermics ,
        obstp:hyperspectral ,
        obstp:igneous-structures ,
        obstp:internal-sequences ,
        obstp:magnetic ,
        obstp:magnetotelluric ,
        obstp:metamorphic-structures ,
        obstp:metamorphic-type ,
        obstp:metamorphism ,
        obstp:mineral-deposit-expression ,
        obstp:mineral-deposit-form ,
        obstp:mineralogical-components ,
        obstp:miscellaneous-observation ,
        obstp:multispectral ,
        obstp:ore-textures ,
        obstp:panchromatic ,
        obstp:photographic ,
        obstp:physical ,
        obstp:quartz-textures ,
        obstp:regolith-observations ,
        obstp:rock-classification ,
        obstp:sedimentary-lithofacies ,
        obstp:sedimentary-structures ,
        obstp:tectonic-structures ,
        obstp:textures ,
        obstp:velocity-survey ,
        obstp:weathering-features ,
        obstp:younging ;
    skos:prefLabel "Sites Observations"@en ;
.

obstp:survey-obs
    a skos:Collection ;
    skos:historyNote "Compiled by the Geological Survey of Queensland" ;
    skos:definition "The observation types pertinent to surveys."@en ;
    skos:member
        obstp:directional ,
        obstp:electrical ,
        obstp:electromagnetic ,
        obstp:geochemical-signature ,
        obstp:geothermics ,
        obstp:gravity ,
        obstp:gravity-gradiometry ,
        obstp:hylogger ,
        obstp:hyperspectral ,
        obstp:magnetic ,
        obstp:magnetic-gradiometry ,
        obstp:magnetotelluric ,
        obstp:multispectral ,
        obstp:panchromatic ,
        obstp:photographic ,
        obstp:radiometric ,
        obstp:seismic-2d ,
        obstp:seismic-3d ,
        obstp:seismic-4d ,
        obstp:seismic-passive ;
    skos:prefLabel "Survey Observations"@en ;
.

obstp:drill-fluid-int
    a skos:Concept ;
    skos:historyNote "Compiled by the Geological Survey of Queensland" ;
    rdfs:isDefinedBy cs: ;
    skos:definition "The observation of an interval within a wellbore that used a specific drilling fluid."@en ;
    skos:inScheme cs: ;
    skos:notation "DRFD" ;
    skos:prefLabel "Drill Fluid Interval"@en ;
    skos:topConceptOf cs: ;
.

obstp:mineralisation
    a skos:Concept ;
    skos:historyNote "Compiled by the Geological Survey of Queensland" ;
    rdfs:isDefinedBy cs: ;
    skos:altLabel "Mineral Occurrence"@en ;
    skos:definition "The observation of minerals or materials that are of potential economic interest."@en ;
    skos:inScheme cs: ;
    skos:notation "MINOCC" ;
    skos:prefLabel "Mineralisation"@en ;
    skos:topConceptOf cs: ;
.

obstp:positional
    a skos:Concept ;
    skos:historyNote "Compiled by the Geological Survey of Queensland" ;
    rdfs:isDefinedBy cs: ;
    skos:altLabel
        "Distance Ranging"@en ,
        "Rangefinding"@en ,
        "Ranging"@en ,
        "Surveying"@en ,
        "Targeting"@en ;
    skos:definition "An observation of the relative spatial properties of a physical object or location, from a known datum point such as the Euclidean distance from the known position of the observer to another point."@en ;
    skos:inScheme cs: ;
    skos:notation "PSTN" ;
    skos:prefLabel "Positional"@en ;
    skos:topConceptOf cs: ;
.

obstp:quarry-plan
    a skos:Concept ;
    skos:historyNote "Compiled by the Geological Survey of Queensland" ;
    rdfs:isDefinedBy cs: ;
    skos:definition "The cadastral information that describes the position of a property or operation, particularly quarries, as administered by the relveant government authority."@en ;
    skos:inScheme cs: ;
    skos:notation "QRRY" ;
    skos:prefLabel "Quarry Plan"@en ;
    skos:topConceptOf cs: ;
.

obstp:sale
    a skos:Concept ;
    skos:historyNote "Compiled by the Geological Survey of Queensland" ;
    rdfs:isDefinedBy cs: ;
    skos:definition "An observation of the metrics of a geological resource sale, such as the tonnage, grade, value, and shipping information."@en ;
    skos:inScheme cs: ;
    skos:notation "SALES" ;
    skos:prefLabel "Sale"@en ;
    skos:topConceptOf cs: ;
.

obstp:cement-int
    a skos:Concept ;
    skos:historyNote "Compiled by the Geological Survey of Queensland" ;
    rdfs:isDefinedBy cs: ;
    skos:definition "An observation detailing the emplacement of cement in a borehole."@en ;
    skos:inScheme cs: ;
    skos:notation "CMNT" ;
    skos:prefLabel "Cementing Interval"@en ;
    skos:topConceptOf cs: ;
.

obstp:drilling-int
    a skos:Concept ;
    skos:historyNote "Compiled by the Geological Survey of Queensland" ;
    rdfs:isDefinedBy cs: ;
    skos:definition "The observation of a drilled interval by a specific wellbit in a borehole."@en ;
    skos:inScheme cs: ;
    skos:notation "DRLL" ;
    skos:prefLabel "Drilling Interval"@en ;
    skos:topConceptOf cs: ;
.

obstp:gravity
    a skos:Concept ;
    skos:historyNote "Compiled by the Geological Survey of Queensland" ;
    rdfs:isDefinedBy cs: ;
    skos:definition "A survey where the variation of the Earth's gravity field in measured to determine the distribution of density in the region."@en ;
    skos:inScheme cs: ;
    skos:notation "GV" ;
    skos:prefLabel "Gravity"@en ;
    skos:topConceptOf cs: ;
.

obstp:gravity-gradiometry
    a skos:Concept ;
    skos:historyNote "Compiled by the Geological Survey of Queensland" ;
    rdfs:isDefinedBy cs: ;
    skos:altLabel "Full tensor gravimetry"@en ;
    skos:definition "A variation of gravity observations where the gradient of the gravity field is measured instead of the field directly."@en ;
    skos:inScheme cs: ;
    skos:notation "GG" ;
    skos:prefLabel "Gravity Gradiometry"@en ;
    skos:topConceptOf cs: ;
.

obstp:hylogger
    a skos:Concept ;
    skos:historyNote "Compiled by the Geological Survey of Queensland" ;
    rdfs:isDefinedBy cs: ;
    skos:broader obstp:hyperspectral ;
    skos:definition "HyLogger is a high resolution hyperspectral core scanner which can interpret mineralogy of up to four dominant minerals, as well as 2D and 3D profiling of alteration signatures from depth to surface."@en ;
    skos:inScheme cs: ;
    skos:notation "HYLG" ;
    skos:prefLabel "HyLogger"@en ;
.

obstp:lith-int
    a skos:Concept ;
    skos:historyNote "Compiled by the Geological Survey of Queensland" ;
    rdfs:isDefinedBy cs: ;
    skos:altLabel "Lithology Interval"@en ;
    skos:definition "An observation detailing the lithological characteristics of a defined interval."@en ;
    skos:inScheme cs: ;
    skos:notation "LITH" ;
    skos:prefLabel "Lithological Interval"@en ;
    skos:topConceptOf cs: ;
.

obstp:magnetic-gradiometry
    a skos:Concept ;
    skos:historyNote "Compiled by the Geological Survey of Queensland" ;
    rdfs:isDefinedBy cs: ;
    skos:definition "A variation of magnetic observations where the gradient of the magnetic field is measured instead of the field directly."@en ;
    skos:inScheme cs: ;
    skos:notation "MY" ;
    skos:prefLabel "Magnetic Gradiometry"@en ;
    skos:topConceptOf cs: ;
.

obstp:perf-int
    a skos:Concept ;
    skos:historyNote "Compiled by the Geological Survey of Queensland" ;
    rdfs:isDefinedBy cs: ;
    skos:definition "An observation detailing the perforations through casing of a defined interval in a borehole."@en ;
    skos:inScheme cs: ;
    skos:notation "PERF" ;
    skos:prefLabel "Perforations"@en ;
    skos:topConceptOf cs: ;
.

obstp:reservoir-int
    a skos:Concept ;
    skos:historyNote "Compiled by the Geological Survey of Queensland" ;
    rdfs:isDefinedBy cs: ;
    skos:altLabel
        "Reservoir Interval"@en ,
        "Reservoir Properties"@en ;
    skos:definition "Observations of reservoir properties within a specific interval within a borehole."@en ;
    skos:inScheme cs: ;
    skos:notation "RSVR" ;
    skos:prefLabel "Reservoirs"@en ;
    skos:topConceptOf cs: ;
.

obstp:strat-int
    a skos:Concept ;
    skos:historyNote "Compiled by the Geological Survey of Queensland" ;
    rdfs:isDefinedBy cs: ;
    skos:altLabel "Stratigraphic Interval"@en ;
    skos:definition "Observations of the formal rock units formations and their depth intervals intersected within a borehole."@en ;
    skos:inScheme cs: ;
    skos:notation "STRT" ;
    skos:prefLabel "Stratigraphy"@en ;
    skos:topConceptOf cs: ;
.

obstp:tubular-int
    a skos:Concept ;
    skos:historyNote "Compiled by the Geological Survey of Queensland" ;
    rdfs:isDefinedBy cs: ;
    skos:altLabel
        "Casing Interval"@en ,
        "Liner"@en ,
        "Tubing"@en ,
        "Tubular"@en ,
        "Tubular Interval"@en ;
    skos:definition "The observations of tubular equipment (casing, tubing, liner) installed in a borehole."@en ;
    skos:inScheme cs: ;
    skos:notation "TBLR" ;
    skos:prefLabel "Casing"@en ;
    skos:topConceptOf cs: ;
.

obstp:well-completion-int
    a skos:Concept ;
    skos:historyNote "Compiled by the Geological Survey of Queensland" ;
    rdfs:isDefinedBy cs: ;
    skos:altLabel
        "Completion"@en ,
        "Completion Interval"@en ,
        "Well Completion Interval"@en ;
    skos:definition "The observations of the interval over which a well is completed. The contact interval or intervals with the reservoir(s) that function as a single unit to produce or inject fluids."@en ;
    skos:inScheme cs: ;
    skos:notation "WCPI" ;
    skos:prefLabel "Well Completion"@en ;
    skos:topConceptOf cs: ;
.

<https://linked.data.gov.au/org/gsq>
    a sdo:Organization ;
    sdo:name "Geological Survey of Queensland" ;
    sdo:url "http://www.business.qld.gov.au/industries/mining-energy-water/resources/geoscience-information/gsq"^^xsd:anyURI ;
.

obstp:alteration
    a skos:Concept ;
    skos:historyNote "Compiled by the Geological Survey of Queensland" ;
    rdfs:isDefinedBy cs: ;
    skos:definition "A change in the mineralogic composition of a rock brought about by physical or chemical means, esp. by the action of hydrothermal solutions; also, a secondary, i.e., supergene, change in a rock or mineral. Alteration excludes that specifically resulting from metamorphic alteration, which is characterised in a unique observation type, Metamorphism."@en ;
    skos:inScheme cs: ;
    skos:notation "ALTN" ;
    skos:prefLabel "Alteration"@en ;
    skos:topConceptOf cs: ;
.

obstp:auger-hole-description
    a skos:Concept ;
    skos:historyNote "Compiled by the Geological Survey of Queensland" ;
    rdfs:isDefinedBy cs: ;
    skos:definition "A description of an auger hole."@en ;
    skos:inScheme cs: ;
    skos:notation "AUGR" ;
    skos:prefLabel "Auger Hole Description"@en ;
    skos:topConceptOf cs: ;
.

obstp:coherance
    a skos:Concept ;
    skos:historyNote "Compiled by the Geological Survey of Queensland" ;
    rdfs:isDefinedBy cs: ;
    skos:definition "How well a rock is lithified."@en ;
    skos:inScheme cs: ;
    skos:notation "COHR" ;
    skos:prefLabel "Coherance"@en ;
    skos:topConceptOf cs: ;
.

obstp:depths-of-supergene-alteration
    a skos:Concept ;
    skos:historyNote "Compiled by the Geological Survey of Queensland" ;
    rdfs:isDefinedBy cs: ;
    skos:definition "The depths at which supergene alteration occurred."@en ;
    skos:inScheme cs: ;
    skos:notation "DSUP" ;
    skos:prefLabel "Depths of Supergene Alteration"@en ;
    skos:topConceptOf cs: ;
.

obstp:directional
    a skos:Concept ;
    skos:historyNote "Compiled by the Geological Survey of Queensland" ;
    rdfs:isDefinedBy cs: ;
    skos:altLabel "Deviation"@en ;
    skos:definition "The process of recording the subsurface geometry of a borehole i.e. direction and position of a wellbore."@en ;
    skos:inScheme cs: ;
    skos:notation "DRCT" ;
    skos:prefLabel "Directional"@en ;
    skos:topConceptOf cs: ;
.

obstp:electrical
    a skos:Concept ;
    skos:historyNote "Compiled by the Geological Survey of Queensland" ;
    rdfs:isDefinedBy cs: ;
    skos:altLabel "Electric"@en ;
    skos:definition "The observations of measuring electrical currents as they travel through conductive pathways in the near surface."@en ;
    skos:inScheme cs: ;
    skos:notation "EL" ;
    skos:prefLabel "Electrical"@en ;
    skos:topConceptOf cs: ;
.

obstp:electromagnetic
    a skos:Concept ;
    skos:historyNote "Compiled by the Geological Survey of Queensland" ;
    rdfs:isDefinedBy cs: ;
    skos:altLabel
        "EM"@en ,
        "EM Survey"@en ;
    skos:definition "A survey measuring induced electromagnetic fields from the earth to determine the resistive/conductive structure of the earth."@en ;
    skos:inScheme cs: ;
    skos:notation "EM" ;
    skos:prefLabel "Electromagnetic"@en ;
    skos:topConceptOf cs: ;
.

obstp:fabric
    a skos:Concept ;
    skos:historyNote "Compiled by the Geological Survey of Queensland" ;
    rdfs:isDefinedBy cs: ;
    skos:definition "The spatial and geometric configuration of a sample."@en ;
    skos:inScheme cs: ;
    skos:notation "FABR" ;
    skos:prefLabel "Fabric"@en ;
    skos:topConceptOf cs: ;
.

obstp:geothermics
    a skos:Concept ;
    skos:historyNote "Compiled by the Geological Survey of Queensland" ;
    rdfs:isDefinedBy cs: ;
    skos:definition "An observation measuring variations of heat flow within the Earth."@en ;
    skos:inScheme cs: ;
    skos:notation "GE" ;
    skos:prefLabel "Geothermics"@en ;
    skos:topConceptOf cs: ;
.

obstp:igneous-structures
    a skos:Concept ;
    skos:historyNote "Compiled by the Geological Survey of Queensland" ;
    rdfs:isDefinedBy cs: ;
    skos:definition "The types of igneous structures observed."@en ;
    skos:inScheme cs: ;
    skos:notation "IGST" ;
    skos:prefLabel "Igneous Structures"@en ;
    skos:topConceptOf cs: ;
.

obstp:internal-sequences
    a skos:Concept ;
    skos:historyNote "Compiled by the Geological Survey of Queensland" ;
    rdfs:isDefinedBy cs: ;
    skos:definition "The sequences observable inside a sample."@en ;
    skos:inScheme cs: ;
    skos:notation "SEQU" ;
    skos:prefLabel "Internal Sequences"@en ;
    skos:topConceptOf cs: ;
.

obstp:magnetotelluric
    a skos:Concept ;
    skos:historyNote "Compiled by the Geological Survey of Queensland" ;
    rdfs:isDefinedBy cs: ;
    skos:altLabel
        "MT"@en ,
        "MT Survey"@en ;
    skos:definition "A survey where recordings of the Earths electric and magnetic fields are taken concurrently to determine the subsurface electrical resistivity at a range of scales."@en ;
    skos:inScheme cs: ;
    skos:notation "MT" ;
    skos:prefLabel "Magnetotelluric"@en ;
    skos:topConceptOf cs: ;
.

obstp:metamorphic-structures
    a skos:Concept ;
    skos:historyNote "Compiled by the Geological Survey of Queensland" ;
    rdfs:isDefinedBy cs: ;
    skos:definition "The metamorphic structures observed."@en ;
    skos:inScheme cs: ;
    skos:notation "METS" ;
    skos:prefLabel "Metamorphic Structures"@en ;
    skos:topConceptOf cs: ;
.

obstp:metamorphic-type
    a skos:Concept ;
    skos:historyNote "Compiled by the Geological Survey of Queensland" ;
    rdfs:isDefinedBy cs: ;
    skos:definition "The type of metamorphism observed."@en ;
    skos:inScheme cs: ;
    skos:notation "METTYP" ;
    skos:prefLabel "Metamorphic Type"@en ;
    skos:topConceptOf cs: ;
.

obstp:metamorphism
    a skos:Concept ;
    skos:historyNote "Compiled by the Geological Survey of Queensland" ;
    rdfs:isDefinedBy cs: ;
    skos:altLabel "Metamorphic Alteration"@en ;
    skos:definition "Mineralogical alterations specifically related to metamorphism."@en ;
    skos:inScheme cs: ;
    skos:notation "META" ;
    skos:prefLabel "Metamorphism"@en ;
    skos:topConceptOf cs: ;
.

obstp:mineral-deposit-expression
    a skos:Concept ;
    skos:historyNote "Compiled by the Geological Survey of Queensland" ;
    rdfs:isDefinedBy cs: ;
    skos:definition "The type expressed by a mineral deposit"@en ;
    skos:inScheme cs: ;
    skos:notation "DEXP" ;
    skos:prefLabel "Mineral Deposit Expression"@en ;
    skos:topConceptOf cs: ;
.

obstp:mineral-deposit-form
    a skos:Concept ;
    skos:historyNote "Compiled by the Geological Survey of Queensland" ;
    rdfs:isDefinedBy cs: ;
    skos:definition "The form expressed by a mineral deposit"@en ;
    skos:inScheme cs: ;
    skos:notation "DFRM" ;
    skos:prefLabel "Mineral Deposit Form"@en ;
    skos:topConceptOf cs: ;
.

obstp:ore-textures
    a skos:Concept ;
    skos:historyNote "Compiled by the Geological Survey of Queensland" ;
    rdfs:isDefinedBy cs: ;
    skos:definition "The textures apparently in an ore."@en ;
    skos:inScheme cs: ;
    skos:notation "OTEX" ;
    skos:prefLabel "Ore Textures"@en ;
    skos:topConceptOf cs: ;
.

obstp:quartz-textures
    a skos:Concept ;
    skos:historyNote "Compiled by the Geological Survey of Queensland" ;
    rdfs:isDefinedBy cs: ;
    skos:definition "The textures visible in quartz."@en ;
    skos:inScheme cs: ;
    skos:notation "QTEX" ;
    skos:prefLabel "Quartz Textures"@en ;
    skos:topConceptOf cs: ;
.

obstp:radiometric
    a skos:Concept ;
    skos:historyNote "Compiled by the Geological Survey of Queensland" ;
    rdfs:isDefinedBy cs: ;
    skos:altLabel
        "Gamma Logs"@en ,
        "Gamma-Ray Spectrography"@en ;
    skos:definition "A survey where the emissions of natural gamma-rays are recorded to determine the quantity of radioelements (Potassium, Uranium, Thorium)."@en ;
    skos:inScheme cs: ;
    skos:notation "RM" ;
    skos:prefLabel "Radiometric"@en ;
    skos:topConceptOf cs: ;
.

obstp:seismic-2d
    a skos:Concept ;
    skos:historyNote "Compiled by the Geological Survey of Queensland" ;
    rdfs:isDefinedBy cs: ;
    skos:altLabel
        "2D"@en ,
        "2D Seismic Survey"@en ,
        "2D Survey"@en ,
        "Seismic 2D"@en ;
    skos:definition "The Fundamental Dataset of a 2D seismic survey is the 'Line'; the Line dataset is a 2D cross-section of the subsurface measured by a chain of geophones. It is described by a function of two parameters : 1) Trace Number and 2) Two-Way Time. A 2D seismic survey may be composed of one or many lines that may or may not intersect with each other."@en ;
    skos:inScheme cs: ;
    skos:notation "2d" ;
    skos:prefLabel "2D Seismic"@en ;
    skos:topConceptOf cs: ;
.

obstp:seismic-3d
    a skos:Concept ;
    skos:historyNote "Compiled by the Geological Survey of Queensland" ;
    rdfs:isDefinedBy cs: ;
    skos:altLabel
        "3D"@en ,
        "3D Seismic Survey"@en ,
        "3D Survey"@en ,
        "Seismic 3D"@en ;
    skos:definition "The Fundamental Dataset of a 3D seismic survey is the 'Volume'; the Volume dataset is a 3D model of the subsurface measured by a grid/array of geophones. It is described by a function of three parameters : 1) In-Line, 2) Cross-Line and 3) Two-Way Time. A 3D seismic survey contains many In-Lines and Cross-Lines that intersect with each other."@en ;
    skos:inScheme cs: ;
    skos:notation "3d" ;
    skos:prefLabel "3D Seismic"@en ;
    skos:topConceptOf cs: ;
.

obstp:seismic-4d
    a skos:Concept ;
    skos:historyNote "Compiled by the Geological Survey of Queensland" ;
    rdfs:isDefinedBy cs: ;
    skos:altLabel
        "3D Time Lapse Survey"@en ,
        "3D Time-Lapse Survey"@en ,
        "4D"@en ,
        "4D Seismic Survey"@en ,
        "4D Survey"@en ,
        "Seismic 4D"@en ,
        "Time Lapse"@en ,
        "Time Lapse Survey"@en ,
        "Time-Lapse"@en ,
        "Time-Lapse Survey"@en ;
    skos:definition "The Fundamental Dataset of a 4D seismic survey is the 'Temporal Volume'; The Temporal Volume is a collection of multiple discrete recordings of a volume of the subsurface measured at successive time intervals. It is described by a function of four parameters: 1) In-Line, 2) Cross-Line, 3) Two-Way Time and 4) Repeat Index. The In-Lines and Cross-Lines intersect with each other."@en ;
    skos:inScheme cs: ;
    skos:notation "4d" ;
    skos:prefLabel "4D Seismic"@en ;
    skos:topConceptOf cs: ;

obstp:seismic-passive
    a skos:Concept ;
    skos:historyNote "Compiled by the Geological Survey of Queensland" ;
    rdfs:isDefinedBy cs: ;
    skos:altLabel
        "Passive Seismic Survey"@en ,
         "Ambient Noise Tomography"@en ;
    skos:definition "Passive seismic is the detection of natural, usually low frequency earth movements, with the purpose of discerning geological structure or resources"@en ;
    skos:inScheme cs: ;
    skos:notation "PS" ;
    skos:prefLabel "Passive Seismic"@en ;
    skos:topConceptOf cs: ;

obstp:tectonic-structures
    a skos:Concept ;
    skos:historyNote "Compiled by the Geological Survey of Queensland" ;
    rdfs:isDefinedBy cs: ;
    skos:definition "The observable tectonic structures."@en ;
    skos:inScheme cs: ;
    skos:notation "TCST" ;
    skos:prefLabel "Tectonic Structures"@en ;
    skos:topConceptOf cs: ;
.

obstp:textures
    a skos:Concept ;
    skos:historyNote "Compiled by the Geological Survey of Queensland" ;
    rdfs:isDefinedBy cs: ;
    skos:definition "The textures observable of a sample."@en ;
    skos:inScheme cs: ;
    skos:notation "TEXT" ;
    skos:prefLabel "Textures"@en ;
    skos:topConceptOf cs: ;
.

obstp:velocity-survey
    a skos:Concept ;
    skos:historyNote "Compiled by the Geological Survey of Queensland" ;
    rdfs:isDefinedBy cs: ;
    skos:altLabel "Seismic Velocity"@en ;
    skos:definition "Observations that generate measurements used to determine average velocity versus depth in a borehole."@en ;
    skos:inScheme cs: ;
    skos:notation "VELS" ;
    skos:prefLabel "Velocity Survey"@en ;
    skos:topConceptOf cs: ;
.

obstp:younging
    a skos:Concept ;
    skos:historyNote "Compiled by the Geological Survey of Queensland" ;
    rdfs:isDefinedBy cs: ;
    skos:definition "The younging direction observed in a sequence."@en ;
    skos:inScheme cs: ;
    skos:notation "YOUNG" ;
    skos:prefLabel "Younging"@en ;
    skos:topConceptOf cs: ;
.

obstp:coal-seam-properties
    a skos:Concept ;
    skos:historyNote "Compiled by the Geological Survey of Queensland" ;
    rdfs:isDefinedBy cs: ;
    skos:definition "An observation of the properties of a coal seam using a variety of analytical techniques."@en ;
    skos:inScheme cs: ;
    skos:notation "CSPR" ;
    skos:prefLabel "Coal Seam Properties"@en ;
    skos:topConceptOf cs: ;
.

obstp:coal-type
    a skos:Concept ;
    skos:historyNote "Compiled by the Geological Survey of Queensland" ;
    rdfs:isDefinedBy cs: ;
    skos:definition "A definition of the type of coal according to a classification scheme."@en ;
    skos:inScheme cs: ;
    skos:notation "COAL" ;
    skos:prefLabel "Coal Type"@en ;
    skos:topConceptOf cs: ;
.

obstp:fossils
    a skos:Concept ;
    skos:historyNote "Compiled by the Geological Survey of Queensland" ;
    rdfs:isDefinedBy cs: ;
    skos:definition "Fossils observed."@en ;
    skos:inScheme cs: ;
    skos:notation "FOSS" ;
    skos:prefLabel "Fossils"@en ;
    skos:topConceptOf cs: ;
.

obstp:geochemical-signature
    a skos:Concept ;
    skos:historyNote "Compiled by the Geological Survey of Queensland" ;
    rdfs:isDefinedBy cs: ;
    skos:definition "The geochemical signature observed."@en ;
    skos:inScheme cs: ;
    skos:notation "GEOC" ;
    skos:prefLabel "Geochemical signature"@en ;
    skos:topConceptOf cs: ;
.

obstp:magnetic
    a skos:Concept ;
    skos:historyNote "Compiled by the Geological Survey of Queensland" ;
    rdfs:isDefinedBy cs: ;
    skos:altLabel "magnetism"@en ;
    skos:definition "The intensity of magnetism observed."@en ;
    skos:inScheme cs: ;
    skos:notation "MG" ;
    skos:prefLabel "Magnetic"@en ;
    skos:topConceptOf cs: ;
.

obstp:mineralogical-components
    a skos:Concept ;
    skos:historyNote "Compiled by the Geological Survey of Queensland" ;
    rdfs:isDefinedBy cs: ;
    skos:definition "The mineralogical components of a sample."@en ;
    skos:inScheme cs: ;
    skos:notation "COMPON" ;
    skos:prefLabel "Components"@en ;
    skos:topConceptOf cs: ;
.

obstp:miscellaneous-observation
    a skos:Concept ;
    skos:historyNote "Compiled by the Geological Survey of Queensland" ;
    rdfs:isDefinedBy cs: ;
    skos:definition "A trivial type of observation, not elsewhere classified."@en ;
    skos:inScheme cs: ;
    skos:notation "MISC" ;
    skos:prefLabel "Miscellaneous Observation"@en ;
    skos:topConceptOf cs: ;
.

obstp:multispectral
    a skos:Concept ;
    skos:historyNote "Compiled by the Geological Survey of Queensland" ;
    rdfs:isDefinedBy cs: ;
    skos:definition "A spectral observation type that captures between 3 and 10 frequency bands."@en ;
    skos:inScheme cs: ;
    skos:notation "MULT" ;
    skos:prefLabel "Multispectral"@en ;
    skos:topConceptOf cs: ;
.

obstp:panchromatic
    a skos:Concept ;
    skos:historyNote "Compiled by the Geological Survey of Queensland" ;
    rdfs:isDefinedBy cs: ;
    skos:altLabel "Monochromatic"@en ;
    skos:definition "A spectral observation type that captures light across a wide bandwidth, typically spanning hundreds of nanometers, as a single band."@en ;
    skos:inScheme cs: ;
    skos:notation "PANC" ;
    skos:prefLabel "Panchromatic"@en ;
    skos:topConceptOf cs: ;
.

obstp:physical
    a skos:Concept ;
    skos:historyNote "Compiled by the Geological Survey of Queensland" ;
    rdfs:isDefinedBy cs: ;
    skos:definition "An observation of the fundamental physical properties of an entity such as shape, size, colour, mass, porosity, permeability, strength, stiffness, composition."@en ;
    skos:inScheme cs: ;
    skos:notation "PHYS" ;
    skos:prefLabel "Physical Properties"@en ;
    skos:topConceptOf cs: ;
.

obstp:regolith-observations
    a skos:Concept ;
    skos:historyNote "Compiled by the Geological Survey of Queensland" ;
    rdfs:isDefinedBy cs: ;
    skos:definition "Observations of regolith."@en ;
    skos:inScheme cs: ;
    skos:notation "REGO" ;
    skos:prefLabel "Regolith Observations"@en ;
    skos:topConceptOf cs: ;
.

obstp:rock-classification
    a skos:Concept ;
    skos:historyNote "Compiled by the Geological Survey of Queensland" ;
    rdfs:isDefinedBy cs: ;
    skos:definition "The classification of a rock."@en ;
    skos:inScheme cs: ;
    skos:notation "RCLASS" ;
    skos:prefLabel "Rock Classification"@en ;
    skos:topConceptOf cs: ;
.

obstp:sedimentary-lithofacies
    a skos:Concept ;
    skos:historyNote "Compiled by the Geological Survey of Queensland" ;
    rdfs:isDefinedBy cs: ;
    skos:definition "The lithofacies observable in a sedimentary sequence."@en ;
    skos:inScheme cs: ;
    skos:notation "SEDFAC" ;
    skos:prefLabel "Sedimentary Lithofacies"@en ;
    skos:topConceptOf cs: ;
.

obstp:sedimentary-structures
    a skos:Concept ;
    skos:historyNote "Compiled by the Geological Survey of Queensland" ;
    rdfs:isDefinedBy cs: ;
    skos:definition "The structures observable in a sedimentary sequence."@en ;
    skos:inScheme cs: ;
    skos:notation "SEDS" ;
    skos:prefLabel "Sedimentary Structures"@en ;
    skos:topConceptOf cs: ;
.

obstp:weathering-features
    a skos:Concept ;
    skos:historyNote "Compiled by the Geological Survey of Queensland" ;
    rdfs:isDefinedBy cs: ;
    skos:definition "The weathering features observable in a sample."@en ;
    skos:inScheme cs: ;
    skos:notation "WETH" ;
    skos:prefLabel "Weathering Features"@en ;
    skos:topConceptOf cs: ;
.

obstp:hyperspectral
    a skos:Concept ;
    skos:historyNote "Compiled by the Geological Survey of Queensland" ;
    rdfs:isDefinedBy cs: ;
    skos:definition "A spectral observation type that captures between greater than 10 frequency bands. Hyperspectal observations typically consist of hundred of narrow bands (10-20nm)."@en ;
    skos:inScheme cs: ;
    skos:notation "HYPR" ;
    skos:prefLabel "Hyperspectral"@en ;
    skos:topConceptOf cs: ;
.

obstp:photographic
    a skos:Concept ;
    skos:historyNote "Compiled by the Geological Survey of Queensland" ;
    rdfs:isDefinedBy cs: ;
    skos:altLabel "Photographic details"@en ;
    skos:definition "The details observable via photogrammetry using standard photographic equipment for image capture without intention for spectral analysis. Including land-based geological photography."@en ;
    skos:inScheme cs: ;
    skos:notation "PHOT" ;
    skos:prefLabel "Photographic"@en ;
    skos:topConceptOf cs: ;
.

cs:
    a
        owl:Ontology ,
        skos:ConceptScheme ;
    dcterms:created "2020-02-07"^^xsd:date ;
    dcterms:creator <https://linked.data.gov.au/org/gsq> ;
    dcterms:modified "2023-03-16"^^xsd:date ;
    skos:historyNote "Compiled by the Geological Survey of Queensland" ;
    dcterms:publisher <https://linked.data.gov.au/org/gsq> ;
    reg:status agldwgstatus:stable ;
    skos:definition "The types of observation in geoscience."@en ;
    skos:hasTopConcept
        obstp:alteration ,
        obstp:auger-hole-description ,
        obstp:cement-int ,
        obstp:coal-seam-properties ,
        obstp:coal-type ,
        obstp:coherance ,
        obstp:depths-of-supergene-alteration ,
        obstp:directional ,
        obstp:drill-fluid-int ,
        obstp:drilling-int ,
        obstp:electrical ,
        obstp:electromagnetic ,
        obstp:fabric ,
        obstp:fossils ,
        obstp:geochemical-signature ,
        obstp:geothermics ,
        obstp:gravity ,
        obstp:gravity-gradiometry ,
        obstp:hyperspectral ,
        obstp:igneous-structures ,
        obstp:internal-sequences ,
        obstp:lith-int ,
        obstp:magnetic ,
        obstp:magnetic-gradiometry ,
        obstp:magnetotelluric ,
        obstp:metamorphic-structures ,
        obstp:metamorphic-type ,
        obstp:metamorphism ,
        obstp:mineral-deposit-expression ,
        obstp:mineral-deposit-form ,
        obstp:mineralisation ,
        obstp:mineralogical-components ,
        obstp:miscellaneous-observation ,
        obstp:multispectral ,
        obstp:ore-textures ,
        obstp:panchromatic ,
        obstp:perf-int ,
        obstp:photographic ,
        obstp:physical ,
        obstp:positional ,
        obstp:quarry-plan ,
        obstp:quartz-textures ,
        obstp:radiometric ,
        obstp:regolith-observations ,
        obstp:reservoir-int ,
        obstp:rock-classification ,
        obstp:sale ,
        obstp:sedimentary-lithofacies ,
        obstp:sedimentary-structures ,
        obstp:seismic-2d ,
        obstp:seismic-3d ,
        obstp:seismic-4d ,
        obstp:seismic-passive ,
        obstp:strat-int ,
        obstp:tectonic-structures ,
        obstp:textures ,
        obstp:tubular-int ,
        obstp:velocity-survey ,
        obstp:weathering-features ,
        obstp:well-completion-int ,
        obstp:younging ;
    skos:prefLabel "Observation Type"@en ;
.

