PREFIX agldwgstatus: <https://linked.data.gov.au/def/reg-statuses/>
PREFIX cs: <http://linked.data.gov.au/def/resource-stockpile-purpose>
PREFIX dcterms: <http://purl.org/dc/terms/>
PREFIX owl: <http://www.w3.org/2002/07/owl#>
PREFIX rdfs: <http://www.w3.org/2000/01/rdf-schema#>
PREFIX reg: <http://purl.org/linked-data/registry#>
PREFIX rsp: <http://linked.data.gov.au/def/resource-stockpile-purpose/>
PREFIX sdo: <https://schema.org/>
PREFIX skos: <http://www.w3.org/2004/02/skos/core#>
PREFIX xsd: <http://www.w3.org/2001/XMLSchema#>

rsp:min-raw-stockpile
    a skos:Collection ;
    dcterms:provenance "Compiled by the Geological Survey of Queensland" ;
    skos:definition "The reason for the stockpiling of raw materials in a mineral mining operation."@en ;
    skos:member
        rsp:economics ,
        rsp:met-characteristics ,
        rsp:other ,
        rsp:processing-capacity ;
    skos:prefLabel "Mineral Mine Raw Material Stockpile"@en ;
.

rsp:transport-capacity
    a skos:Concept ;
    dcterms:provenance "Compiled by the Geological Survey of Queensland" ;
    rdfs:isDefinedBy cs: ;
    skos:broader rsp:capacity ;
    skos:definition "A stockpile kept due to capacity constraints in the ability to transport material to a processing or sales site."@en ;
    skos:inScheme cs: ;
    skos:prefLabel "Transport Capacity"@en ;
.

rsp:met-characteristics
    a skos:Concept ;
    dcterms:provenance "Compiled by the Geological Survey of Queensland" ;
    rdfs:isDefinedBy cs: ;
    skos:broader rsp:material-characteristics ;
    skos:definition "A stockpile kept due to the metallurgic charactieristics of a metallic ore not being suitable for the configuration or capability of the processing plant."@en ;
    skos:inScheme cs: ;
    skos:prefLabel "Metallurgical Characteristics"@en ;
.

rsp:processing-capacity
    a skos:Concept ;
    dcterms:provenance "Compiled by the Geological Survey of Queensland" ;
    rdfs:isDefinedBy cs: ;
    skos:broader rsp:capacity ;
    skos:definition "A stockpile kept due to capacity constraints to process raw material, such as where the raw output from a mine exceeds the throughput capacity of the associated processing plant."@en ;
    skos:inScheme cs: ;
    skos:prefLabel "Processing Capacity"@en ;
.

rsp:economics
    a skos:Concept ;
    dcterms:provenance "Compiled by the Geological Survey of Queensland" ;
    rdfs:isDefinedBy cs: ;
    skos:definition "A stockpile kept due to economic considerations such as a commodity price or cost of processing that makes a raw material sub-economic to process and prepare for sale."@en ;
    skos:inScheme cs: ;
    skos:prefLabel "Economics"@en ;
.

rsp:material-characteristics
    a skos:Concept ;
    dcterms:provenance "Compiled by the Geological Survey of Queensland" ;
    rdfs:isDefinedBy cs: ;
    skos:definition "A stockpile kept due to the physical or chemical properties of a raw material not being suitable for the specification of the available or allocated processing plant."@en ;
    skos:inScheme cs: ;
    skos:prefLabel "Material Characteristics"@en ;
.

rsp:other
    a skos:Concept ;
    dcterms:provenance "Compiled by the Geological Survey of Queensland" ;
    rdfs:isDefinedBy cs: ;
    skos:definition "A stockpile kept due to a reason other than those otherwise listed."@en ;
    skos:inScheme cs: ;
    skos:prefLabel "Other"@en ;
.

<https://linked.data.gov.au/org/gsq>
    a sdo:Organization ;
    sdo:name "Geological Survey of Queensland" ;
    sdo:url "http://www.business.qld.gov.au/industries/mining-energy-water/resources/geoscience-information/gsq"^^xsd:anyURI ;
.

rsp:capacity
    a skos:Concept ;
    dcterms:provenance "Compiled by the Geological Survey of Queensland" ;
    rdfs:isDefinedBy cs: ;
    skos:definition "A stockpile kept due to capacity constraints in the lifecycle of a georesource material from raw material to saleable product."@en ;
    skos:inScheme cs: ;
    skos:prefLabel "Capacity"@en ;
.

cs:
    a
        owl:Ontology ,
        skos:ConceptScheme ;
    dcterms:created "2020-05-12"^^xsd:date ;
    dcterms:creator <https://linked.data.gov.au/org/gsq> ;
    dcterms:modified "2023-03-16"^^xsd:date ;
    dcterms:provenance "Compiled by the Geological Survey of Queensland" ;
    dcterms:publisher <https://linked.data.gov.au/org/gsq> ;
    reg:status agldwgstatus:stable ;
    skos:definition "The purpose or reason for holding a stockpile of a georesource raw material or product."@en ;
    skos:hasTopConcept
        rsp:capacity ,
        rsp:economics ,
        rsp:material-characteristics ,
        rsp:other ;
    skos:prefLabel "Georesource Stockpile Purpose"@en ;
.

