PREFIX agldwgstatus: <https://linked.data.gov.au/def/reg-statuses/>
PREFIX cs: <http://www.w3.org/ns/time/gregorian>
PREFIX dcterms: <http://purl.org/dc/terms/>
PREFIX greg: <http://www.w3.org/ns/time/gregorian/>
PREFIX owl: <http://www.w3.org/2002/07/owl#>
PREFIX prov: <http://www.w3.org/ns/prov#>
PREFIX rdfs: <http://www.w3.org/2000/01/rdf-schema#>
PREFIX reg: <http://purl.org/linked-data/registry#>
PREFIX sdo: <https://schema.org/>
PREFIX skos: <http://www.w3.org/2004/02/skos/core#>
PREFIX time: <http://www.w3.org/2006/time#>
PREFIX xsd: <http://www.w3.org/2001/XMLSchema#>

<http://www.w3.org>
    a sdo:Organization ;
    sdo:name "World Wide Web Consortium" ;
    sdo:url "http://www.w3.org"^^xsd:anyURI ;
.

greg:April
    a
        skos:Concept ,
        time:MonthOfYear ;
    rdfs:isDefinedBy cs: ;
    rdfs:seeAlso <http://en.wikipedia.org/wiki/April> ;
    skos:altLabel "APRIL"@en ;
    skos:definition "April is the fourth month of the year in the Gregorian calendar, the fifth in the early Julian, the first of four months to have a length of 30 days, and the second of five months to have a length of less than 31 days."@en ;
    skos:inScheme cs: ;
    skos:notation "APR" ;
    skos:prefLabel
        "أبريل"@ar ,
        "April"@de ,
        "April"@en ,
        "Abril"@es ,
        "Avril"@fr ,
        "Aprile"@it ,
        "4月"@ja ,
        "April"@nl ,
        "Kwiecień"@pl ,
        "Abril"@pt ,
        "Апрель"@ru ,
        "4月"@zh ;
    time:month "--04"^^xsd:gMonth ;
    time:unitType time:unitMonth ;
    prov:wasDerivedFrom cs: ;
.

greg:August
    a
        skos:Concept ,
        time:MonthOfYear ;
    rdfs:isDefinedBy cs: ;
    rdfs:seeAlso <http://en.wikipedia.org/wiki/August> ;
    skos:altLabel "AUGUST"@en ;
    skos:definition "August is the eighth month of the year in the Julian and Gregorian calendars, and the fifth of seven months to have a length of 31 days."@en ;
    skos:inScheme cs: ;
    skos:notation "AUG" ;
    skos:prefLabel
        "أغسطس"@ar ,
        "August"@de ,
        "August"@en ,
        "Agosto"@es ,
        "Août"@fr ,
        "Agosto"@it ,
        "8月"@ja ,
        "Augustus (maand)"@nl ,
        "Sierpień"@pl ,
        "Agosto"@pt ,
        "Август"@ru ,
        "8月"@zh ;
    time:month "--08"^^xsd:gMonth ;
    time:unitType time:unitMonth ;
    prov:wasDerivedFrom cs: ;
.

greg:December
    a
        skos:Concept ,
        time:MonthOfYear ;
    rdfs:isDefinedBy cs: ;
    rdfs:seeAlso <http://en.wikipedia.org/wiki/December> ;
    skos:altLabel "DECEMBER"@en ;
    skos:definition "December is the twelfth and final month of the year in the Julian and Gregorian Calendars. It is also the last of seven months to have a length of 31 days."@en ;
    skos:inScheme cs: ;
    skos:notation "DEC" ;
    skos:prefLabel
        "ديسمبر"@ar ,
        "Dezember"@de ,
        "December"@en ,
        "Diciembre"@es ,
        "Décembre"@fr ,
        "Dicembre"@it ,
        "12月"@ja ,
        "December"@nl ,
        "Grudzień"@pl ,
        "Dezembro"@pt ,
        "Декабрь"@ru ,
        "12月"@zh ;
    time:month "--12"^^xsd:gMonth ;
    prov:wasDerivedFrom cs: ;
.

greg:February
    a
        skos:Concept ,
        time:MonthOfYear ;
    rdfs:isDefinedBy cs: ;
    rdfs:seeAlso <http://en.wikipedia.org/wiki/February> ;
    skos:altLabel "FEBRUARY"@en ;
    skos:definition "February is the second month of the year in the Julian and Gregorian calendars, with 28 days in common years and 29 days in leap years, with the quadrennial 29th day being called the leap day."@en ;
    skos:inScheme cs: ;
    skos:notation "FEB" ;
    skos:prefLabel
        "فبراير"@ar ,
        "Februar"@de ,
        "February"@en ,
        "Febrero"@es ,
        "Février"@fr ,
        "Febbraio"@it ,
        "2月"@ja ,
        "Februari"@nl ,
        "Luty"@pl ,
        "Fevereiro"@pt ,
        "Февраль"@ru ,
        "2月"@zh ;
    time:month "--02"^^xsd:gMonth ;
    prov:wasDerivedFrom cs: ;
.

greg:January
    a
        skos:Concept ,
        time:MonthOfYear ;
    rdfs:isDefinedBy cs: ;
    rdfs:seeAlso <http://en.wikipedia.org/wiki/January> ;
    skos:altLabel "JANUARY"@en ;
    skos:definition "January is the first month of the year in the Julian and Gregorian calendars and the first of seven months to have a length of 31 days."@en ;
    skos:inScheme cs: ;
    skos:notation "JAN" ;
    skos:prefLabel
        "JF'J1 (4G1)"@ar ,
        "Januar"@de ,
        "January"@en ,
        "Enero"@es ,
        "Janvier"@fr ,
        "Gennaio"@it ,
        "1"@ja ,
        "Januari"@nl ,
        "StyczeD"@pl ,
        "Janeiro"@pt ,
        "/=20@L"@ru ,
        "1"@zh ;
    time:month "--01"^^xsd:gMonth ;
    prov:wasDerivedFrom cs: ;
.

greg:July
    a
        skos:Concept ,
        time:MonthOfYear ;
    rdfs:isDefinedBy cs: ;
    rdfs:seeAlso <http://en.wikipedia.org/wiki/July> ;
    skos:altLabel "JULY"@en ;
    skos:definition "July is the seventh month of the year (between June and August) in the Julian and Gregorian Calendars and the fourth of seven months to have a length of 31 days."@en ;
    skos:inScheme cs: ;
    skos:notation "JUL" ;
    skos:prefLabel
        "JHDJH"@ar ,
        "Juli"@de ,
        "July"@en ,
        "Julio"@es ,
        "Juillet"@fr ,
        "Luglio"@it ,
        "7"@ja ,
        "Juli"@nl ,
        "Lipiec"@pl ,
        "Julho"@pt ,
        "N;L"@ru ,
        "7"@zh ;
    time:month "--07"^^xsd:gMonth ;
    prov:wasDerivedFrom cs: ;
.

greg:June
    a
        skos:Concept ,
        time:MonthOfYear ;
    rdfs:isDefinedBy cs: ;
    rdfs:seeAlso <http://en.wikipedia.org/wiki/June> ;
    skos:altLabel "JUNE"@en ;
    skos:definition "June is the sixth month of the year in the Julian and Gregorian calendars, the second of four months to have a length of 30 days, and the third of five months to have a length of less than 31 days."@en ;
    skos:inScheme cs: ;
    skos:notation "JUN" ;
    skos:prefLabel
        "JHFJH"@ar ,
        "Juni"@de ,
        "June"@en ,
        "Junio"@es ,
        "Juin"@fr ,
        "Giugno"@it ,
        "6"@ja ,
        "Juni"@nl ,
        "Czerwiec"@pl ,
        "Junho"@pt ,
        "N=L"@ru ,
        "6"@zh ;
    time:month "--06"^^xsd:gMonth ;
    prov:wasDerivedFrom cs: ;
.

greg:March
    a
        skos:Concept ,
        time:MonthOfYear ;
    rdfs:isDefinedBy cs: ;
    rdfs:seeAlso <http://en.wikipedia.org/wiki/March> ;
    skos:altLabel "MARCH"@en ;
    skos:definition "March is the third month of the year and named after Mars in both the Julian and Gregorian calendars. It is the second of seven months to have a length of 31 days."@en ;
    skos:inScheme cs: ;
    skos:notation "MAR" ;
    skos:prefLabel
        "مارس"@ar ,
        "März"@de ,
        "March"@en ,
        "Marzo"@es ,
        "Mars (mois)"@fr ,
        "Marzo"@it ,
        "3月"@ja ,
        "Maart"@nl ,
        "Marzec"@pl ,
        "Março"@pt ,
        "Март"@ru ,
        "3月"@zh ;
    time:month "--03"^^xsd:gMonth ;
    prov:wasDerivedFrom cs: ;
.

greg:May
    a
        skos:Concept ,
        time:MonthOfYear ;
    rdfs:isDefinedBy cs: ;
    rdfs:seeAlso <http://en.wikipedia.org/wiki/May> ;
    skos:altLabel "MAY"@en ;
    skos:definition "May is the fifth month of the year in the Julian and Gregorian calendars and the third of seven months to have a length of 31 days."@en ;
    skos:inScheme cs: ;
    skos:notation "MAY" ;
    skos:prefLabel
        "مايو"@ar ,
        "Mai"@de ,
        "May"@en ,
        "Mayo"@es ,
        "Mai"@fr ,
        "Maggio"@it ,
        "5月"@ja ,
        "Mei"@nl ,
        "Maj"@pl ,
        "Maio"@pt ,
        "Май"@ru ,
        "5月"@zh ;
    time:month "--05"^^xsd:gMonth ;
    prov:wasDerivedFrom cs: ;
.

greg:November
    a
        skos:Concept ,
        time:MonthOfYear ;
    rdfs:isDefinedBy cs: ;
    rdfs:seeAlso <http://en.wikipedia.org/wiki/November> ;
    skos:altLabel "NOVEMBER"@en ;
    skos:definition "November is the eleventh month of the year in the Julian and Gregorian Calendars, the fourth and last of four months to have a length of 30 days and the fifth and last of five months to have a length of fewer than 31 days."@en ;
    skos:inScheme cs: ;
    skos:notation "NOV" ;
    skos:prefLabel
        "نوفمبر"@ar ,
        "November"@de ,
        "November"@en ,
        "Noviembre"@es ,
        "Novembre"@fr ,
        "Novembre"@it ,
        "11月"@ja ,
        "November"@nl ,
        "Listopad"@pl ,
        "Novembro"@pt ,
        "Ноябрь"@ru ,
        "11月"@zh ;
    time:month "--11"^^xsd:gMonth ;
    prov:wasDerivedFrom cs: ;
.

greg:October
    a
        skos:Concept ,
        time:MonthOfYear ;
    rdfs:isDefinedBy cs: ;
    rdfs:seeAlso <http://en.wikipedia.org/wiki/October> ;
    skos:altLabel "OCTOBER"@en ;
    skos:definition "October is the tenth month of the year in the Julian and Gregorian Calendars and the sixth of seven months to have a length of 31 days."@en ;
    skos:inScheme cs: ;
    skos:notation "OCT" ;
    skos:prefLabel
        "أكتوبر"@ar ,
        "Oktober"@de ,
        "October"@en ,
        "Octubre"@es ,
        "Octobre"@fr ,
        "Ottobre"@it ,
        "10月"@ja ,
        "Oktober"@nl ,
        "Październik"@pl ,
        "Outubro"@pt ,
        "Октябрь"@ru ,
        "10月"@zh ;
    time:month "--10"^^xsd:gMonth ;
    prov:wasDerivedFrom cs: ;
.

greg:September
    a
        skos:Concept ,
        time:MonthOfYear ;
    rdfs:isDefinedBy cs: ;
    rdfs:seeAlso <http://en.wikipedia.org/wiki/September> ;
    skos:altLabel "SEPTEMBER"@en ;
    skos:definition "September is the ninth month of the year in the Julian and Gregorian calendars, the third of four months to have a length of 30 days, and the fourth of five months to have a length of less than 31 days."@en ;
    skos:inScheme cs: ;
    skos:notation "SEP" ;
    skos:prefLabel
        "سبتمبر"@ar ,
        "September"@de ,
        "September"@en ,
        "Septiembre"@es ,
        "Septembre"@fr ,
        "Settembre"@it ,
        "9月"@ja ,
        "September"@nl ,
        "Wrzesień"@pl ,
        "Setembro"@pt ,
        "Сентябрь"@ru ,
        "9月"@zh ;
    time:month "--09"^^xsd:gMonth ;
    prov:wasDerivedFrom cs: ;
.

<https://linked.data.gov.au/org/csiro>
    a sdo:Organization ;
    sdo:name "CSIRO" ;
    sdo:url "http://www.csiro.au"^^xsd:anyURI ;
.

<https://linked.data.gov.au/org/w3c>
    a sdo:Organization ;
    sdo:name "World Wide Web Consortium" ;
    sdo:url "http://www.iso.org"^^xsd:anyURI ;
.

<https://orcid.org/0000-0002-8742-7730>
    a sdo:Person ;
    sdo:affiliation <https://kurrawong.ai> ;
    sdo:email "nick@kurrawong.ai"^^xsd:anyURI ;
    sdo:identifier <https://orcid.org/0000-0002-8742-7730> ;
    sdo:name "Nicholas J. Car" ;
.

<https://kurrawong.ai>
    a sdo:Organization ;
    sdo:name "KurrawongAI" ;
    sdo:url "https://kurrawong.ai"^^xsd:anyURI ;
.

<http://orcid.org/0000-0002-3884-3420>
    a sdo:Person ;
    sdo:affiliation <https://linked.data.gov.au/org/csiro> ;
    sdo:email "simon.cox@csiro.au"^^xsd:anyURI ;
    sdo:identifier <http://orcid.org/0000-0002-3884-3420> ;
    sdo:name "Simon J.D. Cox" ;
.

cs:
    a
        owl:Ontology ,
        skos:ConceptScheme ;
    dcterms:created "2017-01-20"^^xsd:date ;
    dcterms:creator <http://orcid.org/0000-0002-3884-3420> ;
    dcterms:modified "2023-03-16"^^xsd:date ;
    dcterms:publisher <https://linked.data.gov.au/org/w3c> ;
    reg:status agldwgstatus:stable ;
    owl:imports
        <http://www.w3.org/2004/02/skos/core> ,
        <http://www.w3.org/2006/time> ;
    skos:definition "The set of months-of-the-year from the Gregorian calendar."@en ;
    skos:hasTopConcept
        greg:April ,
        greg:August ,
        greg:December ,
        greg:February ,
        greg:January ,
        greg:July ,
        greg:June ,
        greg:March ,
        greg:May ,
        greg:November ,
        greg:October ,
        greg:September ;
    skos:prefLabel "Gregorian Months"@en ;
    prov:wasDerivedFrom cs: ;
.

