PREFIX agldwgstatus: <https://linked.data.gov.au/def/reg-statuses/>
PREFIX cs: <http://linked.data.gov.au/def/gsq-roles>
PREFIX datac: <http://linked.data.gov.au/def/dataciteroles/>
PREFIX dcat: <http://www.w3.org/ns/dcat#>
PREFIX dcterms: <http://purl.org/dc/terms/>
PREFIX gsqr: <http://linked.data.gov.au/def/gsq-roles/>
PREFIX iso11179: <http://linked.data.gov.au/def/iso11179-6/RolesAndResponsibilities/>
PREFIX isorole: <http://linked.data.gov.au/def/iso19115-1/RoleCode/>
PREFIX owl: <http://www.w3.org/2002/07/owl#>
PREFIX rdfs1: <file:///Users/edmondchuc/projects/gsq-vocabularies/vocabularies-gsq/www.w3.org/2000/01/rdf-schema#>
PREFIX reg: <http://purl.org/linked-data/registry#>
PREFIX sdo: <https://schema.org/>
PREFIX skos: <http://www.w3.org/2004/02/skos/core#>
PREFIX xsd: <http://www.w3.org/2001/XMLSchema#>

gsqr:QdexReportsRoles
    a skos:Collection ;
    dcterms:source "http://standards.iso.org/iso/19115/resources/Codelists/gml/CI_RoleCode.xml"^^xsd:anyURI ;
    skos:definition "A collection of roles used for Agents within the Georesources Reports regime"@en ;
    skos:member
        gsqr:contractor ,
        gsqr:driller ,
        gsqr:operator ,
        iso11179:Submitter ,
        isorole:author ,
        isorole:owner ,
        isorole:publisher ;
    skos:prefLabel "Georesources Reports Roles"@en ;
.

gsqr:consultant
    a skos:Concept ;
    rdfs1:isDefinedBy cs: ;
    dcterms:source "http://standards.iso.org/iso/19115/resources/Codelists/gml/CI_RoleCode.xml"^^xsd:anyURI ;
    skos:broader gsqr:contractor ;
    skos:definition "Consultants are contractors who provide value-added services and advice to other agents, e.g. owners or operators. Consultants may aggregate multiple other roles including project management, data curation, data processing, analysis, and advisory roles. Consultants are commonly an intermediary between agents."@en ;
    skos:inScheme cs: ;
    skos:prefLabel "Consultant"@en ;
    skos:scopeNote "Consultants are a type of contractor, and as such should always act on behalf of (formally: prov:actedObBehalfOf) some other Agent, such as an Owner"@en ;
.

gsqr:des-roles
    a skos:Collection ;
    dcterms:source "http://standards.iso.org/iso/19115/resources/Codelists/gml/CI_RoleCode.xml"^^xsd:anyURI ;
    skos:definition "A collection of roles used by DES"@en ;
    skos:member
        datac:ProjectLeader ,
        datac:ProjectManager ,
        datac:ProjectMember ,
        gsqr:administrator ,
        gsqr:data-creator ,
        gsqr:data-librarian ,
        gsqr:data-steward ,
        gsqr:manager ,
        isorole:collaborator ,
        isorole:contributor ,
        isorole:custodian ,
        isorole:owner ,
        isorole:publisher ,
        isorole:user ;
    skos:prefLabel "Department of Environment and Science Roles"@en ;
.

gsqr:surveyor
    a
        skos:Concept ,
        dcat:Role ;
    rdfs1:isDefinedBy cs: ;
    dcterms:source "http://standards.iso.org/iso/19115/resources/Codelists/gml/CI_RoleCode.xml"^^xsd:anyURI ;
    skos:broader isorole:principalInvestigator ;
    skos:definition "The principal investigator for a land surveying activity creating geomatic survey plans, maps, and project working plans."@en ;
    skos:inScheme cs: ;
    skos:prefLabel "Surveyor"@en ;
.

datac:DataCollector
    a skos:Concept ;
    rdfs1:isDefinedBy cs: ;
    dcterms:source "http://standards.iso.org/iso/19115/resources/Codelists/gml/CI_RoleCode.xml"^^xsd:anyURI ;
    skos:altLabel
        "Interviewer"@en ,
        "Observation Agent"@en ,
        "Observer"@en ,
        "Survey Conductor"@en ;
    skos:definition "Person/institution responsible for finding, gathering/collecting data under the guidelines of the author(s) or Principal Investigator (PI)."@en ;
    skos:inScheme cs: ;
    skos:prefLabel "Data Collector"@en ;
    skos:scopeNote "May also use when crediting survey conductors, interviewers, event or condition observers, person responsible for monitoring key instrument data."@en ;
    skos:topConceptOf cs: ;
.

isorole:editor
    a skos:Concept ;
    dcterms:source "http://standards.iso.org/iso/19115/resources/Codelists/gml/CI_RoleCode.xml"^^xsd:anyURI ;
    skos:altLabel "Reviewer"@en ;
    skos:definition "Party who reviewed or modified the resource to improve the content"@en ;
    skos:historyNote "Agent is known as Party in the original definition from ISO19115"@en ;
    skos:inScheme cs: ;
    skos:prefLabel "Editor"@en ;
    skos:topConceptOf cs: ;
.

isorole:originator
    a skos:Concept ;
    rdfs1:isDefinedBy cs: ;
    dcterms:source "http://standards.iso.org/iso/19115/resources/Codelists/gml/CI_RoleCode.xml"^^xsd:anyURI ;
    skos:altLabel "Sampler"@en ;
    skos:definition "Party who created the resource"@en ;
    skos:inScheme cs: ;
    skos:prefLabel "Originator"@en ;
    skos:topConceptOf cs: ;
.

isorole:processor
    a skos:Concept ;
    rdfs1:isDefinedBy cs: ;
    dcterms:source "http://standards.iso.org/iso/19115/resources/Codelists/gml/CI_RoleCode.xml"^^xsd:anyURI ;
    skos:definition "Party who has processed the data in a manner such that the resource has been modified"@en ;
    skos:inScheme cs: ;
    skos:prefLabel "Processor"@en ;
    skos:topConceptOf cs: ;
.

datac:ProjectLeader
    a skos:Concept ;
    rdfs1:isDefinedBy <http://linked.data.gov.au/def/dataciteroles> ;
    dcterms:source "http://standards.iso.org/iso/19115/resources/Codelists/gml/CI_RoleCode.xml"^^xsd:anyURI ;
    skos:definition "Person officially designated as head of project team or sub-project team instrumental in the work necessary to development of the resource."@en ;
    skos:inScheme cs: ;
    skos:prefLabel "Project Leader"@en ;
    skos:scopeNote "The Project Leader is not 'removed' from the work that resulted in the resource; he or she remains intimately involved throughout the life of the particular project team."@en ;
    skos:topConceptOf cs: ;
.

datac:ProjectManager
    a skos:Concept ;
    rdfs1:isDefinedBy <http://linked.data.gov.au/def/dataciteroles> ;
    dcterms:source "http://standards.iso.org/iso/19115/resources/Codelists/gml/CI_RoleCode.xml"^^xsd:anyURI ;
    skos:definition "Person officially designated as manager of a project. Project may consist of one or many project teams and sub-teams."@en ;
    skos:inScheme cs: ;
    skos:prefLabel "Project Manager"@en ;
    skos:scopeNote "The manager of a project normally has more administrative responsibility than actual work involvement."@en ;
    skos:topConceptOf cs: ;
.

datac:ProjectMember
    a skos:Concept ;
    rdfs1:isDefinedBy <http://linked.data.gov.au/def/dataciteroles> ;
    dcterms:source "http://standards.iso.org/iso/19115/resources/Codelists/gml/CI_RoleCode.xml"^^xsd:anyURI ;
    skos:definition "Person on the membership list of a designated project/project team."@en ;
    skos:inScheme cs: ;
    skos:prefLabel "Project Member"@en ;
    skos:scopeNote "This vocabulary may or may not indicate the quality, quantity, or substance of the person's involvement."@en ;
    skos:topConceptOf cs: ;
.

gsqr:administrator
    a
        skos:Concept ,
        dcat:Role ;
    rdfs1:isDefinedBy cs: ;
    dcterms:source "http://standards.iso.org/iso/19115/resources/Codelists/gml/CI_RoleCode.xml"^^xsd:anyURI ;
    skos:definition "Design, implementation and maintenance of the technology environment that supports/enables the information management lifecycle."@en ;
    skos:inScheme cs: ;
    skos:prefLabel "Data Administrator"@en ;
    skos:related gsqr:manager ;
    skos:topConceptOf cs: ;
.

gsqr:data-creator
    a
        skos:Concept ,
        dcat:Role ;
    rdfs1:isDefinedBy cs: ;
    dcterms:source "http://standards.iso.org/iso/19115/resources/Codelists/gml/CI_RoleCode.xml"^^xsd:anyURI ;
    skos:definition "Responsible for creating and updating data, products and metadata and storing in an appropriate system."@en ;
    skos:inScheme cs: ;
    skos:prefLabel "Data Creator"@en ;
    skos:topConceptOf cs: ;
.

gsqr:data-librarian
    a
        skos:Concept ,
        dcat:Role ;
    rdfs1:isDefinedBy cs: ;
    dcterms:source "http://standards.iso.org/iso/19115/resources/Codelists/gml/CI_RoleCode.xml"^^xsd:anyURI ;
    skos:definition "Responsible for investigating and assisting with implementation of support services relating to description, storage and sharing of research metadata and datasets. Including standards, review processes and training."@en ;
    skos:inScheme cs: ;
    skos:prefLabel "Data Librarian"@en ;
    skos:related gsqr:manager ;
    skos:topConceptOf cs: ;
.

gsqr:data-steward
    a
        skos:Concept ,
        dcat:Role ;
    rdfs1:isDefinedBy cs: ;
    rdfs1:label "Data Steward"@en ;
    dcterms:source "http://standards.iso.org/iso/19115/resources/Codelists/gml/CI_RoleCode.xml"^^xsd:anyURI ;
    skos:definition "Responsible for approving the quality, integrity and use of data and applying data policies, procedures and rules to safeguard data. Provides guidance and training to ensure timely and correct input of quality data."@en ;
    skos:inScheme cs: ;
    skos:prefLabel "Data Steward"@en ;
    skos:related gsqr:manager ;
    skos:topConceptOf cs: ;
.

gsqr:driller
    a skos:Concept ;
    rdfs1:isDefinedBy cs: ;
    dcterms:source "http://standards.iso.org/iso/19115/resources/Codelists/gml/CI_RoleCode.xml"^^xsd:anyURI ;
    skos:definition "The agent who drills or bores the borehole."@en ;
    skos:inScheme cs: ;
    skos:prefLabel "Driller"@en ;
    skos:topConceptOf cs: ;
.

gsqr:operator
    a skos:Concept ;
    rdfs1:isDefinedBy cs: ;
    dcterms:source "http://standards.iso.org/iso/19115/resources/Codelists/gml/CI_RoleCode.xml"^^xsd:anyURI ;
    skos:definition "The corporation or other entity that is the decision-maker and has responsibility for the overall management for the project."@en ;
    skos:inScheme cs: ;
    skos:prefLabel "Operator"@en ;
    skos:topConceptOf cs: ;
.

iso11179:Submitter
    a skos:Concept ;
    dcterms:source "http://standards.iso.org/iso/19115/resources/Codelists/gml/CI_RoleCode.xml"^^xsd:anyURI ;
    skos:altLabel "Lodger"@en ;
    skos:definition "A Submitter should be an organizational unit approved by a process defined by the Registration Authority. A Submitter is authorized to identify and report Administered Items suitable for registration. The Submitter can be viewed as a contact for the Submitting Organization."@en ;
    skos:historyNote "In QDEX Reports, this role has been known as 'Lodger' but 'Submitter' is now the preferred term for it."@en ;
    skos:inScheme cs: ;
    skos:prefLabel "Submitter"@en ;
    skos:topConceptOf cs: ;
.

isorole:author
    a skos:Concept ;
    dcterms:source "http://standards.iso.org/iso/19115/resources/Codelists/gml/CI_RoleCode.xml"^^xsd:anyURI ;
    skos:definition "Agent who authored the resource"@en ;
    skos:historyNote "Agent is known as Party in the original definition from ISO19115"@en ;
    skos:inScheme cs: ;
    skos:prefLabel "Author"@en ;
    skos:topConceptOf cs: ;
.

isorole:collaborator
    a skos:Concept ;
    rdfs1:isDefinedBy cs: ;
    dcterms:source "http://standards.iso.org/iso/19115/resources/Codelists/gml/CI_RoleCode.xml"^^xsd:anyURI ;
    skos:definition "Party who assists with the generation of the resource other than the principal investigator"@en ;
    skos:inScheme cs: ;
    skos:prefLabel "Collaborator"@en ;
    skos:topConceptOf cs: ;
.

isorole:contributor
    a skos:Concept ;
    rdfs1:isDefinedBy <http://linked.data.gov.au/def/iso19115-1/RoleCode> ;
    dcterms:source "http://standards.iso.org/iso/19115/resources/Codelists/gml/CI_RoleCode.xml"^^xsd:anyURI ;
    skos:definition "Party contributing to the resource"@en ;
    skos:inScheme cs: ;
    skos:prefLabel "Contributor"@en ;
    skos:topConceptOf cs: ;
.

isorole:custodian
    a skos:Concept ;
    rdfs1:isDefinedBy <http://linked.data.gov.au/def/iso19115-1/RoleCode> ;
    dcterms:source "http://standards.iso.org/iso/19115/resources/Codelists/gml/CI_RoleCode.xml"^^xsd:anyURI ;
    skos:definition "Party that accepts accountability and responsibility for the resource and ensures appropriate care and maintenance of the resource"@en ;
    skos:inScheme cs: ;
    skos:prefLabel "Custodian"@en ;
    skos:topConceptOf cs: ;
.

isorole:principalInvestigator
    a skos:Concept ;
    rdfs1:isDefinedBy cs: ;
    dcterms:source "http://standards.iso.org/iso/19115/resources/Codelists/gml/CI_RoleCode.xml"^^xsd:anyURI ;
    skos:definition "Key party responsible for gathering information and conducting research"@en ;
    skos:inScheme cs: ;
    skos:prefLabel "Principal Investigator"@en ;
    skos:topConceptOf cs: ;
.

isorole:user
    a skos:Concept ;
    dcterms:source "http://standards.iso.org/iso/19115/resources/Codelists/gml/CI_RoleCode.xml"^^xsd:anyURI ;
    skos:definition "Party who uses the resource"@en ;
    skos:historyNote "Agent is known as Party in the original definition from ISO19115"@en ;
    skos:inScheme cs: ;
    skos:prefLabel "User"@en ;
    skos:topConceptOf cs: ;
.

<https://linked.data.gov.au/org/gsq>
    a sdo:Organization ;
    sdo:name "Geological Survey of Queensland" ;
    sdo:url "http://www.business.qld.gov.au/industries/mining-energy-water/resources/geoscience-information/gsq"^^xsd:anyURI ;
.

gsqr:contractor
    a skos:Concept ;
    rdfs1:isDefinedBy cs: ;
    dcterms:source "http://standards.iso.org/iso/19115/resources/Codelists/gml/CI_RoleCode.xml"^^xsd:anyURI ;
    skos:altLabel "Service Provider"@en ;
    skos:definition "Contractors are agents who receive work contracts to perform activities on behalf of other agents, e.g. owners or operators."@en ;
    skos:inScheme cs: ;
    skos:prefLabel "Contractor"@en ;
    skos:scopeNote "Contractors should always act on behalf of (formally: prov:actedObBehalfOf) some other Agent, such as an Owner"@en ;
    skos:topConceptOf cs: ;
.

isorole:owner
    a skos:Concept ;
    dcterms:source "http://standards.iso.org/iso/19115/resources/Codelists/gml/CI_RoleCode.xml"^^xsd:anyURI ;
    skos:altLabel
        "authority holder"@en ,
        "permit holder"@en ,
        "tenure holder"@en ;
    skos:definition "Agent that owns the resource"@en ;
    skos:historyNote "Agent is known as Party in the original definition from ISO19115. The altLabels are drawn from P&G (general provisions) regulation 2017, section 37(4)"@en ;
    skos:inScheme cs: ;
    skos:prefLabel "Owner"@en ;
    skos:topConceptOf cs: ;
.

isorole:publisher
    a skos:Concept ;
    dcterms:source "http://standards.iso.org/iso/19115/resources/Codelists/gml/CI_RoleCode.xml"^^xsd:anyURI ;
    skos:definition "Agent who published the resource"@en ;
    skos:historyNote "Agent is known as Party in the original definition from ISO19115"@en ;
    skos:inScheme cs: ;
    skos:prefLabel "Publisher"@en ;
    skos:topConceptOf cs: ;
.

gsqr:manager
    a
        skos:Concept ,
        dcat:Role ;
    rdfs1:isDefinedBy cs: ;
    rdfs1:label "Data Manager"@en ;
    dcterms:source "http://standards.iso.org/iso/19115/resources/Codelists/gml/CI_RoleCode.xml"^^xsd:anyURI ;
    skos:definition "The Data Manager is assigned to perform activities associated with the day-to-day interpretation, management, operation and support of data."@en ;
    skos:inScheme cs: ;
    skos:prefLabel "Data Manager"@en ;
    skos:topConceptOf cs: ;
.

cs:
    a
        owl:Ontology ,
        skos:ConceptScheme ;
    dcterms:created "2019-10-17"^^xsd:date ;
    dcterms:creator <https://linked.data.gov.au/org/gsq> ;
    dcterms:modified "2023-03-16"^^xsd:date ;
    dcterms:publisher <https://linked.data.gov.au/org/gsq> ;
    dcterms:source "http://standards.iso.org/iso/19115/resources/Codelists/gml/CI_RoleCode.xml"^^xsd:anyURI ;
    reg:status agldwgstatus:stable ;
    skos:definition "The roles of Agents (People and Organisations) in relation to Entities (Datasets, Samples etc.)."@en ;
    skos:hasTopConcept
        datac:DataCollector ,
        datac:ProjectLeader ,
        datac:ProjectManager ,
        datac:ProjectMember ,
        gsqr:administrator ,
        gsqr:contractor ,
        gsqr:data-creator ,
        gsqr:data-librarian ,
        gsqr:data-steward ,
        gsqr:driller ,
        gsqr:manager ,
        gsqr:operator ,
        iso11179:Submitter ,
        isorole:author ,
        isorole:collaborator ,
        isorole:contributor ,
        isorole:custodian ,
        isorole:editor ,
        isorole:originator ,
        isorole:owner ,
        isorole:principalInvestigator ,
        isorole:processor ,
        isorole:publisher ,
        isorole:user ;
    skos:prefLabel "Geological Survey of Queensland's Agent Roles"@en ;
.

