PREFIX agldwgstatus: <https://linked.data.gov.au/def/reg-statuses/>
PREFIX cs: <http://linked.data.gov.au/def/party-identifier-type>
PREFIX dcterms: <http://purl.org/dc/terms/>
PREFIX id: <http://linked.data.gov.au/def/party-identifier-type/>
PREFIX owl: <http://www.w3.org/2002/07/owl#>
PREFIX rdfs: <http://www.w3.org/2000/01/rdf-schema#>
PREFIX reg: <http://purl.org/linked-data/registry#>
PREFIX sdo: <https://schema.org/>
PREFIX skos: <http://www.w3.org/2004/02/skos/core#>
PREFIX xsd: <http://www.w3.org/2001/XMLSchema#>

id:company-id
    a skos:Collection ;
    skos:historyNote "Compiled by the Geological Survey of Queensland. From (QGOV)<http://account.qld.gov.au/help/faq.html#howDoIProvide100PointsOfIdentification> and (MyMinesOnline) <http://www.business.qld.gov.au/industries/mining-energy-water/resources/minerals-coal/online-services/myminesonline/register>" ;
    skos:definition "Identification numbers for businesses and companies within Australia."@en ;
    skos:member
        id:abn ,
        id:acn ,
        id:c-code ;
    skos:prefLabel "Company ID"@en ;
.

id:mmol-list-a
    a skos:Collection ;
    skos:historyNote "Compiled by the Geological Survey of Queensland. From (QGOV)<http://account.qld.gov.au/help/faq.html#howDoIProvide100PointsOfIdentification> and (MyMinesOnline) <http://www.business.qld.gov.au/industries/mining-energy-water/resources/minerals-coal/online-services/myminesonline/register>" ;
    skos:definition "Personal identification documents that act as primary proof-of-identity in the State of Queensland within MyMinesOnline. Identity checks must include at least one document from List A and one document from List B."@en ;
    skos:member
        id:australian-passport ,
        id:drivers-licence ,
        id:firearms-licence ,
        id:foregin-passport ,
        id:public-service-photo-id ;
    skos:prefLabel "MMOL list A"@en ;
.

id:mmol-list-b
    a skos:Collection ;
    skos:historyNote "Compiled by the Geological Survey of Queensland. From (QGOV)<http://account.qld.gov.au/help/faq.html#howDoIProvide100PointsOfIdentification> and (MyMinesOnline) <http://www.business.qld.gov.au/industries/mining-energy-water/resources/minerals-coal/online-services/myminesonline/register>" ;
    skos:definition "Personal identification documents that act as secondary proof-of-identity in the State of Queensland within MyMinesOnline. Identity checks must include at least one document from List A and one document from List B."@en ;
    skos:member
        id:australian-university-id-card ,
        id:bank-card ,
        id:centrelink-card ,
        id:change-of-name-certificate ,
        id:council-rates-notice ,
        id:electrol-roll-extract ,
        id:letter-from-employer ,
        id:marriage-certificate ,
        id:medicare-card ,
        id:security-guard-licence ,
        id:veterans-affairs-card ;
    skos:prefLabel "MMOL list B"@en ;
.

id:personal-id
    a skos:Collection ;
    skos:historyNote "Compiled by the Geological Survey of Queensland. From (QGOV)<http://account.qld.gov.au/help/faq.html#howDoIProvide100PointsOfIdentification> and (MyMinesOnline) <http://www.business.qld.gov.au/industries/mining-energy-water/resources/minerals-coal/online-services/myminesonline/register>" ;
    skos:definition "Australian or state-issued documents accepted as proof-of-identity for individuals by the Queensland Government."@en ;
    skos:member
        id:australian-passport ,
        id:australian-university-id-card ,
        id:australian-visa ,
        id:bank-card ,
        id:birth-certificate ,
        id:centrelink-card ,
        id:certificate-of-australian-citizenship ,
        id:change-of-name-certificate ,
        id:council-rates-notice ,
        id:drivers-licence ,
        id:electrol-roll-extract ,
        id:firearms-licence ,
        id:foregin-passport ,
        id:letter-from-employer ,
        id:marriage-certificate ,
        id:medicare-card ,
        id:public-service-photo-id ,
        id:security-guard-licence ,
        id:veterans-affairs-card ;
    skos:prefLabel "Personal ID"@en ;
.

id:qgov-primary-documents
    a skos:Collection ;
    skos:historyNote "Compiled by the Geological Survey of Queensland. From (QGOV)<http://account.qld.gov.au/help/faq.html#howDoIProvide100PointsOfIdentification> and (MyMinesOnline) <http://www.business.qld.gov.au/industries/mining-energy-water/resources/minerals-coal/online-services/myminesonline/register>" ;
    skos:definition "Personal identification documents that act as primary proof-of-identity in the State of Queensland within the QGOV identity brokerage system. Identity checks must make up 100 points and include at least one primary document."@en ;
    skos:member
        id:australian-passport ,
        id:birth-certificate ,
        id:drivers-licence ;
    skos:prefLabel "QGOV Primary Documents"@en ;
.

id:qgov-secondary-documents
    a skos:Collection ;
    skos:historyNote "Compiled by the Geological Survey of Queensland. From (QGOV)<http://account.qld.gov.au/help/faq.html#howDoIProvide100PointsOfIdentification> and (MyMinesOnline) <http://www.business.qld.gov.au/industries/mining-energy-water/resources/minerals-coal/online-services/myminesonline/register>" ;
    skos:definition "Personal identification documents that act as secondary proof-of-identity in the State of Queensland within the QGOV identity brokerage system. Identity checks must make up 100 points and include at least one primary document."@en ;
    skos:member
        id:australian-visa ,
        id:certificate-of-australian-citizenship ,
        id:change-of-name-certificate ,
        id:marriage-certificate ,
        id:medicare-card ;
    skos:prefLabel "QGOV Secondary Documents"@en ;
.

id:abn
    a skos:Concept ;
    skos:historyNote "Compiled by the Geological Survey of Queensland. From (QGOV)<http://account.qld.gov.au/help/faq.html#howDoIProvide100PointsOfIdentification> and (MyMinesOnline) <http://www.business.qld.gov.au/industries/mining-energy-water/resources/minerals-coal/online-services/myminesonline/register>" ;
    rdfs:isDefinedBy cs: ;
    skos:altLabel "Australian business number"@en ;
    skos:definition "The Australian Business Number (ABN) is a unique number used to identify business names and companies. The Australian Business Register (ABR) provides ABNs. Source:ASIC"@en ;
    skos:inScheme cs: ;
    skos:prefLabel "ABN"@en ;
    skos:topConceptOf cs: ;
.

id:acn
    a skos:Concept ;
    skos:historyNote "Compiled by the Geological Survey of Queensland. From (QGOV)<http://account.qld.gov.au/help/faq.html#howDoIProvide100PointsOfIdentification> and (MyMinesOnline) <http://www.business.qld.gov.au/industries/mining-energy-water/resources/minerals-coal/online-services/myminesonline/register>" ;
    rdfs:isDefinedBy cs: ;
    skos:altLabel "Australian company number"@en ;
    skos:definition "Every company in Australia is issued with a unique, nine-digit number when registered. This is an Australian Company Number (ACN) and must be displayed on all company documents. Source:ASIC"@en ;
    skos:inScheme cs: ;
    skos:prefLabel "ACN"@en ;
    skos:topConceptOf cs: ;
.

id:c-code
    a skos:Concept ;
    skos:historyNote "Compiled by the Geological Survey of Queensland. From (QGOV)<http://account.qld.gov.au/help/faq.html#howDoIProvide100PointsOfIdentification> and (MyMinesOnline) <http://www.business.qld.gov.au/industries/mining-energy-water/resources/minerals-coal/online-services/myminesonline/register>" ;
    rdfs:isDefinedBy cs: ;
    skos:definition "A locally relevant company code, commonly locally administered by an individual agency."@en ;
    skos:inScheme cs: ;
    skos:prefLabel "Company Code"@en ;
    skos:topConceptOf cs: ;
.

<https://linked.data.gov.au/org/gsq>
    a sdo:Organization ;
    sdo:name "Geological Survey of Queensland" ;
    sdo:url "http://www.business.qld.gov.au/industries/mining-energy-water/resources/geoscience-information/gsq"^^xsd:anyURI ;
.

id:australian-university-id-card
    a skos:Concept ;
    skos:historyNote "Compiled by the Geological Survey of Queensland. From (QGOV)<http://account.qld.gov.au/help/faq.html#howDoIProvide100PointsOfIdentification> and (MyMinesOnline) <http://www.business.qld.gov.au/industries/mining-energy-water/resources/minerals-coal/online-services/myminesonline/register>" ;
    rdfs:isDefinedBy cs: ;
    skos:definition "An identification card issued by a recognised Australian tertiary education institute. Cards must be less than 1 year old to be valid."@en ;
    skos:inScheme cs: ;
    skos:prefLabel "Australian university ID card"@en ;
    skos:topConceptOf cs: ;
.

id:australian-visa
    a skos:Concept ;
    skos:historyNote "Compiled by the Geological Survey of Queensland. From (QGOV)<http://account.qld.gov.au/help/faq.html#howDoIProvide100PointsOfIdentification> and (MyMinesOnline) <http://www.business.qld.gov.au/industries/mining-energy-water/resources/minerals-coal/online-services/myminesonline/register>" ;
    rdfs:isDefinedBy cs: ;
    skos:definition "A conditional permit granted to a foreign national by the Australian Government conveying rights of entry, residence, or work within the country."@en ;
    skos:inScheme cs: ;
    skos:prefLabel "Australian visa"@en ;
    skos:topConceptOf cs: ;
.

id:bank-card
    a skos:Concept ;
    skos:historyNote "Compiled by the Geological Survey of Queensland. From (QGOV)<http://account.qld.gov.au/help/faq.html#howDoIProvide100PointsOfIdentification> and (MyMinesOnline) <http://www.business.qld.gov.au/industries/mining-energy-water/resources/minerals-coal/online-services/myminesonline/register>" ;
    rdfs:isDefinedBy cs: ;
    skos:altLabel
        "Bank passbook"@en ,
        "Credit Card"@en ,
        "Credit card, bank card or bank passbook"@en ;
    skos:definition "A card issued by a financial institution for the purpose of identity and account access."@en ;
    skos:inScheme cs: ;
    skos:prefLabel "Bank Card"@en ;
    skos:topConceptOf cs: ;
.

id:birth-certificate
    a skos:Concept ;
    skos:historyNote "Compiled by the Geological Survey of Queensland. From (QGOV)<http://account.qld.gov.au/help/faq.html#howDoIProvide100PointsOfIdentification> and (MyMinesOnline) <http://www.business.qld.gov.au/industries/mining-energy-water/resources/minerals-coal/online-services/myminesonline/register>" ;
    rdfs:isDefinedBy cs: ;
    skos:definition "A vital record that documents the birth of a child. Birth certificates may be the original document certifying the circumstances of the birth or to a certified copy or representation of the ensuing registration of that birth. "@en ;
    skos:inScheme cs: ;
    skos:prefLabel "Birth certificate"@en ;
    skos:topConceptOf cs: ;
.

id:centrelink-card
    a skos:Concept ;
    skos:historyNote "Compiled by the Geological Survey of Queensland. From (QGOV)<http://account.qld.gov.au/help/faq.html#howDoIProvide100PointsOfIdentification> and (MyMinesOnline) <http://www.business.qld.gov.au/industries/mining-energy-water/resources/minerals-coal/online-services/myminesonline/register>" ;
    rdfs:isDefinedBy cs: ;
    skos:definition "A card issued by the Australian social security agency Centrelink."@en ;
    skos:inScheme cs: ;
    skos:prefLabel "Centrelink card"@en ;
    skos:topConceptOf cs: ;
.

id:certificate-of-australian-citizenship
    a skos:Concept ;
    skos:historyNote "Compiled by the Geological Survey of Queensland. From (QGOV)<http://account.qld.gov.au/help/faq.html#howDoIProvide100PointsOfIdentification> and (MyMinesOnline) <http://www.business.qld.gov.au/industries/mining-energy-water/resources/minerals-coal/online-services/myminesonline/register>" ;
    rdfs:isDefinedBy cs: ;
    skos:definition "An Australian citizenship certificate is an official document issued by the Australian Government that shows that a person is an Australian."@en ;
    skos:inScheme cs: ;
    skos:prefLabel "Certificate of Australian citizenship"@en ;
    skos:topConceptOf cs: ;
.

id:council-rates-notice
    a skos:Concept ;
    skos:historyNote "Compiled by the Geological Survey of Queensland. From (QGOV)<http://account.qld.gov.au/help/faq.html#howDoIProvide100PointsOfIdentification> and (MyMinesOnline) <http://www.business.qld.gov.au/industries/mining-energy-water/resources/minerals-coal/online-services/myminesonline/register>" ;
    rdfs:isDefinedBy cs: ;
    skos:definition "A notice of council rates addressed to the owner of a property in Queensland."@en ;
    skos:inScheme cs: ;
    skos:prefLabel "Council rates notice"@en ;
    skos:topConceptOf cs: ;
.

id:electrol-roll-extract
    a skos:Concept ;
    skos:historyNote "Compiled by the Geological Survey of Queensland. From (QGOV)<http://account.qld.gov.au/help/faq.html#howDoIProvide100PointsOfIdentification> and (MyMinesOnline) <http://www.business.qld.gov.au/industries/mining-energy-water/resources/minerals-coal/online-services/myminesonline/register>" ;
    rdfs:isDefinedBy cs: ;
    skos:definition "An extract from the electoral roll administered by the Australian Electoral Commission. "@en ;
    skos:inScheme cs: ;
    skos:prefLabel "Electrol roll extract"@en ;
    skos:topConceptOf cs: ;
.

id:firearms-licence
    a skos:Concept ;
    skos:historyNote "Compiled by the Geological Survey of Queensland. From (QGOV)<http://account.qld.gov.au/help/faq.html#howDoIProvide100PointsOfIdentification> and (MyMinesOnline) <http://www.business.qld.gov.au/industries/mining-energy-water/resources/minerals-coal/online-services/myminesonline/register>" ;
    rdfs:isDefinedBy cs: ;
    skos:definition "A licence issued by the State of Queensland that allows ownership or use of a firearm."@en ;
    skos:inScheme cs: ;
    skos:prefLabel "Firearms licence"@en ;
    skos:topConceptOf cs: ;
.

id:foregin-passport
    a skos:Concept ;
    skos:historyNote "Compiled by the Geological Survey of Queensland. From (QGOV)<http://account.qld.gov.au/help/faq.html#howDoIProvide100PointsOfIdentification> and (MyMinesOnline) <http://www.business.qld.gov.au/industries/mining-energy-water/resources/minerals-coal/online-services/myminesonline/register>" ;
    rdfs:isDefinedBy cs: ;
    skos:definition "A foreign passport is a basic identity document accepted as valid for crossing international borders, issued by a government, other than Australia's, to its citizens. Source: The New Oxford Companion to Law"@en ;
    skos:inScheme cs: ;
    skos:prefLabel "Foregin passport"@en ;
    skos:topConceptOf cs: ;
.

id:letter-from-employer
    a skos:Concept ;
    skos:historyNote "Compiled by the Geological Survey of Queensland. From (QGOV)<http://account.qld.gov.au/help/faq.html#howDoIProvide100PointsOfIdentification> and (MyMinesOnline) <http://www.business.qld.gov.au/industries/mining-energy-water/resources/minerals-coal/online-services/myminesonline/register>" ;
    rdfs:isDefinedBy cs: ;
    skos:definition "A certified letter from the applicants employer."@en ;
    skos:inScheme cs: ;
    skos:prefLabel "Letter from employer"@en ;
    skos:topConceptOf cs: ;
.

id:public-service-photo-id
    a skos:Concept ;
    skos:historyNote "Compiled by the Geological Survey of Queensland. From (QGOV)<http://account.qld.gov.au/help/faq.html#howDoIProvide100PointsOfIdentification> and (MyMinesOnline) <http://www.business.qld.gov.au/industries/mining-energy-water/resources/minerals-coal/online-services/myminesonline/register>" ;
    rdfs:isDefinedBy cs: ;
    skos:altLabel "Government ID"@en ;
    skos:definition "An identification document or card issued by the Australian Government or one of the State or Territory government to a government employee."@en ;
    skos:inScheme cs: ;
    skos:prefLabel "Public service photo ID"@en ;
    skos:topConceptOf cs: ;
.

id:security-guard-licence
    a skos:Concept ;
    skos:historyNote "Compiled by the Geological Survey of Queensland. From (QGOV)<http://account.qld.gov.au/help/faq.html#howDoIProvide100PointsOfIdentification> and (MyMinesOnline) <http://www.business.qld.gov.au/industries/mining-energy-water/resources/minerals-coal/online-services/myminesonline/register>" ;
    rdfs:isDefinedBy cs: ;
    skos:altLabel "Security guard/crowd control licence"@en ;
    skos:definition "A licence issued by the State of Queensland that allows the bearer to perform duties pertaining to security and public safety."@en ;
    skos:inScheme cs: ;
    skos:prefLabel "Security guard licence"@en ;
    skos:topConceptOf cs: ;
.

id:veterans-affairs-card
    a skos:Concept ;
    skos:historyNote "Compiled by the Geological Survey of Queensland. From (QGOV)<http://account.qld.gov.au/help/faq.html#howDoIProvide100PointsOfIdentification> and (MyMinesOnline) <http://www.business.qld.gov.au/industries/mining-energy-water/resources/minerals-coal/online-services/myminesonline/register>" ;
    rdfs:isDefinedBy cs: ;
    skos:altLabel
        "Department of Veterans Affairs card"@en ,
        "Veteran healthcare card"@en ;
    skos:definition "An identity card issued by the Australian Department of Veterans' Affairs that convey a range of benefits upon the bearer."@en ;
    skos:inScheme cs: ;
    skos:prefLabel "Veterans affairs card"@en ;
    skos:topConceptOf cs: ;
.

id:australian-passport
    a skos:Concept ;
    skos:historyNote "Compiled by the Geological Survey of Queensland. From (QGOV)<http://account.qld.gov.au/help/faq.html#howDoIProvide100PointsOfIdentification> and (MyMinesOnline) <http://www.business.qld.gov.au/industries/mining-energy-water/resources/minerals-coal/online-services/myminesonline/register>" ;
    rdfs:isDefinedBy cs: ;
    skos:definition "An Australian passport is a basic identity document accepted as valid for crossing international borders, issued by the Government of Australia to Australian citizens. Source: The New Oxford Companion to Law"@en ;
    skos:inScheme cs: ;
    skos:prefLabel "Australian passport"@en ;
    skos:topConceptOf cs: ;
.

id:change-of-name-certificate
    a skos:Concept ;
    skos:historyNote "Compiled by the Geological Survey of Queensland. From (QGOV)<http://account.qld.gov.au/help/faq.html#howDoIProvide100PointsOfIdentification> and (MyMinesOnline) <http://www.business.qld.gov.au/industries/mining-energy-water/resources/minerals-coal/online-services/myminesonline/register>" ;
    rdfs:isDefinedBy cs: ;
    skos:definition "A document issued by a a governing body registering a change of name."@en ;
    skos:inScheme cs: ;
    skos:prefLabel "Change of name certificate"@en ;
    skos:topConceptOf cs: ;
.

id:drivers-licence
    a skos:Concept ;
    skos:historyNote "Compiled by the Geological Survey of Queensland. From (QGOV)<http://account.qld.gov.au/help/faq.html#howDoIProvide100PointsOfIdentification> and (MyMinesOnline) <http://www.business.qld.gov.au/industries/mining-energy-water/resources/minerals-coal/online-services/myminesonline/register>" ;
    rdfs:isDefinedBy cs: ;
    skos:altLabel
        "Australian Drivers Licence"@en ,
        "Australian Drivers License"@en ,
        "Drivers License"@en ;
    skos:definition "The official permit required for a person to legally drive a motor vehicle in Australia. Issued by the States and Territories of Australia."@en ;
    skos:inScheme cs: ;
    skos:prefLabel "Drivers licence"@en ;
    skos:topConceptOf cs: ;
.

id:marriage-certificate
    a skos:Concept ;
    skos:historyNote "Compiled by the Geological Survey of Queensland. From (QGOV)<http://account.qld.gov.au/help/faq.html#howDoIProvide100PointsOfIdentification> and (MyMinesOnline) <http://www.business.qld.gov.au/industries/mining-energy-water/resources/minerals-coal/online-services/myminesonline/register>" ;
    rdfs:isDefinedBy cs: ;
    skos:definition "An official statement that two people are married. In most jurisdictions, a marriage certificate is issued by a government official only after the civil registration of the marriage. Source:Wikipedia"@en ;
    skos:inScheme cs: ;
    skos:prefLabel "Marriage certificate"@en ;
    skos:topConceptOf cs: ;
.

id:medicare-card
    a skos:Concept ;
    skos:historyNote "Compiled by the Geological Survey of Queensland. From (QGOV)<http://account.qld.gov.au/help/faq.html#howDoIProvide100PointsOfIdentification> and (MyMinesOnline) <http://www.business.qld.gov.au/industries/mining-energy-water/resources/minerals-coal/online-services/myminesonline/register>" ;
    rdfs:isDefinedBy cs: ;
    skos:definition "A card, issued to Australian citizens and permanent residents and their families. The card or the Medicare number enables the cardholder to receive a rebate of medical expenses under Australia's Medicare system, as well as subsidised medications under the Pharmaceutical Benefits Scheme (PBS). Source:Wikipedia"@en ;
    skos:inScheme cs: ;
    skos:prefLabel "Medicare card"@en ;
    skos:topConceptOf cs: ;
.

cs:
    a
        owl:Ontology ,
        skos:ConceptScheme ;
    dcterms:created "2020-03-25"^^xsd:date ;
    dcterms:creator <https://linked.data.gov.au/org/gsq> ;
    dcterms:modified "2023-03-16"^^xsd:date ;
    skos:historyNote "Compiled by the Geological Survey of Queensland. From (QGOV)<http://account.qld.gov.au/help/faq.html#howDoIProvide100PointsOfIdentification> and (MyMinesOnline) <http://www.business.qld.gov.au/industries/mining-energy-water/resources/minerals-coal/online-services/myminesonline/register>" ;
    dcterms:publisher <https://linked.data.gov.au/org/gsq> ;
    reg:status agldwgstatus:stable ;
    skos:definition "Types of Identification documents and numbers used in Queensland as acceptable proof of identity for individuals, businesses, and companies. Required and accepted documents by the QGOV and MyMinesOnline systems."@en ;
    skos:hasTopConcept
        id:abn ,
        id:acn ,
        id:australian-passport ,
        id:australian-university-id-card ,
        id:australian-visa ,
        id:bank-card ,
        id:birth-certificate ,
        id:c-code ,
        id:centrelink-card ,
        id:certificate-of-australian-citizenship ,
        id:change-of-name-certificate ,
        id:council-rates-notice ,
        id:drivers-licence ,
        id:electrol-roll-extract ,
        id:firearms-licence ,
        id:foregin-passport ,
        id:letter-from-employer ,
        id:marriage-certificate ,
        id:medicare-card ,
        id:public-service-photo-id ,
        id:security-guard-licence ,
        id:veterans-affairs-card ;
    skos:prefLabel "Party Identification Type"@en ;
.

