PREFIX agldwgstatus: <https://linked.data.gov.au/def/reg-statuses/>
PREFIX cs: <http://linked.data.gov.au/def/observation-detail-type>
PREFIX dcterms: <http://purl.org/dc/terms/>
PREFIX obsdt: <http://linked.data.gov.au/def/observation-detail-type/>
PREFIX owl: <http://www.w3.org/2002/07/owl#>
PREFIX reg: <http://purl.org/linked-data/registry#>
PREFIX sdo: <https://schema.org/>
PREFIX skos: <http://www.w3.org/2004/02/skos/core#>
PREFIX xsd: <http://www.w3.org/2001/XMLSchema#>

obsdt:airborne-geophysics
    a skos:Collection ;
    dcterms:provenance "Compiled by the Geological Survey of Queensland" ;
    skos:definition "Additional details that describe Airborne Geophysics surveys."@en ;
    skos:member
        obsdt:reading-interval-hz ,
        obsdt:reading-interval-m ,
        obsdt:survey-configuration ;
    skos:prefLabel "Airborne Geophysics"@en ;
.

obsdt:blended
    a skos:Concept ;
    dcterms:provenance "Compiled by the Geological Survey of Queensland" ;
    skos:definition "A true-false flag indicating whether the observation is of a blended sample. In the case of a resource sale this may refer to the blending of material from different sources (i.e. mines) into a single sale volume."@en ;
    skos:inScheme cs: ;
    skos:prefLabel "Blended Sample"@en ;
    skos:topConceptOf cs: ;
.

obsdt:lot-adjacent
    a skos:Concept ;
    dcterms:provenance "Compiled by the Geological Survey of Queensland" ;
    skos:definition "Is a true-false or y/n flag indicating that the lot-on-plan number used to describe a feature is not within the bounds of that parcel, but instead, adjacent to it."@en ;
    skos:inScheme cs: ;
    skos:prefLabel "Lot Adjacent"@en ;
    skos:topConceptOf cs: ;
.

obsdt:lot-number
    a skos:Concept ;
    dcterms:provenance "Compiled by the Geological Survey of Queensland" ;
    skos:definition "The lot number used to describe a cadastral parcel of land. Used in conjunction with the plan number."@en ;
    skos:inScheme cs: ;
    skos:prefLabel "Lot Number"@en ;
    skos:topConceptOf cs: ;
.

obsdt:plan-number
    a skos:Concept ;
    dcterms:provenance "Compiled by the Geological Survey of Queensland" ;
    skos:definition "The plan number used to describe a cadastral parcel of land. Used in conjunction with the lot number."@en ;
    skos:inScheme cs: ;
    skos:prefLabel "Plan Number"@en ;
    skos:topConceptOf cs: ;
.

obsdt:processing-date
    a skos:Concept ;
    dcterms:provenance "Compiled by the Geological Survey of Queensland" ;
    skos:altLabel "Processing End Date"@en ;
    skos:definition "The date, or effective date, of any processing performed on the observed data. The date that processing was completed."@en ;
    skos:inScheme cs: ;
    skos:prefLabel "Processing Date"@en ;
    skos:topConceptOf cs: ;
.

obsdt:software
    a skos:Concept ;
    dcterms:provenance "Compiled by the Geological Survey of Queensland" ;
    skos:altLabel
        "Firmware"@en ,
        "Software Version"@en ;
    skos:definition "The software or firmware used by the instrument for acquisition, or the software used for data processing."@en ;
    skos:inScheme cs: ;
    skos:prefLabel "Software"@en ;
    skos:topConceptOf cs: ;
.

obsdt:reading-interval-hz
    a skos:Concept ;
    dcterms:provenance "Compiled by the Geological Survey of Queensland" ;
    skos:definition "Frequency of readings or observations in Hertz (1/s)"@en ;
    skos:inScheme cs: ;
    skos:prefLabel "Reading Interval (Hz)"@en ;
    skos:topConceptOf cs: ;
.

obsdt:reading-interval-m
    a skos:Concept ;
    dcterms:provenance "Compiled by the Geological Survey of Queensland" ;
    skos:definition "Distance between readings or observations in metres"@en ;
    skos:inScheme cs: ;
    skos:prefLabel "Reading Interval (m)"@en ;
    skos:topConceptOf cs: ;
.

obsdt:survey-configuration
    a skos:Concept ;
    dcterms:provenance "Compiled by the Geological Survey of Queensland" ;
    skos:definition "Additional information about the survey configuration"@en ;
    skos:inScheme cs: ;
    skos:prefLabel "Survey Configuration"@en ;
    skos:topConceptOf cs: ;
.

<https://linked.data.gov.au/org/gsq>
    a sdo:Organization ;
    sdo:name "Geological Survey of Queensland" ;
    sdo:url "http://www.business.qld.gov.au/industries/mining-energy-water/resources/geoscience-information/gsq"^^xsd:anyURI ;
.

cs:
    a
        owl:Ontology ,
        skos:ConceptScheme ;
    dcterms:created "2020-03-30"^^xsd:date ;
    dcterms:creator <https://linked.data.gov.au/org/gsq> ;
    dcterms:modified "2023-03-16"^^xsd:date ;
    dcterms:provenance "Compiled by the Geological Survey of Queensland" ;
    dcterms:publisher <https://linked.data.gov.au/org/gsq> ;
    reg:status agldwgstatus:stable ;
    skos:definition "Miscellaneous details that describe samples that are outside the common core observation profile."@en ;
    skos:hasTopConcept
        obsdt:blended ,
        obsdt:lot-adjacent ,
        obsdt:lot-number ,
        obsdt:plan-number ,
        obsdt:processing-date ,
        obsdt:reading-interval-hz ,
        obsdt:reading-interval-m ,
        obsdt:software ,
        obsdt:survey-configuration ;
    skos:prefLabel "Observation Detail Type"@en ;
.

