PREFIX agldwgstatus: <https://linked.data.gov.au/def/reg-statuses/>
PREFIX cs: <http://linked.data.gov.au/def/organisation-name-types>
PREFIX dcterms: <http://purl.org/dc/terms/>
PREFIX orgnt: <http://linked.data.gov.au/def/organisation-name-types/>
PREFIX owl: <http://www.w3.org/2002/07/owl#>
PREFIX rdfs: <http://www.w3.org/2000/01/rdf-schema#>
PREFIX reg: <http://purl.org/linked-data/registry#>
PREFIX sdo: <https://schema.org/>
PREFIX skos: <http://www.w3.org/2004/02/skos/core#>
PREFIX xsd: <http://www.w3.org/2001/XMLSchema#>

orgnt:legal-organisation-name
    a skos:Concept ;
    dcterms:provenance "Derived from Australian Standard AS 4590.1:2017." ;
    rdfs:isDefinedBy cs: ;
    skos:definition "This is the name of the owner of the organisation that appears on all legal papers (AS4590.1:2017)."@en ;
    skos:inScheme cs: ;
    skos:notation "LGL" ;
    skos:prefLabel "Legal Organisation Name"@en ;
    skos:topConceptOf cs: ;
.

orgnt:main-organisation
    a skos:Concept ;
    dcterms:provenance "Derived from Australian Standard AS 4590.1:2017." ;
    rdfs:isDefinedBy cs: ;
    skos:definition "Main name of the organisation. This is the name of the entity that appears on all official documents or legal papers. May be the registered Business name where it is different to the Trading name (AS4590.1:2017)."@en ;
    skos:inScheme cs: ;
    skos:notation "MN" ;
    skos:prefLabel "Main Organisation"@en ;
    skos:topConceptOf cs: ;
.

orgnt:main-trading-name
    a skos:Concept ;
    dcterms:provenance "Derived from Australian Standard AS 4590.1:2017." ;
    rdfs:isDefinedBy cs: ;
    skos:altLabel "Trading Name"@en ;
    skos:definition "The main name that the organisation trades under or the name by which suppliers or customers know the organisation (AS4590.1:2017)."@en ;
    skos:inScheme cs: ;
    skos:notation "MTR" ;
    skos:prefLabel "Main Trading Name"@en ;
    skos:topConceptOf cs: ;
.

orgnt:management-accounting-unit
    a skos:Concept ;
    dcterms:provenance "Derived from Australian Standard AS 4590.1:2017." ;
    rdfs:isDefinedBy cs: ;
    skos:definition "Management accounting unit. These are principal business units for which regular accounts are maintained, e.g. a division of a large business such as BHP's Steel Division. MAUs are ABS defined but are a popular way for large businesses to manage diverse undertakings (AS4590.1:2017)."@en ;
    skos:inScheme cs: ;
    skos:notation "MAU" ;
    skos:prefLabel "Management Accounting Unit"@en ;
    skos:topConceptOf cs: ;
.

orgnt:other-name
    a skos:Concept ;
    dcterms:provenance "Derived from Australian Standard AS 4590.1:2017." ;
    rdfs:isDefinedBy cs: ;
    skos:definition "Other name type not listed, e.g. sales and marketing  (AS4590.1:2017)."@en ;
    skos:inScheme cs: ;
    skos:notation "OTH" ;
    skos:prefLabel "Other Name"@en ;
    skos:topConceptOf cs: ;
.

orgnt:other-trading-name
    a skos:Concept ;
    dcterms:provenance "Derived from Australian Standard AS 4590.1:2017." ;
    rdfs:isDefinedBy cs: ;
    skos:definition "Alternative trading name for an organisation that is not registered (AS4590.1:2017)."@en ;
    skos:inScheme cs: ;
    skos:notation "OTR" ;
    skos:prefLabel "Other Trading Name"@en ;
    skos:topConceptOf cs: ;
.

orgnt:unknown
    a skos:Concept ;
    dcterms:provenance "Derived from Australian Standard AS 4590.1:2017." ;
    rdfs:isDefinedBy cs: ;
    skos:definition "There is no information about the name type (AS4590.1:2017)."@en ;
    skos:inScheme cs: ;
    skos:notation "UNK" ;
    skos:prefLabel "Unknown"@en ;
    skos:topConceptOf cs: ;
.

<https://linked.data.gov.au/org/gsq>
    a sdo:Organization ;
    sdo:name "Geological Survey of Queensland" ;
    sdo:url "http://www.business.qld.gov.au/industries/mining-energy-water/resources/geoscience-information/gsq"^^xsd:anyURI ;
.

cs:
    a
        owl:Ontology ,
        skos:ConceptScheme ;
    dcterms:created "2020-03-25"^^xsd:date ;
    dcterms:creator <https://linked.data.gov.au/org/gsq> ;
    dcterms:modified "2023-03-16"^^xsd:date ;
    dcterms:provenance "Derived from Australian Standard AS 4590.1:2017." ;
    dcterms:publisher <https://linked.data.gov.au/org/gsq> ;
    reg:status agldwgstatus:stable ;
    skos:definition "Types of names provided by organisations."@en ;
    skos:hasTopConcept
        orgnt:legal-organisation-name ,
        orgnt:main-organisation ,
        orgnt:main-trading-name ,
        orgnt:management-accounting-unit ,
        orgnt:other-name ,
        orgnt:other-trading-name ,
        orgnt:unknown ;
    skos:prefLabel "Organisation Name Types"@en ;
.

