PREFIX agldwgstatus: <https://linked.data.gov.au/def/reg-statuses/>
PREFIX cs: <http://linked.data.gov.au/def/organisation-activity-status>
PREFIX dcterms: <http://purl.org/dc/terms/>
PREFIX oas: <http://linked.data.gov.au/def/organisation-activity-status/>
PREFIX owl: <http://www.w3.org/2002/07/owl#>
PREFIX rdfs: <http://www.w3.org/2000/01/rdf-schema#>
PREFIX reg: <http://purl.org/linked-data/registry#>
PREFIX sdo: <https://schema.org/>
PREFIX skos: <http://www.w3.org/2004/02/skos/core#>
PREFIX xsd: <http://www.w3.org/2001/XMLSchema#>

oas:strike-off-action-in-progress
    a skos:Concept ;
    dcterms:provenance "Derived from Australian Standard AS4590.1:2017 and ASIC." ;
    rdfs:isDefinedBy cs: ;
    skos:definition "The organisation is being removed from the ASIC organisational register."@en ;
    skos:inScheme cs: ;
    skos:notation "SOFF" ;
    skos:prefLabel "Strike off action in progress"@en ;
    skos:topConceptOf cs: ;
.

oas:suspended-trading
    a skos:Concept ;
    dcterms:provenance "Derived from Australian Standard AS4590.1:2017 and ASIC." ;
    rdfs:isDefinedBy cs: ;
    skos:definition "The organisation has suspended trading or has been suspended from trading on an exchange."@en ;
    skos:inScheme cs: ;
    skos:prefLabel "Suspended Trading"@en ;
    skos:topConceptOf cs: ;
.

oas:trading
    a skos:Concept ;
    dcterms:provenance "Derived from Australian Standard AS4590.1:2017 and ASIC." ;
    rdfs:isDefinedBy cs: ;
    skos:definition "The organisation is trading and carrying out business activities."@en ;
    skos:inScheme cs: ;
    skos:prefLabel "Trading"@en ;
    skos:topConceptOf cs: ;
.

oas:under-external-administration-and-or-controller-appointed
    a skos:Concept ;
    dcterms:provenance "Derived from Australian Standard AS4590.1:2017 and ASIC." ;
    rdfs:isDefinedBy cs: ;
    skos:altLabel
        "Controller Appointed" ,
        "Under External Administration" ;
    skos:definition "The organisation is being administered or controlled by a person or persons independent of that organisation."@en ;
    skos:inScheme cs: ;
    skos:notation "EXAD" ;
    skos:prefLabel "Under external administration and/or controller appointed"@en ;
    skos:topConceptOf cs: ;
.

<https://linked.data.gov.au/org/gsq>
    a sdo:Organization ;
    sdo:name "Geological Survey of Queensland" ;
    sdo:url "http://www.business.qld.gov.au/industries/mining-energy-water/resources/geoscience-information/gsq"^^xsd:anyURI ;
.

cs:
    a
        owl:Ontology ,
        skos:ConceptScheme ;
    dcterms:created "2020-03-25"^^xsd:date ;
    dcterms:creator <https://linked.data.gov.au/org/gsq> ;
    dcterms:modified "2023-03-16"^^xsd:date ;
    dcterms:provenance "Derived from Australian Standard AS4590.1:2017 and ASIC." ;
    dcterms:publisher <https://linked.data.gov.au/org/gsq> ;
    reg:status agldwgstatus:stable ;
    skos:definition "Descriptions of the business activity of an organisation at a point in time."@en ;
    skos:hasTopConcept
        oas:strike-off-action-in-progress ,
        oas:suspended-trading ,
        oas:trading ,
        oas:under-external-administration-and-or-controller-appointed ;
    skos:prefLabel "Organisation Activity Status"@en ;
.

