PREFIX agldwgstatus: <https://linked.data.gov.au/def/reg-statuses/>
PREFIX cs: <http://linked.data.gov.au/def/qld-utm-zones>
PREFIX dcterms: <http://purl.org/dc/terms/>
PREFIX owl: <http://www.w3.org/2002/07/owl#>
PREFIX qldutm: <http://linked.data.gov.au/def/qld-utm-zones/>
PREFIX rdfs: <http://www.w3.org/2000/01/rdf-schema#>
PREFIX reg: <http://purl.org/linked-data/registry#>
PREFIX sdo: <https://schema.org/>
PREFIX skos: <http://www.w3.org/2004/02/skos/core#>
PREFIX xsd: <http://www.w3.org/2001/XMLSchema#>

qldutm:z54
    a skos:Concept ;
    dcterms:provenance "Concepts extracted from OGC sources" ;
    rdfs:isDefinedBy cs: ;
    skos:definition "The 54th UTM zone spanning from 138 to 144 degrees of longitude east. Central Meridian 141 degrees east"@en ;
    skos:inScheme cs: ;
    skos:prefLabel "Z54"@en ;
    skos:topConceptOf cs: ;
.

qldutm:z55
    a skos:Concept ;
    dcterms:provenance "Concepts extracted from OGC sources" ;
    rdfs:isDefinedBy cs: ;
    skos:definition "The 55th UTM zone spanning from 144 to 150 degrees of longitude east. Central Meridian 147 degrees east"@en ;
    skos:inScheme cs: ;
    skos:prefLabel "Z55"@en ;
    skos:topConceptOf cs: ;
.

qldutm:z56
    a skos:Concept ;
    dcterms:provenance "Concepts extracted from OGC sources" ;
    rdfs:isDefinedBy cs: ;
    skos:definition "The 56th UTM zone spanning from 150 to 156 degrees of longitude east. Central Meridian 153 degrees east"@en ;
    skos:inScheme cs: ;
    skos:prefLabel "Z56"@en ;
    skos:topConceptOf cs: ;
.

<https://linked.data.gov.au/org/gsq>
    a sdo:Organization ;
    sdo:name "Geological Survey of Queensland" ;
    sdo:url "http://www.business.qld.gov.au/industries/mining-energy-water/resources/geoscience-information/gsq"^^xsd:anyURI ;
.

cs:
    a
        owl:Ontology ,
        skos:ConceptScheme ;
    dcterms:created "2020-01-31T08:40:52"^^xsd:dateTime ;
    dcterms:creator <https://linked.data.gov.au/org/gsq> ;
    dcterms:modified "2023-03-16"^^xsd:date ;
    dcterms:provenance "Concepts extracted from OGC sources" ;
    dcterms:publisher <https://linked.data.gov.au/org/gsq> ;
    reg:status agldwgstatus:stable ;
    skos:definition "The universal transverse mercator (UTM) zones used and referred to within Queensland. The UTM system divides the Earth into 60 zones, each 6 degrees of longitude in width. Zone 1 covers longitude 180 to 174 W; zone numbering increases eastward to zone 60, which covers longitude 174 to 180E. The polar regions south of 80S and north of 84N are excluded."@en ;
    skos:hasTopConcept
        qldutm:z54 ,
        qldutm:z55 ,
        qldutm:z56 ;
    skos:prefLabel "QLD UTM Zones"@en ;
.

