PREFIX agldwgstatus: <https://linked.data.gov.au/def/reg-statuses/>
PREFIX cs: <http://linked.data.gov.au/def/queensland-crs>
PREFIX dcterms: <http://purl.org/dc/terms/>
PREFIX owl: <http://www.w3.org/2002/07/owl#>
PREFIX qldcrs: <http://linked.data.gov.au/def/queensland-crs/>
PREFIX rdfs: <http://www.w3.org/2000/01/rdf-schema#>
PREFIX reg: <http://purl.org/linked-data/registry#>
PREFIX sdo: <https://schema.org/>
PREFIX skos: <http://www.w3.org/2004/02/skos/core#>
PREFIX xsd: <http://www.w3.org/2001/XMLSchema#>

qldcrs:geographic
    a skos:Collection ;
    skos:historyNote "Compiled by the Geological Survey of Queensland" ;
    skos:definition "A geographic coordinate system (GCS) is a coordinate system which uses a three-dimensional spherical surface (ellipsoid) to define locations on the earth. A common choice of coordinates is latitude and longitude."@en ;
    skos:member
        qldcrs:agd1966 ,
        qldcrs:agd1984 ,
        qldcrs:gda1994 ,
        qldcrs:gda2020 ,
        qldcrs:wgs1984 ;
    skos:prefLabel "Geographic Coordinate Systems"@en ;
.

qldcrs:projected
    a skos:Collection ;
    skos:historyNote "Compiled by the Geological Survey of Queensland" ;
    skos:definition "A projected coordinate system (PCS) is a projection of the geographic coordinate to, on two-dimensional surface (the map). The used to convert between Australian Geodetic Data and their Projected equivalents is the Universal Transverse Mercator projection."@en ;
    skos:member
        qldcrs:amg1966-z54 ,
        qldcrs:amg1966-z55 ,
        qldcrs:amg1966-z56 ,
        qldcrs:amg1984-z54 ,
        qldcrs:amg1984-z55 ,
        qldcrs:amg1984-z56 ,
        qldcrs:mga1994-z54 ,
        qldcrs:mga1994-z55 ,
        qldcrs:mga1994-z56 ,
        qldcrs:mga2020-z54 ,
        qldcrs:mga2020-z55 ,
        qldcrs:mga2020-z56 ;
    skos:prefLabel "Projected Coordinate Systems"@en ;
.

qldcrs:agd1966
    a skos:Concept ;
    skos:historyNote "Compiled by the Geological Survey of Queensland" ;
    rdfs:isDefinedBy cs: ;
    skos:altLabel "Australian Geodetic Datum 1966"@en ;
    skos:definition "The first official national Australian geodetic datum proclaimed in the Australian Commonwealth Gazette No. 84 of 6 October 1966."@en ;
    skos:inScheme cs: ;
    skos:notation "4202" ;
    skos:prefLabel "AGD66"@en ;
    skos:topConceptOf cs: ;
.

qldcrs:agd1984
    a skos:Concept ;
    skos:historyNote "Compiled by the Geological Survey of Queensland" ;
    rdfs:isDefinedBy cs: ;
    skos:altLabel "Australian Geodetic Datum 1984"@en ;
    skos:definition "The update to the official Australian geodetic datum, adopted and in effect from 1984"@en ;
    skos:inScheme cs: ;
    skos:notation "4203" ;
    skos:prefLabel "AGD84"@en ;
    skos:topConceptOf cs: ;
.

qldcrs:amg1966-z54
    a skos:Concept ;
    skos:historyNote "Compiled by the Geological Survey of Queensland" ;
    rdfs:isDefinedBy cs: ;
    skos:altLabel "Australian Map Grid 1966 zone 54"@en ;
    skos:definition "The accompanying national map projection to AGD66, a transverse Mercator projection that conforms to zone 54 of the internationally accepted Universal Transverse Mercator Grid system."@en ;
    skos:inScheme cs: ;
    skos:notation "20254" ;
    skos:prefLabel "AMG66 z54"@en ;
    skos:topConceptOf cs: ;
.

qldcrs:amg1966-z55
    a skos:Concept ;
    skos:historyNote "Compiled by the Geological Survey of Queensland" ;
    rdfs:isDefinedBy cs: ;
    skos:altLabel "Australian Map Grid 1966 zone 55"@en ;
    skos:definition "The accompanying national map projection to AGD66, a transverse Mercator projection that conforms to zone 55 of the internationally accepted Universal Transverse Mercator Grid system."@en ;
    skos:inScheme cs: ;
    skos:notation "20255" ;
    skos:prefLabel "AMG66 z55"@en ;
    skos:topConceptOf cs: ;
.

qldcrs:amg1966-z56
    a skos:Concept ;
    skos:historyNote "Compiled by the Geological Survey of Queensland" ;
    rdfs:isDefinedBy cs: ;
    skos:altLabel "Australian Map Grid 1966 zone 56"@en ;
    skos:definition "The accompanying national map projection to AGD66, a transverse Mercator projection that conforms to zone 56 of the internationally accepted Universal Transverse Mercator Grid system."@en ;
    skos:inScheme cs: ;
    skos:notation "20256" ;
    skos:prefLabel "AMG66 z56"@en ;
    skos:topConceptOf cs: ;
.

qldcrs:amg1984-z54
    a skos:Concept ;
    skos:historyNote "Compiled by the Geological Survey of Queensland" ;
    rdfs:isDefinedBy cs: ;
    skos:altLabel "Australian Map Grid 1984 zone 54"@en ;
    skos:definition "The accompanying national map projection to AGD84, a transverse Mercator projection that conforms to zone 54 of the internationally accepted Universal Transverse Mercator Grid system."@en ;
    skos:inScheme cs: ;
    skos:notation "20354" ;
    skos:prefLabel "AMG84 z54"@en ;
    skos:topConceptOf cs: ;
.

qldcrs:amg1984-z55
    a skos:Concept ;
    skos:historyNote "Compiled by the Geological Survey of Queensland" ;
    rdfs:isDefinedBy cs: ;
    skos:altLabel "Australian Map Grid 1984 zone 55"@en ;
    skos:definition "The accompanying national map projection to AGD84, a transverse Mercator projection that conforms to zone 55 of the internationally accepted Universal Transverse Mercator Grid system."@en ;
    skos:inScheme cs: ;
    skos:notation "20355" ;
    skos:prefLabel "AMG84 z55"@en ;
    skos:topConceptOf cs: ;
.

qldcrs:amg1984-z56
    a skos:Concept ;
    skos:historyNote "Compiled by the Geological Survey of Queensland" ;
    rdfs:isDefinedBy cs: ;
    skos:altLabel "Australian Map Grid 1984 zone 56"@en ;
    skos:definition "The accompanying national map projection to AGD84, a transverse Mercator projection that conforms to zone 56 of the internationally accepted Universal Transverse Mercator Grid system."@en ;
    skos:inScheme cs: ;
    skos:notation "20356" ;
    skos:prefLabel "AMG84 z56"@en ;
    skos:topConceptOf cs: ;
.

qldcrs:gda1994
    a skos:Concept ;
    skos:historyNote "Compiled by the Geological Survey of Queensland" ;
    rdfs:isDefinedBy cs: ;
    skos:altLabel "Geocentric Datum of Australia 1994"@en ;
    skos:definition "The official geodetic datum adopted nationally in January 2000. GDA94 is a coordinate reference system whose origin coincides with a determination of the centre of mass of the earth, hence the term geocentric. GDA94 is a plate-fixed or static coordinate datum based on the International Terrestrial Reference Frame 1992 (ITRF92), held at the reference epoch of 1 January 1994."@en ;
    skos:inScheme cs: ;
    skos:notation "4283" ;
    skos:prefLabel "GDA94"@en ;
    skos:topConceptOf cs: ;
.

qldcrs:gda2020
    a skos:Concept ;
    skos:historyNote "Compiled by the Geological Survey of Queensland" ;
    rdfs:isDefinedBy cs: ;
    skos:altLabel "Geocentric Datum of Australia 2020"@en ;
    skos:definition "The official geodetic datum adopted nationally in June 2020. GDA2020 is a coordinate reference system whose origin coincides with a determination of the centre of mass of the earth, hence the term geocentric. GDA2020 is a plate-fixed or static coordinate datum based on the International Terrestrial Reference Frame 1992 (ITRF92), held at the reference epoch of 1 January 2020."@en ;
    skos:inScheme cs: ;
    skos:notation "7844" ;
    skos:prefLabel "GDA2020"@en ;
    skos:topConceptOf cs: ;
.

qldcrs:mga1994-z54
    a skos:Concept ;
    skos:historyNote "Compiled by the Geological Survey of Queensland" ;
    rdfs:isDefinedBy cs: ;
    skos:altLabel "Map Grid of Australia 1994 zone 54"@en ;
    skos:definition "The accompanying national map projection to GDA94, a transverse Mercator projection that conforms to zone 54 of the internationally accepted Universal Transverse Mercator Grid system."@en ;
    skos:inScheme cs: ;
    skos:notation "28354" ;
    skos:prefLabel "MGA94 z54"@en ;
    skos:topConceptOf cs: ;
.

qldcrs:mga1994-z55
    a skos:Concept ;
    skos:historyNote "Compiled by the Geological Survey of Queensland" ;
    rdfs:isDefinedBy cs: ;
    skos:altLabel "Map Grid of Australia 1994 zone 55"@en ;
    skos:definition "The accompanying national map projection to GDA94, a transverse Mercator projection that conforms to zone 55 of the internationally accepted Universal Transverse Mercator Grid system."@en ;
    skos:inScheme cs: ;
    skos:notation "28355" ;
    skos:prefLabel "MGA94 z55"@en ;
    skos:topConceptOf cs: ;
.

qldcrs:mga1994-z56
    a skos:Concept ;
    skos:historyNote "Compiled by the Geological Survey of Queensland" ;
    rdfs:isDefinedBy cs: ;
    skos:altLabel "Map Grid of Australia 1994 zone 56"@en ;
    skos:definition "The accompanying national map projection to GDA94, a transverse Mercator projection that conforms to zone 56 of the internationally accepted Universal Transverse Mercator Grid system."@en ;
    skos:inScheme cs: ;
    skos:notation "28356" ;
    skos:prefLabel "MGA94 z56"@en ;
    skos:topConceptOf cs: ;
.

qldcrs:mga2020-z54
    a skos:Concept ;
    skos:historyNote "Compiled by the Geological Survey of Queensland" ;
    rdfs:isDefinedBy cs: ;
    skos:altLabel "Map Grid of Australia 2020 zone 54"@en ;
    skos:definition "The accompanying national map projection to GDA2020, a transverse Mercator projection that conforms to zone 54 of the internationally accepted Universal Transverse Mercator Grid system."@en ;
    skos:inScheme cs: ;
    skos:notation "7854" ;
    skos:prefLabel "MGA2020 z54"@en ;
    skos:topConceptOf cs: ;
.

qldcrs:mga2020-z55
    a skos:Concept ;
    skos:historyNote "Compiled by the Geological Survey of Queensland" ;
    rdfs:isDefinedBy cs: ;
    skos:altLabel "Map Grid of Australia 2020 zone 55"@en ;
    skos:definition "The accompanying national map projection to GDA2020, a transverse Mercator projection that conforms to zone 55 of the internationally accepted Universal Transverse Mercator Grid system."@en ;
    skos:inScheme cs: ;
    skos:notation "7855" ;
    skos:prefLabel "MGA2020 z55"@en ;
    skos:topConceptOf cs: ;
.

qldcrs:mga2020-z56
    a skos:Concept ;
    skos:historyNote "Compiled by the Geological Survey of Queensland" ;
    rdfs:isDefinedBy cs: ;
    skos:altLabel "Map Grid of Australia 2020 zone 56"@en ;
    skos:definition "The accompanying national map projection to GDA2020, a transverse Mercator projection that conforms to zone 56 of the internationally accepted Universal Transverse Mercator Grid system."@en ;
    skos:inScheme cs: ;
    skos:notation "7856" ;
    skos:prefLabel "MGA2020 z56"@en ;
    skos:topConceptOf cs: ;
.

qldcrs:wgs1984
    a skos:Concept ;
    skos:historyNote "Compiled by the Geological Survey of Queensland" ;
    rdfs:isDefinedBy cs: ;
    skos:altLabel "World Geodetic System 1984"@en ;
    skos:definition "The official world geodetic datum adopted in 1984. WGS84 is a coordinate reference system whose origin coincides with a determination of the centre of mass of the earth. The datum defines meridan 0 as IERS Reference Meridian and the datum surface is an oblate spheroid."@en ;
    skos:inScheme cs: ;
    skos:notation "4326" ;
    skos:prefLabel "WGS84"@en ;
    skos:topConceptOf cs: ;
.

<https://linked.data.gov.au/org/gsq>
    a sdo:Organization ;
    sdo:name "Geological Survey of Queensland" ;
    sdo:url "http://www.business.qld.gov.au/industries/mining-energy-water/resources/geoscience-information/gsq"^^xsd:anyURI ;
.

cs:
    a
        owl:Ontology ,
        skos:ConceptScheme ;
    dcterms:created "2020-01-30T15:57:41"^^xsd:dateTime ;
    dcterms:creator <https://linked.data.gov.au/org/gsq> ;
    dcterms:modified "2023-03-16"^^xsd:date ;
    skos:historyNote "Compiled by the Geological Survey of Queensland" ;
    dcterms:publisher <https://linked.data.gov.au/org/gsq> ;
    reg:status agldwgstatus:stable ;
    skos:definition "The coordinate reference systems used and referred to within Queensland."@en ;
    skos:hasTopConcept
        qldcrs:agd1966 ,
        qldcrs:agd1984 ,
        qldcrs:amg1966-z54 ,
        qldcrs:amg1966-z55 ,
        qldcrs:amg1966-z56 ,
        qldcrs:amg1984-z54 ,
        qldcrs:amg1984-z55 ,
        qldcrs:amg1984-z56 ,
        qldcrs:gda1994 ,
        qldcrs:gda2020 ,
        qldcrs:mga1994-z54 ,
        qldcrs:mga1994-z55 ,
        qldcrs:mga1994-z56 ,
        qldcrs:mga2020-z54 ,
        qldcrs:mga2020-z55 ,
        qldcrs:mga2020-z56 ,
        qldcrs:wgs1984 ;
    skos:prefLabel "Queensland CRS"@en ;
.

