PREFIX agldwgstatus: <https://linked.data.gov.au/def/reg-statuses/>
PREFIX cs: <http://linked.data.gov.au/def/iso11179-6/RolesAndResponsibilities>
PREFIX dcterms: <http://purl.org/dc/terms/>
PREFIX iso11179: <http://linked.data.gov.au/def/iso11179-6/RolesAndResponsibilities/>
PREFIX owl: <http://www.w3.org/2002/07/owl#>
PREFIX rdfs: <http://www.w3.org/2000/01/rdf-schema#>
PREFIX reg: <http://purl.org/linked-data/registry#>
PREFIX sdo: <https://schema.org/>
PREFIX skos: <http://www.w3.org/2004/02/skos/core#>
PREFIX xsd: <http://www.w3.org/2001/XMLSchema#>

iso11179:AllOthers
    a skos:Concept ;
    dcterms:provenance "ISO/IEC 11179-6 Information technology - Metadata registries (MDR) - Part 6: Registration, Annex C" ;
    rdfs:isDefinedBy cs: ;
    skos:definition "A Registration Authority may establish guidelines on the use of their Metadata Registry by other users. The general goal should be to provide an open area that anyone may use to obtain and explore the metadata that is managed within the Metadata Registry."@en ;
    skos:inScheme cs: ;
    skos:prefLabel "All others"@en ;
    skos:topConceptOf cs: ;
.

iso11179:ControlCommittee
    a skos:Concept ;
    dcterms:provenance "ISO/IEC 11179-6 Information technology - Metadata registries (MDR) - Part 6: Registration, Annex C" ;
    rdfs:isDefinedBy cs: ;
    skos:definition "The Control Committee should be the organizational unit of the Registration Authority that is constituted to provide technical direction and harmonization of Administered Items for the metadata register. The structure, staffing, procedures, and membership of the Control Committee are determined by the Registration Authority. The membership of the Control Committee may include Registrars and Stewards."@en ;
    skos:inScheme cs: ;
    skos:prefLabel "Control Committee"@en ;
    skos:topConceptOf cs: ;
.

iso11179:ExecutiveCommittee
    a skos:Concept ;
    dcterms:provenance "ISO/IEC 11179-6 Information technology - Metadata registries (MDR) - Part 6: Registration, Annex C" ;
    rdfs:isDefinedBy cs: ;
    skos:definition "The Executive Committee should be an organizational unit established by the Registration Authority. It should be responsible for administering responsibilities and authority delegated by the Registration Authority. Responsibilities of the Executive Committee should include overall metadata registration policies and business direction of the Metadata Registry."@en ;
    skos:inScheme cs: ;
    skos:prefLabel "Executive Committee"@en ;
    skos:topConceptOf cs: ;
.

iso11179:OverallRegistrationAuthority
    a skos:Concept ;
    dcterms:provenance "ISO/IEC 11179-6 Information technology - Metadata registries (MDR) - Part 6: Registration, Annex C" ;
    rdfs:isDefinedBy cs: ;
    skos:definition "The Metadata Registry Registration Authority should be an organizational unit that desires to operate and manage a Metadata Registry based upon the ISO/IEC 11179 Metadata Registry standard. It is envisioned that any organization wishing to become a Registration Authority and establish a Metadata Registry for the purpose of registering Administered Items may do so. A Registration Authority should: Establish and publish procedures for the operation of its Metadata Registry; receive and process proposals from Submitting Organizations for registration of Administered Items falling within its registration domain; and be responsible for maintaining the metadata register of Administered Items and issuing of international registration data identifiers (IRDIs)."@en ;
    skos:inScheme cs: ;
    skos:prefLabel "Overall Registration Authority"@en ;
    skos:topConceptOf cs: ;
.

iso11179:OverallResponsibleOrganization
    a skos:Concept ;
    dcterms:provenance "ISO/IEC 11179-6 Information technology - Metadata registries (MDR) - Part 6: Registration, Annex C" ;
    rdfs:isDefinedBy cs: ;
    skos:definition "Responsible Organizations are usually designated by an organizational unit to ensure consistency of related Administered Items managed by its Submitting Organizations. In the absence of a designated Responsible Organization, a Submitting Organization should act as a Responsible Organization. A Responsible Organization is: The organization, or part thereof, that is responsible for the integrity and accuracy of the attributes values of the Administered Item, e.g., the semantics of Administered Items maintained and controlled by a Registration Authority; the subject-matter expert for the Administered Item; the Organization, at the request of the Registration Authority, that should review proposals from Submitting Organizations on relevant attributes, e.g., name, definition, and permissible values for the attributes of the Administered Item; and the Organization that should inform the Registration Authority of any essential modifications in the specification of the assigned Administered Items."@en ;
    skos:inScheme cs: ;
    skos:prefLabel "Overall Responsible Organization"@en ;
    skos:topConceptOf cs: ;
.

iso11179:OverallSubmittingOrganization
    a skos:Concept ;
    dcterms:provenance "ISO/IEC 11179-6 Information technology - Metadata registries (MDR) - Part 6: Registration, Annex C" ;
    rdfs:isDefinedBy cs: ;
    skos:definition "All Submitting Organizations wishing to register Administered Items should be able to do so in accordance with the procedures prescribed in this part of ISO/IEC 11179 and the procedures established by the Registration Authority. Each Registration Authority may establish its own criteria for registration eligibility. A Submitting Organization wishing to register an Administered Item should follow the procedures and requirements prescribed in this part of ISO/IEC 11179 and in and the procedures established by the Registration Authority for submission to the appropriate Registration Authority."@en ;
    skos:inScheme cs: ;
    skos:prefLabel "Overall Submitting Organization"@en ;
    skos:topConceptOf cs: ;
.

iso11179:ReadOnlyUser
    a skos:Concept ;
    dcterms:provenance "ISO/IEC 11179-6 Information technology - Metadata registries (MDR) - Part 6: Registration, Annex C" ;
    rdfs:isDefinedBy cs: ;
    skos:definition "A Read-only User should be an organizational unit or individual that is approved to review the contents of the metadata register. A read-only user has access to the contents in the metadata register, but is not permitted to submit, alter, or delete contents."@en ;
    skos:inScheme cs: ;
    skos:prefLabel "Read-only user"@en ;
    skos:topConceptOf cs: ;
.

iso11179:Registrar
    a skos:Concept ;
    dcterms:provenance "ISO/IEC 11179-6 Information technology - Metadata registries (MDR) - Part 6: Registration, Annex C" ;
    rdfs:isDefinedBy cs: ;
    skos:definition "The Registrar should be an organizational unit within the Registration Authority, expert in registration processes, responsible for facilitating the registration of Administered Items and making those Administered Items widely accessible and available to the community. The Registrar may be viewed as the contact for the Registration Authority. The Registration Authority should appoint the Registrar."@en ;
    skos:inScheme cs: ;
    skos:prefLabel "Registrar"@en ;
    skos:topConceptOf cs: ;
.

iso11179:Steward
    a skos:Concept ;
    dcterms:provenance "ISO/IEC 11179-6 Information technology - Metadata registries (MDR) - Part 6: Registration, Annex C" ;
    rdfs:isDefinedBy cs: ;
    skos:definition "A Steward shall be an organizational unit of the Metadata Registry community. Stewards should be responsible for the accuracy, reliability, and currency of descriptive metadata for Administered Items at a registration status level of â€œQualifiedâ€ or above within an assigned area. A process defined by the Registration Authority approves stewards. Stewards should be responsible for metadata within specific areas and may have responsibilities that cut across multiple areas (e.g., value domains such as date, time, location, codes of the Countries of the World). The Steward can be viewed as a contact for the Responsible Organization."@en ;
    skos:inScheme cs: ;
    skos:prefLabel "Steward"@en ;
    skos:topConceptOf cs: ;
.

iso11179:Submitter
    a skos:Concept ;
    dcterms:provenance "ISO/IEC 11179-6 Information technology - Metadata registries (MDR) - Part 6: Registration, Annex C" ;
    rdfs:isDefinedBy cs: ;
    skos:definition "A Submitter should be an organizational unit approved by a process defined by the Registration Authority. A Submitter is authorized to identify and report Administered Items suitable for registration. The Submitter can be viewed as a contact for the Submitting Organization."@en ;
    skos:inScheme cs: ;
    skos:prefLabel "Submitter"@en ;
    skos:topConceptOf cs: ;
.

<https://linked.data.gov.au/org/gsq>
    a sdo:Organization ;
    sdo:name "Geological Survey of Queensland" ;
    sdo:url "http://www.business.qld.gov.au/industries/mining-energy-water/resources/geoscience-information/gsq"^^xsd:anyURI ;
.

<https://linked.data.gov.au/org/iso>
    a sdo:Organization ;
    sdo:name "International Organization for Standardization" ;
    sdo:url "http://www.iso.org"^^xsd:anyURI ;
.

cs:
    a
        owl:Ontology ,
        skos:ConceptScheme ;
    dcterms:contributor <https://orcid.org/0000-0002-8742-7730> ;
    dcterms:created "2019-10-17"^^xsd:date ;
    dcterms:creator <https://linked.data.gov.au/org/iso> ;
    dcterms:modified "2023-03-16"^^xsd:date ;
    dcterms:provenance "ISO/IEC 11179-6 Information technology - Metadata registries (MDR) - Part 6: Registration, Annex C" ;
    dcterms:publisher <https://linked.data.gov.au/org/gsq> ;
    reg:status agldwgstatus:stable ;
    skos:definition "A SKOS version of the ISO 11179 Annex C Roles and Responsibilities. Organizational roles associated with Administered Item registration processes. The organizational roles specified are Registration Authority, Registrar, Stewards, Submitters, and Read-only users."@en ;
    skos:hasTopConcept
        iso11179:AllOthers ,
        iso11179:ControlCommittee ,
        iso11179:ExecutiveCommittee ,
        iso11179:OverallRegistrationAuthority ,
        iso11179:OverallResponsibleOrganization ,
        iso11179:OverallSubmittingOrganization ,
        iso11179:ReadOnlyUser ,
        iso11179:Registrar ,
        iso11179:Steward ,
        iso11179:Submitter ;
    skos:prefLabel "ISO/IEC 11179-6 Roles and Responsibilities"@en ;
.

