PREFIX agldwgstatus: <https://linked.data.gov.au/def/reg-statuses/>
PREFIX cs: <http://linked.data.gov.au/def/report-detail-type>
PREFIX dcterms: <http://purl.org/dc/terms/>
PREFIX owl: <http://www.w3.org/2002/07/owl#>
PREFIX rdfs: <http://www.w3.org/2000/01/rdf-schema#>
PREFIX reg: <http://purl.org/linked-data/registry#>
PREFIX rptdt: <http://linked.data.gov.au/def/report-detail-type/>
PREFIX sdo: <https://schema.org/>
PREFIX skos: <http://www.w3.org/2004/02/skos/core#>
PREFIX xsd: <http://www.w3.org/2001/XMLSchema#>

rptdt:activities
    a skos:Concept ;
    dcterms:provenance "Compiled by the Geological Survey of Queensland" ;
    rdfs:isDefinedBy cs: ;
    skos:altLabel
        "Activities Undertaken"@en ,
        "Activities to be Undertaken"@en ,
        "Plan"@en ,
        "Planned Activities"@en ;
    skos:definition "A description of the activities referred to in the report or form. This may be a summary of activities undertaken, or a summary of planned activities."@en ;
    skos:inScheme cs: ;
    skos:prefLabel "Activities"@en ;
    skos:topConceptOf cs: ;
.

rptdt:address
    a skos:Concept ;
    dcterms:provenance "Compiled by the Geological Survey of Queensland" ;
    rdfs:isDefinedBy cs: ;
    skos:definition "The address of the company submitting the report or form."@en ;
    skos:inScheme cs: ;
    skos:prefLabel "Address"@en ;
    skos:topConceptOf cs: ;
.

rptdt:comments
    a skos:Concept ;
    dcterms:provenance "Compiled by the Geological Survey of Queensland" ;
    rdfs:isDefinedBy cs: ;
    skos:altLabel
        "Description"@en ,
        "Remarks"@en ,
        "Summary"@en ;
    skos:definition "Any general commentary regarding the report or form, not otherwise captured."@en ;
    skos:inScheme cs: ;
    skos:prefLabel "Comments"@en ;
    skos:topConceptOf cs: ;
.

rptdt:contact
    a skos:Concept ;
    dcterms:provenance "Compiled by the Geological Survey of Queensland" ;
    rdfs:isDefinedBy cs: ;
    skos:definition "The name of the individual contact for the report or form."@en ;
    skos:inScheme cs: ;
    skos:prefLabel "Contact Name"@en ;
    skos:topConceptOf cs: ;
.

rptdt:contracting-company
    a skos:Concept ;
    dcterms:provenance "Compiled by the Geological Survey of Queensland" ;
    rdfs:isDefinedBy cs: ;
    skos:definition "The name of the company who conducted the activities referred to in the report or form."@en ;
    skos:inScheme cs: ;
    skos:prefLabel "Contractor Name"@en ;
    skos:topConceptOf cs: ;
.

rptdt:email
    a skos:Concept ;
    dcterms:provenance "Compiled by the Geological Survey of Queensland" ;
    rdfs:isDefinedBy cs: ;
    skos:definition "The contact email address for the submitter of the report or form."@en ;
    skos:inScheme cs: ;
    skos:prefLabel "E-mail"@en ;
    skos:topConceptOf cs: ;
.

rptdt:operating-company
    a skos:Concept ;
    dcterms:provenance "Compiled by the Geological Survey of Queensland" ;
    rdfs:isDefinedBy cs: ;
    skos:definition "The name of the company submitting the report or form."@en ;
    skos:inScheme cs: ;
    skos:prefLabel "Company Name"@en ;
    skos:topConceptOf cs: ;
.

rptdt:phone
    a skos:Concept ;
    dcterms:provenance "Compiled by the Geological Survey of Queensland" ;
    rdfs:isDefinedBy cs: ;
    skos:definition "The contact phone number for the submitter of the report or form."@en ;
    skos:inScheme cs: ;
    skos:prefLabel "Phone Number"@en ;
    skos:topConceptOf cs: ;
.

rptdt:postcode
    a skos:Concept ;
    dcterms:provenance "Compiled by the Geological Survey of Queensland" ;
    rdfs:isDefinedBy cs: ;
    skos:definition "The contact postcode for the submitter of the report or form."@en ;
    skos:inScheme cs: ;
    skos:prefLabel "Postcode"@en ;
    skos:topConceptOf cs: ;
.

rptdt:project-name
    a skos:Concept ;
    dcterms:provenance "Compiled by the Geological Survey of Queensland" ;
    rdfs:isDefinedBy cs: ;
    skos:definition "The name of the project to which a report relates."@en ;
    skos:inScheme cs: ;
    skos:prefLabel "Project Name"@en ;
    skos:topConceptOf cs: ;
.

rptdt:reportable-incident
    a skos:Concept ;
    dcterms:provenance "Compiled by the Geological Survey of Queensland" ;
    rdfs:isDefinedBy cs: ;
    skos:definition "An indication of the occurrence of a reportable incident to be recorded in the report or form."@en ;
    skos:inScheme cs: ;
    skos:prefLabel "Reportable Incident"@en ;
    skos:topConceptOf cs: ;
.

rptdt:state
    a skos:Concept ;
    dcterms:provenance "Compiled by the Geological Survey of Queensland" ;
    rdfs:isDefinedBy cs: ;
    skos:definition "The contact State for the submitter of the report or form."@en ;
    skos:inScheme cs: ;
    skos:prefLabel "State"@en ;
    skos:topConceptOf cs: ;
.

rptdt:suburb
    a skos:Concept ;
    dcterms:provenance "Compiled by the Geological Survey of Queensland" ;
    rdfs:isDefinedBy cs: ;
    skos:definition "The contact suburb for the submitter of the report or form."@en ;
    skos:inScheme cs: ;
    skos:prefLabel "Suburb"@en ;
    skos:topConceptOf cs: ;
.

<https://linked.data.gov.au/org/gsq>
    a sdo:Organization ;
    sdo:name "Geological Survey of Queensland" ;
    sdo:url "http://www.business.qld.gov.au/industries/mining-energy-water/resources/geoscience-information/gsq"^^xsd:anyURI ;
.

cs:
    a
        owl:Ontology ,
        skos:ConceptScheme ;
    dcterms:created "2020-04-29"^^xsd:date ;
    dcterms:creator <https://linked.data.gov.au/org/gsq> ;
    dcterms:modified "2023-03-16"^^xsd:date ;
    dcterms:provenance "Compiled by the Geological Survey of Queensland" ;
    dcterms:publisher <https://linked.data.gov.au/org/gsq> ;
    reg:status agldwgstatus:stable ;
    skos:definition "Miscellaneous details relating to reports and documents."@en ;
    skos:hasTopConcept
        rptdt:activities ,
        rptdt:address ,
        rptdt:comments ,
        rptdt:contact ,
        rptdt:contracting-company ,
        rptdt:email ,
        rptdt:operating-company ,
        rptdt:phone ,
        rptdt:postcode ,
        rptdt:project-name ,
        rptdt:reportable-incident ,
        rptdt:state ,
        rptdt:suburb ;
    skos:prefLabel "Report Detail Type"@en ;
.

