PREFIX agldwgstatus: <https://linked.data.gov.au/def/reg-statuses/>
PREFIX cs: <http://linked.data.gov.au/def/result-type>
PREFIX dcterms: <http://purl.org/dc/terms/>
PREFIX owl: <http://www.w3.org/2002/07/owl#>
PREFIX rdfs: <http://www.w3.org/2000/01/rdf-schema#>
PREFIX reg: <http://purl.org/linked-data/registry#>
PREFIX rslt: <http://linked.data.gov.au/def/result-type/>
PREFIX sdo: <https://schema.org/>
PREFIX skos: <http://www.w3.org/2004/02/skos/core#>
PREFIX xsd: <http://www.w3.org/2001/XMLSchema#>

rslt:azimuth
    a skos:Concept ;
    skos:historyNote "Compiled by the Geological Survey of Queensland" ;
    rdfs:isDefinedBy cs: ;
    skos:broader rslt:angle ;
    skos:definition "An angle in the horizontal plane relative to North. By default azimuth is relative to True North, but may also be qualified as relative to Magnetic North or Grid North"@en ;
    skos:inScheme cs: ;
    skos:notation "razi" ;
    skos:prefLabel "Azimuth"@en ;
.

rslt:dip
    a skos:Concept ;
    skos:historyNote "Compiled by the Geological Survey of Queensland" ;
    rdfs:isDefinedBy cs: ;
    skos:broader rslt:angle ;
    skos:definition "An angle in the vertrical plane relative to a horizontal reference. 90 degrees is vertical downwards, 0 degrees horizontal, -90 degrees is vertical upwards."@en ;
    skos:inScheme cs: ;
    skos:notation "rdip" ;
    skos:prefLabel "Dip"@en ;
.

rslt:inclination
    a skos:Concept ;
    skos:historyNote "Compiled by the Geological Survey of Queensland" ;
    rdfs:isDefinedBy cs: ;
    skos:broader rslt:angle ;
    skos:definition "An angle in the vertrical plane relative to a reference vector parallel to the force of gravity, i.e. downwards. 0 degrees is vertical downwards, 90 degrees horizontal, 180 degrees is vertical upwards."@en ;
    skos:inScheme cs: ;
    skos:notation "rinc" ;
    skos:prefLabel "Inclination"@en ;
.

rslt:age
    a skos:Concept ;
    skos:historyNote "Compiled by the Geological Survey of Queensland" ;
    rdfs:isDefinedBy cs: ;
    skos:definition "The time before a reference time. Commonly referenced to time before present (BP), before current era (BCE), or represented as Millions of Years Ago (Ma) in geological disciplines"@en ;
    skos:inScheme cs: ;
    skos:notation "rage" ;
    skos:prefLabel "Age"@en ;
    skos:topConceptOf cs: ;
.

rslt:api-gravity
    a skos:Concept ;
    skos:historyNote "Compiled by the Geological Survey of Queensland" ;
    rdfs:isDefinedBy cs: ;
    skos:altLabel "Oil Gravity"@en ;
    skos:definition "A measure of how heavy or light a petroleum liquid is compared to water: if its API gravity is greater than 10, it is lighter and floats on water; if less than 10, it is heavier and sinks."@en ;
    skos:inScheme cs: ;
    skos:notation "rapi" ;
    skos:prefLabel "API Gravity"@en ;
    skos:topConceptOf cs: ;
.

rslt:area
    a skos:Concept ;
    skos:historyNote "Compiled by the Geological Survey of Queensland" ;
    rdfs:isDefinedBy cs: ;
    skos:definition "The quantity that expresses the extent of a two-dimensional figure or shape or planar lamina, in the plane. Surface area is its analog on the two-dimensional surface of a three-dimensional object."@en ;
    skos:inScheme cs: ;
    skos:notation "rara" ;
    skos:prefLabel "Area"@en ;
    skos:topConceptOf cs: ;
.

rslt:capacitance
    a skos:Concept ;
    skos:historyNote "Compiled by the Geological Survey of Queensland" ;
    rdfs:isDefinedBy cs: ;
    skos:altLabel "Chargeability"@en ;
    skos:definition "The ratio of the change in electric charge of a system, to the corresponding change in its electric potential."@en ;
    skos:inScheme cs: ;
    skos:notation "rcap" ;
    skos:prefLabel "Capacitance"@en ;
    skos:topConceptOf cs: ;
.

rslt:casing-weight
    a skos:Concept ;
    skos:historyNote "Compiled by the Geological Survey of Queensland" ;
    rdfs:isDefinedBy cs: ;
    skos:definition "The mass per unit of length of a length of tubular installed in a borehole."@en ;
    skos:inScheme cs: ;
    skos:notation "rcsw" ;
    skos:prefLabel "Casing Weight"@en ;
    skos:topConceptOf cs: ;
.

rslt:colour
    a skos:Concept ;
    skos:historyNote "Compiled by the Geological Survey of Queensland" ;
    rdfs:isDefinedBy cs: ;
    skos:definition "The qualitative description of the colour of an object."@en ;
    skos:inScheme cs: ;
    skos:notation "rcol" ;
    skos:prefLabel "Colour"@en ;
    skos:topConceptOf cs: ;
.

rslt:composition
    a skos:Concept ;
    skos:historyNote "Compiled by the Geological Survey of Queensland" ;
    rdfs:isDefinedBy cs: ;
    skos:definition "A description of the component parts of a sample or object. Typically given as a component with its percentage or ratio within a bulk sample."@en ;
    skos:inScheme cs: ;
    skos:notation "rcmp" ;
    skos:prefLabel "Composition"@en ;
    skos:topConceptOf cs: ;
.

rslt:compressibility
    a skos:Concept ;
    skos:historyNote "Compiled by the Geological Survey of Queensland" ;
    rdfs:isDefinedBy cs: ;
    skos:definition "A measure of the relative volume change of a fluid or solid as a response to a pressure (or mean stress) change."@en ;
    skos:inScheme cs: ;
    skos:notation "rcpb" ;
    skos:prefLabel "Compressibility"@en ;
    skos:topConceptOf cs: ;
.

rslt:compressive-strength
    a skos:Concept ;
    skos:historyNote "Compiled by the Geological Survey of Queensland" ;
    rdfs:isDefinedBy cs: ;
    skos:definition "The capacity to withstand axially directed pushing forces"@en ;
    skos:inScheme cs: ;
    skos:notation "rcps" ;
    skos:prefLabel "Compressive Strength"@en ;
    skos:topConceptOf cs: ;
.

rslt:concentration
    a skos:Concept ;
    skos:historyNote "Compiled by the Geological Survey of Queensland" ;
    rdfs:isDefinedBy cs: ;
    skos:definition "The abundance of a constituent divided by the total volume of a mixture."@en ;
    skos:inScheme cs: ;
    skos:notation "rctn" ;
    skos:prefLabel "Concentration"@en ;
    skos:topConceptOf cs: ;
.

rslt:cost
    a skos:Concept ;
    skos:historyNote "Compiled by the Geological Survey of Queensland" ;
    rdfs:isDefinedBy cs: ;
    skos:definition "The monetary value, cost, or price (in a unit of currency) for goods, services, or items."@en ;
    skos:inScheme cs: ;
    skos:notation "rcst" ;
    skos:prefLabel "Cost"@en ;
    skos:topConceptOf cs: ;
.

rslt:count
    a skos:Concept ;
    skos:historyNote "Compiled by the Geological Survey of Queensland" ;
    rdfs:isDefinedBy cs: ;
    skos:definition "A quanitifation of the absolute number of discrete objects, groups, or sets."@en ;
    skos:inScheme cs: ;
    skos:notation "rcnt" ;
    skos:prefLabel "Count"@en ;
    skos:topConceptOf cs: ;
.

rslt:curvature
    a skos:Concept ;
    skos:historyNote "Compiled by the Geological Survey of Queensland" ;
    rdfs:isDefinedBy cs: ;
    skos:altLabel "Dog Leg Severity"@en ;
    skos:definition "The curvature of a line or length of material. The change in angle per unit of length. Used in oil and gas to describe the curvature of a wellbore."@en ;
    skos:inScheme cs: ;
    skos:notation "rdls" ;
    skos:prefLabel "Curvature"@en ;
    skos:topConceptOf cs: ;
.

rslt:data
    a skos:Concept ;
    skos:historyNote "Compiled by the Geological Survey of Queensland" ;
    rdfs:isDefinedBy cs: ;
    skos:definition "The amount of data or information held by an electronic and measurable means. Typically reported in bytes or a derivative unit."@en ;
    skos:inScheme cs: ;
    skos:notation "rdat" ;
    skos:prefLabel "Data"@en ;
    skos:topConceptOf cs: ;
.

rslt:density
    a skos:Concept ;
    skos:historyNote "Compiled by the Geological Survey of Queensland" ;
    rdfs:isDefinedBy cs: ;
    skos:definition "The density (more precisely, the volumetric mass density; also known as specific mass), of a substance is its mass per unit volume."@en ;
    skos:inScheme cs: ;
    skos:notation "rden" ;
    skos:prefLabel "Density"@en ;
    skos:topConceptOf cs: ;
.

rslt:descriptive
    a skos:Concept ;
    skos:historyNote "Compiled by the Geological Survey of Queensland" ;
    rdfs:isDefinedBy cs: ;
    skos:definition "A decription of a subject or object of interest."@en ;
    skos:inScheme cs: ;
    skos:notation "rdsc" ;
    skos:prefLabel "Descriptive"@en ;
    skos:topConceptOf cs: ;
.

rslt:distance
    a skos:Concept ;
    skos:historyNote "Compiled by the Geological Survey of Queensland" ;
    rdfs:isDefinedBy cs: ;
    skos:definition "The length of travel along a path that may be non-linear."@en ;
    skos:inScheme cs: ;
    skos:notation "rdis" ;
    skos:prefLabel "Distance"@en ;
    skos:topConceptOf cs: ;
.

rslt:drill-rate
    a skos:Concept ;
    skos:historyNote "Compiled by the Geological Survey of Queensland" ;
    rdfs:isDefinedBy cs: ;
    skos:altLabel "Rate of Penetration"@en ;
    skos:definition "The rate that a drillbit penetrates the subsurface substrate and creates wellbore length."@en ;
    skos:inScheme cs: ;
    skos:notation "rdlr" ;
    skos:prefLabel "Drill Rate"@en ;
    skos:topConceptOf cs: ;
.

rslt:electric-charge
    a skos:Concept ;
    skos:historyNote "Compiled by the Geological Survey of Queensland" ;
    rdfs:isDefinedBy cs: ;
    skos:altLabel "Electrical Charge"@en ;
    skos:definition "The physical property of matter that causes it to experience a force when placed in an electromagnetic field. There are two types of electric charge: positive and negative (commonly carried by protons and electrons respectively)."@en ;
    skos:inScheme cs: ;
    skos:notation "relc" ;
    skos:prefLabel "Electric Charge"@en ;
    skos:topConceptOf cs: ;
.

rslt:electric-current
    a skos:Concept ;
    skos:historyNote "Compiled by the Geological Survey of Queensland" ;
    rdfs:isDefinedBy cs: ;
    skos:altLabel "Electrical Current"@en ;
    skos:definition "The rate of flow of electric charge past a point or region."@en ;
    skos:inScheme cs: ;
    skos:notation "relr" ;
    skos:prefLabel "Electric Current"@en ;
    skos:topConceptOf cs: ;
.

rslt:electrical-conductivity
    a skos:Concept ;
    skos:historyNote "Compiled by the Geological Survey of Queensland" ;
    rdfs:isDefinedBy cs: ;
    skos:altLabel "Electrical Conductance"@en ;
    skos:definition "A measure of a material's ability to conduct an electric current."@en ;
    skos:inScheme cs: ;
    skos:notation "recd" ;
    skos:prefLabel "Conductivity"@en ;
    skos:topConceptOf cs: ;
.

rslt:elevation
    a skos:Concept ;
    skos:historyNote "Compiled by the Geological Survey of Queensland" ;
    rdfs:isDefinedBy cs: ;
    skos:altLabel
        "Height" ,
        "Altitude"@en ;
    skos:definition "The distance vertically upward from a reference point, surface, or datum."@en ;
    skos:inScheme cs: ;
    skos:notation "relv" ;
    skos:prefLabel "Elevation"@en ;
    skos:topConceptOf cs: ;
.

rslt:energy
    a skos:Concept ;
    skos:historyNote "Compiled by the Geological Survey of Queensland" ;
    rdfs:isDefinedBy cs: ;
    skos:definition "The quantitative property that must be transferred to an object in order to perform work on, or to heat, the object."@en ;
    skos:inScheme cs: ;
    skos:notation "reng" ;
    skos:prefLabel "Energy"@en ;
    skos:topConceptOf cs: ;
.

rslt:energy-density
    a skos:Concept ;
    skos:historyNote "Compiled by the Geological Survey of Queensland" ;
    rdfs:isDefinedBy cs: ;
    skos:altLabel
        "Gas Quality"@en ,
        "Heat Content"@en ;
    skos:definition "The amount of energy stored in a given system or region of space per unit volume e.g. PJ/Mm3."@en ;
    skos:inScheme cs: ;
    skos:notation "rend" ;
    skos:prefLabel "Energy Density"@en ;
    skos:topConceptOf cs: ;
.

rslt:flow-rate
    a skos:Concept ;
    skos:historyNote "Compiled by the Geological Survey of Queensland" ;
    rdfs:isDefinedBy cs: ;
    skos:altLabel "Volumetric Flow Rate"@en ;
    skos:definition "The volume of fluid which passes a point or region per unit time."@en ;
    skos:inScheme cs: ;
    skos:notation "rflr" ;
    skos:prefLabel "Flow Rate"@en ;
    skos:topConceptOf cs: ;
.

rslt:fluid-density
    a skos:Concept ;
    skos:historyNote "Compiled by the Geological Survey of Queensland" ;
    rdfs:isDefinedBy cs: ;
    skos:altLabel "Mud Weight"@en ;
    skos:definition "The mass per unit volume of a fluid. Commonly used as a quantity for drilling fluids and cement in relation to boreholes."@en ;
    skos:inScheme cs: ;
    skos:notation "rfld" ;
    skos:prefLabel "Fluid Density"@en ;
    skos:topConceptOf cs: ;
.

rslt:force
    a skos:Concept ;
    skos:historyNote "Compiled by the Geological Survey of Queensland" ;
    rdfs:isDefinedBy cs: ;
    skos:definition "Any interaction that, when unopposed, will change the motion of an object."@en ;
    skos:inScheme cs: ;
    skos:notation "rfrc" ;
    skos:prefLabel "Force"@en ;
    skos:topConceptOf cs: ;
.

rslt:frequency
    a skos:Concept ;
    skos:historyNote "Compiled by the Geological Survey of Queensland" ;
    rdfs:isDefinedBy cs: ;
    skos:definition "The number of occurrences of a repeating event per unit of time."@en ;
    skos:inScheme cs: ;
    skos:notation "rfrq" ;
    skos:prefLabel "Frequency"@en ;
    skos:topConceptOf cs: ;
.

rslt:gas-content
    a skos:Concept ;
    skos:historyNote "Compiled by the Geological Survey of Queensland" ;
    rdfs:isDefinedBy cs: ;
    skos:definition "The amount of gas, typically hydrocarbon, contained or within solid or liquid. Commonly used to describe to the amount of gas adsorbed to a mass of coal."@en ;
    skos:inScheme cs: ;
    skos:notation "rgsc" ;
    skos:prefLabel "Gas Content"@en ;
    skos:topConceptOf cs: ;
.

rslt:grain-shape
    a skos:Concept ;
    skos:historyNote "Compiled by the Geological Survey of Queensland" ;
    rdfs:isDefinedBy cs: ;
    skos:altLabel "Roundness"@en ;
    skos:definition "The degree of smoothing due to abrasion of sedimentary particles i.e. well-rounded, rounded, sub-rounded, sub-angular, angular, very angular."@en ;
    skos:inScheme cs: ;
    skos:notation "rgrs" ;
    skos:prefLabel "Grain Shape"@en ;
    skos:topConceptOf cs: ;
.

rslt:grain-size
    a skos:Concept ;
    skos:historyNote "Compiled by the Geological Survey of Queensland" ;
    rdfs:isDefinedBy cs: ;
    skos:definition "The diameter of individual grains of sediment, or the lithified particles in clastic rocks. The term may also be applied to other granular materials."@en ;
    skos:inScheme cs: ;
    skos:notation "rgrz" ;
    skos:prefLabel "Grain Size"@en ;
    skos:topConceptOf cs: ;
.

rslt:heat
    a skos:Concept ;
    skos:historyNote "Compiled by the Geological Survey of Queensland" ;
    rdfs:isDefinedBy cs: ;
    skos:definition "Energy in transfer to or from a thermodynamic system, by mechanisms other than thermodynamic work or transfer of matter."@en ;
    skos:inScheme cs: ;
    skos:notation "rhet" ;
    skos:prefLabel "Heat"@en ;
    skos:topConceptOf cs: ;
.

rslt:illuminance
    a skos:Concept ;
    skos:historyNote "Compiled by the Geological Survey of Queensland" ;
    rdfs:isDefinedBy cs: ;
    skos:definition "The total luminous flux incident on a surface, per unit area."@en ;
    skos:inScheme cs: ;
    skos:notation "rill" ;
    skos:prefLabel "Illuminance"@en ;
    skos:topConceptOf cs: ;
.

rslt:inductance
    a skos:Concept ;
    skos:historyNote "Compiled by the Geological Survey of Queensland" ;
    rdfs:isDefinedBy cs: ;
    skos:definition "The tendency of an electrical conductor to oppose a change in the electric current flowing through it."@en ;
    skos:inScheme cs: ;
    skos:notation "rind" ;
    skos:prefLabel "Inductance"@en ;
    skos:topConceptOf cs: ;
.

rslt:length
    a skos:Concept ;
    skos:historyNote "Compiled by the Geological Survey of Queensland" ;
    rdfs:isDefinedBy cs: ;
    skos:definition "A measure of distance in one dimension."@en ;
    skos:inScheme cs: ;
    skos:notation "rlen" ;
    skos:prefLabel "Length"@en ;
    skos:topConceptOf cs: ;
.

rslt:luminous-flux
    a skos:Concept ;
    skos:historyNote "Compiled by the Geological Survey of Queensland" ;
    rdfs:isDefinedBy cs: ;
    skos:definition "The measure of the perceived power of light. It differs from radiant flux, the measure of the total power of electromagnetic radiation (including infrared, ultraviolet, and visible light), in that luminous flux is adjusted to reflect the varying sensitivity of the human eye to different wavelengths of light."@en ;
    skos:inScheme cs: ;
    skos:notation "rlfx" ;
    skos:prefLabel "Luminous Flux"@en ;
    skos:topConceptOf cs: ;
.

rslt:luminous-intensity
    a skos:Concept ;
    skos:historyNote "Compiled by the Geological Survey of Queensland" ;
    rdfs:isDefinedBy cs: ;
    skos:definition "A measure of the wavelength-weighted power emitted by a light source in a particular direction per unit solid angle, based on the luminosity function, a standardized model of the sensitivity of the human eye."@en ;
    skos:inScheme cs: ;
    skos:notation "rlin" ;
    skos:prefLabel "Luminous Intensity"@en ;
    skos:topConceptOf cs: ;
.

rslt:magnetic-flux
    a skos:Concept ;
    skos:historyNote "Compiled by the Geological Survey of Queensland" ;
    rdfs:isDefinedBy cs: ;
    skos:definition "The surface integral of the normal component of the magnetic field flux density B passing through that surface."@en ;
    skos:inScheme cs: ;
    skos:notation "rmfx" ;
    skos:prefLabel "Magnetic Flux"@en ;
    skos:topConceptOf cs: ;
.

rslt:magnetic-flux-density
    a skos:Concept ;
    skos:historyNote "Compiled by the Geological Survey of Queensland" ;
    rdfs:isDefinedBy cs: ;
    skos:altLabel
        "B-Field"@en ,
        "Magnetic Field"@en ,
        "Magnetic Induction"@en ;
    skos:definition "The force a magnetic field exerts on a moving charged particle."@en ;
    skos:inScheme cs: ;
    skos:notation "rmfd" ;
    skos:prefLabel "Magnetic Flux Density"@en ;
    skos:topConceptOf cs: ;
.

rslt:magnetic-susceptibility
    a skos:Concept ;
    skos:historyNote "Compiled by the Geological Survey of Queensland" ;
    rdfs:isDefinedBy cs: ;
    skos:definition "A measure of how much a material will become magnetized in an applied magnetic field. Mathematically, it is the ratio of magnetization M (magnetic moment per unit volume) to the applied magnetizing field intensity H."@en ;
    skos:inScheme cs: ;
    skos:notation "rmsc" ;
    skos:prefLabel "Magnetic Susceptibility"@en ;
    skos:topConceptOf cs: ;
.

rslt:mass
    a skos:Concept ;
    skos:historyNote "Compiled by the Geological Survey of Queensland" ;
    rdfs:isDefinedBy cs: ;
    skos:definition "A property of a physical body and a measure of its resistance to acceleration (a change in its state of motion) when a net force is applied."@en ;
    skos:inScheme cs: ;
    skos:notation "rmss" ;
    skos:prefLabel "Mass"@en ;
    skos:topConceptOf cs: ;
.

rslt:measured-depth
    a skos:Concept ;
    skos:historyNote "Compiled by the Geological Survey of Queensland" ;
    rdfs:isDefinedBy cs: ;
    skos:altLabel "MD" ;
    skos:definition "The depth below a reference point or reference datum along a defined path. Commonly used along the path of a wellbore."@en ;
    skos:inScheme cs: ;
    skos:notation "rmmd" ;
    skos:prefLabel "Measured Depth"@en ;
    skos:topConceptOf cs: ;
.

rslt:oil-quality
    a skos:Concept ;
    skos:historyNote "Compiled by the Geological Survey of Queensland" ;
    rdfs:isDefinedBy cs: ;
    skos:definition "Value for the thermal quality of oil reported. This is often recorded in British Thermal Units (BTUs) and can be used to calculate the Barrel of Oil Equivalent (BOE)."@en ;
    skos:inScheme cs: ;
    skos:notation "rolq" ;
    skos:prefLabel "Oil Quality"@en ;
    skos:topConceptOf cs: ;
.

rslt:permeability
    a skos:Concept ;
    skos:historyNote "Compiled by the Geological Survey of Queensland" ;
    rdfs:isDefinedBy cs: ;
    skos:definition "A measure of the ability of a material (such as rocks) to transmit fluids."@en ;
    skos:inScheme cs: ;
    skos:notation "rprm" ;
    skos:prefLabel "Permeability"@en ;
    skos:topConceptOf cs: ;
.

rslt:porosity
    a skos:Concept ;
    skos:historyNote "Compiled by the Geological Survey of Queensland" ;
    rdfs:isDefinedBy cs: ;
    skos:definition "A measure of the void (i.e. 'empty') spaces in a material, and is a fraction of the volume of voids over the total volume, between 0 and 1, or as a percentage between 0% and 100%."@en ;
    skos:inScheme cs: ;
    skos:notation "rpor" ;
    skos:prefLabel "Porosity"@en ;
    skos:topConceptOf cs: ;
.

rslt:power
    a skos:Concept ;
    skos:historyNote "Compiled by the Geological Survey of Queensland" ;
    rdfs:isDefinedBy cs: ;
    skos:definition "The rate of doing work or of transferring heat, i.e. the amount of energy transferred or converted per unit time."@en ;
    skos:inScheme cs: ;
    skos:notation "rpow" ;
    skos:prefLabel "Power"@en ;
    skos:topConceptOf cs: ;
.

rslt:pressure
    a skos:Concept ;
    skos:historyNote "Compiled by the Geological Survey of Queensland" ;
    rdfs:isDefinedBy cs: ;
    skos:definition "The force applied perpendicular to the surface of an object per unit area over which that force is distributed."@en ;
    skos:inScheme cs: ;
    skos:notation "rprs" ;
    skos:prefLabel "Pressure"@en ;
    skos:topConceptOf cs: ;
.

rslt:radioactivity
    a skos:Concept ;
    skos:historyNote "Compiled by the Geological Survey of Queensland" ;
    rdfs:isDefinedBy cs: ;
    skos:altLabel
        "nuclear decay"@en ,
        "nuclear disintegration"@en ,
        "radioactive decay"@en ,
        "radioactive disintegration"@en ;
    skos:definition "The process by which an unstable atomic nucleus loses energy by radiation. A material containing unstable nuclei is considered radioactive."@en ;
    skos:inScheme cs: ;
    skos:notation "rrad" ;
    skos:prefLabel "Radioactivity"@en ;
    skos:topConceptOf cs: ;
.

rslt:recovery
    a skos:Concept ;
    skos:historyNote "Compiled by the Geological Survey of Queensland" ;
    rdfs:isDefinedBy cs: ;
    skos:definition "The amount of a target material recovered from an input mixture relative to the total amount of the target material initially present in the input. Expressed as a percentage."@en ;
    skos:inScheme cs: ;
    skos:notation "rrec" ;
    skos:prefLabel "Recovery"@en ;
    skos:topConceptOf cs: ;
.

rslt:resitivity
    a skos:Concept ;
    skos:historyNote "Compiled by the Geological Survey of Queensland" ;
    rdfs:isDefinedBy cs: ;
    skos:altLabel "Resistance"@en ;
    skos:definition "The measure of the degree to which a conductor opposes an electric current through that conductor."@en ;
    skos:inScheme cs: ;
    skos:notation "rres" ;
    skos:prefLabel "Resitivity"@en ;
    skos:topConceptOf cs: ;
.

rslt:rotation
    a skos:Concept ;
    skos:historyNote "Compiled by the Geological Survey of Queensland" ;
    rdfs:isDefinedBy cs: ;
    skos:altLabel "Rotation Rate"@en ;
    skos:definition "A measure of the rate of circular movement of an object around a center (or point) of rotation."@en ;
    skos:inScheme cs: ;
    skos:notation "rrtt" ;
    skos:prefLabel "Rotation"@en ;
    skos:topConceptOf cs: ;
.

rslt:sales-volumetric
    a skos:Concept ;
    skos:historyNote "Compiled by the Geological Survey of Queensland" ;
    rdfs:isDefinedBy cs: ;
    skos:definition "A measure of the amount of a commodity in its unit of sale. A measure of a reserve or resource volume."@en ;
    skos:inScheme cs: ;
    skos:notation "rsal" ;
    skos:prefLabel "Sales Volumetric"@en ;
    skos:scopeNote "Sales volumes are represented by commodity specific units of measure that are internally inconsistent within a standard result type and refer specifically to the context of marketable quantities i.e. a sales quantity may be a volume, energy unit, mass, or other result type."@en ;
    skos:topConceptOf cs: ;
.

rslt:saturation
    a skos:Concept ;
    skos:historyNote "Compiled by the Geological Survey of Queensland" ;
    rdfs:isDefinedBy cs: ;
    skos:definition "A measure of the amount of a substance contained within a volume or another material relative to the maximum theoretical amount of substance that could be contained under the same conditions."@en ;
    skos:inScheme cs: ;
    skos:notation "rsat" ;
    skos:prefLabel "Saturation"@en ;
    skos:topConceptOf cs: ;
.

rslt:shear-strength
    a skos:Concept ;
    skos:historyNote "Compiled by the Geological Survey of Queensland" ;
    rdfs:isDefinedBy cs: ;
    skos:definition "The ability to withstand the strength of a material or component against the type of yield or structural failure when the material or component fails in shear. A shear load is a force that tends to produce a sliding failure on a material along a plane that is parallel to the direction of the force. When a paper is cut with scissors, the paper fails in shear.shearing"@en ;
    skos:inScheme cs: ;
    skos:notation "rshs" ;
    skos:prefLabel "Shear Strength"@en ;
    skos:topConceptOf cs: ;
.

rslt:sorting
    a skos:Concept ;
    skos:historyNote "Compiled by the Geological Survey of Queensland" ;
    rdfs:isDefinedBy cs: ;
    skos:altLabel "Sedimentary Sorting"@en ;
    skos:definition "The distribution of grain size of sediments, either in unconsolidated deposits or in sedimentary rocks. Very poorly sorted indicates that the sediment sizes are mixed (large variance); whereas well sorted indicates that the sediment sizes are similar (low variance)."@en ;
    skos:inScheme cs: ;
    skos:notation "rsrt" ;
    skos:prefLabel "Sorting"@en ;
    skos:topConceptOf cs: ;
.

rslt:spacing
    a skos:Concept ;
    skos:historyNote "Compiled by the Geological Survey of Queensland" ;
    rdfs:isDefinedBy cs: ;
    skos:definition "The regular, or average, distance between recurrences of a feature along a transect or across an object."@en ;
    skos:inScheme cs: ;
    skos:notation "rspc" ;
    skos:prefLabel "Spacing"@en ;
    skos:topConceptOf cs: ;
.

rslt:sphericity
    a skos:Concept ;
    skos:historyNote "Compiled by the Geological Survey of Queensland" ;
    rdfs:isDefinedBy cs: ;
    skos:definition "A measure of how closely the shape of an object resembles that of a perfect sphere."@en ;
    skos:inScheme cs: ;
    skos:notation "rsph" ;
    skos:prefLabel "Sphericity"@en ;
    skos:topConceptOf cs: ;
.

rslt:stiffness
    a skos:Concept ;
    skos:historyNote "Compiled by the Geological Survey of Queensland" ;
    rdfs:isDefinedBy cs: ;
    skos:definition "The extent to which an object resists deformation in response to an applied force."@en ;
    skos:inScheme cs: ;
    skos:notation "rstf" ;
    skos:prefLabel "Stiffness"@en ;
    skos:topConceptOf cs: ;
.

rslt:strain
    a skos:Concept ;
    skos:historyNote "Compiled by the Geological Survey of Queensland" ;
    rdfs:isDefinedBy cs: ;
    skos:definition "Strain is a measure of deformation representing the displacement between particles in the body relative to a reference length."@en ;
    skos:inScheme cs: ;
    skos:notation "rstn" ;
    skos:prefLabel "Strain"@en ;
    skos:topConceptOf cs: ;
.

rslt:stress
    a skos:Concept ;
    skos:historyNote "Compiled by the Geological Survey of Queensland" ;
    rdfs:isDefinedBy cs: ;
    skos:definition "A physical quantity that expresses the internal forces that neighbouring particles of a continuous material exert on each other, while strain is the measure of the deformation of the material."@en ;
    skos:inScheme cs: ;
    skos:notation "rsts" ;
    skos:prefLabel "Stress"@en ;
    skos:topConceptOf cs: ;
.

rslt:temperature
    a skos:Concept ;
    skos:historyNote "Compiled by the Geological Survey of Queensland" ;
    rdfs:isDefinedBy cs: ;
    skos:definition "A physical property of matter that quantitatively expresses hot and cold. Temperature is the manifestation of thermal energy, present in all matter, which is the source of the occurrence of heat, a flow of energy, when a body is in contact with another that is colder."@en ;
    skos:inScheme cs: ;
    skos:notation "rtmp" ;
    skos:prefLabel "Temperature"@en ;
    skos:topConceptOf cs: ;
.

rslt:tensile-strength
    a skos:Concept ;
    skos:historyNote "Compiled by the Geological Survey of Queensland" ;
    rdfs:isDefinedBy cs: ;
    skos:definition "The maximum stress that a material can withstand while being stretched or pulled before breaking."@en ;
    skos:inScheme cs: ;
    skos:notation "rtns" ;
    skos:prefLabel "Tensile Strength"@en ;
    skos:topConceptOf cs: ;
.

rslt:thermal-conductivity
    a skos:Concept ;
    skos:historyNote "Compiled by the Geological Survey of Queensland" ;
    rdfs:isDefinedBy cs: ;
    skos:altLabel "Thermal Conductance"@en ;
    skos:definition "A measure of a material's ability to conduct an thermal energy."@en ;
    skos:inScheme cs: ;
    skos:notation "rtcd" ;
    skos:prefLabel "Thermal Conductivity"@en ;
    skos:topConceptOf cs: ;
.

rslt:time
    a skos:Concept ;
    skos:historyNote "Compiled by the Geological Survey of Queensland" ;
    rdfs:isDefinedBy cs: ;
    skos:definition "The indefinite continued progress of existence and events that occur in an apparently irreversible succession from the past, through the present, into the future."@en ;
    skos:inScheme cs: ;
    skos:notation "rtme" ;
    skos:prefLabel "Time"@en ;
    skos:topConceptOf cs: ;
.

rslt:true-vertical-depth
    a skos:Concept ;
    skos:historyNote "Compiled by the Geological Survey of Queensland" ;
    rdfs:isDefinedBy cs: ;
    skos:altLabel "TVD" ;
    skos:definition "The depth below a reference point or reference datum in a direct vertical direction."@en ;
    skos:inScheme cs: ;
    skos:notation "rtvd" ;
    skos:prefLabel "True Vertical Depth"@en ;
    skos:topConceptOf cs: ;
.

rslt:velocity
    a skos:Concept ;
    skos:historyNote "Compiled by the Geological Survey of Queensland" ;
    rdfs:isDefinedBy cs: ;
    skos:definition "The rate of change of its position with respect to a frame of reference, and is a function of time."@en ;
    skos:inScheme cs: ;
    skos:notation "rvel" ;
    skos:prefLabel "Velocity"@en ;
    skos:topConceptOf cs: ;
.

rslt:viscosity
    a skos:Concept ;
    skos:historyNote "Compiled by the Geological Survey of Queensland" ;
    rdfs:isDefinedBy cs: ;
    skos:definition "A measure of the resistance to deformation of a fluid at a given rate. For liquids, it corresponds to the informal concept of 'thickness': for example, syrup has a higher viscosity than water."@en ;
    skos:inScheme cs: ;
    skos:notation "rvis" ;
    skos:prefLabel "Viscosity"@en ;
    skos:topConceptOf cs: ;
.

rslt:voltage
    a skos:Concept ;
    skos:historyNote "Compiled by the Geological Survey of Queensland" ;
    rdfs:isDefinedBy cs: ;
    skos:altLabel
        "electric potential difference"@en ,
        "electric pressure"@en ,
        "electric tension"@en ;
    skos:definition "The difference in electric potential between two points. The voltage in a static electric field is defined as the work needed per unit of charge to move a test charge between the two points."@en ;
    skos:inScheme cs: ;
    skos:notation "rvlt" ;
    skos:prefLabel "Voltage"@en ;
    skos:topConceptOf cs: ;
.

rslt:volume
    a skos:Concept ;
    skos:historyNote "Compiled by the Geological Survey of Queensland" ;
    rdfs:isDefinedBy cs: ;
    skos:definition "The quantity of three-dimensional space enclosed by a closed surface, for example, the space that a substance (solid, liquid, gas, or plasma) or shape occupies or contains."@en ;
    skos:inScheme cs: ;
    skos:notation "rvol" ;
    skos:prefLabel "Volume"@en ;
    skos:topConceptOf cs: ;
.

rslt:wavelength
    a skos:Concept ;
    skos:historyNote "Compiled by the Geological Survey of Queensland" ;
    rdfs:isDefinedBy cs: ;
    skos:definition "The wavelength is the spatial period of a periodic wave the distance over which the shape of a wave repeats."@en ;
    skos:inScheme cs: ;
    skos:notation "rwvl" ;
    skos:prefLabel "Wavelength"@en ;
    skos:topConceptOf cs: ;
.

rslt:weight
    a skos:Concept ;
    skos:historyNote "Compiled by the Geological Survey of Queensland" ;
    rdfs:isDefinedBy cs: ;
    skos:definition "The weight of an object is related to the force acting on the object, either due to gravity or to a reaction force that holds it in place."@en ;
    skos:inScheme cs: ;
    skos:notation "rwgt" ;
    skos:prefLabel "Weight"@en ;
    skos:topConceptOf cs: ;
.

rslt:weight-on-bit
    a skos:Concept ;
    skos:historyNote "Compiled by the Geological Survey of Queensland" ;
    rdfs:isDefinedBy cs: ;
    skos:definition "The weight or force applied to a drill bit in the process of drilling a borehole."@en ;
    skos:inScheme cs: ;
    skos:notation "rwob" ;
    skos:prefLabel "Weight on Bit"@en ;
    skos:topConceptOf cs: ;
.

rslt:width
    a skos:Concept ;
    skos:historyNote "Compiled by the Geological Survey of Queensland" ;
    rdfs:isDefinedBy cs: ;
    skos:definition "The measurement or extent of something from side to side; the lesser of two or the least of three dimensions of a body."@en ;
    skos:inScheme cs: ;
    skos:notation "rwid" ;
    skos:prefLabel "Width"@en ;
    skos:topConceptOf cs: ;
.

rslt:work
    a skos:Concept ;
    skos:historyNote "Compiled by the Geological Survey of Queensland" ;
    rdfs:isDefinedBy cs: ;
    skos:definition "The product of force and displacement. A force is said to do work if, when acting, there is a movement of the point of application in the direction of the force."@en ;
    skos:inScheme cs: ;
    skos:notation "rwrk" ;
    skos:prefLabel "Work"@en ;
    skos:topConceptOf cs: ;
.

rslt:yield-point
    a skos:Concept ;
    skos:historyNote "Compiled by the Geological Survey of Queensland" ;
    rdfs:isDefinedBy cs: ;
    skos:definition "The point on a stress-strain curve that indicates the limit of elastic behavior and the beginning of plastic behavior."@en ;
    skos:inScheme cs: ;
    skos:notation "ryld" ;
    skos:prefLabel "Yield Point"@en ;
    skos:topConceptOf cs: ;
.

<https://linked.data.gov.au/org/gsq>
    a sdo:Organization ;
    sdo:name "Geological Survey of Queensland" ;
    sdo:url "https://www.business.qld.gov.au/industries/mining-energy-water/resources/geoscience-information/gsq"^^xsd:anyURI ;
.

rslt:angle
    a skos:Concept ;
    skos:historyNote "Compiled by the Geological Survey of Queensland" ;
    rdfs:isDefinedBy cs: ;
    skos:definition "In plane geometry, an angle is the figure formed by two rays, called the sides of the angle, sharing a common endpoint, called the vertex of the angle."@en ;
    skos:inScheme cs: ;
    skos:notation "rang" ;
    skos:prefLabel "Angle"@en ;
    skos:topConceptOf cs: ;
.

cs:
    a
        owl:Ontology ,
        skos:ConceptScheme ;
    dcterms:created "2020-02-08"^^xsd:date ;
    dcterms:creator <https://linked.data.gov.au/org/gsq> ;
    dcterms:modified "2023-03-16"^^xsd:date ;
    skos:historyNote "Compiled by the Geological Survey of Queensland" ;
    dcterms:publisher <https://linked.data.gov.au/org/gsq> ;
    reg:status agldwgstatus:stable ;
    skos:definition "The description and definition of the qualitative and quantitative results obtained through geoscience observations."@en ;
    skos:hasTopConcept
        rslt:age ,
        rslt:angle ,
        rslt:api-gravity ,
        rslt:area ,
        rslt:capacitance ,
        rslt:casing-weight ,
        rslt:colour ,
        rslt:composition ,
        rslt:compressibility ,
        rslt:compressive-strength ,
        rslt:concentration ,
        rslt:cost ,
        rslt:count ,
        rslt:curvature ,
        rslt:data ,
        rslt:density ,
        rslt:descriptive ,
        rslt:distance ,
        rslt:drill-rate ,
        rslt:electric-charge ,
        rslt:electric-current ,
        rslt:electrical-conductivity ,
        rslt:elevation ,
        rslt:energy ,
        rslt:energy-density ,
        rslt:flow-rate ,
        rslt:fluid-density ,
        rslt:force ,
        rslt:frequency ,
        rslt:gas-content ,
        rslt:grain-shape ,
        rslt:grain-size ,
        rslt:heat ,
        rslt:illuminance ,
        rslt:inductance ,
        rslt:length ,
        rslt:luminous-flux ,
        rslt:luminous-intensity ,
        rslt:magnetic-flux ,
        rslt:magnetic-flux-density ,
        rslt:magnetic-susceptibility ,
        rslt:mass ,
        rslt:measured-depth ,
        rslt:oil-quality ,
        rslt:permeability ,
        rslt:porosity ,
        rslt:power ,
        rslt:pressure ,
        rslt:radioactivity ,
        rslt:recovery ,
        rslt:resitivity ,
        rslt:rotation ,
        rslt:sales-volumetric ,
        rslt:saturation ,
        rslt:shear-strength ,
        rslt:sorting ,
        rslt:spacing ,
        rslt:sphericity ,
        rslt:stiffness ,
        rslt:strain ,
        rslt:stress ,
        rslt:temperature ,
        rslt:tensile-strength ,
        rslt:thermal-conductivity ,
        rslt:time ,
        rslt:true-vertical-depth ,
        rslt:velocity ,
        rslt:viscosity ,
        rslt:voltage ,
        rslt:volume ,
        rslt:wavelength ,
        rslt:weight ,
        rslt:weight-on-bit ,
        rslt:width ,
        rslt:work ,
        rslt:yield-point ;
    skos:prefLabel "Result Type"@en ;
.

