PREFIX agldwgstatus: <https://linked.data.gov.au/def/reg-statuses/>
PREFIX cs: <http://linked.data.gov.au/def/sample-preparation-methods>
PREFIX dcterms: <http://purl.org/dc/terms/>
PREFIX owl: <http://www.w3.org/2002/07/owl#>
PREFIX rdfs: <http://www.w3.org/2000/01/rdf-schema#>
PREFIX reg: <http://purl.org/linked-data/registry#>
PREFIX sdo: <https://schema.org/>
PREFIX skos: <http://www.w3.org/2004/02/skos/core#>
PREFIX smprep: <http://linked.data.gov.au/def/sample-preparation-methods/>
PREFIX xsd: <http://www.w3.org/2001/XMLSchema#>

smprep:mine-processing
    a skos:Collection ;
    dcterms:provenance "Compiled by the Geological Survey of Queensland" ;
    skos:definition "Sample preparation steps and multi-step processes that concentrate, refine, or prepare a raw material into a saleable product."@en ;
    skos:member
        smprep:beneficiate ,
        smprep:concentrate ,
        smprep:crush-sort ,
        smprep:cut ,
        smprep:gravity-concentrate ,
        smprep:partial-cut ,
        smprep:refine ,
        smprep:refining-byproduct ,
        smprep:rough-extract ,
        smprep:smelt ,
        smprep:smelt-byproduct ,
        smprep:unprocessed ,
        smprep:unspecified ;
    skos:prefLabel "Mine Processing"@en ;
.

smprep:acidify
    a skos:Concept ;
    dcterms:provenance "Compiled by the Geological Survey of Queensland" ;
    rdfs:isDefinedBy cs: ;
    skos:altLabel "Sour"@en ;
    skos:definition "The process of making a material more acidic."@en ;
    skos:inScheme cs: ;
    skos:prefLabel "Acidify"@en ;
    skos:topConceptOf cs: ;
.

smprep:aggregate
    a skos:Concept ;
    dcterms:provenance "Compiled by the Geological Survey of Queensland" ;
    rdfs:isDefinedBy cs: ;
    skos:altLabel "Compile"@en ;
    skos:definition "To collect or gather into a mass or whole"@en ;
    skos:inScheme cs: ;
    skos:prefLabel "Aggregate"@en ;
    skos:topConceptOf cs: ;
.

smprep:chelate
    a skos:Concept ;
    dcterms:provenance "Compiled by the Geological Survey of Queensland" ;
    rdfs:isDefinedBy cs: ;
    skos:definition "A chemical process to cluster metallic ions."@en ;
    skos:inScheme cs: ;
    skos:prefLabel "Chelate"@en ;
    skos:topConceptOf cs: ;
.

smprep:compress
    a skos:Concept ;
    dcterms:provenance "Compiled by the Geological Survey of Queensland" ;
    rdfs:isDefinedBy cs: ;
    skos:altLabel
        "Compression"@en ,
        "Pressurisation"@en ;
    skos:definition "The action of increasing pressure on a sample."@en ;
    skos:inScheme cs: ;
    skos:prefLabel "Compress"@en ;
    skos:topConceptOf cs: ;
.

smprep:condense
    a skos:Concept ;
    dcterms:provenance "Compiled by the Geological Survey of Queensland" ;
    rdfs:isDefinedBy cs: ;
    skos:definition "To change a gas to a liquid. Typically through decreasing temperature or increasing pressure."@en ;
    skos:inScheme cs: ;
    skos:prefLabel "Condense"@en ;
    skos:topConceptOf cs: ;
.

smprep:cool
    a skos:Concept ;
    dcterms:provenance "Compiled by the Geological Survey of Queensland" ;
    rdfs:isDefinedBy cs: ;
    skos:definition "The process of reducing the sample temperature."@en ;
    skos:inScheme cs: ;
    skos:prefLabel "Cool"@en ;
    skos:topConceptOf cs: ;
.

smprep:cupellation
    a skos:Concept ;
    dcterms:provenance "Compiled by the Geological Survey of Queensland" ;
    rdfs:isDefinedBy cs: ;
    skos:broader smprep:melt ;
    skos:definition "The refining process in metallurgy where ores or alloyed metals are treated under very high temperatures and have controlled operations to separate noble metals, like gold and silver, from base metals, like lead, copper, zinc, arsenic, antimony, or bismuth, present in the ore."@en ;
    skos:inScheme cs: ;
    skos:prefLabel "Cupellation"@en ;
.

smprep:deacidify
    a skos:Concept ;
    dcterms:provenance "Compiled by the Geological Survey of Queensland" ;
    rdfs:isDefinedBy cs: ;
    skos:altLabel "Sweeten"@en ;
    skos:definition "The process of making a material more alkaline."@en ;
    skos:inScheme cs: ;
    skos:prefLabel "Deacidify"@en ;
    skos:topConceptOf cs: ;
.

smprep:decompress
    a skos:Concept ;
    dcterms:provenance "Compiled by the Geological Survey of Queensland" ;
    rdfs:isDefinedBy cs: ;
    skos:altLabel
        "Decompression"@en ,
        "Depressurisation"@en ;
    skos:definition "The action of decreasing pressure on a sample."@en ;
    skos:inScheme cs: ;
    skos:prefLabel "Decompress"@en ;
    skos:topConceptOf cs: ;
.

smprep:deposit
    a skos:Concept ;
    dcterms:provenance "Compiled by the Geological Survey of Queensland" ;
    rdfs:isDefinedBy cs: ;
    skos:definition "To change a gas to a solid. Typically through decreasing temperature or increasing pressure."@en ;
    skos:inScheme cs: ;
    skos:prefLabel "Deposit"@en ;
    skos:topConceptOf cs: ;
.

smprep:dessicate
    a skos:Concept ;
    dcterms:provenance "Compiled by the Geological Survey of Queensland" ;
    rdfs:isDefinedBy cs: ;
    skos:altLabel
        "Dehydrating"@en ,
        "Drying"@en ;
    skos:definition "The removal of a liquid component from a solid."@en ;
    skos:inScheme cs: ;
    skos:prefLabel "Dessicate"@en ;
    skos:topConceptOf cs: ;
.

smprep:dilute
    a skos:Concept ;
    dcterms:provenance "Compiled by the Geological Survey of Queensland" ;
    rdfs:isDefinedBy cs: ;
    skos:definition "Preparation by addition of the solvent or diluting agent(s)."@en ;
    skos:inScheme cs: ;
    skos:prefLabel "Dilute"@en ;
    skos:topConceptOf cs: ;
.

smprep:disaggregate
    a skos:Concept ;
    dcterms:provenance "Compiled by the Geological Survey of Queensland" ;
    rdfs:isDefinedBy cs: ;
    skos:definition "To separate into component parts"@en ;
    skos:inScheme cs: ;
    skos:prefLabel "Disaggregate"@en ;
    skos:topConceptOf cs: ;
.

smprep:dissolve
    a skos:Concept ;
    dcterms:provenance "Compiled by the Geological Survey of Queensland" ;
    rdfs:isDefinedBy cs: ;
    skos:definition "The process of dissolving a material in a solvent."@en ;
    skos:inScheme cs: ;
    skos:prefLabel "Dissolve"@en ;
    skos:topConceptOf cs: ;
.

smprep:distill
    a skos:Concept ;
    dcterms:provenance "Compiled by the Geological Survey of Queensland" ;
    rdfs:isDefinedBy cs: ;
    skos:definition "The action of purifying a liquid by a process of heating and cooling."@en ;
    skos:inScheme cs: ;
    skos:prefLabel "Distill"@en ;
    skos:topConceptOf cs: ;
.

smprep:extract
    a skos:Concept ;
    dcterms:provenance "Compiled by the Geological Survey of Queensland" ;
    rdfs:isDefinedBy cs: ;
    skos:definition "A separation process consisting in the separation of a substance from a matrix. Common examples include liquid-liquid extraction, and solid phase extraction."@en ;
    skos:inScheme cs: ;
    skos:prefLabel "Extract"@en ;
    skos:topConceptOf cs: ;
.

smprep:filter
    a skos:Concept ;
    dcterms:provenance "Compiled by the Geological Survey of Queensland" ;
    rdfs:isDefinedBy cs: ;
    skos:definition "An operation that separates solid matter and fluid from a mixture with a filter medium that has a complex structure through which only the fluid can pass."@en ;
    skos:inScheme cs: ;
    skos:prefLabel "Filter"@en ;
    skos:topConceptOf cs: ;
.

smprep:freeze
    a skos:Concept ;
    dcterms:provenance "Compiled by the Geological Survey of Queensland" ;
    rdfs:isDefinedBy cs: ;
    skos:altLabel "Solidify"@en ;
    skos:definition "To change a liquid to a solid. Typically through decreasing temperature or increasing pressure."@en ;
    skos:inScheme cs: ;
    skos:prefLabel "Freeze"@en ;
    skos:topConceptOf cs: ;
.

smprep:gravity-concentrate
    a skos:Concept ;
    dcterms:provenance "Compiled by the Geological Survey of Queensland" ;
    rdfs:isDefinedBy cs: ;
    skos:altLabel
        "Float-and-Sink Separation"@en ,
        "Gravity Separation"@en ,
        "Sink-and-Float Separation"@en ;
    skos:broader smprep:concentrate ;
    skos:definition "Preparation by removing or reducing the diluting material through the action of gravity by utilising density difference between the target material and host material."@en ;
    skos:inScheme cs: ;
    skos:prefLabel "Gravity Concentrate"@en ;
.

smprep:grind
    a skos:Concept ;
    dcterms:provenance "Compiled by the Geological Survey of Queensland" ;
    rdfs:isDefinedBy cs: ;
    skos:definition "Reduce of material to small particles or powder by crushing it."@en ;
    skos:inScheme cs: ;
    skos:prefLabel "Grind"@en ;
    skos:topConceptOf cs: ;
.

smprep:hydrate
    a skos:Concept ;
    dcterms:provenance "Compiled by the Geological Survey of Queensland" ;
    rdfs:isDefinedBy cs: ;
    skos:altLabel "Wetting"@en ;
    skos:definition "The addition of water to a solid sample."@en ;
    skos:inScheme cs: ;
    skos:prefLabel "Hydrate"@en ;
    skos:topConceptOf cs: ;
.

smprep:ionise
    a skos:Concept ;
    dcterms:provenance "Compiled by the Geological Survey of Queensland" ;
    rdfs:isDefinedBy cs: ;
    skos:altLabel "Ionize"@en ;
    skos:definition "To change a gas to a plasma. Typically through decreasing temperature."@en ;
    skos:inScheme cs: ;
    skos:prefLabel "Ionise"@en ;
    skos:topConceptOf cs: ;
.

smprep:laser-ablate
    a skos:Concept ;
    dcterms:provenance "Compiled by the Geological Survey of Queensland" ;
    rdfs:isDefinedBy cs: ;
    skos:definition "Laser ablation is the process of removing material from a solid (or occasionally liquid) surface by irradiating it with a laser beam."@en ;
    skos:inScheme cs: ;
    skos:prefLabel "Laser Ablate"@en ;
    skos:topConceptOf cs: ;
.

smprep:mount
    a skos:Concept ;
    dcterms:provenance "Compiled by the Geological Survey of Queensland" ;
    rdfs:isDefinedBy cs: ;
    skos:definition "To be mounted on or between media in preparation for petroscopy or other observation technique which requires a stable, protected sample."@en ;
    skos:inScheme cs: ;
    skos:prefLabel "Mount"@en ;
    skos:topConceptOf cs: ;
.

smprep:partial-cut
    a skos:Concept ;
    dcterms:provenance "Compiled by the Geological Survey of Queensland" ;
    rdfs:isDefinedBy cs: ;
    skos:broader smprep:cut ;
    skos:definition "Prepartion by bifurcating any number of times to produce fresh faces or a smaller overall sample, but where un-cut surfaces remain on the sample material."@en ;
    skos:inScheme cs: ;
    skos:prefLabel "Partial Cut"@en ;
.

smprep:precipitate
    a skos:Concept ;
    dcterms:provenance "Compiled by the Geological Survey of Queensland" ;
    rdfs:isDefinedBy cs: ;
    skos:definition "The process of precipitating a material out of a solvent."@en ;
    skos:inScheme cs: ;
    skos:prefLabel "Precipitate"@en ;
    skos:topConceptOf cs: ;
.

smprep:react
    a skos:Concept ;
    dcterms:provenance "Compiled by the Geological Survey of Queensland" ;
    rdfs:isDefinedBy cs: ;
    skos:definition "To change the chemical state of a sample by combination with a reagent."@en ;
    skos:inScheme cs: ;
    skos:prefLabel "React"@en ;
    skos:topConceptOf cs: ;
.

smprep:recombine
    a skos:Concept ;
    dcterms:provenance "Compiled by the Geological Survey of Queensland" ;
    rdfs:isDefinedBy cs: ;
    skos:definition "To change a gas to a plasma. Typically through increasing temperature."@en ;
    skos:inScheme cs: ;
    skos:prefLabel "Recombine"@en ;
    skos:topConceptOf cs: ;
.

smprep:sieve
    a skos:Concept ;
    dcterms:provenance "Compiled by the Geological Survey of Queensland" ;
    rdfs:isDefinedBy cs: ;
    skos:definition "Material characterised by size fractionation through a screen or series of screens."@en ;
    skos:inScheme cs: ;
    skos:prefLabel "Sieve"@en ;
    skos:topConceptOf cs: ;
.

smprep:smelt
    a skos:Concept ;
    dcterms:provenance "Compiled by the Geological Survey of Queensland" ;
    rdfs:isDefinedBy cs: ;
    skos:broader smprep:heat ;
    skos:definition "The process of applying heat to ore in order to extract a base metal. Smelting uses heat and a chemical reducing agent to decompose the ore by separating other elements as gases or slag from the ore and resulting in a purified metal base."@en ;
    skos:inScheme cs: ;
    skos:prefLabel "Smelt"@en ;
.

smprep:smelt-byproduct
    a skos:Concept ;
    dcterms:provenance "Compiled by the Geological Survey of Queensland" ;
    rdfs:isDefinedBy cs: ;
    skos:altLabel
        "Smelt Waste"@en ,
        "Smelting Waste"@en ;
    skos:broader smprep:heat ;
    skos:definition "The by-product pathway parallel to a smelting process that generates waste material or by-products."@en ;
    skos:inScheme cs: ;
    skos:prefLabel "Smelt By-product"@en ;
.

smprep:sublimate
    a skos:Concept ;
    dcterms:provenance "Compiled by the Geological Survey of Queensland" ;
    rdfs:isDefinedBy cs: ;
    skos:definition "To change a solid to a gas. Typically through increasing temperature or decreasing pressure."@en ;
    skos:inScheme cs: ;
    skos:prefLabel "Sublimate"@en ;
    skos:topConceptOf cs: ;
.

smprep:thermal-treatment
    a skos:Concept ;
    dcterms:provenance "Compiled by the Geological Survey of Queensland" ;
    rdfs:isDefinedBy cs: ;
    skos:altLabel
        "Bake"@en ,
        "Baking"@en ,
        "Calcination"@en ;
    skos:broader smprep:heat ;
    skos:definition "The process of applying thermal radiation to a material in order to chemically alter or oxidise it."@en ;
    skos:inScheme cs: ;
    skos:prefLabel "Thermal treatment"@en ;
.

smprep:vaporise
    a skos:Concept ;
    dcterms:provenance "Compiled by the Geological Survey of Queensland" ;
    rdfs:isDefinedBy cs: ;
    skos:altLabel
        "Boil"@en ,
        "Vaporize"@en ;
    skos:definition "To change a liquid to a gas. Typically through increasing temperature or decreasing pressure."@en ;
    skos:inScheme cs: ;
    skos:prefLabel "Vaporise"@en ;
    skos:topConceptOf cs: ;
.

smprep:beneficiate
    a skos:Concept ;
    dcterms:provenance "Compiled by the Geological Survey of Queensland" ;
    rdfs:isDefinedBy cs: ;
    owl:hasPart
        smprep:concentrate ,
        smprep:crush ,
        smprep:wash ;
    skos:definition "A composite process that may include any combination of washing, crushing, and concentrating"@en ;
    skos:inScheme cs: ;
    skos:prefLabel "Beneficiate"@en ;
    skos:topConceptOf cs: ;
.

smprep:crush-sort
    a skos:Concept ;
    dcterms:provenance "Compiled by the Geological Survey of Queensland" ;
    rdfs:isDefinedBy cs: ;
    owl:hasPart
        smprep:crush ,
        smprep:sort ;
    skos:definition "A composite process of deformation or pulverization of material by compressing forcefully (crushing) followed by separation of material components based on a physical property such as size or density (sort)."@en ;
    skos:inScheme cs: ;
    skos:prefLabel "Crush and Sort"@en ;
    skos:topConceptOf cs: ;
.

smprep:electrolysis
    a skos:Concept ;
    dcterms:provenance "Compiled by the Geological Survey of Queensland" ;
    rdfs:isDefinedBy cs: ;
    skos:definition "A technique that uses direct electric current to drive an otherwise non-spontaneous chemical reaction. Electrolysis is commercially important as a stage in the separation of elements from naturally occurring sources such as ores using an electrolytic cell."@en ;
    skos:inScheme cs: ;
    skos:prefLabel "Electrolysis"@en ;
    skos:topConceptOf cs: ;
.

smprep:refine
    a skos:Concept ;
    dcterms:provenance "Compiled by the Geological Survey of Queensland" ;
    rdfs:isDefinedBy cs: ;
    owl:hasPart
        smprep:cupellation ,
        smprep:electrolysis ,
        smprep:melt ,
        smprep:thermal-treatment ;
    skos:definition "A group of post-primary process in resource processing such as electrolysis, cupellation, pyrometallurgical reactions."@en ;
    skos:inScheme cs: ;
    skos:prefLabel "Refine"@en ;
    skos:topConceptOf cs: ;
.

smprep:refining-byproduct
    a skos:Concept ;
    dcterms:provenance "Compiled by the Geological Survey of Queensland" ;
    rdfs:isDefinedBy cs: ;
    skos:altLabel "Refining Waste"@en ;
    skos:definition "The by-product pathway parallel to a refining process that generates waste material or by-products."@en ;
    skos:inScheme cs: ;
    skos:prefLabel "Refining by-product"@en ;
    skos:topConceptOf cs: ;
.

smprep:rough-extract
    a skos:Concept ;
    dcterms:provenance "Compiled by the Geological Survey of Queensland" ;
    rdfs:isDefinedBy cs: ;
    skos:definition "To extract gemstones, typically opal, as extracted from-ground or after the agitation process of washing and tumbling, but without processing by apidary equipment."@en ;
    skos:inScheme cs: ;
    skos:prefLabel "Rough Extract"@en ;
    skos:topConceptOf cs: ;
.

smprep:sort
    a skos:Concept ;
    dcterms:provenance "Compiled by the Geological Survey of Queensland" ;
    rdfs:isDefinedBy cs: ;
    skos:definition "The separation of material components based on a physical property such as size or density (sort)"@en ;
    skos:inScheme cs: ;
    skos:prefLabel "Sort"@en ;
    skos:topConceptOf cs: ;
.

smprep:unprocessed
    a skos:Concept ;
    dcterms:provenance "Compiled by the Geological Survey of Queensland" ;
    rdfs:isDefinedBy cs: ;
    skos:altLabel
        "N/A"@en ,
        "Not Applicable"@en ,
        "Unprocessed"@en ;
    skos:definition "An explicit indication that a sample material was not processed between two states. For example where a raw material requires no processing to be considered a saleable product."@en ;
    skos:inScheme cs: ;
    skos:prefLabel "No Processing"@en ;
    skos:topConceptOf cs: ;
.

smprep:unspecified
    a skos:Concept ;
    dcterms:provenance "Compiled by the Geological Survey of Queensland" ;
    rdfs:isDefinedBy cs: ;
    skos:altLabel "Unknown"@en ;
    skos:definition "Where a process or group of processes has been performed but specific details have not been recorded or are not available."@en ;
    skos:inScheme cs: ;
    skos:prefLabel "Unspecified"@en ;
    skos:topConceptOf cs: ;
.

smprep:wash
    a skos:Concept ;
    dcterms:provenance "Compiled by the Geological Survey of Queensland" ;
    rdfs:isDefinedBy cs: ;
    skos:definition "To mix with water and/or chemicals and physically agitate to remove impurities."@en ;
    skos:inScheme cs: ;
    skos:prefLabel "Wash"@en ;
    skos:topConceptOf cs: ;
.

<https://linked.data.gov.au/org/gsq>
    a sdo:Organization ;
    sdo:name "Geological Survey of Queensland" ;
    sdo:url "http://www.business.qld.gov.au/industries/mining-energy-water/resources/geoscience-information/gsq"^^xsd:anyURI ;
.

smprep:crush
    a skos:Concept ;
    dcterms:provenance "Compiled by the Geological Survey of Queensland" ;
    rdfs:isDefinedBy cs: ;
    skos:definition "The deformation or pulverization of material by compressing forcefully."@en ;
    skos:inScheme cs: ;
    skos:prefLabel "Crush"@en ;
    skos:topConceptOf cs: ;
.

smprep:cut
    a skos:Concept ;
    dcterms:provenance "Compiled by the Geological Survey of Queensland" ;
    rdfs:isDefinedBy cs: ;
    skos:definition "Prepartion by bifurcating any number of times to produce fresh faces or a smaller overall sample."@en ;
    skos:inScheme cs: ;
    skos:prefLabel "Cut"@en ;
    skos:topConceptOf cs: ;
.

smprep:melt
    a skos:Concept ;
    dcterms:provenance "Compiled by the Geological Survey of Queensland" ;
    rdfs:isDefinedBy cs: ;
    skos:definition "To change a solid to a liquid. Typically through increasing temperature or decreasing pressure."@en ;
    skos:inScheme cs: ;
    skos:prefLabel "Melt"@en ;
    skos:topConceptOf cs: ;
.

smprep:concentrate
    a skos:Concept ;
    dcterms:provenance "Compiled by the Geological Survey of Queensland" ;
    rdfs:isDefinedBy cs: ;
    skos:definition "Preparation by removing or reducing the diluting agent(s) or material."@en ;
    skos:inScheme cs: ;
    skos:prefLabel "Concentrate"@en ;
    skos:topConceptOf cs: ;
.

smprep:heat
    a skos:Concept ;
    dcterms:provenance "Compiled by the Geological Survey of Queensland" ;
    rdfs:isDefinedBy cs: ;
    skos:altLabel "Heating"@en ;
    skos:definition "The process of applying thermal radiation to a material in order to raise its surface and or internal temperature."@en ;
    skos:inScheme cs: ;
    skos:prefLabel "Heat"@en ;
    skos:topConceptOf cs: ;
.

cs:
    a
        owl:Ontology ,
        skos:ConceptScheme ;
    dcterms:created "2020-02-07"^^xsd:date ;
    dcterms:creator <https://linked.data.gov.au/org/gsq> ;
    dcterms:modified "2023-03-16"^^xsd:date ;
    dcterms:provenance "Compiled by the Geological Survey of Queensland" ;
    dcterms:publisher <https://linked.data.gov.au/org/gsq> ;
    reg:status agldwgstatus:stable ;
    skos:definition "The methods used to prepare samples for analyses."@en ;
    skos:hasTopConcept
        smprep:acidify ,
        smprep:aggregate ,
        smprep:beneficiate ,
        smprep:chelate ,
        smprep:compress ,
        smprep:concentrate ,
        smprep:condense ,
        smprep:cool ,
        smprep:crush ,
        smprep:crush-sort ,
        smprep:cut ,
        smprep:deacidify ,
        smprep:decompress ,
        smprep:deposit ,
        smprep:dessicate ,
        smprep:dilute ,
        smprep:disaggregate ,
        smprep:dissolve ,
        smprep:distill ,
        smprep:electrolysis ,
        smprep:extract ,
        smprep:filter ,
        smprep:freeze ,
        smprep:grind ,
        smprep:heat ,
        smprep:hydrate ,
        smprep:ionise ,
        smprep:laser-ablate ,
        smprep:melt ,
        smprep:mount ,
        smprep:precipitate ,
        smprep:react ,
        smprep:recombine ,
        smprep:refine ,
        smprep:refining-byproduct ,
        smprep:rough-extract ,
        smprep:sieve ,
        smprep:sort ,
        smprep:sublimate ,
        smprep:unprocessed ,
        smprep:unspecified ,
        smprep:vaporise ,
        smprep:wash ;
    skos:prefLabel "Sample Preparation Methods"@en ;
.

