PREFIX agldwgstatus: <https://linked.data.gov.au/def/reg-statuses/>
PREFIX cs: <http://linked.data.gov.au/def/sample-location-types>
PREFIX dcterms: <http://purl.org/dc/terms/>
PREFIX locdt: <http://linked.data.gov.au/def/sample-location-types/>
PREFIX owl: <http://www.w3.org/2002/07/owl#>
PREFIX rdfs: <http://www.w3.org/2000/01/rdf-schema#>
PREFIX reg: <http://purl.org/linked-data/registry#>
PREFIX sdo: <https://schema.org/>
PREFIX skos: <http://www.w3.org/2004/02/skos/core#>
PREFIX xsd: <http://www.w3.org/2001/XMLSchema#>

locdt:bag
    a skos:Concept ;
    dcterms:provenance "Compiled by the Geological Survey of Queensland" ;
    rdfs:isDefinedBy cs: ;
    skos:altLabel
        "Pack"@en ,
        "Pouch"@en ,
        "Sac"@en ,
        "Sack"@en ;
    skos:definition "A flexible container with an opening at the top, used for carrying or storing things."@en ;
    skos:inScheme cs: ;
    skos:prefLabel "Bag"@en ;
    skos:topConceptOf cs: ;
.

locdt:bin
    a skos:Concept ;
    dcterms:provenance "Compiled by the Geological Survey of Queensland" ;
    rdfs:isDefinedBy cs: ;
    skos:definition "A capacious receptacle for storing a substances and/or artifacts."@en ;
    skos:inScheme cs: ;
    skos:prefLabel "Bin"@en ;
    skos:topConceptOf cs: ;
.

locdt:cabinet
    a skos:Concept ;
    dcterms:provenance "Compiled by the Geological Survey of Queensland" ;
    rdfs:isDefinedBy cs: ;
    skos:altLabel "Cupboard"@en ;
    skos:definition "An enclosed piece of furniture, typically with internal shelves for the storage and organisation of items."@en ;
    skos:inScheme cs: ;
    skos:prefLabel "Cabinet"@en ;
    skos:topConceptOf cs: ;
.

locdt:drawer
    a skos:Concept ;
    dcterms:provenance "Compiled by the Geological Survey of Queensland" ;
    rdfs:isDefinedBy cs: ;
    skos:altLabel "Draw"@en ;
    skos:definition "A a box-shaped container that fits into a piece of furniture in such a way that it can be drawn out horizontally to reach its contents."@en ;
    skos:inScheme cs: ;
    skos:prefLabel "Drawer"@en ;
    skos:topConceptOf cs: ;
.

locdt:drum
    a skos:Concept ;
    dcterms:provenance "Compiled by the Geological Survey of Queensland" ;
    rdfs:isDefinedBy cs: ;
    skos:altLabel
        "Amphora"@en ,
        "Barrel"@en ,
        "Cask"@en ,
        "Vat"@en ;
    skos:definition "A hollow cylindrical container with a bulging center, longer than it is wide."@en ;
    skos:inScheme cs: ;
    skos:prefLabel "Drum"@en ;
    skos:topConceptOf cs: ;
.

locdt:dumpster
    a skos:Concept ;
    dcterms:provenance "Compiled by the Geological Survey of Queensland" ;
    rdfs:isDefinedBy cs: ;
    skos:definition "A movable waste container designed to be brought and taken away by a special collection vehicle, or to a bin that a specially designed garbage truck lifts, empties into its hopper, and lowers, on the spot."@en ;
    skos:inScheme cs: ;
    skos:prefLabel "Dumpster"@en ;
    skos:topConceptOf cs: ;
.

locdt:envelope
    a skos:Concept ;
    dcterms:provenance "Compiled by the Geological Survey of Queensland" ;
    rdfs:isDefinedBy cs: ;
    skos:altLabel "File Folder"@en ;
    skos:definition "A packaging item, usually made of thin, flat material. It is designed to contain a flat object or objects, such as a letter, document, or card."@en ;
    skos:inScheme cs: ;
    skos:prefLabel "Envelope"@en ;
    skos:topConceptOf cs: ;
.

locdt:folder
    a skos:Concept ;
    dcterms:provenance "Compiled by the Geological Survey of Queensland" ;
    rdfs:isDefinedBy cs: ;
    skos:definition "A sheet of heavy paper stock or other thin, but stiff, material which is folded in half, and used to keep paper documents or other flat items."@en ;
    skos:inScheme cs: ;
    skos:prefLabel "Folder"@en ;
    skos:topConceptOf cs: ;
.

locdt:pallet
    a skos:Concept ;
    dcterms:provenance "Compiled by the Geological Survey of Queensland" ;
    rdfs:isDefinedBy cs: ;
    skos:definition "A flat transport structure, which supports goods in a stable fashion while being lifted by a forklift, a pallet jack, a front loader, a jacking device, or an erect crane."@en ;
    skos:inScheme cs: ;
    skos:prefLabel "Pallet"@en ;
    skos:topConceptOf cs: ;
.

locdt:rack
    a skos:Concept ;
    dcterms:provenance "Compiled by the Geological Survey of Queensland" ;
    rdfs:isDefinedBy cs: ;
    skos:definition "A material handling storage aid system designed to store materials on pallets or other standard storage platforms."@en ;
    skos:inScheme cs: ;
    skos:prefLabel "Rack"@en ;
    skos:topConceptOf cs: ;
.

locdt:room
    a skos:Concept ;
    dcterms:provenance "Compiled by the Geological Survey of Queensland" ;
    rdfs:isDefinedBy cs: ;
    skos:definition "Any enclosed space with walls, a ceiling and one-or-many entrances."@en ;
    skos:inScheme cs: ;
    skos:prefLabel "Room"@en ;
    skos:topConceptOf cs: ;
.

locdt:table
    a skos:Concept ;
    dcterms:provenance "Compiled by the Geological Survey of Queensland" ;
    rdfs:isDefinedBy cs: ;
    skos:definition "An item of furniture with a flat top and one or more legs, used as a surface for working at or storing items."@en ;
    skos:inScheme cs: ;
    skos:prefLabel "Table"@en ;
    skos:topConceptOf cs: ;
.

locdt:tray
    a skos:Concept ;
    dcterms:provenance "Compiled by the Geological Survey of Queensland" ;
    rdfs:isDefinedBy cs: ;
    skos:definition "A shallow platform designed for the carrying or storing of items."@en ;
    skos:inScheme cs: ;
    skos:prefLabel "Tray"@en ;
    skos:topConceptOf cs: ;
.

<https://linked.data.gov.au/org/gsq>
    a sdo:Organization ;
    sdo:name "Geological Survey of Queensland" ;
    sdo:url "http://www.business.qld.gov.au/industries/mining-energy-water/resources/geoscience-information/gsq"^^xsd:anyURI ;
.

cs:
    a
        owl:Ontology ,
        skos:ConceptScheme ;
    dcterms:created "2020-02-07T11:48:51"^^xsd:dateTime ;
    dcterms:creator <https://linked.data.gov.au/org/gsq> ;
    dcterms:modified "2023-03-16"^^xsd:date ;
    dcterms:provenance "Compiled by the Geological Survey of Queensland" ;
    dcterms:publisher <https://linked.data.gov.au/org/gsq> ;
    reg:status agldwgstatus:stable ;
    skos:definition "Indexed storage items and locations used in storage facilities for inventory management and warehousing."@en ;
    skos:hasTopConcept
        locdt:bag ,
        locdt:bin ,
        locdt:cabinet ,
        locdt:drawer ,
        locdt:drum ,
        locdt:dumpster ,
        locdt:envelope ,
        locdt:folder ,
        locdt:pallet ,
        locdt:rack ,
        locdt:room ,
        locdt:table ,
        locdt:tray ;
    skos:prefLabel "Sample Location Types"@en ;
.

