PREFIX agldwgstatus: <https://linked.data.gov.au/def/reg-statuses/>
PREFIX cs: <http://linked.data.gov.au/def/sample-relationship>
PREFIX dcterms: <http://purl.org/dc/terms/>
PREFIX owl: <http://www.w3.org/2002/07/owl#>
PREFIX rdfs: <http://www.w3.org/2000/01/rdf-schema#>
PREFIX reg: <http://purl.org/linked-data/registry#>
PREFIX sdo: <https://schema.org/>
PREFIX skos: <http://www.w3.org/2004/02/skos/core#>
PREFIX smrl: <http://linked.data.gov.au/def/sample-relationship/>
PREFIX sosa: <http://www.w3.org/ns/sosa/>
PREFIX xsd: <http://www.w3.org/2001/XMLSchema#>

sosa:hasOriginalSample
    a
        owl:ObjectProperty ,
        skos:Concept ;
    dcterms:provenance "Source information from http://www.w3.org/TR/vocab-ssn/#Sample_Relations and the SOSA Extensions ontology, modified by the Geological Survey of Queensland." ;
    sdo:domainIncludes sosa:Sample ;
    sdo:rangeIncludes sosa:Sample ;
    rdfs:domain sosa:Sample ;
    rdfs:isDefinedBy sosa: ;
    rdfs:range sosa:Sample ;
    skos:definition "A link from the subject sample to the original sample of interest through a chain of isSampleOf relations."@en ;
    skos:inScheme cs: ;
    skos:prefLabel "has original sample"@en ;
    skos:topConceptOf cs: ;
.

sosa:isSampleOf
    a
        owl:ObjectProperty ,
        skos:Concept ;
    dcterms:provenance "Source information from http://www.w3.org/TR/vocab-ssn/#Sample_Relations and the SOSA Extensions ontology, modified by the Geological Survey of Queensland." ;
    sdo:domainIncludes sosa:Sample ;
    sdo:rangeIncludes sosa:FeatureOfInterest ;
    rdfs:isDefinedBy sosa: ;
    owl:inverseOf sosa:hasSample ;
    skos:definition "Relation from a Sample to the entity that it was dervied from."@en ;
    skos:inScheme cs: ;
    skos:prefLabel "is sample of"@en ;
    skos:topConceptOf cs: ;
.

smrl:isAggregateOf
    a skos:Concept ;
    dcterms:provenance "Source information from http://www.w3.org/TR/vocab-ssn/#Sample_Relations and the SOSA Extensions ontology, modified by the Geological Survey of Queensland." ;
    sdo:domainIncludes sosa:Sample ;
    rdfs:isDefinedBy cs: ;
    skos:definition "Relation from a Sample to an entity that it was dervied from, where multiple sources have been aggregated into a composite sample."@en ;
    skos:inScheme cs: ;
    skos:prefLabel "is aggregate of"@en ;
    skos:topConceptOf cs: ;
.

<https://linked.data.gov.au/org/gsq>
    a sdo:Organization ;
    sdo:name "Geological Survey of Queensland" ;
    sdo:url "http://www.business.qld.gov.au/industries/mining-energy-water/resources/geoscience-information/gsq"^^xsd:anyURI ;
.

cs:
    a
        owl:Ontology ,
        skos:ConceptScheme ;
    dcterms:created "2020-03-24"^^xsd:date ;
    dcterms:creator <https://linked.data.gov.au/org/gsq> ;
    dcterms:modified "2023-03-16"^^xsd:date ;
    dcterms:provenance "Source information from http://www.w3.org/TR/vocab-ssn/#Sample_Relations and the SOSA Extensions ontology, modified by the Geological Survey of Queensland." ;
    dcterms:publisher <https://linked.data.gov.au/org/gsq> ;
    reg:status agldwgstatus:stable ;
    skos:definition "Relationships between Samples. This vocabulary is derived from the SOSA Ontology and the SOSA Extensions Ontology where the Samples are defined by the class sosa:Sample and the relationships are OWL objectProperties. It reuses the original ontology URIs directly and retains the relationship's non-SKSO properties too so it is a SKOS+ ontology (SKOS + other things)."@en ;
    skos:hasTopConcept
        sosa:hasOriginalSample ,
        sosa:isSampleOf ,
        smrl:isAggregateOf ;
    skos:prefLabel "Sample Relationship"@en ;
.

