PREFIX agldwgstatus: <https://linked.data.gov.au/def/reg-statuses/>
PREFIX cs: <http://linked.data.gov.au/def/survey-relationship-type>
PREFIX dcterms: <http://purl.org/dc/terms/>
PREFIX owl: <http://www.w3.org/2002/07/owl#>
PREFIX rdfs: <http://www.w3.org/2000/01/rdf-schema#>
PREFIX reg: <http://purl.org/linked-data/registry#>
PREFIX sdo: <https://schema.org/>
PREFIX skos: <http://www.w3.org/2004/02/skos/core#>
PREFIX srt: <http://linked.data.gov.au/def/survey-relationship-type/>
PREFIX xsd: <http://www.w3.org/2001/XMLSchema#>

srt:dependent
    a skos:Concept ;
    skos:historyNote "Developed by the Geological Survey of Queensland." ;
    rdfs:isDefinedBy cs: ;
    skos:broader srt:same-project ;
    skos:definition "A survey that was conducted during the course of a single project that was dependent on the completion of the referenced survey, i.e. a survey that is part of the same project as another survey but is reliant on the other survey has been conducted."@en ;
    skos:inScheme cs: ;
    skos:prefLabel "Same Project - Dependent"@en ;
.

srt:extension
    a skos:Concept ;
    skos:historyNote "Developed by the Geological Survey of Queensland." ;
    rdfs:isDefinedBy cs: ;
    skos:broader srt:follow-up ;
    skos:definition "A follow-up survey designed to extend the coverage of an existing survey, usually using the same parameters to ensure data compatibility."@en ;
    skos:inScheme cs: ;
    skos:prefLabel "Extension"@en ;
.

srt:independent
    a skos:Concept ;
    skos:historyNote "Developed by the Geological Survey of Queensland." ;
    rdfs:isDefinedBy cs: ;
    skos:broader srt:same-project ;
    skos:definition "A survey that was conducted during the course of a single project that is not reliant on another survey or activity within the project, i.e. a survey that can be performed independently of any other surveys within a project."@en ;
    skos:inScheme cs: ;
    skos:prefLabel "Same Project - independent"@en ;
.

srt:infill
    a skos:Concept ;
    skos:historyNote "Developed by the Geological Survey of Queensland." ;
    rdfs:isDefinedBy cs: ;
    skos:broader srt:follow-up ;
    skos:definition "A follow-up survey designed to increase the spatial resolution of a pre-existing survey, usually using the same parameters to ensure data compatibility."@en ;
    skos:inScheme cs: ;
    skos:prefLabel "Infill"@en ;
.

srt:repeat
    a skos:Concept ;
    skos:historyNote "Developed by the Geological Survey of Queensland." ;
    rdfs:isDefinedBy cs: ;
    skos:broader srt:follow-up ;
    skos:definition "A follow-up survey designed to replicate the coverage and parameters of an existing survey. A repeat survey may, for example, be needed to correct errors or to reproduce results from the initial survey."@en ;
    skos:inScheme cs: ;
    skos:prefLabel "Repeat"@en ;
.

srt:reprocessed
    a skos:Concept ;
    skos:historyNote "Developed by the Geological Survey of Queensland." ;
    rdfs:isDefinedBy cs: ;
    skos:definition "The original entity from which a new digital sample was created by reprocessing."@en ;
    skos:inScheme cs: ;
    skos:prefLabel "Reprocessed"@en ;
    skos:topConceptOf cs: ;
.

srt:reprocessing
    a skos:Concept ;
    skos:historyNote "Developed by the Geological Survey of Queensland." ;
    rdfs:isDefinedBy cs: ;
    skos:definition "Generating a new digital sample by reprocessing pre-existing raw data with a new algorithm or processing parameters."@en ;
    skos:inScheme cs: ;
    skos:prefLabel "Reprocessing"@en ;
    skos:topConceptOf cs: ;
.

srt:resampling
    a skos:Concept ;
    skos:historyNote "Developed by the Geological Survey of Queensland." ;
    rdfs:isDefinedBy cs: ;
    skos:altLabel "subsampling"@en ;
    skos:definition "Generating a new physical sample from an existing sample."@en ;
    skos:inScheme cs: ;
    skos:prefLabel "Resampling"@en ;
    skos:topConceptOf cs: ;
.

<https://linked.data.gov.au/org/gsq>
    a sdo:Organization ;
    sdo:name "Geological Survey of Queensland" ;
    sdo:url "http://www.business.qld.gov.au/industries/mining-energy-water/resources/geoscience-information/gsq"^^xsd:anyURI ;
.

srt:same-project
    a skos:Concept ;
    skos:historyNote "Developed by the Geological Survey of Queensland." ;
    rdfs:isDefinedBy cs: ;
    skos:definition "Surveys that were conducted, concurrently or otherwise, during the course of a single project."@en ;
    skos:inScheme cs: ;
    skos:prefLabel "Same project"@en ;
    skos:topConceptOf cs: ;
.

srt:follow-up
    a skos:Concept ;
    skos:historyNote "Developed by the Geological Survey of Queensland." ;
    rdfs:isDefinedBy cs: ;
    skos:definition "A survey that was designed on the basis of lessons learned from a prior survey."@en ;
    skos:inScheme cs: ;
    skos:prefLabel "Follow-up"@en ;
    skos:topConceptOf cs: ;
.

cs:
    a
        owl:Ontology ,
        skos:ConceptScheme ;
    dcterms:created "2020-04-08"^^xsd:date ;
    dcterms:creator <https://linked.data.gov.au/org/gsq> ;
    dcterms:modified "2023-03-16"^^xsd:date ;
    skos:historyNote "Developed by the Geological Survey of Queensland." ;
    dcterms:publisher <https://linked.data.gov.au/org/gsq> ;
    reg:status agldwgstatus:stable ;
    skos:definition "The relationships that exist between surveys."@en ;
    skos:hasTopConcept
        srt:follow-up ,
        srt:reprocessing ,
        srt:resampling ,
        srt:same-project ;
    skos:prefLabel "Survey relationship type"@en ;
.

