PREFIX agldwgstatus: <https://linked.data.gov.au/def/reg-statuses/>
PREFIX cs: <http://linked.data.gov.au/def/telephone-type>
PREFIX dcterms: <http://purl.org/dc/terms/>
PREFIX owl: <http://www.w3.org/2002/07/owl#>
PREFIX rdfs: <http://www.w3.org/2000/01/rdf-schema#>
PREFIX reg: <http://purl.org/linked-data/registry#>
PREFIX sdo: <https://schema.org/>
PREFIX skos: <http://www.w3.org/2004/02/skos/core#>
PREFIX vcard: <http://www.w3.org/2006/vcard/ns#>
PREFIX xsd: <http://www.w3.org/2001/XMLSchema#>

vcard:Cell
    a
        skos:Concept ,
        vcard:TelephoneType ;
    skos:historyNote "Derived from Australian Standard AS 4590.1:2017" ;
    rdfs:isDefinedBy cs: ;
    skos:altLabel
        "Cell"@en ,
        "Cellular"@en ;
    skos:definition "A portable telephone that can make and receive calls over a radio frequency link while the user is moving within a telephone service area."@en ;
    skos:inScheme cs: ;
    skos:notation "01" ;
    skos:prefLabel "Mobile"@en ;
    skos:topConceptOf cs: ;
.

vcard:Voice
    a skos:Concept ;
    skos:historyNote "Derived from Australian Standard AS 4590.1:2017" ;
    rdfs:isDefinedBy cs: ;
    skos:altLabel
        "Landline"@en ,
        "voice"@en ;
    skos:definition "A telephone that can make and receive calls by transmission of communications signals via a cable to a fixed location."@en ;
    skos:inScheme cs: ;
    skos:notation "02" ;
    skos:prefLabel "Fixed Line"@en ;
    skos:topConceptOf cs: ;
.

<https://linked.data.gov.au/org/gsq>
    a sdo:Organization ;
    sdo:name "Geological Survey of Queensland" ;
    sdo:url "http://www.business.qld.gov.au/industries/mining-energy-water/resources/geoscience-information/gsq"^^xsd:anyURI ;
.

cs:
    a
        owl:Ontology ,
        skos:ConceptScheme ;
    dcterms:created "2020-03-25"^^xsd:date ;
    dcterms:creator <https://linked.data.gov.au/org/gsq> ;
    dcterms:modified "2023-03-16"^^xsd:date ;
    skos:historyNote "Derived from Australian Standard AS 4590.1:2017" ;
    dcterms:publisher <https://linked.data.gov.au/org/gsq> ;
    reg:status agldwgstatus:stable ;
    skos:definition "The code and description that differentiates the type of telecommunications device based on the transmission service connected to the telephone network."@en ;
    skos:hasTopConcept
        vcard:Cell ,
        vcard:Voice ;
    skos:prefLabel "Telephone Type"@en ;
.

