PREFIX agldwgstatus: <https://linked.data.gov.au/def/reg-statuses/>
PREFIX cs: <http://linked.data.gov.au/def/transaction-status>
PREFIX dcterms: <http://purl.org/dc/terms/>
PREFIX owl: <http://www.w3.org/2002/07/owl#>
PREFIX rdfs: <http://www.w3.org/2000/01/rdf-schema#>
PREFIX reg: <http://purl.org/linked-data/registry#>
PREFIX sdo: <https://schema.org/>
PREFIX skos: <http://www.w3.org/2004/02/skos/core#>
PREFIX tnst: <http://linked.data.gov.au/def/transaction-status/>
PREFIX xsd: <http://www.w3.org/2001/XMLSchema#>

tnst:adjustment
    a skos:Concept ;
    dcterms:provenance "Compiled by the Geological Survey of Queensland" ;
    rdfs:isDefinedBy cs: ;
    skos:altLabel
        "Variation"@en ,
        "Varied"@en ;
    skos:definition "A sales record that has been corrected with a plus-or-minus variation to a completed sale, i.e. the difference in value and tonnage from originally recorded or reported."@en ;
    skos:inScheme cs: ;
    skos:prefLabel "Adjustment"@en ;
    skos:topConceptOf cs: ;
.

tnst:cancelled
    a skos:Concept ;
    dcterms:provenance "Compiled by the Geological Survey of Queensland" ;
    rdfs:isDefinedBy cs: ;
    skos:definition "A record that a previously recorded or reported contracted sale has subsequently been cancelled by the buyer or seller."@en ;
    skos:inScheme cs: ;
    skos:prefLabel "Cancelled"@en ;
    skos:topConceptOf cs: ;
.

tnst:completed
    a skos:Concept ;
    dcterms:provenance "Compiled by the Geological Survey of Queensland" ;
    rdfs:isDefinedBy cs: ;
    skos:altLabel "Completed"@en ;
    skos:definition "A standard sales record detailing the expected or finalised tonnage and value."@en ;
    skos:inScheme cs: ;
    skos:prefLabel "Original"@en ;
    skos:topConceptOf cs: ;
.

tnst:held
    a skos:Concept ;
    dcterms:provenance "Compiled by the Geological Survey of Queensland" ;
    rdfs:isDefinedBy cs: ;
    skos:definition "A record that a sale is in dispute or is held by an entity that is preventing completion of sale. Where a sale is prevented by an authorised entity, such as a border and customs agency or a financial administrator"@en ;
    skos:inScheme cs: ;
    skos:prefLabel "Held"@en ;
    skos:topConceptOf cs: ;
.

tnst:replacement
    a skos:Concept ;
    dcterms:provenance "Compiled by the Geological Survey of Queensland" ;
    rdfs:isDefinedBy cs: ;
    skos:altLabel
        "Amended"@en ,
        "Amendment"@en ;
    skos:definition "A sales record that has been amended with a final tonnage and value correction to a completed sale, replacing the originally reported values with new total values, i.e. the amended value"@en ;
    skos:inScheme cs: ;
    skos:prefLabel "Replacement"@en ;
    skos:topConceptOf cs: ;
.

<https://linked.data.gov.au/org/gsq>
    a sdo:Organization ;
    sdo:name "Geological Survey of Queensland" ;
    sdo:url "http://www.business.qld.gov.au/industries/mining-energy-water/resources/geoscience-information/gsq"^^xsd:anyURI ;
.

cs:
    a
        owl:Ontology ,
        skos:ConceptScheme ;
    dcterms:created "2022-01-10"^^xsd:date ;
    dcterms:creator <https://linked.data.gov.au/org/gsq> ;
    dcterms:modified "2023-03-16"^^xsd:date ;
    dcterms:provenance "Compiled by the Geological Survey of Queensland" ;
    dcterms:publisher <https://linked.data.gov.au/org/gsq> ;
    reg:status agldwgstatus:stable ;
    skos:definition "The status of a transaction contracted for sale or the type of sales value information being recorded."@en ;
    skos:hasTopConcept
        tnst:adjustment ,
        tnst:cancelled ,
        tnst:completed ,
        tnst:held ,
        tnst:replacement ;
    skos:prefLabel "Transaction Status"@en ;
.

